@prefix owl: <http://www.w3.org/2002/07/owl#> .
@prefix rdf: <http://www.w3.org/1999/02/22-rdf-syntax-ns#> .
@prefix rdfs: <http://www.w3.org/2000/01/rdf-schema#> .
@prefix wiki: <http://www.semanticweb.org/ontologies/Wikidata#> .
@prefix wikidata: <http://www.semanticweb.org/ontologies/Wikidata#> .
@prefix xml: <http://www.w3.org/XML/1998/namespace> .
@prefix xsd: <http://www.w3.org/2001/XMLSchema#> .

wikidata:P1000 rdfs:label "record held"^^xsd:string ;
    rdfs:comment "notable record achieved by a person or entity, include qualifiers for dates held"^^xsd:string ;
    rdfs:range wikidata:Q1241356 .

wikidata:P1001 rdfs:label "applies to jurisdiction"^^xsd:string ;
    rdfs:comment "the item (institution, law, public office, public register...) or statement belongs to or has power over or applies to the value (a territorial jurisdiction: a country, state, municipality, ...)"^^xsd:string ;
    rdfs:domain wikidata:Q102496,
        wikidata:Q105985,
        wikidata:Q1140371,
        wikidata:Q1151067,
        wikidata:Q1197685,
        wikidata:Q12047392,
        wikidata:Q12798556,
        wikidata:Q12804010,
        wikidata:Q13406463,
        wikidata:Q14659,
        wikidata:Q15097084,
        wikidata:Q15238777,
        wikidata:Q1530022,
        wikidata:Q15617994,
        wikidata:Q1572600,
        wikidata:Q17143723,
        wikidata:Q176799,
        wikidata:Q18616576,
        wikidata:Q1864008,
        wikidata:Q191072,
        wikidata:Q20045456,
        wikidata:Q21004260,
        wikidata:Q213283,
        wikidata:Q2135465,
        wikidata:Q21451536,
        wikidata:Q214995,
        wikidata:Q216353,
        wikidata:Q223729,
        wikidata:Q2385804,
        wikidata:Q24962887,
        wikidata:Q30634609,
        wikidata:Q317557,
        wikidata:Q321839,
        wikidata:Q329525,
        wikidata:Q35535,
        wikidata:Q372690,
        wikidata:Q3917681,
        wikidata:Q40357,
        wikidata:Q4164871,
        wikidata:Q42470,
        wikidata:Q43229,
        wikidata:Q43306178,
        wikidata:Q473972,
        wikidata:Q4992061,
        wikidata:Q55876909,
        wikidata:Q56061,
        wikidata:Q567696,
        wikidata:Q618779,
        wikidata:Q65554936,
        wikidata:Q686822,
        wikidata:Q689044,
        wikidata:Q7397,
        wikidata:Q7748,
        wikidata:Q7843791,
        wikidata:Q80071,
        wikidata:Q8142,
        wikidata:Q8161,
        wikidata:Q895526,
        wikidata:Q905765 ;
    rdfs:range wikidata:Q20926517,
        wikidata:Q27096213,
        wikidata:Q2881272,
        wikidata:Q2882257,
        wikidata:Q3624078,
        wikidata:Q3895768,
        wikidata:Q3918,
        wikidata:Q44782,
        wikidata:Q56061,
        wikidata:Q5982983,
        wikidata:Q7188,
        wikidata:Q8222382,
        wikidata:Q82794 ;
    rdfs:subPropertyOf wikidata:P7153 .

wikidata:P1002 rdfs:label "engine configuration"^^xsd:string ;
    rdfs:comment "configuration of an engine's cylinders"^^xsd:string ;
    rdfs:domain wikidata:Q630010 ;
    rdfs:range wikidata:Q2576663 .

wikidata:P1018 rdfs:label "language regulatory body"^^xsd:string ;
    rdfs:comment "regulatory body of a language"^^xsd:string ;
    rdfs:domain wikidata:Q17376908 ;
    rdfs:range wikidata:Q43229,
        wikidata:Q5 .

wikidata:P1026 rdfs:label "academic thesis"^^xsd:string ;
    rdfs:comment "thesis or dissertation written for a degree"^^xsd:string ;
    rdfs:domain wikidata:Q5 ;
    rdfs:range wikidata:Q1266946,
        wikidata:Q187685,
        wikidata:Q1907875,
        wikidata:Q798134 .

wikidata:P1027 rdfs:label "conferred by"^^xsd:string ;
    rdfs:comment "person or organization who grants an award, certification, or role"^^xsd:string ;
    rdfs:domain wikidata:Q214339,
        wikidata:Q374814,
        wikidata:Q618779 .

wikidata:P1029 rdfs:label "crew member"^^xsd:string ;
    rdfs:comment "person that participated operating or serving aboard this vehicle"^^xsd:string ;
    rdfs:range wikidata:Q5,
        wikidata:Q95074 .

wikidata:P103 rdfs:label "native language"^^xsd:string ;
    rdfs:comment "language or languages a person has learned from early childhood"^^xsd:string ;
    rdfs:domain wikidata:Q13002315,
        wikidata:Q21070598,
        wikidata:Q215627,
        wikidata:Q3117863,
        wikidata:Q41710,
        wikidata:Q95074 ;
    rdfs:range wikidata:Q17376908 ;
    rdfs:subPropertyOf wikidata:P1412 .

wikidata:P1040 rdfs:label "film editor"^^xsd:string ;
    rdfs:comment "person who works with the raw footage, selecting shots and combining them into sequences to create a finished motion picture"^^xsd:string ;
    rdfs:domain wikidata:Q11424,
        wikidata:Q15416,
        wikidata:Q21191270,
        wikidata:Q24856,
        wikidata:Q526877 ;
    rdfs:range wikidata:Q14073567,
        wikidata:Q5 ;
    rdfs:subPropertyOf wikidata:P3092 .

wikidata:P1046 rdfs:label "discovery method"^^xsd:string ;
    rdfs:comment "way an exoplanet was discovered"^^xsd:string ;
    rdfs:domain wikidata:Q44559 .

wikidata:P1049 rdfs:label "worshipped by"^^xsd:string ;
    rdfs:comment "religion or group/civilization that worships a given deity"^^xsd:string ;
    rdfs:domain wikidata:Q1509831,
        wikidata:Q1595289,
        wikidata:Q17624054,
        wikidata:Q178885,
        wikidata:Q187616,
        wikidata:Q190,
        wikidata:Q193291,
        wikidata:Q20830276,
        wikidata:Q4588528,
        wikidata:Q5,
        wikidata:Q95074 ;
    rdfs:range wikidata:Q17364638,
        wikidata:Q49447 ;
    rdfs:subPropertyOf wikidata:P361 .

wikidata:P105 rdfs:label "taxon rank"^^xsd:string ;
    rdfs:comment "level in a taxonomic hierarchy"^^xsd:string ;
    rdfs:domain wikidata:Q16521 ;
    rdfs:range wikidata:Q427626 ;
    rdfs:subPropertyOf wikidata:P31 .

wikidata:P1050 rdfs:label "medical condition"^^xsd:string ;
    rdfs:comment "any state relevant to the health of an organism, including diseases and positive conditions"^^xsd:string ;
    rdfs:domain wikidata:Q15304597,
        wikidata:Q215627,
        wikidata:Q30612,
        wikidata:Q4271324,
        wikidata:Q4915012,
        wikidata:Q729,
        wikidata:Q95074 ;
    rdfs:range wikidata:Q12136,
        wikidata:Q1441305,
        wikidata:Q175854,
        wikidata:Q2057971,
        wikidata:Q796194,
        wikidata:Q808 .

wikidata:P1056 rdfs:label "product or material produced"^^xsd:string ;
    rdfs:comment "material or product produced by a government agency, business, industry, facility, or process"^^xsd:string ;
    rdfs:domain wikidata:Q1183543,
        wikidata:Q12737077,
        wikidata:Q13226383,
        wikidata:Q1408286,
        wikidata:Q14897293,
        wikidata:Q177634,
        wikidata:Q1914636,
        wikidata:Q2207288,
        wikidata:Q268592,
        wikidata:Q28640,
        wikidata:Q31464082,
        wikidata:Q3249551,
        wikidata:Q327333,
        wikidata:Q431289,
        wikidata:Q43229,
        wikidata:Q5,
        wikidata:Q8148,
        wikidata:Q820477 ;
    rdfs:range wikidata:Q11028,
        wikidata:Q11344,
        wikidata:Q11379,
        wikidata:Q11651,
        wikidata:Q1172284,
        wikidata:Q1310239,
        wikidata:Q13226383,
        wikidata:Q1371819,
        wikidata:Q1408286,
        wikidata:Q15401930,
        wikidata:Q1799072,
        wikidata:Q2393187,
        wikidata:Q2424752,
        wikidata:Q289472,
        wikidata:Q3566043,
        wikidata:Q7079603,
        wikidata:Q79529 ;
    rdfs:subPropertyOf wikidata:P1536 .

wikidata:P1057 rdfs:label "chromosome"^^xsd:string ;
    rdfs:comment "chromosome on which an entity is localized"^^xsd:string ;
    rdfs:domain wikidata:Q1458444,
        wikidata:Q15304597,
        wikidata:Q7187 ;
    rdfs:range wikidata:Q37748 .

wikidata:P1064 rdfs:label "track gauge"^^xsd:string ;
    rdfs:comment "spacing of the rails on a railway track"^^xsd:string ;
    rdfs:range wikidata:Q214519 .

wikidata:P1071 rdfs:label "location of creation"^^xsd:string ;
    rdfs:comment "place where the item was made; where applicable, location of final assembly"^^xsd:string ;
    rdfs:domain wikidata:Q10929058,
        wikidata:Q17334923,
        wikidata:Q17489659,
        wikidata:Q2095,
        wikidata:Q3231690,
        wikidata:Q3407658,
        wikidata:Q386724,
        wikidata:Q559026,
        wikidata:Q8205328 ;
    rdfs:range wikidata:Q618123 ;
    rdfs:subPropertyOf wikidata:P7153 .

wikidata:P1072 rdfs:label "readable file format"^^xsd:string ;
    rdfs:comment "file format a program can open and read"^^xsd:string ;
    rdfs:domain wikidata:Q20826013,
        wikidata:Q7397 ;
    rdfs:range wikidata:Q235557,
        wikidata:Q26085352 ;
    rdfs:subPropertyOf wikidata:P121 .

wikidata:P1073 rdfs:label "writable file format"^^xsd:string ;
    rdfs:comment "file format a program can create and/or write to"^^xsd:string ;
    rdfs:domain wikidata:Q166142,
        wikidata:Q2858615,
        wikidata:Q7397 ;
    rdfs:range wikidata:Q235557,
        wikidata:Q26085352 .

wikidata:P1074 rdfs:label "fictional analog of"^^xsd:string ;
    rdfs:comment "used to link an entity or class of entities appearing in a creative work with the analogous entity or class of entities in the real world"^^xsd:string ;
    rdfs:domain wikidata:Q14897293,
        wikidata:Q24334685 .

wikidata:P1075 rdfs:label "rector"^^xsd:string ;
    rdfs:comment "rector of a university"^^xsd:string ;
    rdfs:domain wikidata:Q15690029,
        wikidata:Q2822246,
        wikidata:Q38723 ;
    rdfs:range wikidata:Q15632617,
        wikidata:Q215627,
        wikidata:Q28020127,
        wikidata:Q95074 ;
    rdfs:subPropertyOf wikidata:P1037 .

wikidata:P1080 rdfs:label "from narrative universe"^^xsd:string ;
    rdfs:comment "subject's fictional entity is in the object narrative. See also P1441 (present in work) and P1445 (fictional universe described in)"^^xsd:string ;
    rdfs:domain wikidata:Q13002315,
        wikidata:Q14514600,
        wikidata:Q14897293,
        wikidata:Q15831596,
        wikidata:Q207869,
        wikidata:Q21070598,
        wikidata:Q24334685,
        wikidata:Q978 ;
    rdfs:range wikidata:Q559618,
        wikidata:Q867335,
        wikidata:Q9134 ;
    rdfs:subPropertyOf wikidata:P361 .

wikidata:P111 rdfs:label "measured physical quantity"^^xsd:string ;
    rdfs:comment "value of a physical property expressed as number multiplied by a unit"^^xsd:string ;
    rdfs:domain wikidata:Q173227,
        wikidata:Q47574 ;
    rdfs:range wikidata:Q71550118 .

wikidata:P112 rdfs:label "founded by"^^xsd:string ;
    rdfs:comment "founder or co-founder of this organization, religion or place"^^xsd:string ;
    rdfs:domain wikidata:Q1047113,
        wikidata:Q14514600,
        wikidata:Q14623646,
        wikidata:Q16334295,
        wikidata:Q1656682,
        wikidata:Q170584,
        wikidata:Q17364638,
        wikidata:Q177634,
        wikidata:Q18127,
        wikidata:Q2217301,
        wikidata:Q35127,
        wikidata:Q3895768,
        wikidata:Q43229,
        wikidata:Q4830453,
        wikidata:Q49773,
        wikidata:Q58778,
        wikidata:Q60031086,
        wikidata:Q618123,
        wikidata:Q618779,
        wikidata:Q7257,
        wikidata:Q732577,
        wikidata:Q811979 ;
    rdfs:range wikidata:Q13002315,
        wikidata:Q15632617,
        wikidata:Q16334295,
        wikidata:Q21070568,
        wikidata:Q215627,
        wikidata:Q5,
        wikidata:Q7188,
        wikidata:Q95074 ;
    rdfs:subPropertyOf wikidata:P170 .

wikidata:P113 rdfs:label "airline hub"^^xsd:string ;
    rdfs:comment "airport that serves as a hub for an airline"^^xsd:string ;
    rdfs:domain wikidata:Q465909,
        wikidata:Q46970 ;
    rdfs:range wikidata:Q1248784 .

wikidata:P114 rdfs:label "airline alliance"^^xsd:string ;
    rdfs:comment "alliance the airline belongs to"^^xsd:string ;
    rdfs:domain wikidata:Q46970 ;
    rdfs:range wikidata:Q465909 ;
    rdfs:subPropertyOf wikidata:P463 .

wikidata:P1142 rdfs:label "political ideology"^^xsd:string ;
    rdfs:comment "political ideology of this organization or person"^^xsd:string ;
    rdfs:range wikidata:Q10286227,
        wikidata:Q117850,
        wikidata:Q12909644,
        wikidata:Q21286623,
        wikidata:Q49773,
        wikidata:Q5891,
        wikidata:Q58927801,
        wikidata:Q7252,
        wikidata:Q7278 .

wikidata:P115 rdfs:label "home venue"^^xsd:string ;
    rdf:first <http://www.semanticweb.org/ontologies/Wikidata#_:y5>,
        <http://www.semanticweb.org/ontologies/Wikidata#_:y7> ;
    rdfs:comment "home stadium or venue of a sports team or applicable performing arts organization"^^xsd:string ;
    rdfs:domain wikidata:Q215380,
        wikidata:Q27020041,
        wikidata:Q4438121 ;
    rdfs:range wikidata:Q811979 ;
    rdfs:subPropertyOf wikidata:P276 .

wikidata:P1151 a owl:FunctionalProperty ;
    rdfs:label "topic's main Wikimedia portal"^^xsd:string ;
    rdfs:comment "Wikimedia portal associated with this topic"^^xsd:string ;
    rdfs:range wikidata:Q4663903 .

wikidata:P1158 rdfs:label "location of landing"^^xsd:string ;
    rdfs:comment "location where the craft landed"^^xsd:string ;
    rdfs:domain wikidata:Q42889,
        wikidata:Q5916 ;
    rdfs:subPropertyOf wikidata:P276 .

wikidata:P1165 rdfs:label "home world"^^xsd:string ;
    rdfs:comment "home planet or natural satellite for a fictional character or species"^^xsd:string ;
    rdfs:domain wikidata:Q14514600,
        wikidata:Q15238535,
        wikidata:Q15707583,
        wikidata:Q95074,
        wikidata:Q989255 ;
    rdfs:range wikidata:Q3895768,
        wikidata:Q6999 .

wikidata:P118 rdfs:label "league"^^xsd:string ;
    rdfs:comment "league in which team or player plays or has played in"^^xsd:string ;
    rdfs:domain wikidata:Q13406554,
        wikidata:Q15229207,
        wikidata:Q16510064,
        wikidata:Q4438121,
        wikidata:Q5 ;
    rdfs:range wikidata:Q623109 ;
    rdfs:subPropertyOf wikidata:P1344 .

wikidata:P119 rdfs:label "place of burial"^^xsd:string ;
    rdfs:comment "location of grave, resting place, place of ash-scattering, etc. (e.g., town/city or cemetery) for a person or animal. There may be several places: e.g., re-burials, parts of body buried separately."^^xsd:string ;
    rdfs:domain wikidata:Q16334295,
        wikidata:Q199414,
        wikidata:Q21070598,
        wikidata:Q36341,
        wikidata:Q5,
        wikidata:Q502931,
        wikidata:Q57812611,
        wikidata:Q622852,
        wikidata:Q95074 ;
    rdfs:range wikidata:Q16859021,
        wikidata:Q3895768,
        wikidata:Q618123,
        wikidata:Q82794 ;
    rdfs:subPropertyOf wikidata:P276 .

wikidata:P1192 rdfs:label "connecting service"^^xsd:string ;
    rdfs:comment "service stopping at a station"^^xsd:string ;
    rdfs:domain wikidata:Q548662 ;
    rdfs:range wikidata:Q1067164,
        wikidata:Q16858238 .

wikidata:P1196 rdfs:label "manner of death"^^xsd:string ;
    rdfs:comment "general circumstances of a person's death; e.g. natural causes, accident, suicide, homicide, etc.  Use 'cause of death' (P509) for the specific physiological mechanism, e.g. heart attack, trauma, pneumonia..."^^xsd:string ;
    rdfs:domain wikidata:Q14514600,
        wikidata:Q16334298,
        wikidata:Q21070598,
        wikidata:Q215627,
        wikidata:Q26401003,
        wikidata:Q7239,
        wikidata:Q95074 .

wikidata:P1204 rdfs:label "Wikimedia portal's main topic"^^xsd:string ;
    rdfs:comment "primary topic of this Wikimedia portal"^^xsd:string ;
    rdfs:domain wikidata:Q4663903 .

wikidata:P122 rdfs:label "basic form of government"^^xsd:string ;
    rdfs:comment "subject's government"^^xsd:string ;
    rdfs:domain wikidata:Q1048835,
        wikidata:Q1145276,
        wikidata:Q3024240 ;
    rdfs:range wikidata:Q1307214 .

wikidata:P123 rdfs:label "publisher"^^xsd:string ;
    rdf:first <http://www.semanticweb.org/ontologies/Wikidata#_:y3> ;
    rdfs:comment "organization or person responsible for publishing books, periodicals, printed music, podcasts, games or software"^^xsd:string ;
    rdfs:domain wikidata:Q1002697,
        wikidata:Q1004,
        wikidata:Q11410,
        wikidata:Q1151067,
        wikidata:Q1172284,
        wikidata:Q1249682,
        wikidata:Q20655472,
        wikidata:Q20671381,
        wikidata:Q207628,
        wikidata:Q2352616,
        wikidata:Q2608849,
        wikidata:Q317623,
        wikidata:Q3331189,
        wikidata:Q35127,
        wikidata:Q373899,
        wikidata:Q41298,
        wikidata:Q42848,
        wikidata:Q429785,
        wikidata:Q43229,
        wikidata:Q47461344,
        wikidata:Q49848,
        wikidata:Q64341971,
        wikidata:Q7058673,
        wikidata:Q732577,
        wikidata:Q7725634,
        wikidata:Q7889,
        wikidata:Q79509036,
        wikidata:Q7982,
        wikidata:Q80793969,
        wikidata:Q8513,
        wikidata:Q95107111,
        wikidata:Q97180164 ;
    rdfs:range wikidata:Q1002697,
        wikidata:Q11032,
        wikidata:Q14350,
        wikidata:Q152416,
        wikidata:Q183888,
        wikidata:Q2085381,
        wikidata:Q2516866,
        wikidata:Q327333,
        wikidata:Q35127,
        wikidata:Q431289,
        wikidata:Q43229,
        wikidata:Q5,
        wikidata:Q56061 .

wikidata:P126 rdfs:label "maintained by"^^xsd:string ;
    rdfs:comment "person or organization in charge of keeping the subject (for instance an infrastructure) in functioning order"^^xsd:string ;
    rdfs:range wikidata:Q13226383,
        wikidata:Q14623646,
        wikidata:Q4164871,
        wikidata:Q43229,
        wikidata:Q5 .

wikidata:P1269 rdfs:label "facet of"^^xsd:string ;
    rdfs:comment "topic of which this item is an aspect, item that offers a broader perspective on the same topic"^^xsd:string .

wikidata:P128 rdfs:label "regulates (molecular biology)"^^xsd:string ;
    rdfs:comment "process regulated by a protein or RNA in molecular biology"^^xsd:string ;
    rdfs:domain wikidata:Q310899,
        wikidata:Q420927,
        wikidata:Q8054 ;
    rdfs:range wikidata:Q14860489,
        wikidata:Q2996394,
        wikidata:Q7187 .

wikidata:P1283 rdfs:label "filmography"^^xsd:string ;
    rdfs:comment "item for the list of films a person has contributed to. Don't use it to add film items. Instead, add actors as \"cast member\" (P161) on items for films, directors with \"director\" (P57)"^^xsd:string ;
    rdfs:domain wikidata:Q14514600,
        wikidata:Q16334295,
        wikidata:Q215380,
        wikidata:Q5,
        wikidata:Q56884562,
        wikidata:Q95074 ;
    rdfs:range wikidata:Q1371849 ;
    rdfs:subPropertyOf wikidata:P1455 .

wikidata:P1290 rdfs:label "godparent"^^xsd:string ;
    rdfs:comment "person who is the godparent of a given person"^^xsd:string ;
    rdfs:domain wikidata:Q21070598,
        wikidata:Q3500690,
        wikidata:Q5,
        wikidata:Q95074 ;
    rdfs:range wikidata:Q15632617,
        wikidata:Q21070598,
        wikidata:Q5 ;
    rdfs:subPropertyOf wikidata:P1038 .

wikidata:P1299 rdfs:label "depicted by"^^xsd:string ;
    rdf:first <http://www.semanticweb.org/ontologies/Wikidata#_:y1> ;
    rdfs:comment "object depicting this subject (creative works, books of the bible)"^^xsd:string ;
    rdfs:range wikidata:Q15709879,
        wikidata:Q386724,
        wikidata:Q713200 .

wikidata:P1302 rdfs:label "primary destinations"^^xsd:string ;
    rdfs:comment "major cities that a road serves"^^xsd:string .

wikidata:P1303 rdfs:label "instrument"^^xsd:string ;
    rdfs:comment "musical instrument that a person plays or teaches or used in a music occupation"^^xsd:string ;
    rdfs:domain wikidata:Q1278335,
        wikidata:Q146,
        wikidata:Q16145150,
        wikidata:Q16334295,
        wikidata:Q2675537,
        wikidata:Q5,
        wikidata:Q95074 ;
    rdfs:range wikidata:Q17172850,
        wikidata:Q29982117,
        wikidata:Q34379,
        wikidata:Q55990535 .

wikidata:P1308 rdfs:label "officeholder"^^xsd:string ;
    rdfs:comment "persons who hold and/or held an office or noble title"^^xsd:string ;
    rdfs:domain wikidata:Q21451536,
        wikidata:Q355567,
        wikidata:Q4164871 ;
    rdfs:range wikidata:Q5,
        wikidata:Q95074 .

wikidata:P1313 rdfs:label "office held by head of government"^^xsd:string ;
    rdfs:comment "political office that is fulfilled by the head of the government of this item"^^xsd:string ;
    rdfs:domain wikidata:Q15617994,
        wikidata:Q3895768,
        wikidata:Q56061,
        wikidata:Q640506,
        wikidata:Q7188 ;
    rdfs:range wikidata:Q4164871 .

wikidata:P1321 rdfs:label "place of origin (Switzerland)"^^xsd:string ;
    rdfs:comment "lieu d'origine/Heimatort/luogo d'origine of a Swiss national. Not be confused with place of birth or place of residence"^^xsd:string ;
    rdfs:range wikidata:Q70208 .

wikidata:P1336 rdfs:label "territory claimed by"^^xsd:string ;
    rdfs:comment "administrative divisions that claim control of a given area"^^xsd:string ;
    rdfs:domain wikidata:Q2221906,
        wikidata:Q618123 ;
    rdfs:range wikidata:Q43229,
        wikidata:Q5,
        wikidata:Q6256 .

wikidata:P134 rdfs:label "has dialect"^^xsd:string ;
    rdfs:comment "a former property, to be replaced by P4913, that describes a lot of things that are \"dialects\" related"^^xsd:string .

wikidata:P1343 rdfs:label "described by source"^^xsd:string ;
    rdfs:comment "work where this item is described"^^xsd:string ;
    rdfs:range wikidata:Q12139612,
        wikidata:Q1277575,
        wikidata:Q151885,
        wikidata:Q3331189,
        wikidata:Q386724,
        wikidata:Q43229 .

wikidata:P1363 rdfs:label "points/goal scored by"^^xsd:string ;
    rdfs:comment "person who scored a point or goal in a game"^^xsd:string .

wikidata:P137 rdfs:label "operator"^^xsd:string ;
    rdfs:comment "person, profession, or organization that operates the equipment, facility, or service"^^xsd:string ;
    rdfs:range wikidata:Q12737077,
        wikidata:Q14623646,
        wikidata:Q15911314,
        wikidata:Q16334295,
        wikidata:Q170584,
        wikidata:Q215627,
        wikidata:Q43229,
        wikidata:Q5,
        wikidata:Q56061,
        wikidata:Q95074 ;
    rdfs:subPropertyOf wikidata:P1535 .

wikidata:P1376 rdfs:label "capital of"^^xsd:string ;
    rdfs:comment "country, state, department, canton or other administrative division of which the municipality is the governmental seat"^^xsd:string ;
    rdfs:subPropertyOf wikidata:P131 .

wikidata:P138 rdfs:label "named after"^^xsd:string ;
    rdfs:comment "entity or event that inspired the subject's name, or namesake (in at least one language). Qualifier \"applies to name\" (P5168) can be used to indicate which one"^^xsd:string .

wikidata:P1382 a owl:SymmetricProperty ;
    rdfs:label "partially coincident with"^^xsd:string ;
    rdfs:comment "object that is partially part of, but not fully part of (P361), the subject"^^xsd:string .

wikidata:P1387 rdfs:label "political alignment"^^xsd:string ;
    rdfs:comment "political position within the political spectrum"^^xsd:string ;
    rdfs:domain wikidata:Q13473501,
        wikidata:Q163740,
        wikidata:Q20642011,
        wikidata:Q215627,
        wikidata:Q2738074,
        wikidata:Q35127,
        wikidata:Q5,
        wikidata:Q681615,
        wikidata:Q7210356,
        wikidata:Q95074 .

wikidata:P1398 a owl:AsymmetricProperty,
        owl:IrreflexiveProperty ;
    rdfs:label "structure replaces"^^xsd:string ;
    rdfs:comment "the item this building or structure replaced, at the same geographic location"^^xsd:string ;
    rdfs:domain wikidata:Q27096235,
        wikidata:Q811979,
        wikidata:Q82794 ;
    rdfs:range wikidata:Q27096235,
        wikidata:Q811979,
        wikidata:Q82794 ;
    rdfs:subPropertyOf wikidata:P1365 .

wikidata:P1399 rdfs:label "convicted of"^^xsd:string ;
    rdfs:comment "crime a person was convicted of"^^xsd:string ;
    rdfs:domain wikidata:Q16334295,
        wikidata:Q43229,
        wikidata:Q5,
        wikidata:Q95074 ;
    rdfs:range wikidata:Q1184244,
        wikidata:Q124734,
        wikidata:Q1323212,
        wikidata:Q1456832,
        wikidata:Q160598,
        wikidata:Q2628882,
        wikidata:Q41554073,
        wikidata:Q690768,
        wikidata:Q83267 .

wikidata:P140 rdfs:label "religion"^^xsd:string ;
    rdfs:comment "religion of a person, organization or religious building, or associated with this subject"^^xsd:string ;
    rdfs:domain wikidata:Q12518,
        wikidata:Q13414953,
        wikidata:Q1370598,
        wikidata:Q14897293,
        wikidata:Q16334295,
        wikidata:Q16970,
        wikidata:Q17524420,
        wikidata:Q192909,
        wikidata:Q2072238,
        wikidata:Q208145,
        wikidata:Q21029893,
        wikidata:Q21070568,
        wikidata:Q2110808,
        wikidata:Q23847174,
        wikidata:Q24334685,
        wikidata:Q373074,
        wikidata:Q375011,
        wikidata:Q391414,
        wikidata:Q39614,
        wikidata:Q4024737,
        wikidata:Q40953,
        wikidata:Q4164871,
        wikidata:Q43229,
        wikidata:Q44539,
        wikidata:Q44613,
        wikidata:Q47848,
        wikidata:Q49773,
        wikidata:Q5,
        wikidata:Q60469796,
        wikidata:Q607241,
        wikidata:Q628455,
        wikidata:Q63187345,
        wikidata:Q811979,
        wikidata:Q838948 ;
    rdfs:range wikidata:Q11197007,
        wikidata:Q13414953,
        wikidata:Q1530022,
        wikidata:Q16334295,
        wikidata:Q17364638,
        wikidata:Q1826286,
        wikidata:Q2061186,
        wikidata:Q2915955,
        wikidata:Q34651,
        wikidata:Q4392985,
        wikidata:Q6566418,
        wikidata:Q9174 .

wikidata:P1408 rdfs:label "licensed to broadcast to"^^xsd:string ;
    rdfs:comment "place that a radio/TV station is licensed/required to broadcast to"^^xsd:string ;
    rdfs:range wikidata:Q2221906,
        wikidata:Q78758464 .

wikidata:P1411 rdfs:label "nominated for"^^xsd:string ;
    rdfs:comment "award nomination received by a person, organisation or creative work (inspired from \"award received\" (Property:P166))"^^xsd:string ;
    rdfs:domain wikidata:Q26401003,
        wikidata:Q386724,
        wikidata:Q43229,
        wikidata:Q5 ;
    rdfs:range wikidata:Q378427,
        wikidata:Q38033430,
        wikidata:Q4220917,
        wikidata:Q618779 .

wikidata:P1414 rdfs:label "GUI toolkit or framework"^^xsd:string ;
    rdfs:comment "framework or toolkit a program uses to display the graphical user interface"^^xsd:string ;
    rdfs:range wikidata:Q1193246,
        wikidata:Q47146 ;
    rdfs:subPropertyOf wikidata:P1547 .

wikidata:P1423 rdfs:label "template has topic"^^xsd:string ;
    rdfs:comment "topic related to template"^^xsd:string ;
    rdfs:domain wikidata:Q11266439 .

wikidata:P1427 rdfs:label "start point"^^xsd:string ;
    rdfs:comment "starting place of this journey, flight, voyage, trek, migration etc."^^xsd:string ;
    rdfs:domain wikidata:Q1190554,
        wikidata:Q40218,
        wikidata:Q506572,
        wikidata:Q628179,
        wikidata:Q83620 ;
    rdfs:range wikidata:Q17334923,
        wikidata:Q618123 ;
    rdfs:subPropertyOf wikidata:P276 .

wikidata:P1429 rdfs:label "has pet"^^xsd:string ;
    rdfs:comment "pet that a person owns"^^xsd:string ;
    rdfs:domain wikidata:Q14514600,
        wikidata:Q215627,
        wikidata:Q95074 ;
    rdfs:range wikidata:Q2593744,
        wikidata:Q729 .

wikidata:P1431 rdfs:label "executive producer"^^xsd:string ;
    rdfs:comment "executive producer of a movie or TV show"^^xsd:string ;
    rdfs:domain wikidata:Q386724 ;
    rdfs:range wikidata:Q5 .

wikidata:P1432 rdfs:label "B-side"^^xsd:string ;
    rdfs:comment "song/track which is the B-side of this single"^^xsd:string .

wikidata:P1434 rdfs:label "takes place in fictional universe"^^xsd:string ;
    rdfs:comment "the subject is a work describing a fictional universe, i.e. whose plot occurs in this universe."^^xsd:string ;
    rdfs:domain wikidata:Q386724 ;
    rdfs:range wikidata:Q3895768,
        wikidata:Q559618,
        wikidata:Q867335,
        wikidata:Q9134 .

wikidata:P1435 rdfs:label "heritage designation"^^xsd:string ;
    rdfs:comment "heritage designation of a cultural or natural site"^^xsd:string ;
    rdfs:range wikidata:Q210272,
        wikidata:Q386426 ;
    rdfs:subPropertyOf wikidata:P31,
        wikidata:P527 .

wikidata:P144 rdfs:label "based on"^^xsd:string ;
    rdfs:comment "the work(s) used as the basis for subject item"^^xsd:string ;
    rdfs:domain wikidata:Q12047392,
        wikidata:Q16686448,
        wikidata:Q34770,
        wikidata:Q3695082,
        wikidata:Q386724,
        wikidata:Q65943,
        wikidata:Q8192,
        wikidata:Q95107111 ;
    rdfs:range wikidata:Q12047392,
        wikidata:Q16686448,
        wikidata:Q24334685,
        wikidata:Q34770,
        wikidata:Q3695082,
        wikidata:Q386724,
        wikidata:Q65943,
        wikidata:Q8192,
        wikidata:Q95107111 ;
    rdfs:subPropertyOf wikidata:P8371 .

wikidata:P1441 rdfs:label "present in work"^^xsd:string ;
    rdfs:comment "this (fictional or fictionalized) entity or person appears in that work as part of the narration (use P2860 for works citing other works, P361/P1433 for works being part of other works, P1343 for entities described in non-fictional accounts)"^^xsd:string ;
    rdfs:domain wikidata:Q12404340,
        wikidata:Q13002315,
        wikidata:Q14897293,
        wikidata:Q15306849,
        wikidata:Q1707847,
        wikidata:Q21070568,
        wikidata:Q21070598,
        wikidata:Q24334685,
        wikidata:Q3658341,
        wikidata:Q39201,
        wikidata:Q43229,
        wikidata:Q5 ;
    rdfs:range wikidata:Q386724,
        wikidata:Q7725310 .

wikidata:P1444 rdfs:label "destination point"^^xsd:string ;
    rdfs:comment "intended destination for this route (journey, flight, sailing, exploration, migration, etc.)"^^xsd:string ;
    rdfs:domain wikidata:Q1190554,
        wikidata:Q506572,
        wikidata:Q628179,
        wikidata:Q83620 ;
    rdfs:range wikidata:Q17334923 ;
    rdfs:subPropertyOf wikidata:P276 .

wikidata:P1445 rdfs:label "fictional universe described in"^^xsd:string ;
    rdfs:comment "to link a fictional universe with a work that describes it: <universe> \"described in the work:\" <work>"^^xsd:string ;
    rdfs:domain wikidata:Q559618,
        wikidata:Q867335,
        wikidata:Q9134 ;
    rdfs:range wikidata:Q386724 .

wikidata:P1454 rdfs:label "legal form"^^xsd:string ;
    rdfs:comment "legal form of an entity"^^xsd:string ;
    rdfs:domain wikidata:Q14623646,
        wikidata:Q43229,
        wikidata:Q5 ;
    rdfs:range wikidata:Q12047392 ;
    rdfs:subPropertyOf wikidata:P31 .

wikidata:P1456 rdfs:label "list of monuments"^^xsd:string ;
    rdfs:comment "link to the list of heritage monuments in the place/area"^^xsd:string ;
    rdfs:domain wikidata:Q2221906 ;
    rdfs:range wikidata:Q13406463 ;
    rdfs:subPropertyOf wikidata:P1455,
        wikidata:P2354 .

wikidata:P1462 rdfs:label "standards body"^^xsd:string ;
    rdfs:comment "organisation that published or maintains the standard governing an item"^^xsd:string ;
    rdfs:range wikidata:Q43229 ;
    rdfs:subPropertyOf wikidata:P790 .

wikidata:P1464 rdfs:label "category for people born here"^^xsd:string ;
    rdfs:comment "category item that groups people born in this place"^^xsd:string ;
    rdfs:domain wikidata:Q618123,
        wikidata:Q82794 ;
    rdfs:range wikidata:Q4167836 ;
    rdfs:subPropertyOf wikidata:P910 .

wikidata:P1465 rdfs:label "category for people who died here"^^xsd:string ;
    rdfs:comment "category item for people who died in this location"^^xsd:string ;
    rdfs:domain wikidata:Q618123,
        wikidata:Q82794 ;
    rdfs:range wikidata:Q4167836 ;
    rdfs:subPropertyOf wikidata:P910 .

wikidata:P1478 rdfs:label "has immediate cause"^^xsd:string ;
    rdfs:comment "nearest, proximate thing that directly resulted in the subject as outcome or effect. Used in conjunction with 'has cause' (i.e. underlying cause) and 'has contributing factor'. See 'Help:Modeling causes'."^^xsd:string .

wikidata:P149 rdfs:label "architectural style"^^xsd:string ;
    rdfs:comment "architectural style of a structure"^^xsd:string ;
    rdfs:domain wikidata:Q1497375,
        wikidata:Q15243209,
        wikidata:Q391414,
        wikidata:Q811979 ;
    rdfs:range wikidata:Q1792644,
        wikidata:Q32880 ;
    rdfs:subPropertyOf wikidata:P135 .

wikidata:P150 rdfs:label "contains administrative territorial entity"^^xsd:string ;
    rdfs:comment "(list of) direct subdivisions of an administrative territorial entity"^^xsd:string ;
    rdfs:domain wikidata:Q1048835,
        wikidata:Q15042037,
        wikidata:Q3299260,
        wikidata:Q56061 ;
    rdfs:range wikidata:Q56061 ;
    rdfs:subPropertyOf wikidata:P527 .

wikidata:P1531 rdfs:label "parent of this hybrid, breed, or cultivar"^^xsd:string ;
    rdfs:comment "杂交种或品种的祖先物种"^^xsd:string .

wikidata:P1532 rdfs:label "country for sport"^^xsd:string ;
    rdfs:comment "country a person or a team represents when playing a sport"^^xsd:string ;
    rdfs:domain wikidata:Q16334295,
        wikidata:Q2485448,
        wikidata:Q5 ;
    rdfs:range wikidata:Q484652,
        wikidata:Q56061,
        wikidata:Q6256,
        wikidata:Q7275,
        wikidata:Q82794 ;
    rdfs:subPropertyOf wikidata:P17 .

wikidata:P1533 rdfs:label "family name identical to this given name"^^xsd:string ;
    rdfs:comment "last name that is the same as a given first name. Use on items for given names"^^xsd:string ;
    rdfs:domain wikidata:Q202444 ;
    rdfs:range wikidata:Q101352 ;
    rdfs:subPropertyOf wikidata:P1889 .

wikidata:P1546 rdfs:label "motto"^^xsd:string ;
    rdfs:comment "description of the motto of the subject"^^xsd:string ;
    rdfs:domain wikidata:Q43229 ;
    rdfs:range wikidata:Q42470 .

wikidata:P1560 a owl:SymmetricProperty ;
    rdfs:label "name version for other gender"^^xsd:string ;
    rdfs:comment "equivalent name (with respect to the meaning of the name) in the same language: female version of a male first name, male version of a female first name. Add primarily the closest matching one"^^xsd:string .

wikidata:P157 rdfs:label "killed by"^^xsd:string ;
    rdfs:comment "person who killed the subject"^^xsd:string ;
    rdfs:domain wikidata:Q5,
        wikidata:Q95074 ;
    rdfs:range wikidata:Q43229,
        wikidata:Q5,
        wikidata:Q95074 ;
    rdfs:subPropertyOf wikidata:P3342 .

wikidata:P1574 rdfs:label "exemplar of"^^xsd:string ;
    rdfs:comment "property for manuscripts, autographs, incunabula, distinct printed copies"^^xsd:string ;
    rdfs:domain wikidata:Q1261026,
        wikidata:Q18593264,
        wikidata:Q187947,
        wikidata:Q7725634,
        wikidata:Q87167 ;
    rdfs:subPropertyOf wikidata:P31 .

wikidata:P1576 rdfs:label "lifestyle"^^xsd:string ;
    rdfs:comment "typical way of life of an individual, group, or culture"^^xsd:string ;
    rdfs:domain wikidata:Q11042,
        wikidata:Q14514600,
        wikidata:Q15632617,
        wikidata:Q16334295,
        wikidata:Q43229,
        wikidata:Q5,
        wikidata:Q95074 ;
    rdfs:range wikidata:Q117850,
        wikidata:Q188976,
        wikidata:Q1914636,
        wikidata:Q2515887,
        wikidata:Q264965,
        wikidata:Q3769299,
        wikidata:Q5410500 .

wikidata:P1582 rdfs:label "natural product of taxon"^^xsd:string ;
    rdfs:comment "links a natural product with its source (animal, plant, fungal, algal, etc.)"^^xsd:string ;
    rdfs:range wikidata:Q16521,
        wikidata:Q502895,
        wikidata:Q55983715 .

wikidata:P1589 rdfs:label "lowest point"^^xsd:string ;
    rdfs:comment "point with lowest elevation in the country, region, city or area"^^xsd:string ;
    rdfs:domain wikidata:Q618123 ;
    rdfs:range wikidata:Q2221906,
        wikidata:Q618123 .

wikidata:P1596 rdfs:label "penalty"^^xsd:string ;
    rdfs:comment "penalty imposed by an authority"^^xsd:string ;
    rdfs:range wikidata:Q1763090,
        wikidata:Q186361 .

wikidata:P16 rdfs:label "highway system"^^xsd:string ;
    rdfs:comment "system (or specific country specific road type) of which the highway is a part"^^xsd:string ;
    rdfs:domain wikidata:Q34442,
        wikidata:Q353027 ;
    rdfs:range wikidata:Q3241753,
        wikidata:Q34442,
        wikidata:Q358078 ;
    rdfs:subPropertyOf wikidata:P361 .

wikidata:P1611 rdfs:label "NATO code for grade"^^xsd:string ;
    rdfs:comment "NATO Code for Grades of Military Personnel"^^xsd:string ;
    rdfs:domain wikidata:Q56019 .

wikidata:P162 rdfs:label "producer"^^xsd:string ;
    rdfs:comment "person(s) who produced the film, musical work, theatrical production, etc. (for film, this does not include executive producers, associate producers, etc.) [for production company, use P272, video games - use P178]"^^xsd:string ;
    rdfs:domain wikidata:Q386724 ;
    rdfs:range wikidata:Q10648343,
        wikidata:Q14514600,
        wikidata:Q18127,
        wikidata:Q215380,
        wikidata:Q5,
        wikidata:Q7247847,
        wikidata:Q95074 .

wikidata:P163 rdfs:label "flag"^^xsd:string ;
    rdfs:comment "subject's flag"^^xsd:string ;
    rdfs:range wikidata:Q14660,
        wikidata:Q17335294,
        wikidata:Q64682301 .

wikidata:P1639 a owl:SymmetricProperty ;
    rdfs:label "pendant of"^^xsd:string ;
    rdfs:comment "other work in a pair of opposing artworks, such as wedding portraits, commissioned together, but not always"^^xsd:string ;
    rdfs:domain wikidata:Q7725310,
        wikidata:Q838948 ;
    rdfs:range wikidata:Q7725310,
        wikidata:Q838948 .

wikidata:P1640 rdfs:label "curator"^^xsd:string ;
    rdfs:comment "content specialist responsible for this collection or exhibition"^^xsd:string ;
    rdfs:domain wikidata:Q2668072,
        wikidata:Q33506,
        wikidata:Q464980,
        wikidata:Q4801521 ;
    rdfs:subPropertyOf wikidata:P3342 .

wikidata:P1654 rdfs:label "wing configuration"^^xsd:string ;
    rdfs:comment "configuration of wing(s) used by an aircraft"^^xsd:string ;
    rdfs:range wikidata:Q2992500 .

wikidata:P1657 rdfs:label "MPAA film rating"^^xsd:string ;
    rdfs:comment "US film classification administered by the Motion Picture Association of America"^^xsd:string ;
    rdfs:domain wikidata:Q11424 ;
    rdfs:range wikidata:Q23660208 .

wikidata:P167 a owl:AsymmetricProperty,
        owl:IrreflexiveProperty ;
    rdfs:label "structure replaced by"^^xsd:string ;
    rdfs:comment "the item which replaced this building or structure, at the same geographic location"^^xsd:string ;
    rdfs:domain wikidata:Q27096235,
        wikidata:Q811979,
        wikidata:Q82794 ;
    rdfs:range wikidata:Q27096235,
        wikidata:Q811979,
        wikidata:Q82794 ;
    rdfs:subPropertyOf wikidata:P1366 .

wikidata:P1672 rdfs:label "this taxon is source of"^^xsd:string ;
    rdfs:comment "links a taxon to natural products it produces. Note that it does not say \"this taxon is the source of\" or \"this taxon is a source of\" as this may vary. Some products may be yielded by more than one taxon."^^xsd:string ;
    rdfs:domain wikidata:Q16521,
        wikidata:Q502895,
        wikidata:Q55983715 .

wikidata:P169 rdfs:label "chief executive officer"^^xsd:string ;
    rdf:first <http://www.semanticweb.org/ontologies/Wikidata#_:y4> ;
    rdfs:comment "highest-ranking corporate officer appointed as the CEO within an organization"^^xsd:string ;
    rdfs:domain wikidata:Q1880737,
        wikidata:Q43229,
        wikidata:Q5446565 ;
    rdfs:range wikidata:Q15632617,
        wikidata:Q5 ;
    rdfs:subPropertyOf wikidata:P1037,
        wikidata:P2828 .

wikidata:P1716 rdfs:label "brand"^^xsd:string ;
    rdfs:comment "commercial brand associated with the item"^^xsd:string ;
    rdfs:domain wikidata:Q18127,
        wikidata:Q2031291,
        wikidata:Q20671381,
        wikidata:Q22811462,
        wikidata:Q2424752 ;
    rdfs:range wikidata:Q1412386,
        wikidata:Q167270,
        wikidata:Q431289,
        wikidata:Q5 .

wikidata:P172 rdfs:label "ethnic group"^^xsd:string ;
    rdfs:comment "subject's ethnicity (consensus is that a VERY high standard of proof is needed for this field to be used. In general this means 1) the subject claims it themself, or 2) it is widely agreed on by scholars, or 3) is fictional and portrayed as such)"^^xsd:string ;
    rdfs:domain wikidata:Q13002315,
        wikidata:Q133004,
        wikidata:Q215627,
        wikidata:Q2239243,
        wikidata:Q28790362,
        wikidata:Q34770,
        wikidata:Q4271324,
        wikidata:Q64272108,
        wikidata:Q8436,
        wikidata:Q95074 ;
    rdfs:range wikidata:Q103817,
        wikidata:Q133311,
        wikidata:Q21192438,
        wikidata:Q231002,
        wikidata:Q2472587,
        wikidata:Q2531956,
        wikidata:Q2590445,
        wikidata:Q28790362,
        wikidata:Q3254959,
        wikidata:Q41710,
        wikidata:Q6266 .

wikidata:P1731 rdfs:label "Fach"^^xsd:string ;
    rdfs:comment "describes the special ablilites of an operatic singers voice"^^xsd:string ;
    rdfs:domain wikidata:Q5,
        wikidata:Q95074 ;
    rdfs:range wikidata:Q1748957 ;
    rdfs:subPropertyOf wikidata:P412 .

wikidata:P1740 a owl:FunctionalProperty ;
    rdfs:label "category for films shot at this location"^^xsd:string ;
    rdfs:comment "the object is a category for films shot at or in the subject"^^xsd:string ;
    rdfs:domain wikidata:Q618123 .

wikidata:P175 rdfs:label "performer"^^xsd:string ;
    rdfs:comment "actor, musician, band or other performer associated with this role or musical work"^^xsd:string ;
    rdfs:domain wikidata:Q1656682,
        wikidata:Q1707847,
        wikidata:Q386724,
        wikidata:Q95074,
        wikidata:Q98216532 ;
    rdfs:range wikidata:Q15632617,
        wikidata:Q15711870,
        wikidata:Q15773317,
        wikidata:Q16334295,
        wikidata:Q2088357,
        wikidata:Q215380,
        wikidata:Q5,
        wikidata:Q52688389,
        wikidata:Q60614352,
        wikidata:Q6619719 ;
    rdfs:subPropertyOf wikidata:P710 .

wikidata:P1750 rdfs:label "name day"^^xsd:string ;
    rdfs:comment "day of the year associated with a first/given name. A qualifier should be used to identify the calendar that is being used. Distinguish from \"feast day\" (P:P841)"^^xsd:string ;
    rdfs:domain wikidata:Q202444 ;
    rdfs:range wikidata:Q14795564 .

wikidata:P177 rdfs:label "crosses"^^xsd:string ;
    rdfs:comment "obstacle (body of water, road, railway...) which this bridge crosses over or this tunnel goes under"^^xsd:string ;
    rdfs:domain wikidata:Q15720793,
        wikidata:Q25653,
        wikidata:Q811430 ;
    rdfs:range wikidata:Q618123 .

wikidata:P178 rdfs:label "developer"^^xsd:string ;
    rdf:first <http://www.semanticweb.org/ontologies/Wikidata#_:y10> ;
    rdfs:comment "organisation or person that developed the item"^^xsd:string ;
    rdfs:domain wikidata:Q10929058,
        wikidata:Q151885,
        wikidata:Q15401930,
        wikidata:Q1630279,
        wikidata:Q1979154,
        wikidata:Q317623,
        wikidata:Q3249551,
        wikidata:Q58778,
        wikidata:Q63437139,
        wikidata:Q7058673,
        wikidata:Q853614 ;
    rdfs:range wikidata:Q177634,
        wikidata:Q43229,
        wikidata:Q5 ;
    rdfs:subPropertyOf wikidata:P170 .

wikidata:P179 rdfs:label "part of the series"^^xsd:string ;
    rdfs:comment "series which contains the subject"^^xsd:string ;
    rdfs:domain wikidata:Q1238720,
        wikidata:Q15900616,
        wikidata:Q27968055,
        wikidata:Q386724,
        wikidata:Q42889,
        wikidata:Q43229,
        wikidata:Q811704,
        wikidata:Q853614 ;
    rdfs:range wikidata:Q11578774,
        wikidata:Q133250,
        wikidata:Q15275719,
        wikidata:Q16858238,
        wikidata:Q17518557,
        wikidata:Q20937557,
        wikidata:Q3511132,
        wikidata:Q43229,
        wikidata:Q63183159,
        wikidata:Q7725310,
        wikidata:Q811701 ;
    rdfs:subPropertyOf wikidata:P361 .

wikidata:P1791 rdfs:label "category of people buried here"^^xsd:string ;
    rdfs:comment "Wikimedia category for people with a burial site within this area"^^xsd:string ;
    rdfs:domain wikidata:Q27096213 .

wikidata:P1792 rdfs:label "category of associated people"^^xsd:string ;
    rdfs:comment "Wikimedia category for people associated with this place or organization"^^xsd:string ;
    rdfs:domain wikidata:Q15642541,
        wikidata:Q2221906,
        wikidata:Q43229,
        wikidata:Q618123 ;
    rdfs:subPropertyOf wikidata:P910 .

wikidata:P180 rdfs:label "depicts"^^xsd:string ;
    rdfs:comment "depicted entity (see also P921: main subject)"^^xsd:string ;
    rdfs:domain wikidata:Q101002748,
        wikidata:Q1243409,
        wikidata:Q1261026,
        wikidata:Q1406161,
        wikidata:Q1415274,
        wikidata:Q1424805,
        wikidata:Q220659,
        wikidata:Q23649976,
        wikidata:Q386724,
        wikidata:Q47433,
        wikidata:Q478798,
        wikidata:Q52827,
        wikidata:Q68183127,
        wikidata:Q8242,
        wikidata:Q834104 .

wikidata:P1809 rdfs:label "choreographer"^^xsd:string ;
    rdfs:comment "person(s) who did the choreography"^^xsd:string ;
    rdfs:domain wikidata:Q11424,
        wikidata:Q11639,
        wikidata:Q15079786,
        wikidata:Q180856,
        wikidata:Q2743,
        wikidata:Q34508,
        wikidata:Q43099500,
        wikidata:Q58483088 ;
    rdfs:range wikidata:Q5 .

wikidata:P1817 rdfs:label "addressee"^^xsd:string ;
    rdfs:comment "person or organization to whom a letter or note is addressed"^^xsd:string ;
    rdfs:domain wikidata:Q49848 ;
    rdfs:range wikidata:Q16334295,
        wikidata:Q43229,
        wikidata:Q5 .

wikidata:P183 rdfs:label "endemic to"^^xsd:string ;
    rdfs:comment "sole location or habitat type where the taxon lives"^^xsd:string ;
    rdfs:domain wikidata:Q16521,
        wikidata:Q2239243 ;
    rdfs:range wikidata:Q46831,
        wikidata:Q618123,
        wikidata:Q82794 .

wikidata:P184 a owl:AsymmetricProperty,
        owl:IrreflexiveProperty ;
    rdfs:label "doctoral advisor"^^xsd:string ;
    rdfs:comment "person who supervised the doctorate or PhD thesis of the subject"^^xsd:string ;
    rdfs:domain wikidata:Q15632617,
        wikidata:Q5 ;
    rdfs:range wikidata:Q15632617,
        wikidata:Q5 ;
    rdfs:subPropertyOf wikidata:P1066,
        wikidata:P7604 .

wikidata:P1840 rdfs:label "investigated by"^^xsd:string ;
    rdfs:comment "person or organization involved in investigation of the item"^^xsd:string ;
    rdfs:domain wikidata:Q1190554,
        wikidata:Q16334295,
        wikidata:Q5 ;
    rdfs:range wikidata:Q43229,
        wikidata:Q5,
        wikidata:Q732717,
        wikidata:Q8222382 .

wikidata:P186 rdfs:label "made from material"^^xsd:string ;
    rdfs:comment "material the subject is made of or derived from"^^xsd:string ;
    rdfs:domain wikidata:Q223557,
        wikidata:Q25416091 ;
    rdfs:range wikidata:Q11344,
        wikidata:Q1362373,
        wikidata:Q2095,
        wikidata:Q214609,
        wikidata:Q25403900,
        wikidata:Q40050,
        wikidata:Q4936952,
        wikidata:Q7239,
        wikidata:Q79529 ;
    rdfs:subPropertyOf wikidata:P2283 .

wikidata:P1875 a owl:AsymmetricProperty,
        owl:IrreflexiveProperty ;
    rdfs:label "represented by"^^xsd:string ;
    rdfs:comment "person or agency that represents or manages the subject"^^xsd:string ;
    rdfs:domain wikidata:Q16334295,
        wikidata:Q5 ;
    rdfs:range wikidata:Q16334295,
        wikidata:Q5 .

wikidata:P1876 rdfs:label "vehicle"^^xsd:string ;
    rdfs:comment "vessel involved in this mission, voyage or event"^^xsd:string ;
    rdfs:range wikidata:Q42889 .

wikidata:P1877 rdfs:label "after a work by"^^xsd:string ;
    rdfs:comment "artist whose work strongly inspired/ was copied in this item"^^xsd:string ;
    rdfs:domain wikidata:Q386724 ;
    rdfs:range wikidata:Q127843,
        wikidata:Q43229,
        wikidata:Q5 ;
    rdfs:subPropertyOf wikidata:P3342 .

wikidata:P1879 a owl:FunctionalProperty ;
    rdfs:label "income classification (Philippines)"^^xsd:string ;
    rdfs:comment "classification grade of a Philippine local government unit based on income"^^xsd:string ;
    rdfs:domain wikidata:Q1350310 .

wikidata:P1881 rdfs:label "list of characters"^^xsd:string ;
    rdfs:comment "Wikimedia page with the list of characters for this work"^^xsd:string ;
    rdfs:domain wikidata:Q386724 ;
    rdfs:range wikidata:Q13406463 ;
    rdfs:subPropertyOf wikidata:P2354 .

wikidata:P1885 rdfs:label "cathedral"^^xsd:string ;
    rdfs:comment "principal church of a religious district"^^xsd:string ;
    rdfs:domain wikidata:Q1492823,
        wikidata:Q427961,
        wikidata:Q665487 ;
    rdfs:range wikidata:Q2977 ;
    rdfs:subPropertyOf wikidata:P159 .

wikidata:P1891 rdfs:label "signatory"^^xsd:string ;
    rdfs:comment "person, country, or organization that has signed an official document (use P50 for author)"^^xsd:string ;
    rdfs:domain wikidata:Q49848 ;
    rdfs:range wikidata:Q43229,
        wikidata:Q5,
        wikidata:Q7275 ;
    rdfs:subPropertyOf wikidata:P3342 .

wikidata:P190 a owl:SymmetricProperty ;
    rdfs:label "twinned administrative body"^^xsd:string ;
    rdfs:comment "twin towns, sister cities, twinned municipalities and other localities that have a partnership or cooperative agreement, either legally or informally acknowledged by their governments"^^xsd:string ;
    rdfs:domain wikidata:Q123705,
        wikidata:Q3914,
        wikidata:Q486972,
        wikidata:Q4989906,
        wikidata:Q515,
        wikidata:Q55488,
        wikidata:Q56061,
        wikidata:Q7930989 ;
    rdfs:range wikidata:Q123705,
        wikidata:Q3914,
        wikidata:Q486972,
        wikidata:Q4989906,
        wikidata:Q515,
        wikidata:Q55488,
        wikidata:Q56061,
        wikidata:Q7930989 .

wikidata:P1906 rdfs:label "office held by head of state"^^xsd:string ;
    rdfs:comment "political office that is fulfilled by the head of state of this item"^^xsd:string ;
    rdfs:domain wikidata:Q1145276,
        wikidata:Q15617994,
        wikidata:Q3024240,
        wikidata:Q7275 ;
    rdfs:range wikidata:Q21451536,
        wikidata:Q4164871,
        wikidata:Q48352 .

wikidata:P1923 rdfs:label "participating team"^^xsd:string ;
    rdfs:comment "Like 'Participant' (P710) but for teams. For an event like a cycle race or a football match you can use this property to list the teams and P710 to list the individuals (with 'member of sports team' (P54) as a qualifier for the individuals)"^^xsd:string ;
    rdfs:range wikidata:Q12973014,
        wikidata:Q847017 ;
    rdfs:subPropertyOf wikidata:P710 .

wikidata:P193 rdfs:label "main building contractor"^^xsd:string ;
    rdfs:comment "the main organization responsible for construction of this structure or building"^^xsd:string ;
    rdfs:domain wikidata:Q811979 ;
    rdfs:range wikidata:Q289612,
        wikidata:Q43229,
        wikidata:Q5 ;
    rdfs:subPropertyOf wikidata:P176 .

wikidata:P194 rdfs:label "legislative body"^^xsd:string ;
    rdfs:comment "legislative body governing this entity; political institution with elected representatives, such as a parliament/legislature or council"^^xsd:string ;
    rdfs:domain wikidata:Q1048835,
        wikidata:Q1145276,
        wikidata:Q4120211,
        wikidata:Q56061,
        wikidata:Q7188 ;
    rdfs:range wikidata:Q10553309,
        wikidata:Q11204,
        wikidata:Q15238535,
        wikidata:Q6501447 .

wikidata:P195 rdfs:label "collection"^^xsd:string ;
    rdf:first <http://www.semanticweb.org/ontologies/Wikidata#_:y2> ;
    rdfs:comment "art, museum, archival, or bibliographic collection the subject is part of"^^xsd:string ;
    rdfs:domain wikidata:Q20937557,
        wikidata:Q223557,
        wikidata:Q2424752,
        wikidata:Q36161,
        wikidata:Q386724,
        wikidata:Q51255340 ;
    rdfs:range wikidata:Q2668072,
        wikidata:Q334453,
        wikidata:Q3707858,
        wikidata:Q43229,
        wikidata:Q811979,
        wikidata:Q8513 ;
    rdfs:subPropertyOf wikidata:P361 .

wikidata:P1951 rdfs:label "investor"^^xsd:string ;
    rdfs:comment "individual or organization which invests money in the item for the purpose of obtaining financial return on their investment"^^xsd:string .

wikidata:P196 rdfs:label "minor planet group"^^xsd:string ;
    rdfs:comment "is in grouping of minor planets according to similar orbital characteristics"^^xsd:string ;
    rdfs:domain wikidata:Q1022867,
        wikidata:Q947662 ;
    rdfs:range wikidata:Q1022867,
        wikidata:Q2332332,
        wikidata:Q3235978 ;
    rdfs:subPropertyOf wikidata:P361 .

wikidata:P197 a owl:SymmetricProperty ;
    rdfs:label "adjacent station"^^xsd:string ;
    rdfs:comment "the stations next to this station, sharing the same line(s)"^^xsd:string ;
    rdfs:domain wikidata:Q228332 ;
    rdfs:range wikidata:Q228332 .

wikidata:P1981 rdfs:label "FSK film rating"^^xsd:string ;
    rdfs:comment "permitted audience of a film, according to the German film-rating system (add Prüfnummer with qualifier \"P2676\")"^^xsd:string ;
    rdfs:domain wikidata:Q11424,
        wikidata:Q15416,
        wikidata:Q1983062 ;
    rdfs:range wikidata:Q23649976 .

wikidata:P199 rdfs:label "business division"^^xsd:string ;
    rdfs:comment "organizational divisions of this organization (which are not independent legal entities)"^^xsd:string ;
    rdfs:domain wikidata:Q4830453,
        wikidata:Q5446565,
        wikidata:Q783794 .

wikidata:P1990 rdfs:label "species kept"^^xsd:string ;
    rdfs:comment "taxa, preferably species, present at a zoo, botanical garden,  collection, or other institution. NOT specific animals, not for any geographic location"^^xsd:string ;
    rdfs:domain wikidata:Q165044,
        wikidata:Q167346,
        wikidata:Q1714375,
        wikidata:Q181916,
        wikidata:Q194195,
        wikidata:Q2281788,
        wikidata:Q2333552,
        wikidata:Q33506,
        wikidata:Q43501 ;
    rdfs:range wikidata:Q16521,
        wikidata:Q38829,
        wikidata:Q502895 ;
    rdfs:subPropertyOf wikidata:P2670 .

wikidata:P1995 rdfs:label "health specialty"^^xsd:string ;
    rdfs:comment "main specialty that diagnoses, prevent human illness, injury and other physical and mental impairments"^^xsd:string ;
    rdfs:domain wikidata:Q12136,
        wikidata:Q55214844,
        wikidata:Q639907 .

wikidata:P1999 rdfs:label "UNESCO language status"^^xsd:string ;
    rdfs:comment "degree of endangerment of a language conferred by the UNESCO Atlas of World Languages in Danger"^^xsd:string ;
    rdfs:domain wikidata:Q17376908 .

wikidata:P200 rdfs:label "inflows"^^xsd:string ;
    rdfs:comment "major inflow sources — rivers, aquifers, glacial runoff, etc. Some terms may not be place names, e.g. none"^^xsd:string ;
    rdfs:domain wikidata:Q15324,
        wikidata:Q30092755,
        wikidata:Q337567 ;
    rdfs:range wikidata:Q355304 .

wikidata:P201 rdfs:label "lake outflow"^^xsd:string ;
    rdfs:comment "rivers and other outflows waterway names. If evaporation or seepage are notable outflows, they may be included. Some terms may not be place names, e.g. evaporation"^^xsd:string ;
    rdfs:domain wikidata:Q104347069,
        wikidata:Q15324 ;
    rdfs:range wikidata:Q132814,
        wikidata:Q15324,
        wikidata:Q355304 .

wikidata:P2012 rdfs:label "cuisine"^^xsd:string ;
    rdfs:comment "type of food served by a restaurant or restaurant chain"^^xsd:string ;
    rdfs:range wikidata:Q1778821 ;
    rdfs:subPropertyOf wikidata:P101 .

wikidata:P2033 rdfs:label "category for pictures taken with camera"^^xsd:string ;
    rdfs:comment "Commons category for photos taken with that camera model or model line"^^xsd:string ;
    rdfs:domain wikidata:Q10929058,
        wikidata:Q20888711,
        wikidata:Q811701 .

wikidata:P205 rdfs:label "basin country"^^xsd:string ;
    rdfs:comment "country that have drainage to/from or border the body of water"^^xsd:string ;
    rdfs:domain wikidata:Q15324,
        wikidata:Q16500104,
        wikidata:Q166620 ;
    rdfs:range wikidata:Q7275 .

wikidata:P2058 rdfs:label "depositor"^^xsd:string ;
    rdfs:comment "depositor/depositaries for the treaty"^^xsd:string ;
    rdfs:domain wikidata:Q131569 ;
    rdfs:range wikidata:Q4164871,
        wikidata:Q43229 .

wikidata:P206 rdfs:label "located in or next to body of water"^^xsd:string ;
    rdfs:comment "sea, lake, river or stream"^^xsd:string ;
    rdfs:domain wikidata:Q24334893,
        wikidata:Q3895768,
        wikidata:Q618123,
        wikidata:Q66661745,
        wikidata:Q8205328 ;
    rdfs:range wikidata:Q15324,
        wikidata:Q16500104,
        wikidata:Q44782 ;
    rdfs:subPropertyOf wikidata:P276 .

wikidata:P2061 rdfs:label "aspect ratio"^^xsd:string ;
    rdfs:comment "image width to height ratio of films, photographs, and other images"^^xsd:string ;
    rdfs:range wikidata:Q1441762,
        wikidata:Q20970434 .

wikidata:P2079 rdfs:label "fabrication method"^^xsd:string ;
    rdfs:comment "method, process or technique used to grow, cook, weave, build, assemble, manufacture the item"^^xsd:string ;
    rdfs:domain wikidata:Q16686448,
        wikidata:Q22811462,
        wikidata:Q2424752,
        wikidata:Q28732711 ;
    rdfs:range wikidata:Q1914636,
        wikidata:Q3249551 ;
    rdfs:subPropertyOf wikidata:P2283 .

wikidata:P208 rdfs:label "executive body"^^xsd:string ;
    rdfs:comment "branch of government for the daily administration of the state"^^xsd:string ;
    rdfs:domain wikidata:Q15642541 ;
    rdfs:range wikidata:Q35798 .

wikidata:P2094 rdfs:label "competition class"^^xsd:string ;
    rdfs:comment "official classification by a regulating body under which the subject (events, teams, participants, or equipment) qualifies for inclusion"^^xsd:string ;
    rdfs:domain wikidata:Q1241356,
        wikidata:Q13406554,
        wikidata:Q15229207,
        wikidata:Q16334295,
        wikidata:Q16510064,
        wikidata:Q1744559,
        wikidata:Q18608583,
        wikidata:Q29048322,
        wikidata:Q42889,
        wikidata:Q4438121,
        wikidata:Q768186 ;
    rdfs:range wikidata:Q106594809,
        wikidata:Q1744559,
        wikidata:Q2312410,
        wikidata:Q31629,
        wikidata:Q4369513 .

wikidata:P21 rdfs:label "sex or gender"^^xsd:string ;
    rdfs:comment "sex or gender identity of human or animal. For human: male, female, non-binary, intersex, transgender female, transgender male, agender. For animal: male organism, female organism. Groups of same gender use subclass of (P279)"^^xsd:string ;
    rdfs:domain wikidata:Q10832,
        wikidata:Q11012,
        wikidata:Q15619164,
        wikidata:Q16521,
        wikidata:Q201662,
        wikidata:Q21070598,
        wikidata:Q215627,
        wikidata:Q216866,
        wikidata:Q24286894,
        wikidata:Q24334685,
        wikidata:Q40614,
        wikidata:Q7239,
        wikidata:Q729,
        wikidata:Q79600797,
        wikidata:Q95074 .

wikidata:P2175 rdfs:label "medical condition treated"^^xsd:string ;
    rdfs:comment "disease that this pharmaceutical drug, procedure, or therapy is used to treat"^^xsd:string ;
    rdfs:domain wikidata:Q12140,
        wikidata:Q28885102,
        wikidata:Q30612,
        wikidata:Q796194 ;
    rdfs:range wikidata:Q2057971 ;
    rdfs:subPropertyOf wikidata:P366 .

wikidata:P2176 rdfs:label "drug used for treatment"^^xsd:string ;
    rdfs:comment "drug, procedure, or therapy that can be used to treat a medical condition"^^xsd:string ;
    rdfs:domain wikidata:Q2057971 ;
    rdfs:range wikidata:Q12140 .

wikidata:P2184 rdfs:label "history of topic"^^xsd:string ;
    rdfs:comment "item about the historical development of an subject's topic, sample: \"history of Argentina\" for \"Argentina\". To list key events of the topic, use \"significant event\" (P793)"^^xsd:string ;
    rdfs:range wikidata:Q11514315,
        wikidata:Q130788,
        wikidata:Q17524420,
        wikidata:Q186117,
        wikidata:Q309 ;
    rdfs:subPropertyOf wikidata:P2579 .

wikidata:P22 rdfs:label "father"^^xsd:string ;
    rdfs:comment "male parent of the subject. For stepfather, use \"stepparent\" (P3448)"^^xsd:string ;
    rdfs:domain wikidata:Q13002315,
        wikidata:Q16979650,
        wikidata:Q178885,
        wikidata:Q21070568,
        wikidata:Q21070598,
        wikidata:Q284851,
        wikidata:Q4271324,
        wikidata:Q5,
        wikidata:Q64520857,
        wikidata:Q64643615,
        wikidata:Q729,
        wikidata:Q75855169,
        wikidata:Q95074 ;
    rdfs:range wikidata:Q13002315,
        wikidata:Q21070568,
        wikidata:Q21070598,
        wikidata:Q215627,
        wikidata:Q4271324,
        wikidata:Q729,
        wikidata:Q95074 ;
    rdfs:subPropertyOf wikidata:P8810 .

wikidata:P2286 rdfs:label "arterial supply"^^xsd:string ;
    rdfs:comment "arterial supply of an anatomical structure"^^xsd:string ;
    rdfs:range wikidata:Q9655 .

wikidata:P2291 rdfs:label "charted in"^^xsd:string ;
    rdfs:comment "chart where the element reached a position"^^xsd:string ;
    rdfs:domain wikidata:Q386724 ;
    rdfs:range wikidata:Q373899 .

wikidata:P2293 a owl:SymmetricProperty ;
    rdfs:label "genetic association"^^xsd:string ;
    rdfs:comment "general link between a disease and the causal genetic entity, if the detailed mechanism is unknown/unavailable"^^xsd:string ;
    rdfs:domain wikidata:Q12136,
        wikidata:Q7187 .

wikidata:P2341 rdfs:label "indigenous to"^^xsd:string ;
    rdfs:comment "place that a language, folk dance, cooking style, food, species or other cultural expression is found (or was originally found)"^^xsd:string ;
    rdfs:domain wikidata:Q105575966,
        wikidata:Q11460,
        wikidata:Q11639,
        wikidata:Q11921029,
        wikidata:Q1292119,
        wikidata:Q13002315,
        wikidata:Q17376908,
        wikidata:Q188451,
        wikidata:Q2095,
        wikidata:Q223393,
        wikidata:Q2239243,
        wikidata:Q24334685,
        wikidata:Q251777,
        wikidata:Q2531956,
        wikidata:Q2578402,
        wikidata:Q25810847,
        wikidata:Q28823,
        wikidata:Q3172759,
        wikidata:Q41710,
        wikidata:Q4384751,
        wikidata:Q4461766,
        wikidata:Q60733114,
        wikidata:Q736427,
        wikidata:Q7432,
        wikidata:Q771035,
        wikidata:Q7832362,
        wikidata:Q943929 ;
    rdfs:range wikidata:Q2472587,
        wikidata:Q3502482,
        wikidata:Q41710,
        wikidata:Q56061,
        wikidata:Q82794,
        wikidata:Q851990 .

wikidata:P2348 rdfs:label "time period"^^xsd:string ;
    rdfs:comment "time period (historic period or era, sports season, theatre season, legislative period etc.) in which the subject occurred"^^xsd:string .

wikidata:P2359 rdfs:label "Roman nomen gentilicium"^^xsd:string ;
    rdfs:comment "standard part of the name of a Roman, link to items about the Roman gens only"^^xsd:string ;
    rdfs:range wikidata:Q3760158 .

wikidata:P2363 rdfs:label "NMHH film rating"^^xsd:string ;
    rdfs:comment "rating of a film in the Hungarian film rating system"^^xsd:string ;
    rdfs:domain wikidata:Q11424,
        wikidata:Q1261214,
        wikidata:Q1983062 ;
    rdfs:range wikidata:Q23683425 .

wikidata:P237 rdfs:label "coat of arms"^^xsd:string ;
    rdfs:comment "subject's coat of arms"^^xsd:string ;
    rdfs:range wikidata:Q1079693,
        wikidata:Q14659,
        wikidata:Q17335294,
        wikidata:Q2532754 .

wikidata:P2378 rdfs:label "issued by"^^xsd:string ;
    rdfs:comment "organisation that issues or allocates an identifier"^^xsd:string ;
    rdfs:domain wikidata:Q19847637,
        wikidata:Q374814,
        wikidata:Q43812,
        wikidata:Q47988,
        wikidata:Q79719,
        wikidata:Q853614 ;
    rdfs:range wikidata:Q35127,
        wikidata:Q43229 .

wikidata:P2379 a owl:FunctionalProperty ;
    rdfs:label "deprecated in version"^^xsd:string ;
    rdfs:comment "software version it was deprecated in"^^xsd:string .

wikidata:P2388 rdfs:label "office held by head of the organization"^^xsd:string ;
    rdfs:comment "position of the head of this item"^^xsd:string ;
    rdfs:domain wikidata:Q43229 ;
    rdfs:range wikidata:Q4164871 .

wikidata:P2389 rdfs:label "organization directed by the office or position"^^xsd:string ;
    rdfs:comment "organization which is directed by this office"^^xsd:string ;
    rdfs:domain wikidata:Q4164871 ;
    rdfs:range wikidata:Q161837,
        wikidata:Q43229 .

wikidata:P2408 rdfs:label "set in period"^^xsd:string ;
    rdfs:comment "historical, contemporary or future period the work is set in or event featured in the story of the work"^^xsd:string ;
    rdfs:domain wikidata:Q386724 ;
    rdfs:range wikidata:Q14136353,
        wikidata:Q26907166 .

wikidata:P241 rdfs:label "military branch"^^xsd:string ;
    rdfs:comment "branch to which this military unit, award, office, or person belongs, e.g. Royal Navy"^^xsd:string ;
    rdfs:domain wikidata:Q1196123,
        wikidata:Q16334295,
        wikidata:Q16631188,
        wikidata:Q176799,
        wikidata:Q18643213,
        wikidata:Q18691599,
        wikidata:Q26401003,
        wikidata:Q2668072,
        wikidata:Q329864,
        wikidata:Q5,
        wikidata:Q56019,
        wikidata:Q62934160,
        wikidata:Q64353859,
        wikidata:Q6857706,
        wikidata:Q728,
        wikidata:Q91197994,
        wikidata:Q95074 ;
    rdfs:range wikidata:Q18011141,
        wikidata:Q35535,
        wikidata:Q4793045,
        wikidata:Q781132,
        wikidata:Q8473 ;
    rdfs:subPropertyOf wikidata:P361 .

wikidata:P2416 rdfs:label "sports discipline competed in"^^xsd:string ;
    rdfs:comment "discipline an athlete competed in within a sport"^^xsd:string ;
    rdfs:domain wikidata:Q15632617,
        wikidata:Q16334295,
        wikidata:Q5 ;
    rdfs:range wikidata:Q2312410,
        wikidata:Q31629 ;
    rdfs:subPropertyOf wikidata:P101 .

wikidata:P2417 rdfs:label "stage classification"^^xsd:string ;
    rdfs:comment "stage results and ranking of a stage race"^^xsd:string ;
    rdfs:domain wikidata:Q18131152 ;
    rdfs:subPropertyOf wikidata:P2321,
        wikidata:P710 .

wikidata:P2438 rdfs:label "narrator"^^xsd:string ;
    rdfs:comment "narrator, character or person that tells the story"^^xsd:string ;
    rdfs:domain wikidata:Q386724 .

wikidata:P248 rdfs:label "stated in"^^xsd:string ;
    rdfs:comment "to be used in the references field to refer to the information document or database in which a claim is made; for qualifiers use P805"^^xsd:string ;
    rdfs:range wikidata:Q11028,
        wikidata:Q121182,
        wikidata:Q1277575,
        wikidata:Q170584,
        wikidata:Q1789476,
        wikidata:Q2352616,
        wikidata:Q3331189,
        wikidata:Q386724,
        wikidata:Q7094076,
        wikidata:Q8513 .

wikidata:P2499 rdfs:label "league level above"^^xsd:string ;
    rdfs:comment "the league above this sports league"^^xsd:string ;
    rdfs:subPropertyOf wikidata:P3730 .

wikidata:P25 rdfs:label "mother"^^xsd:string ;
    rdfs:comment "female parent of the subject. For stepmother, use \"stepparent\" (P3448)"^^xsd:string ;
    rdfs:domain wikidata:Q13002315,
        wikidata:Q178885,
        wikidata:Q20830276,
        wikidata:Q21070568,
        wikidata:Q21070598,
        wikidata:Q284851,
        wikidata:Q4271324,
        wikidata:Q5,
        wikidata:Q64520857,
        wikidata:Q64643615,
        wikidata:Q729,
        wikidata:Q75855169,
        wikidata:Q95074 ;
    rdfs:range wikidata:Q13002315,
        wikidata:Q178885,
        wikidata:Q21070568,
        wikidata:Q21070598,
        wikidata:Q4271324,
        wikidata:Q5,
        wikidata:Q729,
        wikidata:Q95074 ;
    rdfs:subPropertyOf wikidata:P8810 .

wikidata:P2500 rdfs:label "league level below"^^xsd:string ;
    rdfs:comment "the league below this sports league"^^xsd:string ;
    rdfs:subPropertyOf wikidata:P3729 .

wikidata:P2505 rdfs:label "carries"^^xsd:string ;
    rdfs:comment "item (e.g. road, railway, canal) carried by a bridge, a tunnel or a mountain pass"^^xsd:string ;
    rdfs:domain wikidata:Q105731,
        wikidata:Q12280,
        wikidata:Q12323,
        wikidata:Q12743,
        wikidata:Q1287097,
        wikidata:Q133056,
        wikidata:Q150784,
        wikidata:Q1544071,
        wikidata:Q1777515,
        wikidata:Q1784096,
        wikidata:Q18390875,
        wikidata:Q18984099,
        wikidata:Q2860026,
        wikidata:Q44377,
        wikidata:Q55599109,
        wikidata:Q69719735,
        wikidata:Q892168,
        wikidata:Q93267 ;
    rdfs:range wikidata:Q104526,
        wikidata:Q1067164,
        wikidata:Q355304,
        wikidata:Q83620 ;
    rdfs:subPropertyOf wikidata:P361 .

wikidata:P2512 rdfs:label "series spin-off"^^xsd:string ;
    rdfs:comment "series' spin-offs"^^xsd:string ;
    rdfs:domain wikidata:Q7725310 .

wikidata:P2515 rdfs:label "costume designer"^^xsd:string ;
    rdfs:comment "person who designed the costumes for a film, television programme, etc"^^xsd:string ;
    rdfs:domain wikidata:Q11424,
        wikidata:Q15416,
        wikidata:Q21191270,
        wikidata:Q35140,
        wikidata:Q43099500,
        wikidata:Q43100730 ;
    rdfs:subPropertyOf wikidata:P3342 .

wikidata:P2517 rdfs:label "category for recipients of this award"^^xsd:string ;
    rdfs:comment "link to Wikimedia category for recipients of this award"^^xsd:string ;
    rdfs:domain wikidata:Q216353,
        wikidata:Q38033430,
        wikidata:Q618779 ;
    rdfs:range wikidata:Q4167836 ;
    rdfs:subPropertyOf wikidata:P910 .

wikidata:P2522 rdfs:label "victory"^^xsd:string ;
    rdfs:comment "competition or event won by the subject"^^xsd:string ;
    rdfs:domain wikidata:Q1231729,
        wikidata:Q12973014,
        wikidata:Q2088357,
        wikidata:Q5,
        wikidata:Q63483382,
        wikidata:Q68,
        wikidata:Q726,
        wikidata:Q7397,
        wikidata:Q838948,
        wikidata:Q847017,
        wikidata:Q95074 ;
    rdfs:range wikidata:Q106594095,
        wikidata:Q13406554,
        wikidata:Q15707532,
        wikidata:Q18608583,
        wikidata:Q3464665,
        wikidata:Q841654 ;
    rdfs:subPropertyOf wikidata:P1344 .

wikidata:P2541 rdfs:label "operating area"^^xsd:string ;
    rdfs:comment "geographic area or jurisdiction an organisation or industry operates in, serves, or has responsibility for"^^xsd:string ;
    rdfs:domain wikidata:Q1048835,
        wikidata:Q14623646,
        wikidata:Q18127,
        wikidata:Q268592,
        wikidata:Q43229,
        wikidata:Q58778,
        wikidata:Q7406919,
        wikidata:Q8148 ;
    rdfs:range wikidata:Q17334923,
        wikidata:Q82794 ;
    rdfs:subPropertyOf wikidata:P276 .

wikidata:P2545 a owl:FunctionalProperty ;
    rdfs:label "bowling style"^^xsd:string ;
    rdfs:comment "type of bowling employed by a cricketer"^^xsd:string ;
    rdfs:range wikidata:Q22911714,
        wikidata:Q7860947 .

wikidata:P2546 a owl:IrreflexiveProperty ;
    rdfs:label "sidekick of"^^xsd:string ;
    rdfs:comment "close companion of a fictional character"^^xsd:string ;
    rdfs:domain wikidata:Q95074 ;
    rdfs:range wikidata:Q95074 ;
    rdfs:subPropertyOf wikidata:P3342 .

wikidata:P2554 rdfs:label "production designer"^^xsd:string ;
    rdfs:comment "production designer(s) of this motion picture, play, video game or similar"^^xsd:string ;
    rdfs:domain wikidata:Q11424,
        wikidata:Q15416 ;
    rdfs:subPropertyOf wikidata:P3092,
        wikidata:P3174 .

wikidata:P2563 rdfs:label "superhuman feature or ability"^^xsd:string ;
    rdfs:comment "superhuman, supernatural, or paranormal abilities that the fictional subject exhibits"^^xsd:string ;
    rdfs:domain wikidata:Q17624054,
        wikidata:Q178885,
        wikidata:Q188784,
        wikidata:Q24577840,
        wikidata:Q2590445,
        wikidata:Q47543030,
        wikidata:Q6498903,
        wikidata:Q95074 ;
    rdfs:range wikidata:Q1047698,
        wikidata:Q1347367 ;
    rdfs:subPropertyOf wikidata:P2283 .

wikidata:P2567 rdfs:label "amended by"^^xsd:string ;
    rdfs:comment "document is amended by specified other document"^^xsd:string ;
    rdfs:domain wikidata:Q1151067,
        wikidata:Q1269627,
        wikidata:Q131569,
        wikidata:Q1348305,
        wikidata:Q212971,
        wikidata:Q2795484,
        wikidata:Q352858,
        wikidata:Q49371,
        wikidata:Q820655 ;
    rdfs:range wikidata:Q1269627,
        wikidata:Q1348305,
        wikidata:Q212971,
        wikidata:Q352858 .

wikidata:P2578 rdfs:label "studies"^^xsd:string ;
    rdfs:comment "subject item is the academic field studying the object item of this property"^^xsd:string ;
    rdfs:domain wikidata:Q11862829,
        wikidata:Q34178,
        wikidata:Q48282 .

wikidata:P2596 rdfs:label "culture"^^xsd:string ;
    rdfs:comment "human culture or people (or several cultures) associated with this item"^^xsd:string ;
    rdfs:range wikidata:Q11042,
        wikidata:Q2472587,
        wikidata:Q41710,
        wikidata:Q465299,
        wikidata:Q6256,
        wikidata:Q7275,
        wikidata:Q8432 ;
    rdfs:subPropertyOf wikidata:P361 .

wikidata:P26 a owl:SymmetricProperty ;
    rdfs:label "spouse"^^xsd:string ;
    rdfs:comment "the subject has the object as their spouse (husband, wife, partner, etc.). Use \"unmarried partner\" (P451) for non-married companions"^^xsd:string ;
    rdfs:domain wikidata:Q13002315,
        wikidata:Q21070568,
        wikidata:Q215627,
        wikidata:Q4271324,
        wikidata:Q5,
        wikidata:Q95074 ;
    rdfs:subPropertyOf wikidata:P1038,
        wikidata:P3342 .

wikidata:P2614 rdfs:label "World Heritage criteria"^^xsd:string ;
    rdfs:comment "selection criteria for UNESCO's cultural and natural 'World Heritage' designation since 2005"^^xsd:string .

wikidata:P2629 rdfs:label "BBFC rating"^^xsd:string ;
    rdfs:comment "British media content rating (add BBFC reference with qualifier \"P2676\")"^^xsd:string ;
    rdfs:domain wikidata:Q11424,
        wikidata:Q15416,
        wikidata:Q21191270,
        wikidata:Q7889 ;
    rdfs:range wikidata:Q23790218 .

wikidata:P263 rdfs:label "official residence"^^xsd:string ;
    rdfs:comment "the residence at which heads of government and other senior figures officially reside"^^xsd:string ;
    rdfs:range wikidata:Q41176 ;
    rdfs:subPropertyOf wikidata:P551 .

wikidata:P2633 a owl:FunctionalProperty ;
    rdfs:label "geography of topic"^^xsd:string ;
    rdfs:comment "item that deals with the geography of the subject. Sample: \"Rio de Janeiro\" uses this property with value \"geography of Rio de Janeiro\" (Q10288853). For the location of a subject, use \"location\" (P276)."^^xsd:string .

wikidata:P2637 a owl:FunctionalProperty ;
    rdfs:label "RARS rating"^^xsd:string ;
    rdfs:comment "rating in the russian media content rating system"^^xsd:string ;
    rdfs:domain wikidata:Q2431196,
        wikidata:Q7889 .

wikidata:P264 rdfs:label "record label"^^xsd:string ;
    rdfs:comment "brand and trademark associated with the marketing of subject music recordings and music videos"^^xsd:string ;
    rdfs:domain wikidata:Q106833,
        wikidata:Q11664239,
        wikidata:Q193977,
        wikidata:Q2031291,
        wikidata:Q2088357,
        wikidata:Q215380,
        wikidata:Q2188189,
        wikidata:Q234870,
        wikidata:Q3331189,
        wikidata:Q5,
        wikidata:Q7366,
        wikidata:Q7725310 ;
    rdfs:range wikidata:Q1137109,
        wikidata:Q18127,
        wikidata:Q210167 .

wikidata:P2650 rdfs:label "interested in"^^xsd:string ;
    rdfs:comment "item of special or vested interest to this person or organisation"^^xsd:string ;
    rdfs:domain wikidata:Q170584,
        wikidata:Q43229,
        wikidata:Q49773,
        wikidata:Q5,
        wikidata:Q7406919,
        wikidata:Q95074 .

wikidata:P2652 a owl:SymmetricProperty ;
    rdfs:label "partnership with"^^xsd:string ;
    rdfs:comment "commercial partnership between this organization and another organization or institution"^^xsd:string ;
    rdfs:domain wikidata:Q43229,
        wikidata:Q56061 ;
    rdfs:range wikidata:Q43229,
        wikidata:Q56061 .

wikidata:P2673 rdfs:label "next crossing upstream"^^xsd:string ;
    rdfs:comment "next crossing of this river, canal, etc. upstream of this subject"^^xsd:string ;
    rdfs:domain wikidata:Q12280,
        wikidata:Q12323,
        wikidata:Q18984099,
        wikidata:Q44377 ;
    rdfs:range wikidata:Q12280,
        wikidata:Q12323,
        wikidata:Q44377 .

wikidata:P2674 rdfs:label "next crossing downstream"^^xsd:string ;
    rdfs:comment "next crossing of this river, canal, etc. downstream of this subject"^^xsd:string .

wikidata:P2679 rdfs:label "author of foreword"^^xsd:string ;
    rdfs:comment "person who wrote the preface, foreword, or introduction of the book but who isn't an author of the rest of the book"^^xsd:string ;
    rdfs:domain wikidata:Q3331189,
        wikidata:Q47461344,
        wikidata:Q49848 ;
    rdfs:range wikidata:Q5,
        wikidata:Q95074 .

wikidata:P2684 rdfs:label "Kijkwijzer rating"^^xsd:string ;
    rdfs:comment "Dutch media content rating system"^^xsd:string ;
    rdfs:domain wikidata:Q11424,
        wikidata:Q15416,
        wikidata:Q21191270 ;
    rdfs:range wikidata:Q23649978 .

wikidata:P2695 rdfs:label "type locality (geology)"^^xsd:string ;
    rdfs:comment "the locality where a particular rock type, stratigraphic unit or mineral species is defined from (can coincide but not the same as p189)"^^xsd:string .

wikidata:P2701 rdfs:label "file format"^^xsd:string ;
    rdfs:comment "file format, compression type, or ontology used in a file"^^xsd:string ;
    rdfs:range wikidata:Q235557 .

wikidata:P272 rdfs:label "production company"^^xsd:string ;
    rdfs:comment "company that produced this film, audio or performing arts work"^^xsd:string ;
    rdfs:domain wikidata:Q386724 ;
    rdfs:range wikidata:Q11396960,
        wikidata:Q43229 .

wikidata:P2743 a owl:SymmetricProperty ;
    rdfs:label "this zoological name is coordinate with"^^xsd:string ;
    rdfs:comment "links coordinate zoological names"^^xsd:string ;
    rdfs:domain wikidata:Q16521 ;
    rdfs:subPropertyOf wikidata:P1889 .

wikidata:P2747 rdfs:label "Filmiroda rating"^^xsd:string ;
    rdfs:comment "rating of a film in the former (2004–2011) Hungarian film rating system"^^xsd:string ;
    rdfs:domain wikidata:Q11424,
        wikidata:Q1261214,
        wikidata:Q3464665,
        wikidata:Q5398426 .

wikidata:P275 rdfs:label "copyright license"^^xsd:string ;
    rdfs:comment "license under which this copyrighted work is released"^^xsd:string ;
    rdfs:domain wikidata:Q18593264,
        wikidata:Q2668072,
        wikidata:Q3052382,
        wikidata:Q386724,
        wikidata:Q42848,
        wikidata:Q8513 ;
    rdfs:range wikidata:Q79719 .

wikidata:P2758 rdfs:label "CNC film rating (France)"^^xsd:string ;
    rdfs:comment "category assigned to a film by the Board of Film Classification (CNC) which what audiences may view it in France"^^xsd:string ;
    rdfs:domain wikidata:Q11424 .

wikidata:P277 rdfs:label "programming language"^^xsd:string ;
    rdfs:comment "the programming language(s) in which the software is developed"^^xsd:string ;
    rdfs:range wikidata:Q165194,
        wikidata:Q188860,
        wikidata:Q9143 .

wikidata:P2825 rdfs:label "via"^^xsd:string ;
    rdfs:comment "intermediate point on a journey - stopover location, waystation or routing point"^^xsd:string ;
    rdfs:range wikidata:Q2221906 ;
    rdfs:subPropertyOf wikidata:P276 .

wikidata:P2827 rdfs:label "flower color"^^xsd:string ;
    rdfs:comment "colour of flowers of a plant species, hybrid or cultivar"^^xsd:string ;
    rdfs:domain wikidata:Q4886,
        wikidata:Q756 ;
    rdfs:range wikidata:Q1075 ;
    rdfs:subPropertyOf wikidata:P462 .

wikidata:P2846 rdfs:label "wheelchair accessibility"^^xsd:string ;
    rdfs:comment "describes wheelchair accessibility of location or event"^^xsd:string ;
    rdfs:domain wikidata:Q1030034,
        wikidata:Q1656682,
        wikidata:Q2221906,
        wikidata:Q548662,
        wikidata:Q811979 .

wikidata:P2848 rdfs:label "Wi-Fi access"^^xsd:string ;
    rdfs:comment "internet access availability through Wi-Fi"^^xsd:string ;
    rdfs:domain wikidata:Q1248784,
        wikidata:Q2221906,
        wikidata:Q41176,
        wikidata:Q43229 .

wikidata:P2851 rdfs:label "payment types accepted"^^xsd:string ;
    rdfs:comment "types of payment accepted by a venue"^^xsd:string ;
    rdfs:domain wikidata:Q1656682,
        wikidata:Q2221906,
        wikidata:Q43229 ;
    rdfs:range wikidata:Q190122,
        wikidata:Q689044,
        wikidata:Q986008 .

wikidata:P2852 rdfs:label "emergency phone number"^^xsd:string ;
    rdfs:comment "telephone number to contact the emergency services"^^xsd:string ;
    rdfs:domain wikidata:Q56061,
        wikidata:Q6256 ;
    rdfs:range wikidata:Q694554 .

wikidata:P2853 rdfs:label "electrical plug type"^^xsd:string ;
    rdfs:comment "standard plug type for mains electricity in a country"^^xsd:string ;
    rdfs:domain wikidata:Q56061,
        wikidata:Q6256 ;
    rdfs:range wikidata:Q215292 .

wikidata:P286 rdfs:label "head coach"^^xsd:string ;
    rdfs:comment "on-field manager or head coach of a sports club (not to be confused with a general manager P505, which is not a coaching position) or person"^^xsd:string ;
    rdfs:domain wikidata:Q12973014,
        wikidata:Q1539532,
        wikidata:Q2485448,
        wikidata:Q5,
        wikidata:Q847017 ;
    rdfs:range wikidata:Q5 .

wikidata:P2860 rdfs:label "cites work"^^xsd:string ;
    rdfs:comment "citation from one creative work to another"^^xsd:string ;
    rdfs:subPropertyOf wikidata:P8371 .

wikidata:P2868 rdfs:label "subject has role"^^xsd:string ;
    rdfs:comment "role/generic identity of the item (\"subject\"), also in the context of a statement. For the role of the value of the statement (\"object\"), use P3831 (\"object has role\"). For acting roles, use P453 (\"character role\"). For persons, use P39."^^xsd:string .

wikidata:P2872 rdfs:label "visitor centre"^^xsd:string ;
    rdfs:comment "official tourist office of this destination"^^xsd:string ;
    rdfs:domain wikidata:Q15642541,
        wikidata:Q3895768 ;
    rdfs:range wikidata:Q3689421 .

wikidata:P2881 rdfs:label "promoted"^^xsd:string ;
    rdfs:comment "competitor or team relegated during competition"^^xsd:string ;
    rdfs:domain wikidata:Q27020041 ;
    rdfs:range wikidata:Q4438121,
        wikidata:Q5 .

wikidata:P2882 rdfs:label "relegated"^^xsd:string ;
    rdfs:comment "competitor or team relegated during competition"^^xsd:string ;
    rdfs:domain wikidata:Q27020041 ;
    rdfs:range wikidata:Q4438121,
        wikidata:Q5 .

wikidata:P2894 rdfs:label "day of week"^^xsd:string ;
    rdfs:comment "day of the week on which this item occurs, applies to or is valid"^^xsd:string .

wikidata:P291 rdfs:label "place of publication"^^xsd:string ;
    rdfs:comment "geographical place of publication of the edition (use 1st edition when referring to works)"^^xsd:string ;
    rdfs:domain wikidata:Q11424,
        wikidata:Q17489659,
        wikidata:Q3331189,
        wikidata:Q3523102,
        wikidata:Q386724 ;
    rdfs:range wikidata:Q1254874,
        wikidata:Q1301371,
        wikidata:Q1331793,
        wikidata:Q14350,
        wikidata:Q1616075,
        wikidata:Q1751626,
        wikidata:Q1802587,
        wikidata:Q220505,
        wikidata:Q2221906,
        wikidata:Q2385804,
        wikidata:Q27787439,
        wikidata:Q57305,
        wikidata:Q746611,
        wikidata:Q82794,
        wikidata:Q841645 ;
    rdfs:subPropertyOf wikidata:P7153 .

wikidata:P2922 rdfs:label "month of the year"^^xsd:string ;
    rdfs:comment "month of the year during which this item occurs, applies to or is valid in"^^xsd:string ;
    rdfs:range wikidata:Q5151 ;
    rdfs:subPropertyOf wikidata:P361 .

wikidata:P2925 rdfs:label "domain of saint or deity"^^xsd:string ;
    rdfs:comment "domain(s) which this saint or deity controls or protects"^^xsd:string ;
    rdfs:domain wikidata:Q1509831,
        wikidata:Q17624054,
        wikidata:Q178885,
        wikidata:Q21070568,
        wikidata:Q4271324,
        wikidata:Q5 .

wikidata:P2937 rdfs:label "parliamentary term"^^xsd:string ;
    rdfs:comment "term of a parliament or any deliberative assembly"^^xsd:string ;
    rdfs:domain wikidata:Q5 ;
    rdfs:range wikidata:Q15238777,
        wikidata:Q1812889 .

wikidata:P2959 a owl:SymmetricProperty ;
    rdfs:label "permanent duplicated item"^^xsd:string ;
    rdfs:comment "this item duplicates another item and the two can't be merged, as one Wikimedia project includes two pages, e. g. in different scripts or languages (applies to some wiki, e.g.: cdowiki, gomwiki). Use \"duplicate item\" for other wikis."^^xsd:string .

wikidata:P2962 rdfs:label "title of chess person"^^xsd:string ;
    rdfs:comment "title awarded by a chess federation to a person"^^xsd:string ;
    rdfs:range wikidata:Q5093327 .

wikidata:P2989 rdfs:label "has grammatical case"^^xsd:string ;
    rdfs:comment "case used in this language"^^xsd:string ;
    rdfs:domain wikidata:Q17376908 ;
    rdfs:range wikidata:Q128234 ;
    rdfs:subPropertyOf wikidata:P527 .

wikidata:P2992 rdfs:label "software quality assurance"^^xsd:string ;
    rdfs:comment "quality assurance process in place for a particular software"^^xsd:string ;
    rdfs:domain wikidata:Q132364,
        wikidata:Q2755432,
        wikidata:Q7397 ;
    rdfs:range wikidata:Q836575 .

wikidata:P30 rdfs:label "continent"^^xsd:string ;
    rdfs:comment "continent of which the subject is a part"^^xsd:string ;
    rdfs:domain wikidata:Q19958368,
        wikidata:Q27096213,
        wikidata:Q3895768,
        wikidata:Q66374263 ;
    rdfs:range wikidata:Q17199338,
        wikidata:Q5107,
        wikidata:Q55833,
        wikidata:Q855697 ;
    rdfs:subPropertyOf wikidata:P706 .

wikidata:P301 rdfs:label "category's main topic"^^xsd:string ;
    rdfs:comment "primary topic of the subject Wikimedia category"^^xsd:string ;
    rdfs:domain wikidata:Q4167836 .

wikidata:P3015 rdfs:label "backup or reserve team or crew"^^xsd:string ;
    rdfs:comment "team or crew that is kept ready to act as reserve"^^xsd:string ;
    rdfs:range wikidata:Q16334295,
        wikidata:Q5 .

wikidata:P3018 rdfs:label "located in protected area"^^xsd:string ;
    rdfs:comment "protected area where a place or geographical feature is physically located"^^xsd:string ;
    rdfs:domain wikidata:Q2221906,
        wikidata:Q618123 ;
    rdfs:range wikidata:Q473972,
        wikidata:Q72082844,
        wikidata:Q9259 ;
    rdfs:subPropertyOf wikidata:P131 .

wikidata:P3025 rdfs:label "open days"^^xsd:string ;
    rdfs:comment "days in the week subject item is open within the opening season"^^xsd:string ;
    rdfs:range wikidata:Q1445650,
        wikidata:Q14795564,
        wikidata:Q41825,
        wikidata:Q99731370 .

wikidata:P3032 a owl:SymmetricProperty ;
    rdfs:label "adjacent building"^^xsd:string ;
    rdfs:comment "building adjacent to the item"^^xsd:string ;
    rdfs:domain wikidata:Q41176 .

wikidata:P306 rdfs:label "operating system"^^xsd:string ;
    rdfs:comment "operating system (OS) on which a software works or the OS installed on hardware"^^xsd:string ;
    rdfs:domain wikidata:Q1183543,
        wikidata:Q16070115,
        wikidata:Q17451,
        wikidata:Q7397,
        wikidata:Q7889,
        wikidata:Q9143 ;
    rdfs:range wikidata:Q9135 .

wikidata:P3085 rdfs:label "qualifies for event"^^xsd:string ;
    rdfs:comment "this event qualifies for that event"^^xsd:string ;
    rdfs:domain wikidata:Q27020041,
        wikidata:Q34542757,
        wikidata:Q623109,
        wikidata:Q841654 ;
    rdfs:range wikidata:Q27020041,
        wikidata:Q841654 .

wikidata:P3091 rdfs:label "mount"^^xsd:string ;
    rdfs:comment "creature ridden by the subject, for instance a horse"^^xsd:string ;
    rdfs:domain wikidata:Q21070598,
        wikidata:Q5,
        wikidata:Q95074 .

wikidata:P3095 rdfs:label "practiced by"^^xsd:string ;
    rdfs:comment "type of agents that study this subject or work in this profession"^^xsd:string .

wikidata:P3096 rdfs:label "KML file"^^xsd:string ;
    rdfs:comment "item with sitelinks to wikimedia page containing text of a relevant KML file"^^xsd:string ;
    rdfs:domain wikidata:Q1067164,
        wikidata:Q1322323,
        wikidata:Q13406463,
        wikidata:Q18325841,
        wikidata:Q2221906,
        wikidata:Q22667,
        wikidata:Q4167410,
        wikidata:Q618123,
        wikidata:Q83620 ;
    rdfs:range wikidata:Q26267864 .

wikidata:P3150 rdfs:label "birthday"^^xsd:string ;
    rdfs:comment "item for day and month on which the subject was born. Used when full \"date of birth\" (P569) isn't known."^^xsd:string ;
    rdfs:domain wikidata:Q5,
        wikidata:Q95074 ;
    rdfs:range wikidata:Q14795564,
        wikidata:Q47018901 .

wikidata:P3173 rdfs:label "offers view on"^^xsd:string ;
    rdfs:comment "things, places another place offers views on"^^xsd:string ;
    rdfs:range wikidata:Q618123 .

wikidata:P3195 rdfs:label "league points system"^^xsd:string ;
    rdfs:comment "point system of an e.g. sports league"^^xsd:string ;
    rdfs:range wikidata:Q58778 .

wikidata:P3216 rdfs:label "ClassInd rating"^^xsd:string ;
    rdfs:comment "rating of an audiovisual work, video game or RPG in the Brazilian Advisory Rating System (ClassInd)"^^xsd:string ;
    rdfs:domain wikidata:Q11424,
        wikidata:Q15416,
        wikidata:Q160738,
        wikidata:Q21191270,
        wikidata:Q7889 ;
    rdfs:range wikidata:Q26678730 .

wikidata:P3261 rdfs:label "anatomical branch of"^^xsd:string ;
    rdfs:comment "main stem of this blood vessel, lymphatic vessel or nerve"^^xsd:string ;
    rdfs:range wikidata:Q4936952 ;
    rdfs:subPropertyOf wikidata:P2789 .

wikidata:P3262 rdfs:label "has anatomical branch"^^xsd:string ;
    rdfs:comment "branches of this blood vessel, lymphatic vessel or nerve"^^xsd:string ;
    rdfs:range wikidata:Q4936952 ;
    rdfs:subPropertyOf wikidata:P2789 .

wikidata:P3275 rdfs:label "storyboard artist"^^xsd:string ;
    rdfs:comment "person credited as the storyboard artist of this work"^^xsd:string ;
    rdfs:subPropertyOf wikidata:P3092 .

wikidata:P3279 rdfs:label "statistical leader"^^xsd:string ;
    rdfs:comment "leader of a sports tournament in one of statistical qualities (points, assists, rebounds etc.). Don't use for overall winner. Use a qualifier to link to the item about the quality."^^xsd:string .

wikidata:P3300 rdfs:label "musical conductor"^^xsd:string ;
    rdfs:comment "the person who directs a musical group, orchestra or chorus"^^xsd:string ;
    rdfs:domain wikidata:Q11424,
        wikidata:Q1366112,
        wikidata:Q2031291,
        wikidata:Q20819922,
        wikidata:Q2088357,
        wikidata:Q276,
        wikidata:Q59163902,
        wikidata:Q6942562,
        wikidata:Q7302866,
        wikidata:Q7777570 ;
    rdfs:range wikidata:Q5 ;
    rdfs:subPropertyOf wikidata:P3342 .

wikidata:P3301 rdfs:label "broadcast by"^^xsd:string ;
    rdfs:comment "channel, network, website or service that broadcast this item over radio, TV or the Internet"^^xsd:string .

wikidata:P3306 rdfs:label "ICAA rating"^^xsd:string ;
    rdfs:comment "rating in the Spanish motion picture content rating system"^^xsd:string ;
    rdfs:domain wikidata:Q11424 ;
    rdfs:range wikidata:Q27253938 .

wikidata:P3320 rdfs:label "board member"^^xsd:string ;
    rdfs:comment "member(s) of the board for the organization"^^xsd:string ;
    rdfs:domain wikidata:Q43229 ;
    rdfs:range wikidata:Q43229,
        wikidata:Q5 .

wikidata:P3354 rdfs:label "positive therapeutic predictor"^^xsd:string ;
    rdfs:comment "the presence of the genetic variant helps to predict response to a treatment"^^xsd:string .

wikidata:P3355 rdfs:label "negative therapeutic predictor"^^xsd:string ;
    rdfs:comment "the presence of the genetic variant helps to predict no response or resistance to a treatment"^^xsd:string .

wikidata:P3373 a owl:SymmetricProperty ;
    rdfs:label "sibling"^^xsd:string ;
    rdfs:comment "the subject has the object as their sibling (brother, sister, etc.). Use \"relative\" (P1038) for siblings-in-law (brother-in-law, sister-in-law, etc.) and step-siblings (step-brothers, step-sisters, etc.)"^^xsd:string ;
    rdfs:domain wikidata:Q144,
        wikidata:Q16521,
        wikidata:Q178885,
        wikidata:Q19537,
        wikidata:Q21070568,
        wikidata:Q21070598,
        wikidata:Q26843,
        wikidata:Q301676,
        wikidata:Q36341,
        wikidata:Q4271324,
        wikidata:Q5,
        wikidata:Q57812611,
        wikidata:Q64520857,
        wikidata:Q64643615,
        wikidata:Q726,
        wikidata:Q75855169,
        wikidata:Q839769,
        wikidata:Q876500,
        wikidata:Q95074 ;
    rdfs:range wikidata:Q144,
        wikidata:Q178885,
        wikidata:Q21070598,
        wikidata:Q215627,
        wikidata:Q26401003,
        wikidata:Q26843,
        wikidata:Q301676,
        wikidata:Q36341,
        wikidata:Q4271324,
        wikidata:Q57812611,
        wikidata:Q726,
        wikidata:Q839769,
        wikidata:Q876500,
        wikidata:Q95074 ;
    rdfs:subPropertyOf wikidata:P1038 .

wikidata:P3402 rdfs:label "CNC title rating (Romania)"^^xsd:string ;
    rdfs:comment "rating of a movie in the Romanian content rating system"^^xsd:string ;
    rdfs:domain wikidata:Q11424,
        wikidata:Q1983062 .

wikidata:P3428 a owl:FunctionalProperty ;
    rdfs:label "INCAA film rating"^^xsd:string ;
    rdfs:comment "rating of a movie in the Argentinian content rating system"^^xsd:string ;
    rdfs:domain wikidata:Q11424 .

wikidata:P3433 a owl:FunctionalProperty ;
    rdfs:label "biological variant of"^^xsd:string ;
    rdfs:comment "a variant of a physical biological entity (e.g., gene sequence, protein sequence, epigenetic mark)"^^xsd:string ;
    rdfs:domain wikidata:Q15304597 .

wikidata:P3438 rdfs:label "vehicle normally used"^^xsd:string ;
    rdfs:comment "vehicle the subject normally uses"^^xsd:string ;
    rdfs:range wikidata:Q20871196,
        wikidata:Q29048322,
        wikidata:Q42889,
        wikidata:Q811704 ;
    rdfs:subPropertyOf wikidata:P121 .

wikidata:P344 rdfs:label "director of photography"^^xsd:string ;
    rdfs:comment "person responsible for the framing, lighting, and filtration of the subject work"^^xsd:string ;
    rdfs:domain wikidata:Q11424,
        wikidata:Q15416,
        wikidata:Q21191270,
        wikidata:Q24856 ;
    rdfs:range wikidata:Q15632617,
        wikidata:Q5 ;
    rdfs:subPropertyOf wikidata:P3092 .

wikidata:P3448 a owl:AsymmetricProperty,
        owl:IrreflexiveProperty ;
    rdfs:label "stepparent"^^xsd:string ;
    rdfs:comment "subject has the object as their stepparent"^^xsd:string ;
    rdfs:domain wikidata:Q21070598,
        wikidata:Q5,
        wikidata:Q95074 ;
    rdfs:range wikidata:Q21070598,
        wikidata:Q5,
        wikidata:Q95074 ;
    rdfs:subPropertyOf wikidata:P1038 .

wikidata:P3450 rdfs:label "sports season of league or competition"^^xsd:string ;
    rdfs:comment "property that shows the competition of which the item is a season. Use P5138 for \"season of club or team\"."^^xsd:string ;
    rdfs:domain wikidata:Q13406554,
        wikidata:Q27020041,
        wikidata:Q27968055 ;
    rdfs:subPropertyOf wikidata:P361 .

wikidata:P3489 rdfs:label "pregnancy category"^^xsd:string ;
    rdfs:comment "official categorisation of safety of medicine in pregnancy"^^xsd:string ;
    rdfs:domain wikidata:Q108149,
        wikidata:Q11173,
        wikidata:Q12140,
        wikidata:Q17339814 .

wikidata:P3494 rdfs:label "points classification"^^xsd:string ;
    rdfs:comment "classement établi en fonction de points marqués par des coureurs"^^xsd:string ;
    rdfs:domain wikidata:Q13406554 .

wikidata:P3496 rdfs:label "teams classification by points"^^xsd:string ;
    rdfs:comment "teams classification by points"^^xsd:string ;
    rdfs:domain wikidata:Q13406554 .

wikidata:P3497 rdfs:label "teams classification by time"^^xsd:string ;
    rdfs:comment "teams classification by time"^^xsd:string ;
    rdfs:domain wikidata:Q13406554 .

wikidata:P35 rdfs:label "head of state"^^xsd:string ;
    rdfs:comment "official with the highest formal authority in a country/state"^^xsd:string ;
    rdfs:domain wikidata:Q1145276,
        wikidata:Q3024240,
        wikidata:Q7275 ;
    rdfs:range wikidata:Q22950320,
        wikidata:Q5,
        wikidata:Q95074 ;
    rdfs:subPropertyOf wikidata:P488 .

wikidata:P355 a owl:AsymmetricProperty,
        owl:IrreflexiveProperty ;
    rdfs:label "subsidiary"^^xsd:string ;
    rdfs:comment "subsidiary of a company or organization; generally a fully owned separate corporation. Compare with \"business division\" (P199). Opposite of parent organization (P749)."^^xsd:string ;
    rdfs:domain wikidata:Q14623646,
        wikidata:Q170584,
        wikidata:Q43229 ;
    rdfs:range wikidata:Q14623646,
        wikidata:Q170584,
        wikidata:Q43229 ;
    rdfs:subPropertyOf wikidata:P1830 .

wikidata:P3592 rdfs:label "Saros cycle of eclipse"^^xsd:string ;
    rdfs:comment "گرہن کے لئے ساروس کی مدت کا تعین"^^xsd:string ;
    rdfs:domain wikidata:Q3887,
        wikidata:Q44235 ;
    rdfs:range wikidata:Q220397 .

wikidata:P36 rdfs:label "capital"^^xsd:string ;
    rdfs:comment "seat of government of a country, province, state or other type of administrative territorial entity"^^xsd:string ;
    rdfs:domain wikidata:Q1145276,
        wikidata:Q1414991,
        wikidata:Q23442,
        wikidata:Q2775969,
        wikidata:Q3327870,
        wikidata:Q486972,
        wikidata:Q56061,
        wikidata:Q82794 ;
    rdfs:range wikidata:Q1048835,
        wikidata:Q1964689,
        wikidata:Q486972,
        wikidata:Q56061 .

wikidata:P360 rdfs:label "is a list of"^^xsd:string ;
    rdfs:comment "common element between all listed items"^^xsd:string ;
    rdfs:domain wikidata:Q12139612 ;
    rdfs:subPropertyOf wikidata:P2670 .

wikidata:P3650 a owl:FunctionalProperty ;
    rdfs:label "JMK film rating"^^xsd:string ;
    rdfs:comment "rating of a film in the Austrian film rating system"^^xsd:string ;
    rdfs:domain wikidata:Q11424 .

wikidata:P369 rdfs:label "Sandbox-Item"^^xsd:string ;
    rdfs:comment "sandbox property for value of type \"Item\""^^xsd:string .

wikidata:P37 rdfs:label "official language"^^xsd:string ;
    rdfs:comment "language designated as official by this item"^^xsd:string ;
    rdfs:domain wikidata:Q1145276,
        wikidata:Q14623646,
        wikidata:Q15831598,
        wikidata:Q43229,
        wikidata:Q56061 ;
    rdfs:range wikidata:Q17376908 ;
    rdfs:subPropertyOf wikidata:P2936 .

wikidata:P3716 rdfs:label "social classification"^^xsd:string ;
    rdfs:comment "social class as recognized in traditional or state law"^^xsd:string ;
    rdfs:domain wikidata:Q13002315,
        wikidata:Q1642895,
        wikidata:Q21070598,
        wikidata:Q4271324,
        wikidata:Q5,
        wikidata:Q75855169,
        wikidata:Q8436,
        wikidata:Q95074 ;
    rdfs:range wikidata:Q187588,
        wikidata:Q2628882 .

wikidata:P375 rdfs:label "space launch vehicle"^^xsd:string ;
    rdfs:comment "type of rocket or other vehicle for launching subject payload into outer space"^^xsd:string ;
    rdfs:domain wikidata:Q21211206,
        wikidata:Q3099911,
        wikidata:Q40218,
        wikidata:Q5916 ;
    rdfs:range wikidata:Q697175 .

wikidata:P376 rdfs:label "located on astronomical body"^^xsd:string ;
    rdfs:comment "astronomical body on which features or places are situated"^^xsd:string ;
    rdfs:domain wikidata:Q220397,
        wikidata:Q2221906,
        wikidata:Q3895768,
        wikidata:Q47495022,
        wikidata:Q618123,
        wikidata:Q6999,
        wikidata:Q82794 ;
    rdfs:range wikidata:Q15831598,
        wikidata:Q3132741,
        wikidata:Q523 .

wikidata:P3764 rdfs:label "pole position"^^xsd:string ;
    rdfs:comment "person, who starts race at first row (leader in the starting grid)"^^xsd:string ;
    rdfs:domain wikidata:Q22938576 ;
    rdfs:range wikidata:Q5 ;
    rdfs:subPropertyOf wikidata:P3342 .

wikidata:P3777 rdfs:label "antisense inhibitor of"^^xsd:string ;
    rdfs:comment "protein/gene for which this chemical (e.g. a miRNA/siRNA) acts as an antisense inhibitor"^^xsd:string .

wikidata:P3780 rdfs:label "active ingredient in"^^xsd:string ;
    rdfs:comment "is part of and forms biologically active component. Inverse of \"has active ingredient\""^^xsd:string ;
    rdfs:subPropertyOf wikidata:P361 .

wikidata:P3781 rdfs:label "has active ingredient"^^xsd:string ;
    rdfs:comment "has part biologically active component. Inverse of \"active ingredient in\""^^xsd:string ;
    rdfs:subPropertyOf wikidata:P527 .

wikidata:P38 rdfs:label "currency"^^xsd:string ;
    rdfs:comment "currency used by item"^^xsd:string ;
    rdfs:domain wikidata:Q1145276,
        wikidata:Q15642541 ;
    rdfs:range wikidata:Q3622170,
        wikidata:Q8142 .

wikidata:P3818 a owl:FunctionalProperty ;
    rdfs:label "KMRB film rating"^^xsd:string ;
    rdfs:comment "rating of a film in the South Korean film/video rating system"^^xsd:string ;
    rdfs:domain wikidata:Q11424 .

wikidata:P3822 rdfs:label "rules for classification"^^xsd:string ;
    rdfs:comment "the rules for classification of a sports league"^^xsd:string .

wikidata:P3834 rdfs:label "RTC film rating"^^xsd:string ;
    rdfs:comment "rating of a film in the Mexican film classification system"^^xsd:string ;
    rdfs:domain wikidata:Q11424 .

wikidata:P3858 rdfs:label "route diagram"^^xsd:string ;
    rdfs:comment "Wikimedia route diagram template"^^xsd:string ;
    rdfs:range wikidata:Q11266439,
        wikidata:Q17146139 ;
    rdfs:subPropertyOf wikidata:P1424 .

wikidata:P3876 rdfs:label "category for alumni of educational institution"^^xsd:string ;
    rdfs:comment "category containing people who studied at this institution"^^xsd:string ;
    rdfs:domain wikidata:Q5341295 ;
    rdfs:range wikidata:Q4167836 ;
    rdfs:subPropertyOf wikidata:P910 .

wikidata:P3919 rdfs:label "contributed to creative work"^^xsd:string ;
    rdfs:comment "person is cited as contributing to some creative or published work or series (qualify with \"subject has role\", P2868)"^^xsd:string ;
    rdfs:domain wikidata:Q5 ;
    rdfs:range wikidata:Q12772819,
        wikidata:Q17537576,
        wikidata:Q2031291,
        wikidata:Q2352616,
        wikidata:Q732577,
        wikidata:Q7725310 .

wikidata:P397 rdfs:label "parent astronomical body"^^xsd:string ;
    rdfs:comment "major astronomical body the item belongs to"^^xsd:string ;
    rdfs:domain wikidata:Q15831598,
        wikidata:Q40218,
        wikidata:Q6999 ;
    rdfs:range wikidata:Q15831598,
        wikidata:Q17444909,
        wikidata:Q6999 .

wikidata:P3975 rdfs:label "secretary general"^^xsd:string ;
    rdfs:comment "leader of a political or international organization, sometimes below the chairperson (P488)"^^xsd:string ;
    rdfs:domain wikidata:Q43229 ;
    rdfs:range wikidata:Q5,
        wikidata:Q95074 ;
    rdfs:subPropertyOf wikidata:P3342 .

wikidata:P398 rdfs:label "child astronomical body"^^xsd:string ;
    rdfs:comment "minor body that belongs to the item"^^xsd:string ;
    rdfs:domain wikidata:Q15831598,
        wikidata:Q17444909,
        wikidata:Q36906466,
        wikidata:Q5961257,
        wikidata:Q6999 ;
    rdfs:range wikidata:Q15831598,
        wikidata:Q17444909,
        wikidata:Q5961257,
        wikidata:Q6999 .

wikidata:P3989 rdfs:label "members have occupation"^^xsd:string ;
    rdfs:comment "all members of this group share the occupation"^^xsd:string ;
    rdfs:domain wikidata:Q14514600,
        wikidata:Q14623646,
        wikidata:Q16334295 ;
    rdfs:range wikidata:Q12737077,
        wikidata:Q17305127 .

wikidata:P40 rdfs:label "child"^^xsd:string ;
    rdfs:comment "subject has object as child. Do not use for stepchildren"^^xsd:string ;
    rdfs:domain wikidata:Q13002315,
        wikidata:Q16979650,
        wikidata:Q178885,
        wikidata:Q21070568,
        wikidata:Q21070598,
        wikidata:Q215627,
        wikidata:Q24334299,
        wikidata:Q4271324,
        wikidata:Q729,
        wikidata:Q95074 ;
    rdfs:range wikidata:Q13002315,
        wikidata:Q16979650,
        wikidata:Q178885,
        wikidata:Q21070568,
        wikidata:Q21070598,
        wikidata:Q24334299,
        wikidata:Q4271324,
        wikidata:Q5,
        wikidata:Q729,
        wikidata:Q95074 ;
    rdfs:subPropertyOf wikidata:P1038,
        wikidata:P3342 .

wikidata:P400 rdfs:label "platform"^^xsd:string ;
    rdfs:comment "platform for which a work was developed or released, or the specific platform version of a software product"^^xsd:string ;
    rdfs:domain wikidata:Q11253473,
        wikidata:Q128093,
        wikidata:Q165194,
        wikidata:Q192851,
        wikidata:Q222910,
        wikidata:Q28114058,
        wikidata:Q40056,
        wikidata:Q40213094,
        wikidata:Q416,
        wikidata:Q47146,
        wikidata:Q7397,
        wikidata:Q7889,
        wikidata:Q7927908,
        wikidata:Q904997,
        wikidata:Q97180164 ;
    rdfs:range wikidata:Q13522376,
        wikidata:Q1406,
        wikidata:Q14116,
        wikidata:Q170434,
        wikidata:Q241317,
        wikidata:Q26884850,
        wikidata:Q388,
        wikidata:Q600659,
        wikidata:Q60644919,
        wikidata:Q6368,
        wikidata:Q8076 .

wikidata:P403 rdfs:label "mouth of the watercourse"^^xsd:string ;
    rdfs:comment "the body of water to which the watercourse drains"^^xsd:string ;
    rdfs:domain wikidata:Q104347069,
        wikidata:Q124714,
        wikidata:Q16338046,
        wikidata:Q24336031,
        wikidata:Q285451,
        wikidata:Q355304,
        wikidata:Q35666,
        wikidata:Q39816 ;
    rdfs:range wikidata:Q15324,
        wikidata:Q16500104,
        wikidata:Q39816 .

wikidata:P404 rdfs:label "game mode"^^xsd:string ;
    rdfs:comment "a video game's available playing mode(s)"^^xsd:string ;
    rdfs:domain wikidata:Q1971694,
        wikidata:Q5519929,
        wikidata:Q7058673,
        wikidata:Q7889 ;
    rdfs:subPropertyOf wikidata:P366 .

wikidata:P4044 rdfs:label "therapeutic area"^^xsd:string ;
    rdfs:comment "disease area in which a medical intervention is applied"^^xsd:string .

wikidata:P406 rdfs:label "soundtrack release"^^xsd:string ;
    rdf:first <http://www.semanticweb.org/ontologies/Wikidata#_:y11>,
        <http://www.semanticweb.org/ontologies/Wikidata#_:y13> ;
    rdfs:comment "music release that incorporates music directly recorded from the soundtrack of an audiovisual work"^^xsd:string ;
    rdfs:domain wikidata:Q17489659,
        wikidata:Q386724 ;
    rdfs:range wikidata:Q134556,
        wikidata:Q169930,
        wikidata:Q29652773,
        wikidata:Q4176708,
        wikidata:Q482994,
        wikidata:Q65091986,
        wikidata:Q66049140 .

wikidata:P408 rdfs:label "software engine"^^xsd:string ;
    rdfs:comment "software engine employed by the subject item"^^xsd:string ;
    rdfs:domain wikidata:Q101191533,
        wikidata:Q15938550,
        wikidata:Q166142,
        wikidata:Q1714118 ;
    rdfs:range wikidata:Q271680,
        wikidata:Q63533016,
        wikidata:Q7397 ;
    rdfs:subPropertyOf wikidata:P2283 .

wikidata:P410 rdfs:label "military rank"^^xsd:string ;
    rdfs:comment "military rank achieved by a person (should usually have a \"start time\" qualifier), or military rank associated with a position"^^xsd:string ;
    rdfs:domain wikidata:Q1479965,
        wikidata:Q26401003,
        wikidata:Q5,
        wikidata:Q95074 ;
    rdfs:range wikidata:Q18325582,
        wikidata:Q19476593,
        wikidata:Q56019 .

wikidata:P4101 rdfs:label "dissertation submitted to"^^xsd:string ;
    rdfs:comment "institution to whom a thesis or dissertation is submitted"^^xsd:string ;
    rdfs:domain wikidata:Q1266946 ;
    rdfs:range wikidata:Q5341295 .

wikidata:P411 rdfs:label "canonization status"^^xsd:string ;
    rdfs:comment "stage in the process of attaining sainthood per the subject's religious organization"^^xsd:string ;
    rdfs:domain wikidata:Q16334295,
        wikidata:Q21070598,
        wikidata:Q5 ;
    rdfs:range wikidata:Q15978876 .

wikidata:P4132 rdfs:label "linguistic typology"^^xsd:string ;
    rdfs:comment "classification of languages according to their linguistic trait (as opposed to historical families like romance languages)"^^xsd:string ;
    rdfs:domain wikidata:Q17376908 .

wikidata:P414 rdfs:label "stock exchange"^^xsd:string ;
    rdfs:comment "exchange on which this company is traded"^^xsd:string ;
    rdfs:domain wikidata:Q223371,
        wikidata:Q4830453,
        wikidata:Q783794 ;
    rdfs:range wikidata:Q11691 .

wikidata:P415 rdfs:label "radio format"^^xsd:string ;
    rdfs:comment "describes the overall content broadcast on a radio station"^^xsd:string ;
    rdfs:domain wikidata:Q1061197,
        wikidata:Q14350,
        wikidata:Q60153785 ;
    rdfs:range wikidata:Q589183 .

wikidata:P417 rdfs:label "patron saint"^^xsd:string ;
    rdfs:comment "patron saint adopted by the subject"^^xsd:string ;
    rdfs:domain wikidata:Q12737077,
        wikidata:Q17149090,
        wikidata:Q1826286,
        wikidata:Q200334,
        wikidata:Q2221906,
        wikidata:Q391009 ;
    rdfs:range wikidata:Q10648343,
        wikidata:Q10822464,
        wikidata:Q1087471,
        wikidata:Q14073567,
        wikidata:Q1509831,
        wikidata:Q16334295,
        wikidata:Q20643955,
        wikidata:Q21070568,
        wikidata:Q2634521,
        wikidata:Q375011,
        wikidata:Q5,
        wikidata:Q95074 .

wikidata:P4195 rdfs:label "category for employees of the organization"^^xsd:string ;
    rdfs:comment "Wikimedia category for people who work or worked at this organization"^^xsd:string ;
    rdfs:domain wikidata:Q43229 ;
    rdfs:range wikidata:Q4167836 .

wikidata:P421 rdfs:label "located in time zone"^^xsd:string ;
    rdfs:comment "time zone for this item"^^xsd:string ;
    rdfs:domain wikidata:Q1190554,
        wikidata:Q12410555,
        wikidata:Q17272482,
        wikidata:Q1777301,
        wikidata:Q2221906,
        wikidata:Q27096213,
        wikidata:Q36669 ;
    rdfs:range wikidata:Q12143 .

wikidata:P4224 rdfs:label "category contains"^^xsd:string ;
    rdfs:comment "category contains elements that are instances of this item"^^xsd:string ;
    rdfs:domain wikidata:Q4167836 .

wikidata:P425 rdfs:label "field of this occupation"^^xsd:string ;
    rdfs:comment "activity corresponding to this occupation or profession (use only for occupations/professions - for people use Property:P101, for companies use P452)"^^xsd:string ;
    rdfs:domain wikidata:Q12737077,
        wikidata:Q17305127 ;
    rdfs:range wikidata:Q11862829,
        wikidata:Q17524420,
        wikidata:Q1756157,
        wikidata:Q1914636,
        wikidata:Q60733114,
        wikidata:Q7406919,
        wikidata:Q9081 .

wikidata:P4320 rdfs:label "mountains classification"^^xsd:string ;
    rdfs:comment "person ranked for this cycling stage or race"^^xsd:string ;
    rdfs:subPropertyOf wikidata:P2321 .

wikidata:P4322 rdfs:label "best sprinter classification"^^xsd:string ;
    rdfs:comment "person ranked as \"best sprinter\" for this cycling stage or race"^^xsd:string ;
    rdfs:range wikidata:Q5 ;
    rdfs:subPropertyOf wikidata:P2321 .

wikidata:P4323 rdfs:label "young rider classification"^^xsd:string ;
    rdfs:comment "person ranked as young participant for this cycling stage or race"^^xsd:string ;
    rdfs:subPropertyOf wikidata:P2321 .

wikidata:P4329 rdfs:label "template or module that populates category"^^xsd:string ;
    rdfs:comment "this category is populated by the following template or module"^^xsd:string ;
    rdfs:domain wikidata:Q4167836 ;
    rdfs:range wikidata:Q11266439,
        wikidata:Q15184295 .

wikidata:P437 rdfs:label "distribution format"^^xsd:string ;
    rdfs:comment "method (or type) of distribution for the subject"^^xsd:string ;
    rdfs:domain wikidata:Q11424,
        wikidata:Q386724,
        wikidata:Q42848,
        wikidata:Q82014556 ;
    rdfs:range wikidata:Q1020767,
        wikidata:Q1048236,
        wikidata:Q105858921,
        wikidata:Q1209283,
        wikidata:Q1261026,
        wikidata:Q1351368,
        wikidata:Q15416,
        wikidata:Q18602566,
        wikidata:Q190399,
        wikidata:Q1995395,
        wikidata:Q22661286,
        wikidata:Q24633474,
        wikidata:Q26971562,
        wikidata:Q37787110,
        wikidata:Q394970,
        wikidata:Q408978,
        wikidata:Q41349,
        wikidata:Q54820071,
        wikidata:Q55648452,
        wikidata:Q57790812,
        wikidata:Q63367831,
        wikidata:Q682626,
        wikidata:Q723685,
        wikidata:Q759853,
        wikidata:Q81935689,
        wikidata:Q81941037,
        wikidata:Q81945865,
        wikidata:Q81986407,
        wikidata:Q82036085,
        wikidata:Q82046811,
        wikidata:Q830450,
        wikidata:Q86850 .

wikidata:P4428 rdfs:label "implementation of"^^xsd:string ;
    rdfs:comment "implementation of a standard, program, specification or programming language"^^xsd:string ;
    rdfs:range wikidata:Q10673035,
        wikidata:Q1151067,
        wikidata:Q165194,
        wikidata:Q317623,
        wikidata:Q40056,
        wikidata:Q8366,
        wikidata:Q9143 ;
    rdfs:subPropertyOf wikidata:P1557 .

wikidata:P4446 rdfs:label "reward program"^^xsd:string ;
    rdfs:comment "reward program associated with the item"^^xsd:string .

wikidata:P449 rdfs:label "original broadcaster"^^xsd:string ;
    rdfs:comment "network(s) or service(s) that originally broadcasted a radio or television program"^^xsd:string ;
    rdfs:domain wikidata:Q386724 ;
    rdfs:range wikidata:Q14350,
        wikidata:Q15265344,
        wikidata:Q1616075,
        wikidata:Q2001305,
        wikidata:Q59152282,
        wikidata:Q66547481,
        wikidata:Q721830,
        wikidata:Q841645 .

wikidata:P450 rdfs:label "astronaut mission"^^xsd:string ;
    rdfs:comment "space mission that the subject is or has been a member of (do not include future missions)"^^xsd:string ;
    rdfs:domain wikidata:Q5,
        wikidata:Q863531,
        wikidata:Q95074 ;
    rdfs:range wikidata:Q14637321,
        wikidata:Q5916,
        wikidata:Q7217761 ;
    rdfs:subPropertyOf wikidata:P121,
        wikidata:P1344 .

wikidata:P451 a owl:SymmetricProperty ;
    rdfs:label "unmarried partner"^^xsd:string ;
    rdfs:comment "someone with whom the person is in a relationship without being married. Use \"spouse\" (P26) for married couples"^^xsd:string ;
    rdfs:domain wikidata:Q13002315,
        wikidata:Q168658,
        wikidata:Q178885,
        wikidata:Q2239243,
        wikidata:Q4271324,
        wikidata:Q5,
        wikidata:Q729,
        wikidata:Q95074 ;
    rdfs:range wikidata:Q13002315,
        wikidata:Q178885,
        wikidata:Q2239243,
        wikidata:Q4271324,
        wikidata:Q5,
        wikidata:Q729,
        wikidata:Q95074 ;
    rdfs:subPropertyOf wikidata:P3342 .

wikidata:P4510 rdfs:label "describes a project that uses"^^xsd:string ;
    rdfs:comment "essential component or tool that was used in the project described in this publication"^^xsd:string ;
    rdfs:domain wikidata:Q732577,
        wikidata:Q79250806,
        wikidata:Q97180164 .

wikidata:P452 rdfs:label "industry"^^xsd:string ;
    rdfs:comment "specific industry of company or organization"^^xsd:string ;
    rdfs:domain wikidata:Q1047113,
        wikidata:Q12737077,
        wikidata:Q14623646,
        wikidata:Q170584,
        wikidata:Q17305127,
        wikidata:Q431289,
        wikidata:Q43229,
        wikidata:Q5446565,
        wikidata:Q7406919,
        wikidata:Q8187769 ;
    rdfs:range wikidata:Q121359,
        wikidata:Q268592,
        wikidata:Q3958441,
        wikidata:Q8148,
        wikidata:Q8187769 ;
    rdfs:subPropertyOf wikidata:P361 .

wikidata:P453 rdfs:label "character role"^^xsd:string ;
    rdfs:comment "specific role played or filled by subject -- use only as qualifier of \"cast member\" (P161), \"voice actor\" (P725)"^^xsd:string ;
    rdfs:range wikidata:Q1707847,
        wikidata:Q18086706,
        wikidata:Q21070598,
        wikidata:Q215627,
        wikidata:Q24577840,
        wikidata:Q95074 .

wikidata:P4552 rdfs:label "mountain range"^^xsd:string ;
    rdfs:comment "range or subrange to which the geographical item belongs"^^xsd:string ;
    rdfs:domain wikidata:Q618123 ;
    rdfs:range wikidata:Q1061151,
        wikidata:Q1174791,
        wikidata:Q1437459,
        wikidata:Q19850234,
        wikidata:Q46831 ;
    rdfs:subPropertyOf wikidata:P4688 .

wikidata:P457 rdfs:label "foundational text"^^xsd:string ;
    rdfs:comment "text through which an institution or object has been created or established"^^xsd:string ;
    rdfs:range wikidata:Q1058236,
        wikidata:Q2571972,
        wikidata:Q49848 .

wikidata:P4586 rdfs:label "type foundry"^^xsd:string ;
    rdfs:comment "company releasing or distributing a font or typeface"^^xsd:string ;
    rdfs:domain wikidata:Q17451,
        wikidata:Q58481926 ;
    rdfs:range wikidata:Q377688 ;
    rdfs:subPropertyOf wikidata:P170 .

wikidata:P460 a owl:SymmetricProperty ;
    rdfs:label "said to be the same as"^^xsd:string ;
    rdfs:comment "this item is said to be the same as that item, but it's uncertain or disputed"^^xsd:string .

wikidata:P4608 rdfs:label "scenographer"^^xsd:string ;
    rdfs:comment "person who designed the stage or film set of this item"^^xsd:string ;
    rdfs:range wikidata:Q5 ;
    rdfs:subPropertyOf wikidata:P3342 .

wikidata:P461 a owl:SymmetricProperty ;
    rdfs:label "opposite of"^^xsd:string ;
    rdfs:comment "item that is the opposite of this item"^^xsd:string .

wikidata:P4614 rdfs:label "drainage basin"^^xsd:string ;
    rdfs:comment "area where precipitation collects and drains off into a common outlet, such as into a river, bay, or other body of water"^^xsd:string ;
    rdfs:range wikidata:Q166620 ;
    rdfs:subPropertyOf wikidata:P706 .

wikidata:P4628 a owl:FunctionalProperty ;
    rdfs:label "ICTV virus genome composition"^^xsd:string ;
    rdfs:comment "classification of viruses of the International Committee on Taxonomy of Viruses by the molecular composition of the virus genome (DNA, RNA, double or single stranded and translational polarity)"^^xsd:string .

wikidata:P4647 rdfs:label "location of first performance"^^xsd:string ;
    rdfs:comment "location where a work was first debuted, performed or broadcasted"^^xsd:string ;
    rdfs:domain wikidata:Q386724,
        wikidata:Q43099500 ;
    rdfs:range wikidata:Q132241,
        wikidata:Q1955280,
        wikidata:Q27968055,
        wikidata:Q43229,
        wikidata:Q464980,
        wikidata:Q618123 ;
    rdfs:subPropertyOf wikidata:P7153 .

wikidata:P466 rdfs:label "occupant"^^xsd:string ;
    rdfs:comment "a person or organization occupying property"^^xsd:string ;
    rdfs:domain wikidata:Q13226383,
        wikidata:Q18247357,
        wikidata:Q2775969,
        wikidata:Q3895768,
        wikidata:Q39546,
        wikidata:Q58778,
        wikidata:Q63959448,
        wikidata:Q699405,
        wikidata:Q811979,
        wikidata:Q82794 ;
    rdfs:range wikidata:Q14514600,
        wikidata:Q14623646,
        wikidata:Q16334295,
        wikidata:Q21192438,
        wikidata:Q4164871,
        wikidata:Q43229,
        wikidata:Q5,
        wikidata:Q8719053,
        wikidata:Q95074 .

wikidata:P467 rdfs:label "legislated by"^^xsd:string ;
    rdfs:comment "indicates that an act or bill was passed by a legislature.  The value can be a particular session of the legislature"^^xsd:string ;
    rdfs:domain wikidata:Q2751586,
        wikidata:Q6453643,
        wikidata:Q699907,
        wikidata:Q820655 ;
    rdfs:range wikidata:Q11204,
        wikidata:Q116,
        wikidata:Q15238777,
        wikidata:Q1812889,
        wikidata:Q2500378,
        wikidata:Q3044,
        wikidata:Q4358176 .

wikidata:P468 rdfs:label "dan/kyu rank"^^xsd:string ;
    rdfs:comment "rank system used in several board games (e.g. go, shogi, renju), martial arts (e.g. judo, kendo, wushu) and some other games"^^xsd:string ;
    rdfs:domain wikidata:Q215627,
        wikidata:Q3257925 ;
    rdfs:range wikidata:Q373498 .

wikidata:P469 rdfs:label "lakes on river"^^xsd:string ;
    rdfs:comment "lakes, reservoirs, waterfalls the river flows through"^^xsd:string ;
    rdfs:domain wikidata:Q355304 ;
    rdfs:range wikidata:Q15324 .

wikidata:P47 a owl:SymmetricProperty ;
    rdfs:label "shares border with"^^xsd:string ;
    rdfs:comment "countries or administrative subdivisions, of equal level, that this item borders, either by land or water. A single common point is enough."^^xsd:string ;
    rdfs:domain wikidata:Q2221906,
        wikidata:Q24334893,
        wikidata:Q3895768,
        wikidata:Q4006,
        wikidata:Q618123,
        wikidata:Q8928 ;
    rdfs:range wikidata:Q24334893,
        wikidata:Q3895768,
        wikidata:Q4006,
        wikidata:Q618123,
        wikidata:Q8928 .

wikidata:P479 rdfs:label "input method"^^xsd:string ;
    rdfs:comment "input method or device used to interact with a software product"^^xsd:string ;
    rdfs:domain wikidata:Q11253473,
        wikidata:Q1668024,
        wikidata:Q17589470,
        wikidata:Q192851,
        wikidata:Q26884850,
        wikidata:Q2858615,
        wikidata:Q56682555,
        wikidata:Q7397,
        wikidata:Q8076,
        wikidata:Q864114 ;
    rdfs:range wikidata:Q47146 .

wikidata:P4791 rdfs:label "commanded by"^^xsd:string ;
    rdfs:comment "commander of a military unit/army/security service, operation, etc."^^xsd:string ;
    rdfs:domain wikidata:Q17149090,
        wikidata:Q176799,
        wikidata:Q178561,
        wikidata:Q18011131,
        wikidata:Q18011141,
        wikidata:Q18691599,
        wikidata:Q42889,
        wikidata:Q48900561,
        wikidata:Q645883,
        wikidata:Q6619802,
        wikidata:Q939616 ;
    rdfs:range wikidata:Q215627,
        wikidata:Q95074 .

wikidata:P4794 rdfs:label "season starts"^^xsd:string ;
    rdfs:comment "month or season when sports competition begins"^^xsd:string .

wikidata:P4810 rdfs:label "reads environment variable"^^xsd:string ;
    rdfs:comment "an environment variable which a software program reads and may be effected by"^^xsd:string ;
    rdfs:domain wikidata:Q7397 ;
    rdfs:range wikidata:Q400857 .

wikidata:P483 rdfs:label "recorded at studio or venue"^^xsd:string ;
    rdfs:comment "studio or location where a musical composition was recorded"^^xsd:string ;
    rdfs:domain wikidata:Q2188189,
        wikidata:Q482994,
        wikidata:Q6942562,
        wikidata:Q7302866 ;
    rdfs:range wikidata:Q16560,
        wikidata:Q16970,
        wikidata:Q17350442,
        wikidata:Q182832,
        wikidata:Q18674739,
        wikidata:Q22698,
        wikidata:Q22746,
        wikidata:Q24354,
        wikidata:Q33506,
        wikidata:Q3469910,
        wikidata:Q3918,
        wikidata:Q40357,
        wikidata:Q41582469,
        wikidata:Q483110,
        wikidata:Q641226,
        wikidata:Q746369,
        wikidata:Q868557,
        wikidata:Q8719053 ;
    rdfs:subPropertyOf wikidata:P8546 .

wikidata:P4873 a owl:SymmetricProperty ;
    rdfs:label "isoschizomer"^^xsd:string ;
    rdfs:comment "isoschizomers of the restriction restriction enzyme, which have the same recognition sequence and the cutting site."^^xsd:string ;
    rdfs:domain wikidata:Q219715 ;
    rdfs:range wikidata:Q219715 .

wikidata:P4875 a owl:SymmetricProperty ;
    rdfs:label "neoschizomer"^^xsd:string ;
    rdfs:comment "neoschizomers of the restriction restriction enzyme, which have the same recognition sequence but a different cutting site."^^xsd:string ;
    rdfs:domain wikidata:Q219715 ;
    rdfs:range wikidata:Q219715 .

wikidata:P4913 rdfs:label "dialect of"^^xsd:string ;
    rdfs:comment "language of which an item with this property is a dialect. Use in addition to \"subclass of\" (P279) if a languoid is also considered a dialect."^^xsd:string ;
    rdfs:domain wikidata:Q1208380,
        wikidata:Q20671152,
        wikidata:Q2630831,
        wikidata:Q33384,
        wikidata:Q8217193 ;
    rdfs:range wikidata:Q34770 .

wikidata:P4915 a owl:SymmetricProperty ;
    rdfs:label "isocaudomer"^^xsd:string ;
    rdfs:comment "isocaudomer of the restriction restriction enzyme, which have the different recognition sequence but produces the same termini"^^xsd:string ;
    rdfs:domain wikidata:Q219715 ;
    rdfs:range wikidata:Q219715 .

wikidata:P500 rdfs:label "exclave of"^^xsd:string ;
    rdfs:comment "territory is legally or politically attached to a main territory with which it is not physically contiguous because of surrounding alien territory. It may also be an enclave."^^xsd:string ;
    rdfs:domain wikidata:Q933394 ;
    rdfs:range wikidata:Q15642541 .

wikidata:P501 rdfs:label "enclave within"^^xsd:string ;
    rdfs:comment "territory is entirely surrounded by the other (enclaved)"^^xsd:string ;
    rdfs:domain wikidata:Q171441 ;
    rdfs:range wikidata:Q56061,
        wikidata:Q7275 .

wikidata:P504 rdfs:label "home port"^^xsd:string ;
    rdfs:comment "home port of the vessel (if different from \"ship registry\"): For civilian ships, the primary port from which the ship operates. Port of registry →P532 should be listed in \"Ship registry\". For warships, this will be the ship's assigned naval base"^^xsd:string ;
    rdfs:domain wikidata:Q1229765 ;
    rdfs:range wikidata:Q2221906 ;
    rdfs:subPropertyOf wikidata:P7153 .

wikidata:P505 rdfs:label "general manager"^^xsd:string ;
    rdfs:comment "general manager of a sports team. If they are also an on-field manager use P286 instead"^^xsd:string ;
    rdfs:domain wikidata:Q12973014 ;
    rdfs:range wikidata:Q215627 .

wikidata:P509 rdfs:label "cause of death"^^xsd:string ;
    rdfs:comment "underlying or immediate cause of death.  Underlying cause (e.g. car accident, stomach cancer) preferred.  Use 'manner of death' (P1196) for broadest category, e.g. natural causes, accident, homicide, suicide"^^xsd:string ;
    rdfs:domain wikidata:Q14514600,
        wikidata:Q16334298,
        wikidata:Q21070598,
        wikidata:Q215627,
        wikidata:Q7239,
        wikidata:Q95074 ;
    rdfs:range wikidata:Q124490,
        wikidata:Q15169167,
        wikidata:Q1520311,
        wikidata:Q171558,
        wikidata:Q1931388,
        wikidata:Q2057971,
        wikidata:Q2485083,
        wikidata:Q33753,
        wikidata:Q650711 .

wikidata:P511 rdfs:label "honorific prefix"^^xsd:string ;
    rdfs:comment "word or expression used before a name, in addressing or referring to a person"^^xsd:string ;
    rdfs:domain wikidata:Q215627,
        wikidata:Q4120621,
        wikidata:Q4164871 ;
    rdfs:range wikidata:Q3320743,
        wikidata:Q5767753,
        wikidata:Q95074 .

wikidata:P512 rdfs:label "academic degree"^^xsd:string ;
    rdfs:comment "academic degree that the person holds"^^xsd:string ;
    rdfs:domain wikidata:Q215627,
        wikidata:Q5,
        wikidata:Q95074 ;
    rdfs:range wikidata:Q189533 .

wikidata:P516 rdfs:label "powered by"^^xsd:string ;
    rdfs:comment "equipment or engine used by the subject to convert a source or energy into mechanical energy"^^xsd:string ;
    rdfs:domain wikidata:Q4406616,
        wikidata:Q7184903 ;
    rdfs:range wikidata:Q15057021,
        wikidata:Q1753139,
        wikidata:Q44167 ;
    rdfs:subPropertyOf wikidata:P527 .

wikidata:P517 rdfs:label "interaction"^^xsd:string ;
    rdfs:comment "subset of the four fundamental forces (strong (Q11415), electromagnetic (Q849919), weak (Q11418), and gravitation (Q11412) with which a particle interacts"^^xsd:string ;
    rdfs:domain wikidata:Q1621273,
        wikidata:Q22675015 ;
    rdfs:range wikidata:Q104934 .

wikidata:P520 rdfs:label "armament"^^xsd:string ;
    rdfs:comment "equippable weapon item for the subject"^^xsd:string ;
    rdfs:range wikidata:Q15720870,
        wikidata:Q25519785,
        wikidata:Q39546,
        wikidata:Q728 ;
    rdfs:subPropertyOf wikidata:P912 .

wikidata:P521 a owl:SymmetricProperty ;
    rdfs:label "scheduled service destination"^^xsd:string ;
    rdfs:comment "airport or station connected by regular direct service to the subject; for the destination of a trip see P1444"^^xsd:string ;
    rdfs:domain wikidata:Q12819564,
        wikidata:Q44782,
        wikidata:Q62447 ;
    rdfs:range wikidata:Q12819564,
        wikidata:Q44782,
        wikidata:Q62447 .

wikidata:P53 rdfs:label "family"^^xsd:string ;
    rdfs:comment "family, including dynasty and nobility houses. Not family name (use P734 for family name)."^^xsd:string ;
    rdfs:domain wikidata:Q101352,
        wikidata:Q1313923,
        wikidata:Q15331236,
        wikidata:Q21070598,
        wikidata:Q5,
        wikidata:Q5433312,
        wikidata:Q64520857,
        wikidata:Q64643615,
        wikidata:Q75855169,
        wikidata:Q95074 ;
    rdfs:range wikidata:Q13417114,
        wikidata:Q15331236,
        wikidata:Q19791817,
        wikidata:Q2240474,
        wikidata:Q24074280,
        wikidata:Q8436 ;
    rdfs:subPropertyOf wikidata:P463 .

wikidata:P530 a owl:SymmetricProperty ;
    rdfs:label "diplomatic relation"^^xsd:string ;
    rdfs:comment "diplomatic relations of the country"^^xsd:string ;
    rdfs:domain wikidata:Q245065,
        wikidata:Q3024240,
        wikidata:Q7275 ;
    rdfs:range wikidata:Q1335818,
        wikidata:Q6256,
        wikidata:Q7275 .

wikidata:P532 rdfs:label "port of registry"^^xsd:string ;
    rdfs:comment "ship's port of registry. This is generally painted on the ship's stern (for the \"home port\", see Property:P504)"^^xsd:string ;
    rdfs:domain wikidata:Q1229765 ;
    rdfs:range wikidata:Q486972 .

wikidata:P533 rdfs:label "target"^^xsd:string ;
    rdfs:comment "target of an attack or military operation"^^xsd:string ;
    rdfs:domain wikidata:Q1174599,
        wikidata:Q1456832,
        wikidata:Q149377,
        wikidata:Q28945444,
        wikidata:Q3199915,
        wikidata:Q645883 ;
    rdfs:subPropertyOf wikidata:P3712 .

wikidata:P534 rdfs:label "streak color"^^xsd:string ;
    rdfs:comment "color of a mineral or material when abraded"^^xsd:string ;
    rdfs:domain wikidata:Q7946 ;
    rdfs:range wikidata:Q1075 ;
    rdfs:subPropertyOf wikidata:P462 .

wikidata:P541 rdfs:label "office contested"^^xsd:string ;
    rdfs:comment "title of office which election will determine the next holder of"^^xsd:string ;
    rdfs:domain wikidata:Q11642595,
        wikidata:Q19571328,
        wikidata:Q40231,
        wikidata:Q6138528,
        wikidata:Q905151 ;
    rdfs:range wikidata:Q4164871 .

wikidata:P542 rdfs:label "officially opened by"^^xsd:string ;
    rdfs:comment "person that officially opened the event or place"^^xsd:string ;
    rdfs:domain wikidata:Q121359,
        wikidata:Q1656682,
        wikidata:Q2221906,
        wikidata:Q33506,
        wikidata:Q464980,
        wikidata:Q4830453,
        wikidata:Q58778,
        wikidata:Q811430 ;
    rdfs:range wikidata:Q5 .

wikidata:P547 rdfs:label "commemorates"^^xsd:string ;
    rdfs:comment "what the place, monument, memorial, or holiday, commemorates"^^xsd:string ;
    rdfs:domain wikidata:Q10884,
        wikidata:Q1445650,
        wikidata:Q14795564,
        wikidata:Q15275719,
        wikidata:Q1656682,
        wikidata:Q173387,
        wikidata:Q17537576,
        wikidata:Q2221906,
        wikidata:Q37930,
        wikidata:Q4989906,
        wikidata:Q5,
        wikidata:Q5003624,
        wikidata:Q657449,
        wikidata:Q721747,
        wikidata:Q838948,
        wikidata:Q855973,
        wikidata:Q933348 ;
    rdfs:subPropertyOf wikidata:P921 .

wikidata:P552 rdfs:label "handedness"^^xsd:string ;
    rdfs:comment "handedness of the person"^^xsd:string ;
    rdfs:domain wikidata:Q215627,
        wikidata:Q95074 ;
    rdfs:range wikidata:Q10927834 .

wikidata:P553 rdfs:label "website account on"^^xsd:string ;
    rdfs:comment "website that the person or organization has an account on (use with P554) Note: only used with reliable source or if the person or organization disclosed it."^^xsd:string ;
    rdfs:range wikidata:Q210980,
        wikidata:Q287198,
        wikidata:Q2989352,
        wikidata:Q3133368,
        wikidata:Q340169,
        wikidata:Q42336871 .

wikidata:P556 rdfs:label "crystal system"^^xsd:string ;
    rdfs:comment "type of crystal for minerals and/or for crystal compounds"^^xsd:string ;
    rdfs:range wikidata:Q898786 .

wikidata:P559 a owl:IrreflexiveProperty ;
    rdfs:label "terminus"^^xsd:string ;
    rdfs:comment "the feature (intersecting road, train station, etc.) at the end of a linear feature"^^xsd:string ;
    rdfs:domain wikidata:Q27096213 ;
    rdfs:range wikidata:Q27096213 .

wikidata:P562 rdfs:label "central bank/issuer"^^xsd:string ;
    rdfs:comment "central bank or other issuing authority for the currency"^^xsd:string ;
    rdfs:domain wikidata:Q8142 ;
    rdfs:range wikidata:Q43229 .

wikidata:P567 rdfs:label "underlies"^^xsd:string ;
    rdfs:comment "stratigraphic unit that this unit lies under (i.e. the overlying unit)"^^xsd:string .

wikidata:P568 rdfs:label "overlies"^^xsd:string ;
    rdfs:comment "stratigraphic unit that this unit lies over (i.e. the underlying unit)"^^xsd:string .

wikidata:P57 rdfs:label "director"^^xsd:string ;
    rdfs:comment "director(s) of film, TV-series, stageplay, video game or similar"^^xsd:string ;
    rdfs:domain wikidata:Q106046707,
        wikidata:Q11424,
        wikidata:Q14623351,
        wikidata:Q15416,
        wikidata:Q2431196,
        wikidata:Q24856,
        wikidata:Q25379,
        wikidata:Q26204053,
        wikidata:Q43099500,
        wikidata:Q7889 ;
    rdfs:range wikidata:Q5 ;
    rdfs:subPropertyOf wikidata:P3342,
        wikidata:P50 .

wikidata:P579 rdfs:label "IMA status and/or rank"^^xsd:string ;
    rdfs:comment "status given to each mineral by the IMA (International Mineralogical Association)"^^xsd:string .

wikidata:P58 rdfs:label "screenwriter"^^xsd:string ;
    rdfs:comment "person(s) who wrote the script for subject item"^^xsd:string ;
    rdfs:domain wikidata:Q386724 ;
    rdfs:range wikidata:Q10648343,
        wikidata:Q16017119,
        wikidata:Q16334295,
        wikidata:Q3046146,
        wikidata:Q5 ;
    rdfs:subPropertyOf wikidata:P3092,
        wikidata:P50 .

wikidata:P588 rdfs:label "coolant"^^xsd:string ;
    rdfs:comment "substance used by the subject to dissipate excess thermal energy"^^xsd:string .

wikidata:P59 rdfs:label "constellation"^^xsd:string ;
    rdfs:comment "the area of the celestial sphere of which the subject is a part (from a scientific standpoint, not an astrological one)"^^xsd:string ;
    rdfs:domain wikidata:Q280855,
        wikidata:Q6999,
        wikidata:Q751989 ;
    rdfs:range wikidata:Q8928 ;
    rdfs:subPropertyOf wikidata:P361 .

wikidata:P598 rdfs:label "commander of (DEPRECATED)"^^xsd:string ;
    rdfs:comment "for persons who are notable as commanding officers, the units they commanded"^^xsd:string ;
    rdfs:domain wikidata:Q215627,
        wikidata:Q95074 ;
    rdfs:range wikidata:Q17149090,
        wikidata:Q176799,
        wikidata:Q18011131,
        wikidata:Q18643213,
        wikidata:Q18691599,
        wikidata:Q42889,
        wikidata:Q48900561,
        wikidata:Q645883,
        wikidata:Q6619802,
        wikidata:Q939616 .

wikidata:P6 rdfs:label "head of government"^^xsd:string ;
    rdfs:comment "head of the executive power of this town, city, municipality, state, country, or other governmental body"^^xsd:string ;
    rdfs:domain wikidata:Q1048835,
        wikidata:Q1145276,
        wikidata:Q1964689,
        wikidata:Q327333,
        wikidata:Q524572,
        wikidata:Q56061,
        wikidata:Q640506,
        wikidata:Q6866562,
        wikidata:Q7188 ;
    rdfs:range wikidata:Q5,
        wikidata:Q95074 ;
    rdfs:subPropertyOf wikidata:P1037,
        wikidata:P488 .

wikidata:P607 rdfs:label "conflict"^^xsd:string ;
    rdfs:comment "battles, wars or other military engagements in which the person or item participated"^^xsd:string ;
    rdfs:domain wikidata:Q1156741,
        wikidata:Q11976958,
        wikidata:Q15142894,
        wikidata:Q16334295,
        wikidata:Q176799,
        wikidata:Q178561,
        wikidata:Q18011131,
        wikidata:Q18011141,
        wikidata:Q18643213,
        wikidata:Q188055,
        wikidata:Q21070598,
        wikidata:Q26401003,
        wikidata:Q29048322,
        wikidata:Q2961496,
        wikidata:Q39546,
        wikidata:Q47272186,
        wikidata:Q5,
        wikidata:Q5003624,
        wikidata:Q57821,
        wikidata:Q718893,
        wikidata:Q95074 ;
    rdfs:range wikidata:Q1168287,
        wikidata:Q14136353,
        wikidata:Q180684,
        wikidata:Q18812548,
        wikidata:Q3199915,
        wikidata:Q45382,
        wikidata:Q645883,
        wikidata:Q718893,
        wikidata:Q842332 ;
    rdfs:subPropertyOf wikidata:P1344 .

wikidata:P608 rdfs:label "exhibition history"^^xsd:string ;
    rdfs:comment "exhibitions where the item is or was displayed"^^xsd:string ;
    rdfs:domain wikidata:Q18593264,
        wikidata:Q220659,
        wikidata:Q386724 ;
    rdfs:range wikidata:Q33506,
        wikidata:Q464980 .

wikidata:P609 rdfs:label "terminus location"^^xsd:string ;
    rdfs:comment "location of the terminus of a linear feature"^^xsd:string ;
    rdfs:domain wikidata:Q12284,
        wikidata:Q34442,
        wikidata:Q83620 ;
    rdfs:range wikidata:Q486972,
        wikidata:Q56061 .

wikidata:P61 rdfs:label "discoverer or inventor"^^xsd:string ;
    rdfs:comment "subject  who discovered, first described, invented, or developed this discovery or invention"^^xsd:string ;
    rdfs:range wikidata:Q13226383,
        wikidata:Q1378139,
        wikidata:Q14514600,
        wikidata:Q16334295,
        wikidata:Q18327510,
        wikidata:Q43229,
        wikidata:Q5,
        wikidata:Q550089,
        wikidata:Q6502154,
        wikidata:Q7397,
        wikidata:Q95074 .

wikidata:P610 rdfs:label "highest point"^^xsd:string ;
    rdfs:comment "point with highest elevation in a region, or on the path of a race or route"^^xsd:string ;
    rdfs:domain wikidata:Q2221906,
        wikidata:Q24334893,
        wikidata:Q3895768,
        wikidata:Q82794,
        wikidata:Q878123 ;
    rdfs:range wikidata:Q133056,
        wikidata:Q207326,
        wikidata:Q3393392,
        wikidata:Q3895768,
        wikidata:Q46831,
        wikidata:Q54050,
        wikidata:Q8072,
        wikidata:Q8502 ;
    rdfs:subPropertyOf wikidata:P527 .

wikidata:P611 rdfs:label "religious order"^^xsd:string ;
    rdfs:comment "order of monks or nuns to which an individual or religious house belongs"^^xsd:string ;
    rdfs:domain wikidata:Q1088552,
        wikidata:Q1128397,
        wikidata:Q160742,
        wikidata:Q16334295,
        wikidata:Q16970,
        wikidata:Q2750108,
        wikidata:Q3914,
        wikidata:Q43229,
        wikidata:Q5,
        wikidata:Q618123 ;
    rdfs:range wikidata:Q2061186 ;
    rdfs:subPropertyOf wikidata:P463 .

wikidata:P612 a owl:AsymmetricProperty,
        owl:IrreflexiveProperty ;
    rdfs:label "mother house"^^xsd:string ;
    rdfs:comment "principal house or community for a religious institute"^^xsd:string ;
    rdfs:domain wikidata:Q44613 ;
    rdfs:range wikidata:Q44613 .

wikidata:P618 rdfs:label "source of energy"^^xsd:string ;
    rdfs:comment "describes the source of energy an animated object (machine or animal) uses"^^xsd:string ;
    rdfs:domain wikidata:Q4406616,
        wikidata:Q7184903 ;
    rdfs:range wikidata:Q1522115,
        wikidata:Q3935690,
        wikidata:Q42501,
        wikidata:Q837718 ;
    rdfs:subPropertyOf wikidata:P2283 .

wikidata:P629 rdfs:label "edition or translation of"^^xsd:string ;
    rdfs:comment "is an edition or translation of this entity"^^xsd:string ;
    rdfs:domain wikidata:Q104696061,
        wikidata:Q131436,
        wikidata:Q17776219,
        wikidata:Q26160672,
        wikidata:Q3331189,
        wikidata:Q379755,
        wikidata:Q63141557,
        wikidata:Q79719 ;
    rdfs:range wikidata:Q386724 .

wikidata:P631 rdfs:label "structural engineer"^^xsd:string ;
    rdfs:comment "person, group or organisation responsible for the structural engineering of a building or structure"^^xsd:string ;
    rdfs:domain wikidata:Q811430 .

wikidata:P634 rdfs:label "captain"^^xsd:string ;
    rdfs:comment "captain of this sports team"^^xsd:string ;
    rdfs:domain wikidata:Q12973014 ;
    rdfs:range wikidata:Q15632617,
        wikidata:Q5 .

wikidata:P636 rdfs:label "route of administration"^^xsd:string ;
    rdfs:comment "path by which a drug, fluid, poison, or other substance is taken into the body"^^xsd:string ;
    rdfs:domain wikidata:Q11173,
        wikidata:Q12140,
        wikidata:Q28885102 ;
    rdfs:range wikidata:Q621636 .

wikidata:P642 rdfs:label "of"^^xsd:string ;
    rdfs:comment "qualifier stating that a statement applies within the scope of a particular item"^^xsd:string .

wikidata:P647 rdfs:label "drafted by"^^xsd:string ;
    rdfs:comment "which team the player was drafted by"^^xsd:string ;
    rdfs:domain wikidata:Q5 ;
    rdfs:range wikidata:Q4438121 .

wikidata:P65 rdfs:label "site of astronomical discovery"^^xsd:string ;
    rdfs:comment "the place where an astronomical object was discovered (observatory, satellite)"^^xsd:string ;
    rdfs:domain wikidata:Q6999,
        wikidata:Q751989 ;
    rdfs:range wikidata:Q17334923 ;
    rdfs:subPropertyOf wikidata:P189 .

wikidata:P658 rdfs:label "tracklist"^^xsd:string ;
    rdf:first <http://www.semanticweb.org/ontologies/Wikidata#_:y14> ;
    rdfs:comment "audio tracks contained in this release"^^xsd:string ;
    rdfs:domain wikidata:Q2031291,
        wikidata:Q7410139 ;
    rdfs:range wikidata:Q2188189,
        wikidata:Q64917966,
        wikidata:Q7302866,
        wikidata:Q7366 ;
    rdfs:subPropertyOf wikidata:P527 .

wikidata:P66 rdfs:label "ancestral home"^^xsd:string ;
    rdfs:comment "place of origin for ancestors of subject"^^xsd:string ;
    rdfs:domain wikidata:Q15831596,
        wikidata:Q215627,
        wikidata:Q41710,
        wikidata:Q8436 ;
    rdfs:range wikidata:Q3895768,
        wikidata:Q618123 .

wikidata:P664 rdfs:label "organizer"^^xsd:string ;
    rdfs:comment "person or institution organizing an event"^^xsd:string ;
    rdfs:domain wikidata:Q1190554,
        wikidata:Q14136353 ;
    rdfs:range wikidata:Q14623646,
        wikidata:Q16334295,
        wikidata:Q43229,
        wikidata:Q49773,
        wikidata:Q5 .

wikidata:P669 rdfs:label "located on street"^^xsd:string ;
    rdfs:comment "street, road, or square, where the item is located. To add the number, use Property:P670 \"street number\" as qualifier. Use property P6375 if there is no item for the street"^^xsd:string ;
    rdfs:domain wikidata:Q1190554,
        wikidata:Q2668072,
        wikidata:Q3895768,
        wikidata:Q41176,
        wikidata:Q43229,
        wikidata:Q4830453,
        wikidata:Q618123,
        wikidata:Q838948 ;
    rdfs:range wikidata:Q1251403,
        wikidata:Q174782,
        wikidata:Q18948595,
        wikidata:Q269949,
        wikidata:Q34442,
        wikidata:Q79007,
        wikidata:Q83620 ;
    rdfs:subPropertyOf wikidata:P276,
        wikidata:P361 .

wikidata:P674 rdfs:label "characters"^^xsd:string ;
    rdfs:comment "characters which appear in this item (like plays, operas, operettas, books, comics, films, TV series, video games)"^^xsd:string ;
    rdfs:domain wikidata:Q1185607,
        wikidata:Q15306849,
        wikidata:Q386724 ;
    rdfs:range wikidata:Q13002315,
        wikidata:Q14514600,
        wikidata:Q15706911,
        wikidata:Q20830276,
        wikidata:Q21192438,
        wikidata:Q215627,
        wikidata:Q2607197,
        wikidata:Q4271324,
        wikidata:Q622852,
        wikidata:Q95074 .

wikidata:P676 rdfs:label "lyrics by"^^xsd:string ;
    rdfs:comment "author of song lyrics"^^xsd:string ;
    rdfs:domain wikidata:Q2188189,
        wikidata:Q4327689,
        wikidata:Q7302866 ;
    rdfs:range wikidata:Q16334295,
        wikidata:Q5 ;
    rdfs:subPropertyOf wikidata:P50 .

wikidata:P680 rdfs:label "molecular function"^^xsd:string ;
    rdfs:comment "represents gene ontology function annotations"^^xsd:string ;
    rdfs:domain wikidata:Q172847,
        wikidata:Q22325163,
        wikidata:Q8054,
        wikidata:Q84467700 ;
    rdfs:subPropertyOf wikidata:P1542 .

wikidata:P682 rdfs:label "biological process"^^xsd:string ;
    rdfs:comment "is involved in the biological process"^^xsd:string ;
    rdfs:domain wikidata:Q134219,
        wikidata:Q22325163,
        wikidata:Q420927,
        wikidata:Q7187,
        wikidata:Q8054,
        wikidata:Q84467700 ;
    rdfs:subPropertyOf wikidata:P710 .

wikidata:P684 a owl:SymmetricProperty ;
    rdfs:label "ortholog"^^xsd:string ;
    rdfs:comment "orthologous gene in another species (use with 'species' qualifier)"^^xsd:string .

wikidata:P688 rdfs:label "encodes"^^xsd:string ;
    rdfs:comment "the product of a gene (protein or RNA)"^^xsd:string ;
    rdfs:domain wikidata:Q121438,
        wikidata:Q7187 .

wikidata:P689 rdfs:label "afflicts"^^xsd:string ;
    rdfs:comment "type of organism or organ which a condition or disease afflicts"^^xsd:string ;
    rdfs:domain wikidata:Q7189713 .

wikidata:P694 rdfs:label "replaced synonym (for nom. nov.)"^^xsd:string ;
    rdfs:comment "previously published name on which a replacement name (avowed substitute, nomen novum) is based."^^xsd:string ;
    rdfs:domain wikidata:Q16521,
        wikidata:Q23729754 ;
    rdfs:range wikidata:Q10753560,
        wikidata:Q16521,
        wikidata:Q23729754 .

wikidata:P708 rdfs:label "diocese"^^xsd:string ;
    rdfs:comment "administrative division of the church to which the element belongs; use P5607 for other types of ecclesiastical territorial entities"^^xsd:string ;
    rdfs:range wikidata:Q105072162,
        wikidata:Q105388829,
        wikidata:Q105390172,
        wikidata:Q1431554,
        wikidata:Q1492823,
        wikidata:Q1531518,
        wikidata:Q1778235,
        wikidata:Q2288631,
        wikidata:Q2665272,
        wikidata:Q285181,
        wikidata:Q3146899,
        wikidata:Q3732788,
        wikidata:Q384003,
        wikidata:Q620225,
        wikidata:Q665487 .

wikidata:P720 rdfs:label "asteroid spectral type"^^xsd:string ;
    rdfs:comment "spectral classifications of asteroids based on  spectral shape, color, and albedo"^^xsd:string ;
    rdfs:domain wikidata:Q3863 ;
    rdfs:range wikidata:Q1750705 .

wikidata:P725 rdfs:label "voice actor"^^xsd:string ;
    rdfs:comment "performer of a spoken role in a creative work such as animation, video game, radio drama, or dubbing over [use \"character role\" (P453) as qualifier] [use \"cast member\" (P161) for live acting]"^^xsd:string ;
    rdfs:domain wikidata:Q106833,
        wikidata:Q11424,
        wikidata:Q15416,
        wikidata:Q15524954,
        wikidata:Q1555508,
        wikidata:Q2031291,
        wikidata:Q2431196,
        wikidata:Q24856,
        wikidata:Q26204053,
        wikidata:Q56561355,
        wikidata:Q7889,
        wikidata:Q95074 ;
    rdfs:range wikidata:Q5 ;
    rdfs:subPropertyOf wikidata:P3092 .

wikidata:P734 rdfs:label "family name"^^xsd:string ;
    rdfs:comment "part of full name of person"^^xsd:string ;
    rdfs:domain wikidata:Q13417114,
        wikidata:Q1517820,
        wikidata:Q15331236,
        wikidata:Q16979650,
        wikidata:Q201662,
        wikidata:Q21070598,
        wikidata:Q211503,
        wikidata:Q215627,
        wikidata:Q5,
        wikidata:Q62792750,
        wikidata:Q8436,
        wikidata:Q95074 ;
    rdfs:range wikidata:Q101352 ;
    rdfs:subPropertyOf wikidata:P2561 .

wikidata:P737 rdfs:label "influenced by"^^xsd:string ;
    rdfs:comment "this person, idea, etc. is informed by that other person, idea, etc., e.g. “Heidegger was influenced by Aristotle”"^^xsd:string .

wikidata:P739 rdfs:label "ammunition"^^xsd:string ;
    rdfs:comment "cartridge or other ammunition used by the subject firearm"^^xsd:string ;
    rdfs:domain wikidata:Q12796,
        wikidata:Q15720870,
        wikidata:Q181947,
        wikidata:Q42889,
        wikidata:Q46311,
        wikidata:Q728 ;
    rdfs:range wikidata:Q185785 .

wikidata:P740 rdfs:label "location of formation"^^xsd:string ;
    rdfs:comment "location where a group or organization was formed"^^xsd:string ;
    rdfs:domain wikidata:Q15275719,
        wikidata:Q1964689,
        wikidata:Q2088357,
        wikidata:Q215380,
        wikidata:Q386724,
        wikidata:Q43229,
        wikidata:Q618779,
        wikidata:Q8436,
        wikidata:Q9174 ;
    rdfs:subPropertyOf wikidata:P276 .

wikidata:P741 rdfs:label "playing hand"^^xsd:string ;
    rdfs:comment "hand used to play a racket sport"^^xsd:string ;
    rdfs:domain wikidata:Q5 .

wikidata:P744 a owl:FunctionalProperty ;
    rdfs:label "asteroid family"^^xsd:string ;
    rdfs:comment "population of asteroids that share similar proper orbital elements"^^xsd:string ;
    rdfs:domain wikidata:Q1022867 ;
    rdfs:range wikidata:Q249083 .

wikidata:P747 rdfs:label "has edition or translation"^^xsd:string ;
    rdfs:comment "link to an edition of this item"^^xsd:string ;
    rdfs:domain wikidata:Q386724,
        wikidata:Q95107111 ;
    rdfs:range wikidata:Q17776219,
        wikidata:Q26160672,
        wikidata:Q3331189,
        wikidata:Q63141557 .

wikidata:P748 rdfs:label "appointed by"^^xsd:string ;
    rdfs:comment "who appointed the person to the office, can be used as a qualifier"^^xsd:string ;
    rdfs:domain wikidata:Q21451536,
        wikidata:Q4164871,
        wikidata:Q5,
        wikidata:Q95074 ;
    rdfs:range wikidata:Q14897293,
        wikidata:Q267628,
        wikidata:Q4164871,
        wikidata:Q43229,
        wikidata:Q5 .

wikidata:P749 a owl:AsymmetricProperty,
        owl:IrreflexiveProperty ;
    rdfs:label "parent organization"^^xsd:string ;
    rdfs:comment "parent organization of an organization, opposite of subsidiaries (P355)"^^xsd:string ;
    rdfs:domain wikidata:Q14623646,
        wikidata:Q170584,
        wikidata:Q43229 ;
    rdfs:range wikidata:Q14623646,
        wikidata:Q170584,
        wikidata:Q43229 ;
    rdfs:subPropertyOf wikidata:P127 .

wikidata:P750 rdfs:label "distributed by"^^xsd:string ;
    rdfs:comment "distributor of a creative work; distributor for a record label; news agency; film distributor"^^xsd:string ;
    rdfs:domain wikidata:Q18127,
        wikidata:Q2085381,
        wikidata:Q386724,
        wikidata:Q42848 ;
    rdfs:range wikidata:Q19307174,
        wikidata:Q24229398,
        wikidata:Q24634210,
        wikidata:Q30899001,
        wikidata:Q35127,
        wikidata:Q55341040,
        wikidata:Q72588 .

wikidata:P751 rdfs:label "introduced feature"^^xsd:string ;
    rdfs:comment "feature introduced by this version of a product item"^^xsd:string ;
    rdfs:domain wikidata:Q386724 ;
    rdfs:range wikidata:Q4485156 .

wikidata:P756 a owl:InverseFunctionalProperty ;
    rdfs:label "removed feature"^^xsd:string ;
    rdfs:comment "which feature was removed by this version of a product item"^^xsd:string ;
    rdfs:domain wikidata:Q386724 ;
    rdfs:range wikidata:Q4485156 .

wikidata:P767 rdfs:label "contributor to the creative work or subject"^^xsd:string ;
    rdfs:comment "person or organization that contributed to a subject: co-creator of a creative work or subject"^^xsd:string ;
    rdfs:domain wikidata:Q101965,
        wikidata:Q105420,
        wikidata:Q11016,
        wikidata:Q11177771,
        wikidata:Q11862829,
        wikidata:Q12772819,
        wikidata:Q1406161,
        wikidata:Q18593264,
        wikidata:Q2668072,
        wikidata:Q33104279,
        wikidata:Q3331189,
        wikidata:Q386724,
        wikidata:Q464980,
        wikidata:Q5,
        wikidata:Q5281760,
        wikidata:Q7725310 ;
    rdfs:range wikidata:Q16334295,
        wikidata:Q5 .

wikidata:P769 a owl:IrreflexiveProperty ;
    rdfs:label "significant drug interaction"^^xsd:string ;
    rdfs:comment "clinically significant interaction between two pharmacologically active substances (i.e., drugs and/or active metabolites) where concomitant intake can lead to altered effectiveness or adverse drug events."^^xsd:string ;
    rdfs:domain wikidata:Q12140 ;
    rdfs:range wikidata:Q12140 .

wikidata:P770 rdfs:label "cause of destruction"^^xsd:string ;
    rdfs:comment "item which caused the destruction of the subject item"^^xsd:string ;
    rdfs:domain wikidata:Q1229765,
        wikidata:Q15706911,
        wikidata:Q15893266,
        wikidata:Q183366,
        wikidata:Q41176,
        wikidata:Q488383,
        wikidata:Q744913 ;
    rdfs:range wikidata:Q1190554,
        wikidata:Q168983,
        wikidata:Q171558,
        wikidata:Q180684,
        wikidata:Q58197759 ;
    rdfs:subPropertyOf wikidata:P828 .

wikidata:P78 rdfs:label "top-level Internet domain"^^xsd:string ;
    rdfs:comment "Internet domain name system top-level code"^^xsd:string ;
    rdfs:domain wikidata:Q1048835 ;
    rdfs:range wikidata:Q42032 .

wikidata:P780 rdfs:label "symptoms"^^xsd:string ;
    rdfs:comment "possible symptoms of a medical condition"^^xsd:string ;
    rdfs:domain wikidata:Q18596079,
        wikidata:Q7189713 ;
    rdfs:range wikidata:Q1441305,
        wikidata:Q169872 .

wikidata:P787 rdfs:label "spore print color"^^xsd:string ;
    rdfs:comment "color of a mushroom spore print (see documentation for allowed values)"^^xsd:string .

wikidata:P795 rdfs:label "located on linear feature"^^xsd:string ;
    rdfs:comment "linear feature along which distance is specified from a specified datum point"^^xsd:string ;
    rdfs:range wikidata:Q12284,
        wikidata:Q34442,
        wikidata:Q355304,
        wikidata:Q728937,
        wikidata:Q924286 .

wikidata:P797 rdfs:label "authority"^^xsd:string ;
    rdfs:comment "entity having executive power on given entity"^^xsd:string .

wikidata:P800 rdfs:label "notable work"^^xsd:string ;
    rdfs:comment "notable scientific, artistic or literary work, or other work of significance among subject's works"^^xsd:string ;
    rdfs:domain wikidata:Q14514600,
        wikidata:Q16334295,
        wikidata:Q5,
        wikidata:Q52688389,
        wikidata:Q61002,
        wikidata:Q95074 ;
    rdfs:range wikidata:Q1151067,
        wikidata:Q11862829,
        wikidata:Q12047392,
        wikidata:Q12772819,
        wikidata:Q1293220,
        wikidata:Q1298668,
        wikidata:Q14208553,
        wikidata:Q151885,
        wikidata:Q170584,
        wikidata:Q17737,
        wikidata:Q1799072,
        wikidata:Q211364,
        wikidata:Q2424752,
        wikidata:Q2668072,
        wikidata:Q36534,
        wikidata:Q386724,
        wikidata:Q43229,
        wikidata:Q486902,
        wikidata:Q65943,
        wikidata:Q82604 .

wikidata:P802 rdfs:label "student"^^xsd:string ;
    rdfs:comment "notable student(s) of the subject individual"^^xsd:string ;
    rdfs:domain wikidata:Q5,
        wikidata:Q95074 ;
    rdfs:range wikidata:Q5,
        wikidata:Q7380,
        wikidata:Q95074 ;
    rdfs:subPropertyOf wikidata:P3342 .

wikidata:P803 rdfs:label "professorship"^^xsd:string ;
    rdfs:comment "professorship position held by this academic person"^^xsd:string ;
    rdfs:domain wikidata:Q5 ;
    rdfs:range wikidata:Q1363750,
        wikidata:Q486983,
        wikidata:Q81752537 .

wikidata:P805 rdfs:label "statement is subject of"^^xsd:string ;
    rdfs:comment "(qualifying) item that describes the relation identified in this statement"^^xsd:string .

wikidata:P807 a owl:AsymmetricProperty,
        owl:IrreflexiveProperty ;
    rdfs:label "separated from"^^xsd:string ;
    rdfs:comment "subject was founded or started by separating from identified object"^^xsd:string ;
    rdfs:domain wikidata:Q43229,
        wikidata:Q56061,
        wikidata:Q7397 ;
    rdfs:range wikidata:Q43229,
        wikidata:Q56061,
        wikidata:Q7397 .

wikidata:P81 rdfs:label "connecting line"^^xsd:string ;
    rdfs:comment "railway line(s) subject is directly connected to"^^xsd:string ;
    rdfs:domain wikidata:Q1067164,
        wikidata:Q1311670,
        wikidata:Q1318558,
        wikidata:Q181348,
        wikidata:Q1891817,
        wikidata:Q20180855,
        wikidata:Q39486269,
        wikidata:Q44696264,
        wikidata:Q50331459,
        wikidata:Q548662 ;
    rdfs:range wikidata:Q728937 ;
    rdfs:subPropertyOf wikidata:P361 .

wikidata:P812 rdfs:label "academic major"^^xsd:string ;
    rdfs:comment "subject someone studied at college/university"^^xsd:string ;
    rdfs:domain wikidata:Q15632617,
        wikidata:Q5 ;
    rdfs:range wikidata:Q1047113,
        wikidata:Q11862829,
        wikidata:Q17376908,
        wikidata:Q1792379,
        wikidata:Q223393,
        wikidata:Q22684100,
        wikidata:Q336,
        wikidata:Q34379,
        wikidata:Q56055944,
        wikidata:Q62302889,
        wikidata:Q629206,
        wikidata:Q8434 .

wikidata:P822 rdfs:label "mascot"^^xsd:string ;
    rdfs:comment "mascot of an organization, e.g. a sports team or university"^^xsd:string ;
    rdfs:domain wikidata:Q167270,
        wikidata:Q18608583,
        wikidata:Q23807345,
        wikidata:Q2424752,
        wikidata:Q43229,
        wikidata:Q570116,
        wikidata:Q58778,
        wikidata:Q841654 ;
    rdfs:range wikidata:Q386208 .

wikidata:P823 rdfs:label "speaker"^^xsd:string ;
    rdfs:comment "person who is speaker for this event, ceremony, keynote, presentation or in a literary work"^^xsd:string ;
    rdfs:domain wikidata:Q1656682,
        wikidata:Q7725634 ;
    rdfs:range wikidata:Q21070568,
        wikidata:Q4271324,
        wikidata:Q5 ;
    rdfs:subPropertyOf wikidata:P710 .

wikidata:P825 rdfs:label "dedicated to"^^xsd:string ;
    rdfs:comment "person or organization to whom the subject was dedicated"^^xsd:string ;
    rdfs:domain wikidata:Q1656682,
        wikidata:Q488383 .

wikidata:P832 rdfs:label "public holiday"^^xsd:string ;
    rdfs:comment "official public holiday that occurs in this place in its honor, usually a non-working day"^^xsd:string ;
    rdfs:domain wikidata:Q1048835 ;
    rdfs:range wikidata:Q1197685,
        wikidata:Q1445650 ;
    rdfs:subPropertyOf wikidata:P793 .

wikidata:P833 a owl:SymmetricProperty ;
    rdfs:label "interchange station"^^xsd:string ;
    rdfs:comment "station to which passengers can transfer to from this station, normally without extra expense"^^xsd:string ;
    rdfs:domain wikidata:Q548662 ;
    rdfs:range wikidata:Q548662 .

wikidata:P837 rdfs:label "day in year for periodic occurrence"^^xsd:string ;
    rdfs:comment "when a specific holiday or periodic event occurs. Can be used as property or qualifier"^^xsd:string ;
    rdfs:range wikidata:Q14795564 .

wikidata:P84 rdfs:label "architect"^^xsd:string ;
    rdfs:comment "person or architectural firm responsible for designing this building"^^xsd:string ;
    rdfs:domain wikidata:Q123705,
        wikidata:Q1371819,
        wikidata:Q1497375,
        wikidata:Q22652,
        wikidata:Q294440,
        wikidata:Q811979 ;
    rdfs:range wikidata:Q16334295,
        wikidata:Q5 ;
    rdfs:subPropertyOf wikidata:P287 .

wikidata:P840 rdfs:label "narrative location"^^xsd:string ;
    rdfs:comment "the narrative of the work is set in this location"^^xsd:string ;
    rdfs:domain wikidata:Q1185607,
        wikidata:Q386724 ;
    rdfs:range wikidata:Q13226383,
        wikidata:Q14623646,
        wikidata:Q14637321,
        wikidata:Q1656682,
        wikidata:Q17334923,
        wikidata:Q18670171,
        wikidata:Q20203388,
        wikidata:Q24334893,
        wikidata:Q3895768,
        wikidata:Q4169,
        wikidata:Q47306921,
        wikidata:Q47495022,
        wikidata:Q618123,
        wikidata:Q82794 ;
    rdfs:subPropertyOf wikidata:P7153 .

wikidata:P841 rdfs:label "feast day"^^xsd:string ;
    rdfs:comment "saint's principal feast day"^^xsd:string ;
    rdfs:domain wikidata:Q13002315,
        wikidata:Q1509831,
        wikidata:Q16334295,
        wikidata:Q21070568,
        wikidata:Q22704077,
        wikidata:Q4818719,
        wikidata:Q5 .

wikidata:P85 rdfs:label "anthem"^^xsd:string ;
    rdfs:comment "subject's official anthem"^^xsd:string ;
    rdfs:range wikidata:Q207628 .

wikidata:P852 rdfs:label "ESRB rating"^^xsd:string ;
    rdfs:comment "North American video game content rating"^^xsd:string ;
    rdfs:domain wikidata:Q16070115,
        wikidata:Q620615,
        wikidata:Q65972034,
        wikidata:Q7889 ;
    rdfs:range wikidata:Q23683568 .

wikidata:P853 a owl:FunctionalProperty ;
    rdfs:label "CERO rating"^^xsd:string ;
    rdfs:comment "Japanese video game rating system - see talk page for appropriate values"^^xsd:string ;
    rdfs:domain wikidata:Q16070115,
        wikidata:Q209163,
        wikidata:Q7889 ;
    rdfs:range wikidata:Q23683472 .

wikidata:P859 rdfs:label "sponsor"^^xsd:string ;
    rdfs:comment "organization or individual that sponsors this item"^^xsd:string ;
    rdfs:range wikidata:Q1298668,
        wikidata:Q431289,
        wikidata:Q43229,
        wikidata:Q5,
        wikidata:Q6958747 .

wikidata:P86 rdfs:label "composer"^^xsd:string ;
    rdfs:comment "person(s) who wrote the music [for lyricist, use \"lyrics by\" (P676)]"^^xsd:string ;
    rdfs:domain wikidata:Q17489659,
        wikidata:Q386724 ;
    rdfs:range wikidata:Q10648343,
        wikidata:Q215380,
        wikidata:Q29881657,
        wikidata:Q5,
        wikidata:Q54982412,
        wikidata:Q59755569 ;
    rdfs:subPropertyOf wikidata:P170 .

wikidata:P87 rdfs:label "librettist"^^xsd:string ;
    rdfs:comment "author of the libretto (words) of an opera, operetta, oratorio or cantata, or of the book of a musical"^^xsd:string ;
    rdfs:domain wikidata:Q386724,
        wikidata:Q43099500 ;
    rdfs:range wikidata:Q15632617,
        wikidata:Q16334295,
        wikidata:Q5 ;
    rdfs:subPropertyOf wikidata:P50 .

wikidata:P870 rdfs:label "instrumentation"^^xsd:string ;
    rdfs:comment "combination of musical instruments employed in a composition or accompanying a (folk) dance"^^xsd:string ;
    rdfs:domain wikidata:Q105756498,
        wikidata:Q11639,
        wikidata:Q2188189,
        wikidata:Q6942560 ;
    rdfs:range wikidata:Q2088357,
        wikidata:Q34379 .

wikidata:P872 rdfs:label "printed by"^^xsd:string ;
    rdfs:comment "organization or person who printed the creative work (if different from \"publisher\")"^^xsd:string ;
    rdfs:domain wikidata:Q1002697,
        wikidata:Q11060274,
        wikidata:Q20655472,
        wikidata:Q3331189,
        wikidata:Q429785,
        wikidata:Q47433,
        wikidata:Q673383 ;
    rdfs:range wikidata:Q5,
        wikidata:Q6500733,
        wikidata:Q783794 .

wikidata:P88 rdfs:label "commissioned by"^^xsd:string ;
    rdfs:comment "person or organization that commissioned this work"^^xsd:string ;
    rdfs:domain wikidata:Q16686448,
        wikidata:Q170584,
        wikidata:Q17489659,
        wikidata:Q2424752,
        wikidata:Q386724 ;
    rdfs:range wikidata:Q43229,
        wikidata:Q5 .

wikidata:P880 rdfs:label "CPU"^^xsd:string ;
    rdfs:comment "central processing unit found within the subject item"^^xsd:string ;
    rdfs:domain wikidata:Q121117,
        wikidata:Q178648,
        wikidata:Q192525,
        wikidata:Q192851,
        wikidata:Q22645,
        wikidata:Q241317,
        wikidata:Q2858615,
        wikidata:Q4321,
        wikidata:Q68,
        wikidata:Q7889,
        wikidata:Q8076 ;
    rdfs:range wikidata:Q1466064,
        wikidata:Q5300,
        wikidata:Q80831 ;
    rdfs:subPropertyOf wikidata:P527 .

wikidata:P885 rdfs:label "origin of the watercourse"^^xsd:string ;
    rdfs:comment "main source of a river, stream or lake"^^xsd:string ;
    rdfs:domain wikidata:Q16338046,
        wikidata:Q23397,
        wikidata:Q271669,
        wikidata:Q355304 ;
    rdfs:range wikidata:Q15324,
        wikidata:Q17334923 .

wikidata:P908 rdfs:label "PEGI rating"^^xsd:string ;
    rdfs:comment "European video game content rating system - see talk page for appropriate values"^^xsd:string ;
    rdfs:domain wikidata:Q16070115,
        wikidata:Q209163,
        wikidata:Q4393107,
        wikidata:Q7397,
        wikidata:Q7889 ;
    rdfs:range wikidata:Q23686802 .

wikidata:P91 rdfs:label "sexual orientation"^^xsd:string ;
    rdfs:comment "the sexual orientation of the person — use IF AND ONLY IF they have stated it themselves, unambiguously, or it has been widely agreed upon by historians after their death"^^xsd:string ;
    rdfs:domain wikidata:Q201662,
        wikidata:Q21070598,
        wikidata:Q5,
        wikidata:Q95074 ;
    rdfs:range wikidata:Q17888 .

wikidata:P914 rdfs:label "USK rating"^^xsd:string ;
    rdfs:comment "German video game content rating - see talk page for appropriate values"^^xsd:string ;
    rdfs:domain wikidata:Q16070115,
        wikidata:Q209163,
        wikidata:Q620615,
        wikidata:Q65972034,
        wikidata:Q7889 ;
    rdfs:range wikidata:Q24561417 .

wikidata:P915 rdfs:label "filming location"^^xsd:string ;
    rdfs:comment "actual place where this scene/film was shot. For the setting, use \"narrative location\" (P840)"^^xsd:string ;
    rdfs:domain wikidata:Q11424,
        wikidata:Q15416,
        wikidata:Q1555508,
        wikidata:Q17558136,
        wikidata:Q1983062,
        wikidata:Q20742776,
        wikidata:Q20899,
        wikidata:Q24856,
        wikidata:Q34508,
        wikidata:Q3464665,
        wikidata:Q3895768,
        wikidata:Q5398426,
        wikidata:Q7889 ;
    rdfs:range wikidata:Q11446,
        wikidata:Q121359,
        wikidata:Q123705,
        wikidata:Q1415274,
        wikidata:Q15642541,
        wikidata:Q1656682,
        wikidata:Q17334923,
        wikidata:Q618123 ;
    rdfs:subPropertyOf wikidata:P8546 .

wikidata:P92 rdfs:label "main regulatory text"^^xsd:string ;
    rdfs:comment "text setting the main rules by which the subject is regulated"^^xsd:string ;
    rdfs:range wikidata:Q1864008,
        wikidata:Q2571972,
        wikidata:Q4122445,
        wikidata:Q428148,
        wikidata:Q45736416,
        wikidata:Q694045,
        wikidata:Q820655,
        wikidata:Q98491862 .

wikidata:P927 rdfs:label "anatomical location"^^xsd:string ;
    rdfs:comment "where in the body does this anatomical feature lie"^^xsd:string ;
    rdfs:domain wikidata:Q27043950,
        wikidata:Q2996394 ;
    rdfs:subPropertyOf wikidata:P276,
        wikidata:P361 .

wikidata:P930 rdfs:label "type of electrification"^^xsd:string ;
    rdfs:comment "electrification system scheme and/or voltage"^^xsd:string ;
    rdfs:domain wikidata:Q1067164,
        wikidata:Q1210334,
        wikidata:Q1311958,
        wikidata:Q1414135,
        wikidata:Q15141321,
        wikidata:Q18199879,
        wikidata:Q19832486,
        wikidata:Q211382,
        wikidata:Q22667,
        wikidata:Q2516436,
        wikidata:Q2678338,
        wikidata:Q29048322,
        wikidata:Q3491904,
        wikidata:Q3565868,
        wikidata:Q357685,
        wikidata:Q5639,
        wikidata:Q639030,
        wikidata:Q728937,
        wikidata:Q811704,
        wikidata:Q870 ;
    rdfs:range wikidata:Q23012297,
        wikidata:Q388201 .

wikidata:P931 rdfs:label "place served by transport hub"^^xsd:string ;
    rdfs:comment "territorial entity or entities served by this transport hub (airport, train station, etc.)"^^xsd:string ;
    rdfs:domain wikidata:Q376799 ;
    rdfs:range wikidata:Q1496967,
        wikidata:Q486972 ;
    rdfs:subPropertyOf wikidata:P7153 .

wikidata:P941 rdfs:label "inspired by"^^xsd:string ;
    rdfs:comment "work, human, place or event which inspired this creative work or fictional entity"^^xsd:string ;
    rdfs:domain wikidata:Q1190554,
        wikidata:Q15709879,
        wikidata:Q215380,
        wikidata:Q24334685,
        wikidata:Q386724,
        wikidata:Q483394 ;
    rdfs:range wikidata:Q1190554,
        wikidata:Q13002315,
        wikidata:Q15632617,
        wikidata:Q15706911,
        wikidata:Q16521,
        wikidata:Q16798631,
        wikidata:Q2061186,
        wikidata:Q20643955,
        wikidata:Q2088357,
        wikidata:Q215380,
        wikidata:Q223557,
        wikidata:Q24334685,
        wikidata:Q386724,
        wikidata:Q486972,
        wikidata:Q5,
        wikidata:Q618123,
        wikidata:Q74817647 .

wikidata:P943 rdfs:label "programmer"^^xsd:string ;
    rdfs:comment "the programmer that wrote the piece of software"^^xsd:string ;
    rdfs:domain wikidata:Q386724 .

wikidata:P944 a owl:FunctionalProperty ;
    rdfs:label "Code of nomenclature"^^xsd:string ;
    rdfs:comment "the Code that governs the scientific name of this taxon"^^xsd:string ;
    rdfs:domain wikidata:Q16521 .

wikidata:P945 rdfs:label "allegiance"^^xsd:string ;
    rdfs:comment "country (or other power) that the person or organization serves"^^xsd:string ;
    rdfs:domain wikidata:Q14623646,
        wikidata:Q43229,
        wikidata:Q5,
        wikidata:Q6857706,
        wikidata:Q95074 ;
    rdfs:range wikidata:Q1145276,
        wikidata:Q14623646,
        wikidata:Q176799,
        wikidata:Q3024240,
        wikidata:Q4164871,
        wikidata:Q43229,
        wikidata:Q6256,
        wikidata:Q6857706,
        wikidata:Q95074 .

wikidata:P97 rdfs:label "noble title"^^xsd:string ;
    rdfs:comment "titles held by the person"^^xsd:string ;
    rdfs:domain wikidata:Q13002315,
        wikidata:Q21070598,
        wikidata:Q5,
        wikidata:Q95074 ;
    rdfs:range wikidata:Q17468125,
        wikidata:Q3320743,
        wikidata:Q355567 .

wikidata:P972 rdfs:label "catalog"^^xsd:string ;
    rdfs:comment "catalog for the item, or, as a qualifier of P528 – catalog for which the 'catalog code' is valid"^^xsd:string ;
    rdfs:range wikidata:Q2352616,
        wikidata:Q36524 ;
    rdfs:subPropertyOf wikidata:P361 .

wikidata:P974 rdfs:label "tributary"^^xsd:string ;
    rdfs:comment "stream or river that flows into a larger river (for lake inflows use P200)"^^xsd:string ;
    rdfs:domain wikidata:Q16338046,
        wikidata:Q355304 ;
    rdfs:range wikidata:Q124714,
        wikidata:Q16338046,
        wikidata:Q355304 .

wikidata:P991 rdfs:label "successful candidate"^^xsd:string ;
    rdfs:comment "person(s) elected after the election"^^xsd:string ;
    rdfs:domain wikidata:Q40231 ;
    rdfs:range wikidata:Q5,
        wikidata:Q7210356 ;
    rdfs:subPropertyOf wikidata:P1346,
        wikidata:P726 .

() rdf:rest <http://www.semanticweb.org/ontologies/Wikidata#_:y10>,
        <http://www.semanticweb.org/ontologies/Wikidata#_:y12>,
        <http://www.semanticweb.org/ontologies/Wikidata#_:y14>,
        <http://www.semanticweb.org/ontologies/Wikidata#_:y2>,
        <http://www.semanticweb.org/ontologies/Wikidata#_:y4>,
        <http://www.semanticweb.org/ontologies/Wikidata#_:y6>,
        <http://www.semanticweb.org/ontologies/Wikidata#_:y8> .

wikidata:P1066 rdfs:label "student of"^^xsd:string ;
    rdfs:comment "person who has taught this person"^^xsd:string ;
    rdfs:domain wikidata:Q5,
        wikidata:Q95074 ;
    rdfs:range wikidata:Q16334295,
        wikidata:Q5,
        wikidata:Q95074 ;
    rdfs:subPropertyOf wikidata:P3342 .

wikidata:P1268 rdfs:label "represents"^^xsd:string ;
    rdfs:comment "organization, individual, or concept that an entity represents"^^xsd:string ;
    rdfs:range wikidata:Q1207505,
        wikidata:Q14514600,
        wikidata:Q14623646,
        wikidata:Q16334295,
        wikidata:Q34394,
        wikidata:Q35718073,
        wikidata:Q4042967,
        wikidata:Q43229,
        wikidata:Q48277,
        wikidata:Q5,
        wikidata:Q56061,
        wikidata:Q7397,
        wikidata:Q844569,
        wikidata:Q95074 .

wikidata:P129 a owl:IrreflexiveProperty ;
    rdfs:label "physically interacts with"^^xsd:string ;
    rdfs:comment "physical entity that the subject interacts with"^^xsd:string ;
    rdfs:domain wikidata:Q223557,
        wikidata:Q98119401 ;
    rdfs:range wikidata:Q223557,
        wikidata:Q98119401 .

wikidata:P1346 rdfs:label "winner"^^xsd:string ;
    rdfs:comment "winner of an event or an award; on award items use P166/P1346 on the item for the awarded work instead; do not use for wars or battles"^^xsd:string ;
    rdfs:domain wikidata:Q106594095,
        wikidata:Q13406554,
        wikidata:Q15707532,
        wikidata:Q18608583,
        wikidata:Q3464665,
        wikidata:Q618779,
        wikidata:Q841654 ;
    rdfs:range wikidata:Q15621286,
        wikidata:Q43229,
        wikidata:Q5,
        wikidata:Q5107,
        wikidata:Q6266,
        wikidata:Q726 ;
    rdfs:subPropertyOf wikidata:P710 .

wikidata:P135 rdfs:label "movement"^^xsd:string ;
    rdfs:comment "literary, artistic, scientific or philosophical movement or scene associated with this person or work"^^xsd:string ;
    rdfs:domain wikidata:Q16334295,
        wikidata:Q2668072,
        wikidata:Q386724,
        wikidata:Q5,
        wikidata:Q811979 ;
    rdfs:range wikidata:Q1387659,
        wikidata:Q16895642,
        wikidata:Q2198855,
        wikidata:Q23834194,
        wikidata:Q2738074,
        wikidata:Q28820001,
        wikidata:Q2915955,
        wikidata:Q3533467,
        wikidata:Q49773,
        wikidata:Q968159 .

wikidata:P1365 rdfs:label "replaces"^^xsd:string ;
    rdfs:comment "person, state or item replaced. Use \"structure replaces\" (P1398) for structures. Use \"follows\" (P155) if the previous item was not replaced or predecessor and successor are identical"^^xsd:string ;
    rdfs:subPropertyOf wikidata:P155 .

wikidata:P1366 rdfs:label "replaced by"^^xsd:string ;
    rdfs:comment "other person or item which continues the item by replacing it in its role. Use P156 (followed by) if the item is not replaced (e.g. books in a series), nor identical, but adds to the series without dropping the role of this item in that series"^^xsd:string ;
    rdfs:subPropertyOf wikidata:P156 .

wikidata:P1412 rdfs:label "languages spoken, written or signed"^^xsd:string ;
    rdfs:comment "language(s) that a person or a people speaks, writes or signs, including the native language(s)"^^xsd:string .

wikidata:P1416 rdfs:label "affiliation"^^xsd:string ;
    rdfs:comment "organization that a person or organization is affiliated with (not necessarily member of or employed by)"^^xsd:string ;
    rdfs:domain wikidata:Q14623646,
        wikidata:Q15831598,
        wikidata:Q16334295,
        wikidata:Q21192438,
        wikidata:Q24577840,
        wikidata:Q43229,
        wikidata:Q5,
        wikidata:Q95074 ;
    rdfs:range wikidata:Q13414953,
        wikidata:Q1370598,
        wikidata:Q14623646,
        wikidata:Q1664720,
        wikidata:Q16970,
        wikidata:Q170584,
        wikidata:Q1729207,
        wikidata:Q178706,
        wikidata:Q24577840,
        wikidata:Q43229,
        wikidata:Q56561355,
        wikidata:Q56670043,
        wikidata:Q62662717,
        wikidata:Q995347 ;
    rdfs:subPropertyOf wikidata:P361 .

wikidata:P1424 rdfs:label "topic's main template"^^xsd:string ;
    rdfs:comment "the main template relating to a topic"^^xsd:string ;
    rdfs:range wikidata:Q11266439 .

wikidata:P1535 rdfs:label "used by"^^xsd:string ;
    rdfs:comment "item or concept that makes use of the subject (use sub-properties when appropriate)"^^xsd:string .

wikidata:P1536 rdfs:label "immediate cause of"^^xsd:string ;
    rdfs:comment "immediate cause of this effect"^^xsd:string .

wikidata:P1542 rdfs:label "has effect"^^xsd:string ;
    rdfs:comment "effect of this item"^^xsd:string ;
    rdfs:subPropertyOf wikidata:P156 .

wikidata:P1547 a owl:AsymmetricProperty,
        owl:IrreflexiveProperty ;
    rdfs:label "depends on software"^^xsd:string ;
    rdfs:comment "subject software depends on object software"^^xsd:string ;
    rdfs:domain wikidata:Q7397 ;
    rdfs:range wikidata:Q7397 ;
    rdfs:subPropertyOf wikidata:P2283 .

wikidata:P1552 rdfs:label "has quality"^^xsd:string ;
    rdfs:comment "the entity has an inherent or distinguishing non-material characteristic"^^xsd:string .

wikidata:P1557 rdfs:label "manifestation of"^^xsd:string ;
    rdfs:comment "inherent and characteristic embodiment of a given concept"^^xsd:string ;
    rdfs:subPropertyOf wikidata:P1552 .

wikidata:P159 rdfs:label "headquarters location"^^xsd:string ;
    rdfs:comment "city, where an organization's headquarters is or has been situated. Use P276 qualifier for specific building"^^xsd:string .

wikidata:P17 rdfs:label "country"^^xsd:string ;
    rdfs:comment "sovereign state of this item (not to be used for human beings)"^^xsd:string .

wikidata:P176 rdfs:label "manufacturer"^^xsd:string ;
    rdfs:comment "manufacturer or producer of this product"^^xsd:string ;
    rdfs:range wikidata:Q1294787,
        wikidata:Q14514600,
        wikidata:Q28640,
        wikidata:Q43229,
        wikidata:Q5,
        wikidata:Q729,
        wikidata:Q95074 .

wikidata:P1830 rdfs:label "owner of"^^xsd:string ;
    rdfs:comment "entities owned by the subject"^^xsd:string ;
    rdfs:domain wikidata:Q43229,
        wikidata:Q5,
        wikidata:Q95074 ;
    rdfs:range wikidata:Q15401930,
        wikidata:Q43229,
        wikidata:Q4406616,
        wikidata:Q6671777 .

wikidata:P189 rdfs:label "location of discovery"^^xsd:string ;
    rdfs:comment "where the item was located when discovered"^^xsd:string ;
    rdfs:range wikidata:Q17334923,
        wikidata:Q27096213,
        wikidata:Q3895768 ;
    rdfs:subPropertyOf wikidata:P7153 .

wikidata:P2561 rdfs:label "name"^^xsd:string ;
    rdfs:comment "name the subject is known by. If a more specific property is available, use that"^^xsd:string .

wikidata:P2579 rdfs:label "studied by"^^xsd:string ;
    rdfs:comment "subject is studied by this science or domain or by this type of student"^^xsd:string ;
    rdfs:range wikidata:Q1047113,
        wikidata:Q48282 ;
    rdfs:subPropertyOf wikidata:P101 .

wikidata:P2828 rdfs:label "corporate officer"^^xsd:string ;
    rdfs:comment "person who holds a specific position"^^xsd:string .

wikidata:P287 rdfs:label "designed by"^^xsd:string ;
    rdfs:comment "person(s) or organization which designed the object"^^xsd:string ;
    rdfs:domain wikidata:Q10929058,
        wikidata:Q16686448 ;
    rdfs:range wikidata:Q12737077,
        wikidata:Q14623646,
        wikidata:Q16334295,
        wikidata:Q31855,
        wikidata:Q327245,
        wikidata:Q43229,
        wikidata:Q4830453,
        wikidata:Q5,
        wikidata:Q95074 ;
    rdfs:subPropertyOf wikidata:P170 .

wikidata:P2936 rdfs:label "language used"^^xsd:string ;
    rdfs:comment "language widely used (spoken or written) in this place or at this event"^^xsd:string ;
    rdfs:domain wikidata:Q103817,
        wikidata:Q1190554,
        wikidata:Q2944660,
        wikidata:Q37260,
        wikidata:Q3895768,
        wikidata:Q41710,
        wikidata:Q43229,
        wikidata:Q618123 ;
    rdfs:range wikidata:Q1208380,
        wikidata:Q25295,
        wikidata:Q2623733,
        wikidata:Q33384,
        wikidata:Q34770,
        wikidata:Q3953107 .

wikidata:P3174 rdfs:label "art director"^^xsd:string ;
    rdfs:comment "person credited as the art director/artistic director of this work"^^xsd:string ;
    rdfs:domain wikidata:Q386724 ;
    rdfs:range wikidata:Q5 .

wikidata:P3712 rdfs:label "objective of project or action"^^xsd:string ;
    rdfs:comment "desired result or outcome"^^xsd:string .

wikidata:P3729 rdfs:label "next lower rank"^^xsd:string ;
    rdfs:comment "lower rank or level in a ranked hierarchy like sport league, military ranks. If there are several possible, list each one and qualify with \"criterion used\" (P1013), avoid using ranks and date qualifiers. For sports leagues/taxa, use specific properties instead."^^xsd:string .

wikidata:P3730 rdfs:label "next higher rank"^^xsd:string ;
    rdfs:comment "higher rank or level in a ranked hierarchy like sport league, military ranks. If there are several possible, list each one and qualify with \"criterion used\" (P1013), avoid using ranks and date qualifiers. For sports leagues/taxa, use specific properties instead."^^xsd:string .

wikidata:P3931 rdfs:label "copyright holder"^^xsd:string ;
    rdfs:comment "person or organisation who holds the copyright of a work according to the Berne Convention"^^xsd:string ;
    rdfs:range wikidata:Q154954,
        wikidata:Q155076,
        wikidata:Q16334295,
        wikidata:Q43229 ;
    rdfs:subPropertyOf wikidata:P127 .

wikidata:P412 rdfs:label "voice type"^^xsd:string ;
    rdfs:comment "person's voice type. expected values: soprano, mezzo-soprano, contralto, countertenor, tenor, baritone, bass (and derivatives)"^^xsd:string ;
    rdfs:domain wikidata:Q1707847,
        wikidata:Q5,
        wikidata:Q95074 ;
    rdfs:range wikidata:Q1063547 .

wikidata:P4688 rdfs:label "geomorphological unit"^^xsd:string ;
    rdfs:comment "topographic or bathymetric feature to which this geographical item belongs"^^xsd:string .

wikidata:P485 rdfs:label "archives at"^^xsd:string ;
    rdfs:comment "the institution holding the subject's archives"^^xsd:string ;
    rdfs:range wikidata:Q43229,
        wikidata:Q5 ;
    rdfs:subPropertyOf wikidata:P7153 .

wikidata:P551 rdfs:label "residence"^^xsd:string ;
    rdfs:comment "the place where the person is or has been, resident"^^xsd:string ;
    rdfs:domain wikidata:Q14514600,
        wikidata:Q16334295,
        wikidata:Q20643955,
        wikidata:Q21070568,
        wikidata:Q4271324,
        wikidata:Q4671277,
        wikidata:Q5,
        wikidata:Q57812559,
        wikidata:Q622852,
        wikidata:Q729,
        wikidata:Q95074 ;
    rdfs:range wikidata:Q1497375,
        wikidata:Q2221906,
        wikidata:Q24334893,
        wikidata:Q27096213,
        wikidata:Q3895768,
        wikidata:Q3947,
        wikidata:Q41176,
        wikidata:Q699405,
        wikidata:Q82794,
        wikidata:Q837142 ;
    rdfs:subPropertyOf wikidata:P276 .

wikidata:P726 rdfs:label "candidate"^^xsd:string ;
    rdfs:comment "person or party that is an option for an office in this election"^^xsd:string ;
    rdfs:domain wikidata:Q11642595,
        wikidata:Q19571328,
        wikidata:Q40231,
        wikidata:Q847301 ;
    rdfs:range wikidata:Q22137478,
        wikidata:Q5,
        wikidata:Q7210356,
        wikidata:Q99659193 ;
    rdfs:subPropertyOf wikidata:P710 .

wikidata:P7604 rdfs:label "supervised by"^^xsd:string ;
    rdfs:comment "Is the natural person who has the authority of giving instructions and/or orders to subordinates and is held responsible for the work and actions of subordinates."^^xsd:string .

wikidata:P790 rdfs:label "approved by"^^xsd:string ;
    rdfs:comment "item is approved by other item(s) [qualifier: statement is approved by other item(s)]"^^xsd:string ;
    rdfs:range wikidata:Q16334295,
        wikidata:Q4164871,
        wikidata:Q5 .

wikidata:P793 rdfs:label "significant event"^^xsd:string ;
    rdfs:comment "significant or notable events associated with the subject"^^xsd:string ;
    rdfs:domain wikidata:Q35120 ;
    rdfs:range wikidata:Q1190554,
        wikidata:Q14136353,
        wikidata:Q1656682,
        wikidata:Q171558,
        wikidata:Q24336466,
        wikidata:Q26907166 .

wikidata:P828 rdfs:label "has cause"^^xsd:string ;
    rdfs:comment "underlying cause, thing that ultimately resulted in this effect"^^xsd:string ;
    rdfs:subPropertyOf wikidata:P155 .

wikidata:P831 a owl:AsymmetricProperty,
        owl:IrreflexiveProperty ;
    rdfs:label "parent club"^^xsd:string ;
    rdfs:comment "parent club of this team"^^xsd:string ;
    rdfs:domain wikidata:Q12973014,
        wikidata:Q847017 ;
    rdfs:range wikidata:Q12973014,
        wikidata:Q847017 .

wikidata:P912 rdfs:label "has facility"^^xsd:string ;
    rdfs:comment "the subject item has this type of facility, e.g. toilet, car park"^^xsd:string ;
    rdfs:domain wikidata:Q13226383,
        wikidata:Q14623646,
        wikidata:Q17334923,
        wikidata:Q182676,
        wikidata:Q22698,
        wikidata:Q33506,
        wikidata:Q3895768,
        wikidata:Q41176,
        wikidata:Q43229,
        wikidata:Q867393 ;
    rdfs:subPropertyOf wikidata:P2670 .

wikidata:P921 rdfs:label "main subject"^^xsd:string ;
    rdfs:comment "primary topic of a work (see also P180: depicts)"^^xsd:string .

wikidata:P98 rdfs:label "editor"^^xsd:string ;
    rdfs:comment "editor of a compiled work such as a book or a periodical (newspaper or an academic journal)"^^xsd:string ;
    rdfs:domain wikidata:Q1002697,
        wikidata:Q105420,
        wikidata:Q192283,
        wikidata:Q2985386,
        wikidata:Q3331189,
        wikidata:Q386724,
        wikidata:Q41298 ;
    rdfs:range wikidata:Q43229,
        wikidata:Q5 .

wikidata:Q1004 rdfs:label "comics"^^xsd:string ;
    rdfs:comment "creative work in which pictures and text convey information such as narratives"^^xsd:string ;
    rdfs:subClassOf wikidata:Q47461344,
        wikidata:Q7725634 .

wikidata:Q100775361 rdfs:label "Wikimedia list of musical works by composer"^^xsd:string ;
    rdfs:comment "subclass of Wikimedia list of musical works"^^xsd:string .

wikidata:Q100775856 rdfs:label "Wikimedia list of dramatico-musical works by composer"^^xsd:string ;
    rdfs:comment "subclass of Wikimedia list of dramatico-musical works"^^xsd:string .

wikidata:Q101002748 rdfs:label "drinking can"^^xsd:string ;
    rdfs:comment "container used in the storage, packaging, and shipping of non-alcoholic beverage"^^xsd:string .

wikidata:Q101191533 rdfs:label "online catalog"^^xsd:string ;
    rdfs:comment "каталог, доступ до якого здійснюється через Інтернет"^^xsd:string ;
    rdfs:subClassOf wikidata:Q2352616 .

wikidata:Q10286227 rdfs:label "religious fundamentalism"^^xsd:string ;
    rdfs:comment "interpretazione letterale dogmatica di testi sacri"^^xsd:string .

wikidata:Q104526 rdfs:label "pipe"^^xsd:string ;
    rdfs:comment "tool specifically made to smoke tobacco or other products"^^xsd:string ;
    rdfs:subClassOf wikidata:Q39546 .

wikidata:Q104696061 rdfs:label "Wikibooks page"^^xsd:string ;
    rdfs:comment "page in a Wikibook"^^xsd:string ;
    rdfs:subClassOf wikidata:Q17537576 .

wikidata:Q1047698 rdfs:label "superpower"^^xsd:string ;
    rdfs:comment "superhuman ability of a fictional character"^^xsd:string ;
    rdfs:subClassOf wikidata:Q14897293 .

wikidata:Q104934 rdfs:label "fundamental interaction"^^xsd:string ;
    rdfs:comment "any of the physical interactions or forces: gravitational, electromagnetic, strong nuclear, and weak nuclear"^^xsd:string ;
    rdfs:subClassOf wikidata:Q1293220 .

wikidata:Q105072162 rdfs:label "Catholic archdiocese not metropolitan"^^xsd:string ;
    rdfs:comment "Catholic diocese that due to its importance is headed by an archbishop, but has no suffragan diocese"^^xsd:string .

wikidata:Q105390172 rdfs:label "roman catholic metropolitan archdiocese"^^xsd:string ;
    rdfs:comment "Archdiocese of the Roman Catholic Church that has a suffragan diocese under its jurisdiction"^^xsd:string ;
    rdfs:subClassOf wikidata:Q2665272,
        wikidata:Q427961 .

wikidata:Q10553309 rdfs:label "legislative house"^^xsd:string ;
    rdfs:comment "deliberative assembly acting as part of a legislature"^^xsd:string .

wikidata:Q105575966 rdfs:label "traditional melody"^^xsd:string ;
    rdfs:comment "melody with anonymous or unknown composer without authorized original version; melody that is part of a musical tradition"^^xsd:string .

wikidata:Q105731 rdfs:label "lock"^^xsd:string ;
    rdfs:comment "device for raising and lowering boats or ships"^^xsd:string ;
    rdfs:subClassOf wikidata:Q12284 .

wikidata:Q105756498 rdfs:label "type of musical group"^^xsd:string ;
    rdfs:comment "type of musical group or band, defined by genre, by instrumentation, or some other criteria"^^xsd:string .

wikidata:Q1058236 rdfs:label "administrative act"^^xsd:string ;
    rdfs:comment "acte administratif est un acte juridique fait dans le cadre de l'administration"^^xsd:string ;
    rdfs:subClassOf wikidata:Q1864008 .

wikidata:Q105858921 rdfs:label "extension de mémoire externe"^^xsd:string ;
    rdfs:comment "support électronique pour logiciels"^^xsd:string .

wikidata:Q105985 rdfs:label "judiciary"^^xsd:string ;
    rdfs:comment "system of courts that interprets and applies the law"^^xsd:string .

wikidata:Q106046707 rdfs:label "VR experience"^^xsd:string ;
    rdfs:comment "immersive experience taking advantage of virtual reality"^^xsd:string .

wikidata:Q1061151 rdfs:label "massif"^^xsd:string ;
    rdfs:comment "section of a planet's crust that is demarcated by faults or flexures"^^xsd:string ;
    rdfs:subClassOf wikidata:Q271669 .

wikidata:Q1061197 rdfs:label "radio network"^^xsd:string ;
    rdfs:comment "type of audio-only broadcast network"^^xsd:string ;
    rdfs:subClassOf wikidata:Q4830453 .

wikidata:Q106594809 rdfs:label "music competition class"^^xsd:string ;
    rdfs:comment "classification of participants in a music competition used to qualify entries"^^xsd:string .

wikidata:Q10673035 rdfs:label "specification"^^xsd:string ;
    rdfs:comment "technical standard, explicit set of requirements to be satisfied by a software"^^xsd:string .

wikidata:Q10753560 rdfs:label "scientific name"^^xsd:string ;
    rdfs:comment "scientific name used in the study of biology or in the study of botany"^^xsd:string .

wikidata:Q1079693 rdfs:label "national emblem"^^xsd:string ;
    rdfs:comment "emblem or seal reserved for use by a nation state or multi-national state as a symbol of that nation"^^xsd:string .

wikidata:Q108149 rdfs:label "nuclide"^^xsd:string ;
    rdfs:comment "atomic species characterized by the specific constitution of its nucleus"^^xsd:string .

wikidata:Q10822464 rdfs:label "angel in Christianity"^^xsd:string ;
    rdfs:comment "view on angels in Christian tradition"^^xsd:string .

wikidata:Q10832 rdfs:label "sex doll"^^xsd:string ;
    rdfs:comment "anthropomorphic sexual device"^^xsd:string ;
    rdfs:subClassOf wikidata:Q168658 .

wikidata:Q1087471 rdfs:label "relic associated with Jesus"^^xsd:string ;
    rdfs:comment "reliquies cristianes sobre Xesucristu, oxetu de veneración"^^xsd:string .

wikidata:Q10884 rdfs:label "tree"^^xsd:string ;
    rdfs:comment "perennial woody plant"^^xsd:string .

wikidata:Q10927834 rdfs:label "laterality"^^xsd:string ;
    rdfs:comment "preference most humans show for one side of their body over the other"^^xsd:string .

wikidata:Q11060274 rdfs:label "print"^^xsd:string ;
    rdfs:comment "work of art printed from a block or plate"^^xsd:string ;
    rdfs:subClassOf wikidata:Q3331189 .

wikidata:Q11177771 rdfs:label "artistic technique"^^xsd:string ;
    rdfs:comment "method by which art is produced"^^xsd:string .

wikidata:Q11197007 rdfs:label "ethnoreligious group"^^xsd:string ;
    rdfs:comment "ethnic group of people whose members are also unified by a common religious background"^^xsd:string ;
    rdfs:subClassOf wikidata:Q41710,
        wikidata:Q4392985 .

wikidata:Q1128397 rdfs:label "convent"^^xsd:string ;
    rdfs:comment "religious community"^^xsd:string ;
    rdfs:subClassOf wikidata:Q44613 .

wikidata:Q1137109 rdfs:label "video game publisher"^^xsd:string ;
    rdfs:comment "group or corporation that publishes a developer's video games"^^xsd:string ;
    rdfs:subClassOf wikidata:Q4830453 .

wikidata:Q11379 rdfs:label "energy"^^xsd:string ;
    rdfs:comment "measure for the ability of a system to do work"^^xsd:string .

wikidata:Q11396960 rdfs:label "production company"^^xsd:string ;
    rdfs:comment "company producing works in the realms of the performing arts, media art, film, radio, and video"^^xsd:string ;
    rdfs:subClassOf wikidata:Q1331793,
        wikidata:Q783794 .

wikidata:Q1140371 rdfs:label "national identification number"^^xsd:string ;
    rdfs:comment "number used by a country for its residents"^^xsd:string .

wikidata:Q11460 rdfs:label "clothing"^^xsd:string ;
    rdfs:comment "covering worn on the human body"^^xsd:string ;
    rdfs:subClassOf wikidata:Q223557,
        wikidata:Q2424752,
        wikidata:Q28877,
        wikidata:Q386724 .

wikidata:Q11514315 rdfs:label "historical period"^^xsd:string ;
    rdfs:comment "segment of time in history"^^xsd:string .

wikidata:Q1156741 rdfs:label "Time Lord"^^xsd:string ;
    rdfs:comment "fictional alien species"^^xsd:string ;
    rdfs:subClassOf wikidata:Q2590445,
        wikidata:Q28020127 .

wikidata:Q116 rdfs:label "monarch"^^xsd:string ;
    rdfs:comment "person at the head of a monarchy"^^xsd:string ;
    rdfs:subClassOf wikidata:Q4164871,
        wikidata:Q48352 .

wikidata:Q11651 rdfs:label "electric current"^^xsd:string ;
    rdfs:comment "flow of electric charge (for specific quantities see Q29996 or Q234072)"^^xsd:string .

wikidata:Q11664239 rdfs:label "music unit"^^xsd:string ;
    rdfs:comment "type of musical group in Japan"^^xsd:string ;
    rdfs:subClassOf wikidata:Q16334295 .

wikidata:Q1168287 rdfs:label "intervention"^^xsd:string ;
    rdfs:comment "use of force by one country or sovereign state in the internal or external affairs of another"^^xsd:string .

wikidata:Q11691 rdfs:label "stock exchange"^^xsd:string ;
    rdfs:comment "organization that provides services for stock brokers and traders to trade securities"^^xsd:string .

wikidata:Q1174599 rdfs:label "attack"^^xsd:string ;
    rdfs:comment "action to injure another organism"^^xsd:string .

wikidata:Q1174791 rdfs:label "escarpment"^^xsd:string ;
    rdfs:comment "type of slope landform"^^xsd:string ;
    rdfs:subClassOf wikidata:Q271669 .

wikidata:Q1184244 rdfs:label "delict"^^xsd:string ;
    rdfs:comment "civil wrong"^^xsd:string ;
    rdfs:subClassOf wikidata:Q24962887 .

wikidata:Q11921029 rdfs:label "music style"^^xsd:string ;
    rdfs:comment "characteristic uses of instrumentation, production, and musical ideas to fit within a genre"^^xsd:string ;
    rdfs:subClassOf wikidata:Q1292119 .

wikidata:Q1193246 rdfs:label "widget toolkit"^^xsd:string ;
    rdfs:comment "framework or toolkit a program uses to display the graphical user interface"^^xsd:string .

wikidata:Q1196123 rdfs:label "military uniform"^^xsd:string ;
    rdfs:comment "standardised dress worn by members of the armed forces and paramilitaries of various nations"^^xsd:string .

wikidata:Q11976958 rdfs:label "illegal newspaper"^^xsd:string ;
    rdfs:comment "avis som blir fremstilt og distribuert i hemmelighet"^^xsd:string .

wikidata:Q121117 rdfs:label "supercomputer"^^xsd:string ;
    rdfs:comment "extremely powerful computer for its era"^^xsd:string ;
    rdfs:subClassOf wikidata:Q68 .

wikidata:Q121182 rdfs:label "information system"^^xsd:string ;
    rdfs:comment "combination of information, resources, activities and people that support tasks in an organization; group of components that interact to produce information"^^xsd:string ;
    rdfs:subClassOf wikidata:Q2424752,
        wikidata:Q58778 .

wikidata:Q121438 rdfs:label "transposable element"^^xsd:string ;
    rdfs:comment "semiparasitic DNA sequence"^^xsd:string .

wikidata:Q1231729 rdfs:label "contrada of Siena"^^xsd:string ;
    rdfs:comment "historical subdivision of the city of Siena"^^xsd:string .

wikidata:Q1238720 rdfs:label "volume"^^xsd:string ;
    rdfs:comment "book in a series, typically identified sequentially (e.g. Volume 3)"^^xsd:string ;
    rdfs:subClassOf wikidata:Q3331189,
        wikidata:Q571 .

wikidata:Q12404340 rdfs:label "biblical place"^^xsd:string ;
    rdfs:comment "place mentioned in the Bible"^^xsd:string .

wikidata:Q12410555 rdfs:label "shooting attack"^^xsd:string ;
    rdfs:comment "form of firearms-related violence"^^xsd:string .

wikidata:Q1243409 rdfs:label "heraldic attitude"^^xsd:string ;
    rdfs:comment "orientation and pose of a creature in heraldry"^^xsd:string ;
    rdfs:subClassOf wikidata:Q834104 .

wikidata:Q124490 rdfs:label "violence"^^xsd:string ;
    rdfs:comment "use of physical force or power with the intent to inflict harm"^^xsd:string ;
    rdfs:subClassOf wikidata:Q1914636 .

wikidata:Q1249682 rdfs:label "editio princeps"^^xsd:string ;
    rdfs:comment "in classical scholarship, first printed edition of the work, that previously had existed only in manuscripts"^^xsd:string ;
    rdfs:subClassOf wikidata:Q3331189 .

wikidata:Q1251403 rdfs:label "alleyway"^^xsd:string ;
    rdfs:comment "narrow street"^^xsd:string ;
    rdfs:subClassOf wikidata:Q79007 .

wikidata:Q1254874 rdfs:label "television network"^^xsd:string ;
    rdfs:comment "telecommunications network for distribution of television program content"^^xsd:string .

wikidata:Q12743 rdfs:label "ford"^^xsd:string ;
    rdfs:comment "crossing in a river"^^xsd:string ;
    rdfs:subClassOf wikidata:Q34442 .

wikidata:Q1278335 rdfs:label "instrumentalist"^^xsd:string ;
    rdfs:comment "person who plays a musical instrument"^^xsd:string .

wikidata:Q127843 rdfs:label "pen name"^^xsd:string ;
    rdfs:comment "pseudonym adopted by an author (or a group of authors) and printed on the title page in place of their real name"^^xsd:string ;
    rdfs:subClassOf wikidata:Q201662,
        wikidata:Q61002 .

wikidata:Q12796 rdfs:label "firearm"^^xsd:string ;
    rdfs:comment "gun designed to be carried and operated by individuals"^^xsd:string .

wikidata:Q12798556 rdfs:label "personal parish"^^xsd:string ;
    rdfs:comment "Catholic parish not tied to a parish-like territory"^^xsd:string ;
    rdfs:subClassOf wikidata:Q17143723 .

wikidata:Q12804010 rdfs:label "territorial parish"^^xsd:string ;
    rdfs:comment "Catholic parish with a territory"^^xsd:string ;
    rdfs:subClassOf wikidata:Q17143723,
        wikidata:Q20926517 .

wikidata:Q128093 rdfs:label "e-book"^^xsd:string ;
    rdfs:comment "book-length publication in digital form"^^xsd:string ;
    rdfs:subClassOf wikidata:Q3331189,
        wikidata:Q571 .

wikidata:Q128234 rdfs:label "case"^^xsd:string ;
    rdfs:comment "grammatical category whose value reflects the grammatical function performed by a noun or pronoun in a phrase, clause, or sentence"^^xsd:string .

wikidata:Q1287097 rdfs:label "cable ferry"^^xsd:string ;
    rdfs:comment "ship type"^^xsd:string ;
    rdfs:subClassOf wikidata:Q25653 .

wikidata:Q12909644 rdfs:label "political ideology"^^xsd:string ;
    rdfs:comment "ideology that advocates social, political and economic organization of human life"^^xsd:string ;
    rdfs:subClassOf wikidata:Q7257 .

wikidata:Q1294787 rdfs:label "artisan"^^xsd:string ;
    rdfs:comment "skilled craft worker who makes or creates things by hand"^^xsd:string .

wikidata:Q1307214 rdfs:label "form of government"^^xsd:string ;
    rdfs:comment "organisational model of government"^^xsd:string .

wikidata:Q130788 rdfs:label "chronology"^^xsd:string ;
    rdfs:comment "science of arranging events in their order of occurrence in time"^^xsd:string ;
    rdfs:subClassOf wikidata:Q336 .

wikidata:Q1310239 rdfs:label "component"^^xsd:string ;
    rdfs:comment "smaller, self-contained part of technical entity consisting of components"^^xsd:string .

wikidata:Q1311958 rdfs:label "railway tunnel"^^xsd:string ;
    rdfs:comment "tunnel built for rail traffic"^^xsd:string ;
    rdfs:subClassOf wikidata:Q1311670,
        wikidata:Q44377,
        wikidata:Q728937 .

wikidata:Q131436 rdfs:label "board game"^^xsd:string ;
    rdfs:comment "game that involves counters or pieces moved or placed on a pre-marked surface or \"board\", according to a set of rules"^^xsd:string .

wikidata:Q1323212 rdfs:label "insurgency"^^xsd:string ;
    rdfs:comment "armed rebellion against a constituted authority when those taking part in the rebellion are not recognized as belligerents"^^xsd:string ;
    rdfs:subClassOf wikidata:Q124734 .

wikidata:Q132814 rdfs:label "evaporation"^^xsd:string ;
    rdfs:comment "type of vaporization of a liquid that occurs from its surface; surface phenomenon"^^xsd:string .

wikidata:Q133004 rdfs:label "diaspora"^^xsd:string ;
    rdfs:comment "dispersion of ethnic communities"^^xsd:string .

wikidata:Q133250 rdfs:label "sequence"^^xsd:string ;
    rdfs:comment "ordered list of elements (finite or infinite)"^^xsd:string ;
    rdfs:subClassOf wikidata:Q20937557 .

wikidata:Q1335818 rdfs:label "supranational union"^^xsd:string ;
    rdfs:comment "international organisation with power and influence in the jurisdictions of its member states"^^xsd:string ;
    rdfs:subClassOf wikidata:Q484652 .

wikidata:Q134219 rdfs:label "polysaccharides"^^xsd:string ;
    rdfs:comment "long chain of polymeric carbohydrate modules"^^xsd:string .

wikidata:Q1350310 rdfs:label "administrative territorial entity of the Philippines"^^xsd:string ;
    rdfs:comment "subdivisión territorial de Filipinas"^^xsd:string ;
    rdfs:subClassOf wikidata:Q1048835 .

wikidata:Q1351368 rdfs:label "archive file format"^^xsd:string ;
    rdfs:comment "file that is composed of one or more computer files along with metadata; used to collect multiple data files together into a single file for easier portability and storage, or simply to compress files to use less storage space"^^xsd:string ;
    rdfs:subClassOf wikidata:Q235557 .

wikidata:Q13522376 rdfs:label "Classic Mac OS"^^xsd:string ;
    rdfs:comment "original operating system of Apple Mac (1984–2001)"^^xsd:string .

wikidata:Q1363750 rdfs:label "chair"^^xsd:string ;
    rdfs:comment "named and usually endowed university professorship"^^xsd:string ;
    rdfs:subClassOf wikidata:Q81752537 .

wikidata:Q1366112 rdfs:label "television drama"^^xsd:string ;
    rdfs:comment "television genre"^^xsd:string ;
    rdfs:subClassOf wikidata:Q15416 .

wikidata:Q1371849 rdfs:label "filmography"^^xsd:string ;
    rdfs:comment "list of films related by some criteria"^^xsd:string ;
    rdfs:subClassOf wikidata:Q1631107 .

wikidata:Q1378139 rdfs:label "robotic spacecraft"^^xsd:string ;
    rdfs:comment "uncrewed spacecraft, usually under telerobotic control"^^xsd:string ;
    rdfs:subClassOf wikidata:Q11012 .

wikidata:Q1406 rdfs:label "Microsoft Windows"^^xsd:string ;
    rdfs:comment "family of operating systems produced for personal computers, servers, smartphones and embedded devices"^^xsd:string .

wikidata:Q14116 rdfs:label "macOS"^^xsd:string ;
    rdfs:comment "operating system for Apple computers, launched in 2001 as Mac OS X"^^xsd:string .

wikidata:Q1412386 rdfs:label "fictional brand"^^xsd:string ;
    rdfs:comment "fictional product, created for movies or TV"^^xsd:string ;
    rdfs:subClassOf wikidata:Q15706911 .

wikidata:Q1414991 rdfs:label "area"^^xsd:string ;
    rdfs:comment "country subdivision"^^xsd:string ;
    rdfs:subClassOf wikidata:Q1496967 .

wikidata:Q14208553 rdfs:label "invention"^^xsd:string ;
    rdfs:comment "unique or novel device, method, composition or process"^^xsd:string ;
    rdfs:subClassOf wikidata:Q1656682,
        wikidata:Q6958747 .

wikidata:Q1424805 rdfs:label "charge"^^xsd:string ;
    rdfs:comment "heraldic motif; an ordinary, common charge or symbol"^^xsd:string ;
    rdfs:subClassOf wikidata:Q80071 .

wikidata:Q1431554 rdfs:label "apostolic administration"^^xsd:string ;
    rdfs:comment "structure ecclésiastique"^^xsd:string ;
    rdfs:subClassOf wikidata:Q1492823 .

wikidata:Q1437459 rdfs:label "non-geologically related mountain range"^^xsd:string ;
    rdfs:comment "geographic area containing numerous mountains, not necessarily geologically related to each other"^^xsd:string ;
    rdfs:subClassOf wikidata:Q46831,
        wikidata:Q82794 .

wikidata:Q1441762 rdfs:label "aspect ratio"^^xsd:string ;
    rdfs:comment "proportion between the width and the height of an image"^^xsd:string ;
    rdfs:subClassOf wikidata:Q20970434 .

wikidata:Q1458444 rdfs:label "noncoding DNA"^^xsd:string ;
    rdfs:comment "DNA not coding for protein. Often translated to RNA and critical in regulating other genes"^^xsd:string .

wikidata:Q14623351 rdfs:label "radio series"^^xsd:string ;
    rdfs:comment "recurring show on radio"^^xsd:string ;
    rdfs:subClassOf wikidata:Q1555508 .

wikidata:Q14660 rdfs:label "flag"^^xsd:string ;
    rdfs:comment "piece of fabric with a distinctive design, used as a symbol"^^xsd:string ;
    rdfs:subClassOf wikidata:Q17335294 .

wikidata:Q1479965 rdfs:label "Blessed Virgin Mary of El Pilar"^^xsd:string ;
    rdfs:comment "title of the Virgin Mary"^^xsd:string .

wikidata:Q14860489 rdfs:label "molecular function"^^xsd:string ;
    rdfs:comment "Elemental activities, such as catalysis or binding, describing the actions of a gene product at the molecular level. A given gene product may exhibit one or more molecular functions."^^xsd:string .

wikidata:Q149377 rdfs:label "military operation plan"^^xsd:string ;
    rdfs:comment "formal plan for military armed forces"^^xsd:string ;
    rdfs:subClassOf wikidata:Q1371819 .

wikidata:Q15042037 rdfs:label "statistical territorial entity"^^xsd:string ;
    rdfs:comment "areas designated as significant due to high population density, economic activity, or other reasons"^^xsd:string ;
    rdfs:subClassOf wikidata:Q15642541 .

wikidata:Q15057021 rdfs:label "engine model"^^xsd:string ;
    rdfs:comment "specific engine design"^^xsd:string ;
    rdfs:subClassOf wikidata:Q10929058,
        wikidata:Q2424752 .

wikidata:Q150784 rdfs:label "canyon"^^xsd:string ;
    rdfs:comment "deep ravine between cliffs"^^xsd:string .

wikidata:Q15079786 rdfs:label "ballet"^^xsd:string ;
    rdfs:comment "theatre work that uses ballet dancing"^^xsd:string ;
    rdfs:subClassOf wikidata:Q58483088 .

wikidata:Q15097084 rdfs:label "heritage register"^^xsd:string ;
    rdfs:comment "register listing items having heritage value"^^xsd:string ;
    rdfs:subClassOf wikidata:Q2352616,
        wikidata:Q8513 .

wikidata:Q15142894 rdfs:label "weapon model"^^xsd:string ;
    rdfs:comment "specific weapon design, pattern, or version of which all examples are essentially identical"^^xsd:string ;
    rdfs:subClassOf wikidata:Q10929058 .

wikidata:Q15169167 rdfs:label "execution method"^^xsd:string ;
    rdfs:comment "method to carry out execution"^^xsd:string ;
    rdfs:subClassOf wikidata:Q1799072,
        wikidata:Q1931388 .

wikidata:Q15184295 rdfs:label "Wikimedia module"^^xsd:string ;
    rdfs:comment "use with 'instance of' (P31) for modules written in Lua, and working with the Scribunto extension for MediaWiki installed on a Wikimedia wiki"^^xsd:string .

wikidata:Q1520311 rdfs:label "violent crime"^^xsd:string ;
    rdfs:comment "crime in which an offender uses or threatens force upon a victim"^^xsd:string ;
    rdfs:subClassOf wikidata:Q83267 .

wikidata:Q152416 rdfs:label "samizdat"^^xsd:string ;
    rdfs:comment "key form of dissident activity across the Soviet bloc in which individuals reproduced censored and underground publications by hand and passed the documents from reader to reader"^^xsd:string ;
    rdfs:subClassOf wikidata:Q732577,
        wikidata:Q8242 .

wikidata:Q15243209 rdfs:label "historic district"^^xsd:string ;
    rdfs:comment "section of a city which contains older buildings considered valuable for historical or architectural reasons"^^xsd:string ;
    rdfs:subClassOf wikidata:Q15642541 .

wikidata:Q1531518 rdfs:label "military ordinariate"^^xsd:string ;
    rdfs:comment "Catholic ecclesiastical jurisdiction providing religious services for armed forces"^^xsd:string ;
    rdfs:subClassOf wikidata:Q2665272 .

wikidata:Q1539532 rdfs:label "sports season of a sports club"^^xsd:string ;
    rdfs:comment "activity of a sports club during the portion of one year in which regulated games of a sport are played as part of a league or other multi match tournament"^^xsd:string ;
    rdfs:subClassOf wikidata:Q27020041 .

wikidata:Q1544071 rdfs:label "narrows (landform)"^^xsd:string ;
    rdfs:comment "route constricted by natural features"^^xsd:string ;
    rdfs:subClassOf wikidata:Q271669 .

wikidata:Q15524954 rdfs:label "voice banking"^^xsd:string ;
    rdfs:comment "recording of one's natural voice for future reproduction"^^xsd:string .

wikidata:Q15690029 rdfs:label "fictional educational institution"^^xsd:string ;
    rdfs:comment "educational institution existing only in fictional story"^^xsd:string ;
    rdfs:subClassOf wikidata:Q14623646,
        wikidata:Q14897293,
        wikidata:Q15720793 .

wikidata:Q1572600 rdfs:label "proclamation"^^xsd:string ;
    rdfs:comment "official declaration"^^xsd:string ;
    rdfs:subClassOf wikidata:Q15621286,
        wikidata:Q49848 .

wikidata:Q15773317 rdfs:label "television character"^^xsd:string ;
    rdfs:comment "fictional character who appears in a television series or web series"^^xsd:string ;
    rdfs:subClassOf wikidata:Q95074 .

wikidata:Q15893266 rdfs:label "former entity"^^xsd:string ;
    rdfs:comment "entity that no longer operates or is terminated"^^xsd:string ;
    rdfs:subClassOf wikidata:Q35120 .

wikidata:Q15900616 rdfs:label "event sequence"^^xsd:string ;
    rdfs:comment "coherent series of individual events, shows, gatherings, performances etc. under organisational continuity"^^xsd:string ;
    rdfs:subClassOf wikidata:Q15275719 .

wikidata:Q1595289 rdfs:label "sacred mountain"^^xsd:string ;
    rdfs:comment "mountains are central to certain religions and are the subjects of many legends"^^xsd:string ;
    rdfs:subClassOf wikidata:Q4588528,
        wikidata:Q8502 .

wikidata:Q15978876 rdfs:label "canonization status"^^xsd:string ;
    rdfs:comment "stage in the process of attaining sainthood"^^xsd:string .

wikidata:Q160598 rdfs:label "heresy"^^xsd:string ;
    rdfs:comment "belief or theory that is strongly at variance with established beliefs or customs"^^xsd:string ;
    rdfs:subClassOf wikidata:Q117850 .

wikidata:Q160738 rdfs:label "role-playing game"^^xsd:string ;
    rdfs:comment "game in which players assume the roles of characters in a fictional setting. Use Tabletop role-playing game (Q1643932) for the leasure activity."^^xsd:string ;
    rdfs:subClassOf wikidata:Q11410 .

wikidata:Q160742 rdfs:label "abbey"^^xsd:string ;
    rdfs:comment "monastery or convent, under the authority of an abbot or an abbess"^^xsd:string ;
    rdfs:subClassOf wikidata:Q44613 .

wikidata:Q16145150 rdfs:label "music pedagogue"^^xsd:string ;
    rdfs:comment "profession and academic title"^^xsd:string ;
    rdfs:subClassOf wikidata:Q2675537 .

wikidata:Q1621273 rdfs:label "particle"^^xsd:string ;
    rdfs:comment "small localized object in physical sciences"^^xsd:string ;
    rdfs:subClassOf wikidata:Q223557 .

wikidata:Q1630279 rdfs:label "guideline"^^xsd:string ;
    rdfs:comment "instruction as to the preferred, recommended, or approved way of performing a task"^^xsd:string ;
    rdfs:subClassOf wikidata:Q1151067 .

wikidata:Q163740 rdfs:label "nonprofit organization"^^xsd:string ;
    rdfs:comment "organization that uses its income to achieve its goals rather than distributing it as profit or dividends"^^xsd:string ;
    rdfs:subClassOf wikidata:Q43229 .

wikidata:Q165044 rdfs:label "greenhouse"^^xsd:string ;
    rdfs:comment "building in which plants are grown"^^xsd:string ;
    rdfs:subClassOf wikidata:Q811979 .

wikidata:Q16560 rdfs:label "palace"^^xsd:string ;
    rdfs:comment "grand residence, especially a royal residence or the home of a head of state"^^xsd:string ;
    rdfs:subClassOf wikidata:Q41176 .

wikidata:Q16631188 rdfs:label "military position"^^xsd:string ;
    rdfs:comment "assignment of a person's place in a military organization defining responsibilities and privileges"^^xsd:string ;
    rdfs:subClassOf wikidata:Q4164871 .

wikidata:Q1668024 rdfs:label "service on internet"^^xsd:string ;
    rdfs:comment "technical ability afforded by the internet"^^xsd:string ;
    rdfs:subClassOf wikidata:Q340169 .

wikidata:Q167346 rdfs:label "botanical garden"^^xsd:string ;
    rdfs:comment "well-tended area displaying a wide range of plants labelled with their botanical names"^^xsd:string ;
    rdfs:subClassOf wikidata:Q1030034,
        wikidata:Q13226383,
        wikidata:Q22652,
        wikidata:Q31855 .

wikidata:Q16859021 rdfs:label "cemetery, burial plot, or tomb"^^xsd:string ;
    rdfs:comment "specific place of burial for a human or animal, to be used with coordinate qualifier"^^xsd:string ;
    rdfs:subClassOf wikidata:Q27096235 .

wikidata:Q16895642 rdfs:label "philosophical school"^^xsd:string ;
    rdfs:comment "school of thought within philosophy"^^xsd:string ;
    rdfs:subClassOf wikidata:Q1387659 .

wikidata:Q168983 rdfs:label "conflagration"^^xsd:string ;
    rdfs:comment "large and destructive fire that threatens human life, animal life, health, and/or property"^^xsd:string .

wikidata:Q169872 rdfs:label "symptom"^^xsd:string ;
    rdfs:comment "departure from normal function or feeling which is noticed by a patient, reflecting the presence of an unusual state, or of a disease; subjective, observed by the patient, cannot be measured directly"^^xsd:string ;
    rdfs:subClassOf wikidata:Q2057971,
        wikidata:Q7189713 .

wikidata:Q170434 rdfs:label "DOS"^^xsd:string ;
    rdfs:comment "group of closely-related PC-compatible operating systems"^^xsd:string ;
    rdfs:subClassOf wikidata:Q600659 .

wikidata:Q17099416 rdfs:label "Wikimedia list of songs"^^xsd:string ;
    rdfs:comment "page on a Wikimedia project with a list of songs"^^xsd:string .

wikidata:Q1714375 rdfs:label "game reserve"^^xsd:string ;
    rdfs:comment "entity reserved for game"^^xsd:string ;
    rdfs:subClassOf wikidata:Q473972,
        wikidata:Q82794 .

wikidata:Q171441 rdfs:label "enclave"^^xsd:string ;
    rdfs:comment "territory entirely surrounded by another territory"^^xsd:string .

wikidata:Q17146139 rdfs:label "Wikimedia route diagram"^^xsd:string ;
    rdfs:comment "старонка ў праекце Вікімэдыі, дзе прадстаўленая схема трасы"^^xsd:string .

wikidata:Q17172850 rdfs:label "voice"^^xsd:string ;
    rdfs:comment "human voice as musical instrument"^^xsd:string ;
    rdfs:subClassOf wikidata:Q34379 .

wikidata:Q17199338 rdfs:label "fictional continent"^^xsd:string ;
    rdfs:comment "continent that only exists in fictional works"^^xsd:string ;
    rdfs:subClassOf wikidata:Q3895768 .

wikidata:Q17272482 rdfs:label "time zone named for a UTC offset"^^xsd:string ;
    rdfs:comment "iluciones creativas"^^xsd:string ;
    rdfs:subClassOf wikidata:Q12143 .

wikidata:Q172847 rdfs:label "peptide"^^xsd:string ;
    rdfs:comment "natural biological or artificially manufactured short chains of amino acid monomers linked by peptide (amide) bonds"^^xsd:string .

wikidata:Q173227 rdfs:label "physical constant"^^xsd:string ;
    rdfs:comment "physical quantity that is generally believed to be both universal in nature and constant in time"^^xsd:string .

wikidata:Q173387 rdfs:label "grave"^^xsd:string ;
    rdfs:comment "location where one dead person or a limited amount of people are buried"^^xsd:string .

wikidata:Q17468125 rdfs:label "political function in fiction"^^xsd:string ;
    rdfs:comment "political function, as depicted in works of fiction"^^xsd:string ;
    rdfs:subClassOf wikidata:Q21451536 .

wikidata:Q174782 rdfs:label "square"^^xsd:string ;
    rdfs:comment "open public spaces in cities or towns, usually rectilinear, surrounded by buildings, and often located at the junction of two or more thoroughfares"^^xsd:string ;
    rdfs:subClassOf wikidata:Q294440,
        wikidata:Q811979,
        wikidata:Q83620 .

wikidata:Q1748957 rdfs:label "Fach"^^xsd:string ;
    rdfs:comment "method of classifying singers according to the range, weight, and color of their voices"^^xsd:string ;
    rdfs:subClassOf wikidata:Q1063547,
        wikidata:Q1707847 .

wikidata:Q1750705 rdfs:label "asteroid spectral type"^^xsd:string ;
    rdfs:comment "classification type of a class of objects"^^xsd:string .

wikidata:Q1751626 rdfs:label "theatre festival"^^xsd:string ;
    rdfs:comment "type of arts festival"^^xsd:string ;
    rdfs:subClassOf wikidata:Q4801521 .

wikidata:Q17518557 rdfs:label "collection of articles"^^xsd:string ;
    rdfs:comment "group of articles published in a periodical under the same collective name"^^xsd:string ;
    rdfs:subClassOf wikidata:Q105420 .

wikidata:Q1753139 rdfs:label "electric power source"^^xsd:string ;
    rdfs:comment "equipment or engine which provides electrical energy"^^xsd:string ;
    rdfs:subClassOf wikidata:Q1522115 .

wikidata:Q17558136 rdfs:label "YouTube channel"^^xsd:string ;
    rdfs:comment "user channel on YouTube"^^xsd:string ;
    rdfs:subClassOf wikidata:Q17489659 .

wikidata:Q1756157 rdfs:label "area of law"^^xsd:string ;
    rdfs:comment "branch of law focused on a specific subject"^^xsd:string .

wikidata:Q175854 rdfs:label "phobia"^^xsd:string ;
    rdfs:comment "an anxiety disorder defined by a persistent and excessive fear of an object or situation"^^xsd:string .

wikidata:Q17589470 rdfs:label "home video game console"^^xsd:string ;
    rdfs:comment "type of video game console that can only be used stationary"^^xsd:string ;
    rdfs:subClassOf wikidata:Q8076 .

wikidata:Q1763090 rdfs:label "sentence"^^xsd:string ;
    rdfs:comment "decree of punishment in law"^^xsd:string .

wikidata:Q17737 rdfs:label "theory"^^xsd:string ;
    rdfs:comment "contemplative and rational type of abstract or generalizing thinking, or the results of such thinking"^^xsd:string ;
    rdfs:subClassOf wikidata:Q151885 .

wikidata:Q1777301 rdfs:label "standard time"^^xsd:string ;
    rdfs:comment "synchronization of clocks within a geographical area or region"^^xsd:string .

wikidata:Q1777515 rdfs:label "junction"^^xsd:string ;
    rdfs:comment "location where traffic can change between different routes, directions, or sometimes modes, of travel"^^xsd:string ;
    rdfs:subClassOf wikidata:Q2221906,
        wikidata:Q83620 .

wikidata:Q1778235 rdfs:label "territorial abbey"^^xsd:string ;
    rdfs:comment "It is a territorially delimited particular church, whose attention is entrusted to a prelate or an abbot, who governs it as its own pastor, in the same way as a diocesan bishop"^^xsd:string ;
    rdfs:subClassOf wikidata:Q105388829 .

wikidata:Q1778821 rdfs:label "cuisine"^^xsd:string ;
    rdfs:comment "characteristic style of cooking practices and traditions"^^xsd:string ;
    rdfs:subClassOf wikidata:Q11042 .

wikidata:Q1784096 rdfs:label "flight of locks"^^xsd:string ;
    rdfs:comment "series of locks in close proximity"^^xsd:string ;
    rdfs:subClassOf wikidata:Q12284,
        wikidata:Q18247357,
        wikidata:Q58778 .

wikidata:Q178651 rdfs:label "interview"^^xsd:string ;
    rdfs:comment "structured series of questions and answers"^^xsd:string ;
    rdfs:subClassOf wikidata:Q15621286 .

wikidata:Q17888 rdfs:label "sexual orientation"^^xsd:string ;
    rdfs:comment "enduring pattern of sexual attraction"^^xsd:string ;
    rdfs:subClassOf wikidata:Q4042967 .

wikidata:Q1789476 rdfs:label "bibliographic database"^^xsd:string ;
    rdfs:comment "database providing an authoritative source of bibliographic information"^^xsd:string ;
    rdfs:subClassOf wikidata:Q2352616 .

wikidata:Q1802587 rdfs:label "German public state broadcaster"^^xsd:string ;
    rdfs:comment "gruppo di enti radiotelevisivi pubblici regionali tedeschi"^^xsd:string .

wikidata:Q180856 rdfs:label "choreography"^^xsd:string ;
    rdfs:comment "art of arranging movements"^^xsd:string .

wikidata:Q18086706 rdfs:label "themselves"^^xsd:string ;
    rdfs:comment "to be used with \"character role\" (P453)"^^xsd:string ;
    rdfs:subClassOf wikidata:Q15773347,
        wikidata:Q1707847 .

wikidata:Q18131152 rdfs:label "round"^^xsd:string ;
    rdfs:comment "part of a race that spans multiple days"^^xsd:string ;
    rdfs:subClassOf wikidata:Q878123 .

wikidata:Q181916 rdfs:label "herbarium"^^xsd:string ;
    rdfs:comment "scientific collection of dried plants"^^xsd:string .

wikidata:Q181947 rdfs:label "crossbow"^^xsd:string ;
    rdfs:comment "type of ranged weapon based on the bow"^^xsd:string .

wikidata:Q18199879 rdfs:label "trolleybus system"^^xsd:string ;
    rdfs:comment "system of trolleybuses travelling the streets of a town"^^xsd:string .

wikidata:Q182676 rdfs:label "mountain hut"^^xsd:string ;
    rdfs:comment "building located in the mountains"^^xsd:string ;
    rdfs:subClassOf wikidata:Q41176 .

wikidata:Q182832 rdfs:label "concert"^^xsd:string ;
    rdfs:comment "live performance of music"^^xsd:string ;
    rdfs:subClassOf wikidata:Q6942562 .

wikidata:Q18325582 rdfs:label "fictional military rank"^^xsd:string ;
    rdfs:comment "military rank that exists only in fiction"^^xsd:string ;
    rdfs:subClassOf wikidata:Q21451536 .

wikidata:Q18327510 rdfs:label "fictional robot"^^xsd:string ;
    rdfs:comment "robot which only exists in fiction"^^xsd:string ;
    rdfs:subClassOf wikidata:Q11012,
        wikidata:Q95074 .

wikidata:Q183888 rdfs:label "software developer"^^xsd:string ;
    rdfs:comment "person or company concerned with facets of the software development process"^^xsd:string .

wikidata:Q18390875 rdfs:label "Rock shed"^^xsd:string ;
    rdfs:comment "beskyttelse mot steinskred"^^xsd:string .

wikidata:Q185785 rdfs:label "ammunition"^^xsd:string ;
    rdfs:comment "general term for a wide range of weapon items such as bombs, missiles, mines and projectiles"^^xsd:string ;
    rdfs:subClassOf wikidata:Q728,
        wikidata:Q8205328 .

wikidata:Q18596079 rdfs:label "fictional medical condition"^^xsd:string ;
    rdfs:comment "medical condition that only exists in fictional works"^^xsd:string ;
    rdfs:subClassOf wikidata:Q14897293 .

wikidata:Q186117 rdfs:label "timeline"^^xsd:string ;
    rdfs:comment "way of displaying a list of events in chronological order"^^xsd:string .

wikidata:Q186361 rdfs:label "punishment"^^xsd:string ;
    rdfs:comment "imposition of an undesirable or unpleasant outcome as a response and deterrent to an action or behaviour that is deemed undesirable or unacceptable"^^xsd:string .

wikidata:Q187616 rdfs:label "relic"^^xsd:string ;
    rdfs:comment "ancient religious object preserved for purposes of veneration"^^xsd:string .

wikidata:Q187685 rdfs:label "doctoral thesis"^^xsd:string ;
    rdfs:comment "document submitted in support of candidature for a doctorate"^^xsd:string ;
    rdfs:subClassOf wikidata:Q1266946 .

wikidata:Q187947 rdfs:label "score"^^xsd:string ;
    rdfs:comment "full musical score showing each part on a separate line or staff"^^xsd:string ;
    rdfs:subClassOf wikidata:Q4327689,
        wikidata:Q49848 .

wikidata:Q188055 rdfs:label "siege"^^xsd:string ;
    rdfs:comment "military blockade of a city or fortress"^^xsd:string .

wikidata:Q1880737 rdfs:label "branch office"^^xsd:string ;
    rdfs:comment "outlet of a company or an organization that – unlike a subsidiary (Q658255) – does not constitute a separate legal entity, while being physically separated from the organization's main office"^^xsd:string ;
    rdfs:subClassOf wikidata:Q334453 .

wikidata:Q188451 rdfs:label "music genre"^^xsd:string ;
    rdfs:comment "category that identifies pieces of music as belonging to a shared tradition or set of conventions"^^xsd:string ;
    rdfs:subClassOf wikidata:Q1792379 .

wikidata:Q188784 rdfs:label "superhero"^^xsd:string ;
    rdfs:comment "type of stock character usually possessing \"supernatural or superhuman powers\" and dedicated to protecting the public"^^xsd:string .

wikidata:Q188976 rdfs:label "counterculture"^^xsd:string ;
    rdfs:comment "subculture whose values and norms of behavior deviate from those of mainstream society"^^xsd:string ;
    rdfs:subClassOf wikidata:Q264965 .

wikidata:Q1891817 rdfs:label "industrial spur"^^xsd:string ;
    rdfs:comment "Schienenweg zur Erschließung eines Geländes oder Gebäudes, das selbst nicht zur Eisenbahninfrastruktur gehört, durch Eisenbahngleise zum Gütertransport"^^xsd:string ;
    rdfs:subClassOf wikidata:Q728937 .

wikidata:Q18948595 rdfs:label "fictional thoroughfare"^^xsd:string ;
    rdfs:comment "thoroughfare that is made up for fictional stories, and does not exist in real life"^^xsd:string ;
    rdfs:subClassOf wikidata:Q3895768 .

wikidata:Q189533 rdfs:label "academic degree"^^xsd:string ;
    rdfs:comment "college or university diploma"^^xsd:string .

wikidata:Q190 rdfs:label "God"^^xsd:string ;
    rdfs:comment "principal object of faith in monotheistic religions; a divine entity that supervises all existence"^^xsd:string ;
    rdfs:subClassOf wikidata:Q178885,
        wikidata:Q215627 .

wikidata:Q190122 rdfs:label "promissory note"^^xsd:string ;
    rdfs:comment "negotiable instrument, wherein one party makes an unconditional promise in writing to pay a determinate sum of money to the other"^^xsd:string .

wikidata:Q190399 rdfs:label "pamphlet"^^xsd:string ;
    rdfs:comment "unbound booklet containing text"^^xsd:string ;
    rdfs:subClassOf wikidata:Q18602566,
        wikidata:Q49848,
        wikidata:Q732577 .

wikidata:Q1907875 rdfs:label "master's thesis"^^xsd:string ;
    rdfs:comment "thesis submitted in support of candidature for a master's degree"^^xsd:string ;
    rdfs:subClassOf wikidata:Q1266946 .

wikidata:Q191072 rdfs:label "cadastre"^^xsd:string ;
    rdfs:comment "comprehensive register of the real estate or real property's metes-and-bounds of a country"^^xsd:string ;
    rdfs:subClassOf wikidata:Q36524,
        wikidata:Q4006 .

wikidata:Q192283 rdfs:label "news agency"^^xsd:string ;
    rdfs:comment "news gathering organization"^^xsd:string ;
    rdfs:subClassOf wikidata:Q11032,
        wikidata:Q1331793 .

wikidata:Q192525 rdfs:label "workstation"^^xsd:string ;
    rdfs:comment "high-end computer designed for technical or scientific applications"^^xsd:string ;
    rdfs:subClassOf wikidata:Q68 .

wikidata:Q192909 rdfs:label "scandal"^^xsd:string ;
    rdfs:comment "widely publicized damaging allegations triggering the outrage of public opinion"^^xsd:string ;
    rdfs:subClassOf wikidata:Q180684 .

wikidata:Q19307174 rdfs:label "digital distribution platform"^^xsd:string ;
    rdfs:comment "platform for distributing and managing software"^^xsd:string ;
    rdfs:subClassOf wikidata:Q7397 .

wikidata:Q193291 rdfs:label "spirit"^^xsd:string ;
    rdfs:comment "immaterial being"^^xsd:string ;
    rdfs:subClassOf wikidata:Q15619164,
        wikidata:Q4271324 .

wikidata:Q193977 rdfs:label "music video"^^xsd:string ;
    rdfs:comment "short film integrating a song and imagery"^^xsd:string ;
    rdfs:subClassOf wikidata:Q2188189,
        wikidata:Q34508 .

wikidata:Q194195 rdfs:label "amusement park"^^xsd:string ;
    rdfs:comment "park with rides and attractions"^^xsd:string ;
    rdfs:subClassOf wikidata:Q43229,
        wikidata:Q570116 .

wikidata:Q19476593 rdfs:label "police rank"^^xsd:string ;
    rdfs:comment "element of hierarchy in law enforcement"^^xsd:string ;
    rdfs:subClassOf wikidata:Q4120621,
        wikidata:Q4164871 .

wikidata:Q19537 rdfs:label "bonobo"^^xsd:string ;
    rdfs:comment "one of two species in the genus Pan, along with the chimpanzee"^^xsd:string .

wikidata:Q1971694 rdfs:label "game mode"^^xsd:string ;
    rdfs:comment "variant of a computer game"^^xsd:string .

wikidata:Q19791817 rdfs:label "fictional noble family"^^xsd:string ;
    rdfs:comment "noble family only appearing in works of fiction"^^xsd:string ;
    rdfs:subClassOf wikidata:Q15331236 .

wikidata:Q19832486 rdfs:label "locomotive class"^^xsd:string ;
    rdfs:comment "locomotive type"^^xsd:string ;
    rdfs:subClassOf wikidata:Q29048322,
        wikidata:Q811704 .

wikidata:Q19847637 rdfs:label "Wikidata property for an identifier"^^xsd:string ;
    rdfs:comment "Wikidata property to identify something in an external source"^^xsd:string ;
    rdfs:subClassOf wikidata:Q18616576 .

wikidata:Q19850234 rdfs:label "hill group"^^xsd:string ;
    rdfs:comment "group of hills"^^xsd:string ;
    rdfs:subClassOf wikidata:Q16887380 .

wikidata:Q199414 rdfs:label "bog body"^^xsd:string ;
    rdfs:comment "corpse conserved in a bog"^^xsd:string .

wikidata:Q1995395 rdfs:label "Digipak"^^xsd:string ;
    rdfs:comment "trademark; patented type of optical disc packaging"^^xsd:string ;
    rdfs:subClassOf wikidata:Q63367831 .

wikidata:Q200334 rdfs:label "bell tower"^^xsd:string ;
    rdfs:comment "a tower that contains one or more bells, or that is designed to hold bells"^^xsd:string ;
    rdfs:subClassOf wikidata:Q12518 .

wikidata:Q20045456 rdfs:label "political position"^^xsd:string ;
    rdfs:comment "a person or organization's view on a particular political subject"^^xsd:string .

wikidata:Q20180855 rdfs:label "train ferry route"^^xsd:string ;
    rdfs:comment "ferry route where railway cars are transported inside the ferry during trip"^^xsd:string ;
    rdfs:subClassOf wikidata:Q15141321,
        wikidata:Q18984099 .

wikidata:Q20203388 rdfs:label "extremity"^^xsd:string ;
    rdfs:comment "endpoint or starting point; most extreme point in a set by a given measure"^^xsd:string .

wikidata:Q20642011 rdfs:label "guerrilla movement"^^xsd:string ;
    rdfs:comment "military organization practicing irregular warfare against a larger and less-mobile traditional military"^^xsd:string .

wikidata:Q20671152 rdfs:label "dialect family"^^xsd:string ;
    rdfs:comment ""^^xsd:string ;
    rdfs:subClassOf wikidata:Q25295 .

wikidata:Q207326 rdfs:label "summit"^^xsd:string ;
    rdfs:comment "point on a surface that is higher in elevation than all points immediately adjacent to it, in topography"^^xsd:string ;
    rdfs:subClassOf wikidata:Q2221906,
        wikidata:Q271669 .

wikidata:Q20742776 rdfs:label "video artwork"^^xsd:string ;
    rdfs:comment "video art piece"^^xsd:string ;
    rdfs:subClassOf wikidata:Q2431196 .

wikidata:Q207869 rdfs:label "epithet"^^xsd:string ;
    rdfs:comment "descriptive term"^^xsd:string .

wikidata:Q208145 rdfs:label "iconography"^^xsd:string ;
    rdfs:comment "branch of art history"^^xsd:string .

wikidata:Q20819922 rdfs:label "opera company"^^xsd:string ;
    rdfs:comment "company that produces and stages operas"^^xsd:string ;
    rdfs:subClassOf wikidata:Q16334295,
        wikidata:Q43229 .

wikidata:Q20888711 rdfs:label "camera product line"^^xsd:string ;
    rdfs:comment ""^^xsd:string ;
    rdfs:subClassOf wikidata:Q811701 .

wikidata:Q20899 rdfs:label "podcasting"^^xsd:string ;
    rdfs:comment "type of digital media"^^xsd:string ;
    rdfs:subClassOf wikidata:Q2431196 .

wikidata:Q210167 rdfs:label "video game developer"^^xsd:string ;
    rdfs:comment "group or corporation that develops video games"^^xsd:string ;
    rdfs:subClassOf wikidata:Q12737077 .

wikidata:Q210980 rdfs:label "virtual community"^^xsd:string ;
    rdfs:comment "social network of individuals who interact through specific social media"^^xsd:string ;
    rdfs:subClassOf wikidata:Q177634 .

wikidata:Q2110808 rdfs:label "religious behaviour"^^xsd:string ;
    rdfs:comment "behaviour motivated by religious belief"^^xsd:string .

wikidata:Q211364 rdfs:label "principle"^^xsd:string ;
    rdfs:comment "guiding rule or inevitable consequence of something, such as the laws observed in nature"^^xsd:string ;
    rdfs:subClassOf wikidata:Q1151067,
        wikidata:Q6671777 .

wikidata:Q211382 rdfs:label "High-speed rail"^^xsd:string ;
    rdfs:comment "significantly faster advanced rail transport & tech-enhanced infrastructure systems"^^xsd:string ;
    rdfs:subClassOf wikidata:Q3565868 .

wikidata:Q21211206 rdfs:label "payload"^^xsd:string ;
    rdfs:comment "mission load on a space vehicle"^^xsd:string .

wikidata:Q21286623 rdfs:label "fictional political faction"^^xsd:string ;
    rdfs:comment "political faction which only exists works of fiction"^^xsd:string ;
    rdfs:subClassOf wikidata:Q14623646 .

wikidata:Q2135465 rdfs:label "legal concept"^^xsd:string ;
    rdfs:comment "lexeme with a specific meaning in jurisprudence"^^xsd:string ;
    rdfs:subClassOf wikidata:Q151885 .

wikidata:Q214519 rdfs:label "track gauge"^^xsd:string ;
    rdfs:comment "spacing of the rails on a railway track"^^xsd:string .

wikidata:Q215292 rdfs:label "AC power connector"^^xsd:string ;
    rdfs:comment "power connector used to connect appliances to mains power"^^xsd:string .

wikidata:Q216866 rdfs:label "conjoined twins"^^xsd:string ;
    rdfs:comment "identical twins joined in utero"^^xsd:string .

wikidata:Q22006653 rdfs:label "color"^^xsd:string ;
    rdfs:comment "filmed in color, the opposite of black-and-white"^^xsd:string .

wikidata:Q220505 rdfs:label "film festival"^^xsd:string ;
    rdfs:comment "event with films being shown"^^xsd:string ;
    rdfs:subClassOf wikidata:Q4801521 .

wikidata:Q2207288 rdfs:label "craft"^^xsd:string ;
    rdfs:comment "pastime that requires particular skills and knowledge of skilled work"^^xsd:string ;
    rdfs:subClassOf wikidata:Q1914636 .

wikidata:Q22137478 rdfs:label "presidential ticket"^^xsd:string ;
    rdfs:comment "set of two people running for a presidential election, as president and vice-president"^^xsd:string ;
    rdfs:subClassOf wikidata:Q10648343 .

wikidata:Q222910 rdfs:label "compilation album"^^xsd:string ;
    rdfs:comment "music album made by combining previously made tracks"^^xsd:string ;
    rdfs:subClassOf wikidata:Q105420,
        wikidata:Q482994 .

wikidata:Q223371 rdfs:label "stock market index"^^xsd:string ;
    rdfs:comment "measures a stock market to help investors compare stock prices"^^xsd:string .

wikidata:Q223729 rdfs:label "white paper"^^xsd:string ;
    rdfs:comment "authoritative report that provides information about a specific issue"^^xsd:string ;
    rdfs:subClassOf wikidata:Q49848 .

wikidata:Q2240474 rdfs:label "Norse clan"^^xsd:string ;
    rdfs:comment "Scandanavian lineage"^^xsd:string ;
    rdfs:subClassOf wikidata:Q1517820,
        wikidata:Q211503 .

wikidata:Q22645 rdfs:label "smartphone"^^xsd:string ;
    rdfs:comment "multi-purpose mobile device"^^xsd:string ;
    rdfs:subClassOf wikidata:Q11253473 .

wikidata:Q22661286 rdfs:label "Flatpak"^^xsd:string ;
    rdfs:comment "system for application virtualization"^^xsd:string .

wikidata:Q22675015 rdfs:label "type of quantum particle"^^xsd:string ;
    rdfs:comment "type or family of quantum mechanical particles, often subatomic but also may be unrelated to atoms"^^xsd:string .

wikidata:Q22684100 rdfs:label "Muhaddith"^^xsd:string ;
    rdfs:comment "Scholar of hadith"^^xsd:string .

wikidata:Q22704077 rdfs:label "biblical episode"^^xsd:string ;
    rdfs:comment "story, narrated in the Bible"^^xsd:string ;
    rdfs:subClassOf wikidata:Q1406161 .

wikidata:Q22746 rdfs:label "urban park"^^xsd:string ;
    rdfs:comment "park in a city or other incorporated place"^^xsd:string ;
    rdfs:subClassOf wikidata:Q22698,
        wikidata:Q294440 .

wikidata:Q2281788 rdfs:label "public aquarium"^^xsd:string ;
    rdfs:comment "facility with large tanks for water-dwelling species"^^xsd:string ;
    rdfs:subClassOf wikidata:Q43501,
        wikidata:Q570116 .

wikidata:Q2288631 rdfs:label "archeparchy"^^xsd:string ;
    rdfs:comment "similar a archidiócesis pero en las iglesias orientales, ortodoxa y católica"^^xsd:string ;
    rdfs:subClassOf wikidata:Q1492823,
        wikidata:Q285181,
        wikidata:Q51041800 .

wikidata:Q22911714 rdfs:label "bowling style"^^xsd:string ;
    rdfs:comment "bir kriket oyuncusu tarafından kullanılan bowling türü"^^xsd:string .

wikidata:Q22938576 rdfs:label "race"^^xsd:string ;
    rdfs:comment "competitive event in which participants attempt to complete objectives as fast as possible"^^xsd:string ;
    rdfs:subClassOf wikidata:Q16510064 .

wikidata:Q22950320 rdfs:label "collective head of state"^^xsd:string ;
    rdfs:comment "head of state that is a group rather than a person"^^xsd:string ;
    rdfs:subClassOf wikidata:Q43229 .

wikidata:Q23012297 rdfs:label "type of electricity transmission"^^xsd:string ;
    rdfs:comment ""^^xsd:string .

wikidata:Q231002 rdfs:label "nationality"^^xsd:string ;
    rdfs:comment "a legal identification of a person in international law, establishing the person as a subject, a national, of a sovereign state"^^xsd:string ;
    rdfs:subClassOf wikidata:Q41710 .

wikidata:Q2332332 rdfs:label "minor-planet group"^^xsd:string ;
    rdfs:comment "population of minor planets that share broadly similar orbits"^^xsd:string ;
    rdfs:subClassOf wikidata:Q6999 .

wikidata:Q2333552 rdfs:label "hatchery"^^xsd:string ;
    rdfs:comment "facility for incubating and hatching animals"^^xsd:string ;
    rdfs:subClassOf wikidata:Q13226383 .

wikidata:Q23397 rdfs:label "lake"^^xsd:string ;
    rdfs:comment "body of relatively still water, localized in a basin"^^xsd:string ;
    rdfs:subClassOf wikidata:Q271669,
        wikidata:Q337567 .

wikidata:Q23442 rdfs:label "island"^^xsd:string ;
    rdfs:comment "sub-continental land that is surrounded by water"^^xsd:string ;
    rdfs:subClassOf wikidata:Q271669 .

wikidata:Q234870 rdfs:label "optical disc"^^xsd:string ;
    rdfs:comment "flat, usually circular disc which encodes binary data"^^xsd:string ;
    rdfs:subClassOf wikidata:Q1048236 .

wikidata:Q23649978 rdfs:label "Kijkwijzer rating category"^^xsd:string ;
    rdfs:comment "single rating in the Kijkwijzer rating system"^^xsd:string ;
    rdfs:subClassOf wikidata:Q23649976 .

wikidata:Q23660208 rdfs:label "MPAA classification category"^^xsd:string ;
    rdfs:comment "single classification in the Motion Picture of America film rating system"^^xsd:string ;
    rdfs:subClassOf wikidata:Q23649976 .

wikidata:Q23683425 rdfs:label "NMHH rating category"^^xsd:string ;
    rdfs:comment "single rating in the NMHH rating system"^^xsd:string ;
    rdfs:subClassOf wikidata:Q23649976 .

wikidata:Q23683472 rdfs:label "CERO rating category"^^xsd:string ;
    rdfs:comment "single category of the CERO content rating system"^^xsd:string ;
    rdfs:subClassOf wikidata:Q23649976 .

wikidata:Q23683568 rdfs:label "ESRB rating category"^^xsd:string ;
    rdfs:comment ""^^xsd:string ;
    rdfs:subClassOf wikidata:Q23649976 .

wikidata:Q23686802 rdfs:label "PEGI rating category"^^xsd:string ;
    rdfs:comment "single rating category in PEGI"^^xsd:string ;
    rdfs:subClassOf wikidata:Q23649976 .

wikidata:Q23790218 rdfs:label "BBFC classification category"^^xsd:string ;
    rdfs:comment "single classification in the British Board of Film Classification rating system"^^xsd:string ;
    rdfs:subClassOf wikidata:Q23649976 .

wikidata:Q23834194 rdfs:label "literary group"^^xsd:string ;
    rdfs:comment "group or school of writers"^^xsd:string ;
    rdfs:subClassOf wikidata:Q16334295 .

wikidata:Q23847174 rdfs:label "religious concept"^^xsd:string ;
    rdfs:comment "abstract object associated with religion"^^xsd:string ;
    rdfs:subClassOf wikidata:Q151885 .

wikidata:Q2393187 rdfs:label "molecular entity"^^xsd:string ;
    rdfs:comment "any constitutionally or isotopically distinct atom, molecule, ion, ion pair, radical, radical ion, complex, conformer, etc., identifiable as a separately distinguishable entity"^^xsd:string .

wikidata:Q24074280 rdfs:label "noble family name"^^xsd:string ;
    rdfs:comment "common name held by members of a noble house"^^xsd:string ;
    rdfs:subClassOf wikidata:Q101352 .

wikidata:Q24286894 rdfs:label "fictional humanoid species"^^xsd:string ;
    rdfs:comment "coherent large group of humanoids"^^xsd:string ;
    rdfs:subClassOf wikidata:Q21192438 .

wikidata:Q24336031 rdfs:label "mythical river"^^xsd:string ;
    rdfs:comment "river that only exists in myth"^^xsd:string ;
    rdfs:subClassOf wikidata:Q16338046,
        wikidata:Q24334893 .

wikidata:Q24354 rdfs:label "theatre"^^xsd:string ;
    rdfs:comment "performing arts venue or building"^^xsd:string ;
    rdfs:subClassOf wikidata:Q17350442 .

wikidata:Q245065 rdfs:label "intergovernmental organization"^^xsd:string ;
    rdfs:comment "organization composed primarily of sovereign states"^^xsd:string ;
    rdfs:subClassOf wikidata:Q484652,
        wikidata:Q7210356 .

wikidata:Q24561417 rdfs:label "USK rating category"^^xsd:string ;
    rdfs:comment "категорія вікових обмежень для програмного забезпечення"^^xsd:string ;
    rdfs:subClassOf wikidata:Q23649976 .

wikidata:Q24633474 rdfs:label "audio podcast"^^xsd:string ;
    rdfs:comment "podcast in audio format"^^xsd:string ;
    rdfs:subClassOf wikidata:Q24634210 .

wikidata:Q2485083 rdfs:label "suicide method"^^xsd:string ;
    rdfs:comment "means by which a person completes suicide"^^xsd:string ;
    rdfs:subClassOf wikidata:Q1799072,
        wikidata:Q1931388 .

wikidata:Q249083 rdfs:label "asteroid family"^^xsd:string ;
    rdfs:comment "population of asteroids that share similar proper orbital elements"^^xsd:string .

wikidata:Q2500378 rdfs:label "department of the United Kingdom Government"^^xsd:string ;
    rdfs:comment "British Government Departments"^^xsd:string ;
    rdfs:subClassOf wikidata:Q327333 .

wikidata:Q2516866 rdfs:label "publisher"^^xsd:string ;
    rdfs:comment "person heading a publishing company or who publishes media"^^xsd:string .

wikidata:Q251777 rdfs:label "custom"^^xsd:string ;
    rdfs:comment "set of agreed, stipulated, or generally accepted standards, norms, social norms, or criteria"^^xsd:string .

wikidata:Q2532754 rdfs:label "achievement"^^xsd:string ;
    rdfs:comment "full display or depiction of all the heraldic components to which the bearer of a coat of arms is entitled"^^xsd:string ;
    rdfs:subClassOf wikidata:Q17335294,
        wikidata:Q80071 .

wikidata:Q25403900 rdfs:label "food ingredient"^^xsd:string ;
    rdfs:comment "ingredient used in food product"^^xsd:string ;
    rdfs:subClassOf wikidata:Q2095 .

wikidata:Q25519785 rdfs:label "artillery weapons"^^xsd:string ;
    rdfs:comment ""^^xsd:string ;
    rdfs:subClassOf wikidata:Q18643213,
        wikidata:Q728 .

wikidata:Q2560570 rdfs:label "thematic catalog"^^xsd:string ;
    rdfs:comment "index used to identify musical compositions through the citation of either the opening notes or main theme of the work"^^xsd:string ;
    rdfs:subClassOf wikidata:Q5051330 .

wikidata:Q2576663 rdfs:label "engine configuration"^^xsd:string ;
    rdfs:comment "arrangement of cylinders within a reciprocating engine"^^xsd:string ;
    rdfs:subClassOf wikidata:Q151885 .

wikidata:Q2578402 rdfs:label "hand tool"^^xsd:string ;
    rdfs:comment "tool equipment powered manually"^^xsd:string ;
    rdfs:subClassOf wikidata:Q39546 .

wikidata:Q25810847 rdfs:label "folkloristic character"^^xsd:string ;
    rdfs:comment "personaje que forma parte del folclore de un pueblo"^^xsd:string ;
    rdfs:subClassOf wikidata:Q95074 .

wikidata:Q2607197 rdfs:label "character race"^^xsd:string ;
    rdfs:comment "somewhat analogous with \"humanoid species\" in fantasy and science fiction; e.g. elves and dwarves"^^xsd:string ;
    rdfs:subClassOf wikidata:Q15831596 .

wikidata:Q2608849 rdfs:label "imprint"^^xsd:string ;
    rdfs:comment "trade name under which works are published; a publishing division of a publishing company"^^xsd:string ;
    rdfs:subClassOf wikidata:Q2085381 .

wikidata:Q2623733 rdfs:label "fictional language"^^xsd:string ;
    rdfs:comment "constructed languages that have been created as part of a fictional setting"^^xsd:string ;
    rdfs:subClassOf wikidata:Q14897293,
        wikidata:Q34770 .

wikidata:Q26267864 rdfs:label "Wikimedia KML file"^^xsd:string ;
    rdfs:comment "KML file stored as wikitext on a Wikimedia project"^^xsd:string ;
    rdfs:subClassOf wikidata:Q11266439 .

wikidata:Q2630831 rdfs:label "supradialect"^^xsd:string ;
    rdfs:comment "dialectological category between the levels of language and dialect"^^xsd:string .

wikidata:Q2634521 rdfs:label "title of Jesus"^^xsd:string ;
    rdfs:comment "designations for Jesus"^^xsd:string ;
    rdfs:subClassOf wikidata:Q216353,
        wikidata:Q3320743 .

wikidata:Q2638480 rdfs:label "church congregation"^^xsd:string ;
    rdfs:comment "Christian religious organization meeting at a particular location"^^xsd:string ;
    rdfs:subClassOf wikidata:Q1530022 .

wikidata:Q26678730 rdfs:label "ClassInd category"^^xsd:string ;
    rdfs:comment "a single rating in the Brazilian Advisory Rating System"^^xsd:string ;
    rdfs:subClassOf wikidata:Q23649976 .

wikidata:Q267628 rdfs:label "column"^^xsd:string ;
    rdfs:comment "recurring piece or article in a periodical"^^xsd:string .

wikidata:Q26971562 rdfs:label "comic format"^^xsd:string ;
    rdfs:comment "term"^^xsd:string .

wikidata:Q269949 rdfs:label "highway"^^xsd:string ;
    rdfs:comment "public or private road or other public way on land"^^xsd:string ;
    rdfs:subClassOf wikidata:Q34442 .

wikidata:Q271680 rdfs:label "software framework"^^xsd:string ;
    rdfs:comment "computer programming concept"^^xsd:string ;
    rdfs:subClassOf wikidata:Q188860,
        wikidata:Q241317,
        wikidata:Q40056 .

wikidata:Q27253938 rdfs:label "ICAA rating category"^^xsd:string ;
    rdfs:comment "a single rating in the ICAA rating system"^^xsd:string ;
    rdfs:subClassOf wikidata:Q23649976 .

wikidata:Q2743 rdfs:label "musical"^^xsd:string ;
    rdfs:comment "work that combines songs, music, spoken dialogue, acting, and dance"^^xsd:string ;
    rdfs:subClassOf wikidata:Q2188189,
        wikidata:Q2431196,
        wikidata:Q25379,
        wikidata:Q43099500 .

wikidata:Q2750108 rdfs:label "priory"^^xsd:string ;
    rdfs:comment "religious houses that rank immediately below abbeys and are presided over by a prior or prioress"^^xsd:string ;
    rdfs:subClassOf wikidata:Q44613 .

wikidata:Q2751586 rdfs:label "resolution"^^xsd:string ;
    rdfs:comment "written declaration adopted by a deliberative body"^^xsd:string ;
    rdfs:subClassOf wikidata:Q49848 .

wikidata:Q2755432 rdfs:label "compression algorithm"^^xsd:string ;
    rdfs:comment "type of algorithm used for reducing the storage size of data"^^xsd:string ;
    rdfs:subClassOf wikidata:Q8366 .

wikidata:Q276 rdfs:label "Eurovision Song Contest"^^xsd:string ;
    rdfs:comment "annual song competition held among the member countries of the European Broadcasting Union"^^xsd:string ;
    rdfs:subClassOf wikidata:Q15416,
        wikidata:Q1955280,
        wikidata:Q868557 .

wikidata:Q27787439 rdfs:label "film festival edition"^^xsd:string ;
    rdfs:comment "specific edition of a film festival, e.g. in a given year of an annual festival"^^xsd:string ;
    rdfs:subClassOf wikidata:Q27968055 .

wikidata:Q2795484 rdfs:label "implementing regulation"^^xsd:string ;
    rdfs:comment "regulation on the details of the implementation of a law"^^xsd:string ;
    rdfs:subClassOf wikidata:Q694045 .

wikidata:Q280855 rdfs:label "astrophotography"^^xsd:string ;
    rdfs:comment "specialized type of photography for recording images of astronomical objects and large areas of the night sky"^^xsd:string .

wikidata:Q2822246 rdfs:label "academic district"^^xsd:string ;
    rdfs:comment "administrative division in France for education"^^xsd:string ;
    rdfs:subClassOf wikidata:Q161837,
        wikidata:Q43229 .

wikidata:Q285451 rdfs:label "drainage system"^^xsd:string ;
    rdfs:comment "pattern formed by the streams, rivers, and lakes in a particular drainage basin"^^xsd:string .

wikidata:Q2860026 rdfs:label "arch"^^xsd:string ;
    rdfs:comment "Bogen, der in der Lage ist, einen Raum zu überqueren und dabei ein bedeutendes Gewicht zu tragen"^^xsd:string ;
    rdfs:subClassOf wikidata:Q391414 .

wikidata:Q287198 rdfs:label "online chat"^^xsd:string ;
    rdfs:comment "communication over the Internet that offers a real-time transmission of text messages from sender to receiver"^^xsd:string .

wikidata:Q2881272 rdfs:label "district of New Zealand"^^xsd:string ;
    rdfs:comment "district administered by a territorial authority in New Zealand"^^xsd:string .

wikidata:Q28820001 rdfs:label "music scene"^^xsd:string ;
    rdfs:comment "groups of artists who share common features within region or time-period"^^xsd:string ;
    rdfs:subClassOf wikidata:Q2198855 .

wikidata:Q2882257 rdfs:label "First Nation band"^^xsd:string ;
    rdfs:comment "First Nations government in Canada"^^xsd:string ;
    rdfs:subClassOf wikidata:Q28790362 .

wikidata:Q28823 rdfs:label "textile"^^xsd:string ;
    rdfs:comment "material produced by twining, weaving, felting, knotting, or otherwise processing natural or synthetic fibers"^^xsd:string ;
    rdfs:subClassOf wikidata:Q15401930,
        wikidata:Q214609,
        wikidata:Q28877,
        wikidata:Q8205328 .

wikidata:Q28945444 rdfs:label "failed attack"^^xsd:string ;
    rdfs:comment "ataque que no logró su objetivo"^^xsd:string .

wikidata:Q289472 rdfs:label "biogenic substance"^^xsd:string ;
    rdfs:comment "substance produced by life processes; it may be either constituents, or secretions, of plants or animals"^^xsd:string ;
    rdfs:subClassOf wikidata:Q25416091 .

wikidata:Q289612 rdfs:label "general contractor"^^xsd:string ;
    rdfs:comment "profession"^^xsd:string .

wikidata:Q2944660 rdfs:label "lexical item"^^xsd:string ;
    rdfs:comment "element of a lexicon"^^xsd:string .

wikidata:Q2961496 rdfs:label "ship's cat"^^xsd:string ;
    rdfs:comment "cat carried on ships for many reasons, most importantly to control rodents"^^xsd:string ;
    rdfs:subClassOf wikidata:Q146 .

wikidata:Q29652773 rdfs:label "film soundtrack"^^xsd:string ;
    rdfs:comment "recorded music accompanying and synchronized to the images of a motion picture"^^xsd:string .

wikidata:Q2977 rdfs:label "cathedral"^^xsd:string ;
    rdfs:comment "Christian church, which is seat of a bishop"^^xsd:string ;
    rdfs:subClassOf wikidata:Q16970 .

wikidata:Q2985386 rdfs:label "editorial board"^^xsd:string ;
    rdfs:comment "group of experts, usually at a publication, who dictate the tone and direction the publication's editorial policy will take"^^xsd:string .

wikidata:Q29881657 rdfs:label "vocal-musical ensemble"^^xsd:string ;
    rdfs:comment "musical ensemble in which both instrumentalists and singers perform"^^xsd:string ;
    rdfs:subClassOf wikidata:Q215380 .

wikidata:Q2989352 rdfs:label "free software community"^^xsd:string ;
    rdfs:comment "community of people who make and promote software that can be run for any purpose, studied, changed, and redistributed"^^xsd:string ;
    rdfs:subClassOf wikidata:Q177634,
        wikidata:Q63437139 .

wikidata:Q2992500 rdfs:label "wing configuration"^^xsd:string ;
    rdfs:comment "describes the general shape and layout of an aircraft wing"^^xsd:string .

wikidata:Q29982117 rdfs:label "musical instrument model"^^xsd:string ;
    rdfs:comment "Modell eines Musikinstruments"^^xsd:string ;
    rdfs:subClassOf wikidata:Q10929058 .

wikidata:Q30092755 rdfs:label "surface water body"^^xsd:string ;
    rdfs:comment "an inland water body, except groundwater; transitional waters and coastal water bodies, except in respect of chemical status for which it shall also include territorial waters."^^xsd:string .

wikidata:Q3044 rdfs:label "Charlemagne"^^xsd:string ;
    rdfs:comment "King of the Franks, King of Italy, and Holy Roman Emperor"^^xsd:string .

wikidata:Q3046146 rdfs:label "married couple"^^xsd:string ;
    rdfs:comment "two people who are married to each other"^^xsd:string ;
    rdfs:subClassOf wikidata:Q8436 .

wikidata:Q30634609 rdfs:label "heritage designation"^^xsd:string ;
    rdfs:comment "act or effect of recognizing the historical, artistic or cultural value of a property"^^xsd:string ;
    rdfs:subClassOf wikidata:Q3249551 .

wikidata:Q30899001 rdfs:label "software distributor"^^xsd:string ;
    rdfs:comment "empresa que media entre las empresas de desarrollo de software y los minoristas"^^xsd:string ;
    rdfs:subClassOf wikidata:Q4830453 .

wikidata:Q309 rdfs:label "history"^^xsd:string ;
    rdfs:comment "past events and their tracks or records, studied by various branches of human sciences of history"^^xsd:string .

wikidata:Q310899 rdfs:label "microRNA"^^xsd:string ;
    rdfs:comment "small non-coding RNA molecule (of ca. 22 nucleotides) found in plants, animals and some viruses, that functions in RNA silencing and post-transcriptional regulation of gene expression"^^xsd:string .

wikidata:Q3117863 rdfs:label "isolated human group"^^xsd:string ;
    rdfs:comment "group of humans living together isolated from other human beings"^^xsd:string ;
    rdfs:subClassOf wikidata:Q16334295 .

wikidata:Q3133368 rdfs:label "repository"^^xsd:string ;
    rdfs:comment "data storage for software revision control"^^xsd:string ;
    rdfs:subClassOf wikidata:Q8513 .

wikidata:Q3172759 rdfs:label "traditional costume"^^xsd:string ;
    rdfs:comment "expression of identity through costume, which is usually associated with a geographic area or a period of time in history"^^xsd:string .

wikidata:Q3231690 rdfs:label "automobile model"^^xsd:string ;
    rdfs:comment "industrial automobile model associated with a brand, defined usually from an engineering point of view by a combination of chassis/bodywork"^^xsd:string ;
    rdfs:subClassOf wikidata:Q29048322 .

wikidata:Q3235978 rdfs:label "circumstellar disk"^^xsd:string ;
    rdfs:comment "torus, pancake or ring-shaped accumulation of matter in orbit around a star"^^xsd:string ;
    rdfs:subClassOf wikidata:Q6999 .

wikidata:Q3254959 rdfs:label "race"^^xsd:string ;
    rdfs:comment "controversial classification system used to categorize humans on the basis of hereditary physical traits"^^xsd:string .

wikidata:Q3257925 rdfs:label "Go software"^^xsd:string ;
    rdfs:comment "software playing the board game Go"^^xsd:string ;
    rdfs:subClassOf wikidata:Q40056,
        wikidata:Q7889 .

wikidata:Q32880 rdfs:label "architectural style"^^xsd:string ;
    rdfs:comment "a specific method of construction"^^xsd:string ;
    rdfs:subClassOf wikidata:Q1792644 .

wikidata:Q329525 rdfs:label "criminal charge"^^xsd:string ;
    rdfs:comment "formal accusation of wrongdoing in common law"^^xsd:string .

wikidata:Q329864 rdfs:label "military technology"^^xsd:string ;
    rdfs:comment "application of technology for use in warfare"^^xsd:string ;
    rdfs:subClassOf wikidata:Q11016 .

wikidata:Q3299260 rdfs:label "local government area"^^xsd:string ;
    rdfs:comment "administrative division of a country that a local government is responsible for"^^xsd:string ;
    rdfs:subClassOf wikidata:Q56061 .

wikidata:Q33104279 rdfs:label "philosophical concept"^^xsd:string ;
    rdfs:comment "concept used in philosophy"^^xsd:string ;
    rdfs:subClassOf wikidata:Q151885 .

wikidata:Q3327870 rdfs:label "municipal corporation in the United States"^^xsd:string ;
    rdfs:comment "ABD'de bölgesel yönetim"^^xsd:string .

wikidata:Q33753 rdfs:label "metamorphosis"^^xsd:string ;
    rdfs:comment "profound change in body structure during the postembryonic development of an organism"^^xsd:string ;
    rdfs:subClassOf wikidata:Q2996394 .

wikidata:Q3393392 rdfs:label "highest point"^^xsd:string ;
    rdfs:comment "highest elevation of a geographical zone"^^xsd:string ;
    rdfs:subClassOf wikidata:Q271669 .

wikidata:Q3407658 rdfs:label "tram"^^xsd:string ;
    rdfs:comment "public transport vehicle running on rails predominantly located on streets"^^xsd:string ;
    rdfs:subClassOf wikidata:Q1414135 .

wikidata:Q34178 rdfs:label "theology"^^xsd:string ;
    rdfs:comment "study of the nature of God and religious belief"^^xsd:string ;
    rdfs:subClassOf wikidata:Q1047113 .

wikidata:Q34542757 rdfs:label "international association football clubs cup"^^xsd:string ;
    rdfs:comment "international association football tournament with club teams participating"^^xsd:string .

wikidata:Q34651 rdfs:label "Christian Church"^^xsd:string ;
    rdfs:comment "bless up the lord, Jesus Christ"^^xsd:string ;
    rdfs:subClassOf wikidata:Q1530022 .

wikidata:Q3469910 rdfs:label "performing arts center"^^xsd:string ;
    rdfs:comment "multi-use performance space"^^xsd:string ;
    rdfs:subClassOf wikidata:Q18674739,
        wikidata:Q68773434 .

wikidata:Q3491904 rdfs:label "urban rail transit"^^xsd:string ;
    rdfs:comment "term for various types of local rail systems"^^xsd:string ;
    rdfs:subClassOf wikidata:Q18325841,
        wikidata:Q2516436,
        wikidata:Q2678338 .

wikidata:Q3500690 rdfs:label "church bell"^^xsd:string ;
    rdfs:comment "bell in a church"^^xsd:string ;
    rdfs:subClassOf wikidata:Q391414 .

wikidata:Q3502482 rdfs:label "cultural region"^^xsd:string ;
    rdfs:comment "aspects of culture associated with an ethnolinguistic group and the territory it inhabits"^^xsd:string ;
    rdfs:subClassOf wikidata:Q15642541 .

wikidata:Q3511132 rdfs:label "series"^^xsd:string ;
    rdfs:comment "term in archival science; collection of records grouped as a result of their original function, use, or other relationship to one another"^^xsd:string ;
    rdfs:subClassOf wikidata:Q3052382 .

wikidata:Q3523102 rdfs:label "source of information"^^xsd:string ;
    rdfs:comment "source of information for somebody, i.e. anything that might inform a person about something or provide knowledge about it"^^xsd:string ;
    rdfs:subClassOf wikidata:Q31464082 .

wikidata:Q353027 rdfs:label "long-distance cycling route"^^xsd:string ;
    rdfs:comment "designated cycling routes in various countries around the world for bicycle tourism, normally longer than local cycling paths"^^xsd:string ;
    rdfs:subClassOf wikidata:Q1322323 .

wikidata:Q3566043 rdfs:label "bad"^^xsd:string ;
    rdfs:comment "item with negative value to the consumer"^^xsd:string ;
    rdfs:subClassOf wikidata:Q488383 .

wikidata:Q35666 rdfs:label "glacier"^^xsd:string ;
    rdfs:comment "large persistent body of ice"^^xsd:string .

wikidata:Q35718073 rdfs:label "nations in the Eurovision Song Contest"^^xsd:string ;
    rdfs:comment "countries that have participated at the Eurovision Song Contest"^^xsd:string .

wikidata:Q357685 rdfs:label "abandoned railway"^^xsd:string ;
    rdfs:comment "railway line which is no longer used for that purpose"^^xsd:string ;
    rdfs:subClassOf wikidata:Q728937 .

wikidata:Q358078 rdfs:label "road network"^^xsd:string ;
    rdfs:comment "system of interconnecting lines and points that represent a system of streets or roads for a given area"^^xsd:string ;
    rdfs:subClassOf wikidata:Q3241753,
        wikidata:Q376799 .

wikidata:Q36161 rdfs:label "set"^^xsd:string ;
    rdfs:comment "well-defined mathematical collection of distinct objects"^^xsd:string .

wikidata:Q3622170 rdfs:label "fictional currency"^^xsd:string ;
    rdfs:comment "currency existing only in fictional works"^^xsd:string .

wikidata:Q3624078 rdfs:label "sovereign state"^^xsd:string ;
    rdfs:comment "political organization with a centralized independent government"^^xsd:string ;
    rdfs:subClassOf wikidata:Q6256,
        wikidata:Q7275 .

wikidata:Q36534 rdfs:label "chemical reaction"^^xsd:string ;
    rdfs:comment "process that results in the interconversion of chemical species"^^xsd:string .

wikidata:Q3658341 rdfs:label "literary character"^^xsd:string ;
    rdfs:comment "fictional character appearing in written works"^^xsd:string ;
    rdfs:subClassOf wikidata:Q95074 .

wikidata:Q36669 rdfs:label "daylight saving time"^^xsd:string ;
    rdfs:comment "practice of advancing clocks so that evenings have more daylight and mornings have less"^^xsd:string .

wikidata:Q3689421 rdfs:label "destination marketing organisation"^^xsd:string ;
    rdfs:comment "organization promoting tourism to increase the number of visitors"^^xsd:string ;
    rdfs:subClassOf wikidata:Q43229 .

wikidata:Q36906466 rdfs:label "universe"^^xsd:string ;
    rdfs:comment "class of which Our Universe is an instance, and parallel universes, if any, are also instances"^^xsd:string .

wikidata:Q372690 rdfs:label "consulate general"^^xsd:string ;
    rdfs:comment "diplomatic mission"^^xsd:string ;
    rdfs:subClassOf wikidata:Q213283,
        wikidata:Q7843791 .

wikidata:Q373074 rdfs:label "suffragan diocese"^^xsd:string ;
    rdfs:comment "one of the dioceses other than the metropolitan archdiocese that constitute an ecclesiastical province"^^xsd:string ;
    rdfs:subClassOf wikidata:Q20926517 .

wikidata:Q3732788 rdfs:label "apostolic exarchate"^^xsd:string ;
    rdfs:comment "forma administrativního uspořádání ve východních církvích sui iuris"^^xsd:string ;
    rdfs:subClassOf wikidata:Q1492823,
        wikidata:Q3146899 .

wikidata:Q373498 rdfs:label "dan"^^xsd:string ;
    rdfs:comment "Japanese mark of level"^^xsd:string .

wikidata:Q3760158 rdfs:label "nomen"^^xsd:string ;
    rdfs:comment "name in Ancient Rome which identified people as members of a gens (ie. family or clan)"^^xsd:string ;
    rdfs:subClassOf wikidata:Q101352 .

wikidata:Q37748 rdfs:label "chromosome"^^xsd:string ;
    rdfs:comment "structure composed of a very long molecule of DNA and associated proteins (e.g. histones) that carries hereditary information"^^xsd:string .

wikidata:Q377688 rdfs:label "type foundry"^^xsd:string ;
    rdfs:comment "company that designs or distributes typefaces"^^xsd:string ;
    rdfs:subClassOf wikidata:Q4830453 .

wikidata:Q37787110 rdfs:label "file system object"^^xsd:string ;
    rdfs:comment "object in a computer filesystem, such as a file, directory, or symlink"^^xsd:string .

wikidata:Q378427 rdfs:label "literary award"^^xsd:string ;
    rdfs:comment "award for authors and literary associations"^^xsd:string ;
    rdfs:subClassOf wikidata:Q1656682,
        wikidata:Q618779 .

wikidata:Q379755 rdfs:label "arrangement"^^xsd:string ;
    rdfs:comment "musical composition in altered form"^^xsd:string ;
    rdfs:subClassOf wikidata:Q2188189 .

wikidata:Q384003 rdfs:label "apostolic prefecture"^^xsd:string ;
    rdfs:comment "missionary area not yet developed enough to become a diocese"^^xsd:string ;
    rdfs:subClassOf wikidata:Q1492823 .

wikidata:Q386208 rdfs:label "mascot character"^^xsd:string ;
    rdfs:comment "created character used as a mascot by an organisation"^^xsd:string .

wikidata:Q3863 rdfs:label "asteroid"^^xsd:string ;
    rdfs:comment "minor planet that is not a comet"^^xsd:string ;
    rdfs:subClassOf wikidata:Q1022867 .

wikidata:Q388 rdfs:label "Linux"^^xsd:string ;
    rdfs:comment "family of unix-like operating systems that use the Linux kernel and are open source"^^xsd:string .

wikidata:Q388201 rdfs:label "railway electrification system"^^xsd:string ;
    rdfs:comment "electric power to railway trains and trams without an on-board prime mover or local fuel supply"^^xsd:string .

wikidata:Q38829 rdfs:label "breed"^^xsd:string ;
    rdfs:comment "specific group of domestic animals"^^xsd:string ;
    rdfs:subClassOf wikidata:Q55983715 .

wikidata:Q3887 rdfs:label "solar eclipse"^^xsd:string ;
    rdfs:comment "natural phenomenon wherein the Sun is obscured by the Moon"^^xsd:string ;
    rdfs:subClassOf wikidata:Q27968055 .

wikidata:Q391009 rdfs:label "Catholic order"^^xsd:string ;
    rdfs:comment "tipo di istituto religioso cattolico i cui membri emettono i voti in forma semplice"^^xsd:string .

wikidata:Q3917681 rdfs:label "embassy"^^xsd:string ;
    rdfs:comment "permanent diplomatic mission of higher level, representing its operator in the country the embassy is in"^^xsd:string ;
    rdfs:subClassOf wikidata:Q17334923,
        wikidata:Q213283 .

wikidata:Q3935690 rdfs:label "form of energy"^^xsd:string ;
    rdfs:comment "concept in physical sciences"^^xsd:string .

wikidata:Q39486269 rdfs:label "railway viaduct"^^xsd:string ;
    rdfs:comment "bridge, usually resting on a number of raised arches, carrying a railway across low-lying land, water, gorge or valley"^^xsd:string ;
    rdfs:subClassOf wikidata:Q1210334,
        wikidata:Q181348 .

wikidata:Q394970 rdfs:label "box set"^^xsd:string ;
    rdfs:comment "compilation of various media or other items contained in a box"^^xsd:string ;
    rdfs:subClassOf wikidata:Q1020767,
        wikidata:Q2031291 .

wikidata:Q3953107 rdfs:label "logographic writing system"^^xsd:string ;
    rdfs:comment "writing system that is based on logograms"^^xsd:string ;
    rdfs:subClassOf wikidata:Q8192 .

wikidata:Q3958441 rdfs:label "economic sector"^^xsd:string ;
    rdfs:comment "conceptual grouping of economic activities"^^xsd:string ;
    rdfs:subClassOf wikidata:Q58778 .

wikidata:Q39614 rdfs:label "cemetery"^^xsd:string ;
    rdfs:comment "place of burial"^^xsd:string ;
    rdfs:subClassOf wikidata:Q13226383,
        wikidata:Q1497375 .

wikidata:Q40050 rdfs:label "drink"^^xsd:string ;
    rdfs:comment "kind of liquid which is specifically prepared for human consumption"^^xsd:string ;
    rdfs:subClassOf wikidata:Q2095 .

wikidata:Q400857 rdfs:label "environment variable"^^xsd:string ;
    rdfs:comment "dynamic value that affects the behavior of processes on a computer"^^xsd:string .

wikidata:Q40213094 rdfs:label "fictional video game"^^xsd:string ;
    rdfs:comment "fictional videogame in a narrative form of arts"^^xsd:string ;
    rdfs:subClassOf wikidata:Q15306849 .

wikidata:Q4024737 rdfs:label "Pastoral region"^^xsd:string ;
    rdfs:comment "Administrative subdivision of a diocese, headed by an episcopal vicar"^^xsd:string ;
    rdfs:subClassOf wikidata:Q20926517 .

wikidata:Q408978 rdfs:label "airplay"^^xsd:string ;
    rdfs:comment "the frequency that a song is broadcasted on radio stations"^^xsd:string .

wikidata:Q40953 rdfs:label "prayer"^^xsd:string ;
    rdfs:comment "invocation or act that seeks to activate a rapport with a deity"^^xsd:string ;
    rdfs:subClassOf wikidata:Q1914636 .

wikidata:Q4120211 rdfs:label "regional organization"^^xsd:string ;
    rdfs:comment "international organizations that act within a specific region"^^xsd:string ;
    rdfs:subClassOf wikidata:Q484652,
        wikidata:Q56061 .

wikidata:Q4122445 rdfs:label "service regulations"^^xsd:string ;
    rdfs:comment "rules regarding the organization and implementation of certain services (in the states and organizations)"^^xsd:string ;
    rdfs:subClassOf wikidata:Q1151067 .

wikidata:Q41349 rdfs:label "smart card"^^xsd:string ;
    rdfs:comment "pocket-sized card with embedded integrated circuits for security-related functions"^^xsd:string ;
    rdfs:subClassOf wikidata:Q1048236,
        wikidata:Q986008 .

wikidata:Q41554073 rdfs:label "delict"^^xsd:string ;
    rdfs:comment "category of crimes in Italian law"^^xsd:string .

wikidata:Q41582469 rdfs:label "music festival edition"^^xsd:string ;
    rdfs:comment "specific edition of a music festival, e.g. in a given year of an annual festival"^^xsd:string .

wikidata:Q416 rdfs:label "disk magazine"^^xsd:string ;
    rdfs:comment "electronic magazine to be read using computers"^^xsd:string ;
    rdfs:subClassOf wikidata:Q41298,
        wikidata:Q7397 .

wikidata:Q4167410 rdfs:label "Wikimedia disambiguation page"^^xsd:string ;
    rdfs:comment "Wikimedia page that lists different meanings for the same string"^^xsd:string ;
    rdfs:subClassOf wikidata:Q12139612 .

wikidata:Q4169 rdfs:label "outer space"^^xsd:string ;
    rdfs:comment "void between celestial bodies"^^xsd:string .

wikidata:Q4176708 rdfs:label "soundtrack album"^^xsd:string ;
    rdfs:comment "album containing music from another work, such as a film, video game, television series"^^xsd:string ;
    rdfs:subClassOf wikidata:Q482994 .

wikidata:Q41825 rdfs:label "day of the week"^^xsd:string ;
    rdfs:comment "day within a week"^^xsd:string .

wikidata:Q42032 rdfs:label "country code top-level domain"^^xsd:string ;
    rdfs:comment "internet top-level domain generally used or reserved for a country"^^xsd:string .

wikidata:Q4220917 rdfs:label "film award"^^xsd:string ;
    rdfs:comment "recognition for cinematic achievements"^^xsd:string ;
    rdfs:subClassOf wikidata:Q618779,
        wikidata:Q841654 .

wikidata:Q42336871 rdfs:label "crowdfunding platform"^^xsd:string ;
    rdfs:comment "online platform for campaigns to get funding from crowds"^^xsd:string .

wikidata:Q4233718 rdfs:label "anonymous"^^xsd:string ;
    rdfs:comment "term used to describe the unknown creator of a work"^^xsd:string ;
    rdfs:subClassOf wikidata:Q5 .

wikidata:Q42501 rdfs:label "combustible matter"^^xsd:string ;
    rdfs:comment "any material that stores energy that can later be extracted, in presence of a oxidizer or a catalyser, or under the effect of a tool, but which is not conserved after the reaction"^^xsd:string ;
    rdfs:subClassOf wikidata:Q79529,
        wikidata:Q837718 .

wikidata:Q427626 rdfs:label "taxonomic rank"^^xsd:string ;
    rdfs:comment "level in a taxonomic hierarchy"^^xsd:string ;
    rdfs:subClassOf wikidata:Q4120621 .

wikidata:Q428148 rdfs:label "regulation"^^xsd:string ;
    rdfs:comment "general term for rules or controls, including delegated legislation and self-regulation"^^xsd:string ;
    rdfs:subClassOf wikidata:Q1151067 .

wikidata:Q43100730 rdfs:label "series of performances"^^xsd:string ;
    rdfs:comment "series of performances of the same work of the performing arts, subset of the performances of a performing arts production (e.g. taking place at the same venue)"^^xsd:string ;
    rdfs:subClassOf wikidata:Q1656682,
        wikidata:Q20937557 .

wikidata:Q4321 rdfs:label "Motherboard"^^xsd:string ;
    rdfs:comment "main printed circuit board (PCB) for a computing device"^^xsd:string .

wikidata:Q43306178 rdfs:label "supreme audit institution"^^xsd:string ;
    rdfs:comment "entidad fiscalizadora"^^xsd:string .

wikidata:Q4369513 rdfs:label "sex of humans"^^xsd:string ;
    rdfs:comment "biological sex as opposed to gender identity"^^xsd:string .

wikidata:Q43812 rdfs:label "passport"^^xsd:string ;
    rdfs:comment "travel document usually issued by a country's government"^^xsd:string ;
    rdfs:subClassOf wikidata:Q47988 .

wikidata:Q4384751 rdfs:label "traditional culture"^^xsd:string ;
    rdfs:comment "traditional dance and song and stories both in traditional society and in modern revival"^^xsd:string ;
    rdfs:subClassOf wikidata:Q11042 .

wikidata:Q4393107 rdfs:label "video game remake"^^xsd:string ;
    rdfs:comment "remake of an existing video game, usually involving new/updated game mechanics"^^xsd:string ;
    rdfs:subClassOf wikidata:Q7889 .

wikidata:Q44167 rdfs:label "engine"^^xsd:string ;
    rdfs:comment "machine designed to produce mechanical energy from another form of energy"^^xsd:string ;
    rdfs:subClassOf wikidata:Q11019 .

wikidata:Q44235 rdfs:label "lunar eclipse"^^xsd:string ;
    rdfs:comment "when the Moon passes directly behind the Earth"^^xsd:string .

wikidata:Q44559 rdfs:label "extrasolar planet"^^xsd:string ;
    rdfs:comment "any planet beyond the Solar System"^^xsd:string ;
    rdfs:subClassOf wikidata:Q634 .

wikidata:Q4461766 rdfs:label "traditional culture"^^xsd:string ;
    rdfs:comment ""^^xsd:string ;
    rdfs:subClassOf wikidata:Q11042 .

wikidata:Q44696264 rdfs:label "aerial tramway station"^^xsd:string ;
    rdfs:comment "station of an aerial lift"^^xsd:string .

wikidata:Q45382 rdfs:label "coup d'état"^^xsd:string ;
    rdfs:comment "sudden deposition of a government; illegal and overt seizure of a state by the military or other elites within the state apparatus"^^xsd:string ;
    rdfs:subClassOf wikidata:Q83267 .

wikidata:Q4539 rdfs:label "cooperative"^^xsd:string ;
    rdfs:comment "autonomous association of persons or organizations"^^xsd:string ;
    rdfs:subClassOf wikidata:Q783794 .

wikidata:Q45736416 rdfs:label "plan of management"^^xsd:string ;
    rdfs:comment "legal document outlining how public lands (particularly national parks and nature reserves) are to be used and managed"^^xsd:string ;
    rdfs:subClassOf wikidata:Q1371819,
        wikidata:Q49848 .

wikidata:Q46311 rdfs:label "bow"^^xsd:string ;
    rdfs:comment "ranged weapon system consisting of an elastic launching device and long-shafted projectiles"^^xsd:string .

wikidata:Q465299 rdfs:label "archaeological culture"^^xsd:string ;
    rdfs:comment "recurring assemblage of artifacts from a specific time and place that may constitute the material culture remains of a particular past human society"^^xsd:string ;
    rdfs:subClassOf wikidata:Q11042,
        wikidata:Q151885 .

wikidata:Q47018901 rdfs:label "calendar month"^^xsd:string ;
    rdfs:comment "one of generally twelve months of a specific calendar. Use with P31"^^xsd:string ;
    rdfs:subClassOf wikidata:Q5151 .

wikidata:Q47272186 rdfs:label "headquarters"^^xsd:string ;
    rdfs:comment "military unit type designation"^^xsd:string ;
    rdfs:subClassOf wikidata:Q176799 .

wikidata:Q47306921 rdfs:label "fictional parallel universe"^^xsd:string ;
    rdfs:comment "parallel (to Q1 or another) universe that exists in fiction"^^xsd:string ;
    rdfs:subClassOf wikidata:Q559618 .

wikidata:Q47543030 rdfs:label "regeneration of The Doctor"^^xsd:string ;
    rdfs:comment ""^^xsd:string ;
    rdfs:subClassOf wikidata:Q28020127,
        wikidata:Q95074 .

wikidata:Q47848 rdfs:label "sacred architecture"^^xsd:string ;
    rdfs:comment "architectural practices used in places of worship"^^xsd:string .

wikidata:Q4793045 rdfs:label "combat arm"^^xsd:string ;
    rdfs:comment "military service branch which conducts direct military combat operations in land warfare"^^xsd:string .

wikidata:Q4818719 rdfs:label "attributes of God in Christianity"^^xsd:string ;
    rdfs:comment ""^^xsd:string ;
    rdfs:subClassOf wikidata:Q1207505 .

wikidata:Q48277 rdfs:label "gender"^^xsd:string ;
    rdfs:comment "range of physical, mental, and behavioral characteristics distinguishing between masculinity and femininity"^^xsd:string ;
    rdfs:subClassOf wikidata:Q844569 .

wikidata:Q483110 rdfs:label "stadium"^^xsd:string ;
    rdfs:comment "place or venue for (mostly) outdoor sports, concerts, or other events"^^xsd:string ;
    rdfs:subClassOf wikidata:Q641226,
        wikidata:Q811979 .

wikidata:Q486902 rdfs:label "mathematical model"^^xsd:string ;
    rdfs:comment "description of a system using mathematical concepts and language"^^xsd:string ;
    rdfs:subClassOf wikidata:Q1979154 .

wikidata:Q486983 rdfs:label "academic rank"^^xsd:string ;
    rdfs:comment "hierarchical rank found amongst scholars in academia; title denoting the rank of a faculty member in a college or university"^^xsd:string ;
    rdfs:subClassOf wikidata:Q216353 .

wikidata:Q4886 rdfs:label "cultivar"^^xsd:string ;
    rdfs:comment "plant or grouping of plants selected for desirable characteristics"^^xsd:string ;
    rdfs:subClassOf wikidata:Q1362373,
        wikidata:Q16521 .

wikidata:Q4915012 rdfs:label "biological pathway"^^xsd:string ;
    rdfs:comment "set of inter-connected reactions and interactions whose delineation and scope are used as a model for exploring and studying, describing and understanding the working of and relationships between biomolecules within a context"^^xsd:string ;
    rdfs:subClassOf wikidata:Q2996394,
        wikidata:Q386724 .

wikidata:Q49459835 rdfs:label "fraternal hall"^^xsd:string ;
    rdfs:comment "community building operated by a fraternal or veterans organization primarily for the benefit of its members"^^xsd:string .

wikidata:Q4992061 rdfs:label "police district"^^xsd:string ;
    rdfs:comment "police subdivision, responsible for a certain geographic area"^^xsd:string ;
    rdfs:subClassOf wikidata:Q1496967,
        wikidata:Q334453 .

wikidata:Q500834 rdfs:label "tournament"^^xsd:string ;
    rdfs:comment "competition involving a relatively large number of competitors"^^xsd:string ;
    rdfs:subClassOf wikidata:Q13406554 .

wikidata:Q502931 rdfs:label "humanoid"^^xsd:string ;
    rdfs:comment "something that has an appearance resembling a human without actually being one"^^xsd:string ;
    rdfs:subClassOf wikidata:Q215627 .

wikidata:Q50331459 rdfs:label "S-Bahn route"^^xsd:string ;
    rdfs:comment "train route in an S-Bahn system"^^xsd:string .

wikidata:Q5093327 rdfs:label "chess title"^^xsd:string ;
    rdfs:comment "title awarded by a chess governing body and bestowed upon outstanding performances"^^xsd:string ;
    rdfs:subClassOf wikidata:Q618779 .

wikidata:Q51255340 rdfs:label "type specimen"^^xsd:string ;
    rdfs:comment "either, in taxonomy: one of several possible forms of a type, or, in zoology: a specimen belonging to a type series"^^xsd:string ;
    rdfs:subClassOf wikidata:Q18593264,
        wikidata:Q3707858,
        wikidata:Q7239 .

wikidata:Q523 rdfs:label "star"^^xsd:string ;
    rdfs:comment "astronomical object consisting of a luminous spheroid of plasma held together by its own gravity"^^xsd:string ;
    rdfs:subClassOf wikidata:Q6999 .

wikidata:Q524572 rdfs:label "term of office"^^xsd:string ;
    rdfs:comment "time limit for a politician holding a given position (sometimes renewable)"^^xsd:string .

wikidata:Q526877 rdfs:label "web series"^^xsd:string ;
    rdfs:comment "video serial broadcast on the Internet"^^xsd:string ;
    rdfs:subClassOf wikidata:Q2431196 .

wikidata:Q5281760 rdfs:label "discourse topic"^^xsd:string ;
    rdfs:comment "central participant or idea of a stretch of connected discourse or dialogue"^^xsd:string .

wikidata:Q52827 rdfs:label "pictogram"^^xsd:string ;
    rdfs:comment "ideogram that conveys its meaning through its pictorial resemblance to a physical object"^^xsd:string .

wikidata:Q5300 rdfs:label "central processing unit"^^xsd:string ;
    rdfs:comment "electronic circuitry within a computer that carries out the instructions of a computer program by performing the basic arithmetic, logical, control and input/output (I/O) operations specified by the instructions"^^xsd:string ;
    rdfs:subClassOf wikidata:Q1466064 .

wikidata:Q5410500 rdfs:label "faith"^^xsd:string ;
    rdfs:comment "belief in tenets of a religion"^^xsd:string ;
    rdfs:subClassOf wikidata:Q34394 .

wikidata:Q5433312 rdfs:label "family association"^^xsd:string ;
    rdfs:comment "organization of people with shared ancestry or name"^^xsd:string .

wikidata:Q546113 rdfs:label "public policy"^^xsd:string ;
    rdfs:comment "principled guide to action taken by the administrative executive branches of the state with regard to a class of issues"^^xsd:string .

wikidata:Q54820071 rdfs:label "digital download"^^xsd:string ;
    rdfs:comment "commercial product distributed as a download; not to be confused with digital distribution, which additionally includes streaming"^^xsd:string .

wikidata:Q54933017 rdfs:label "race result"^^xsd:string ;
    rdfs:comment "classification of competitors at the conclusion of a race"^^xsd:string ;
    rdfs:subClassOf wikidata:Q8513 .

wikidata:Q54982412 rdfs:label "songwriting team"^^xsd:string ;
    rdfs:comment "team of two or more songwriters"^^xsd:string ;
    rdfs:subClassOf wikidata:Q16334295,
        wikidata:Q327245 .

wikidata:Q550089 rdfs:label "astronomical survey"^^xsd:string ;
    rdfs:comment "general map or image of a region of the sky with no specific observational target."^^xsd:string ;
    rdfs:subClassOf wikidata:Q1298668 .

wikidata:Q5519929 rdfs:label "game creation system"^^xsd:string ;
    rdfs:comment "self-contained game creation software"^^xsd:string ;
    rdfs:subClassOf wikidata:Q166142 .

wikidata:Q55214844 rdfs:label "medical procedure type"^^xsd:string ;
    rdfs:comment "type or family of medical procedure"^^xsd:string .

wikidata:Q55341040 rdfs:label "video game database"^^xsd:string ;
    rdfs:comment "video game database accessible through the internet"^^xsd:string ;
    rdfs:subClassOf wikidata:Q7094076 .

wikidata:Q55599109 rdfs:label "border crossing"^^xsd:string ;
    rdfs:comment "point for the crossing of international borders"^^xsd:string .

wikidata:Q55648452 rdfs:label "non-fungible token"^^xsd:string ;
    rdfs:comment "special type of cryptographic token which represents something unique"^^xsd:string .

wikidata:Q55657615 rdfs:label "commission"^^xsd:string ;
    rdfs:comment "group of appointed persons given a mandate to perform some duty"^^xsd:string ;
    rdfs:subClassOf wikidata:Q4358176 .

wikidata:Q55760865 rdfs:label "sketch"^^xsd:string ;
    rdfs:comment "short comedy scene or vignette"^^xsd:string ;
    rdfs:subClassOf wikidata:Q1185607,
        wikidata:Q386724 .

wikidata:Q55833 rdfs:label "supercontinent"^^xsd:string ;
    rdfs:comment "landmass comprising more than one continental core, or craton"^^xsd:string ;
    rdfs:subClassOf wikidata:Q5107 .

wikidata:Q55876909 rdfs:label "catholic parish church"^^xsd:string ;
    rdfs:comment "church that acts as the religious center of a Catholic parish"^^xsd:string ;
    rdfs:subClassOf wikidata:Q1088552,
        wikidata:Q317557 .

wikidata:Q559026 rdfs:label "ship class"^^xsd:string ;
    rdfs:comment "group of ships of a similar design"^^xsd:string .

wikidata:Q55990535 rdfs:label "computer model"^^xsd:string ;
    rdfs:comment "computer with specific abilities"^^xsd:string ;
    rdfs:subClassOf wikidata:Q10929058 .

wikidata:Q56055944 rdfs:label "art form"^^xsd:string ;
    rdfs:comment "form of art distinguished by its medium of expression (e.g. literature, music, visual arts)"^^xsd:string .

wikidata:Q5639 rdfs:label "trolleybus"^^xsd:string ;
    rdfs:comment "Electric bus that draws power from dual overhead wires"^^xsd:string .

wikidata:Q56670043 rdfs:label "fictional municipal police"^^xsd:string ;
    rdfs:comment "fictional law enforcement agencies that only exists in a work of fiction"^^xsd:string .

wikidata:Q56682555 rdfs:label "video game console model"^^xsd:string ;
    rdfs:comment "model of a video game console with other properties than it"^^xsd:string ;
    rdfs:subClassOf wikidata:Q10929058 .

wikidata:Q567696 rdfs:label "order"^^xsd:string ;
    rdfs:comment "instruction directed by law, judgment or administrative act to a natural or legal person to obey a certain behavior"^^xsd:string .

wikidata:Q56884562 rdfs:label "animated film series"^^xsd:string ;
    rdfs:comment "series of animated films"^^xsd:string ;
    rdfs:subClassOf wikidata:Q24856 .

wikidata:Q57305 rdfs:label "trade fair"^^xsd:string ;
    rdfs:comment "exhibition organized so that companies can showcase or/and demonstrate their newest products"^^xsd:string .

wikidata:Q5767753 rdfs:label "style"^^xsd:string ;
    rdfs:comment "legal, official, or recognized title"^^xsd:string .

wikidata:Q57790812 rdfs:label "print book"^^xsd:string ;
    rdfs:comment "physical book printed on paper"^^xsd:string ;
    rdfs:subClassOf wikidata:Q1261026,
        wikidata:Q571 .

wikidata:Q57821 rdfs:label "fortification"^^xsd:string ;
    rdfs:comment "military constructions and buildings designed for defense in warfare and military bases"^^xsd:string .

wikidata:Q58197759 rdfs:label "hurricane"^^xsd:string ;
    rdfs:comment "group of tropical storms of the Atlantic and east Pacific basins with sustained wind speeds > 64 kt. Classified by Saffir–Simpson sale"^^xsd:string .

wikidata:Q58481926 rdfs:label "typeface family"^^xsd:string ;
    rdfs:comment "group of stylistically related typefaces"^^xsd:string ;
    rdfs:subClassOf wikidata:Q16887380,
        wikidata:Q386724 .

wikidata:Q5891 rdfs:label "philosophy"^^xsd:string ;
    rdfs:comment "intellectual and/or logical study of general and fundamental problems"^^xsd:string .

wikidata:Q589183 rdfs:label "radio format"^^xsd:string ;
    rdfs:comment "overall content broadcast on a radio station"^^xsd:string .

wikidata:Q58927801 rdfs:label "ethical theory"^^xsd:string ;
    rdfs:comment "philosophically coherent set of propositions related to ethics or morality"^^xsd:string .

wikidata:Q59152282 rdfs:label "video streaming service"^^xsd:string ;
    rdfs:comment "service that delivers video content via the Internet"^^xsd:string .

wikidata:Q59163902 rdfs:label "musical production"^^xsd:string ;
    rdfs:comment "run of quasi-identical performances of the same music work"^^xsd:string ;
    rdfs:subClassOf wikidata:Q43099500 .

wikidata:Q59755569 rdfs:label "special purpose artist"^^xsd:string ;
    rdfs:comment "type of artist credit used when the original creator of a musical work is unknown, anonymous, a corporate pseudonym, or in the the public domain"^^xsd:string ;
    rdfs:subClassOf wikidata:Q16334295 .

wikidata:Q60031086 rdfs:label "branch of pseudoscience"^^xsd:string ;
    rdfs:comment "discipline which is claimed to be scientific, but fails to meet the criteria of a science"^^xsd:string ;
    rdfs:subClassOf wikidata:Q1047113 .

wikidata:Q60153785 rdfs:label "fictional radio station"^^xsd:string ;
    rdfs:comment "radio station which only exist in a work of fiction"^^xsd:string ;
    rdfs:subClassOf wikidata:Q5446565 .

wikidata:Q60469796 rdfs:label "religious symbol"^^xsd:string ;
    rdfs:comment "iconic representation intended to represent a specific religion, or a concept within a given religion"^^xsd:string ;
    rdfs:subClassOf wikidata:Q80071 .

wikidata:Q60614352 rdfs:label "uncredited artist"^^xsd:string ;
    rdfs:comment "session musician or backing band participating on a recording but whose name is not on the cover"^^xsd:string ;
    rdfs:subClassOf wikidata:Q713200 .

wikidata:Q60644919 rdfs:label "fictional video game console"^^xsd:string ;
    rdfs:comment "video game console in a narrative form of arts"^^xsd:string ;
    rdfs:subClassOf wikidata:Q15706911 .

wikidata:Q607241 rdfs:label "clergy house"^^xsd:string ;
    rdfs:comment "buildings in connection with a church used for secular activities"^^xsd:string ;
    rdfs:subClassOf wikidata:Q3947 .

wikidata:Q6138528 rdfs:label "political coalition"^^xsd:string ;
    rdfs:comment "cooperation by political parties"^^xsd:string ;
    rdfs:subClassOf wikidata:Q124964 .

wikidata:Q620225 rdfs:label "apostolic vicariate"^^xsd:string ;
    rdfs:comment "Diözese unter päpstlicher Hoheit"^^xsd:string .

wikidata:Q621636 rdfs:label "route of administration"^^xsd:string ;
    rdfs:comment "path by which a drug, fluid, poison, or other substance is taken into the body"^^xsd:string .

wikidata:Q62302889 rdfs:label "art practice"^^xsd:string ;
    rdfs:comment "academic discipline"^^xsd:string .

wikidata:Q625994 rdfs:label "convention"^^xsd:string ;
    rdfs:comment "meeting of a group of individuals and/or companies in a certain field"^^xsd:string ;
    rdfs:subClassOf wikidata:Q1656682 .

wikidata:Q62662717 rdfs:label "fictional place of worship"^^xsd:string ;
    rdfs:comment "place of worship that only exists in a work of fiction"^^xsd:string ;
    rdfs:subClassOf wikidata:Q3895768 .

wikidata:Q62792750 rdfs:label "Spanish noble family"^^xsd:string ;
    rdfs:comment "family belonging to the Spanish aristocracy"^^xsd:string ;
    rdfs:subClassOf wikidata:Q13417114 .

wikidata:Q628455 rdfs:label "rite"^^xsd:string ;
    rdfs:comment "established, ceremonial, usually religious, act"^^xsd:string .

wikidata:Q630010 rdfs:label "reciprocating engine"^^xsd:string ;
    rdfs:comment "heat engine that uses one or more reciprocating pistons to convert pressure into a rotating motion"^^xsd:string .

wikidata:Q63183159 rdfs:label "series of video game compilations"^^xsd:string ;
    rdfs:comment "series of video game compilations with the same name"^^xsd:string ;
    rdfs:subClassOf wikidata:Q7058673 .

wikidata:Q63188808 rdfs:label "Catholic religious occupation"^^xsd:string ;
    rdfs:comment ""^^xsd:string ;
    rdfs:subClassOf wikidata:Q4164871,
        wikidata:Q63188683 .

wikidata:Q63483382 rdfs:label "song contest entry"^^xsd:string ;
    rdfs:comment "song+artist combination participating in a song competition"^^xsd:string ;
    rdfs:subClassOf wikidata:Q6942562 .

wikidata:Q63533016 rdfs:label "game engine version"^^xsd:string ;
    rdfs:comment "defined and identifiable development stage of a game engine"^^xsd:string ;
    rdfs:subClassOf wikidata:Q20826013 .

wikidata:Q6368 rdfs:label "web browser"^^xsd:string ;
    rdfs:comment "software application for retrieving, presenting, and traversing information resources on the World Wide Web"^^xsd:string ;
    rdfs:subClassOf wikidata:Q166142,
        wikidata:Q241317 .

wikidata:Q639030 rdfs:label "people mover"^^xsd:string ;
    rdfs:comment "automated guideway transit system, generally serving relatively small areas such as airports, downtown districts or theme parks"^^xsd:string ;
    rdfs:subClassOf wikidata:Q1067164 .

wikidata:Q64272108 rdfs:label "cultural festival"^^xsd:string ;
    rdfs:comment "event celebrating a culture"^^xsd:string ;
    rdfs:subClassOf wikidata:Q132241 .

wikidata:Q64341971 rdfs:label "single series"^^xsd:string ;
    rdfs:comment "series of recorded music released in single format"^^xsd:string ;
    rdfs:subClassOf wikidata:Q7725310 .

wikidata:Q64353859 rdfs:label "Police Squad"^^xsd:string ;
    rdfs:comment "לתיאור יחידה משטרתית"^^xsd:string ;
    rdfs:subClassOf wikidata:Q35535 .

wikidata:Q6453643 rdfs:label "decree law"^^xsd:string ;
    rdfs:comment "lei que emana do Poder Executivo"^^xsd:string ;
    rdfs:subClassOf wikidata:Q49371 .

wikidata:Q64682301 rdfs:label "fictional flag"^^xsd:string ;
    rdfs:comment "flag which only exists in fiction"^^xsd:string ;
    rdfs:subClassOf wikidata:Q15706911 .

wikidata:Q64917966 rdfs:label "sample"^^xsd:string ;
    rdfs:comment "recorded piece of sound that is used as part of a piece of music"^^xsd:string .

wikidata:Q6498903 rdfs:label "supervillain"^^xsd:string ;
    rdfs:comment "variant of the villain character type, sometimes possessing \"supernatural or superhuman powers\""^^xsd:string .

wikidata:Q6500733 rdfs:label "printer"^^xsd:string ;
    rdfs:comment "company for printed products"^^xsd:string ;
    rdfs:subClassOf wikidata:Q4830453 .

wikidata:Q6501447 rdfs:label "local government"^^xsd:string ;
    rdfs:comment "lowest tier of administration within a given state"^^xsd:string ;
    rdfs:subClassOf wikidata:Q43229,
        wikidata:Q7188 .

wikidata:Q6502154 rdfs:label "exploration"^^xsd:string ;
    rdfs:comment "act of searching or traveling around a terrain for the purpose of discovery"^^xsd:string .

wikidata:Q65091986 rdfs:label "soundtrack single"^^xsd:string ;
    rdfs:comment "single containing music from another work, such as a film, video game, radio programme or television series"^^xsd:string ;
    rdfs:subClassOf wikidata:Q134556 .

wikidata:Q65554936 rdfs:label "fictional legislation"^^xsd:string ;
    rdfs:comment "legislation which only exists in a work of fiction"^^xsd:string ;
    rdfs:subClassOf wikidata:Q14897293 .

wikidata:Q6566418 rdfs:label "Catholic particular church sui iuris"^^xsd:string ;
    rdfs:comment "autonomous particular church of the Catholic Church"^^xsd:string ;
    rdfs:subClassOf wikidata:Q51041800 .

wikidata:Q657449 rdfs:label "parade"^^xsd:string ;
    rdfs:comment "procession of people"^^xsd:string ;
    rdfs:subClassOf wikidata:Q1656682,
        wikidata:Q3533467 .

wikidata:Q66049140 rdfs:label "soundtrack extended play"^^xsd:string ;
    rdfs:comment "extended play containing music from another work, such as a film, video game, television series"^^xsd:string ;
    rdfs:subClassOf wikidata:Q169930 .

wikidata:Q6619719 rdfs:label "fictional music group"^^xsd:string ;
    rdfs:comment "music group appearing in fictional stories"^^xsd:string ;
    rdfs:subClassOf wikidata:Q14514600 .

wikidata:Q66374263 rdfs:label "religion of an area"^^xsd:string ;
    rdfs:comment "distinct religious practices and beliefs held, that take place in, or originate from, a geographic location"^^xsd:string ;
    rdfs:subClassOf wikidata:Q74817647,
        wikidata:Q9174 .

wikidata:Q66547481 rdfs:label "fictional television network"^^xsd:string ;
    rdfs:comment "television network which only exists in a work of fiction"^^xsd:string ;
    rdfs:subClassOf wikidata:Q5446565 .

wikidata:Q673383 rdfs:label "stamp series"^^xsd:string ;
    rdfs:comment "type of series"^^xsd:string ;
    rdfs:subClassOf wikidata:Q20937557,
        wikidata:Q37930 .

wikidata:Q681615 rdfs:label "syndicate"^^xsd:string ;
    rdfs:comment "social organisations of various types"^^xsd:string ;
    rdfs:subClassOf wikidata:Q12047392,
        wikidata:Q43229 .

wikidata:Q68183127 rdfs:label "content descriptor"^^xsd:string ;
    rdfs:comment "single content descriptor in a rating system"^^xsd:string .

wikidata:Q682626 rdfs:label "audio file format"^^xsd:string ;
    rdfs:comment "file format for storing digital audio data on a computer system"^^xsd:string ;
    rdfs:subClassOf wikidata:Q235557 .

wikidata:Q6866562 rdfs:label "ministry"^^xsd:string ;
    rdfs:comment "collective body of government ministers"^^xsd:string ;
    rdfs:subClassOf wikidata:Q35798,
        wikidata:Q4358176 .

wikidata:Q686822 rdfs:label "bill"^^xsd:string ;
    rdfs:comment "proposed law"^^xsd:string ;
    rdfs:subClassOf wikidata:Q49848 .

wikidata:Q690768 rdfs:label "black magic"^^xsd:string ;
    rdfs:comment "use of supernatural powers or magic for evil and selfish purposes"^^xsd:string .

wikidata:Q6942560 rdfs:label "musical repertoire"^^xsd:string ;
    rdfs:comment "set of prepared musical compositions"^^xsd:string ;
    rdfs:subClassOf wikidata:Q17489659 .

wikidata:Q694554 rdfs:label "emergency telephone number"^^xsd:string ;
    rdfs:comment "telephone number that allows caller to contact local emergency services for assistance"^^xsd:string ;
    rdfs:subClassOf wikidata:Q214995 .

wikidata:Q697175 rdfs:label "launch vehicle"^^xsd:string ;
    rdfs:comment "rocket used to carry payload into outer space"^^xsd:string .

wikidata:Q69719735 rdfs:label "drive-through tree"^^xsd:string ;
    rdfs:comment ""^^xsd:string ;
    rdfs:subClassOf wikidata:Q44377 .

wikidata:Q699907 rdfs:label "capitulary"^^xsd:string ;
    rdfs:comment "Carolingian legal document"^^xsd:string ;
    rdfs:subClassOf wikidata:Q49848 .

wikidata:Q70208 rdfs:label "municipality of Switzerland"^^xsd:string ;
    rdfs:comment "smallest government division in Switzerland"^^xsd:string .

wikidata:Q7079603 rdfs:label "official statistics"^^xsd:string ;
    rdfs:comment "statistics published by government agencies or other public bodies such as international organizations as a public good"^^xsd:string ;
    rdfs:subClassOf wikidata:Q1172284,
        wikidata:Q340169 .

wikidata:Q71550118 rdfs:label "individual quantity"^^xsd:string ;
    rdfs:comment "superclass of physical, chemical, ... quantity; members are individual quantities like 5 kg, 2 apples, ..."^^xsd:string ;
    rdfs:subClassOf wikidata:Q15619164 .

wikidata:Q72082844 rdfs:label "protected area section"^^xsd:string ;
    rdfs:comment "sous-partie d'une zone destinée à la conservation naturelle"^^xsd:string ;
    rdfs:subClassOf wikidata:Q1496967 .

wikidata:Q721747 rdfs:label "commemorative plaque"^^xsd:string ;
    rdfs:comment "plate or tablet fixed to a wall to mark an event, person, etc"^^xsd:string ;
    rdfs:subClassOf wikidata:Q5003624 .

wikidata:Q7217761 rdfs:label "manned spacecraft"^^xsd:string ;
    rdfs:comment "spacecraft designed to carry humans"^^xsd:string ;
    rdfs:subClassOf wikidata:Q40218 .

wikidata:Q721830 rdfs:label "pay television"^^xsd:string ;
    rdfs:comment "subscription-based television services"^^xsd:string .

wikidata:Q723685 rdfs:label "video on demand"^^xsd:string ;
    rdfs:comment "systems which allow users to select and watch/listen to video or audio content on demand"^^xsd:string .

wikidata:Q7247847 rdfs:label "production team"^^xsd:string ;
    rdfs:comment "group of technical staff who produce a play, television show, recording or film"^^xsd:string ;
    rdfs:subClassOf wikidata:Q327245 .

wikidata:Q7252 rdfs:label "feminism"^^xsd:string ;
    rdfs:comment "group of movements that come about defining, and defending gender equity, including equal rights for women and girls"^^xsd:string .

wikidata:Q72588 rdfs:label "content delivery network"^^xsd:string ;
    rdfs:comment "umbrella term spanning different types of content delivery services"^^xsd:string ;
    rdfs:subClassOf wikidata:Q1301371 .

wikidata:Q7278 rdfs:label "political party"^^xsd:string ;
    rdfs:comment "organized group of people who have the same ideology, or who otherwise have the same political positions, and who field candidates for elections, in an attempt to get them elected and thereby implement their agenda"^^xsd:string ;
    rdfs:subClassOf wikidata:Q155076,
        wikidata:Q7210356 .

wikidata:Q736427 rdfs:label "staple food"^^xsd:string ;
    rdfs:comment "food that is eaten routinely, and considered a dominant portion of a standard diet"^^xsd:string ;
    rdfs:subClassOf wikidata:Q2095 .

wikidata:Q7380 rdfs:label "primate"^^xsd:string ;
    rdfs:comment "order of mammals"^^xsd:string .

wikidata:Q7410139 rdfs:label "sample library"^^xsd:string ;
    rdfs:comment "collection of digital sound recordings, known as samples, for use by composers, arrangers, performers, and producers of music"^^xsd:string .

wikidata:Q7432 rdfs:label "species"^^xsd:string ;
    rdfs:comment "one of the basic units of biological classification and a taxonomic rank"^^xsd:string .

wikidata:Q744913 rdfs:label "aviation accident"^^xsd:string ;
    rdfs:comment "aviation occurrence involving serious injury, death, or destruction of aircraft"^^xsd:string .

wikidata:Q746369 rdfs:label "recording studio"^^xsd:string ;
    rdfs:comment "facility for sound recording"^^xsd:string ;
    rdfs:subClassOf wikidata:Q13226383 .

wikidata:Q746611 rdfs:label "DVD region code"^^xsd:string ;
    rdfs:comment "characteristic of DVDs"^^xsd:string .

wikidata:Q768186 rdfs:label "sports equipment"^^xsd:string ;
    rdfs:comment "object used for sport or exercise"^^xsd:string ;
    rdfs:subClassOf wikidata:Q16798631 .

wikidata:Q771035 rdfs:label "traditional medicine"^^xsd:string ;
    rdfs:comment "medicine based on traditional beliefs"^^xsd:string .

wikidata:Q7777570 rdfs:label "theatrical production"^^xsd:string ;
    rdfs:comment "production consisting of a run of quasi-identical performances of the same theatrical work"^^xsd:string ;
    rdfs:subClassOf wikidata:Q43099500 .

wikidata:Q781132 rdfs:label "military branch"^^xsd:string ;
    rdfs:comment "subdivision of the national armed forces of a sovereign nation or state"^^xsd:string ;
    rdfs:subClassOf wikidata:Q176799 .

wikidata:Q7832362 rdfs:label "traditional story"^^xsd:string ;
    rdfs:comment "stories about traditions, like legends, folk tales, myths, fairy tales"^^xsd:string .

wikidata:Q7860947 rdfs:label "Types of bowlers in cricket"^^xsd:string ;
    rdfs:comment ""^^xsd:string .

wikidata:Q78758464 rdfs:label "broadcasting licence area"^^xsd:string ;
    rdfs:comment "geographical area for which a broadcasting licence has been issued"^^xsd:string ;
    rdfs:subClassOf wikidata:Q15642541 .

wikidata:Q79250806 rdfs:label "fictional document"^^xsd:string ;
    rdfs:comment "document which only exists in a work of fiction"^^xsd:string ;
    rdfs:subClassOf wikidata:Q15306849 .

wikidata:Q7927908 rdfs:label "video game accessory"^^xsd:string ;
    rdfs:comment "type of accessory"^^xsd:string .

wikidata:Q7946 rdfs:label "mineral"^^xsd:string ;
    rdfs:comment "naturally occurring usually inorganic substance that has a (more or less) definite chemical composition and a crystal structure"^^xsd:string ;
    rdfs:subClassOf wikidata:Q214609,
        wikidata:Q79529 .

wikidata:Q79509036 rdfs:label "portfolio"^^xsd:string ;
    rdfs:comment "unbound collection of visual artworks housed in a binder, folder or other container"^^xsd:string ;
    rdfs:subClassOf wikidata:Q16887380 .

wikidata:Q79600797 rdfs:label "synthetic voice"^^xsd:string ;
    rdfs:comment "a human sounding voice generated by a computer"^^xsd:string ;
    rdfs:subClassOf wikidata:Q7397 .

wikidata:Q798134 rdfs:label "bachelor thesis"^^xsd:string ;
    rdfs:comment "a thesis reporting a research project undertaken as part of an undergraduate course of education leading to a bachelor's degree"^^xsd:string ;
    rdfs:subClassOf wikidata:Q1266946 .

wikidata:Q7982 rdfs:label "CD-ROM"^^xsd:string ;
    rdfs:comment "pre-pressed compact disc containing computer data"^^xsd:string ;
    rdfs:subClassOf wikidata:Q1048236,
        wikidata:Q386724 .

wikidata:Q8072 rdfs:label "volcano"^^xsd:string ;
    rdfs:comment "natural, surface vent or fissure usually in a mountainous form"^^xsd:string ;
    rdfs:subClassOf wikidata:Q31464082,
        wikidata:Q8502 .

wikidata:Q808 rdfs:label "virus"^^xsd:string ;
    rdfs:comment "non-cellular, submicroscopic infectious agent that replicates only inside the living cells of an organism"^^xsd:string .

wikidata:Q80831 rdfs:label "integrated circuit"^^xsd:string ;
    rdfs:comment "electronic circuit manufactured by lithography; set of electronic circuits on one small flat piece of semiconductor material, normally silicon"^^xsd:string .

wikidata:Q8161 rdfs:label "tax"^^xsd:string ;
    rdfs:comment "method to impose financial charge or other levy upon a taxpayer by a government or functional equivalent"^^xsd:string ;
    rdfs:subClassOf wikidata:Q7748 .

wikidata:Q81935689 rdfs:label "gramophone record format"^^xsd:string ;
    rdfs:comment "physical format and playback speed of a gramophone record"^^xsd:string ;
    rdfs:subClassOf wikidata:Q1207505,
        wikidata:Q82036085 .

wikidata:Q81945865 rdfs:label "multi-disc album format"^^xsd:string ;
    rdfs:comment "music album which spans two or more units of the primary medium in which it is sold or distributed"^^xsd:string ;
    rdfs:subClassOf wikidata:Q482994 .

wikidata:Q81986407 rdfs:label "e-book file format"^^xsd:string ;
    rdfs:comment "type of file format used by e-books"^^xsd:string ;
    rdfs:subClassOf wikidata:Q235557 .

wikidata:Q82014556 rdfs:label "streaming channel"^^xsd:string ;
    rdfs:comment "type of video stream"^^xsd:string ;
    rdfs:subClassOf wikidata:Q2001305 .

wikidata:Q82046811 rdfs:label "print book format"^^xsd:string ;
    rdfs:comment "physical format of a printed book"^^xsd:string ;
    rdfs:subClassOf wikidata:Q82036085 .

wikidata:Q820477 rdfs:label "mine"^^xsd:string ;
    rdfs:comment "place for the extraction of minerals"^^xsd:string ;
    rdfs:subClassOf wikidata:Q13226383 .

wikidata:Q8217193 rdfs:label "subdialect"^^xsd:string ;
    rdfs:comment "dialectological category between the levels of dialect and idiolect"^^xsd:string .

wikidata:Q82604 rdfs:label "design"^^xsd:string ;
    rdfs:comment "creation of a plan or convention for the construction of an object or a system; process of creation; act of creativity and innovation"^^xsd:string ;
    rdfs:subClassOf wikidata:Q1914636,
        wikidata:Q3249551 .

wikidata:Q829080 rdfs:label "professional association"^^xsd:string ;
    rdfs:comment "typically nonprofit organization seeking to further a particular profession"^^xsd:string ;
    rdfs:subClassOf wikidata:Q15911314,
        wikidata:Q43229,
        wikidata:Q48204 .

wikidata:Q830450 rdfs:label "microform"^^xsd:string ;
    rdfs:comment "scaled-down reproductions of documents made for the purposes of transmission, storage, reading, and printing"^^xsd:string ;
    rdfs:subClassOf wikidata:Q81941037 .

wikidata:Q836575 rdfs:label "quality assurance"^^xsd:string ;
    rdfs:comment "way of preventing mistakes or defects in manufactured products and avoiding problems when delivering solutions or services to customers; (ISO 9000) part of quality management focused on providing confidence that quality requirements will be fulfilled"^^xsd:string .

wikidata:Q837142 rdfs:label "nursing home"^^xsd:string ;
    rdfs:comment "type of residential care"^^xsd:string .

wikidata:Q842332 rdfs:label "war front"^^xsd:string ;
    rdfs:comment "contested armed frontier between opposing forces"^^xsd:string ;
    rdfs:subClassOf wikidata:Q718893 .

wikidata:Q8432 rdfs:label "civilization"^^xsd:string ;
    rdfs:comment "organized cultural society that encounters many communities, on a scale of a nation or human, as well as a system of development"^^xsd:string .

wikidata:Q8434 rdfs:label "education"^^xsd:string ;
    rdfs:comment "learning in which knowledge and skills are transferred through teaching"^^xsd:string ;
    rdfs:subClassOf wikidata:Q7406919 .

wikidata:Q8473 rdfs:label "military"^^xsd:string ;
    rdfs:comment "organized body primarily tasked with preparing for and conducting war"^^xsd:string ;
    rdfs:subClassOf wikidata:Q17149090 .

wikidata:Q855697 rdfs:label "subcontinent"^^xsd:string ;
    rdfs:comment "large, relatively self-contained landmass forming a subdivision of a continent"^^xsd:string ;
    rdfs:subClassOf wikidata:Q82794 .

wikidata:Q855973 rdfs:label "commemorative coin"^^xsd:string ;
    rdfs:comment "coins issued to commemorate some particular event or issue"^^xsd:string .

wikidata:Q863531 rdfs:label "monkeys in space"^^xsd:string ;
    rdfs:comment "space travel by monkeys"^^xsd:string .

wikidata:Q864114 rdfs:label "input device"^^xsd:string ;
    rdfs:comment "peripheral to provide data and signals to an information processing system"^^xsd:string ;
    rdfs:subClassOf wikidata:Q178648,
        wikidata:Q47146 .

wikidata:Q867393 rdfs:label "amenity"^^xsd:string ;
    rdfs:comment "infrastructure available for use and improving quality of life"^^xsd:string ;
    rdfs:subClassOf wikidata:Q7406919 .

wikidata:Q86850 rdfs:label "film gauge"^^xsd:string ;
    rdfs:comment "width of photographic or motion picture film"^^xsd:string ;
    rdfs:subClassOf wikidata:Q759853 .

wikidata:Q870 rdfs:label "train"^^xsd:string ;
    rdfs:comment "form of rail transport consisting of a series of connected vehicles"^^xsd:string .

wikidata:Q87167 rdfs:label "manuscript"^^xsd:string ;
    rdfs:comment "document written by hand"^^xsd:string ;
    rdfs:subClassOf wikidata:Q18593264,
        wikidata:Q49848 .

wikidata:Q892168 rdfs:label "causeway"^^xsd:string ;
    rdfs:comment "route raised up on an embankment"^^xsd:string ;
    rdfs:subClassOf wikidata:Q618123,
        wikidata:Q83620 .

wikidata:Q89753576 rdfs:label "assembly (the subject of article 11 ECHR)"^^xsd:string ;
    rdfs:comment "Eine Zusammenkunft von Menschen mit einem gemeinsamen Zweck (z.B. unterschiedliche Meinungen diskutieren; gemeinsame Meinungen bekunden; einem Vortrag zu hören) - sei es unter freiem Himmel oder in geschlossenen Räumen"^^xsd:string ;
    rdfs:subClassOf wikidata:Q16334295 .

wikidata:Q898786 rdfs:label "crystal system"^^xsd:string ;
    rdfs:comment "class of space groups, lattices, point groups, or crystals"^^xsd:string .

wikidata:Q904997 rdfs:label "diaporama"^^xsd:string ;
    rdfs:comment "succession de diapositives destinées à être projetées sur écran et intégrant ou non une bande sonore"^^xsd:string .

wikidata:Q905151 rdfs:label "ballot"^^xsd:string ;
    rdfs:comment "document used to cast votes in an election"^^xsd:string .

wikidata:Q905765 rdfs:label "Command paper"^^xsd:string ;
    rdfs:comment "Command paper, a type of UK government document used in parliamentary presentations"^^xsd:string ;
    rdfs:subClassOf wikidata:Q49848 .

wikidata:Q91197994 rdfs:label "military unit designation"^^xsd:string ;
    rdfs:comment "official name or identifier used by one or more military formations"^^xsd:string ;
    rdfs:subClassOf wikidata:Q853614 .

wikidata:Q9259 rdfs:label "UNESCO World Heritage Site"^^xsd:string ;
    rdfs:comment "place listed by the UNESCO as of special cultural or physical significance"^^xsd:string ;
    rdfs:subClassOf wikidata:Q210272,
        wikidata:Q386426 .

wikidata:Q93267 rdfs:label "isthmus"^^xsd:string ;
    rdfs:comment "narrow strip of land connecting two larger land areas"^^xsd:string ;
    rdfs:subClassOf wikidata:Q271669 .

wikidata:Q933348 rdfs:label "commemorative publication"^^xsd:string ;
    rdfs:comment "publication for the celebration of a jubilee (person or organisation); academic work honoring a respected person, usually an academic, and presented during their lifetime"^^xsd:string ;
    rdfs:subClassOf wikidata:Q386724,
        wikidata:Q618779 .

wikidata:Q933394 rdfs:label "exclave"^^xsd:string ;
    rdfs:comment "territory legally or politically attached to a main territory with which it is not physically contiguous because of surrounding alien territory"^^xsd:string .

wikidata:Q943929 rdfs:label "traditional song"^^xsd:string ;
    rdfs:comment "song with anonymous or unknown writer without authorized original version; song that is part of the oral tradition"^^xsd:string ;
    rdfs:subClassOf wikidata:Q7366 .

wikidata:Q947662 rdfs:label "binary asteroid"^^xsd:string ;
    rdfs:comment "system of two asteroids orbiting their common center of mass"^^xsd:string .

wikidata:Q9655 rdfs:label "artery"^^xsd:string ;
    rdfs:comment "blood vessel that carry blood away from the heart"^^xsd:string .

wikidata:Q968159 rdfs:label "art movement"^^xsd:string ;
    rdfs:comment "tendency or style in art with a specific common philosophy or goal, possibly associated with a specific historical period"^^xsd:string ;
    rdfs:subClassOf wikidata:Q2198855,
        wikidata:Q735 .

wikidata:Q978 rdfs:label "meme"^^xsd:string ;
    rdfs:comment "idea, behavior or style that spreads within a culture"^^xsd:string ;
    rdfs:subClassOf wikidata:Q11028,
        wikidata:Q17537576 .

wikidata:Q98216532 rdfs:label "recording session"^^xsd:string ;
    rdfs:comment "period of time devoted to recording music in a studio"^^xsd:string ;
    rdfs:subClassOf wikidata:Q1190554 .

wikidata:Q98491862 rdfs:label "committee directives"^^xsd:string ;
    rdfs:comment "terms of reference of a commission of inquiry"^^xsd:string ;
    rdfs:subClassOf wikidata:Q49848 .

wikidata:Q989255 rdfs:label "Middle-earth race"^^xsd:string ;
    rdfs:comment "a fictional race within Tolkien's Middle-earth universe, for peoples use Q17412916"^^xsd:string ;
    rdfs:subClassOf wikidata:Q2590445 .

wikidata:Q995347 rdfs:label "Christian movement"^^xsd:string ;
    rdfs:comment "theological, political, or philosophical interpretation of Christianity that is not generally represented by a specific church, sect, or denomination"^^xsd:string ;
    rdfs:subClassOf wikidata:Q1826286 .

wikidata:Q99659193 rdfs:label "referendum options"^^xsd:string ;
    rdfs:comment "object referendum questions"^^xsd:string .

wikidata:Q99731370 rdfs:label "range of days of the week"^^xsd:string ;
    rdfs:comment ""^^xsd:string .

wikidata:P127 rdfs:label "owned by"^^xsd:string ;
    rdf:first <http://www.semanticweb.org/ontologies/Wikidata#_:y6>,
        <http://www.semanticweb.org/ontologies/Wikidata#_:y8> ;
    rdfs:comment "owner of the subject"^^xsd:string ;
    rdfs:domain wikidata:Q1496967,
        wikidata:Q15401930,
        wikidata:Q26401003,
        wikidata:Q43229,
        wikidata:Q4406616,
        wikidata:Q473972,
        wikidata:Q6671777 ;
    rdfs:range wikidata:Q14623646,
        wikidata:Q215627,
        wikidata:Q34627,
        wikidata:Q3778211,
        wikidata:Q43229,
        wikidata:Q56061,
        wikidata:Q874405,
        wikidata:Q95074 .

wikidata:P131 rdfs:label "located in the administrative territorial entity"^^xsd:string ;
    rdfs:comment "the item is located on the territory of the following administrative entity. Use P276 (location) for specifying locations that are non-administrative places and for items about events"^^xsd:string .

wikidata:P1455 rdfs:label "list of works"^^xsd:string ;
    rdfs:comment "link to the article with the works of a person; use P358 for discographies"^^xsd:string ;
    rdfs:domain wikidata:Q215627 ;
    rdfs:range wikidata:Q100775361,
        wikidata:Q100775856,
        wikidata:Q1631107,
        wikidata:Q17099416,
        wikidata:Q2560570,
        wikidata:Q5051330 ;
    rdfs:subPropertyOf wikidata:P2354 .

wikidata:P155 rdfs:label "follows"^^xsd:string ;
    rdf:first <http://www.semanticweb.org/ontologies/Wikidata#_:y9> ;
    rdfs:comment "immediately prior item in a series of which the subject is a part [if the subject has replaced the preceding item, e.g. political offices, use \"replaces\" (P1365)]"^^xsd:string .

wikidata:P156 rdfs:label "followed by"^^xsd:string ;
    rdfs:comment "immediately following item in a series of which the subject is a part [if the subject has been replaced, e.g. political offices, use \"replaced by\" (P1366)]"^^xsd:string .

wikidata:P1889 a owl:SymmetricProperty ;
    rdfs:label "different from"^^xsd:string ;
    rdfs:comment "item that is different from another item, with which it is often confused"^^xsd:string .

wikidata:P2789 a owl:SymmetricProperty ;
    rdfs:label "connects with"^^xsd:string ;
    rdfs:comment "item with which the item is physically connected"^^xsd:string ;
    rdfs:subPropertyOf wikidata:P129 .

wikidata:P366 rdfs:label "use"^^xsd:string ;
    rdfs:comment "main use of the subject (includes current and former usage)"^^xsd:string .

wikidata:P462 rdfs:label "color"^^xsd:string ;
    rdfs:comment "color of subject"^^xsd:string ;
    rdfs:range wikidata:Q1075,
        wikidata:Q22006653 .

wikidata:P488 rdfs:label "chairperson"^^xsd:string ;
    rdfs:comment "presiding member of an organization, group or body"^^xsd:string ;
    rdfs:domain wikidata:Q14623646,
        wikidata:Q1656682,
        wikidata:Q21004260,
        wikidata:Q43229,
        wikidata:Q48204,
        wikidata:Q51041800,
        wikidata:Q829080 ;
    rdfs:range wikidata:Q5,
        wikidata:Q95074 ;
    rdfs:subPropertyOf wikidata:P3342 .

wikidata:P706 rdfs:label "located on terrain feature"^^xsd:string ;
    rdfs:comment "located on the specified landform. Should not be used when the value is only political/administrative (P131) or a mountain range (P4552)."^^xsd:string ;
    rdfs:domain wikidata:Q1190554,
        wikidata:Q1322005,
        wikidata:Q2221906,
        wikidata:Q24334893,
        wikidata:Q3099911,
        wikidata:Q3895768,
        wikidata:Q486972,
        wikidata:Q618123,
        wikidata:Q634 ;
    rdfs:range wikidata:Q2221906,
        wikidata:Q24334893,
        wikidata:Q3895768,
        wikidata:Q618123,
        wikidata:Q82794 ;
    rdfs:subPropertyOf wikidata:P276,
        wikidata:P361 .

wikidata:P8371 rdfs:label "references work, tradition or theory"^^xsd:string ;
    rdfs:comment "creative work, tradition or theory this creative work references by allusion, quote or similar means (for citations in scholarly and legal works use P2860, for other more specific properties have a look at \"see also\" on the property page)"^^xsd:string .

wikidata:P8546 rdfs:label "recording location"^^xsd:string ;
    rdfs:comment "location where a media item (sound/video/etc) was recorded"^^xsd:string .

wikidata:P8810 rdfs:label "parent (unspecified)"^^xsd:string ;
    rdfs:comment "parent of the subject. Only use if neither father (P22) nor mother (P25) is applicable"^^xsd:string .

wikidata:P942 rdfs:label "theme music"^^xsd:string ;
    rdfs:comment "the theme music/song used by the item"^^xsd:string ;
    rdfs:domain wikidata:Q1190554,
        wikidata:Q21070598,
        wikidata:Q2431196,
        wikidata:Q43229,
        wikidata:Q5,
        wikidata:Q95074 ;
    rdfs:range wikidata:Q2188189,
        wikidata:Q7302866,
        wikidata:Q7889 .

wikidata:Q1003030 rdfs:label "test"^^xsd:string ;
    rdfs:comment "way of checking something for quality or attributes"^^xsd:string .

wikidata:Q101965 rdfs:label "experiment"^^xsd:string ;
    rdfs:comment "scientific procedure carried out to support, refute, or validate a hypothesis"^^xsd:string ;
    rdfs:subClassOf wikidata:Q1003030 .

wikidata:Q1020767 rdfs:label "product bundling"^^xsd:string ;
    rdfs:comment "several products combined for sale as one product"^^xsd:string .

wikidata:Q102496 rdfs:label "parish"^^xsd:string ;
    rdfs:comment "type of ecclesiastical subdivision of a diocese"^^xsd:string ;
    rdfs:subClassOf wikidata:Q20926517,
        wikidata:Q51041800 .

wikidata:Q103817 rdfs:label "indigenous people"^^xsd:string ;
    rdfs:comment "ethnic group descended from and identified with the original inhabitants of a given region"^^xsd:string ;
    rdfs:subClassOf wikidata:Q2472587,
        wikidata:Q41710,
        wikidata:Q851990 .

wikidata:Q104347069 rdfs:label "lake system"^^xsd:string ;
    rdfs:comment "part of river basin formed by lakes connected with short rivers, straits or narrows.; system of surface and ground waters flowing into a common terminus such as the sea, lake or aquifer"^^xsd:string ;
    rdfs:subClassOf wikidata:Q166620 .

wikidata:Q105388829 rdfs:label "Roman Catholic diocese"^^xsd:string ;
    rdfs:comment "see under the supervision of a bishop of the Roman Catholic church"^^xsd:string ;
    rdfs:subClassOf wikidata:Q3146899 .

wikidata:Q1063547 rdfs:label "voice type"^^xsd:string ;
    rdfs:comment "group of voices with similar vocal ranges"^^xsd:string .

wikidata:Q106594095 rdfs:label "annual music competition edition"^^xsd:string ;
    rdfs:comment "edition in a specific year of an annual music competition, song contest, etc."^^xsd:string ;
    rdfs:subClassOf wikidata:Q27968055 .

wikidata:Q106833 rdfs:label "audiobook"^^xsd:string ;
    rdfs:comment "recording of a text being read"^^xsd:string ;
    rdfs:subClassOf wikidata:Q2431196,
        wikidata:Q571 .

wikidata:Q1088552 rdfs:label "Catholic church building"^^xsd:string ;
    rdfs:comment "church building of the Catholic Church (for the Catholic Church institution itself, use Q9592)"^^xsd:string ;
    rdfs:subClassOf wikidata:Q16970 .

wikidata:Q11016 rdfs:label "technology"^^xsd:string ;
    rdfs:comment "making, modification, usage, and knowledge of tools, machines, techniques, crafts, systems, and methods of organization"^^xsd:string .

wikidata:Q11032 rdfs:label "newspaper"^^xsd:string ;
    rdfs:comment "scheduled publication containing news of events, articles, features, editorials, and advertising"^^xsd:string ;
    rdfs:subClassOf wikidata:Q1002697,
        wikidata:Q28877,
        wikidata:Q43229,
        wikidata:Q4830453 .

wikidata:Q11173 rdfs:label "chemical compound"^^xsd:string ;
    rdfs:comment "pure chemical substance consisting of two or more different chemical elements"^^xsd:string .

wikidata:Q11204 rdfs:label "legislature"^^xsd:string ;
    rdfs:comment "kind of deliberative assembly with the power to pass, amend, and repeal laws"^^xsd:string ;
    rdfs:subClassOf wikidata:Q178706,
        wikidata:Q895526 .

wikidata:Q11344 rdfs:label "chemical element"^^xsd:string ;
    rdfs:comment "species of atoms having the same number of protons in the atomic nucleus"^^xsd:string .

wikidata:Q11410 rdfs:label "game"^^xsd:string ;
    rdfs:comment "a structured form of play, usually for entertainment"^^xsd:string .

wikidata:Q11446 rdfs:label "ship"^^xsd:string ;
    rdfs:comment "large buoyant watercraft"^^xsd:string ;
    rdfs:subClassOf wikidata:Q1229765 .

wikidata:Q11642595 rdfs:label "election campaign"^^xsd:string ;
    rdfs:comment "political campaign to win an election"^^xsd:string ;
    rdfs:subClassOf wikidata:Q847301 .

wikidata:Q1197685 rdfs:label "public holiday"^^xsd:string ;
    rdfs:comment "holiday generally established by law and is usually a non-working day for most people during the year"^^xsd:string ;
    rdfs:subClassOf wikidata:Q1445650 .

wikidata:Q1208380 rdfs:label "dialect group"^^xsd:string ;
    rdfs:comment "group of related dialects"^^xsd:string ;
    rdfs:subClassOf wikidata:Q17376908 .

wikidata:Q1209283 rdfs:label "electronic media"^^xsd:string ;
    rdfs:comment "media that use electronics or electromechanical energy for the audience to access the content"^^xsd:string ;
    rdfs:subClassOf wikidata:Q340169 .

wikidata:Q1210334 rdfs:label "railway bridge"^^xsd:string ;
    rdfs:comment "bridge that can be crossed by a train"^^xsd:string ;
    rdfs:subClassOf wikidata:Q12280,
        wikidata:Q1311670 .

wikidata:Q12143 rdfs:label "time zone"^^xsd:string ;
    rdfs:comment "region on Earth that has a uniform standard time for legal, commercial, and social purposes"^^xsd:string .

wikidata:Q1241356 rdfs:label "record"^^xsd:string ;
    rdfs:comment "quantified value of an event that is more extreme than that of all comparable events"^^xsd:string ;
    rdfs:subClassOf wikidata:Q1190554,
        wikidata:Q1207505 .

wikidata:Q124714 rdfs:label "spring"^^xsd:string ;
    rdfs:comment "water source"^^xsd:string ;
    rdfs:subClassOf wikidata:Q15324 .

wikidata:Q124734 rdfs:label "rebellion"^^xsd:string ;
    rdfs:comment "open resistance against the orders of an established authority that seeks to gain concessions from an oppressive power"^^xsd:string ;
    rdfs:subClassOf wikidata:Q180684 .

wikidata:Q1248784 rdfs:label "airport"^^xsd:string ;
    rdfs:comment "location where aircraft take off and land with extended support facilities for aircraft operation"^^xsd:string ;
    rdfs:subClassOf wikidata:Q12819564,
        wikidata:Q56061,
        wikidata:Q62447 .

wikidata:Q124964 rdfs:label "coalition"^^xsd:string ;
    rdfs:comment "alliance for combined action"^^xsd:string .

wikidata:Q12518 rdfs:label "tower"^^xsd:string ;
    rdfs:comment "structure with height greater than width"^^xsd:string ;
    rdfs:subClassOf wikidata:Q41176 .

wikidata:Q1261214 rdfs:label "television special"^^xsd:string ;
    rdfs:comment "type of television program"^^xsd:string ;
    rdfs:subClassOf wikidata:Q15416 .

wikidata:Q1269627 rdfs:label "amendment"^^xsd:string ;
    rdfs:comment "alteration made or proposed to be made in a bill or motion that adds, changes, substitutes, or omits"^^xsd:string .

wikidata:Q1277575 rdfs:label "correspondence"^^xsd:string ;
    rdfs:comment "mails or messages written by a person and sent to one or several other persons"^^xsd:string ;
    rdfs:subClassOf wikidata:Q37260 .

wikidata:Q1293220 rdfs:label "physical phenomenon"^^xsd:string ;
    rdfs:comment "phenomenon of the material world"^^xsd:string .

wikidata:Q1301371 rdfs:label "computer network"^^xsd:string ;
    rdfs:comment "network that allows computers to share resources and communicate with each other"^^xsd:string .

wikidata:Q131569 rdfs:label "treaty"^^xsd:string ;
    rdfs:comment "express agreement under international law entered into by actors in international law"^^xsd:string ;
    rdfs:subClassOf wikidata:Q1151067,
        wikidata:Q321839,
        wikidata:Q49848,
        wikidata:Q820655 .

wikidata:Q1318558 rdfs:label "operation point"^^xsd:string ;
    rdfs:comment "any non-straight feature  on a railway where an operation can take place"^^xsd:string .

wikidata:Q1322005 rdfs:label "natural phenomenon"^^xsd:string ;
    rdfs:comment "observable event which is not man-made"^^xsd:string .

wikidata:Q132364 rdfs:label "communications protocol"^^xsd:string ;
    rdfs:comment "system for exchanging messages between computing systems"^^xsd:string ;
    rdfs:subClassOf wikidata:Q317623 .

wikidata:Q133056 rdfs:label "mountain pass"^^xsd:string ;
    rdfs:comment "pass through a saddle or col to cross a mountain range"^^xsd:string .

wikidata:Q133311 rdfs:label "tribe"^^xsd:string ;
    rdfs:comment "social group existing before the development of, or outside of, states"^^xsd:string ;
    rdfs:subClassOf wikidata:Q41710,
        wikidata:Q874405 .

wikidata:Q134556 rdfs:label "single"^^xsd:string ;
    rdfs:comment "type of music release usually containing one or two tracks"^^xsd:string ;
    rdfs:subClassOf wikidata:Q2031291 .

wikidata:Q13473501 rdfs:label "collective"^^xsd:string ;
    rdfs:comment "group of entities sharing interest"^^xsd:string ;
    rdfs:subClassOf wikidata:Q16334295,
        wikidata:Q43229 .

wikidata:Q1348305 rdfs:label "erratum"^^xsd:string ;
    rdfs:comment "published correction to a previous publication"^^xsd:string ;
    rdfs:subClassOf wikidata:Q483394,
        wikidata:Q732577 .

wikidata:Q1362373 rdfs:label "cultigen"^^xsd:string ;
    rdfs:comment "plant that has been deliberately altered or selected by humans; result of artificial selection; man-made or anthropogenic plants"^^xsd:string ;
    rdfs:subClassOf wikidata:Q16334298,
        wikidata:Q2424752,
        wikidata:Q756 .

wikidata:Q1387659 rdfs:label "school of thought"^^xsd:string ;
    rdfs:comment "group of people sharing common outlook on an academic issue or field"^^xsd:string ;
    rdfs:subClassOf wikidata:Q16334295,
        wikidata:Q2198855 .

wikidata:Q14073567 rdfs:label "sibling duo"^^xsd:string ;
    rdfs:comment "two siblings that work together"^^xsd:string ;
    rdfs:subClassOf wikidata:Q10648343,
        wikidata:Q16334295,
        wikidata:Q16979650 .

wikidata:Q1408286 rdfs:label "production process"^^xsd:string ;
    rdfs:comment "process of producing goods"^^xsd:string .

wikidata:Q1414135 rdfs:label "rolling stock"^^xsd:string ;
    rdfs:comment "railway vehicles, both powered & unpowered"^^xsd:string .

wikidata:Q1415274 rdfs:label "film set"^^xsd:string ;
    rdfs:comment "luogo in cui si svolgono le riprese cinematografiche"^^xsd:string ;
    rdfs:subClassOf wikidata:Q27096235 .

wikidata:Q144 rdfs:label "dog"^^xsd:string ;
    rdfs:comment "domestic animal"^^xsd:string ;
    rdfs:subClassOf wikidata:Q39201 .

wikidata:Q1441305 rdfs:label "clinical sign"^^xsd:string ;
    rdfs:comment "objective indication of a medical fact or characteristic of a disease, injury, or abnormal physiological state that may be detected during the physical examination of a patient"^^xsd:string ;
    rdfs:subClassOf wikidata:Q7189713 .

wikidata:Q146 rdfs:label "house cat"^^xsd:string ;
    rdfs:comment "domesticated feline"^^xsd:string ;
    rdfs:subClassOf wikidata:Q39201 .

wikidata:Q14637321 rdfs:label "fictional spacecraft"^^xsd:string ;
    rdfs:comment "spacecraft in fictional stories"^^xsd:string ;
    rdfs:subClassOf wikidata:Q18670171,
        wikidata:Q20871196 .

wikidata:Q14659 rdfs:label "coat of arms"^^xsd:string ;
    rdfs:comment "unique heraldic design on a shield or escutcheon"^^xsd:string ;
    rdfs:subClassOf wikidata:Q17335294,
        wikidata:Q80071 .

wikidata:Q1466064 rdfs:label "processor"^^xsd:string ;
    rdfs:comment "class of electronic units for electronic data processings"^^xsd:string ;
    rdfs:subClassOf wikidata:Q241317 .

wikidata:Q15141321 rdfs:label "train service"^^xsd:string ;
    rdfs:comment "passenger or good transport by a specific train following a specific route at regular times"^^xsd:string ;
    rdfs:subClassOf wikidata:Q1067164 .

wikidata:Q1517820 rdfs:label "lineage"^^xsd:string ;
    rdfs:comment "line of ancestors and descendants of a person"^^xsd:string ;
    rdfs:subClassOf wikidata:Q1313923 .

wikidata:Q1522115 rdfs:label "energy source"^^xsd:string ;
    rdfs:comment "physical or chemical phenomenon from which one can extract energy"^^xsd:string ;
    rdfs:subClassOf wikidata:Q31464082 .

wikidata:Q15229207 rdfs:label "sports award"^^xsd:string ;
    rdfs:comment "object (cup, medal...) awarded to a sports winner"^^xsd:string .

wikidata:Q15238535 rdfs:label "fictional government"^^xsd:string ;
    rdfs:comment "fictional entity"^^xsd:string ;
    rdfs:subClassOf wikidata:Q14623646 .

wikidata:Q154954 rdfs:label "natural person"^^xsd:string ;
    rdfs:comment "real human being as opposed to a non-human legal person"^^xsd:string ;
    rdfs:subClassOf wikidata:Q3778211 .

wikidata:Q1569167 rdfs:label "video game character"^^xsd:string ;
    rdfs:comment "character found in computer and video game"^^xsd:string ;
    rdfs:subClassOf wikidata:Q95074 .

wikidata:Q15707532 rdfs:label "fictional competition"^^xsd:string ;
    rdfs:comment "competition which only exists in a fictional universe"^^xsd:string ;
    rdfs:subClassOf wikidata:Q14136353 .

wikidata:Q15707583 rdfs:label "fictional taxon"^^xsd:string ;
    rdfs:comment "group of one or more fictional organism(s), which a (fictional) taxonomist adjudges to be a unit"^^xsd:string ;
    rdfs:subClassOf wikidata:Q15831596 .

wikidata:Q15709879 rdfs:label "artwork series"^^xsd:string ;
    rdfs:comment "thematic group of an artist's works"^^xsd:string ;
    rdfs:subClassOf wikidata:Q18593264,
        wikidata:Q7725310 .

wikidata:Q15711870 rdfs:label "animated character"^^xsd:string ;
    rdfs:comment "fictional character who appears in animated films, television, and other animated works"^^xsd:string ;
    rdfs:subClassOf wikidata:Q95074 .

wikidata:Q15720793 rdfs:label "fictional building"^^xsd:string ;
    rdfs:comment "building which only exists in fiction"^^xsd:string ;
    rdfs:subClassOf wikidata:Q63959448 .

wikidata:Q15720870 rdfs:label "fictional weapon"^^xsd:string ;
    rdfs:comment "weapon which only exists in fiction"^^xsd:string ;
    rdfs:subClassOf wikidata:Q15706911 .

wikidata:Q15773347 rdfs:label "film character"^^xsd:string ;
    rdfs:comment "fictional character appearing in a film"^^xsd:string ;
    rdfs:subClassOf wikidata:Q95074 .

wikidata:Q15938550 rdfs:label "electronic publication"^^xsd:string ;
    rdfs:comment "product distribution method"^^xsd:string ;
    rdfs:subClassOf wikidata:Q732577,
        wikidata:Q81941037 .

wikidata:Q16017119 rdfs:label "collective pseudonym"^^xsd:string ;
    rdfs:comment "pseudonym that is used by multiple persons"^^xsd:string ;
    rdfs:subClassOf wikidata:Q16334295,
        wikidata:Q61002 .

wikidata:Q1616075 rdfs:label "television station"^^xsd:string ;
    rdfs:comment "organization that transmits content on television"^^xsd:string ;
    rdfs:subClassOf wikidata:Q15265344 .

wikidata:Q161837 rdfs:label "public service"^^xsd:string ;
    rdfs:comment "Economic service provided by a government to people living within its jurisdiction"^^xsd:string ;
    rdfs:subClassOf wikidata:Q7406919 .

wikidata:Q1631107 rdfs:label "bibliography"^^xsd:string ;
    rdfs:comment "list of books or documents relevant to a particular subject or author"^^xsd:string .

wikidata:Q1642895 rdfs:label "lineage"^^xsd:string ;
    rdfs:comment "kinship"^^xsd:string ;
    rdfs:subClassOf wikidata:Q1313923,
        wikidata:Q16334298,
        wikidata:Q43229 .

wikidata:Q1664720 rdfs:label "institute"^^xsd:string ;
    rdfs:comment "organisational body created for a certain purpose"^^xsd:string ;
    rdfs:subClassOf wikidata:Q178706 .

wikidata:Q16858238 rdfs:label "train category"^^xsd:string ;
    rdfs:comment "group of train services sharing the same characteristics (such as service pattern, speed, fare, etc.); used in some jurisdictions"^^xsd:string .

wikidata:Q168658 rdfs:label "doll"^^xsd:string ;
    rdfs:comment "model of a character or a human beings, often used as a toy for children or an artistic hobby for adults"^^xsd:string .

wikidata:Q169930 rdfs:label "extended play"^^xsd:string ;
    rdfs:comment "musical recording that contains more tracks than a single but is usually unqualified as an album or LP"^^xsd:string ;
    rdfs:subClassOf wikidata:Q2031291,
        wikidata:Q22811462 .

wikidata:Q1714118 rdfs:label "online publication"^^xsd:string ;
    rdfs:comment "work manifested in Internet"^^xsd:string ;
    rdfs:subClassOf wikidata:Q15938550,
        wikidata:Q17537576 .

wikidata:Q1729207 rdfs:label "Christian ministry"^^xsd:string ;
    rdfs:comment "activity carried out by Christians to express or spread their faith"^^xsd:string ;
    rdfs:subClassOf wikidata:Q1914636,
        wikidata:Q43229 .

wikidata:Q17339814 rdfs:label "group or class of chemical substances"^^xsd:string ;
    rdfs:comment "set of chemical substances that share a common characteristic"^^xsd:string ;
    rdfs:subClassOf wikidata:Q98119401 .

wikidata:Q1744559 rdfs:label "classification in sports"^^xsd:string ;
    rdfs:comment "classification of age groups, sexes and levels within sports"^^xsd:string .

wikidata:Q17451 rdfs:label "typeface"^^xsd:string ;
    rdfs:comment "set of characters that share common design features"^^xsd:string ;
    rdfs:subClassOf wikidata:Q15621286,
        wikidata:Q18593264 .

wikidata:Q17776219 rdfs:label "lyrical text translated using paraphrasing"^^xsd:string ;
    rdfs:comment "free translation, rendering, of a lyrical text"^^xsd:string .

wikidata:Q178561 rdfs:label "battle"^^xsd:string ;
    rdfs:comment "part of a war which is well defined in duration, area and force commitment"^^xsd:string ;
    rdfs:subClassOf wikidata:Q645883,
        wikidata:Q650711 .

wikidata:Q178648 rdfs:label "peripheral"^^xsd:string ;
    rdfs:comment "hardware device which attaches to a computer and which provided input, output, storage or communication facilities"^^xsd:string ;
    rdfs:subClassOf wikidata:Q2858615 .

wikidata:Q1792644 rdfs:label "art style"^^xsd:string ;
    rdfs:comment "visual appearance of a creative work, shared with other works of the same movement or school"^^xsd:string ;
    rdfs:subClassOf wikidata:Q1292119,
        wikidata:Q1792379 .

wikidata:Q1812889 rdfs:label "legislative session"^^xsd:string ;
    rdfs:comment "period in which a legislature is convened; subdivision of a legislative term"^^xsd:string ;
    rdfs:subClassOf wikidata:Q1656682 .

wikidata:Q181348 rdfs:label "viaduct"^^xsd:string ;
    rdfs:comment "type of bridge crossing a valley or a gorge"^^xsd:string ;
    rdfs:subClassOf wikidata:Q12280 .

wikidata:Q18325841 rdfs:label "public transport network"^^xsd:string ;
    rdfs:comment "network for public transport"^^xsd:string ;
    rdfs:subClassOf wikidata:Q924286 .

wikidata:Q183366 rdfs:label "territory"^^xsd:string ;
    rdfs:comment "area of land under the jurisdiction"^^xsd:string ;
    rdfs:subClassOf wikidata:Q1496967 .

wikidata:Q18602566 rdfs:label "book format"^^xsd:string ;
    rdfs:comment "the form a book is produced into"^^xsd:string .

wikidata:Q18616576 rdfs:label "Wikidata property"^^xsd:string ;
    rdfs:comment "part of statements according to the Wikidata data model"^^xsd:string .

wikidata:Q18670171 rdfs:label "fictional vessel"^^xsd:string ;
    rdfs:comment "vessel which only exists in fiction"^^xsd:string ;
    rdfs:subClassOf wikidata:Q20871196 .

wikidata:Q187588 rdfs:label "social class"^^xsd:string ;
    rdfs:comment "hierarchical social stratification"^^xsd:string ;
    rdfs:subClassOf wikidata:Q874405 .

wikidata:Q188860 rdfs:label "software library"^^xsd:string ;
    rdfs:comment "collection of non-volatile resources used by computer programs, often to develop software; software component that can be reused by other software for a specific purpose"^^xsd:string .

wikidata:Q1955280 rdfs:label "music competition"^^xsd:string ;
    rdfs:comment "contest that rewards the best musical performer"^^xsd:string ;
    rdfs:subClassOf wikidata:Q23807345 .

wikidata:Q19571328 rdfs:label "electoral result"^^xsd:string ;
    rdfs:comment ""^^xsd:string .

wikidata:Q1979154 rdfs:label "model"^^xsd:string ;
    rdfs:comment "simplified representation of an entity"^^xsd:string .

wikidata:Q19958368 rdfs:label "culture of an area"^^xsd:string ;
    rdfs:comment "distinct human activities and values that take place in, or originate from, a geographic location"^^xsd:string ;
    rdfs:subClassOf wikidata:Q11042,
        wikidata:Q74817647 .

wikidata:Q202444 rdfs:label "given name"^^xsd:string ;
    rdfs:comment "name typically used to differentiate people from the same family, clan, or other social group who have a common last name"^^xsd:string .

wikidata:Q20655472 rdfs:label "editorial collection"^^xsd:string ;
    rdfs:comment "collection of written works, publications"^^xsd:string ;
    rdfs:subClassOf wikidata:Q2668072,
        wikidata:Q277759,
        wikidata:Q732577 .

wikidata:Q20671381 rdfs:label "album series"^^xsd:string ;
    rdfs:comment "series of recorded music released in album format"^^xsd:string ;
    rdfs:subClassOf wikidata:Q7725310 .

wikidata:Q2072238 rdfs:label "archdiocese"^^xsd:string ;
    rdfs:comment "district or see under the supervision of a bishop, with more significance than a diocese"^^xsd:string ;
    rdfs:subClassOf wikidata:Q665487 .

wikidata:Q20826013 rdfs:label "software version"^^xsd:string ;
    rdfs:comment "defined and identifiable development stage of a software product"^^xsd:string ;
    rdfs:subClassOf wikidata:Q3331189 .

wikidata:Q20970434 rdfs:label "width to height ratio"^^xsd:string ;
    rdfs:comment "arithmetic relationship between the width and height of a geometric figure"^^xsd:string .

wikidata:Q21004260 rdfs:label "inquiry"^^xsd:string ;
    rdfs:comment "process that has the aim of augmenting knowledge, resolving doubt, or solving a problem"^^xsd:string .

wikidata:Q21029893 rdfs:label "religious object"^^xsd:string ;
    rdfs:comment "object used in a religion"^^xsd:string ;
    rdfs:subClassOf wikidata:Q8205328 .

wikidata:Q211503 rdfs:label "clan"^^xsd:string ;
    rdfs:comment "group of people united by actual or perceived kinship and descent"^^xsd:string ;
    rdfs:subClassOf wikidata:Q133311,
        wikidata:Q8436 .

wikidata:Q212971 rdfs:label "Request for Comments"^^xsd:string ;
    rdfs:comment "publication of the development and standards for the Internet"^^xsd:string ;
    rdfs:subClassOf wikidata:Q317623,
        wikidata:Q49848 .

wikidata:Q214995 rdfs:label "telephone number"^^xsd:string ;
    rdfs:comment "unique sequence of digits assigned to a telephone subscription"^^xsd:string ;
    rdfs:subClassOf wikidata:Q853614 .

wikidata:Q220397 rdfs:label "saros cycle"^^xsd:string ;
    rdfs:comment "period of 223 synodic months that can be used to predict eclipses of the Sun and Moon"^^xsd:string ;
    rdfs:subClassOf wikidata:Q20937557 .

wikidata:Q220659 rdfs:label "archaeological artifact"^^xsd:string ;
    rdfs:comment "something made by humans and of archaeological interest"^^xsd:string .

wikidata:Q223393 rdfs:label "literary genre"^^xsd:string ;
    rdfs:comment "category of literary composition"^^xsd:string ;
    rdfs:subClassOf wikidata:Q483394 .

wikidata:Q22667 rdfs:label "railway"^^xsd:string ;
    rdfs:comment "interconnected network of infrastructure and vehicles used for train rail transport"^^xsd:string .

wikidata:Q2312410 rdfs:label "sports discipline"^^xsd:string ;
    rdfs:comment "subtype of a sport, an event within a sport"^^xsd:string ;
    rdfs:subClassOf wikidata:Q31629 .

wikidata:Q23729754 rdfs:label "scientific name, published under a Code of nomenclature"^^xsd:string ;
    rdfs:comment "name formally established according to the requirements of a Code of nomenclature"^^xsd:string .

wikidata:Q24334299 rdfs:label "mythical animal"^^xsd:string ;
    rdfs:comment "class of creature in mythology"^^xsd:string ;
    rdfs:subClassOf wikidata:Q2239243 .

wikidata:Q24336466 rdfs:label "mythical event"^^xsd:string ;
    rdfs:comment "fictional episode in a body of myth"^^xsd:string ;
    rdfs:subClassOf wikidata:Q14136353,
        wikidata:Q24334685 .

wikidata:Q24634210 rdfs:label "podcast"^^xsd:string ;
    rdfs:comment "kind of broadcasting program"^^xsd:string ;
    rdfs:subClassOf wikidata:Q1002697,
        wikidata:Q11578774,
        wikidata:Q2431196,
        wikidata:Q7725310 .

wikidata:Q2485448 rdfs:label "sports governing body"^^xsd:string ;
    rdfs:comment "sports organization that has a regulatory or sanctioning function"^^xsd:string .

wikidata:Q2515887 rdfs:label "pattern of behaviour"^^xsd:string ;
    rdfs:comment "type of animal behavior, humans included"^^xsd:string .

wikidata:Q2516436 rdfs:label "traffic system"^^xsd:string ;
    rdfs:comment "System"^^xsd:string ;
    rdfs:subClassOf wikidata:Q43229,
        wikidata:Q58778 .

wikidata:Q25295 rdfs:label "language family"^^xsd:string ;
    rdfs:comment "group of languages related through descent from a common ancestor"^^xsd:string ;
    rdfs:subClassOf wikidata:Q17376908 .

wikidata:Q2531956 rdfs:label "ethnic group"^^xsd:string ;
    rdfs:comment "ethnic group, minority within a state, especially a single ethnic group within a polyethnic state"^^xsd:string ;
    rdfs:subClassOf wikidata:Q874405 .

wikidata:Q25379 rdfs:label "play"^^xsd:string ;
    rdfs:comment "dramatic work"^^xsd:string .

wikidata:Q25416091 rdfs:label "substance"^^xsd:string ;
    rdfs:comment "any composed matter whose origin is either biological, chemical, or mineral"^^xsd:string .

wikidata:Q25653 rdfs:label "ferry ship"^^xsd:string ;
    rdfs:comment "type of ship travelling over short to medium distances between two places transporting people, cars or trains and acting like a replacement for a bridge"^^xsd:string ;
    rdfs:subClassOf wikidata:Q11446 .

wikidata:Q2571972 rdfs:label "decree"^^xsd:string ;
    rdfs:comment "rule of law usually issued by a head of state"^^xsd:string ;
    rdfs:subClassOf wikidata:Q1151067,
        wikidata:Q694045,
        wikidata:Q820655 .

wikidata:Q2593744 rdfs:label "fictional creature"^^xsd:string ;
    rdfs:comment "organism not more specified in a work of fiction"^^xsd:string ;
    rdfs:subClassOf wikidata:Q95074 .

wikidata:Q26085352 rdfs:label "file format family"^^xsd:string ;
    rdfs:comment "family of related or similar file formats"^^xsd:string .

wikidata:Q2628882 rdfs:label "legal status"^^xsd:string ;
    rdfs:comment "status in law"^^xsd:string ;
    rdfs:subClassOf wikidata:Q214339 .

wikidata:Q264965 rdfs:label "subculture"^^xsd:string ;
    rdfs:comment "group of people within a culture that differentiates themselves from the larger culture to which they belong"^^xsd:string ;
    rdfs:subClassOf wikidata:Q11042,
        wikidata:Q19958368,
        wikidata:Q874405 .

wikidata:Q2675537 rdfs:label "music teacher"^^xsd:string ;
    rdfs:comment "person who teaches music"^^xsd:string .

wikidata:Q2678338 rdfs:label "railway network"^^xsd:string ;
    rdfs:comment "set of multiple railway lines with a common trait"^^xsd:string ;
    rdfs:subClassOf wikidata:Q121359,
        wikidata:Q618123,
        wikidata:Q924286 .

wikidata:Q26843 rdfs:label "orca"^^xsd:string ;
    rdfs:comment "species in the oceanic dolphin family"^^xsd:string .

wikidata:Q26884850 rdfs:label "smart speaker"^^xsd:string ;
    rdfs:comment "Speaker with features or services that go beyond audio playback"^^xsd:string ;
    rdfs:subClassOf wikidata:Q11253473 .

wikidata:Q27043950 rdfs:label "anatomical entity"^^xsd:string ;
    rdfs:comment "biological entity that's either member of a species or a unit of its structural organization"^^xsd:string .

wikidata:Q2738074 rdfs:label "political movement"^^xsd:string ;
    rdfs:comment "movement to obtain a political goal"^^xsd:string ;
    rdfs:subClassOf wikidata:Q49773,
        wikidata:Q7210356 .

wikidata:Q2775969 rdfs:label "fictional planet"^^xsd:string ;
    rdfs:comment "planet that only appears in works of fiction"^^xsd:string ;
    rdfs:subClassOf wikidata:Q15831598 .

wikidata:Q277759 rdfs:label "book series"^^xsd:string ;
    rdfs:comment "sequence of books having certain characteristics in common that are formally identified together as a group"^^xsd:string ;
    rdfs:subClassOf wikidata:Q2217301,
        wikidata:Q47461344,
        wikidata:Q7725310 .

wikidata:Q28114058 rdfs:label "game franchise"^^xsd:string ;
    rdfs:comment "any type of game under a common theme or story"^^xsd:string ;
    rdfs:subClassOf wikidata:Q17537576 .

wikidata:Q284851 rdfs:label "archaic human"^^xsd:string ;
    rdfs:comment "extinct relative of modern humans (Homo) from the past half million years (such as Neanderthals)"^^xsd:string ;
    rdfs:subClassOf wikidata:Q40614 .

wikidata:Q285181 rdfs:label "eparchy"^^xsd:string ;
    rdfs:comment "administrative territorial entity of Greek-Catholic, Orthodox and Eastern Churches"^^xsd:string ;
    rdfs:subClassOf wikidata:Q1492823,
        wikidata:Q20926517,
        wikidata:Q51041800 .

wikidata:Q28732711 rdfs:label "physical substance"^^xsd:string ;
    rdfs:comment "substance composed of quantum particle(s)/field(s), such as matter and/or radiation; that of which objects/systems are composed; physical stuff that can be considered concrete (not strictly abstract)"^^xsd:string ;
    rdfs:subClassOf wikidata:Q4406616 .

wikidata:Q2915955 rdfs:label "philosophical movement"^^xsd:string ;
    rdfs:comment "appearance or increased popularity of a specific school of philosophy"^^xsd:string ;
    rdfs:subClassOf wikidata:Q49773 .

wikidata:Q301676 rdfs:label "crab-eating macaque"^^xsd:string ;
    rdfs:comment "species of mammal"^^xsd:string .

wikidata:Q3026787 rdfs:label "saying"^^xsd:string ;
    rdfs:comment "short, usually meaningful phrase, such as a maxim, proverb, motto, or adage"^^xsd:string ;
    rdfs:subClassOf wikidata:Q386724 .

wikidata:Q3052382 rdfs:label "fonds"^^xsd:string ;
    rdfs:comment "aggregation of works that originate from the same source"^^xsd:string ;
    rdfs:subClassOf wikidata:Q17489659,
        wikidata:Q2668072 .

wikidata:Q30612 rdfs:label "clinical trial"^^xsd:string ;
    rdfs:comment "phase of clinical research in medicine"^^xsd:string ;
    rdfs:subClassOf wikidata:Q101965,
        wikidata:Q1298668 .

wikidata:Q3099911 rdfs:label "scientific instrument"^^xsd:string ;
    rdfs:comment "equipment specifically designed to facilitate the acquisition of scientific data"^^xsd:string .

wikidata:Q3132741 rdfs:label "substellar object"^^xsd:string ;
    rdfs:comment "astronomical object whose mass is smaller than the smallest mass at which a star can sustain hydrogen fusion"^^xsd:string ;
    rdfs:subClassOf wikidata:Q6999 .

wikidata:Q317557 rdfs:label "parish church"^^xsd:string ;
    rdfs:comment "church which acts as the religious centre of a parish"^^xsd:string ;
    rdfs:subClassOf wikidata:Q16970 .

wikidata:Q3199915 rdfs:label "massacre"^^xsd:string ;
    rdfs:comment "incident where some group is killed by another"^^xsd:string ;
    rdfs:subClassOf wikidata:Q1190554 .

wikidata:Q3241753 rdfs:label "road number"^^xsd:string ;
    rdfs:comment "number or alphanumeric characters assigned to a stretch of public roadway often dependent on the type of road"^^xsd:string .

wikidata:Q33384 rdfs:label "dialect"^^xsd:string ;
    rdfs:comment "geographically- or socially-determined language variety"^^xsd:string .

wikidata:Q336 rdfs:label "science"^^xsd:string ;
    rdfs:comment "systematic enterprise that builds and organizes knowledge"^^xsd:string .

wikidata:Q337567 rdfs:label "still waters"^^xsd:string ;
    rdfs:comment "body of water without noticeable current"^^xsd:string .

wikidata:Q34627 rdfs:label "synagogue"^^xsd:string ;
    rdfs:comment "Jewish (or rarely Samaritan) house of prayer"^^xsd:string ;
    rdfs:subClassOf wikidata:Q1530022,
        wikidata:Q44539 .

wikidata:Q35140 rdfs:label "performance"^^xsd:string ;
    rdfs:comment "public presentation of a performance work, a play, concert, or other form of entertainment"^^xsd:string ;
    rdfs:subClassOf wikidata:Q1656682,
        wikidata:Q16686448,
        wikidata:Q1914636 .

wikidata:Q352858 rdfs:label "addendum"^^xsd:string ;
    rdfs:comment "addition made to a document following its publication"^^xsd:string ;
    rdfs:subClassOf wikidata:Q49848 .

wikidata:Q355567 rdfs:label "noble title"^^xsd:string ;
    rdfs:comment "legal privilege given to some members in monarchial and princely societies"^^xsd:string ;
    rdfs:subClassOf wikidata:Q187588,
        wikidata:Q216353,
        wikidata:Q4120621 .

wikidata:Q3565868 rdfs:label "rail transport"^^xsd:string ;
    rdfs:comment "conveyance of passengers and goods by way of wheeled vehicles running on rail tracks"^^xsd:string .

wikidata:Q36524 rdfs:label "authority control"^^xsd:string ;
    rdfs:comment "unique headings used for bibliographic information"^^xsd:string .

wikidata:Q3707858 rdfs:label "type"^^xsd:string ;
    rdfs:comment "anchoring point (of a name) in taxonomy"^^xsd:string .

wikidata:Q37260 rdfs:label "writing"^^xsd:string ;
    rdfs:comment "representation of language in a textual medium; tool developed by human society"^^xsd:string .

wikidata:Q373899 rdfs:label "record chart"^^xsd:string ;
    rdfs:comment "ranking of recorded music during a particular time period"^^xsd:string ;
    rdfs:subClassOf wikidata:Q80793969 .

wikidata:Q374814 rdfs:label "certification"^^xsd:string ;
    rdfs:comment "formal attestation of certain characteristics of an object, person, or organization"^^xsd:string .

wikidata:Q375011 rdfs:label "religious festival"^^xsd:string ;
    rdfs:comment "time of special importance marked by adherents to that religion"^^xsd:string ;
    rdfs:subClassOf wikidata:Q132241,
        wikidata:Q1445650 .

wikidata:Q3769299 rdfs:label "human behaviour"^^xsd:string ;
    rdfs:comment "array of every physical action and observable emotion associated with humans"^^xsd:string .

wikidata:Q37930 rdfs:label "postage stamp"^^xsd:string ;
    rdfs:comment "small piece of paper that is purchased and displayed on an item of mail as evidence of payment of postage"^^xsd:string ;
    rdfs:subClassOf wikidata:Q386724 .

wikidata:Q38033430 rdfs:label "class of award"^^xsd:string ;
    rdfs:comment "class of award (order, medal etc.)"^^xsd:string ;
    rdfs:subClassOf wikidata:Q618779 .

wikidata:Q386426 rdfs:label "natural heritage"^^xsd:string ;
    rdfs:comment "elements of biodiversity, including flora and fauna, ecosystems, fossils and geological structures"^^xsd:string .

wikidata:Q38723 rdfs:label "higher education institution"^^xsd:string ;
    rdfs:comment "institution that provides higher education (e.g., universities, vocational universities, community colleges, liberal arts colleges, institutes of technology, and others)"^^xsd:string ;
    rdfs:subClassOf wikidata:Q2385804 .

wikidata:Q3918 rdfs:label "university"^^xsd:string ;
    rdfs:comment "academic institution for further education"^^xsd:string ;
    rdfs:subClassOf wikidata:Q38723,
        wikidata:Q4671277 .

wikidata:Q3947 rdfs:label "house"^^xsd:string ;
    rdfs:comment "building usually intended for living in"^^xsd:string ;
    rdfs:subClassOf wikidata:Q386724 .

wikidata:Q39816 rdfs:label "valley"^^xsd:string ;
    rdfs:comment "low area between hills, often with a river running through it"^^xsd:string ;
    rdfs:subClassOf wikidata:Q271669,
        wikidata:Q82794 .

wikidata:Q40357 rdfs:label "prison"^^xsd:string ;
    rdfs:comment "place in which people legally are physically confined and usually deprived of a range of personal freedoms"^^xsd:string ;
    rdfs:subClassOf wikidata:Q13226383,
        wikidata:Q178706 .

wikidata:Q4042967 rdfs:label "sexuality"^^xsd:string ;
    rdfs:comment "anything that is characterized or distinguished by sex"^^xsd:string .

wikidata:Q40614 rdfs:label "fossil"^^xsd:string ;
    rdfs:comment "preserved remains or traces of organisms from a past geological age"^^xsd:string ;
    rdfs:subClassOf wikidata:Q223557 .

wikidata:Q420927 rdfs:label "protein complex"^^xsd:string ;
    rdfs:comment "stable macromolecular complex"^^xsd:string ;
    rdfs:subClassOf wikidata:Q22325163,
        wikidata:Q8054 .

wikidata:Q42470 rdfs:label "motto"^^xsd:string ;
    rdfs:comment "short sentence expressing a motivation"^^xsd:string ;
    rdfs:subClassOf wikidata:Q3026787,
        wikidata:Q386724 .

wikidata:Q427961 rdfs:label "metropolis"^^xsd:string ;
    rdfs:comment "diocese headed by an archbishop and having suffragan dioceses under its jurisdiction"^^xsd:string ;
    rdfs:subClassOf wikidata:Q2072238,
        wikidata:Q665487 .

wikidata:Q429785 rdfs:label "poster"^^xsd:string ;
    rdfs:comment "type of graphic advertisement"^^xsd:string ;
    rdfs:subClassOf wikidata:Q1261026 .

wikidata:Q4327689 rdfs:label "sheet music"^^xsd:string ;
    rdfs:comment "notated music printed on unbound sheets of paper; printed representation of a musical work"^^xsd:string ;
    rdfs:subClassOf wikidata:Q1261026,
        wikidata:Q2188189 .

wikidata:Q43501 rdfs:label "zoo"^^xsd:string ;
    rdfs:comment "collection of assorted wild animal species kept for purposes like: study, conservation and, or, commercial exhibition"^^xsd:string ;
    rdfs:subClassOf wikidata:Q178706,
        wikidata:Q22698,
        wikidata:Q570116 .

wikidata:Q4392985 rdfs:label "religious identity"^^xsd:string ;
    rdfs:comment "type of identity create by a type of religious belief"^^xsd:string ;
    rdfs:subClassOf wikidata:Q844569 .

wikidata:Q44539 rdfs:label "temple"^^xsd:string ;
    rdfs:comment "structure reserved for religious or spiritual activities"^^xsd:string ;
    rdfs:subClassOf wikidata:Q1370598 .

wikidata:Q4485156 rdfs:label "software feature"^^xsd:string ;
    rdfs:comment "distinguishing characteristic or capability of software"^^xsd:string ;
    rdfs:subClassOf wikidata:Q1207505,
        wikidata:Q1347367 .

wikidata:Q4588528 rdfs:label "holy place"^^xsd:string ;
    rdfs:comment "sites that a religion considers to be of special religious significance"^^xsd:string .

wikidata:Q465909 rdfs:label "airline alliance"^^xsd:string ;
    rdfs:comment "cooperation agreement between two or more airlines"^^xsd:string .

wikidata:Q4663903 rdfs:label "Wikimedia portal"^^xsd:string ;
    rdfs:comment "pages on a Wikimedia wiki intended to serve as \"Main Pages\" for specific areas of knowledge or information, or for specific audiences and activities. Use with P31 'instance of' for them"^^xsd:string .

wikidata:Q4671277 rdfs:label "academic institution"^^xsd:string ;
    rdfs:comment "educational institution dedicated to education and research"^^xsd:string ;
    rdfs:subClassOf wikidata:Q2385804,
        wikidata:Q31855 .

wikidata:Q46970 rdfs:label "airline"^^xsd:string ;
    rdfs:comment "company that provides air transport services for traveling passengers and freight"^^xsd:string .

wikidata:Q47433 rdfs:label "banknote"^^xsd:string ;
    rdfs:comment "form of physical currency made of paper (or less commonly, polymer)"^^xsd:string ;
    rdfs:subClassOf wikidata:Q8205328 .

wikidata:Q47495022 rdfs:label "shell of an astronomical object"^^xsd:string ;
    rdfs:comment "ߓߙߎߡߎ߲ ߡߍ߲ ߘߏ߲߬ߣߍ߲߬ ߦߋ߫ ߕߋ߬ߟߋ ߡߊ߬ ߡߐ߲ߕߐ߲߫߹"^^xsd:string .

wikidata:Q47574 rdfs:label "unit of measurement"^^xsd:string ;
    rdfs:comment "quantity, defined and adopted by convention"^^xsd:string .

wikidata:Q478798 rdfs:label "image"^^xsd:string ;
    rdfs:comment "artifact that depicts or records visual perception"^^xsd:string .

wikidata:Q47988 rdfs:label "identity document"^^xsd:string ;
    rdfs:comment "document which may be used to identify a person"^^xsd:string .

wikidata:Q48282 rdfs:label "student"^^xsd:string ;
    rdfs:comment "learner, or someone who attends an educational institution"^^xsd:string .

wikidata:Q48352 rdfs:label "head of state"^^xsd:string ;
    rdfs:comment "official who holds the highest-ranked executive position in a sovereign state"^^xsd:string .

wikidata:Q48900561 rdfs:label "fictional military facility"^^xsd:string ;
    rdfs:comment "military facility that only exits in works of fiction"^^xsd:string ;
    rdfs:subClassOf wikidata:Q3895768 .

wikidata:Q5051330 rdfs:label "catalogue of classical compositions"^^xsd:string ;
    rdfs:comment "index and classification of classical music compositions"^^xsd:string .

wikidata:Q506572 rdfs:label "submarine communications cable"^^xsd:string ;
    rdfs:comment "long range communications device placed underwater, often intercontinental"^^xsd:string .

wikidata:Q515 rdfs:label "city"^^xsd:string ;
    rdfs:comment "large permanent human settlement"^^xsd:string ;
    rdfs:subClassOf wikidata:Q177634,
        wikidata:Q486972,
        wikidata:Q7930989 .

wikidata:Q5151 rdfs:label "month"^^xsd:string ;
    rdfs:comment "irregular unit of time dividing a calendar year"^^xsd:string .

wikidata:Q52688389 rdfs:label "animal actor"^^xsd:string ;
    rdfs:comment "animal which has performed in film or television"^^xsd:string ;
    rdfs:subClassOf wikidata:Q26401003 .

wikidata:Q5398426 rdfs:label "television series"^^xsd:string ;
    rdfs:comment "connected set of television program episodes under the same title"^^xsd:string ;
    rdfs:subClassOf wikidata:Q15416,
        wikidata:Q7725310 .

wikidata:Q54050 rdfs:label "hill"^^xsd:string ;
    rdfs:comment "landform that extends above the surrounding terrain"^^xsd:string ;
    rdfs:subClassOf wikidata:Q2221906,
        wikidata:Q271669 .

wikidata:Q55006986 rdfs:label "transport facility"^^xsd:string ;
    rdfs:comment ""^^xsd:string ;
    rdfs:subClassOf wikidata:Q13226383,
        wikidata:Q376799 .

wikidata:Q55488 rdfs:label "railway station"^^xsd:string ;
    rdfs:comment "railway facility where trains regularly stop to load or unload passengers and/or freight"^^xsd:string ;
    rdfs:subClassOf wikidata:Q12819564,
        wikidata:Q1318558 .

wikidata:Q56561355 rdfs:label "fictional gang"^^xsd:string ;
    rdfs:comment "gang which only exists in a work of fiction"^^xsd:string ;
    rdfs:subClassOf wikidata:Q14514600 .

wikidata:Q58483088 rdfs:label "choreographic work"^^xsd:string ;
    rdfs:comment "work, like a ballet, having a story, plot or abstract idea devised or used for the purpose of interpretation by dancing and/or miming; see also \"dramatico-musical work\" (Q58483083)"^^xsd:string .

wikidata:Q5961257 rdfs:label "hypothetical astronomical object"^^xsd:string ;
    rdfs:comment "astronomical object assumed to exist, or earlier assumed to exist"^^xsd:string ;
    rdfs:subClassOf wikidata:Q6999 .

wikidata:Q5982983 rdfs:label "jurisdiction"^^xsd:string ;
    rdfs:comment "distinct area subject to a government and set of laws, such as a country or federated state"^^xsd:string ;
    rdfs:subClassOf wikidata:Q56061 .

wikidata:Q600659 rdfs:label "disk operating system"^^xsd:string ;
    rdfs:comment "type of operating system"^^xsd:string ;
    rdfs:subClassOf wikidata:Q9135 .

wikidata:Q60733114 rdfs:label "music tradition"^^xsd:string ;
    rdfs:comment "musical repertoire, techniques, and style of an area, people or social class that is passed down through subsequent generations"^^xsd:string .

wikidata:Q620615 rdfs:label "mobile app"^^xsd:string ;
    rdfs:comment "software application designed to run on mobile devices"^^xsd:string ;
    rdfs:subClassOf wikidata:Q166142,
        wikidata:Q340169 .

wikidata:Q623109 rdfs:label "sports league"^^xsd:string ;
    rdfs:comment "group of sports teams or individual athletes that compete against each other"^^xsd:string ;
    rdfs:subClassOf wikidata:Q18608583,
        wikidata:Q4438121 .

wikidata:Q6266 rdfs:label "nation"^^xsd:string ;
    rdfs:comment "community of people who share a common language, culture, ethnicity, descent, or history"^^xsd:string ;
    rdfs:subClassOf wikidata:Q16334295 .

wikidata:Q628179 rdfs:label "trail"^^xsd:string ;
    rdfs:comment "path with a rough beaten or dirt/stone surface used for travel"^^xsd:string .

wikidata:Q629206 rdfs:label "computer language"^^xsd:string ;
    rdfs:comment "language used to design, develop or make use of computer systems"^^xsd:string ;
    rdfs:subClassOf wikidata:Q15621286 .

wikidata:Q62934160 rdfs:label "military unit class"^^xsd:string ;
    rdfs:comment "classification of military organizations by specific features"^^xsd:string .

wikidata:Q63141557 rdfs:label "translated song"^^xsd:string ;
    rdfs:comment "song lyrics translated or adapted from an original song in another language"^^xsd:string ;
    rdfs:subClassOf wikidata:Q7366 .

wikidata:Q63188683 rdfs:label "Christian religious occupation"^^xsd:string ;
    rdfs:comment ""^^xsd:string ;
    rdfs:subClassOf wikidata:Q28640,
        wikidata:Q4164871,
        wikidata:Q63187345 .

wikidata:Q63367831 rdfs:label "optical disc packaging"^^xsd:string ;
    rdfs:comment "case or other packaging used to protect optical discs"^^xsd:string .

wikidata:Q634 rdfs:label "planet"^^xsd:string ;
    rdfs:comment "celestial body directly orbiting a star or stellar remnant"^^xsd:string .

wikidata:Q63437139 rdfs:label "software project"^^xsd:string ;
    rdfs:comment "project organized for the development of a specific software program"^^xsd:string ;
    rdfs:subClassOf wikidata:Q170584,
        wikidata:Q43229 .

wikidata:Q63959448 rdfs:label "fictional architectural structure"^^xsd:string ;
    rdfs:comment "architectural structure which only exists in a work of fiction"^^xsd:string ;
    rdfs:subClassOf wikidata:Q3895768 .

wikidata:Q639907 rdfs:label "medical finding"^^xsd:string ;
    rdfs:comment "collective physical and psychological occurrences of patients surveyed by a medical doctor"^^xsd:string .

wikidata:Q640506 rdfs:label "cabinet"^^xsd:string ;
    rdfs:comment "group of high ranking officials, usually representing the executive branch of government"^^xsd:string ;
    rdfs:subClassOf wikidata:Q35798 .

wikidata:Q641226 rdfs:label "arena"^^xsd:string ;
    rdfs:comment "enclosed area designed to host theater, musical performances and sporting events"^^xsd:string ;
    rdfs:subClassOf wikidata:Q18674739 .

wikidata:Q650711 rdfs:label "combat"^^xsd:string ;
    rdfs:comment "purposeful violent conflict, typically refers to armed conflict or melee"^^xsd:string ;
    rdfs:subClassOf wikidata:Q180684,
        wikidata:Q1931388 .

wikidata:Q65972034 rdfs:label "trailer"^^xsd:string ;
    rdfs:comment "advertisement for a video game"^^xsd:string .

wikidata:Q66661745 rdfs:label "group of artificial physical objects"^^xsd:string ;
    rdfs:comment "group of physical objects made or shaped by human hand"^^xsd:string .

wikidata:Q68773434 rdfs:label "center"^^xsd:string ;
    rdfs:comment "dedicated facility providing a place for a particular activity or service"^^xsd:string ;
    rdfs:subClassOf wikidata:Q13226383,
        wikidata:Q43229 .

wikidata:Q689044 rdfs:label "voucher"^^xsd:string ;
    rdfs:comment "receipt or bond with a certain value"^^xsd:string ;
    rdfs:subClassOf wikidata:Q4406616 .

wikidata:Q6958747 rdfs:label "work"^^xsd:string ;
    rdfs:comment "particular form of activity, sold by many people to sustain themselves"^^xsd:string ;
    rdfs:subClassOf wikidata:Q1914636 .

wikidata:Q699405 rdfs:label "residence"^^xsd:string ;
    rdfs:comment "self-contained unit of accommodation (house, apartment, mobile home, houseboat or other structure) used as a home"^^xsd:string ;
    rdfs:subClassOf wikidata:Q17334923,
        wikidata:Q811979 .

wikidata:Q7094076 rdfs:label "online database"^^xsd:string ;
    rdfs:comment "database accessible from a network, including from the Internet"^^xsd:string ;
    rdfs:subClassOf wikidata:Q1172284,
        wikidata:Q8513 .

wikidata:Q713200 rdfs:label "performing artist"^^xsd:string ;
    rdfs:comment "artist who participates in performing arts in front of an audience: actors, comedians, dancers, magicians, circus artists, musicians, singers"^^xsd:string .

wikidata:Q732717 rdfs:label "law enforcement agency"^^xsd:string ;
    rdfs:comment "government agency responsible for the enforcement of the laws"^^xsd:string ;
    rdfs:subClassOf wikidata:Q17149090,
        wikidata:Q327333 .

wikidata:Q751989 rdfs:label "astronomical phenomenon"^^xsd:string ;
    rdfs:comment "event involving astronomical objects"^^xsd:string ;
    rdfs:subClassOf wikidata:Q1322005 .

wikidata:Q756 rdfs:label "plant"^^xsd:string ;
    rdfs:comment "multicellular eukaryote of the kingdom Plantae"^^xsd:string ;
    rdfs:subClassOf wikidata:Q7239 .

wikidata:Q759853 rdfs:label "film format"^^xsd:string ;
    rdfs:comment "standardized set of characteristics for photographic film"^^xsd:string .

wikidata:Q7748 rdfs:label "law"^^xsd:string ;
    rdfs:comment "system of rules and guidelines, generally backed by governmental authority"^^xsd:string ;
    rdfs:subClassOf wikidata:Q1151067 .

wikidata:Q7843791 rdfs:label "consulate"^^xsd:string ;
    rdfs:comment "small official office of one country in another country"^^xsd:string ;
    rdfs:subClassOf wikidata:Q213283 .

wikidata:Q79007 rdfs:label "street"^^xsd:string ;
    rdfs:comment "public thoroughfare in a built environment"^^xsd:string ;
    rdfs:subClassOf wikidata:Q34442 .

wikidata:Q796194 rdfs:label "medical procedure"^^xsd:string ;
    rdfs:comment "process of medicine done to heal; course of action intended to achieve a result in the delivery of healthcare"^^xsd:string ;
    rdfs:subClassOf wikidata:Q3249551 .

wikidata:Q80793969 rdfs:label "ranked list"^^xsd:string ;
    rdfs:comment "type of list that is ranked by some criteria"^^xsd:string ;
    rdfs:subClassOf wikidata:Q12139612,
        wikidata:Q386724 .

wikidata:Q81752537 rdfs:label "professorship"^^xsd:string ;
    rdfs:comment "position held by a university professor"^^xsd:string ;
    rdfs:subClassOf wikidata:Q4164871 .

wikidata:Q8187769 rdfs:label "economic activity"^^xsd:string ;
    rdfs:comment "financial transactions of products, goods, or services"^^xsd:string ;
    rdfs:subClassOf wikidata:Q61788060 .

wikidata:Q8222382 rdfs:label "legal proceeding"^^xsd:string ;
    rdfs:comment "evaluation of evidence to make a decision"^^xsd:string ;
    rdfs:subClassOf wikidata:Q3249551 .

wikidata:Q8242 rdfs:label "literature"^^xsd:string ;
    rdfs:comment "written art form"^^xsd:string ;
    rdfs:subClassOf wikidata:Q17537576,
        wikidata:Q735 .

wikidata:Q834104 rdfs:label "heraldic attribute"^^xsd:string ;
    rdfs:comment "describing term used in heraldry"^^xsd:string .

wikidata:Q8366 rdfs:label "algorithm"^^xsd:string ;
    rdfs:comment "unambiguous specification of how to solve a class of problems"^^xsd:string ;
    rdfs:subClassOf wikidata:Q386724 .

wikidata:Q837718 rdfs:label "energy storage"^^xsd:string ;
    rdfs:comment "capture of energy produced at one time for use at a later time"^^xsd:string ;
    rdfs:subClassOf wikidata:Q28877 .

wikidata:Q839769 rdfs:label "Eurasian brown bear"^^xsd:string ;
    rdfs:comment "subspecies of brown bear"^^xsd:string .

wikidata:Q841645 rdfs:label "Internet television"^^xsd:string ;
    rdfs:comment "distribution of television content via the public Internet"^^xsd:string ;
    rdfs:subClassOf wikidata:Q2001305 .

wikidata:Q84467700 rdfs:label "group or class of proteins"^^xsd:string ;
    rdfs:comment "any class, set, or group of proteins; proteins need not be related"^^xsd:string ;
    rdfs:subClassOf wikidata:Q17339814 .

wikidata:Q847301 rdfs:label "political campaign"^^xsd:string ;
    rdfs:comment "attempt to influence the decision making process within a specific group"^^xsd:string ;
    rdfs:subClassOf wikidata:Q18812548,
        wikidata:Q1914636,
        wikidata:Q43229 .

wikidata:Q851990 rdfs:label "population group"^^xsd:string ;
    rdfs:comment "demographic classification of people"^^xsd:string ;
    rdfs:subClassOf wikidata:Q874405 .

wikidata:Q868557 rdfs:label "music festival"^^xsd:string ;
    rdfs:comment "festival oriented towards music"^^xsd:string ;
    rdfs:subClassOf wikidata:Q4801521 .

wikidata:Q8719053 rdfs:label "music venue"^^xsd:string ;
    rdfs:comment "any location used for a concert or musical performance"^^xsd:string ;
    rdfs:subClassOf wikidata:Q17350442 .

wikidata:Q876500 rdfs:label "Gorilla gorilla gorilla"^^xsd:string ;
    rdfs:comment "subspecies of ape"^^xsd:string ;
    rdfs:subClassOf wikidata:Q729 .

wikidata:Q878123 rdfs:label "racing"^^xsd:string ;
    rdfs:comment "competitive athletic discipline"^^xsd:string ;
    rdfs:subClassOf wikidata:Q13406554 .

wikidata:Q9081 rdfs:label "knowledge"^^xsd:string ;
    rdfs:comment "experience or education by perceiving, discovering, or learning; theoretical or practical understanding of a subject"^^xsd:string .

wikidata:Q9135 rdfs:label "operating system"^^xsd:string ;
    rdfs:comment "software that manages computer hardware resources"^^xsd:string ;
    rdfs:subClassOf wikidata:Q241317 .

wikidata:Q939616 rdfs:label "secret service"^^xsd:string ;
    rdfs:comment "government agency concerned with the gathering of intelligence data"^^xsd:string ;
    rdfs:subClassOf wikidata:Q327333 .

wikidata:Q986008 rdfs:label "payment system"^^xsd:string ;
    rdfs:comment "system used to transfer monetary value, including institutions, instruments, people, rules, procedures, standards, and technologies"^^xsd:string ;
    rdfs:subClassOf wikidata:Q58778 .

<http://www.semanticweb.org/ontologies/Wikidata#_:y1> owl:propertyChainAxiom wikidata:P485 .

<http://www.semanticweb.org/ontologies/Wikidata#_:y10> rdf:rest <http://www.semanticweb.org/ontologies/Wikidata#_:y9> .

<http://www.semanticweb.org/ontologies/Wikidata#_:y11> owl:propertyChainAxiom wikidata:P942 .

<http://www.semanticweb.org/ontologies/Wikidata#_:y12> rdf:rest <http://www.semanticweb.org/ontologies/Wikidata#_:y11> .

<http://www.semanticweb.org/ontologies/Wikidata#_:y13> owl:propertyChainAxiom wikidata:P942 .

<http://www.semanticweb.org/ontologies/Wikidata#_:y14> rdf:rest <http://www.semanticweb.org/ontologies/Wikidata#_:y13> .

<http://www.semanticweb.org/ontologies/Wikidata#_:y2> rdf:rest <http://www.semanticweb.org/ontologies/Wikidata#_:y1> .

<http://www.semanticweb.org/ontologies/Wikidata#_:y3> owl:propertyChainAxiom wikidata:P98 .

<http://www.semanticweb.org/ontologies/Wikidata#_:y4> rdf:rest <http://www.semanticweb.org/ontologies/Wikidata#_:y3> .

<http://www.semanticweb.org/ontologies/Wikidata#_:y5> owl:propertyChainAxiom wikidata:P1268 .

<http://www.semanticweb.org/ontologies/Wikidata#_:y6> rdf:rest <http://www.semanticweb.org/ontologies/Wikidata#_:y5> .

<http://www.semanticweb.org/ontologies/Wikidata#_:y7> owl:propertyChainAxiom wikidata:P831 .

<http://www.semanticweb.org/ontologies/Wikidata#_:y8> rdf:rest <http://www.semanticweb.org/ontologies/Wikidata#_:y7> .

<http://www.semanticweb.org/ontologies/Wikidata#_:y9> owl:propertyChainAxiom wikidata:P3931 .

wikidata:P101 rdfs:label "field of work"^^xsd:string ;
    rdfs:comment "specialization of a person or organization; see P106 for the occupation"^^xsd:string ;
    rdfs:domain wikidata:Q1002697,
        wikidata:Q1003030,
        wikidata:Q132241,
        wikidata:Q13473501,
        wikidata:Q14623646,
        wikidata:Q16334295,
        wikidata:Q170584,
        wikidata:Q20830276,
        wikidata:Q215627,
        wikidata:Q33506,
        wikidata:Q4164871,
        wikidata:Q43229,
        wikidata:Q5,
        wikidata:Q546113,
        wikidata:Q618779,
        wikidata:Q625994,
        wikidata:Q68773434,
        wikidata:Q729,
        wikidata:Q735,
        wikidata:Q7406919,
        wikidata:Q8148,
        wikidata:Q95074 .

wikidata:P1037 rdfs:label "director / manager"^^xsd:string ;
    rdfs:comment "person who manages any kind of group"^^xsd:string ;
    rdfs:domain wikidata:Q14623646,
        wikidata:Q43229,
        wikidata:Q89753576 ;
    rdfs:range wikidata:Q5,
        wikidata:Q95074 .

wikidata:P121 rdfs:label "item operated"^^xsd:string ;
    rdfs:comment "equipment, installation or service operated by the subject"^^xsd:string ;
    rdfs:domain wikidata:Q1067164,
        wikidata:Q1190554,
        wikidata:Q13226383,
        wikidata:Q14623646,
        wikidata:Q16334295,
        wikidata:Q43229,
        wikidata:Q5,
        wikidata:Q55006986,
        wikidata:Q62934160,
        wikidata:Q95074 ;
    rdfs:range wikidata:Q13226383,
        wikidata:Q2668072,
        wikidata:Q28877,
        wikidata:Q7406919,
        wikidata:Q8513 ;
    rdfs:subPropertyOf wikidata:P2283 .

wikidata:P2354 rdfs:label "has list"^^xsd:string ;
    rdfs:comment "Wikimedia list related to this subject"^^xsd:string ;
    rdfs:range wikidata:Q13406463 .

wikidata:P2670 rdfs:label "has parts of the class"^^xsd:string ;
    rdfs:comment "the subject instance has parts of the object class (the subject is usually not a class)"^^xsd:string .

wikidata:P463 rdfs:label "member of"^^xsd:string ;
    rdfs:comment "organization, club or musical group to which the subject belongs. Do not use for membership in ethnic or social groups, nor for holding a position such as a member of parliament (use P39 for that)."^^xsd:string ;
    rdfs:domain wikidata:Q1048835,
        wikidata:Q13002315,
        wikidata:Q14623646,
        wikidata:Q183366,
        wikidata:Q214339,
        wikidata:Q215627,
        wikidata:Q43229,
        wikidata:Q49848,
        wikidata:Q5,
        wikidata:Q63187345,
        wikidata:Q63188683,
        wikidata:Q63188808,
        wikidata:Q6857706,
        wikidata:Q95074 ;
    rdfs:range wikidata:Q14514600,
        wikidata:Q14623646,
        wikidata:Q16334295,
        wikidata:Q16887380,
        wikidata:Q1729207,
        wikidata:Q2638480,
        wikidata:Q34627,
        wikidata:Q43229,
        wikidata:Q48204,
        wikidata:Q49459835,
        wikidata:Q49773,
        wikidata:Q55657615 ;
    rdfs:subPropertyOf wikidata:P1416 .

wikidata:Q1075 rdfs:label "color"^^xsd:string ;
    rdfs:comment "visual perception of light wavelengths"^^xsd:string ;
    rdfs:subClassOf wikidata:Q1207505 .

wikidata:Q11012 rdfs:label "robot"^^xsd:string ;
    rdfs:comment "mechanical or virtual artificial agent carrying out physical activities, which can be guided by an external control device or the control may be embedded within"^^xsd:string ;
    rdfs:subClassOf wikidata:Q11019 .

wikidata:Q11639 rdfs:label "dance"^^xsd:string ;
    rdfs:comment "rhythmic movement of the body"^^xsd:string ;
    rdfs:subClassOf wikidata:Q17537576 .

wikidata:Q117850 rdfs:label "doctrine"^^xsd:string ;
    rdfs:comment "codification of beliefs"^^xsd:string .

wikidata:Q1183543 rdfs:label "device"^^xsd:string ;
    rdfs:comment "complex equipment, such as with a motor or powered by electricity or another source of energy that it converts"^^xsd:string ;
    rdfs:subClassOf wikidata:Q16686448,
        wikidata:Q16798631,
        wikidata:Q39546 .

wikidata:Q1185607 rdfs:label "scene"^^xsd:string ;
    rdfs:comment "each of the divisions of a theatrical, cinematographic or television work"^^xsd:string .

wikidata:Q12136 rdfs:label "disease"^^xsd:string ;
    rdfs:comment "abnormal condition negatively affecting organisms"^^xsd:string ;
    rdfs:subClassOf wikidata:Q2057971,
        wikidata:Q7189713 .

wikidata:Q12323 rdfs:label "dam"^^xsd:string ;
    rdfs:comment "barrier that impounds water or underground streams"^^xsd:string ;
    rdfs:subClassOf wikidata:Q121359 .

wikidata:Q12772819 rdfs:label "discovery"^^xsd:string ;
    rdfs:comment "act of detecting something new"^^xsd:string ;
    rdfs:subClassOf wikidata:Q1190554 .

wikidata:Q1292119 rdfs:label "style"^^xsd:string ;
    rdfs:comment "manner of expression particular to a specific period, group, or person"^^xsd:string ;
    rdfs:subClassOf wikidata:Q3533467 .

wikidata:Q1322323 rdfs:label "itinerary"^^xsd:string ;
    rdfs:comment "route of a journey"^^xsd:string ;
    rdfs:subClassOf wikidata:Q83620 .

wikidata:Q13414953 rdfs:label "religious denomination"^^xsd:string ;
    rdfs:comment "identifiable religious subgroup with a common structure and doctrine"^^xsd:string ;
    rdfs:subClassOf wikidata:Q1530022 .

wikidata:Q13417114 rdfs:label "noble family"^^xsd:string ;
    rdfs:comment "family part of the nobility of a region or country"^^xsd:string ;
    rdfs:subClassOf wikidata:Q1642895,
        wikidata:Q8436 .

wikidata:Q1347367 rdfs:label "capability"^^xsd:string ;
    rdfs:comment "ability to perform an action or fulfill a role"^^xsd:string ;
    rdfs:subClassOf wikidata:Q1207505 .

wikidata:Q1406161 rdfs:label "artistic theme"^^xsd:string ;
    rdfs:comment "theme or subject in a work of art"^^xsd:string ;
    rdfs:subClassOf wikidata:Q11028 .

wikidata:Q1456832 rdfs:label "offense"^^xsd:string ;
    rdfs:comment "action against the law, subject to punishment"^^xsd:string .

wikidata:Q15238777 rdfs:label "legislative term"^^xsd:string ;
    rdfs:comment "period from one election of a legislature until the next"^^xsd:string ;
    rdfs:subClassOf wikidata:Q1656682 .

wikidata:Q15265344 rdfs:label "broadcaster"^^xsd:string ;
    rdfs:comment "organization responsible for production and transmission of radio and television programs"^^xsd:string ;
    rdfs:subClassOf wikidata:Q43229 .

wikidata:Q15304597 rdfs:label "sequence variant"^^xsd:string ;
    rdfs:comment "non-exact copy of a sequence feature or genome exhibiting one or more sequence alterations"^^xsd:string ;
    rdfs:subClassOf wikidata:Q7187 .

wikidata:Q155076 rdfs:label "juridical person"^^xsd:string ;
    rdfs:comment "legal entity which is different from a natural person"^^xsd:string ;
    rdfs:subClassOf wikidata:Q3778211,
        wikidata:Q43229 .

wikidata:Q1555508 rdfs:label "radio program"^^xsd:string ;
    rdfs:comment "sound segment of content intended for broadcast on radio"^^xsd:string ;
    rdfs:subClassOf wikidata:Q11578774,
        wikidata:Q2431196 .

wikidata:Q15617994 rdfs:label "designation for an administrative territorial entity"^^xsd:string ;
    rdfs:comment "type of administrative divisions, usually used in several countries"^^xsd:string ;
    rdfs:subClassOf wikidata:Q12047392 .

wikidata:Q15911314 rdfs:label "association"^^xsd:string ;
    rdfs:comment "group of individuals (natural persons) or entities (legal persons) of all kinds"^^xsd:string ;
    rdfs:subClassOf wikidata:Q16334295,
        wikidata:Q16887380,
        wikidata:Q24229398,
        wikidata:Q43229 .

wikidata:Q16510064 rdfs:label "sporting event"^^xsd:string ;
    rdfs:comment "single event at a sports festival"^^xsd:string ;
    rdfs:subClassOf wikidata:Q13406554,
        wikidata:Q841654 .

wikidata:Q165194 rdfs:label "application programming interface"^^xsd:string ;
    rdfs:comment "set of subroutine definitions, protocols, and tools for building software and applications"^^xsd:string ;
    rdfs:subClassOf wikidata:Q132364,
        wikidata:Q241317 .

wikidata:Q166620 rdfs:label "drainage basin"^^xsd:string ;
    rdfs:comment "area of land where precipitation collects and drains off into a common outlet, such as into a river, bay, or other body of water"^^xsd:string ;
    rdfs:subClassOf wikidata:Q82794 .

wikidata:Q167270 rdfs:label "trademark"^^xsd:string ;
    rdfs:comment "recognizable sign, design or expression which identifies products or services"^^xsd:string ;
    rdfs:subClassOf wikidata:Q3695082,
        wikidata:Q80071 .

wikidata:Q17143723 rdfs:label "catholic parish"^^xsd:string ;
    rdfs:comment "the lowest ecclesiastical subdivision in the Catholic episcopal polity, and the primary constituent unit of a diocese"^^xsd:string ;
    rdfs:subClassOf wikidata:Q102496,
        wikidata:Q51041800 .

wikidata:Q171558 rdfs:label "accident"^^xsd:string ;
    rdfs:comment "unforeseen and unplanned event or circumstance, often with a negative outcome"^^xsd:string .

wikidata:Q17305127 rdfs:label "fictional profession"^^xsd:string ;
    rdfs:comment "profession in fictional stories"^^xsd:string .

wikidata:Q17364638 rdfs:label "fictional religion"^^xsd:string ;
    rdfs:comment "religion which only exists in a work of fiction"^^xsd:string ;
    rdfs:subClassOf wikidata:Q14897293 .

wikidata:Q17444909 rdfs:label "astronomical object type"^^xsd:string ;
    rdfs:comment "each instance is a subclass in the hierarchy under <astronomical object>(Q6999); such a subclass's instances in turn are particular identified objects in Our Universe"^^xsd:string .

wikidata:Q17524420 rdfs:label "aspect of history"^^xsd:string ;
    rdfs:comment "topic viewed from a historical point of view"^^xsd:string ;
    rdfs:subClassOf wikidata:Q1047113 .

wikidata:Q17624054 rdfs:label "fictional deity"^^xsd:string ;
    rdfs:comment "deity that is only mentioned in fictional works and is not subject of an actual belief"^^xsd:string ;
    rdfs:subClassOf wikidata:Q95074 .

wikidata:Q1792379 rdfs:label "art genre"^^xsd:string ;
    rdfs:comment "form of art in terms of a medium (painted eggs vs. carved tree trunks) or format (landscape vs portraiture) or theme (religious vs funerary)"^^xsd:string ;
    rdfs:subClassOf wikidata:Q17537576,
        wikidata:Q483394 .

wikidata:Q18011131 rdfs:label "fictional military unit"^^xsd:string ;
    rdfs:comment "military unit that exists only in fiction"^^xsd:string ;
    rdfs:subClassOf wikidata:Q14623646 .

wikidata:Q18011141 rdfs:label "fictional military organization"^^xsd:string ;
    rdfs:comment "army that exists only in fiction"^^xsd:string ;
    rdfs:subClassOf wikidata:Q14623646 .

wikidata:Q18247357 rdfs:label "group of structures or buildings"^^xsd:string ;
    rdfs:comment "structures or buildings that do not form a building complex, but are treated as a group"^^xsd:string ;
    rdfs:subClassOf wikidata:Q66661745,
        wikidata:Q811430 .

wikidata:Q1826286 rdfs:label "religious movement"^^xsd:string ;
    rdfs:comment "social and ideological movement in the religious sphere"^^xsd:string ;
    rdfs:subClassOf wikidata:Q49773 .

wikidata:Q18674739 rdfs:label "event venue"^^xsd:string ;
    rdfs:comment "location suitable for hosting events"^^xsd:string ;
    rdfs:subClassOf wikidata:Q17350442,
        wikidata:Q41176 .

wikidata:Q18691599 rdfs:label "military facility"^^xsd:string ;
    rdfs:comment "place developed for and utilized by military forces"^^xsd:string ;
    rdfs:subClassOf wikidata:Q13226383 .

wikidata:Q18812548 rdfs:label "campaign"^^xsd:string ;
    rdfs:comment "series of operations undertaken to achieve a defined goal"^^xsd:string ;
    rdfs:subClassOf wikidata:Q1190554,
        wikidata:Q180684 .

wikidata:Q18984099 rdfs:label "ferry route"^^xsd:string ;
    rdfs:comment "regularly scheduled ship route providing ferry service"^^xsd:string ;
    rdfs:subClassOf wikidata:Q1067164 .

wikidata:Q192851 rdfs:label "arcade game machine"^^xsd:string ;
    rdfs:comment "coin-operated entertainment machine"^^xsd:string ;
    rdfs:subClassOf wikidata:Q241317 .

wikidata:Q1964689 rdfs:label "fictional city"^^xsd:string ;
    rdfs:comment "town or city that does not exist in real life"^^xsd:string ;
    rdfs:subClassOf wikidata:Q3895768 .

wikidata:Q2001305 rdfs:label "television channel"^^xsd:string ;
    rdfs:comment "channel over which a television station is distributed"^^xsd:string .

wikidata:Q2061186 rdfs:label "religious order"^^xsd:string ;
    rdfs:comment "group of people set apart from society and other groups based on their religious devotion"^^xsd:string ;
    rdfs:subClassOf wikidata:Q1530022 .

wikidata:Q207628 rdfs:label "musical composition"^^xsd:string ;
    rdfs:comment "original piece or work of music, either vocal or instrumental, the structure of a musical piece"^^xsd:string ;
    rdfs:subClassOf wikidata:Q2188189 .

wikidata:Q2085381 rdfs:label "publisher"^^xsd:string ;
    rdfs:comment "organisation that prints and distributes pressed goods or electronic media"^^xsd:string ;
    rdfs:subClassOf wikidata:Q1331793,
        wikidata:Q43229 .

wikidata:Q20871196 rdfs:label "fictional vehicle"^^xsd:string ;
    rdfs:comment "vehicle only appearing in fictional stories"^^xsd:string ;
    rdfs:subClassOf wikidata:Q15706911,
        wikidata:Q42889,
        wikidata:Q6619802 .

wikidata:Q209163 rdfs:label "video game expansion pack"^^xsd:string ;
    rdfs:comment "addition to an existing video game"^^xsd:string ;
    rdfs:subClassOf wikidata:Q7889 .

wikidata:Q210272 rdfs:label "cultural heritage"^^xsd:string ;
    rdfs:comment "physical artifact or intangible attribute of a society inherited from past generations"^^xsd:string ;
    rdfs:subClassOf wikidata:Q11862829 .

wikidata:Q214609 rdfs:label "material"^^xsd:string ;
    rdfs:comment "substance that can occur in different amounts, all with some similar [mixture of some] characteristics, and of which objects can be made up"^^xsd:string ;
    rdfs:subClassOf wikidata:Q2424752 .

wikidata:Q2217301 rdfs:label "serial"^^xsd:string ;
    rdfs:comment "publication in any medium issued under the same title in a succession of discrete parts, usually numbered (or dated) and appearing at regular or irregular intervals with no predetermined conclusion"^^xsd:string ;
    rdfs:subClassOf wikidata:Q732577,
        wikidata:Q7725310 .

wikidata:Q22325163 rdfs:label "protein-containing complex"^^xsd:string ;
    rdfs:comment "stable assembly of two or more macromolecules, i.e. proteins, nucleic acids, carbohydrates or lipids, in which at least one component is a protein and the constituent parts function together"^^xsd:string .

wikidata:Q22652 rdfs:label "green space"^^xsd:string ;
    rdfs:comment "green area planned in an urban location"^^xsd:string .

wikidata:Q228332 rdfs:label "entry point"^^xsd:string ;
    rdfs:comment "generic term for places where passengers and goods get on and off public transport"^^xsd:string ;
    rdfs:subClassOf wikidata:Q13226383,
        wikidata:Q618123 .

wikidata:Q23807345 rdfs:label "competition"^^xsd:string ;
    rdfs:comment "term referring either to competition in nature or between contestants (see talk page)"^^xsd:string ;
    rdfs:subClassOf wikidata:Q1914636 .

wikidata:Q24229398 rdfs:label "agent"^^xsd:string ;
    rdfs:comment "an individual and identifiable entity capable of performing actions"^^xsd:string .

wikidata:Q24962887 rdfs:label "violation of law"^^xsd:string ;
    rdfs:comment "act (or omission) that fails to abide by existing law"^^xsd:string .

wikidata:Q26160672 rdfs:label "revoiced work"^^xsd:string ;
    rdfs:comment "work revoiced in another language"^^xsd:string ;
    rdfs:subClassOf wikidata:Q3331189,
        wikidata:Q386724 .

wikidata:Q26204053 rdfs:label "dubbing of film"^^xsd:string ;
    rdfs:comment "revoiced film; film version, in which the original voices are replaced with voices in another language"^^xsd:string ;
    rdfs:subClassOf wikidata:Q26160672 .

wikidata:Q2665272 rdfs:label "Ecclesiastical circumscription immediately subject to the Holy See"^^xsd:string ;
    rdfs:comment ""^^xsd:string ;
    rdfs:subClassOf wikidata:Q3146899 .

wikidata:Q2684591 rdfs:label "statement"^^xsd:string ;
    rdfs:comment "meaningful declarative sentence that is either true or false, or that which a true or false declarative sentence asserts"^^xsd:string .

wikidata:Q268592 rdfs:label "industry"^^xsd:string ;
    rdfs:comment "group of companies that produce a closely related set of raw materials, goods, or services"^^xsd:string ;
    rdfs:subClassOf wikidata:Q58778 .

wikidata:Q26907166 rdfs:label "temporal entity"^^xsd:string ;
    rdfs:comment "thing that can be contained within a period of time, or change in state (e.g. events, periods, acts)"^^xsd:string .

wikidata:Q28790362 rdfs:label "ethnic community"^^xsd:string ;
    rdfs:comment "in a specific country or region"^^xsd:string ;
    rdfs:subClassOf wikidata:Q41710 .

wikidata:Q28885102 rdfs:label "pharmaceutical product"^^xsd:string ;
    rdfs:comment "qualitative and quantitative composition of a medicinal product in the dose form authorized for administration by a medicines regulatory agency and as represented with any corresponding regulated product information"^^xsd:string .

wikidata:Q31629 rdfs:label "type of sport"^^xsd:string ;
    rdfs:comment "specific sport"^^xsd:string .

wikidata:Q31855 rdfs:label "research institute"^^xsd:string ;
    rdfs:comment "establishment endowed for doing research"^^xsd:string ;
    rdfs:subClassOf wikidata:Q1664720 .

wikidata:Q3320743 rdfs:label "title of honor"^^xsd:string ;
    rdfs:comment "title bestowed upon individuals or organizations as an award in recognition of their merits"^^xsd:string ;
    rdfs:subClassOf wikidata:Q216353,
        wikidata:Q618779 .

wikidata:Q334453 rdfs:label "division"^^xsd:string ;
    rdfs:comment "distinct and large part of an organization"^^xsd:string .

wikidata:Q34394 rdfs:label "belief"^^xsd:string ;
    rdfs:comment "psychological state in which an individual holds a proposition or premise to be true"^^xsd:string .

wikidata:Q34508 rdfs:label "videotape recording"^^xsd:string ;
    rdfs:comment "electronic medium for the recording, copying and broadcasting of moving visual images"^^xsd:string ;
    rdfs:subClassOf wikidata:Q1209283,
        wikidata:Q2431196 .

wikidata:Q35535 rdfs:label "police"^^xsd:string ;
    rdfs:comment "constituted body of persons empowered by the state to enforce the law"^^xsd:string ;
    rdfs:subClassOf wikidata:Q12737077,
        wikidata:Q732717 .

wikidata:Q35798 rdfs:label "executive branch"^^xsd:string ;
    rdfs:comment "part of government that has sole authority and responsibility for the daily administration of the state"^^xsd:string ;
    rdfs:subClassOf wikidata:Q7210356 .

wikidata:Q36341 rdfs:label "brown bear"^^xsd:string ;
    rdfs:comment "species of mammal"^^xsd:string .

wikidata:Q3914 rdfs:label "school"^^xsd:string ;
    rdfs:comment "institution designed to teach students under the direction of school teacher"^^xsd:string ;
    rdfs:subClassOf wikidata:Q2385804,
        wikidata:Q811979 .

wikidata:Q39201 rdfs:label "pet"^^xsd:string ;
    rdfs:comment "animal kept for companionship and a person's enjoyment"^^xsd:string ;
    rdfs:subClassOf wikidata:Q26401003,
        wikidata:Q28877,
        wikidata:Q57812559,
        wikidata:Q622852 .

wikidata:Q4006 rdfs:label "map"^^xsd:string ;
    rdfs:comment "visual representation of a geographical area"^^xsd:string .

wikidata:Q40231 rdfs:label "election"^^xsd:string ;
    rdfs:comment "process by which a population chooses an individual to hold public office or some other position, such as in an organization or society"^^xsd:string ;
    rdfs:subClassOf wikidata:Q841654 .

wikidata:Q41298 rdfs:label "magazine"^^xsd:string ;
    rdfs:comment "publication type"^^xsd:string ;
    rdfs:subClassOf wikidata:Q1002697,
        wikidata:Q340169 .

wikidata:Q4358176 rdfs:label "council"^^xsd:string ;
    rdfs:comment "group of people who come together to consult, deliberate, or make decisions"^^xsd:string ;
    rdfs:subClassOf wikidata:Q16334295,
        wikidata:Q43229,
        wikidata:Q895526 .

wikidata:Q48204 rdfs:label "voluntary association"^^xsd:string ;
    rdfs:comment "group of people with shared interests or aims"^^xsd:string ;
    rdfs:subClassOf wikidata:Q15911314 .

wikidata:Q4936952 rdfs:label "anatomical structure"^^xsd:string ;
    rdfs:comment "entity with a single connected inherent 3D shape that's created by coordinated expression of the organism's own DNA"^^xsd:string .

wikidata:Q49371 rdfs:label "legislation"^^xsd:string ;
    rdfs:comment "law enacted by a legislature or other governing body"^^xsd:string ;
    rdfs:subClassOf wikidata:Q820655 .

wikidata:Q49447 rdfs:label "world view"^^xsd:string ;
    rdfs:comment "fundamental cognitive orientation of an individual or society encompassing the entirety of the individual or society's knowledge and point of view"^^xsd:string .

wikidata:Q5003624 rdfs:label "memorial"^^xsd:string ;
    rdfs:comment "area or object which serves as a focus for memory of something"^^xsd:string ;
    rdfs:subClassOf wikidata:Q4989906 .

wikidata:Q502895 rdfs:label "common name"^^xsd:string ;
    rdfs:comment "name generally used for a taxon, group of taxa or organism(s)"^^xsd:string .

wikidata:Q5107 rdfs:label "continent"^^xsd:string ;
    rdfs:comment "very large landmass"^^xsd:string ;
    rdfs:subClassOf wikidata:Q2221906 .

wikidata:Q5341295 rdfs:label "educational organization"^^xsd:string ;
    rdfs:comment "body with an aim of education"^^xsd:string ;
    rdfs:subClassOf wikidata:Q43229 .

wikidata:Q55983715 rdfs:label "organisms known by a particular common name"^^xsd:string ;
    rdfs:comment "living organism Wikidata metaclass"^^xsd:string .

wikidata:Q56019 rdfs:label "military rank"^^xsd:string ;
    rdfs:comment "element of hierarchy in armed forces"^^xsd:string .

wikidata:Q57812559 rdfs:label "animal living in captivity"^^xsd:string ;
    rdfs:comment ""^^xsd:string ;
    rdfs:subClassOf wikidata:Q26401003 .

wikidata:Q57812611 rdfs:label "mammal living in captivity"^^xsd:string ;
    rdfs:comment "individual mammal"^^xsd:string ;
    rdfs:subClassOf wikidata:Q57812559 .

wikidata:Q5916 rdfs:label "spaceflight"^^xsd:string ;
    rdfs:comment "use of technology to achieve the flight of spacecraft into and through outer space, used in space exploration, and also in commercial activities like space tourism and satellite telecommunications"^^xsd:string .

wikidata:Q61788060 rdfs:label "human activity"^^xsd:string ;
    rdfs:comment "activity initiated by a human, intentionally or unintentionally"^^xsd:string ;
    rdfs:subClassOf wikidata:Q1914636 .

wikidata:Q62447 rdfs:label "aerodrome"^^xsd:string ;
    rdfs:comment "location from which aircraft flight operations take place"^^xsd:string ;
    rdfs:subClassOf wikidata:Q17350442,
        wikidata:Q43229,
        wikidata:Q811979 .

wikidata:Q63187345 rdfs:label "religious occupation"^^xsd:string ;
    rdfs:comment "occupation or profession that serves a purpose within the context of a religion"^^xsd:string ;
    rdfs:subClassOf wikidata:Q12737077,
        wikidata:Q4164871 .

wikidata:Q65943 rdfs:label "theorem"^^xsd:string ;
    rdfs:comment "(within mathematic and logic) a mathematical statement that can be proven"^^xsd:string ;
    rdfs:subClassOf wikidata:Q2684591 .

wikidata:Q6619802 rdfs:label "fictional mode of transport"^^xsd:string ;
    rdfs:comment "any form of fictional vehicle or fictional system used to transport people or goods from one place to another"^^xsd:string ;
    rdfs:subClassOf wikidata:Q14897293 .

wikidata:Q694045 rdfs:label "delegated legislation"^^xsd:string ;
    rdfs:comment "law made by someone other than the legislature but with the legislature's authority"^^xsd:string ;
    rdfs:subClassOf wikidata:Q1864008,
        wikidata:Q49371 .

wikidata:Q718893 rdfs:label "theater"^^xsd:string ;
    rdfs:comment "area or place in which important military events occur or are progressing"^^xsd:string ;
    rdfs:subClassOf wikidata:Q15642541 .

wikidata:Q7257 rdfs:label "ideology"^^xsd:string ;
    rdfs:comment "set of ideas that form one's aims, expectations and actions"^^xsd:string .

wikidata:Q735 rdfs:label "art"^^xsd:string ;
    rdfs:comment "expressive work intended to be appreciated for its beauty or emotional power; or the process of creating such a work"^^xsd:string ;
    rdfs:subClassOf wikidata:Q1914636,
        wikidata:Q3249551 .

wikidata:Q74817647 rdfs:label "aspect in a geographic region"^^xsd:string ;
    rdfs:comment "type of aspect"^^xsd:string .

wikidata:Q7930989 rdfs:label "city/town"^^xsd:string ;
    rdfs:comment "human settlement"^^xsd:string ;
    rdfs:subClassOf wikidata:Q486972,
        wikidata:Q56061 .

wikidata:Q79719 rdfs:label "license"^^xsd:string ;
    rdfs:comment "set of permissions and restrictions to use something"^^xsd:string .

wikidata:Q811701 rdfs:label "model series"^^xsd:string ;
    rdfs:comment "group of related products, sold simultaneously or consecutively"^^xsd:string ;
    rdfs:subClassOf wikidata:Q20937557 .

wikidata:Q8142 rdfs:label "currency"^^xsd:string ;
    rdfs:comment "generally accepted medium of exchange for goods or services"^^xsd:string ;
    rdfs:subClassOf wikidata:Q47574 .

wikidata:Q8192 rdfs:label "writing system"^^xsd:string ;
    rdfs:comment "any conventional method of visually representing verbal or signed communication"^^xsd:string .

wikidata:Q81941037 rdfs:label "product distribution method"^^xsd:string ;
    rdfs:comment "method of product distribution and delivery"^^xsd:string .

wikidata:Q83267 rdfs:label "crime"^^xsd:string ;
    rdfs:comment "unlawful act forbidden and punishable by criminal law"^^xsd:string ;
    rdfs:subClassOf wikidata:Q1456832,
        wikidata:Q24962887 .

wikidata:Q8502 rdfs:label "mountain"^^xsd:string ;
    rdfs:comment "large landform that stretches above the surrounding land"^^xsd:string ;
    rdfs:subClassOf wikidata:Q2221906,
        wikidata:Q54050 .

wikidata:Q867335 rdfs:label "literary cycle"^^xsd:string ;
    rdfs:comment "group of stories grouped around common figures"^^xsd:string ;
    rdfs:subClassOf wikidata:Q7725310,
        wikidata:Q7725634 .

wikidata:Q8928 rdfs:label "constellation"^^xsd:string ;
    rdfs:comment "one of the 88 divisions of the celestial sphere, defined by the IAU, many of which derive from traditional asterisms"^^xsd:string ;
    rdfs:subClassOf wikidata:Q6999 .

wikidata:Q895526 rdfs:label "organ"^^xsd:string ;
    rdfs:comment "human or group of people forming a body designated to exercise certain activities on behalf of a legal entity or a state"^^xsd:string ;
    rdfs:subClassOf wikidata:Q43229 .

wikidata:Q9134 rdfs:label "mythology"^^xsd:string ;
    rdfs:comment "stories of gods and fairies and fantastic creatures"^^xsd:string ;
    rdfs:subClassOf wikidata:Q34394,
        wikidata:Q49447 .

wikidata:Q9143 rdfs:label "programming language"^^xsd:string ;
    rdfs:comment "language designed to communicate instructions to a machine"^^xsd:string ;
    rdfs:subClassOf wikidata:Q629206 .

wikidata:Q9174 rdfs:label "religion"^^xsd:string ;
    rdfs:comment "set of beliefs, practices and traditions for a group or community"^^xsd:string ;
    rdfs:subClassOf wikidata:Q11862829,
        wikidata:Q49447,
        wikidata:Q7257 .

wikidata:Q924286 rdfs:label "transport network"^^xsd:string ;
    rdfs:comment "physical spacial network for vehicle movement and transportation of goods over thoroughfares between multiple locations"^^xsd:string ;
    rdfs:subClassOf wikidata:Q121359,
        wikidata:Q27096235,
        wikidata:Q376799,
        wikidata:Q58778 .

wikidata:Q97180164 rdfs:label "Dessin artistique sur ordinateur"^^xsd:string ;
    rdfs:comment ""^^xsd:string .

wikidata:Q98119401 rdfs:label "group or class of physical objects"^^xsd:string ;
    rdfs:comment ""^^xsd:string .

wikidata:P1344 rdfs:label "participant in"^^xsd:string ;
    rdfs:comment "event in which a person or organization was/is a participant; inverse of P710 or P1923"^^xsd:string .

wikidata:P2321 rdfs:label "general classification of race participants"^^xsd:string ;
    rdfs:comment "classification of race participants"^^xsd:string ;
    rdfs:domain wikidata:Q13406554 ;
    rdfs:range wikidata:Q12973014,
        wikidata:Q5 ;
    rdfs:subPropertyOf wikidata:P710 .

wikidata:P31 rdfs:label "instance of"^^xsd:string ;
    rdfs:comment "that class of which this subject is a particular example and member"^^xsd:string .

wikidata:P50 rdfs:label "author"^^xsd:string ;
    rdfs:comment "main creator(s) of a written work (use on works, not humans); use P2093 when Wikidata item is unknown or does not exist"^^xsd:string ;
    rdfs:domain wikidata:Q15306849,
        wikidata:Q2668072,
        wikidata:Q277759,
        wikidata:Q3026787,
        wikidata:Q3331189,
        wikidata:Q386724,
        wikidata:Q55760865,
        wikidata:Q571 ;
    rdfs:range wikidata:Q16334295,
        wikidata:Q215627,
        wikidata:Q43229,
        wikidata:Q5,
        wikidata:Q61002,
        wikidata:Q95074 ;
    rdfs:subPropertyOf wikidata:P170 .

wikidata:Q1022867 rdfs:label "minor planet"^^xsd:string ;
    rdfs:comment "astronomical object in direct orbit around a star that is neither a planet nor a comet"^^xsd:string ;
    rdfs:subClassOf wikidata:Q3132741 .

wikidata:Q1030034 rdfs:label "GLAM"^^xsd:string ;
    rdfs:comment "acronym for \"galleries, libraries, archives, and museums\" that refers to cultural institutions that have access to knowledge as their mission"^^xsd:string ;
    rdfs:subClassOf wikidata:Q294440 .

wikidata:Q1048236 rdfs:label "machine-readable medium"^^xsd:string ;
    rdfs:comment "medium capable of storing data in a format readable by a mechanical device (rather than human readable)"^^xsd:string .

wikidata:Q11253473 rdfs:label "smart device"^^xsd:string ;
    rdfs:comment "electronic device connected via different wireless protocols to its environment"^^xsd:string ;
    rdfs:subClassOf wikidata:Q2858615 .

wikidata:Q11578774 rdfs:label "broadcasting program"^^xsd:string ;
    rdfs:comment "segment of content for broadcast"^^xsd:string ;
    rdfs:subClassOf wikidata:Q1190554,
        wikidata:Q732577 .

wikidata:Q12284 rdfs:label "canal"^^xsd:string ;
    rdfs:comment "man-made channel for water"^^xsd:string ;
    rdfs:subClassOf wikidata:Q355304 .

wikidata:Q1229765 rdfs:label "watercraft"^^xsd:string ;
    rdfs:comment "vehicles that are intended for locomotion on or in the water"^^xsd:string ;
    rdfs:subClassOf wikidata:Q42889 .

wikidata:Q123705 rdfs:label "neighborhood"^^xsd:string ;
    rdfs:comment "geographically localised community within a larger city, town or suburb"^^xsd:string ;
    rdfs:subClassOf wikidata:Q15642541,
        wikidata:Q486972,
        wikidata:Q56061 .

wikidata:Q12819564 rdfs:label "station"^^xsd:string ;
    rdfs:comment "intermediate stopping places along transportation routes"^^xsd:string ;
    rdfs:subClassOf wikidata:Q41176,
        wikidata:Q548662,
        wikidata:Q55006986 .

wikidata:Q1298668 rdfs:label "research project"^^xsd:string ;
    rdfs:comment "project of one or more scientists or an institute or a scientific society"^^xsd:string ;
    rdfs:subClassOf wikidata:Q170584 .

wikidata:Q1311670 rdfs:label "rail infrastructure"^^xsd:string ;
    rdfs:comment "immovable parts of rail transport"^^xsd:string ;
    rdfs:subClassOf wikidata:Q376799 .

wikidata:Q1331793 rdfs:label "media company"^^xsd:string ;
    rdfs:comment "business that focuses primarily in mass media"^^xsd:string ;
    rdfs:subClassOf wikidata:Q4830453,
        wikidata:Q783794 .

wikidata:Q1371819 rdfs:label "plan"^^xsd:string ;
    rdfs:comment "outline of a strategy for achievement of an objective"^^xsd:string ;
    rdfs:subClassOf wikidata:Q49848,
        wikidata:Q7184903 .

wikidata:Q14350 rdfs:label "radio station"^^xsd:string ;
    rdfs:comment "organization for the production and transmission of radio programs"^^xsd:string ;
    rdfs:subClassOf wikidata:Q15265344 .

wikidata:Q1497375 rdfs:label "architectural ensemble"^^xsd:string ;
    rdfs:comment "group of multiple related objects, such as buildings"^^xsd:string ;
    rdfs:subClassOf wikidata:Q18247357 .

wikidata:Q1509831 rdfs:label "title of Virgin Mary"^^xsd:string ;
    rdfs:comment "designation for Mary, mother of Jesus Christ"^^xsd:string ;
    rdfs:subClassOf wikidata:Q216353 .

wikidata:Q15331236 rdfs:label "fictional family"^^xsd:string ;
    rdfs:comment "family which only exists in a work of fiction"^^xsd:string ;
    rdfs:subClassOf wikidata:Q14514600 .

wikidata:Q15831596 rdfs:label "class of fictional entities"^^xsd:string ;
    rdfs:comment "Class and variable-order metaclass"^^xsd:string .

wikidata:Q16500104 rdfs:label "fictional body of water"^^xsd:string ;
    rdfs:comment "waterbody only existing in fiction"^^xsd:string ;
    rdfs:subClassOf wikidata:Q3895768 .

wikidata:Q1799072 rdfs:label "method"^^xsd:string ;
    rdfs:comment "planned path to reaching an objective"^^xsd:string ;
    rdfs:subClassOf wikidata:Q16686448 .

wikidata:Q1864008 rdfs:label "legal act"^^xsd:string ;
    rdfs:comment "juridical fact in which the subject who made it happen acted under free will"^^xsd:string ;
    rdfs:subClassOf wikidata:Q15621286 .

wikidata:Q18706315 rdfs:label "hypothetical entity"^^xsd:string ;
    rdfs:comment "entity whose existence is possible, but not proven"^^xsd:string ;
    rdfs:subClassOf wikidata:Q35120 .

wikidata:Q1931388 rdfs:label "cause of death"^^xsd:string ;
    rdfs:comment "specific disease or injury resulting in a human's death, which may be recorded on a death certificate"^^xsd:string .

wikidata:Q201662 rdfs:label "alter ego"^^xsd:string ;
    rdfs:comment "second self"^^xsd:string ;
    rdfs:subClassOf wikidata:Q844569 .

wikidata:Q20643955 rdfs:label "human biblical figure"^^xsd:string ;
    rdfs:comment "human (as opposed to supernatural) character in the Old Testament/Hebrew Bible or New Testament"^^xsd:string ;
    rdfs:subClassOf wikidata:Q21070568 .

wikidata:Q20830276 rdfs:label "group of mythical characters"^^xsd:string ;
    rdfs:comment "class of groupings of mythical entities"^^xsd:string ;
    rdfs:subClassOf wikidata:Q14514600,
        wikidata:Q24334685 .

wikidata:Q213283 rdfs:label "diplomatic mission"^^xsd:string ;
    rdfs:comment "group of people from one state present in another state to represent the sending state"^^xsd:string ;
    rdfs:subClassOf wikidata:Q27096235,
        wikidata:Q327333 .

wikidata:Q214339 rdfs:label "role"^^xsd:string ;
    rdfs:comment "set of behaviours, rights, obligations, beliefs, and norms expected from an individual that has a certain social status"^^xsd:string .

wikidata:Q2198855 rdfs:label "cultural movement"^^xsd:string ;
    rdfs:comment "period and movement in cultural history"^^xsd:string ;
    rdfs:subClassOf wikidata:Q3533467,
        wikidata:Q49773 .

wikidata:Q22698 rdfs:label "park"^^xsd:string ;
    rdfs:comment "permanently dedicated recreation area, often open to the public and generally characterized by natural, historic, or landscape features"^^xsd:string ;
    rdfs:subClassOf wikidata:Q13226383,
        wikidata:Q2221906,
        wikidata:Q22652,
        wikidata:Q294440 .

wikidata:Q22811462 rdfs:label "type of manufactured good"^^xsd:string ;
    rdfs:comment "first-order metaclass"^^xsd:string .

wikidata:Q24577840 rdfs:label "fictional group of characters"^^xsd:string ;
    rdfs:comment "group of characters that has been defined in a fictional work itself, as opposed to by a real person commenting on the work"^^xsd:string ;
    rdfs:subClassOf wikidata:Q14514600,
        wikidata:Q14623646 .

wikidata:Q2472587 rdfs:label "people"^^xsd:string ;
    rdfs:comment "plurality of persons considered as a whole, from a government perspective"^^xsd:string ;
    rdfs:subClassOf wikidata:Q16334295,
        wikidata:Q41710 .

wikidata:Q2590445 rdfs:label "fictional ethnic group"^^xsd:string ;
    rdfs:comment "ethnic group that only exists in fiction"^^xsd:string ;
    rdfs:subClassOf wikidata:Q14514600 .

wikidata:Q28020127 rdfs:label "fictional humanoid"^^xsd:string ;
    rdfs:comment "individual humanoid only appearing in fictional stories"^^xsd:string ;
    rdfs:subClassOf wikidata:Q2593744 .

wikidata:Q28640 rdfs:label "profession"^^xsd:string ;
    rdfs:comment "occupation requiring specialized training"^^xsd:string ;
    rdfs:subClassOf wikidata:Q1047113,
        wikidata:Q12737077 .

wikidata:Q2996394 rdfs:label "biological process"^^xsd:string ;
    rdfs:comment "process specifically pertinent to the functioning of integrated living units"^^xsd:string ;
    rdfs:subClassOf wikidata:Q3249551 .

wikidata:Q31464082 rdfs:label "source"^^xsd:string ;
    rdfs:comment "object (person, place, text, thing, etc.) from which something (information, goods, etc.) comes or is acquired"^^xsd:string ;
    rdfs:subClassOf wikidata:Q488383 .

wikidata:Q3146899 rdfs:label "diocese of the Catholic Church"^^xsd:string ;
    rdfs:comment "see under the supervision of a bishop of the Catholic church"^^xsd:string ;
    rdfs:subClassOf wikidata:Q20926517,
        wikidata:Q665487 .

wikidata:Q321839 rdfs:label "agreement"^^xsd:string ;
    rdfs:comment "understanding, agreement between two or more contracting persons, parties or entities"^^xsd:string .

wikidata:Q34379 rdfs:label "musical instrument"^^xsd:string ;
    rdfs:comment "sound-producing object used by a musician for this purpose"^^xsd:string ;
    rdfs:subClassOf wikidata:Q39546 .

wikidata:Q3464665 rdfs:label "television series season"^^xsd:string ;
    rdfs:comment "set of episodes produced for a television series"^^xsd:string ;
    rdfs:subClassOf wikidata:Q15416,
        wikidata:Q7725310 .

wikidata:Q3695082 rdfs:label "sign"^^xsd:string ;
    rdfs:comment "semiotic concept; object, quality, event, or entity whose presence or occurrence indicates the probable presence or occurrence of something else; includes words, punctuation, expressions, gestures, notices, road signs, symbols, pictures, etc."^^xsd:string ;
    rdfs:subClassOf wikidata:Q11028,
        wikidata:Q7184903 .

wikidata:Q3778211 rdfs:label "legal person"^^xsd:string ;
    rdfs:comment "any human or non-human entity that is recognized as having privileges and obligations; a legal fiction which is used to abstract away the differences between natural persons, juridical persons and other entities such as countries"^^xsd:string ;
    rdfs:subClassOf wikidata:Q24229398 .

wikidata:Q391414 rdfs:label "architectural element"^^xsd:string ;
    rdfs:comment "forms primarily as components of architecture"^^xsd:string ;
    rdfs:subClassOf wikidata:Q618123 .

wikidata:Q40056 rdfs:label "computer program"^^xsd:string ;
    rdfs:comment "sequence of instructions written in programming language to perform a specified task with a computer"^^xsd:string .

wikidata:Q40218 rdfs:label "spacecraft"^^xsd:string ;
    rdfs:comment "manned vehicle or unmanned machine designed to fly in outer space"^^xsd:string .

wikidata:Q4120621 rdfs:label "rank"^^xsd:string ;
    rdfs:comment "level in a hierarchy"^^xsd:string .

wikidata:Q42848 rdfs:label "data"^^xsd:string ;
    rdfs:comment "facts represented for handling"^^xsd:string ;
    rdfs:subClassOf wikidata:Q11028 .

wikidata:Q44782 rdfs:label "port"^^xsd:string ;
    rdfs:comment "maritime facility where ships may dock to load and discharge passengers and cargo"^^xsd:string ;
    rdfs:subClassOf wikidata:Q13226383 .

wikidata:Q46831 rdfs:label "mountain range"^^xsd:string ;
    rdfs:comment "geographic area containing numerous geologically related mountains"^^xsd:string ;
    rdfs:subClassOf wikidata:Q2221906,
        wikidata:Q271669 .

wikidata:Q47146 rdfs:label "user interface"^^xsd:string ;
    rdfs:comment "means by which a user interacts with and controls a machine"^^xsd:string ;
    rdfs:subClassOf wikidata:Q340169 .

wikidata:Q473972 rdfs:label "protected area"^^xsd:string ;
    rdfs:comment "area which receives protection because of its recognized natural, ecological, or cultural values"^^xsd:string ;
    rdfs:subClassOf wikidata:Q56061 .

wikidata:Q4801521 rdfs:label "arts festival"^^xsd:string ;
    rdfs:comment "festival that features the arts in a wide sense of the word, not just visual arts"^^xsd:string ;
    rdfs:subClassOf wikidata:Q132241 .

wikidata:Q483394 rdfs:label "genre"^^xsd:string ;
    rdfs:comment "category of creative works based on stylistic, thematic or technical criteria"^^xsd:string .

wikidata:Q484652 rdfs:label "international organization"^^xsd:string ;
    rdfs:comment "organization with an international membership, scope, or presence"^^xsd:string ;
    rdfs:subClassOf wikidata:Q43229 .

wikidata:Q4989906 rdfs:label "monument"^^xsd:string ;
    rdfs:comment "type of structure either explicitly created to commemorate a person or important event, or used for that purpose"^^xsd:string ;
    rdfs:subClassOf wikidata:Q210272,
        wikidata:Q811979 .

wikidata:Q559618 rdfs:label "fictional universe"^^xsd:string ;
    rdfs:comment "self-consistent fictional setting with elements that may differ from the real world"^^xsd:string ;
    rdfs:subClassOf wikidata:Q14897293 .

wikidata:Q61002 rdfs:label "pseudonym"^^xsd:string ;
    rdfs:comment "name that a person or group assumes for a particular purpose, which differs from their original or true name (orthonym)"^^xsd:string .

wikidata:Q622852 rdfs:label "domesticated animal"^^xsd:string ;
    rdfs:comment "animal that has been tamed and that lives with humans"^^xsd:string ;
    rdfs:subClassOf wikidata:Q729 .

wikidata:Q64520857 rdfs:label "fictional human formerly considered to be historical"^^xsd:string ;
    rdfs:comment "people who never existed but were once thought to have"^^xsd:string ;
    rdfs:subClassOf wikidata:Q15632617 .

wikidata:Q64643615 rdfs:label "prosopographical phantom"^^xsd:string ;
    rdfs:comment "hypothetical person deduced by modern historians who has been shown to have not existed"^^xsd:string ;
    rdfs:subClassOf wikidata:Q75855169 .

wikidata:Q68 rdfs:label "computer"^^xsd:string ;
    rdfs:comment "general-purpose device for performing arithmetic or logical operations"^^xsd:string ;
    rdfs:subClassOf wikidata:Q241317,
        wikidata:Q2858615 .

wikidata:Q6857706 rdfs:label "military specialism"^^xsd:string ;
    rdfs:comment "trade or career specialty in the armed forces which demand from the individuals achievement of qualifications"^^xsd:string ;
    rdfs:subClassOf wikidata:Q1047113,
        wikidata:Q28640 .

wikidata:Q6942562 rdfs:label "musical performance"^^xsd:string ;
    rdfs:comment "execution of music and/or song"^^xsd:string ;
    rdfs:subClassOf wikidata:Q35140 .

wikidata:Q7058673 rdfs:label "video game series"^^xsd:string ;
    rdfs:comment "multiple video games marketed under the same series name"^^xsd:string ;
    rdfs:subClassOf wikidata:Q28114058,
        wikidata:Q7725310 .

wikidata:Q726 rdfs:label "horse"^^xsd:string ;
    rdfs:comment "domesticated (work) animal"^^xsd:string .

wikidata:Q7366 rdfs:label "song"^^xsd:string ;
    rdfs:comment "musical composition for voice(s)"^^xsd:string ;
    rdfs:subClassOf wikidata:Q207628,
        wikidata:Q2188189,
        wikidata:Q7725634 .

wikidata:Q79529 rdfs:label "chemical substance"^^xsd:string ;
    rdfs:comment "matter of constant composition best characterized by the entities (molecules, formula units, atoms) it is composed of and characterized by physical properties like density"^^xsd:string ;
    rdfs:subClassOf wikidata:Q28732711 .

wikidata:Q8054 rdfs:label "protein"^^xsd:string ;
    rdfs:comment "biological molecule consisting of chains of amino acid residues"^^xsd:string .

wikidata:Q8076 rdfs:label "video game console"^^xsd:string ;
    rdfs:comment "interactive entertainment computer or customized computer system for running video games"^^xsd:string ;
    rdfs:subClassOf wikidata:Q241317 .

wikidata:Q811704 rdfs:label "rolling stock class"^^xsd:string ;
    rdfs:comment "part of railroad rolling stock classification system"^^xsd:string ;
    rdfs:subClassOf wikidata:Q29048322 .

wikidata:Q8148 rdfs:label "industry"^^xsd:string ;
    rdfs:comment "economic branch characterized by large scale automated manufacturing as in industrialization"^^xsd:string ;
    rdfs:subClassOf wikidata:Q1914636 .

wikidata:Q82036085 rdfs:label "physical media format"^^xsd:string ;
    rdfs:comment "umbrella class; any physical format for distribution of written words, images, audio, video, etc."^^xsd:string ;
    rdfs:subClassOf wikidata:Q1207505 .

wikidata:Q844569 rdfs:label "identity"^^xsd:string ;
    rdfs:comment "qualities, beliefs, personality, looks and/or expressions that distinguish a person or group"^^xsd:string ;
    rdfs:subClassOf wikidata:Q1207505 .

wikidata:Q95107111 rdfs:label "license scheme"^^xsd:string ;
    rdfs:comment "a group of software licenses"^^xsd:string ;
    rdfs:subClassOf wikidata:Q16887380 .

wikidata:P1038 rdfs:label "relative"^^xsd:string ;
    rdfs:comment "family member (qualify with \"type of kinship\", P1039; for direct family member please use specific property)"^^xsd:string ;
    rdfs:domain wikidata:Q1313923,
        wikidata:Q15632617,
        wikidata:Q1569167,
        wikidata:Q15711870,
        wikidata:Q15773347,
        wikidata:Q16979650,
        wikidata:Q178885,
        wikidata:Q21070598,
        wikidata:Q5,
        wikidata:Q8436,
        wikidata:Q95074 ;
    rdfs:range wikidata:Q1569167,
        wikidata:Q178885,
        wikidata:Q21070598,
        wikidata:Q5,
        wikidata:Q95074 ;
    rdfs:subPropertyOf wikidata:P3342 .

wikidata:P910 rdfs:label "topic's main category"^^xsd:string ;
    rdfs:comment "main Wikimedia category"^^xsd:string ;
    rdfs:range wikidata:Q4167836 .

wikidata:Q101352 rdfs:label "family name"^^xsd:string ;
    rdfs:comment "part of a naming scheme for individuals, used in many cultures worldwide"^^xsd:string .

wikidata:Q105420 rdfs:label "anthology"^^xsd:string ;
    rdfs:comment "collection of creative works chosen by the compiler"^^xsd:string ;
    rdfs:subClassOf wikidata:Q17489659,
        wikidata:Q2668072 .

wikidata:Q11019 rdfs:label "machine"^^xsd:string ;
    rdfs:comment "tool containing one or more parts that uses energy to perform an intended action"^^xsd:string ;
    rdfs:subClassOf wikidata:Q1183543,
        wikidata:Q39546 .

wikidata:Q11266439 rdfs:label "Wikimedia template"^^xsd:string ;
    rdfs:comment "type of page in the Wikimedia system. Use with P31 'instance of' for template pages"^^xsd:string .

wikidata:Q1172284 rdfs:label "data set"^^xsd:string ;
    rdfs:comment "collection of data"^^xsd:string ;
    rdfs:subClassOf wikidata:Q15621286,
        wikidata:Q2668072 .

wikidata:Q12280 rdfs:label "bridge"^^xsd:string ;
    rdfs:comment "structure that spans and provides a passage over a road, railway, river, or some other obstacle"^^xsd:string ;
    rdfs:subClassOf wikidata:Q811979,
        wikidata:Q83620 .

wikidata:Q1266946 rdfs:label "thesis"^^xsd:string ;
    rdfs:comment "document submitted in support of candidature for an academic degree"^^xsd:string .

wikidata:Q132241 rdfs:label "festival"^^xsd:string ;
    rdfs:comment "celebration that focuses upon a theme, and may run for hours to weeks; usually repeated regularily, eg. once a year"^^xsd:string ;
    rdfs:subClassOf wikidata:Q15275719,
        wikidata:Q43229 .

wikidata:Q13406463 rdfs:label "Wikimedia list article"^^xsd:string ;
    rdfs:comment "page of a Wikimedia project with a list of something"^^xsd:string ;
    rdfs:subClassOf wikidata:Q12139612 .

wikidata:Q1370598 rdfs:label "place of worship"^^xsd:string ;
    rdfs:comment "specially designed structure or consecrated space for use in worshipping"^^xsd:string ;
    rdfs:subClassOf wikidata:Q13226383,
        wikidata:Q21029893,
        wikidata:Q811979 .

wikidata:Q1445650 rdfs:label "holiday"^^xsd:string ;
    rdfs:comment "festive day set aside by custom or by law"^^xsd:string ;
    rdfs:subClassOf wikidata:Q14795564,
        wikidata:Q15275719 .

wikidata:Q15306849 rdfs:label "fictitious work"^^xsd:string ;
    rdfs:comment "creative work that only exists within a fictional narative"^^xsd:string ;
    rdfs:subClassOf wikidata:Q14897293 .

wikidata:Q15619164 rdfs:label "abstract being"^^xsd:string ;
    rdfs:comment "entity that has no physical realisation"^^xsd:string .

wikidata:Q16070115 rdfs:label "video game compilation"^^xsd:string ;
    rdfs:comment "multiple computer and video games sold as a single product"^^xsd:string ;
    rdfs:subClassOf wikidata:Q105420,
        wikidata:Q7889 .

wikidata:Q16334298 rdfs:label "group of living things"^^xsd:string ;
    rdfs:comment "set of live physical entities of any nature"^^xsd:string .

wikidata:Q16338046 rdfs:label "fictional river"^^xsd:string ;
    rdfs:comment "river which only exists in fiction"^^xsd:string ;
    rdfs:subClassOf wikidata:Q16500104 .

wikidata:Q16798631 rdfs:label "equipment"^^xsd:string ;
    rdfs:comment "collective term for all items that are required to exercise a certain activity"^^xsd:string ;
    rdfs:subClassOf wikidata:Q2424752,
        wikidata:Q8205328 .

wikidata:Q17335294 rdfs:label "flag or coat of arms"^^xsd:string ;
    rdfs:comment "class for all items that are a flag or coat of arms"^^xsd:string .

wikidata:Q17350442 rdfs:label "venue"^^xsd:string ;
    rdfs:comment "place used for some activity"^^xsd:string ;
    rdfs:subClassOf wikidata:Q13226383,
        wikidata:Q1496967,
        wikidata:Q2221906 .

wikidata:Q178706 rdfs:label "institution"^^xsd:string ;
    rdfs:comment "structure or mechanism of social order and cooperation governing the behaviour of a set of individuals within a given community"^^xsd:string ;
    rdfs:subClassOf wikidata:Q43229 .

wikidata:Q18643213 rdfs:label "military equipment"^^xsd:string ;
    rdfs:comment "item in use by or designed for use by military forces"^^xsd:string ;
    rdfs:subClassOf wikidata:Q16798631 .

wikidata:Q1983062 rdfs:label "episode"^^xsd:string ;
    rdfs:comment "part of a work such as a serial television or radio drama"^^xsd:string ;
    rdfs:subClassOf wikidata:Q2431196 .

wikidata:Q21192438 rdfs:label "fictional species"^^xsd:string ;
    rdfs:comment "species that only exists in fiction; for individual fictional organisms, use Q30017383"^^xsd:string ;
    rdfs:subClassOf wikidata:Q14897293,
        wikidata:Q15707583 .

wikidata:Q2385804 rdfs:label "educational institution"^^xsd:string ;
    rdfs:comment "institution that provides education"^^xsd:string ;
    rdfs:subClassOf wikidata:Q5341295 .

wikidata:Q3024240 rdfs:label "historical country"^^xsd:string ;
    rdfs:comment "country, state or territory that once existed"^^xsd:string ;
    rdfs:subClassOf wikidata:Q6256 .

wikidata:Q317623 rdfs:label "technical standard"^^xsd:string ;
    rdfs:comment "established norm or requirement to facilitate consistency"^^xsd:string ;
    rdfs:subClassOf wikidata:Q49848,
        wikidata:Q7406919 .

wikidata:Q327245 rdfs:label "team"^^xsd:string ;
    rdfs:comment "group linked in a common purpose"^^xsd:string ;
    rdfs:subClassOf wikidata:Q16334295,
        wikidata:Q43229 .

wikidata:Q35120 rdfs:label "entity"^^xsd:string ;
    rdfs:comment "thing with independent and distinct existence"^^xsd:string .

wikidata:Q3533467 rdfs:label "group action"^^xsd:string ;
    rdfs:comment "term in sociology"^^xsd:string .

wikidata:Q44377 rdfs:label "tunnel"^^xsd:string ;
    rdfs:comment "underground passage"^^xsd:string .

wikidata:Q464980 rdfs:label "exhibition"^^xsd:string ;
    rdfs:comment "organized presentation and display of a selection of items or pictures"^^xsd:string ;
    rdfs:subClassOf wikidata:Q1030034,
        wikidata:Q1190554,
        wikidata:Q386724 .

wikidata:Q482994 rdfs:label "album"^^xsd:string ;
    rdfs:comment "collection of recorded music, words, sounds"^^xsd:string ;
    rdfs:subClassOf wikidata:Q2031291 .

wikidata:Q5446565 rdfs:label "fictional company"^^xsd:string ;
    rdfs:comment "business organization which only exists in fiction"^^xsd:string ;
    rdfs:subClassOf wikidata:Q14623646 .

wikidata:Q570116 rdfs:label "tourist attraction"^^xsd:string ;
    rdfs:comment "place of interest where tourists visit"^^xsd:string .

wikidata:Q571 rdfs:label "book"^^xsd:string ;
    rdfs:comment "a written text that can be published in printed or electronic form"^^xsd:string ;
    rdfs:subClassOf wikidata:Q49848,
        wikidata:Q732577 .

wikidata:Q645883 rdfs:label "military operation"^^xsd:string ;
    rdfs:comment "coordinated military actions of a state or a non-state actor in response to a developing situation"^^xsd:string ;
    rdfs:subClassOf wikidata:Q1190554 .

wikidata:Q665487 rdfs:label "diocese"^^xsd:string ;
    rdfs:comment "Christian district or see under the supervision of a bishop"^^xsd:string ;
    rdfs:subClassOf wikidata:Q1492823,
        wikidata:Q20926517,
        wikidata:Q51041800 .

wikidata:Q6671777 rdfs:label "structure"^^xsd:string ;
    rdfs:comment "arrangement and organization of interrelated elements in an object or system, or the object or system so organized"^^xsd:string ;
    rdfs:subClassOf wikidata:Q35120 .

wikidata:Q728 rdfs:label "weapon"^^xsd:string ;
    rdfs:comment "tool used to inflict damage or harm"^^xsd:string ;
    rdfs:subClassOf wikidata:Q18643213,
        wikidata:Q39546 .

wikidata:Q7302866 rdfs:label "audio track"^^xsd:string ;
    rdfs:comment "track on a music album, EP or single"^^xsd:string .

wikidata:Q811430 rdfs:label "human-made geographic feature"^^xsd:string ;
    rdfs:comment "artificial construction meant to remain at a fixed geographic location"^^xsd:string ;
    rdfs:subClassOf wikidata:Q386724,
        wikidata:Q618123 .

wikidata:Q847017 rdfs:label "sports club"^^xsd:string ;
    rdfs:comment "organization for the purpose of playing one or more sports"^^xsd:string ;
    rdfs:subClassOf wikidata:Q4438121 .

wikidata:Q853614 rdfs:label "identifier"^^xsd:string ;
    rdfs:comment "name that identifies either a unique object or a unique class of objects"^^xsd:string .

wikidata:P170 rdfs:label "creator"^^xsd:string ;
    rdfs:comment "maker of this creative work or other object (where no more specific property exists). Paintings with unknown painters, use \"anonymous\" (Q4233718) as value."^^xsd:string ;
    rdfs:domain wikidata:Q151885,
        wikidata:Q1656682,
        wikidata:Q16686448,
        wikidata:Q170584,
        wikidata:Q17489659,
        wikidata:Q18593264,
        wikidata:Q18706315,
        wikidata:Q18812548,
        wikidata:Q2424752,
        wikidata:Q2684591,
        wikidata:Q321839,
        wikidata:Q386724,
        wikidata:Q58778,
        wikidata:Q61788060,
        wikidata:Q80071 ;
    rdfs:range wikidata:Q11019,
        wikidata:Q14514600,
        wikidata:Q16017119,
        wikidata:Q16334295,
        wikidata:Q20643955,
        wikidata:Q4233718,
        wikidata:Q4271324,
        wikidata:Q43229,
        wikidata:Q5,
        wikidata:Q729,
        wikidata:Q95074 .

wikidata:P3092 rdfs:label "film crew member"^^xsd:string ;
    rdfs:comment "member of the crew creating an audiovisual work, used for miscellaneous roles qualified with the job title when no specific property exists. Don't use if such a property is available: notably for cast member (P161), director (P57), etc."^^xsd:string ;
    rdfs:domain wikidata:Q2431196,
        wikidata:Q26204053 ;
    rdfs:range wikidata:Q5 ;
    rdfs:subPropertyOf wikidata:P3342 .

wikidata:Q10648343 rdfs:label "duo"^^xsd:string ;
    rdfs:comment "two people that work together"^^xsd:string ;
    rdfs:subClassOf wikidata:Q16334295,
        wikidata:Q327245 .

wikidata:Q12140 rdfs:label "medication"^^xsd:string ;
    rdfs:comment "substance used to diagnose, cure, treat, or prevent disease"^^xsd:string ;
    rdfs:subClassOf wikidata:Q28885102 .

wikidata:Q1261026 rdfs:label "printed matter"^^xsd:string ;
    rdfs:comment "printed material produced by printers or publishers"^^xsd:string ;
    rdfs:subClassOf wikidata:Q2424752,
        wikidata:Q49848,
        wikidata:Q82036085 .

wikidata:Q1313923 rdfs:label "kindred"^^xsd:string ;
    rdfs:comment "group of related persons"^^xsd:string ;
    rdfs:subClassOf wikidata:Q16334295 .

wikidata:Q14795564 rdfs:label "point in time with respect to recurrent timeframe"^^xsd:string ;
    rdfs:comment "item to calculate dates of periodic occurence"^^xsd:string ;
    rdfs:subClassOf wikidata:Q1190554 .

wikidata:Q166142 rdfs:label "application"^^xsd:string ;
    rdfs:comment "program or group of programs designed for end-users"^^xsd:string ;
    rdfs:subClassOf wikidata:Q7397 .

wikidata:Q16979650 rdfs:label "sibling group"^^xsd:string ;
    rdfs:comment "group of humans, they are siblings; e.g. Grimm brothers, Brontë sisters"^^xsd:string ;
    rdfs:subClassOf wikidata:Q1313923,
        wikidata:Q16334295 .

wikidata:Q1707847 rdfs:label "role"^^xsd:string ;
    rdfs:comment "character or part played by a performer"^^xsd:string .

wikidata:Q17149090 rdfs:label "armed organization"^^xsd:string ;
    rdfs:comment "organization which achieves or tries to achieve its goals using weapons"^^xsd:string ;
    rdfs:subClassOf wikidata:Q43229 .

wikidata:Q180684 rdfs:label "conflict"^^xsd:string ;
    rdfs:comment "friction, disagreement, or discord within a group or between different groups"^^xsd:string .

wikidata:Q18127 rdfs:label "record label"^^xsd:string ;
    rdfs:comment "brand and trademark associated with the marketing of music recordings and music videos"^^xsd:string ;
    rdfs:subClassOf wikidata:Q431289 .

wikidata:Q18608583 rdfs:label "recurring sporting event"^^xsd:string ;
    rdfs:comment "sports festival event scheduled to recur within a decided interval"^^xsd:string ;
    rdfs:subClassOf wikidata:Q15275719 .

wikidata:Q2057971 rdfs:label "health problem"^^xsd:string ;
    rdfs:comment "condition negatively affecting the health of an organism"^^xsd:string ;
    rdfs:subClassOf wikidata:Q639907,
        wikidata:Q7189713 .

wikidata:Q2095 rdfs:label "food"^^xsd:string ;
    rdfs:comment "any substance consumed to provide nutritional support for the body; form of energy stored in chemical"^^xsd:string .

wikidata:Q21191270 rdfs:label "television series episode"^^xsd:string ;
    rdfs:comment "single installment of a television series"^^xsd:string ;
    rdfs:subClassOf wikidata:Q15416,
        wikidata:Q1983062,
        wikidata:Q2431196 .

wikidata:Q21451536 rdfs:label "fictional office, position, or title"^^xsd:string ;
    rdfs:comment "fictional political, administrative or civil servant position"^^xsd:string ;
    rdfs:subClassOf wikidata:Q14897293 .

wikidata:Q219715 rdfs:label "restriction enzyme"^^xsd:string ;
    rdfs:comment "class of enzymes that cleaves DNA into fragments at or near specific recognition sites within the molecule known as restriction sites"^^xsd:string .

wikidata:Q2239243 rdfs:label "mythical creature"^^xsd:string ;
    rdfs:comment "supernatural animal, generally a hybrid, sometimes part human, whose existence cannot be proven, described in legends, myths, fables, folklore"^^xsd:string ;
    rdfs:subClassOf wikidata:Q24334685,
        wikidata:Q95074 .

wikidata:Q235557 rdfs:label "file format"^^xsd:string ;
    rdfs:comment "formalized structure of information stored on a computer"^^xsd:string .

wikidata:Q24856 rdfs:label "film series"^^xsd:string ;
    rdfs:comment "collection of related films in succession"^^xsd:string ;
    rdfs:subClassOf wikidata:Q2431196,
        wikidata:Q7725310,
        wikidata:Q838948 .

wikidata:Q27968055 rdfs:label "recurrent event edition"^^xsd:string ;
    rdfs:comment "edition in a specific year of an event held regularly, e.g. every year"^^xsd:string ;
    rdfs:subClassOf wikidata:Q1656682 .

wikidata:Q2858615 rdfs:label "electronic machine"^^xsd:string ;
    rdfs:comment "electric device where the main functionality is provided by electronic circuits"^^xsd:string ;
    rdfs:subClassOf wikidata:Q11019 .

wikidata:Q34770 rdfs:label "language"^^xsd:string ;
    rdfs:comment "particular system of communication, usually named for the region or peoples that use it"^^xsd:string ;
    rdfs:subClassOf wikidata:Q17376908 .

wikidata:Q35127 rdfs:label "website"^^xsd:string ;
    rdfs:comment "set of related web pages served from a single web domain"^^xsd:string ;
    rdfs:subClassOf wikidata:Q1714118 .

wikidata:Q431289 rdfs:label "brand"^^xsd:string ;
    rdfs:comment "identification for a good or service"^^xsd:string ;
    rdfs:subClassOf wikidata:Q167270 .

wikidata:Q44613 rdfs:label "monastery"^^xsd:string ;
    rdfs:comment "complex of buildings comprising the domestic quarters and workplace(s) of monks or nuns"^^xsd:string ;
    rdfs:subClassOf wikidata:Q1370598,
        wikidata:Q43229 .

wikidata:Q548662 rdfs:label "transport stop"^^xsd:string ;
    rdfs:comment "designated place of stopping a vehicle of public transportation for the purpose of allowing passengers to embark or disembark"^^xsd:string ;
    rdfs:subClassOf wikidata:Q228332,
        wikidata:Q376799 .

wikidata:Q7187 rdfs:label "gene"^^xsd:string ;
    rdfs:comment "basic physical and functional unit of heredity"^^xsd:string .

wikidata:Q7188 rdfs:label "government"^^xsd:string ;
    rdfs:comment "system or group of people governing an organized community, often a state"^^xsd:string .

wikidata:Q7189713 rdfs:label "physiological condition"^^xsd:string ;
    rdfs:comment "conditions of the external or internal milieu that may occur in nature for that organism"^^xsd:string .

wikidata:Q728937 rdfs:label "railway line"^^xsd:string ;
    rdfs:comment "constructional unit in rail transport, the route or way of rail tracks between defined locations"^^xsd:string ;
    rdfs:subClassOf wikidata:Q1311670,
        wikidata:Q618123,
        wikidata:Q83620 .

wikidata:Q75855169 rdfs:label "hypothetical person"^^xsd:string ;
    rdfs:comment "a human being whose existence is not directly attested, but is deduced by other evidence"^^xsd:string ;
    rdfs:subClassOf wikidata:Q18706315,
        wikidata:Q215627 .

wikidata:Q7725634 rdfs:label "literary work"^^xsd:string ;
    rdfs:comment "creative work by a writer created with aesthetic, academic or recreative purposes"^^xsd:string ;
    rdfs:subClassOf wikidata:Q17537576,
        wikidata:Q47461344 .

wikidata:Q820655 rdfs:label "legislative act"^^xsd:string ;
    rdfs:comment "formal written document that creates law, including acts, executive orders, and by-laws"^^xsd:string .

wikidata:P2283 rdfs:label "uses"^^xsd:string ;
    rdfs:comment "item or concept used by the subject or in the operation (see also instrument [P1303] and armament [P520])"^^xsd:string .

wikidata:Q11028 rdfs:label "information"^^xsd:string ;
    rdfs:comment "that which informs; the answer to a question of some kind; that from which data and knowledge can be derived"^^xsd:string ;
    rdfs:subClassOf wikidata:Q7184903 .

wikidata:Q11862829 rdfs:label "academic discipline"^^xsd:string ;
    rdfs:comment "academic field of study or profession"^^xsd:string ;
    rdfs:subClassOf wikidata:Q1047113 .

wikidata:Q12047392 rdfs:label "legal form"^^xsd:string ;
    rdfs:comment "type of legal entity within certain legal system"^^xsd:string .

wikidata:Q121359 rdfs:label "infrastructure"^^xsd:string ;
    rdfs:comment "fundamental facilities and systems serving a country, city, or other areas"^^xsd:string ;
    rdfs:subClassOf wikidata:Q28877 .

wikidata:Q12139612 rdfs:label "list"^^xsd:string ;
    rdfs:comment "ordered listing of all items in a collection"^^xsd:string ;
    rdfs:subClassOf wikidata:Q11028 .

wikidata:Q14136353 rdfs:label "fictional event"^^xsd:string ;
    rdfs:comment "happening which occur in a fiction"^^xsd:string ;
    rdfs:subClassOf wikidata:Q14897293 .

wikidata:Q15275719 rdfs:label "recurring event"^^xsd:string ;
    rdfs:comment "event recurring at an interval"^^xsd:string ;
    rdfs:subClassOf wikidata:Q1656682 .

wikidata:Q16970 rdfs:label "church building"^^xsd:string ;
    rdfs:comment "building constructed for Christian worship"^^xsd:string ;
    rdfs:subClassOf wikidata:Q1370598 .

wikidata:Q216353 rdfs:label "title"^^xsd:string ;
    rdfs:comment "prefix or suffix added to someone's name in certain contexts"^^xsd:string ;
    rdfs:subClassOf wikidata:Q618779 .

wikidata:Q2352616 rdfs:label "catalogue"^^xsd:string ;
    rdfs:comment "work comprising an ordered list of items"^^xsd:string ;
    rdfs:subClassOf wikidata:Q1172284,
        wikidata:Q12139612,
        wikidata:Q2668072,
        wikidata:Q47461344 .

wikidata:Q27020041 rdfs:label "sports season"^^xsd:string ;
    rdfs:comment "season of a sports league or competition, generally a specific one year period"^^xsd:string ;
    rdfs:subClassOf wikidata:Q13406554,
        wikidata:Q18608583,
        wikidata:Q23807345 .

wikidata:Q29048322 rdfs:label "vehicle model"^^xsd:string ;
    rdfs:comment "specific vehicle design of which all instances are produced to identical specifications"^^xsd:string ;
    rdfs:subClassOf wikidata:Q10929058,
        wikidata:Q7184903 .

wikidata:Q294440 rdfs:label "public space"^^xsd:string ;
    rdfs:comment "places for public use"^^xsd:string ;
    rdfs:subClassOf wikidata:Q27096213 .

wikidata:Q327333 rdfs:label "government agency"^^xsd:string ;
    rdfs:comment "organization in the machinery of government responsible for specific functions"^^xsd:string ;
    rdfs:subClassOf wikidata:Q783794 .

wikidata:Q33506 rdfs:label "museum"^^xsd:string ;
    rdfs:comment "institution that holds artifacts and other objects of scientific, artistic, cultural, historical, or other importance"^^xsd:string ;
    rdfs:subClassOf wikidata:Q1030034,
        wikidata:Q17334923,
        wikidata:Q294440,
        wikidata:Q570116 .

wikidata:Q7210356 rdfs:label "political organisation"^^xsd:string ;
    rdfs:comment "group involved in political activities"^^xsd:string ;
    rdfs:subClassOf wikidata:Q43229 .

wikidata:Q7239 rdfs:label "organism"^^xsd:string ;
    rdfs:comment "any contiguous alive physical entity; entity or being that is living; an individual living thing, such as one animal, plant, fungus, or bacterium"^^xsd:string ;
    rdfs:subClassOf wikidata:Q27043950 .

wikidata:Q783794 rdfs:label "company"^^xsd:string ;
    rdfs:comment "legal entity representing an association of people, whether natural, legal or a mixture of both, with a specific objective"^^xsd:string ;
    rdfs:subClassOf wikidata:Q3778211,
        wikidata:Q43229 .

wikidata:Q80071 rdfs:label "symbol"^^xsd:string ;
    rdfs:comment "something that represents an idea, a process, or a physical entity"^^xsd:string ;
    rdfs:subClassOf wikidata:Q3695082,
        wikidata:Q478798 .

wikidata:P527 rdfs:label "has part"^^xsd:string ;
    rdf:first <http://www.semanticweb.org/ontologies/Wikidata#_:y12> ;
    rdfs:comment "part of this subject; inverse property of \"part of\" (P361). See also \"has parts of the class\" (P2670)."^^xsd:string .

wikidata:P710 rdfs:label "participant"^^xsd:string ;
    rdfs:comment "person, group of people or organization (object) that actively takes/took part in an event or process (subject).  Preferably qualify with \"object has role\" (P3831). Use P1923 for participants that are teams."^^xsd:string ;
    rdfs:domain wikidata:Q1190554,
        wikidata:Q124964,
        wikidata:Q13406554,
        wikidata:Q14136353,
        wikidata:Q16334295,
        wikidata:Q170584,
        wikidata:Q178651,
        wikidata:Q24336466,
        wikidata:Q321839,
        wikidata:Q3249551,
        wikidata:Q4539,
        wikidata:Q5,
        wikidata:Q500834,
        wikidata:Q54933017,
        wikidata:Q58778 ;
    rdfs:subPropertyOf wikidata:P3342 .

wikidata:Q1002697 rdfs:label "periodical"^^xsd:string ;
    rdfs:comment "serial publication that appears in a new edition on a regular schedule"^^xsd:string ;
    rdfs:subClassOf wikidata:Q15621286,
        wikidata:Q2217301,
        wikidata:Q340169,
        wikidata:Q732577 .

wikidata:Q11042 rdfs:label "culture"^^xsd:string ;
    rdfs:comment "society's way of life within anthropology"^^xsd:string ;
    rdfs:subClassOf wikidata:Q2515887,
        wikidata:Q3769299 .

wikidata:Q12973014 rdfs:label "sports team"^^xsd:string ;
    rdfs:comment "individual team that plays sports"^^xsd:string ;
    rdfs:subClassOf wikidata:Q327245,
        wikidata:Q4438121 .

wikidata:Q1492823 rdfs:label "ecclesiastical district"^^xsd:string ;
    rdfs:comment ""^^xsd:string ;
    rdfs:subClassOf wikidata:Q51041800 .

wikidata:Q1496967 rdfs:label "territorial entity"^^xsd:string ;
    rdfs:comment "entity that covers a part of the Earth's surface with specified borders"^^xsd:string ;
    rdfs:subClassOf wikidata:Q82794 .

wikidata:Q1530022 rdfs:label "religious organization"^^xsd:string ;
    rdfs:comment "organization that supports the practice of a religion"^^xsd:string ;
    rdfs:subClassOf wikidata:Q43229 .

wikidata:Q15401930 rdfs:label "product"^^xsd:string ;
    rdfs:comment "result of some kind of work or effort"^^xsd:string ;
    rdfs:subClassOf wikidata:Q16686448 .

wikidata:Q15706911 rdfs:label "fictional object"^^xsd:string ;
    rdfs:comment "object appearing only in fictional stories"^^xsd:string ;
    rdfs:subClassOf wikidata:Q14897293 .

wikidata:Q15831598 rdfs:label "fictional astronomical object"^^xsd:string ;
    rdfs:comment "astronomical object that exists only in fiction and not in reality"^^xsd:string ;
    rdfs:subClassOf wikidata:Q3895768 .

wikidata:Q176799 rdfs:label "military unit"^^xsd:string ;
    rdfs:comment "organization formed as part of an armed force"^^xsd:string ;
    rdfs:subClassOf wikidata:Q17149090 .

wikidata:Q177634 rdfs:label "community"^^xsd:string ;
    rdfs:comment "social unit of human organisms who share common values"^^xsd:string ;
    rdfs:subClassOf wikidata:Q16334295,
        wikidata:Q43229,
        wikidata:Q874405 .

wikidata:Q2088357 rdfs:label "musical ensemble"^^xsd:string ;
    rdfs:comment "group of people who perform instrumental and/or vocal music, with the ensemble typically known by a distinct name"^^xsd:string ;
    rdfs:subClassOf wikidata:Q16334295 .

wikidata:Q20926517 rdfs:label "religious administrative territorial entity"^^xsd:string ;
    rdfs:comment "religious administration over a geographic area"^^xsd:string ;
    rdfs:subClassOf wikidata:Q15642541,
        wikidata:Q51041800,
        wikidata:Q56061 .

wikidata:Q340169 rdfs:label "communication medium"^^xsd:string ;
    rdfs:comment "storage and delivering agent of information or data"^^xsd:string .

wikidata:Q34442 rdfs:label "road"^^xsd:string ;
    rdfs:comment "way on land between two places"^^xsd:string ;
    rdfs:subClassOf wikidata:Q376799,
        wikidata:Q83620 .

wikidata:Q376799 rdfs:label "transport infrastructure"^^xsd:string ;
    rdfs:comment "fixed installations that allow vehicles to operate"^^xsd:string ;
    rdfs:subClassOf wikidata:Q121359,
        wikidata:Q27096235,
        wikidata:Q618123 .

wikidata:Q43099500 rdfs:label "performing arts production"^^xsd:string ;
    rdfs:comment "production of the performing arts, consisting of a run of quasi-identical performances of the same performance work"^^xsd:string ;
    rdfs:subClassOf wikidata:Q1656682,
        wikidata:Q838948 .

wikidata:Q4406616 rdfs:label "concrete object"^^xsd:string ;
    rdfs:comment "object with a physical referent"^^xsd:string ;
    rdfs:subClassOf wikidata:Q488383 .

wikidata:Q47461344 rdfs:label "written work"^^xsd:string ;
    rdfs:comment "any creative work expressed in writing like: inscriptions, manuscripts, documents or maps"^^xsd:string ;
    rdfs:subClassOf wikidata:Q17537576,
        wikidata:Q386724 .

wikidata:Q7184903 rdfs:label "abstract object"^^xsd:string ;
    rdfs:comment "object with no physical referents"^^xsd:string ;
    rdfs:subClassOf wikidata:Q488383 .

wikidata:Q8205328 rdfs:label "artificial physical object"^^xsd:string ;
    rdfs:comment "physical object made or shaped by human hand"^^xsd:string ;
    rdfs:subClassOf wikidata:Q16686448,
        wikidata:Q223557 .

wikidata:Q841654 rdfs:label "competition"^^xsd:string ;
    rdfs:comment "contest for a prize or award"^^xsd:string ;
    rdfs:subClassOf wikidata:Q1656682 .

wikidata:Q874405 rdfs:label "social group"^^xsd:string ;
    rdfs:comment "two or more humans who interact with one another"^^xsd:string ;
    rdfs:subClassOf wikidata:Q16334295,
        wikidata:Q58778 .

wikidata:P7153 rdfs:label "significant place"^^xsd:string ;
    rdfs:comment "significant or notable places associated with the subject"^^xsd:string .

wikidata:Q1067164 rdfs:label "service"^^xsd:string ;
    rdfs:comment "regular operation of a particular path for a type of transportation"^^xsd:string ;
    rdfs:subClassOf wikidata:Q1322323 .

wikidata:Q1145276 rdfs:label "fictional country"^^xsd:string ;
    rdfs:comment "country that exists only in fiction and not in reality"^^xsd:string .

wikidata:Q1207505 rdfs:label "quality"^^xsd:string ;
    rdfs:comment "characteristic trait that differentiates an entity"^^xsd:string .

wikidata:Q15324 rdfs:label "body of water"^^xsd:string ;
    rdfs:comment "any significant accumulation of water, generally on a planet's surface"^^xsd:string ;
    rdfs:subClassOf wikidata:Q82794 .

wikidata:Q15621286 rdfs:label "intellectual work"^^xsd:string ;
    rdfs:comment "work created through human thought and perception, including creative work"^^xsd:string ;
    rdfs:subClassOf wikidata:Q386724 .

wikidata:Q16887380 rdfs:label "group"^^xsd:string ;
    rdfs:comment "well-defined collection of discrete entities who choose or are assigned to be part of a collective whole"^^xsd:string .

wikidata:Q24334893 rdfs:label "mythical place"^^xsd:string ;
    rdfs:comment "place that exists only in myth and not in reality"^^xsd:string ;
    rdfs:subClassOf wikidata:Q24334685 .

wikidata:Q28877 rdfs:label "goods"^^xsd:string ;
    rdfs:comment "tangible and intangible thing, except labor tied services, that satisfies human wants and provides utility"^^xsd:string ;
    rdfs:subClassOf wikidata:Q488383 .

wikidata:Q39546 rdfs:label "tool"^^xsd:string ;
    rdfs:comment "physical item that can be used to achieve a goal"^^xsd:string ;
    rdfs:subClassOf wikidata:Q16798631,
        wikidata:Q2424752 .

wikidata:Q4167836 rdfs:label "Wikimedia category"^^xsd:string ;
    rdfs:comment "use with 'instance of' (P31) for Wikimedia category"^^xsd:string ;
    rdfs:subClassOf wikidata:Q12139612 .

wikidata:Q4438121 rdfs:label "sports organization"^^xsd:string ;
    rdfs:comment "organization involved primarily in sports"^^xsd:string ;
    rdfs:subClassOf wikidata:Q43229 .

wikidata:Q488383 rdfs:label "object"^^xsd:string ;
    rdfs:comment "anything that we can think or talk about; a thing that is observed by a subject"^^xsd:string ;
    rdfs:subClassOf wikidata:Q35120 .

wikidata:Q51041800 rdfs:label "religious administrative entity"^^xsd:string ;
    rdfs:comment "entity with control over a religion or part of a religion"^^xsd:string ;
    rdfs:subClassOf wikidata:Q1530022,
        wikidata:Q5982983 .

wikidata:Q6256 rdfs:label "country"^^xsd:string ;
    rdfs:comment "distinct region in geography; a broad term that can include political divisions or regions associated with distinct political characteristics"^^xsd:string ;
    rdfs:subClassOf wikidata:Q1048835 .

wikidata:Q838948 rdfs:label "work of art"^^xsd:string ;
    rdfs:comment "aesthetic physical item or artistic creation"^^xsd:string ;
    rdfs:subClassOf wikidata:Q17537576,
        wikidata:Q18593264,
        wikidata:Q28877 .

wikidata:Q8513 rdfs:label "database"^^xsd:string ;
    rdfs:comment "organized collection of data"^^xsd:string ;
    rdfs:subClassOf wikidata:Q15401930,
        wikidata:Q386724 .

wikidata:Q1047113 rdfs:label "specialty"^^xsd:string ;
    rdfs:comment "field limited to a specific area of ​​knowledge; specialization in an occupation or branch of learning; a specific use"^^xsd:string ;
    rdfs:subClassOf wikidata:Q9081 .

wikidata:Q10929058 rdfs:label "model"^^xsd:string ;
    rdfs:comment "class of manufactured objects of similar design sold under a specific brand"^^xsd:string ;
    rdfs:subClassOf wikidata:Q22811462,
        wikidata:Q386724 .

wikidata:Q151885 rdfs:label "concept"^^xsd:string ;
    rdfs:comment "semantic unit understood in different ways, e.g. as mental representation, ability or abstract object"^^xsd:string ;
    rdfs:subClassOf wikidata:Q1347367,
        wikidata:Q7184903 .

wikidata:Q18593264 rdfs:label "item of collection or exhibition"^^xsd:string ;
    rdfs:comment "defines an item, such as an object or document, that is a member of a collection or part of a repository"^^xsd:string ;
    rdfs:subClassOf wikidata:Q488383 .

wikidata:Q2031291 rdfs:label "release"^^xsd:string ;
    rdfs:comment "publication of a musical artist's creative output"^^xsd:string ;
    rdfs:subClassOf wikidata:Q2188189,
        wikidata:Q732577 .

wikidata:Q215380 rdfs:label "musical group"^^xsd:string ;
    rdfs:comment "musical ensemble which performs music"^^xsd:string ;
    rdfs:subClassOf wikidata:Q2088357 .

wikidata:Q241317 rdfs:label "computing platform"^^xsd:string ;
    rdfs:comment "hardware architecture and/or software framework"^^xsd:string .

wikidata:Q26401003 rdfs:label "individual animal"^^xsd:string ;
    rdfs:comment "class for particular creatures"^^xsd:string ;
    rdfs:subClassOf wikidata:Q729 .

wikidata:Q3249551 rdfs:label "process"^^xsd:string ;
    rdfs:comment "series of events which occur over an extended period of time"^^xsd:string ;
    rdfs:subClassOf wikidata:Q1190554,
        wikidata:Q20937557 .

wikidata:Q355304 rdfs:label "watercourse"^^xsd:string ;
    rdfs:comment "channel that a flowing body of water follows"^^xsd:string .

wikidata:Q42889 rdfs:label "vehicle"^^xsd:string ;
    rdfs:comment "mobile machine that transports people, animals or cargo"^^xsd:string ;
    rdfs:subClassOf wikidata:Q11019 .

wikidata:Q7275 rdfs:label "state"^^xsd:string ;
    rdfs:comment "organised community living under a system of government; either a sovereign state, constituent state, or federated state"^^xsd:string ;
    rdfs:subClassOf wikidata:Q1048835,
        wikidata:Q155076,
        wikidata:Q177634,
        wikidata:Q43229,
        wikidata:Q56061 .

wikidata:Q7406919 rdfs:label "service"^^xsd:string ;
    rdfs:comment "activity that directly satisfies wants without producing a lasting asset"^^xsd:string .

wikidata:Q8436 rdfs:label "family"^^xsd:string ;
    rdfs:comment "group of people affiliated by consanguinity, affinity, or co-residence"^^xsd:string ;
    rdfs:subClassOf wikidata:Q1313923,
        wikidata:Q16334295,
        wikidata:Q874405 .

wikidata:Q12737077 rdfs:label "occupation"^^xsd:string ;
    rdfs:comment "label applied to a person based on an activity they participate in"^^xsd:string ;
    rdfs:subClassOf wikidata:Q61788060 .

wikidata:Q17376908 rdfs:label "languoid"^^xsd:string ;
    rdfs:comment "language, variety of a language, or group of languages"^^xsd:string ;
    rdfs:subClassOf wikidata:Q7184903 .

wikidata:Q17489659 rdfs:label "group of works"^^xsd:string ;
    rdfs:comment "any set of works"^^xsd:string ;
    rdfs:subClassOf wikidata:Q16887380,
        wikidata:Q17537576 .

wikidata:Q20937557 rdfs:label "series"^^xsd:string ;
    rdfs:comment "ordered set of similar objects"^^xsd:string ;
    rdfs:subClassOf wikidata:Q16887380 .

wikidata:Q49773 rdfs:label "social movement"^^xsd:string ;
    rdfs:comment "type of group action"^^xsd:string ;
    rdfs:subClassOf wikidata:Q16334295,
        wikidata:Q3533467 .

wikidata:Q1048835 rdfs:label "political territorial entity"^^xsd:string ;
    rdfs:comment "a region accepted to be in the jurisdiction of a particular government entity"^^xsd:string ;
    rdfs:subClassOf wikidata:Q15642541 .

wikidata:Q1151067 rdfs:label "rule"^^xsd:string ;
    rdfs:comment "prescription, including laws, regulations, instructions, guidelines, and social conventions; determinate method for performing any operation"^^xsd:string ;
    rdfs:subClassOf wikidata:Q16686448,
        wikidata:Q2684591 .

wikidata:Q223557 rdfs:label "physical object"^^xsd:string ;
    rdfs:comment "singular aggregation of substance(s) such as matter or radiation, with overall properties such as mass, position or momentum"^^xsd:string ;
    rdfs:subClassOf wikidata:Q4406616 .

wikidata:Q23649976 rdfs:label "content rating category"^^xsd:string ;
    rdfs:comment "single content rating in a rating system"^^xsd:string .

wikidata:Q27096235 rdfs:label "artificial geographic entity"^^xsd:string ;
    rdfs:comment "elements of the ground or the underground that have been greatly modified by human being (roads, houses, ...)"^^xsd:string ;
    rdfs:subClassOf wikidata:Q27096213,
        wikidata:Q8205328 .

wikidata:Q271669 rdfs:label "landform"^^xsd:string ;
    rdfs:comment "geomorphological unit in the Earth sciences"^^xsd:string .

wikidata:Q41176 rdfs:label "building"^^xsd:string ;
    rdfs:comment "structure, typically with a roof and walls, standing more or less permanently in one place"^^xsd:string ;
    rdfs:subClassOf wikidata:Q13226383,
        wikidata:Q811979 .

wikidata:Q486972 rdfs:label "human settlement"^^xsd:string ;
    rdfs:comment "community of any size, in which people live"^^xsd:string ;
    rdfs:subClassOf wikidata:Q177634,
        wikidata:Q2221906,
        wikidata:Q27096235,
        wikidata:Q82794 .

wikidata:P276 rdfs:label "location"^^xsd:string ;
    rdfs:comment "location of the object, structure or event. In the case of an administrative entity as containing item use P131 for statistical entities P8138. In the case of a geographic entity use P706. Use P7153 for locations associated with the object."^^xsd:string .

wikidata:Q16521 rdfs:label "taxon"^^xsd:string ;
    rdfs:comment "group of one or more organism(s), which a taxonomist adjudges to be a unit"^^xsd:string .

wikidata:Q2188189 rdfs:label "musical work"^^xsd:string ;
    rdfs:comment "musical work of art"^^xsd:string ;
    rdfs:subClassOf wikidata:Q838948 .

wikidata:Q27096213 rdfs:label "geographic entity"^^xsd:string ;
    rdfs:comment "place or entity that could be a place"^^xsd:string .

wikidata:Q41710 rdfs:label "ethnic group"^^xsd:string ;
    rdfs:comment "socially defined category of people who identify with each other"^^xsd:string ;
    rdfs:subClassOf wikidata:Q16334295 .

wikidata:Q4830453 rdfs:label "business"^^xsd:string ;
    rdfs:comment "organization involved in commercial, industrial, or professional activity"^^xsd:string ;
    rdfs:subClassOf wikidata:Q43229 .

wikidata:Q83620 rdfs:label "thoroughfare"^^xsd:string ;
    rdfs:comment "transportation route connecting one location to another"^^xsd:string ;
    rdfs:subClassOf wikidata:Q27096235,
        wikidata:Q294440,
        wikidata:Q376799 .

wikidata:Q13406554 rdfs:label "sports competition"^^xsd:string ;
    rdfs:comment "event, during which one or more sporting events are held"^^xsd:string ;
    rdfs:subClassOf wikidata:Q1656682 .

wikidata:Q24334685 rdfs:label "mythical entity"^^xsd:string ;
    rdfs:comment "entity that only exists in myth"^^xsd:string ;
    rdfs:subClassOf wikidata:Q18706315 .

wikidata:Q6999 rdfs:label "astronomical object"^^xsd:string ;
    rdfs:comment "physical body of astronomically-significant size,  mass, or role, naturally occurring in a universe"^^xsd:string ;
    rdfs:subClassOf wikidata:Q17334923,
        wikidata:Q223557 .

wikidata:Q15642541 rdfs:label "human-geographic territorial entity"^^xsd:string ;
    rdfs:comment "territorial entity of which the borders are determined by physiographic and human features"^^xsd:string ;
    rdfs:subClassOf wikidata:Q1496967,
        wikidata:Q16686448 .

wikidata:Q17334923 rdfs:label "location"^^xsd:string ;
    rdfs:comment "location of physical or non-physical object in space"^^xsd:string ;
    rdfs:subClassOf wikidata:Q27096213 .

wikidata:Q178885 rdfs:label "deity"^^xsd:string ;
    rdfs:comment "natural or supernatural god or goddess, divine being"^^xsd:string ;
    rdfs:subClassOf wikidata:Q15619164,
        wikidata:Q4271324 .

wikidata:Q2668072 rdfs:label "collection"^^xsd:string ;
    rdfs:comment "set of purposefully gathered physical or digital objects with some common characteristics"^^xsd:string ;
    rdfs:subClassOf wikidata:Q16686448,
        wikidata:Q16887380,
        wikidata:Q223557,
        wikidata:Q386724 .

wikidata:Q618779 rdfs:label "award"^^xsd:string ;
    rdfs:comment "something given to a person or a group of people to recognize their merit or excellence"^^xsd:string .

wikidata:Q732577 rdfs:label "publication"^^xsd:string ;
    rdfs:comment "content made available to the general public"^^xsd:string ;
    rdfs:subClassOf wikidata:Q386724 .

wikidata:Q15632617 rdfs:label "fictional human"^^xsd:string ;
    rdfs:comment "human being that only exists in fictional works"^^xsd:string ;
    rdfs:subClassOf wikidata:Q28020127,
        wikidata:Q95074 .

wikidata:Q16686448 rdfs:label "artificial entity"^^xsd:string ;
    rdfs:comment "anything created by humans (either material or mental)"^^xsd:string ;
    rdfs:subClassOf wikidata:Q488383 .

wikidata:Q170584 rdfs:label "project"^^xsd:string ;
    rdfs:comment "collaborative enterprise, frequently involving research or design, that is carefully planned to achieve a particular aim"^^xsd:string ;
    rdfs:subClassOf wikidata:Q1914636,
        wikidata:Q43229 .

wikidata:Q17537576 rdfs:label "creative work"^^xsd:string ;
    rdfs:comment "distinct artistic creation such as artwork, literature, music, and paintings"^^xsd:string ;
    rdfs:subClassOf wikidata:Q15621286 .

wikidata:Q1914636 rdfs:label "activity"^^xsd:string ;
    rdfs:comment "event; actions that result in changes of state"^^xsd:string ;
    rdfs:subClassOf wikidata:Q20937557 .

wikidata:Q21070568 rdfs:label "human who may be fictional"^^xsd:string ;
    rdfs:comment "human who may be real or may be based on a real human but who some say is fictional"^^xsd:string ;
    rdfs:subClassOf wikidata:Q21070598,
        wikidata:Q215627,
        wikidata:Q5 .

wikidata:Q2424752 rdfs:label "product"^^xsd:string ;
    rdfs:comment "result of work that can be offered to a market"^^xsd:string ;
    rdfs:subClassOf wikidata:Q15401930,
        wikidata:Q28877 .

wikidata:Q58778 rdfs:label "system"^^xsd:string ;
    rdfs:comment "set of interacting or interdependent components"^^xsd:string ;
    rdfs:subClassOf wikidata:Q6671777 .

wikidata:Q15416 rdfs:label "television program"^^xsd:string ;
    rdfs:comment "segment of audiovisual content intended for broadcast on television"^^xsd:string ;
    rdfs:subClassOf wikidata:Q11578774,
        wikidata:Q2431196,
        wikidata:Q7725310 .

wikidata:Q3331189 rdfs:label "version, edition, or translation"^^xsd:string ;
    rdfs:comment "specific version of a work, resulting from its edition, adaptation, or translation; set of substantially similar copies of a work"^^xsd:string ;
    rdfs:subClassOf wikidata:Q386724,
        wikidata:Q732577 .

wikidata:Q729 rdfs:label "animal"^^xsd:string ;
    rdfs:comment "kingdom of multicellular eukaryotic organisms"^^xsd:string ;
    rdfs:subClassOf wikidata:Q7239 .

wikidata:Q2431196 rdfs:label "audiovisual work"^^xsd:string ;
    rdfs:comment "creative work possessing both a sound and a visual component"^^xsd:string ;
    rdfs:subClassOf wikidata:Q17537576 .

wikidata:P3342 rdfs:label "significant person"^^xsd:string ;
    rdfs:comment "person linked to the item in any possible way"^^xsd:string ;
    rdfs:range wikidata:Q215627,
        wikidata:Q4271324,
        wikidata:Q95074 .

wikidata:P361 rdfs:label "part of"^^xsd:string ;
    rdfs:comment "object of which the subject is a part (if this subject is already part of object A which is a part of object B, then please only make the subject part of object A). Inverse property of \"has part\" (P527, see also \"has parts of the class\" (P2670))."^^xsd:string .

wikidata:Q7725310 rdfs:label "series of creative works"^^xsd:string ;
    rdfs:comment "ordered set of creative works"^^xsd:string ;
    rdfs:subClassOf wikidata:Q17489659,
        wikidata:Q20937557 .

wikidata:Q7889 rdfs:label "video game"^^xsd:string ;
    rdfs:comment "electronic game that involves interaction with a user interface to generate visual feedback on a video device such as a TV screen or computer monitor"^^xsd:string ;
    rdfs:subClassOf wikidata:Q166142,
        wikidata:Q17537576,
        wikidata:Q2431196 .

wikidata:Q13002315 rdfs:label "legendary figure"^^xsd:string ;
    rdfs:comment "named person or animal that appears in legends that have some claim to be historical"^^xsd:string ;
    rdfs:subClassOf wikidata:Q21070598 .

wikidata:Q7397 rdfs:label "software"^^xsd:string ;
    rdfs:comment "non-tangible executable component of a computer"^^xsd:string ;
    rdfs:subClassOf wikidata:Q17537576,
        wikidata:Q2424752,
        wikidata:Q47461344 .

wikidata:Q4271324 rdfs:label "mythical character"^^xsd:string ;
    rdfs:comment "character from mythology"^^xsd:string ;
    rdfs:subClassOf wikidata:Q15619164,
        wikidata:Q21070598,
        wikidata:Q24334685 .

wikidata:Q14897293 rdfs:label "fictional entity"^^xsd:string ;
    rdfs:comment "entity that only exists in a work of fiction"^^xsd:string ;
    rdfs:subClassOf wikidata:Q17537576 .

wikidata:Q13226383 rdfs:label "facility"^^xsd:string ;
    rdfs:comment "place for doing something"^^xsd:string ;
    rdfs:subClassOf wikidata:Q2221906,
        wikidata:Q27096235,
        wikidata:Q618123 .

wikidata:Q4164871 rdfs:label "position"^^xsd:string ;
    rdfs:comment "social role with a set of powers and responsibilities within a private or public organization or the state"^^xsd:string ;
    rdfs:subClassOf wikidata:Q16686448,
        wikidata:Q214339 .

wikidata:Q49848 rdfs:label "document"^^xsd:string ;
    rdfs:comment "preserved information"^^xsd:string ;
    rdfs:subClassOf wikidata:Q223557,
        wikidata:Q47461344 .

wikidata:Q811979 rdfs:label "architectural structure"^^xsd:string ;
    rdfs:comment "human-designed and -made structure"^^xsd:string ;
    rdfs:subClassOf wikidata:Q386724,
        wikidata:Q4406616,
        wikidata:Q618123,
        wikidata:Q811430 .

wikidata:Q11424 rdfs:label "film"^^xsd:string ;
    rdfs:comment "audiovisual work"^^xsd:string ;
    rdfs:subClassOf wikidata:Q20937557,
        wikidata:Q2431196 .

wikidata:Q1190554 rdfs:label "occurrence"^^xsd:string ;
    rdfs:comment "occurrence of a fact or object in space-time; instantiation of a property in an object"^^xsd:string ;
    rdfs:subClassOf wikidata:Q26907166 .

wikidata:Q14514600 rdfs:label "group of fictional characters"^^xsd:string ;
    rdfs:comment "set of fictional characters"^^xsd:string ;
    rdfs:subClassOf wikidata:Q14897293,
        wikidata:Q95074 .

wikidata:Q1656682 rdfs:label "event"^^xsd:string ;
    rdfs:comment "temporary and scheduled happening, like a conference, festival or competition"^^xsd:string ;
    rdfs:subClassOf wikidata:Q1190554 .

wikidata:Q82794 rdfs:label "geographic region"^^xsd:string ;
    rdfs:comment "2D or 3D defined space, mainly in terrestrial and astrophysics sciences"^^xsd:string ;
    rdfs:subClassOf wikidata:Q2221906,
        wikidata:Q27096213,
        wikidata:Q618123 .

wikidata:Q3895768 rdfs:label "fictional location"^^xsd:string ;
    rdfs:comment "place that exists only in fiction and not in reality"^^xsd:string ;
    rdfs:subClassOf wikidata:Q14897293 .

wikidata:Q21070598 rdfs:label "narrative entity"^^xsd:string ;
    rdfs:comment "character that may or may not be fictional"^^xsd:string ;
    rdfs:subClassOf wikidata:Q18706315 .

wikidata:Q2221906 rdfs:label "geographic location"^^xsd:string ;
    rdfs:comment "point or an area on the Earth's surface or elsewhere"^^xsd:string ;
    rdfs:subClassOf wikidata:Q17334923 .

wikidata:Q56061 rdfs:label "administrative territorial entity"^^xsd:string ;
    rdfs:comment "territorial entity for administration purposes, with or without its own local government"^^xsd:string ;
    rdfs:subClassOf wikidata:Q15642541 .

wikidata:Q14623646 rdfs:label "fictional organization"^^xsd:string ;
    rdfs:comment "organisation that exists only in fiction"^^xsd:string ;
    rdfs:subClassOf wikidata:Q14514600,
        wikidata:Q14897293 .

wikidata:Q215627 rdfs:label "person"^^xsd:string ;
    rdfs:comment "being that has certain capacities or attributes constituting personhood (avoid use with P31; use Q5 for humans)"^^xsd:string .

wikidata:Q618123 rdfs:label "geographical feature"^^xsd:string ;
    rdfs:comment "point; object that can be uniquely identified with geographical data, may be man-made or naturally-created"^^xsd:string ;
    rdfs:subClassOf wikidata:Q2221906,
        wikidata:Q27096213 .

wikidata:Q386724 rdfs:label "work"^^xsd:string ;
    rdfs:comment "physical or virtual object made by humans"^^xsd:string ;
    rdfs:subClassOf wikidata:Q15401930,
        wikidata:Q16686448 .

wikidata:Q16334295 rdfs:label "group of humans"^^xsd:string ;
    rdfs:comment "any set of human beings"^^xsd:string ;
    rdfs:subClassOf wikidata:Q16334298 .

wikidata:Q95074 rdfs:label "fictional character"^^xsd:string ;
    rdfs:comment "fictional human or non-human character in a narrative work of art"^^xsd:string ;
    rdfs:subClassOf wikidata:Q14897293 .

wikidata:Q43229 rdfs:label "organization"^^xsd:string ;
    rdfs:comment "social entity (not necessarily commercial) uniting people into a structured group managing shared means to meet some needs, or to pursue collective goals"^^xsd:string ;
    rdfs:subClassOf wikidata:Q16334295,
        wikidata:Q6671777 .

wikidata:Q5 rdfs:label "human"^^xsd:string ;
    rdfs:comment "common name of Homo sapiens, unique extant species of the genus Homo"^^xsd:string ;
    rdfs:subClassOf wikidata:Q154954,
        wikidata:Q215627 .

