@prefix nell: <http://www.semanticweb.org/ontologies/NELL#> .
@prefix owl: <http://www.w3.org/2002/07/owl#> .
@prefix rdf: <http://www.w3.org/1999/02/22-rdf-syntax-ns#> .
@prefix rdfs: <http://www.w3.org/2000/01/rdf-schema#> .
@prefix xml: <http://www.w3.org/XML/1998/namespace> .
@prefix xsd: <http://www.w3.org/2001/XMLSchema#> .

nell:academicfieldhasperson rdfs:comment "People trained or active in a given academic field"^^xsd:string ;
    rdfs:domain nell:academicfield ;
    rdfs:range nell:person ;
    rdfs:subPropertyOf nell:relatedto .

nell:academicfieldhassubfield rdfs:comment "Subfields within a given academic field"^^xsd:string ;
    rdfs:domain nell:academicfield ;
    rdfs:range nell:academicfield ;
    rdfs:subPropertyOf nell:academicfieldconcernssubject,
        nell:superpartof .

nell:academicfieldsuchasacademicfield a owl:AsymmetricProperty,
        owl:IrreflexiveProperty ;
    rdfs:comment "Describes a specialization fo an Academic Field"^^xsd:string ;
    rdfs:domain nell:academicfield ;
    rdfs:range nell:academicfield ;
    rdfs:subPropertyOf nell:generalizationof .

nell:academicfieldusedbyeconomicsector rdfs:comment "Academic fields used by economic fields"^^xsd:string ;
    rdfs:domain nell:academicfield ;
    rdfs:range nell:economicsector ;
    rdfs:subPropertyOf nell:relatedto .

nell:academicfieldusedinjobposition rdfs:comment "Academic fields useful for job positions"^^xsd:string ;
    rdfs:domain nell:academicfield ;
    rdfs:range nell:jobposition ;
    rdfs:subPropertyOf nell:relatedto .

nell:academicprogramatuniversity rdfs:comment "this academic program is offered by this university"^^xsd:string ;
    rdfs:domain nell:academicfield ;
    rdfs:range nell:university ;
    rdfs:subPropertyOf nell:relatedto .

nell:actorcanbethesameasathlete rdfs:comment "Describes actors that are the same instances as athlete"^^xsd:string ;
    rdfs:domain nell:actor ;
    rdfs:range nell:athlete ;
    rdfs:subPropertyOf nell:canbethesameas .

nell:actorofprotest rdfs:domain nell:person ;
    rdfs:range nell:protestevent ;
    rdfs:subPropertyOf nell:relatedto .

nell:actorstarredinmovie rdfs:comment "to perform as an actor (in movie) "^^xsd:string ;
    rdfs:domain nell:actor ;
    rdfs:range nell:movie ;
    rdfs:subPropertyOf nell:agentcontributedtocreativework .

nell:actorsuchasactor rdfs:comment "Describes the actor types that are generalizations of specific actors"^^xsd:string ;
    rdfs:domain nell:actor ;
    rdfs:range nell:actor ;
    rdfs:subPropertyOf nell:generalizationof .

nell:actorworkedwithdirector rdfs:comment "Relates the actors and directors that at least once worked together"^^xsd:string ;
    rdfs:domain nell:actor ;
    rdfs:range nell:director ;
    rdfs:subPropertyOf nell:agentcollaborateswithagent .

nell:agentcausedevent rdfs:comment "Companion to agentParticipatedInEvent. Note that one needn't participate in an event in order to be a causal factor."^^xsd:string ;
    rdfs:domain nell:agent ;
    rdfs:range nell:event ;
    rdfs:subPropertyOf nell:agentcreated .

nell:agentcreatedorganization rdfs:comment "The person organization or geopoiltical entity that founded the given organization"^^xsd:string ;
    rdfs:domain nell:person ;
    rdfs:range nell:organization ;
    rdfs:subPropertyOf nell:agentcreated .

nell:agentholdssharesincompany rdfs:comment "Any organization person or geopolitical entity that holds shares (majority or otherwise) of the given company."^^xsd:string ;
    rdfs:domain nell:agent ;
    rdfs:range nell:company ;
    rdfs:subPropertyOf nell:agentcollaborateswithagent .

nell:agentowns rdfs:comment "an agent owns any object animal product company etc."^^xsd:string ;
    rdfs:domain nell:humanagent ;
    rdfs:range nell:everypromotedthing ;
    rdfs:subPropertyOf nell:relatedto .

nell:agentstudiesphysiologicalcondition rdfs:comment "This predicate holds between a HumanAgent and a condition and means that the HumanAgent performs research related to condition."^^xsd:string ;
    rdfs:domain nell:person ;
    rdfs:range nell:physiologicalcondition ;
    rdfs:subPropertyOf nell:relatedto .

nell:agentworkedondrug rdfs:comment "This predicate relates a substance and a HumanAgent who is responsible for it. Responsibility is understoond relatively broadly and includes people or organizations responsible for the substance's discovery or marketing and manufacturing.  Additionally agents that own the rights to the substance are also eligible to participate in this relationship.  Note that the humanAgent category include organizations including universities companies and government agencies."^^xsd:string ;
    rdfs:domain nell:humanagent ;
    rdfs:range nell:drug ;
    rdfs:subPropertyOf nell:agentinvolvedwithitem .

nell:ageofperson rdfs:comment "the age of this person"^^xsd:string ;
    rdfs:domain nell:nonneginteger ;
    rdfs:range nell:person ;
    rdfs:subPropertyOf nell:relatedto .

nell:agriculturalproductcamefromcountry rdfs:comment "Describes the agricultural products that came from a country"^^xsd:string ;
    rdfs:domain nell:agriculturalproduct ;
    rdfs:range nell:country ;
    rdfs:subPropertyOf nell:itemexistsatlocation .

nell:agriculturalproductcanbethesameasvegetable rdfs:comment "Describes two instances that are the same thing in these two different categories"^^xsd:string ;
    rdfs:domain nell:agriculturalproduct ;
    rdfs:range nell:vegetable ;
    rdfs:subPropertyOf nell:canbethesameas .

nell:agriculturalproductcomingfromvertebrate rdfs:comment "Describes the agricultural products that come from a vertebrate"^^xsd:string ;
    rdfs:domain nell:agriculturalproduct ;
    rdfs:range nell:vertebrate ;
    rdfs:subPropertyOf nell:relatedto .

nell:agriculturalproductcontainchemical rdfs:comment "Describes the agricultural products that contain a chemical"^^xsd:string ;
    rdfs:domain nell:agriculturalproduct ;
    rdfs:range nell:chemical ;
    rdfs:subPropertyOf nell:relatedto .

nell:agriculturalproductcookedwithagriculturalproduct a owl:IrreflexiveProperty,
        owl:SymmetricProperty ;
    rdfs:comment "Describes the agricultural products that are usually cooked with another agricultural product"^^xsd:string ;
    rdfs:domain nell:agriculturalproduct ;
    rdfs:range nell:agriculturalproduct ;
    rdfs:subPropertyOf nell:relatedto .

nell:agriculturalproductcutintogeometricshape rdfs:comment "Describes the agricultural products that are usually cut into geometric shapes"^^xsd:string ;
    rdfs:domain nell:agriculturalproduct ;
    rdfs:range nell:geometricshape ;
    rdfs:subPropertyOf nell:relatedto .

nell:agriculturalproductgrowinginstateorprovince rdfs:comment "Describes the agricultural products that are produced in a state or province"^^xsd:string ;
    rdfs:domain nell:agriculturalproduct ;
    rdfs:range nell:stateorprovince ;
    rdfs:subPropertyOf nell:itemexistsatlocation .

nell:agriculturalproductgrowninlandscapefeatures rdfs:comment "Describes the agricultural products that are grown in landscape features"^^xsd:string ;
    rdfs:domain nell:agriculturalproduct ;
    rdfs:range nell:landscapefeatures ;
    rdfs:subPropertyOf nell:relatedto .

nell:agriculturalproductincludingagriculturalproduct a owl:AsymmetricProperty,
        owl:IrreflexiveProperty ;
    rdfs:comment "Describes the agricultural products that are generalizations of other agriculture products"^^xsd:string ;
    rdfs:domain nell:agriculturalproduct ;
    rdfs:range nell:agriculturalproduct ;
    rdfs:subPropertyOf nell:generalizationof .

nell:agriculturalproductproducedbyfarm rdfs:comment "the agricultural products produced by a farm"^^xsd:string ;
    rdfs:domain nell:agriculturalproduct ;
    rdfs:range nell:farm ;
    rdfs:subPropertyOf nell:itemexistsatlocation .

nell:agriculturalproducttoattractinsect rdfs:comment "Describes the agricultural products that attract insects"^^xsd:string ;
    rdfs:domain nell:agriculturalproduct ;
    rdfs:range nell:insect ;
    rdfs:subPropertyOf nell:relatedto .

nell:airportincity a owl:FunctionalProperty ;
    rdfs:comment "The city an airport is located in."^^xsd:string ;
    rdfs:domain nell:airport ;
    rdfs:range nell:city ;
    rdfs:subPropertyOf nell:buildinglocatedincity .

nell:airportsuchasairport rdfs:comment "Describes the airport types that are generalizations of specific aiports"^^xsd:string ;
    rdfs:domain nell:airport ;
    rdfs:range nell:airport ;
    rdfs:subPropertyOf nell:generalizationof .

nell:amphibiansuchasamphibian rdfs:comment "Describes the amphibian types that are generalizations of specific amphibians"^^xsd:string ;
    rdfs:domain nell:amphibian ;
    rdfs:range nell:amphibian ;
    rdfs:subPropertyOf nell:generalizationof .

nell:animaldevelopdisease rdfs:comment "Describes the diseases that can be developed by an animal"^^xsd:string ;
    rdfs:domain nell:animal ;
    rdfs:range nell:disease ;
    rdfs:subPropertyOf nell:relatedto .

nell:animaleatvegetable rdfs:comment "Describes the vegetables eaten by an animal"^^xsd:string ;
    rdfs:domain nell:animal ;
    rdfs:range nell:vegetable ;
    rdfs:subPropertyOf nell:animaleatfood .

nell:animalssuchasmammals rdfs:comment "Describes the animal types that are generalizations of mammals"^^xsd:string ;
    rdfs:domain nell:animal ;
    rdfs:range nell:mammal ;
    rdfs:subPropertyOf nell:generalizationof .

nell:animalsuchasfish rdfs:comment "Describes the fish that are from a specific type of animals"^^xsd:string ;
    rdfs:domain nell:animal ;
    rdfs:range nell:fish ;
    rdfs:subPropertyOf nell:animaltypehasanimal .

nell:animalsuchasinsect rdfs:comment "Describes the insect that are from a specific type of animals"^^xsd:string ;
    rdfs:domain nell:animal ;
    rdfs:range nell:insect ;
    rdfs:subPropertyOf nell:animalsuchasinvertebrate .

nell:animalsuchasmollusk rdfs:comment "Describes the mollusk that are from a specific type of animals"^^xsd:string ;
    rdfs:domain nell:animal ;
    rdfs:range nell:mollusk ;
    rdfs:subPropertyOf nell:animalsuchasinvertebrate .

nell:aquariumincity rdfs:comment "The city an aquarium is located in."^^xsd:string ;
    rdfs:domain nell:aquarium ;
    rdfs:range nell:city ;
    rdfs:subPropertyOf nell:attractionofcity .

nell:aquariumssuchasaquariums rdfs:comment "Describes the specific aquarium types that are generalizations of aquariums"^^xsd:string ;
    rdfs:domain nell:aquarium ;
    rdfs:range nell:aquarium ;
    rdfs:subPropertyOf nell:generalizationof .

nell:arachnidiseatenbybird rdfs:comment "Describes arachnids that are hunted and eaten by this bird"^^xsd:string ;
    rdfs:domain nell:arachnid ;
    rdfs:range nell:bird ;
    rdfs:subPropertyOf nell:animalpreyson .

nell:arachnidssuchasarachnids rdfs:comment "Describes the specific arachnid types that are generalizations of arachnids"^^xsd:string ;
    rdfs:domain nell:arachnid ;
    rdfs:range nell:arachnid ;
    rdfs:subPropertyOf nell:generalizationof .

nell:archaeasuchasarchaea rdfs:comment "Describes the specific archaea types that are generalizations of archaeas"^^xsd:string ;
    rdfs:domain nell:archaea ;
    rdfs:range nell:archaea ;
    rdfs:subPropertyOf nell:generalizationof .

nell:architectssuchasarchitects rdfs:comment "Describes the specific architect types that are generalizations of architects"^^xsd:string ;
    rdfs:domain nell:architect ;
    rdfs:range nell:architect ;
    rdfs:subPropertyOf nell:generalizationof .

nell:arteriessuchasarteries rdfs:comment "Describes the specific artery types that are generalizations of arteries"^^xsd:string ;
    rdfs:domain nell:artery ;
    rdfs:range nell:artery ;
    rdfs:subPropertyOf nell:generalizationof .

nell:arteryarisesfromartery rdfs:comment "Describes the arteries that arises from other arteries"^^xsd:string ;
    rdfs:domain nell:artery ;
    rdfs:range nell:artery ;
    rdfs:subPropertyOf nell:relatedto .

nell:arterycalledartery rdfs:comment "Describes the names an artery can be called"^^xsd:string ;
    rdfs:domain nell:artery ;
    rdfs:range nell:artery ;
    rdfs:subPropertyOf nell:relatedto .

nell:arthropodandotherarthropod a owl:AsymmetricProperty,
        owl:IrreflexiveProperty ;
    rdfs:comment "Describes similar arthropods"^^xsd:string ;
    rdfs:domain nell:arthropod ;
    rdfs:range nell:arthropod ;
    rdfs:subPropertyOf nell:animalistypeofanimal .

nell:arthropodbesometimesconfusewithinsect rdfs:comment "Arthropodes that usually are confunded by insects"^^xsd:string ;
    rdfs:domain nell:arthropod ;
    rdfs:range nell:insect ;
    rdfs:subPropertyOf nell:relatedto .

nell:arthropodcalledarthropod rdfs:comment "Describes the names an artery can be called"^^xsd:string ;
    rdfs:domain nell:arthropod ;
    rdfs:range nell:arthropod ;
    rdfs:subPropertyOf nell:synonymfor .

nell:arthropodcanbeveryirritatingtomammal rdfs:comment "Arthropode that usually irritates mammal"^^xsd:string ;
    rdfs:domain nell:arthropod ;
    rdfs:range nell:mammal ;
    rdfs:subPropertyOf nell:relatedto .

nell:arthropodlookslikeinsect rdfs:comment "Describes the arthropod that look like specific insects"^^xsd:string ;
    rdfs:domain nell:arthropod ;
    rdfs:range nell:insect ;
    rdfs:subPropertyOf nell:relatedto .

nell:arthropodsuchascrustacean rdfs:comment "Hyponym Relation"^^xsd:string ;
    rdfs:domain nell:crustacean ;
    rdfs:range nell:arthropod ;
    rdfs:subPropertyOf nell:generalizationof .

nell:arthropodthatfeedoninsect rdfs:comment "Describes the names an artery can be called"^^xsd:string ;
    rdfs:domain nell:arthropod ;
    rdfs:range nell:insect ;
    rdfs:subPropertyOf nell:relatedto .

nell:astronautssuchasaustronauts rdfs:comment "Describes the specific astronaut types that are generalizations of astronauts"^^xsd:string ;
    rdfs:domain nell:astronaut ;
    rdfs:range nell:astronaut ;
    rdfs:subPropertyOf nell:generalizationof .

nell:astronautwasonamissionwithastronaut rdfs:comment "Describes astronauts that were at a space mission togheter"^^xsd:string ;
    rdfs:domain nell:astronaut ;
    rdfs:range nell:astronaut ;
    rdfs:subPropertyOf nell:relatedto .

nell:athletealsoknownas rdfs:comment "this is another name for this athlete"^^xsd:string ;
    rdfs:domain nell:athlete ;
    rdfs:range nell:athlete ;
    rdfs:subPropertyOf nell:personalsoknownas .

nell:athletebeatathlete a owl:AsymmetricProperty,
        owl:IrreflexiveProperty ;
    rdfs:comment "Describes the athletes whom beat other athletes"^^xsd:string ;
    rdfs:domain nell:athlete ;
    rdfs:range nell:athlete ;
    rdfs:subPropertyOf nell:relatedto .

nell:athletecanbethesameasactor rdfs:comment "Describes actors that are the same instances as athlete"^^xsd:string ;
    rdfs:domain nell:athlete ;
    rdfs:range nell:actor ;
    rdfs:subPropertyOf nell:canbethesameas .

nell:athletecoach rdfs:comment "to give instruction or advice to in the capacity of a coach; instruct "^^xsd:string ;
    rdfs:domain nell:athlete ;
    rdfs:range nell:coach ;
    rdfs:subPropertyOf nell:agenthierarchicallybelowagent .

nell:athleteflyouttosportsteamposition rdfs:domain nell:athlete ;
    rdfs:range nell:sportsteamposition ;
    rdfs:subPropertyOf nell:relatedto .

nell:athletefracturedbone rdfs:comment "Bone fracture that an athlete had"^^xsd:string ;
    rdfs:domain nell:athlete ;
    rdfs:range nell:bone ;
    rdfs:subPropertyOf nell:athleteinjuredhisbodypart .

nell:athletehomestadium rdf:first <http://www.semanticweb.org/ontologies/NELL#_:y28>,
        <http://www.semanticweb.org/ontologies/NELL#_:y32>,
        <http://www.semanticweb.org/ontologies/NELL#_:y6> ;
    rdfs:comment "a sports arena usually oval or horseshoe-shaped with tiers of seats for spectators (which is home for an athlete) "^^xsd:string ;
    rdfs:domain nell:athlete ;
    rdfs:range nell:stadiumoreventvenue ;
    rdfs:subPropertyOf nell:agentactsinlocation .

nell:athleteledsportsteam rdfs:comment "Describes the athletes that lead/led a sports team"^^xsd:string ;
    rdfs:domain nell:athlete ;
    rdfs:range nell:sportsteam ;
    rdfs:subPropertyOf nell:athleteplaysforteam .

nell:athleteplayedforschool rdfs:comment "The school that an athlete used to play for its team"^^xsd:string ;
    rdfs:domain nell:athlete ;
    rdfs:range nell:school ;
    rdfs:subPropertyOf nell:personbelongstoorganization .

nell:athleteplaysinleague rdfs:comment "a group of athletic teams organized to promote mutual interests and to compete chiefly among themselves "^^xsd:string ;
    rdfs:domain nell:athlete ;
    rdfs:range nell:sportsleague ;
    rdfs:subPropertyOf nell:personbelongstoorganization .

nell:athleteplayssport rdfs:comment "to engage in (a game pastime etc.) "^^xsd:string ;
    rdfs:domain nell:athlete ;
    rdfs:range nell:sport ;
    rdfs:subPropertyOf nell:relatedto .

nell:athleteplayssportsteamposition rdfs:comment "The team position played by an athlete."^^xsd:string ;
    rdfs:domain nell:athlete ;
    rdfs:range nell:sportsteamposition ;
    rdfs:subPropertyOf nell:relatedto .

nell:athletepublishesinblog rdfs:comment "The blog where an athlete publishes"^^xsd:string ;
    rdfs:domain nell:athlete ;
    rdfs:range nell:blog ;
    rdfs:subPropertyOf nell:relatedto .

nell:athletessuchasathletes rdfs:comment "Describes the specific athlete types that are generalizations of athletes"^^xsd:string ;
    rdfs:domain nell:athlete ;
    rdfs:range nell:athlete ;
    rdfs:subPropertyOf nell:generalizationof .

nell:athletewinsawardtrophytournament rdf:first <http://www.semanticweb.org/ontologies/NELL#_:y20> ;
    rdfs:comment "Describes the athletes who won an award trophy tournament"^^xsd:string ;
    rdfs:domain nell:athlete ;
    rdfs:range nell:awardtrophytournament ;
    rdfs:subPropertyOf nell:relatedto .

nell:attackerinbombing rdfs:domain nell:agent ;
    rdfs:range nell:bombingevent ;
    rdfs:subPropertyOf nell:relatedto .

nell:attractionbefallincity rdfs:comment "Attraction occurs in the city"^^xsd:string ;
    rdfs:domain nell:attraction ;
    rdfs:range nell:city ;
    rdfs:subPropertyOf nell:attractionofcity .

nell:attractionmadeofbuildingmaterial rdfs:comment "Describes the materials used to build attractions"^^xsd:string ;
    rdfs:domain nell:attraction ;
    rdfs:range nell:buildingmaterial ;
    rdfs:subPropertyOf nell:relatedto .

nell:automakerproducesmodel rdfs:comment "this automobile manufacturer produces this particular automobile make or model"^^xsd:string ;
    rdfs:domain nell:automobilemaker ;
    rdfs:range nell:automobilemodel ;
    rdfs:subPropertyOf nell:producesproduct .

nell:automobileenginesuchasautomobileengine rdfs:comment "Describes the specific automobile Engine types that are generalizations of automobile Engines"^^xsd:string ;
    rdfs:domain nell:automobileengine ;
    rdfs:range nell:automobileengine ;
    rdfs:subPropertyOf nell:generalizationof .

nell:automobilemakercardealersinstateorprovince rdfs:comment "Describes the car dealers in a state or province"^^xsd:string ;
    rdfs:domain nell:automobilemaker ;
    rdfs:range nell:stateorprovince ;
    rdfs:subPropertyOf nell:relatedto .

nell:automobilemakerchiefexecutiveceo rdfs:comment "Describes the CEOs of automobile maker companies"^^xsd:string ;
    rdfs:domain nell:automobilemaker ;
    rdfs:range nell:ceo ;
    rdfs:subPropertyOf nell:companyceo .

nell:automobilemakerdealersincity rdfs:comment "Describes the car dealers in a city"^^xsd:string ;
    rdfs:domain nell:automobilemaker ;
    rdfs:range nell:city ;
    rdfs:subPropertyOf nell:hasofficeincity .

nell:automobilemakerdealersincountry rdfs:comment "Describes the car dealers in a country"^^xsd:string ;
    rdfs:domain nell:automobilemaker ;
    rdfs:range nell:country ;
    rdfs:subPropertyOf nell:hasofficeincountry .

nell:automodelproducedbymaker rdfs:comment "this automobile manufacturer produces this particular automobile make or model"^^xsd:string ;
    rdfs:domain nell:automobilemodel ;
    rdfs:range nell:automobilemaker ;
    rdfs:subPropertyOf nell:producedby .

nell:awardtrophytournamentisthechampionshipgameofthenationalsport rdfs:comment "Describes award trophy tournaments related to specific sports"^^xsd:string ;
    rdfs:domain nell:awardtrophytournament ;
    rdfs:range nell:sport ;
    rdfs:subPropertyOf nell:relatedto .

nell:awardtrophytournamentwasawardedonstadium rdfs:comment "Stadium of event venue where a award trophy tournament was at least once awarded"^^xsd:string ;
    rdfs:domain nell:awardtrophytournament ;
    rdfs:range nell:stadiumoreventvenue ;
    rdfs:subPropertyOf nell:atlocation .

nell:awayteamingame rdfs:comment "Specifies that a particular team is the away team in a particular sportsGame."^^xsd:string ;
    rdfs:domain nell:sportsteam ;
    rdfs:range nell:sportsgame ;
    rdfs:subPropertyOf nell:teamingame .

nell:bacteriacancauseillnessfromfood rdfs:comment "Describes the foods that bacterias can cause illness from"^^xsd:string ;
    rdfs:domain nell:bacteria ;
    rdfs:range nell:food ;
    rdfs:subPropertyOf nell:relatedto .

nell:bacteriaisthecausativeagentofphysiologicalcondition rdfs:comment "Describes the bacterias that causes physiological conditions"^^xsd:string ;
    rdfs:domain nell:bacteria ;
    rdfs:range nell:physiologicalcondition ;
    rdfs:subPropertyOf nell:relatedto .

nell:bakedgoodservedwithbeverage rdfs:comment "Describes the baked goods that are usually served with a beverage"^^xsd:string ;
    rdfs:domain nell:bakedgood ;
    rdfs:range nell:beverage ;
    rdfs:subPropertyOf nell:itemusedwithitem .

nell:bakegoodistypicalincountry rdfs:comment "Describes the typicall bakegoods of the countries"^^xsd:string ;
    rdfs:domain nell:bakedgood ;
    rdfs:range nell:country ;
    rdfs:subPropertyOf nell:relatedto .

nell:bankbankincountry rdfs:comment "Describes the banks in a country"^^xsd:string ;
    rdfs:domain nell:bank ;
    rdfs:range nell:country ;
    rdfs:subPropertyOf nell:hasofficeincountry .

nell:bankboughtbank a owl:AsymmetricProperty,
        owl:IrreflexiveProperty ;
    rdfs:comment "Describes the banks that bought other banks"^^xsd:string ;
    rdfs:domain nell:bank ;
    rdfs:range nell:bank ;
    rdfs:subPropertyOf nell:acquired .

nell:bankchiefexecutiveceo rdfs:comment "Describes the CEOs of banks"^^xsd:string ;
    rdfs:domain nell:bank ;
    rdfs:range nell:ceo ;
    rdfs:subPropertyOf nell:companyceo .

nell:bathroomitem rdfs:comment "Any item that is commonly found in a bathroom or restroom."^^xsd:string ;
    rdfs:subClassOf nell:householditem .

nell:beach rdfs:comment "geological landform along the shoreline of an ocean sea or lake. It usually consists of loose particles which are often composed of rock such as sand gravel shingle pebbles waves or cobblestones"^^xsd:string ;
    rdfs:subClassOf nell:location .

nell:bedroomitem rdfs:comment "Any item that is commonly found in a bedroom."^^xsd:string ;
    rdfs:subClassOf nell:householditem .

nell:beveragecansoftendisease rdfs:comment "Describes beverages that can help soften the symptons of diseases"^^xsd:string ;
    rdfs:domain nell:beverage ;
    rdfs:range nell:disease ;
    rdfs:subPropertyOf nell:relatedto .

nell:beveragecontainsprotein rdfs:comment "Describes the proteins contained in beverages"^^xsd:string ;
    rdfs:domain nell:beverage ;
    rdfs:range nell:protein ;
    rdfs:subPropertyOf nell:relatedto .

nell:beveragemadefrombeverage rdfs:comment "Describes the names an artery can be called"^^xsd:string ;
    rdfs:domain nell:beverage ;
    rdfs:range nell:beverage ;
    rdfs:subPropertyOf nell:relatedto .

nell:biologicalfatherofperson rdfs:comment "is biological father of a person"^^xsd:string ;
    rdfs:domain nell:male ;
    rdfs:range nell:person ;
    rdfs:subPropertyOf nell:agentcreated,
        nell:fatherofperson .

nell:biologicalmotherofperson rdfs:comment "is biological mother of a person"^^xsd:string ;
    rdfs:domain nell:female ;
    rdfs:range nell:person ;
    rdfs:subPropertyOf nell:agentcreated,
        nell:motherofperson .

nell:biotechcompany rdfs:comment "A company in a biotechnology field including pharmaceutical companies."^^xsd:string ;
    rdfs:subClassOf nell:company .

nell:birdmayconsumeprotein rdfs:comment "Describes the proteins eaten by a bird"^^xsd:string ;
    rdfs:domain nell:bird ;
    rdfs:range nell:protein ;
    rdfs:subPropertyOf nell:relatedto .

nell:boardgame rdfs:comment "Games played with physical pieces on a board (electronic games not allowed)"^^xsd:string ;
    rdfs:subClassOf nell:traditionalgame .

nell:bodypartcontainsbodypart rdfs:comment "indicates that one body part is contained inside another"^^xsd:string ;
    rdfs:domain nell:bodypart ;
    rdfs:range nell:bodypart ;
    rdfs:subPropertyOf nell:superpartof .

nell:bodypartcontainsmuscle rdfs:comment "Describes the muscles in body parts"^^xsd:string ;
    rdfs:domain nell:bodypart ;
    rdfs:range nell:muscle ;
    rdfs:subPropertyOf nell:superpartof .

nell:bodypartwithinbodypart a owl:AsymmetricProperty,
        owl:IrreflexiveProperty ;
    rdfs:comment "indicates that one body part is contained inside another"^^xsd:string ;
    rdfs:domain nell:bodypart ;
    rdfs:range nell:bodypart ;
    rdfs:subPropertyOf nell:subpartof .

nell:bombingarrested rdfs:domain nell:bombingevent ;
    rdfs:range nell:nonneginteger ;
    rdfs:subPropertyOf nell:relatedto .

nell:bombingattacker rdfs:domain nell:bombingevent ;
    rdfs:range nell:agent ;
    rdfs:subPropertyOf nell:relatedto .

nell:bombingcausedbyexplosive rdfs:domain nell:bombingevent ;
    rdfs:range nell:chemical ;
    rdfs:subPropertyOf nell:relatedto .

nell:bombingcommentedby rdfs:domain nell:bombingevent ;
    rdfs:range nell:person ;
    rdfs:subPropertyOf nell:relatedto .

nell:bombingdamaged rdfs:domain nell:bombingevent ;
    rdfs:range nell:geolocatablething ;
    rdfs:subPropertyOf nell:relatedto .

nell:bombingeventtime rdfs:domain nell:bombingevent ;
    rdfs:range nell:time ;
    rdfs:subPropertyOf nell:relatedto .

nell:bombinghaswitness rdfs:domain nell:person ;
    rdfs:range nell:bombingevent ;
    rdfs:subPropertyOf nell:relatedto .

nell:bombinginjured rdfs:domain nell:bombingevent ;
    rdfs:range nell:nonneginteger ;
    rdfs:subPropertyOf nell:relatedto .

nell:bombinginjuried rdfs:domain nell:bombingevent ;
    rdfs:range nell:person ;
    rdfs:subPropertyOf nell:relatedto .

nell:bombingkilled rdfs:domain nell:bombingevent ;
    rdfs:range nell:nonneginteger ;
    rdfs:subPropertyOf nell:relatedto .

nell:bombingoccuredin rdfs:domain nell:bombingevent ;
    rdfs:range nell:location ;
    rdfs:subPropertyOf nell:relatedto .

nell:bombingsecurity rdfs:domain nell:bombingevent ;
    rdfs:range nell:agent ;
    rdfs:subPropertyOf nell:relatedto .

nell:bombingtarget rdfs:domain nell:bombingevent ;
    rdfs:range nell:everypromotedthing ;
    rdfs:subPropertyOf nell:relatedto .

nell:bombingvictim rdfs:domain nell:bombingevent ;
    rdfs:range nell:person ;
    rdfs:subPropertyOf nell:relatedto .

nell:bombingwitness rdfs:domain nell:bombingevent ;
    rdfs:range nell:person ;
    rdfs:subPropertyOf nell:relatedto .

nell:booksuchasbook rdfs:comment "Describes the specific book types that are generalizations of actors"^^xsd:string ;
    rdfs:domain nell:book ;
    rdfs:range nell:book ;
    rdfs:subPropertyOf nell:generalizationof .

nell:bookwriter rdfs:comment "author of a book"^^xsd:string ;
    rdfs:domain nell:book ;
    rdfs:range nell:writer ;
    rdfs:subPropertyOf nell:creativeworkcontributedtobyagent .

nell:braintissue rdfs:comment "any subregion of the brain but not including single nerves"^^xsd:string ;
    rdfs:subClassOf nell:bodypart .

nell:bridge rdfs:comment "A bridge is a structure across water valleys railway cuts areas of low elevation or other features which are difficult to cross."^^xsd:string ;
    rdfs:subClassOf nell:building .

nell:brotherof rdfs:comment "person has a brother"^^xsd:string ;
    rdfs:domain nell:male ;
    rdfs:range nell:person ;
    rdfs:subPropertyOf nell:hassibling .

nell:buildingbelongstoorganization rdfs:comment "Which organization a building belongs to"^^xsd:string ;
    rdfs:domain nell:building ;
    rdfs:range nell:organization ;
    rdfs:subPropertyOf nell:locationactedinbyorganization .

nell:buildingfeaturebuiltabovelake rdfs:comment "buildingfeature and lake are related"^^xsd:string ;
    rdfs:domain nell:buildingfeature ;
    rdfs:range nell:lake ;
    rdfs:subPropertyOf nell:relatedto .

nell:buildingfeaturemadefrombuildingmaterial rdfs:comment "Describes the building features that are made of a building material"^^xsd:string ;
    rdfs:domain nell:buildingfeature ;
    rdfs:range nell:buildingmaterial ;
    rdfs:subPropertyOf nell:relatedto .

nell:buildinghasofficebuildingroom rdfs:comment "Which office-style building a particular room is found in"^^xsd:string ;
    rdfs:domain nell:building ;
    rdfs:range nell:officebuildingroom ;
    rdfs:subPropertyOf nell:locationcontainslocation .

nell:buildinghostsmeetingeventtitle rdfs:comment "In which building a particular meeting will take place"^^xsd:string ;
    rdfs:domain nell:building ;
    rdfs:range nell:meetingeventtitle ;
    rdfs:subPropertyOf nell:locationofevent .

nell:buildingispartofuniversity rdfs:comment "Describes buildings that universities might own"^^xsd:string ;
    rdfs:domain nell:building ;
    rdfs:range nell:university ;
    rdfs:subPropertyOf nell:relatedto .

nell:cafeservescoffeedrink rdfs:domain nell:caf_ ;
    rdfs:range nell:coffeedrink ;
    rdfs:subPropertyOf nell:agentinvolvedwithitem .

nell:cardgame rdfs:comment "Games that are played with only a physical deck of cards (electronic games not allowed)"^^xsd:string ;
    rdfs:subClassOf nell:traditionalgame .

nell:cave rdfs:comment "An underground space humans or animals can enter - a cave."^^xsd:string ;
    rdfs:subClassOf nell:location .

nell:celebritycanbethesameasceo rdfs:comment "Describes two instances that are the same thing in these two different categories"^^xsd:string ;
    rdfs:domain nell:celebrity ;
    rdfs:range nell:ceo ;
    rdfs:subPropertyOf nell:canbethesameas .

nell:celebritysuchascelebrity rdfs:comment "Describes the specific celebrity types that are generalizations of celebrities"^^xsd:string ;
    rdfs:domain nell:celebrity ;
    rdfs:range nell:celebrity ;
    rdfs:subPropertyOf nell:generalizationof .

nell:celltype rdfs:comment "A cell type is a distinct morphological or functional form of cell "^^xsd:string ;
    rdfs:subClassOf nell:abstractthing .

nell:ceocanbethesameascelebrity rdfs:comment "Describes two instances that are the same thing in these two different categories"^^xsd:string ;
    rdfs:domain nell:ceo ;
    rdfs:range nell:celebrity ;
    rdfs:subPropertyOf nell:canbethesameas .

nell:charactertrait rdfs:comment "habitual patterns of behavior thought and emotion "^^xsd:string ;
    rdfs:subClassOf nell:abstractthing .

nell:cheese rdfs:comment "Any cheese"^^xsd:string ;
    rdfs:subClassOf nell:food .

nell:chef rdfs:comment "A chef is a professional cook."^^xsd:string ;
    rdfs:subClassOf nell:person .

nell:chemicalistypeofchemical rdfs:comment "indicates that one chemical is special case of another chemical"^^xsd:string ;
    rdfs:domain nell:chemical ;
    rdfs:range nell:chemical ;
    rdfs:subPropertyOf nell:specializationof .

nell:chemicaltypehaschemical a owl:AsymmetricProperty,
        owl:IrreflexiveProperty ;
    rdfs:comment "indicates that one chemical is special case of another chemical"^^xsd:string ;
    rdfs:domain nell:chemical ;
    rdfs:range nell:chemical ;
    rdfs:subPropertyOf nell:generalizationof .

nell:cityalsoknownas a owl:IrreflexiveProperty,
        owl:SymmetricProperty ;
    rdfs:comment "this is another name for this city"^^xsd:string ;
    rdfs:domain nell:city ;
    rdfs:range nell:city ;
    rdfs:subPropertyOf nell:synonymfor .

nell:cityaquariums rdfs:comment "The city an aquarium is located in."^^xsd:string ;
    rdfs:domain nell:city ;
    rdfs:range nell:aquarium ;
    rdfs:subPropertyOf nell:cityattractions .

nell:citycapitalofcountry rdfs:comment "specifies that a particular city is the capital of a particular country"^^xsd:string ;
    rdfs:domain nell:city ;
    rdfs:range nell:country ;
    rdfs:subPropertyOf nell:citylocatedincountry,
        nell:proxyfor .

nell:citycapitalofstate rdfs:comment "The capital city of a state where the main governing apparatus is located."^^xsd:string ;
    rdfs:domain nell:city ;
    rdfs:range nell:stateorprovince ;
    rdfs:subPropertyOf nell:citylocatedinstate,
        nell:proxyfor .

nell:cityhasairport rdfs:comment "The city an airport is located in."^^xsd:string ;
    rdfs:domain nell:city ;
    rdfs:range nell:airport ;
    rdfs:subPropertyOf nell:citycontainsbuilding .

nell:cityhashospital rdfs:comment "The city a hostpital is located in."^^xsd:string ;
    rdfs:domain nell:city ;
    rdfs:range nell:hospital ;
    rdfs:subPropertyOf nell:citycontainsbuilding .

nell:cityhasshoppingmall rdfs:comment "The city a shopping mall is located in."^^xsd:string ;
    rdfs:domain nell:city ;
    rdfs:range nell:shoppingmall ;
    rdfs:subPropertyOf nell:citycontainsbuilding .

nell:cityhasstreet rdfs:comment "this street is at least partly inside this city"^^xsd:string ;
    rdfs:domain nell:city ;
    rdfs:range nell:street ;
    rdfs:subPropertyOf nell:locationcontainslocation .

nell:cityhastrainstation rdfs:comment "The city a train station is in."^^xsd:string ;
    rdfs:domain nell:city ;
    rdfs:range nell:trainstation ;
    rdfs:subPropertyOf nell:locationcontainslocation .

nell:cityhastransportation rdfs:comment "City of a transportation system."^^xsd:string ;
    rdfs:domain nell:city ;
    rdfs:range nell:transportation ;
    rdfs:subPropertyOf nell:cityattractions .

nell:cityhostsattraction rdfs:comment "Attraction occurs in the city"^^xsd:string ;
    rdfs:domain nell:city ;
    rdfs:range nell:attraction ;
    rdfs:subPropertyOf nell:cityattractions .

nell:cityhotels a owl:InverseFunctionalProperty ;
    rdfs:comment "The city a hotel is located in."^^xsd:string ;
    rdfs:domain nell:city ;
    rdfs:range nell:hotel ;
    rdfs:subPropertyOf nell:citycontainsbuilding .

nell:citylanguage rdfs:comment "Typical language spoken in a city (official or otherwise)"^^xsd:string ;
    rdfs:domain nell:city ;
    rdfs:range nell:language ;
    rdfs:subPropertyOf nell:relatedto .

nell:cityleadbyperson rdfs:comment "specifies that a particular person is the leader (e.g. Mayor) of a particular city"^^xsd:string ;
    rdfs:domain nell:city ;
    rdfs:range nell:politician ;
    rdfs:subPropertyOf nell:geopoliticalorganizationleadbyperson .

nell:cityliesonriver rdfs:comment "Rivers that flow or through or immediately adjacent to the city."^^xsd:string ;
    rdfs:domain nell:city ;
    rdfs:range nell:river ;
    rdfs:subPropertyOf nell:atlocation .

nell:citymuseums rdfs:comment "The city that a museum is located in"^^xsd:string ;
    rdfs:domain nell:city ;
    rdfs:range nell:museum ;
    rdfs:subPropertyOf nell:cityattractions,
        nell:citycontainsbuilding .

nell:citynewspaper a owl:InverseFunctionalProperty ;
    rdfs:comment "Specifies the city in which a particular newspaper is headquartered"^^xsd:string ;
    rdfs:domain nell:city ;
    rdfs:range nell:newspaper ;
    rdfs:subPropertyOf nell:locationactedinbyagent .

nell:cityofpersondeath rdfs:comment "the city that a person died in"^^xsd:string ;
    rdfs:domain nell:city ;
    rdfs:range nell:person ;
    rdfs:subPropertyOf nell:locationofpersondeath .

nell:cityparks a owl:InverseFunctionalProperty ;
    rdfs:comment "The city a park is located in."^^xsd:string ;
    rdfs:domain nell:city ;
    rdfs:range nell:park ;
    rdfs:subPropertyOf nell:cityattractions .

nell:cityradiostation a owl:InverseFunctionalProperty ;
    rdfs:comment "Specifies that a particular radio station is headquarted in a particular city"^^xsd:string ;
    rdfs:domain nell:city ;
    rdfs:range nell:radiostation ;
    rdfs:subPropertyOf nell:cityhascompanyoffice .

nell:cityresidenceofperson rdfs:comment "the city that a person has residence in"^^xsd:string ;
    rdfs:domain nell:city ;
    rdfs:range nell:person ;
    rdfs:subPropertyOf nell:locationresidenceofperson .

nell:cityrestaurants rdfs:comment "The city a restaurant is located in."^^xsd:string ;
    rdfs:domain nell:city ;
    rdfs:range nell:restaurant ;
    rdfs:subPropertyOf nell:citycontainsbuilding .

nell:citysportsteams rdfs:comment "The home city of a sports team typically a location where the team frequently competes."^^xsd:string ;
    rdfs:domain nell:city ;
    rdfs:range nell:sportsteam ;
    rdfs:subPropertyOf nell:locationactedinbyorganization,
        nell:proxyfor .

nell:citystadiums rdfs:comment "The city where a stadium is located"^^xsd:string ;
    rdfs:domain nell:city ;
    rdfs:range nell:stadiumoreventvenue ;
    rdfs:subPropertyOf nell:cityattractions,
        nell:citycontainsbuilding,
        nell:proxyfor .

nell:citytelevisionstation a owl:InverseFunctionalProperty ;
    rdfs:comment "The city where a TV station is located or broadcasts to."^^xsd:string ;
    rdfs:domain nell:city ;
    rdfs:range nell:televisionstation ;
    rdfs:subPropertyOf nell:cityhascompanyoffice .

nell:cityuniversities rdfs:comment "The city a university is located in."^^xsd:string ;
    rdfs:domain nell:city ;
    rdfs:range nell:university ;
    rdfs:subPropertyOf nell:locationactedinbyorganization .

nell:cityzoos rdfs:comment "The city a zoo is located in"^^xsd:string ;
    rdfs:domain nell:city ;
    rdfs:range nell:zoo ;
    rdfs:subPropertyOf nell:cityattractions .

nell:clothingmadefromplant rdfs:comment "Describes the clothing items made of a plant"^^xsd:string ;
    rdfs:domain nell:clothing ;
    rdfs:range nell:plant ;
    rdfs:subPropertyOf nell:relatedto .

nell:clothingtogowithclothing a owl:IrreflexiveProperty,
        owl:SymmetricProperty ;
    rdfs:comment "Describes clothing pieces that \"should\" (or can) be used with each other"^^xsd:string ;
    rdfs:domain nell:clothing ;
    rdfs:range nell:clothing ;
    rdfs:subPropertyOf nell:itemusedwithitem .

nell:clothmadeofplant rdfs:comment "Plants that can be used to make cloths"^^xsd:string ;
    rdfs:domain nell:clothing ;
    rdfs:range nell:plant ;
    rdfs:subPropertyOf nell:relatedto .

nell:coachalsoknownas rdfs:comment "this is another name for this coach"^^xsd:string ;
    rdfs:domain nell:coach ;
    rdfs:range nell:coach ;
    rdfs:subPropertyOf nell:personalsoknownas .

nell:coachcanspeaklanguage rdfs:comment "Describes the languages that coaches might speak"^^xsd:string ;
    rdfs:domain nell:coach ;
    rdfs:range nell:language ;
    rdfs:subPropertyOf nell:relatedto .

nell:coachesathlete rdfs:comment "to give instruction or advice to in the capacity of a coach; instruct "^^xsd:string ;
    rdfs:domain nell:coach ;
    rdfs:range nell:athlete ;
    rdfs:subPropertyOf nell:agenthierarchicallyaboveagent .

nell:coachesinleague rdfs:comment "specifies that a particular coach coaches a team that plays in a particular league"^^xsd:string ;
    rdfs:domain nell:coach ;
    rdfs:range nell:sportsleague ;
    rdfs:subPropertyOf nell:personbelongstoorganization .

nell:coachesteam rdfs:comment "specifies that a particular coach coaches a particular team"^^xsd:string ;
    rdfs:domain nell:coach ;
    rdfs:range nell:sportsteam ;
    rdfs:subPropertyOf nell:worksfor .

nell:coachstudiedatuniversity rdfs:comment "Describes the university where the coach studied at"^^xsd:string ;
    rdfs:domain nell:coach ;
    rdfs:range nell:university ;
    rdfs:subPropertyOf nell:relatedto .

nell:coachwontrophy rdfs:comment "specifies that a particular coach coaches a team that won a particular award or trophy"^^xsd:string ;
    rdfs:domain nell:coach ;
    rdfs:range nell:awardtrophytournament ;
    rdfs:subPropertyOf nell:relatedto .

nell:coachworksincountry rdfs:comment "Describes the country where a coach works"^^xsd:string ;
    rdfs:domain nell:coach ;
    rdfs:range nell:country ;
    rdfs:subPropertyOf nell:agentactsinlocation .

nell:coffeeservedbycafe rdfs:domain nell:coffeedrink ;
    rdfs:range nell:caf_ ;
    rdfs:subPropertyOf nell:iteminvolvedwithagent .

nell:cognitiveactions rdfs:comment "pertaining \"to the action or process of knowing\" "^^xsd:string ;
    rdfs:subClassOf nell:abstractthing .

nell:collidedwith rdfs:domain nell:roadaccidentevent ;
    rdfs:range nell:everypromotedthing ;
    rdfs:subPropertyOf nell:relatedto .

nell:colorassociatedwithvisualizableattribute rdfs:comment "color and visualizableattribute are related"^^xsd:string ;
    rdfs:domain nell:color ;
    rdfs:range nell:visualizableattribute ;
    rdfs:subPropertyOf nell:relatedto .

nell:colorofobject rdfs:comment "Object has color (NEIL)"^^xsd:string ;
    rdfs:domain nell:color ;
    rdfs:range nell:visualizablething ;
    rdfs:subPropertyOf nell:relatedto .

nell:comediancanbethesameasfemale rdfs:comment "Describes two instances that are the same thing in these two different categories"^^xsd:string ;
    rdfs:domain nell:comedian ;
    rdfs:range nell:female ;
    rdfs:subPropertyOf nell:canbethesameas .

nell:comediancanbethesameasmale rdfs:comment "Describes two instances that are the same thing in these two different categories"^^xsd:string ;
    rdfs:domain nell:comedian ;
    rdfs:range nell:male ;
    rdfs:subPropertyOf nell:canbethesameas .

nell:commentatorofbombing rdfs:domain nell:person ;
    rdfs:range nell:bombingevent ;
    rdfs:subPropertyOf nell:relatedto .

nell:commentatorofearthquake rdfs:domain nell:person ;
    rdfs:range nell:earthquakeevent ;
    rdfs:subPropertyOf nell:relatedto .

nell:commentatorofprotest rdfs:domain nell:person ;
    rdfs:range nell:protestevent ;
    rdfs:subPropertyOf nell:relatedto .

nell:commentatorofroadaccident rdfs:domain nell:person ;
    rdfs:range nell:roadaccidentevent ;
    rdfs:subPropertyOf nell:relatedto .

nell:companiesheadquarteredhere rdfs:comment "specifies that a particular company is headquartered in a particular city"^^xsd:string ;
    rdfs:domain nell:city ;
    rdfs:range nell:company ;
    rdfs:subPropertyOf nell:cityhascompanyoffice,
        nell:cityoforganizationheadquarters .

nell:companyalsoknownas a owl:IrreflexiveProperty,
        owl:SymmetricProperty ;
    rdfs:comment "this is another name for this company"^^xsd:string ;
    rdfs:domain nell:company ;
    rdfs:range nell:company ;
    rdfs:subPropertyOf nell:organizationalsoknownas .

nell:companycompetingwithproduuctlaunch rdfs:domain nell:company ;
    rdfs:range nell:productlaunchevent ;
    rdfs:subPropertyOf nell:relatedto .

nell:companyeconomicsector rdfs:comment "specifies that a particular company does business in a particular economic sector"^^xsd:string ;
    rdfs:domain nell:company ;
    rdfs:range nell:economicsector ;
    rdfs:subPropertyOf nell:relatedto .

nell:companyhasshareholder rdfs:comment "Any organization person or geopolitical entity that holds shares (majority or otherwise) of the given company."^^xsd:string ;
    rdfs:domain nell:company ;
    rdfs:range nell:agent ;
    rdfs:subPropertyOf nell:agentcollaborateswithagent .

nell:companyofproductlaunch rdfs:domain nell:company ;
    rdfs:range nell:productlaunchevent ;
    rdfs:subPropertyOf nell:relatedto .

nell:companyproducesvideogamesystem rdfs:comment "company produces a video game system"^^xsd:string ;
    rdfs:domain nell:company ;
    rdfs:range nell:videogamesystem ;
    rdfs:subPropertyOf nell:relatedto .

nell:competeswith a owl:IrreflexiveProperty,
        owl:SymmetricProperty ;
    rdfs:comment "specifies that a particular company has been in competition with another particular company"^^xsd:string ;
    rdfs:domain nell:company ;
    rdfs:range nell:company ;
    rdfs:subPropertyOf nell:agentcompeteswithagent .

nell:competitorofproductlaunch rdfs:domain nell:product ;
    rdfs:range nell:productlaunchevent ;
    rdfs:subPropertyOf nell:relatedto .

nell:concepthasprerequisite rdfs:comment "Prerequisite relationship between scientific terms (currently biased towards ML and AI areas)"^^xsd:string ;
    rdfs:domain nell:scientificterm ;
    rdfs:range nell:scientificterm ;
    rdfs:subPropertyOf nell:relatedto .

nell:conceptprerequisiteof a owl:AsymmetricProperty,
        owl:IrreflexiveProperty ;
    rdfs:comment "Prerequisite relationship between scientific terms (currently biased towards ML and AI areas)"^^xsd:string ;
    rdfs:domain nell:scientificterm ;
    rdfs:range nell:scientificterm ;
    rdfs:subPropertyOf nell:relatedto .

nell:condiment rdfs:comment "A sauce or seasoning added to food to impart a particular flavor or to complement the dish. (Wikipedia)"^^xsd:string ;
    rdfs:subClassOf nell:food .

nell:conferencessuchasconferences rdfs:comment "Describes the conferences types that are generalizations of specific conferences"^^xsd:string ;
    rdfs:domain nell:conference ;
    rdfs:range nell:conference ;
    rdfs:subPropertyOf nell:generalizationof .

nell:continent rdfs:comment "A continent is a large land mass defined mostly by conventional use but closely related to tectonic plates within the earth's crust."^^xsd:string ;
    rdfs:subClassOf nell:geopoliticallocation .

nell:convention rdfs:comment "a large meeting such as the Star Trek Convention"^^xsd:string ;
    rdfs:subClassOf nell:event .

nell:countriessuchascountries a owl:AsymmetricProperty,
        owl:IrreflexiveProperty ;
    rdfs:comment "Describes the countries types that are generalizations of specific countries"^^xsd:string ;
    rdfs:domain nell:country ;
    rdfs:range nell:country ;
    rdfs:subPropertyOf nell:generalizationof .

nell:countryalsoknownas a owl:IrreflexiveProperty,
        owl:SymmetricProperty ;
    rdfs:comment "this is another name for this country"^^xsd:string ;
    rdfs:domain nell:country ;
    rdfs:range nell:country ;
    rdfs:subPropertyOf nell:synonymfor .

nell:countrycapital a owl:InverseFunctionalProperty ;
    rdf:first <http://www.semanticweb.org/ontologies/NELL#_:y35>,
        <http://www.semanticweb.org/ontologies/NELL#_:y40> ;
    rdfs:comment "specifies that a particular city is the capital of a particular country"^^xsd:string ;
    rdfs:domain nell:country ;
    rdfs:range nell:city ;
    rdfs:subPropertyOf nell:countrycities,
        nell:proxyof .

nell:countrycontainsfarm rdfs:comment "The country a farm is located in"^^xsd:string ;
    rdfs:domain nell:country ;
    rdfs:range nell:farm ;
    rdfs:subPropertyOf nell:locationcontainslocation .

nell:countrycurrency rdfs:comment "specifies that a particular country uses a particular currency"^^xsd:string ;
    rdfs:domain nell:country ;
    rdfs:range nell:currency ;
    rdfs:subPropertyOf nell:relatedto .

nell:countryhascitizen rdf:first <http://www.semanticweb.org/ontologies/NELL#_:y21>,
        <http://www.semanticweb.org/ontologies/NELL#_:y23>,
        <http://www.semanticweb.org/ontologies/NELL#_:y30> ;
    rdfs:comment "the citizenship of a person"^^xsd:string ;
    rdfs:domain nell:country ;
    rdfs:range nell:person ;
    rdfs:subPropertyOf nell:locationrelatedtoagent .

nell:countryisthehomeofsportsteam rdfs:comment "Describes the home country of sports teams"^^xsd:string ;
    rdfs:domain nell:country ;
    rdfs:range nell:sportsteam ;
    rdfs:subPropertyOf nell:locationrelatedtoagent .

nell:countrylanguage rdfs:comment "Typical language spoken in a country (official or otherwise)"^^xsd:string ;
    rdfs:domain nell:country ;
    rdfs:range nell:language ;
    rdfs:subPropertyOf nell:relatedto .

nell:countryleadbyperson rdfs:comment "specifies that a particular person is the leader of a particular country"^^xsd:string ;
    rdfs:domain nell:country ;
    rdfs:range nell:politician ;
    rdfs:subPropertyOf nell:controlledbyagent,
        nell:locationrelatedtoagent,
        nell:proxyof .

nell:countrylocatedingeopoliticallocation rdfs:comment "specifies that a particular country is located in a particular geopolitical entity"^^xsd:string ;
    rdfs:domain nell:country ;
    rdfs:range nell:geopoliticallocation ;
    rdfs:subPropertyOf nell:locationlocatedwithinlocation .

nell:countryofpersonbirth rdfs:comment "the country that a person was born in"^^xsd:string ;
    rdfs:domain nell:country ;
    rdfs:range nell:person ;
    rdfs:subPropertyOf nell:locationofpersonbirth .

nell:countryofpersondeath rdfs:comment "the country that a person died in"^^xsd:string ;
    rdfs:domain nell:country ;
    rdfs:range nell:person ;
    rdfs:subPropertyOf nell:locationofpersondeath .

nell:countryproducesproduct rdfs:comment "Describes the products produced by a country"^^xsd:string ;
    rdfs:domain nell:country ;
    rdfs:range nell:product ;
    rdfs:subPropertyOf nell:locationofitemexistence .

nell:countryresidenceofperson rdfs:comment "the country that a person has residence in"^^xsd:string ;
    rdfs:domain nell:country ;
    rdfs:range nell:person ;
    rdfs:subPropertyOf nell:locationresidenceofperson .

nell:county rdfs:comment "Intermediate administrative region between state/province and local munincipal. This category also encompasses customary abberations such as the boroughs of the City of Greater New York being treated as logically equivalent to counties."^^xsd:string ;
    rdfs:subClassOf nell:geopoliticallocation,
        nell:geopoliticalorganization .

nell:creditunion rdfs:comment "Banks that are credit unions"^^xsd:string ;
    rdfs:subClassOf nell:company .

nell:crimeorchargeofperson rdfs:comment "Charges or crimes (alleged or convicted) of the given person"^^xsd:string ;
    rdfs:domain nell:crimeorcharge ;
    rdfs:range nell:person ;
    rdfs:subPropertyOf nell:eventhasparticipantagent .

nell:criminalarrestedincountry rdfs:comment "Country where criminal was arrested"^^xsd:string ;
    rdfs:domain nell:criminal ;
    rdfs:range nell:country ;
    rdfs:subPropertyOf nell:agentrelatedtolocation .

nell:criminalssuchascriminals rdfs:comment "Describes the criminals types that are generalizations of specific criminals"^^xsd:string ;
    rdfs:domain nell:criminal ;
    rdfs:range nell:criminal ;
    rdfs:subPropertyOf nell:generalizationof .

nell:crustaceanisatypeofarthropod rdfs:comment "Hyponym Relation"^^xsd:string ;
    rdfs:domain nell:arthropod ;
    rdfs:range nell:crustacean ;
    rdfs:subPropertyOf nell:specializationof .

nell:currencycountry a owl:InverseFunctionalProperty ;
    rdfs:comment "specifies that a particular country uses a particular currency"^^xsd:string ;
    rdfs:domain nell:currency ;
    rdfs:range nell:country ;
    rdfs:subPropertyOf nell:relatedto .

nell:damagedinbombing rdfs:domain nell:geolocatablething ;
    rdfs:range nell:bombingevent ;
    rdfs:subPropertyOf nell:relatedto .

nell:damagedinearthquake rdfs:domain nell:geolocatablething ;
    rdfs:range nell:earthquakeevent ;
    rdfs:subPropertyOf nell:relatedto .

nell:damagedinprotest rdfs:domain nell:geolocatablething ;
    rdfs:range nell:protestevent ;
    rdfs:subPropertyOf nell:relatedto .

nell:dateatwhichexistsitem rdfs:comment "a item exists in a determined time (or date)"^^xsd:string ;
    rdfs:domain nell:date ;
    rdfs:range nell:item ;
    rdfs:subPropertyOf nell:dateof .

nell:dateatwhichexistslocation rdfs:comment "Most general location-to-date relation. Note that locations are not eternal."^^xsd:string ;
    rdfs:domain nell:date ;
    rdfs:range nell:location ;
    rdfs:subPropertyOf nell:dateof .

nell:dateofevent rdfs:domain nell:date ;
    rdfs:range nell:event ;
    rdfs:subPropertyOf nell:relatedto .

nell:dateofmeetingeventtitle rdfs:comment "When a particular meeting will take place"^^xsd:string ;
    rdfs:domain nell:dateliteral ;
    rdfs:range nell:meetingeventtitle ;
    rdfs:subPropertyOf nell:dateevent .

nell:dateoforganizationcreation rdfs:comment "The date on which a given organization was founded"^^xsd:string ;
    rdfs:domain nell:date ;
    rdfs:range nell:organization ;
    rdfs:subPropertyOf nell:dateof .

nell:dateoforganzationdissolution rdfs:comment "The date on which a given organization was dissolved"^^xsd:string ;
    rdfs:domain nell:date ;
    rdfs:range nell:organization ;
    rdfs:subPropertyOf nell:dateof .

nell:dateofpersonbirth rdfs:comment "the date on which this person was born"^^xsd:string ;
    rdfs:domain nell:dateliteral ;
    rdfs:range nell:person ;
    rdfs:subPropertyOf nell:dateof .

nell:dateofpersondeath rdfs:comment "the date on which this person died"^^xsd:string ;
    rdfs:domain nell:dateliteral ;
    rdfs:range nell:person ;
    rdfs:subPropertyOf nell:dateof .

nell:dateofsportsgame rdfs:comment "the date on which this game occurred"^^xsd:string ;
    rdfs:domain nell:dateliteral ;
    rdfs:range nell:sportsgame ;
    rdfs:subPropertyOf nell:dateevent .

nell:dayofweek rdfs:comment "Seven named days of the week"^^xsd:string ;
    rdfs:subClassOf nell:date .

nell:deathageofperson rdfs:comment "the age at which this person died"^^xsd:string ;
    rdfs:domain nell:nonneginteger ;
    rdfs:range nell:person ;
    rdfs:subPropertyOf nell:relatedto .

nell:directordirectedmovie rdfs:comment "to direct a monvie"^^xsd:string ;
    rdfs:domain nell:director ;
    rdfs:range nell:movie ;
    rdfs:subPropertyOf nell:agentcontributedtocreativework .

nell:directorworkedwithactor rdfs:comment "Relates the actors and directors that at least once worked together"^^xsd:string ;
    rdfs:domain nell:director ;
    rdfs:range nell:actor ;
    rdfs:subPropertyOf nell:agentcollaborateswithagent .

nell:diseasecausesphysiologicalcondition rdfs:comment "Describes diseases that may cause a physiological condition"^^xsd:string ;
    rdfs:domain nell:disease ;
    rdfs:range nell:physiologicalcondition ;
    rdfs:subPropertyOf nell:relatedto .

nell:diseasemaybecausedbydrug rdfs:comment "Describes a disease that can be caused by a drug"^^xsd:string ;
    rdfs:domain nell:disease ;
    rdfs:range nell:drug ;
    rdfs:subPropertyOf nell:relatedto .

nell:drugexpectedreleasedate rdfs:comment "This predicate represents the relationship between a pharmaceutical substance and the date when it is expected to be approved for legal marketing. For our purposes the date will typically correspond to a date for FDA approval but the relationship itself is not restricted to approval for sale in the United States."^^xsd:string ;
    rdfs:domain nell:drug ;
    rdfs:range nell:date ;
    rdfs:subPropertyOf nell:atdate .

nell:drughassideeffect rdfs:comment "This predicate indicates that the use of a drug has a physiologicalCondition as a side-effect. Uses of this predicate may include both very common side-effects and rare but reported side-effects."^^xsd:string ;
    rdfs:domain nell:drug ;
    rdfs:range nell:physiologicalcondition ;
    rdfs:subPropertyOf nell:relatedto .

nell:drugpossiblytreatsphysiologicalcondition rdfs:comment "relates a substance to a condition that it might treat. This relation includes conditions that the substance has been designed or approved to treat as well as conditions for which it is being investigated as a possible treatment.  Common folk remedies would also be eligible for this relation.  For example it would be reasonable to say that \"chicken noodle soup\" is a possible treatment for \"colds\"."^^xsd:string ;
    rdfs:domain nell:drug ;
    rdfs:range nell:physiologicalcondition ;
    rdfs:subPropertyOf nell:relatedto .

nell:drugworkedonbyagent rdfs:comment "This predicate relates a substance and a HumanAgent who is responsible for it. Responsibility is understoond relatively broadly and includes people or organizations responsible for the substance's discovery or marketing and manufacturing.  Additionally agents that own the rights to the substance are also eligible to participate in this relationship.  Note that the humanAgent category include organizations including universities companies and government agencies."^^xsd:string ;
    rdfs:domain nell:drug ;
    rdfs:range nell:humanagent ;
    rdfs:subPropertyOf nell:iteminvolvedwithagent .

nell:earthquakecasualtiesnumber rdfs:domain nell:earthquakeevent ;
    rdfs:range nell:nonneginteger ;
    rdfs:subPropertyOf nell:relatedto .

nell:earthquakecomentedby rdfs:domain nell:earthquakeevent ;
    rdfs:range nell:person ;
    rdfs:subPropertyOf nell:relatedto .

nell:earthquakedamaged rdfs:domain nell:earthquakeevent ;
    rdfs:range nell:geolocatablething ;
    rdfs:subPropertyOf nell:relatedto .

nell:earthquakeeventtime rdfs:domain nell:earthquakeevent ;
    rdfs:range nell:time ;
    rdfs:subPropertyOf nell:relatedto .

nell:earthquakehadepicenter rdfs:domain nell:earthquakeevent ;
    rdfs:range nell:geolocatablething ;
    rdfs:subPropertyOf nell:relatedto .

nell:earthquakehadmagnitude rdfs:domain nell:earthquakeevent ;
    rdfs:range nell:everypromotedthing ;
    rdfs:subPropertyOf nell:relatedto .

nell:earthquakehadsource rdfs:domain nell:earthquakeevent ;
    rdfs:range nell:everypromotedthing ;
    rdfs:subPropertyOf nell:relatedto .

nell:earthquakehadvictim rdfs:domain nell:earthquakeevent ;
    rdfs:range nell:victim ;
    rdfs:subPropertyOf nell:relatedto .

nell:earthquakeinjured rdfs:domain nell:earthquakeevent ;
    rdfs:range nell:victim ;
    rdfs:subPropertyOf nell:relatedto .

nell:earthquakeinjurednumber rdfs:domain nell:earthquakeevent ;
    rdfs:range nell:nonneginteger ;
    rdfs:subPropertyOf nell:relatedto .

nell:earthquakeocurredin rdfs:domain nell:earthquakeevent ;
    rdfs:range nell:location ;
    rdfs:subPropertyOf nell:relatedto .

nell:economicsectorcompany rdfs:comment "specifies that a particular company does business in a particular economic sector"^^xsd:string ;
    rdfs:domain nell:economicsector ;
    rdfs:range nell:company ;
    rdfs:subPropertyOf nell:relatedto .

nell:economicsectorhasperson rdfs:comment "People who work in a given economic sector"^^xsd:string ;
    rdfs:domain nell:economicsector ;
    rdfs:range nell:person ;
    rdfs:subPropertyOf nell:relatedto .

nell:economicsectorusingacademicfield rdfs:comment "Academic fields used by economic fields"^^xsd:string ;
    rdfs:domain nell:economicsector ;
    rdfs:range nell:academicfield ;
    rdfs:subPropertyOf nell:relatedto .

nell:election rdfs:comment "An opportunity for constituents to vote for a political party or candidate for a governmental office or seat or the ability to run for a governmental office or seat (as is the case with primaries). (FreeBase)"^^xsd:string ;
    rdfs:subClassOf nell:event .

nell:emotionassociatedwithdisease rdfs:comment "Describes the emotions associated with a disease"^^xsd:string ;
    rdfs:domain nell:emotion ;
    rdfs:range nell:disease ;
    rdfs:subPropertyOf nell:relatedto .

nell:epicenterofearthquake rdfs:domain nell:geolocatablething ;
    rdfs:range nell:earthquakeevent ;
    rdfs:subPropertyOf nell:relatedto .

nell:equipmentusedbysport rdfs:comment "Specifies equipment that is used by a particular sport."^^xsd:string ;
    rdfs:domain nell:sportsequipment ;
    rdfs:range nell:sport ;
    rdfs:subPropertyOf nell:relatedto .

nell:ethnicgroupofperson rdfs:comment "The ethnicity of a person"^^xsd:string ;
    rdfs:domain nell:ethnicgroup ;
    rdfs:range nell:person ;
    rdfs:subPropertyOf nell:relatedto .

nell:eventcausedbyagent rdfs:comment "Companion to agentParticipatedInEvent. Note that one needn't participate in an event in order to be a causal factor."^^xsd:string ;
    rdfs:domain nell:event ;
    rdfs:range nell:agent ;
    rdfs:subPropertyOf nell:createdbyagent .

nell:eventcausedbyevent rdfs:comment "Any events that is caused by another event"^^xsd:string ;
    rdfs:domain nell:event ;
    rdfs:range nell:event ;
    rdfs:subPropertyOf nell:relatedto .

nell:eventcausedevent rdfs:comment "Any events that is caused by another event"^^xsd:string ;
    rdfs:domain nell:event ;
    rdfs:range nell:event ;
    rdfs:subPropertyOf nell:relatedto .

nell:eventinvolveditem rdfs:comment "Umbrella relation for identifying items in events."^^xsd:string ;
    rdfs:domain nell:event ;
    rdfs:range nell:item ;
    rdfs:subPropertyOf nell:superpartof .

nell:eventoutcome rdfs:comment "a final product or end result; consequence; issue "^^xsd:string ;
    rdfs:subClassOf nell:event .

nell:eventsubeventof rdfs:comment "event that is happened as a sub-event of another event"^^xsd:string ;
    rdfs:domain nell:event ;
    rdfs:range nell:event ;
    rdfs:subPropertyOf nell:subpartof .

nell:eventsupereventof rdfs:comment "event that is happened as a sub-event of another event"^^xsd:string ;
    rdfs:domain nell:event ;
    rdfs:range nell:event ;
    rdfs:subPropertyOf nell:superpartof .

nell:explosivesinbombing rdfs:domain nell:chemical ;
    rdfs:range nell:bombingevent ;
    rdfs:subPropertyOf nell:relatedto .

nell:farmlocatedincountry rdfs:comment "The country a farm is located in"^^xsd:string ;
    rdfs:domain nell:farm ;
    rdfs:range nell:country ;
    rdfs:subPropertyOf nell:locationlocatedwithinlocation .

nell:farmlocatedinstate rdfs:comment "The state/province a farm is located in"^^xsd:string ;
    rdfs:domain nell:farm ;
    rdfs:range nell:stateorprovince ;
    rdfs:subPropertyOf nell:locationlocatedwithinlocation .

nell:farmproducesagriculturalproduct rdfs:comment "the agricultural products produced by a farm"^^xsd:string ;
    rdfs:domain nell:farm ;
    rdfs:range nell:agriculturalproduct ;
    rdfs:subPropertyOf nell:locationofitemexistence .

nell:femalecanbethesameascomedian rdfs:comment "Describes two instances that are the same thing in these two different categories"^^xsd:string ;
    rdfs:domain nell:female ;
    rdfs:range nell:comedian ;
    rdfs:subPropertyOf nell:canbethesameas .

nell:filmfestival rdfs:comment "Film festivals at which movies are shown."^^xsd:string ;
    rdfs:subClassOf nell:event .

nell:fishservedwithfood rdfs:comment "Describes the kind of food that are tipically serverd with a fish"^^xsd:string ;
    rdfs:domain nell:fish ;
    rdfs:range nell:food ;
    rdfs:subPropertyOf nell:relatedto .

nell:flooritem rdfs:comment "Any item that is commonly found on the floor"^^xsd:string ;
    rdfs:subClassOf nell:householditem .

nell:foodcancausedisease rdfs:comment "Describes the diseases that can be caused by a food"^^xsd:string ;
    rdfs:domain nell:food ;
    rdfs:range nell:disease ;
    rdfs:subPropertyOf nell:relatedto .

nell:fooddecreasestheriskofdisease rdfs:comment "Describes the foods that can reduce the risks of having a disease"^^xsd:string ;
    rdfs:domain nell:food ;
    rdfs:range nell:disease ;
    rdfs:subPropertyOf nell:relatedto .

nell:fungus rdfs:comment "Member of kingom fungi."^^xsd:string ;
    rdfs:subClassOf nell:item,
        nell:species .

nell:furniturefoundinroom rdfs:comment "Relates furniture to rooms in which it is often found"^^xsd:string ;
    rdfs:domain nell:furniture ;
    rdfs:range nell:room ;
    rdfs:subPropertyOf nell:itemfoundinroom .

nell:geopoliticallocationcontainscountry rdf:first <http://www.semanticweb.org/ontologies/NELL#_:y11>,
        <http://www.semanticweb.org/ontologies/NELL#_:y29>,
        <http://www.semanticweb.org/ontologies/NELL#_:y39>,
        <http://www.semanticweb.org/ontologies/NELL#_:y7> ;
    rdfs:comment "specifies that a particular country is located in a particular geopolitical entity"^^xsd:string ;
    rdfs:domain nell:geopoliticallocation ;
    rdfs:range nell:country ;
    rdfs:subPropertyOf nell:locationcontainslocation .

nell:governmentorganization rdfs:comment "A government is the organization or agency through which a political unit exercises its authority "^^xsd:string ;
    rdfs:subClassOf nell:politicsgroup .

nell:grainusedtomakecandy rdfs:comment "grain and candy are related"^^xsd:string ;
    rdfs:domain nell:grain ;
    rdfs:range nell:candy ;
    rdfs:subPropertyOf nell:relatedto .

nell:grandprix rdfs:comment "one of several international races."^^xsd:string ;
    rdfs:subClassOf nell:sportsevent .

nell:guiltyofroadaccident rdfs:domain nell:person ;
    rdfs:range nell:roadaccidentevent ;
    rdfs:subPropertyOf nell:relatedto .

nell:hallwayitem rdfs:comment "Any item that is commonly found in a hallway."^^xsd:string ;
    rdfs:subClassOf nell:householditem .

nell:hasbrother rdfs:comment "person has a brother"^^xsd:string ;
    rdfs:domain nell:person ;
    rdfs:range nell:male ;
    rdfs:subPropertyOf nell:hassibling .

nell:hashusband rdfs:comment "person has a husband"^^xsd:string ;
    rdfs:domain nell:person ;
    rdfs:range nell:male ;
    rdfs:subPropertyOf nell:hasspouse .

nell:hassister rdfs:comment "person has a sister"^^xsd:string ;
    rdfs:domain nell:person ;
    rdfs:range nell:female ;
    rdfs:subPropertyOf nell:hassibling .

nell:hasvisualappearance rdfs:comment "The NEIL-learned visual appearance of something"^^xsd:string ;
    rdfs:domain nell:visualizablething ;
    rdfs:range nell:url ;
    rdfs:subPropertyOf nell:atlocation .

nell:haswife rdfs:comment "person has a wife"^^xsd:string ;
    rdfs:domain nell:person ;
    rdfs:range nell:female ;
    rdfs:subPropertyOf nell:hasspouse .

nell:haswikipediaurl rdfs:comment "The Wikipedia page for a given category instance"^^xsd:string ;
    rdfs:domain nell:everypromotedthing ;
    rdfs:range nell:url ;
    rdfs:subPropertyOf nell:atlocation .

nell:headquarteredin rdfs:comment "specifies that a particular company is headquartered in a particular city"^^xsd:string ;
    rdfs:domain nell:company ;
    rdfs:range nell:city ;
    rdfs:subPropertyOf nell:hasofficeincity,
        nell:organizationheadquarteredincity .

nell:highschool rdfs:comment "Schools whose graduates would go directly on to universities vocational schools or other higher education.  No particular limit on age of incoming students."^^xsd:string ;
    rdfs:subClassOf nell:school .

nell:highway rdfs:comment "is a public road especially a major road connecting two or more destinations."^^xsd:string ;
    rdfs:subClassOf nell:location .

nell:hobbiessuchashobbies a owl:AsymmetricProperty,
        owl:IrreflexiveProperty ;
    rdfs:comment "Describes the hobbies types that are generalizations of specific hobbies"^^xsd:string ;
    rdfs:domain nell:hobby ;
    rdfs:range nell:hobby ;
    rdfs:subPropertyOf nell:generalizationof .

nell:hometeamingame rdfs:comment "Specifies that a particular team is the home team in a particular sportsGame"^^xsd:string ;
    rdfs:domain nell:sportsteam ;
    rdfs:range nell:sportsgame ;
    rdfs:subPropertyOf nell:teamingame .

nell:hospitalincity rdfs:comment "The city a hostpital is located in."^^xsd:string ;
    rdfs:domain nell:hospital ;
    rdfs:range nell:city ;
    rdfs:subPropertyOf nell:buildinglocatedincity .

nell:hotelbuiltatpark rdfs:comment "hotel and park are related"^^xsd:string ;
    rdfs:domain nell:hotel ;
    rdfs:range nell:park ;
    rdfs:subPropertyOf nell:relatedto .

nell:hotelincity rdfs:comment "The city a hotel is located in."^^xsd:string ;
    rdfs:domain nell:hotel ;
    rdfs:range nell:city ;
    rdfs:subPropertyOf nell:buildinglocatedincity .

nell:hotelwasbuiltatfarm rdfs:comment "Describes hotels built at farms"^^xsd:string ;
    rdfs:domain nell:hotel ;
    rdfs:range nell:farm ;
    rdfs:subPropertyOf nell:locationlocatedwithinlocation .

nell:husbandof rdfs:comment "person has a husband"^^xsd:string ;
    rdfs:domain nell:male ;
    rdfs:range nell:person ;
    rdfs:subPropertyOf nell:hasspouse .

nell:injuredinbombing rdfs:domain nell:person ;
    rdfs:range nell:bombingevent ;
    rdfs:subPropertyOf nell:relatedto .

nell:injuredinearthquake rdfs:domain nell:victim ;
    rdfs:range nell:earthquakeevent ;
    rdfs:subPropertyOf nell:relatedto .

nell:injuredinprotest rdfs:domain nell:person ;
    rdfs:range nell:protestevent ;
    rdfs:subPropertyOf nell:relatedto .

nell:injuredinroadaccident rdfs:domain nell:person ;
    rdfs:range nell:roadaccidentevent ;
    rdfs:subPropertyOf nell:relatedto .

nell:insectcanbeconfundedwitharthropod rdfs:comment "Arthropodes that usually are confunded by insects"^^xsd:string ;
    rdfs:domain nell:insect ;
    rdfs:range nell:arthropod ;
    rdfs:subPropertyOf nell:relatedto .

nell:insecteatsgrain rdfs:comment "Describes the grains eaten by an insect"^^xsd:string ;
    rdfs:domain nell:insect ;
    rdfs:range nell:grain ;
    rdfs:subPropertyOf nell:animaleatfood .

nell:instrumentplayedbymusician rdfs:comment "Specifies that a musical instrument is played by a paritcular musician"^^xsd:string ;
    rdfs:domain nell:musicinstrument ;
    rdfs:range nell:musician ;
    rdfs:subPropertyOf nell:iteminvolvedwithagent .

nell:inverseofacademicfieldsuchasacademicfield rdfs:comment "Describes a specialization fo an Academic Field"^^xsd:string ;
    rdfs:domain nell:academicfield ;
    rdfs:range nell:academicfield ;
    rdfs:subPropertyOf nell:specializationof .

nell:inverseofactorsuchasactor rdfs:comment "Describes the actor types that are generalizations of specific actors"^^xsd:string ;
    rdfs:domain nell:actor ;
    rdfs:range nell:actor ;
    rdfs:subPropertyOf nell:specializationof .

nell:inverseofagriculturalproductcamefromcountry rdfs:comment "Describes the agricultural products that came from a country"^^xsd:string ;
    rdfs:domain nell:country ;
    rdfs:range nell:agriculturalproduct ;
    rdfs:subPropertyOf nell:locationofitemexistence .

nell:inverseofagriculturalproductcomingfromvertebrate rdfs:comment "Describes the agricultural products that come from a vertebrate"^^xsd:string ;
    rdfs:domain nell:vertebrate ;
    rdfs:range nell:agriculturalproduct ;
    rdfs:subPropertyOf nell:relatedto .

nell:inverseofagriculturalproductcontainchemical rdfs:comment "Describes the agricultural products that contain a chemical"^^xsd:string ;
    rdfs:domain nell:chemical ;
    rdfs:range nell:agriculturalproduct ;
    rdfs:subPropertyOf nell:relatedto .

nell:inverseofagriculturalproductcookedwithagricultureproduct rdfs:comment "Describes the agricultural products that are usually cooked with another agricultural product"^^xsd:string ;
    rdfs:domain nell:agriculturalproduct ;
    rdfs:range nell:agriculturalproduct ;
    rdfs:subPropertyOf nell:relatedto .

nell:inverseofagriculturalproductcutintogeometricshape rdfs:comment "Describes the agricultural products that are usually cut into geometric shapes"^^xsd:string ;
    rdfs:domain nell:geometricshape ;
    rdfs:range nell:agriculturalproduct ;
    rdfs:subPropertyOf nell:relatedto .

nell:inverseofagriculturalproductgrowinginstateorprovince rdfs:comment "Describes the agricultural products that are produced in a state or province"^^xsd:string ;
    rdfs:domain nell:stateorprovince ;
    rdfs:range nell:agriculturalproduct ;
    rdfs:subPropertyOf nell:locationofitemexistence .

nell:inverseofagriculturalproductgrowninlandscapefeature rdfs:comment "Describes the agricultural products that are grown in landscape features"^^xsd:string ;
    rdfs:domain nell:landscapefeatures ;
    rdfs:range nell:agriculturalproduct ;
    rdfs:subPropertyOf nell:relatedto .

nell:inverseofagriculturalproductincludingagriculturalproduct rdfs:comment "Describes the agricultural products that are generalizations of other agriculture products"^^xsd:string ;
    rdfs:domain nell:agriculturalproduct ;
    rdfs:range nell:agriculturalproduct ;
    rdfs:subPropertyOf nell:specializationof .

nell:inverseofagriculturalproducttoattractinsect rdfs:comment "Describes the agricultural products that attract insects"^^xsd:string ;
    rdfs:domain nell:insect ;
    rdfs:range nell:agriculturalproduct ;
    rdfs:subPropertyOf nell:relatedto .

nell:inverseofamphibiansuchasamphibian rdfs:comment "Describes the amphibian types that are generalizations of specific amphibians"^^xsd:string ;
    rdfs:domain nell:amphibian ;
    rdfs:range nell:amphibian ;
    rdfs:subPropertyOf nell:specializationof .

nell:inverseofanimaldevelopdisease rdfs:comment "Describes the diseases that can be developed by an animal"^^xsd:string ;
    rdfs:domain nell:disease ;
    rdfs:range nell:animal ;
    rdfs:subPropertyOf nell:relatedto .

nell:inverseofanimaleatvegetable rdfs:comment "Describes the vegetables eaten by an animal"^^xsd:string ;
    rdfs:domain nell:vegetable ;
    rdfs:range nell:animal ;
    rdfs:subPropertyOf nell:inverseofanimaleatfood .

nell:inverseofanimalssuchasmammals rdfs:comment "Describes the animal types that are generalizations of mammals"^^xsd:string ;
    rdfs:domain nell:mammal ;
    rdfs:range nell:animal ;
    rdfs:subPropertyOf nell:specializationof .

nell:inverseofanimalsuchasfish rdfs:comment "Describes the fish that are from a specific type of animals"^^xsd:string ;
    rdfs:domain nell:fish ;
    rdfs:range nell:animal ;
    rdfs:subPropertyOf nell:animalistypeofanimal .

nell:inverseofanimalsuchasinsect rdfs:comment "Describes the insect that are from a specific type of animals"^^xsd:string ;
    rdfs:domain nell:insect ;
    rdfs:range nell:animal ;
    rdfs:subPropertyOf nell:inverseofanimalsuchasinvertebrate .

nell:inverseofanimalsuchasmollusk rdfs:comment "Describes the mollusk that are from a specific type of animals"^^xsd:string ;
    rdfs:domain nell:mollusk ;
    rdfs:range nell:animal ;
    rdfs:subPropertyOf nell:inverseofanimalsuchasinvertebrate .

nell:inverseofaquariumsuchasaquarium rdfs:comment "Describes the specific aquarium types that are generalizations of aquariums"^^xsd:string ;
    rdfs:domain nell:aquarium ;
    rdfs:range nell:aquarium ;
    rdfs:subPropertyOf nell:specializationof .

nell:inverseofarachnidiseatenbybird rdfs:comment "Describes arachnids that are hunted and eaten by this bird"^^xsd:string ;
    rdfs:domain nell:bird ;
    rdfs:range nell:arachnid ;
    rdfs:subPropertyOf nell:animalpredators .

nell:inverseofarachnidssuchasarachnides rdfs:comment "Describes the specific arachnid types that are generalizations of arachnids"^^xsd:string ;
    rdfs:domain nell:arachnid ;
    rdfs:range nell:arachnid ;
    rdfs:subPropertyOf nell:specializationof .

nell:inverseofarchaeasuchasarchaea rdfs:comment "Describes the specific archaea types that are generalizations of archaeas"^^xsd:string ;
    rdfs:domain nell:archaea ;
    rdfs:range nell:archaea ;
    rdfs:subPropertyOf nell:specializationof .

nell:inverseofarchitectssuchasarchitects rdfs:comment "Describes the specific architect types that are generalizations of architects"^^xsd:string ;
    rdfs:domain nell:architect ;
    rdfs:range nell:architect ;
    rdfs:subPropertyOf nell:specializationof .

nell:inverseofarteryarisesfromartery rdfs:comment "Describes the arteries that arises from other arteries"^^xsd:string ;
    rdfs:domain nell:artery ;
    rdfs:range nell:artery ;
    rdfs:subPropertyOf nell:relatedto .

nell:inverseofarterycalledartery rdfs:comment "Describes the names an artery can be called"^^xsd:string ;
    rdfs:domain nell:artery ;
    rdfs:range nell:artery ;
    rdfs:subPropertyOf nell:relatedto .

nell:inverseofarterysuchasartery rdfs:comment "Describes the specific artery types that are generalizations of arteries"^^xsd:string ;
    rdfs:domain nell:artery ;
    rdfs:range nell:artery ;
    rdfs:subPropertyOf nell:specializationof .

nell:inverseofarthropodandotherarthropod rdfs:comment "Describes similar arthropods"^^xsd:string ;
    rdfs:domain nell:arthropod ;
    rdfs:range nell:arthropod ;
    rdfs:subPropertyOf nell:animaltypehasanimal .

nell:inverseofarthropodcalledarthropod a owl:IrreflexiveProperty ;
    rdfs:comment "Describes the names an artery can be called"^^xsd:string ;
    rdfs:domain nell:arthropod ;
    rdfs:range nell:arthropod ;
    rdfs:subPropertyOf nell:synonymfor .

nell:inverseofarthropodfeedoninsect rdfs:comment "Describes the names an artery can be called"^^xsd:string ;
    rdfs:domain nell:insect ;
    rdfs:range nell:arthropod ;
    rdfs:subPropertyOf nell:relatedto .

nell:inverseofarthropodlooklikeinsect rdfs:comment "Describes the arthropod that look like specific insects"^^xsd:string ;
    rdfs:domain nell:insect ;
    rdfs:range nell:arthropod ;
    rdfs:subPropertyOf nell:relatedto .

nell:inverseofastronautsuchasastronaut rdfs:comment "Describes the specific astronaut types that are generalizations of astronauts"^^xsd:string ;
    rdfs:domain nell:astronaut ;
    rdfs:range nell:astronaut ;
    rdfs:subPropertyOf nell:specializationof .

nell:inverseofastronautwasonamissionwithastronaut rdfs:comment "Describes astronauts that were at a space mission togheter"^^xsd:string ;
    rdfs:domain nell:astronaut ;
    rdfs:range nell:astronaut ;
    rdfs:subPropertyOf nell:relatedto .

nell:inverseofathletebeatathlete rdfs:comment "Describes the athletes whom beat other athletes"^^xsd:string ;
    rdfs:domain nell:athlete ;
    rdfs:range nell:athlete ;
    rdfs:subPropertyOf nell:relatedto .

nell:inverseofathletefracturedbone rdfs:comment "Bone fracture that an athlete had"^^xsd:string ;
    rdfs:domain nell:bone ;
    rdfs:range nell:athlete ;
    rdfs:subPropertyOf nell:inverseofathleteinjuredhisbodypart .

nell:inverseofathleteledsportsteam rdfs:comment "Describes the athletes that lead/led a sports team"^^xsd:string ;
    rdfs:domain nell:sportsteam ;
    rdfs:range nell:athlete ;
    rdfs:subPropertyOf nell:teammember .

nell:inverseofathleteplayedforschool rdfs:comment "The school that an athlete used to play for its team"^^xsd:string ;
    rdfs:domain nell:school ;
    rdfs:range nell:athlete ;
    rdfs:subPropertyOf nell:organizationhasperson .

nell:inverseofathletepublishesinblog rdfs:comment "The blog where an athlete publishes"^^xsd:string ;
    rdfs:domain nell:blog ;
    rdfs:range nell:athlete ;
    rdfs:subPropertyOf nell:relatedto .

nell:inverseofathletesuchasathlete rdfs:comment "Describes the specific athlete types that are generalizations of athletes"^^xsd:string ;
    rdfs:domain nell:athlete ;
    rdfs:range nell:athlete ;
    rdfs:subPropertyOf nell:specializationof .

nell:inverseofathletewinsawardtrophytournament rdfs:comment "Describes the athletes who won an award trophy tournament"^^xsd:string ;
    rdfs:domain nell:awardtrophytournament ;
    rdfs:range nell:athlete ;
    rdfs:subPropertyOf nell:relatedto .

nell:inverseofattractionmadeofbuildingmaterial rdfs:comment "Describes the materials used to build attractions"^^xsd:string ;
    rdfs:domain nell:buildingmaterial ;
    rdfs:range nell:attraction ;
    rdfs:subPropertyOf nell:relatedto .

nell:inverseofautomobileenginesuchasautomobileengine rdfs:comment "Describes the specific automobile Engine types that are generalizations of automobile Engines"^^xsd:string ;
    rdfs:domain nell:automobileengine ;
    rdfs:range nell:automobileengine ;
    rdfs:subPropertyOf nell:specializationof .

nell:inverseofautomobilemakercardealersinstateorprovince rdfs:comment "Describes the car dealers in a state or province"^^xsd:string ;
    rdfs:domain nell:stateorprovince ;
    rdfs:range nell:automobilemaker ;
    rdfs:subPropertyOf nell:relatedto .

nell:inverseofautomobilemakerchiefexecutiveceo rdfs:comment "Describes the CEOs of automobile maker companies"^^xsd:string ;
    rdfs:domain nell:ceo ;
    rdfs:range nell:automobilemaker ;
    rdfs:subPropertyOf nell:ceoof .

nell:inverseofautomobilemakerdealersincity rdfs:comment "Describes the car dealers in a city"^^xsd:string ;
    rdfs:domain nell:city ;
    rdfs:range nell:automobilemaker ;
    rdfs:subPropertyOf nell:cityhascompanyoffice .

nell:inverseofautomobilemakerdealersincountry rdfs:comment "Describes the car dealers in a country"^^xsd:string ;
    rdfs:domain nell:country ;
    rdfs:range nell:automobilemaker ;
    rdfs:subPropertyOf nell:countryhascompanyoffice .

nell:inverseofawardtrophytournamentisthechampionshipgameofthenationalsport rdfs:comment "Describes award trophy tournaments related to specific sports"^^xsd:string ;
    rdfs:domain nell:sport ;
    rdfs:range nell:awardtrophytournament ;
    rdfs:subPropertyOf nell:relatedto .

nell:inverseofawardtrophytournamentwasawardedonstadium rdfs:comment "Stadium of event venue where a award trophy tournament was at least once awarded"^^xsd:string ;
    rdfs:domain nell:stadiumoreventvenue ;
    rdfs:range nell:awardtrophytournament ;
    rdfs:subPropertyOf nell:locatedat .

nell:inverseofbacteriacancauseillnessfromfood rdfs:comment "Describes the foods that bacterias can cause illness from"^^xsd:string ;
    rdfs:domain nell:food ;
    rdfs:range nell:bacteria ;
    rdfs:subPropertyOf nell:relatedto .

nell:inverseofbacteriaisthecausativeagentofphysiologicalcondition rdfs:comment "Describes the bacterias that causes physiological conditions"^^xsd:string ;
    rdfs:domain nell:physiologicalcondition ;
    rdfs:range nell:bacteria ;
    rdfs:subPropertyOf nell:relatedto .

nell:inverseofbakedgoodservedwithbeverage rdfs:comment "Describes the baked goods that are usually served with a beverage"^^xsd:string ;
    rdfs:domain nell:beverage ;
    rdfs:range nell:bakedgood ;
    rdfs:subPropertyOf nell:itemusedwithitem .

nell:inverseofbakegoodistypicalincountry rdfs:comment "Describes the typicall bakegoods of the countries"^^xsd:string ;
    rdfs:domain nell:country ;
    rdfs:range nell:bakedgood ;
    rdfs:subPropertyOf nell:relatedto .

nell:inverseofbankbankincountry rdfs:comment "Describes the banks in a country"^^xsd:string ;
    rdfs:domain nell:country ;
    rdfs:range nell:bank ;
    rdfs:subPropertyOf nell:countryhascompanyoffice .

nell:inverseofbankboughtbank rdfs:comment "Describes the banks that bought other banks"^^xsd:string ;
    rdfs:domain nell:bank ;
    rdfs:range nell:bank ;
    rdfs:subPropertyOf nell:acquiredby .

nell:inverseofbankchiefexecutiveceo rdfs:comment "Describes the CEOs of banks"^^xsd:string ;
    rdfs:domain nell:ceo ;
    rdfs:range nell:bank ;
    rdfs:subPropertyOf nell:ceoof .

nell:inverseofbeveragecansoftendisease rdfs:comment "Describes beverages that can help soften the symptons of diseases"^^xsd:string ;
    rdfs:domain nell:disease ;
    rdfs:range nell:beverage ;
    rdfs:subPropertyOf nell:relatedto .

nell:inverseofbeveragecontainsprotein rdfs:comment "Describes the proteins contained in beverages"^^xsd:string ;
    rdfs:domain nell:protein ;
    rdfs:range nell:beverage ;
    rdfs:subPropertyOf nell:relatedto .

nell:inverseofbeveragemadefrombeverage rdfs:comment "Describes the names an artery can be called"^^xsd:string ;
    rdfs:domain nell:beverage ;
    rdfs:range nell:beverage ;
    rdfs:subPropertyOf nell:relatedto .

nell:inverseofbirdmayconsumeprotein rdfs:comment "Describes the proteins eaten by a bird"^^xsd:string ;
    rdfs:domain nell:protein ;
    rdfs:range nell:bird ;
    rdfs:subPropertyOf nell:relatedto .

nell:inverseofbooksuchasbook rdfs:comment "Describes the specific book types that are generalizations of actors"^^xsd:string ;
    rdfs:domain nell:book ;
    rdfs:range nell:book ;
    rdfs:subPropertyOf nell:specializationof .

nell:inverseofbuildingfeaturebuiltabovelak rdfs:comment "buildingfeature and lake are related"^^xsd:string ;
    rdfs:domain nell:lake ;
    rdfs:range nell:buildingfeature ;
    rdfs:subPropertyOf nell:relatedto .

nell:inverseofbuildingfeaturemadefrombuildingmaterial rdfs:comment "Describes the building features that are made of a building material"^^xsd:string ;
    rdfs:domain nell:buildingmaterial ;
    rdfs:range nell:buildingfeature ;
    rdfs:subPropertyOf nell:relatedto .

nell:inverseofbuildingispartofuniversity rdfs:comment "Describes buildings that universities might own"^^xsd:string ;
    rdfs:domain nell:university ;
    rdfs:range nell:building ;
    rdfs:subPropertyOf nell:relatedto .

nell:inverseofcelebritysuchascelebrity rdfs:comment "Describes the specific celebrity types that are generalizations of celebrities"^^xsd:string ;
    rdfs:domain nell:celebrity ;
    rdfs:range nell:celebrity ;
    rdfs:subPropertyOf nell:specializationof .

nell:inverseofclothingmadefromplant rdfs:comment "Describes the clothing items made of a plant"^^xsd:string ;
    rdfs:domain nell:plant ;
    rdfs:range nell:clothing ;
    rdfs:subPropertyOf nell:relatedto .

nell:inverseofclothmadeofplant rdfs:comment "Plants that can be used to make cloths"^^xsd:string ;
    rdfs:domain nell:plant ;
    rdfs:range nell:clothing ;
    rdfs:subPropertyOf nell:relatedto .

nell:inverseofcoachcanspeaklanguage rdfs:comment "Describes the languages that coaches might speak"^^xsd:string ;
    rdfs:domain nell:language ;
    rdfs:range nell:coach ;
    rdfs:subPropertyOf nell:relatedto .

nell:inverseofcoachstudiedatuniversity rdfs:comment "Describes the university where the coach studied at"^^xsd:string ;
    rdfs:domain nell:university ;
    rdfs:range nell:coach ;
    rdfs:subPropertyOf nell:relatedto .

nell:inverseofcoachworksincountry rdfs:comment "Describes the country where a coach works"^^xsd:string ;
    rdfs:domain nell:country ;
    rdfs:range nell:coach ;
    rdfs:subPropertyOf nell:locationactedinbyagent .

nell:inverseofcolorassociatedwithvisualizableattribut rdfs:comment "color and visualizableattribute are related"^^xsd:string ;
    rdfs:domain nell:visualizableattribute ;
    rdfs:range nell:color ;
    rdfs:subPropertyOf nell:relatedto .

nell:inverseofcompanyproducesvideogamesystem rdfs:comment "company produces a video game system"^^xsd:string ;
    rdfs:domain nell:videogamesystem ;
    rdfs:range nell:company ;
    rdfs:subPropertyOf nell:relatedto .

nell:inverseofconferencessuchasconferences rdfs:comment "Describes the conferences types that are generalizations of specific conferences"^^xsd:string ;
    rdfs:domain nell:conference ;
    rdfs:range nell:conference ;
    rdfs:subPropertyOf nell:specializationof .

nell:inverseofcountriessuchascountries rdfs:comment "Describes the countries types that are generalizations of specific countries"^^xsd:string ;
    rdfs:domain nell:country ;
    rdfs:range nell:country ;
    rdfs:subPropertyOf nell:specializationof .

nell:inverseofcountryisthehomeofsportsteam rdfs:comment "Describes the home country of sports teams"^^xsd:string ;
    rdfs:domain nell:sportsteam ;
    rdfs:range nell:country ;
    rdfs:subPropertyOf nell:agentrelatedtolocation .

nell:inverseofcriminalarrestedincountry rdfs:comment "Country where criminal was arrested"^^xsd:string ;
    rdfs:domain nell:country ;
    rdfs:range nell:criminal ;
    rdfs:subPropertyOf nell:locationrelatedtoagent .

nell:inverseofcriminalssuchascriminals rdfs:comment "Describes the criminals types that are generalizations of specific criminals"^^xsd:string ;
    rdfs:domain nell:criminal ;
    rdfs:range nell:criminal ;
    rdfs:subPropertyOf nell:specializationof .

nell:inverseofdateofevent rdfs:domain nell:event ;
    rdfs:range nell:date ;
    rdfs:subPropertyOf nell:relatedto .

nell:inverseofdiseasecausesphysiologicalcondition rdfs:comment "Describes diseases that may cause a physiological condition"^^xsd:string ;
    rdfs:domain nell:physiologicalcondition ;
    rdfs:range nell:disease ;
    rdfs:subPropertyOf nell:relatedto .

nell:inverseofdiseasemaybecausedbydrug rdfs:comment "Describes a disease that can be caused by a drug"^^xsd:string ;
    rdfs:domain nell:drug ;
    rdfs:range nell:disease ;
    rdfs:subPropertyOf nell:relatedto .

nell:inverseofemotionassocietedwithdisease rdfs:comment "Describes the emotions associated with a disease"^^xsd:string ;
    rdfs:domain nell:disease ;
    rdfs:range nell:emotion ;
    rdfs:subPropertyOf nell:relatedto .

nell:inverseoffishservedwithfood rdfs:comment "Describes the kind of food that are tipically serverd with a fish"^^xsd:string ;
    rdfs:domain nell:food ;
    rdfs:range nell:fish ;
    rdfs:subPropertyOf nell:relatedto .

nell:inverseoffoodcancausedisease rdfs:comment "Describes the diseases that can be caused by a food"^^xsd:string ;
    rdfs:domain nell:disease ;
    rdfs:range nell:food ;
    rdfs:subPropertyOf nell:relatedto .

nell:inverseoffooddecreasestheriskofdisease rdfs:comment "Describes the foods that can reduce the risks of having a disease"^^xsd:string ;
    rdfs:domain nell:disease ;
    rdfs:range nell:food ;
    rdfs:subPropertyOf nell:relatedto .

nell:inverseofgrainusedtomakecandy rdfs:comment "grain and candy are related"^^xsd:string ;
    rdfs:domain nell:candy ;
    rdfs:range nell:grain ;
    rdfs:subPropertyOf nell:relatedto .

nell:inverseofhobbiessuchashobbies rdfs:comment "Describes the hobbies types that are generalizations of specific hobbies"^^xsd:string ;
    rdfs:domain nell:hobby ;
    rdfs:range nell:hobby ;
    rdfs:subPropertyOf nell:specializationof .

nell:inverseofhotelbuiltatpark rdfs:comment "hotel and park are related"^^xsd:string ;
    rdfs:domain nell:park ;
    rdfs:range nell:hotel ;
    rdfs:subPropertyOf nell:relatedto .

nell:inverseofhotelwasbuiltatfarm rdfs:comment "Describes hotels built at farms"^^xsd:string ;
    rdfs:domain nell:farm ;
    rdfs:range nell:hotel ;
    rdfs:subPropertyOf nell:locationcontainslocation .

nell:inverseofinsecteatsgrain rdfs:comment "Describes the grains eaten by an insect"^^xsd:string ;
    rdfs:domain nell:grain ;
    rdfs:range nell:insect ;
    rdfs:subPropertyOf nell:inverseofanimaleatfood .

nell:inverseofinvertebratefeedonfood rdfs:comment "Describes the foods that are eaten by an invertebrate"^^xsd:string ;
    rdfs:domain nell:food ;
    rdfs:range nell:invertebrate ;
    rdfs:subPropertyOf nell:inverseofanimaleatfood .

nell:inverseofinvertebratehascolor rdfs:comment "Describes the color of invertebrates"^^xsd:string ;
    rdfs:domain nell:color ;
    rdfs:range nell:invertebrate ;
    rdfs:subPropertyOf nell:relatedto .

nell:inverseofinvertebrateturnintoinsect rdfs:comment "Describes the metamorphosis of some invertebrates into another insects"^^xsd:string ;
    rdfs:domain nell:insect ;
    rdfs:range nell:invertebrate ;
    rdfs:subPropertyOf nell:relatedto .

nell:inverseofislandhasskiarea rdfs:comment "Describes island that have ski a area"^^xsd:string ;
    rdfs:domain nell:skiarea ;
    rdfs:range nell:island ;
    rdfs:subPropertyOf nell:relatedto .

nell:inverseoflanguagespokenatisland rdfs:comment "Describes languages spoken at islands"^^xsd:string ;
    rdfs:domain nell:island ;
    rdfs:range nell:language ;
    rdfs:subPropertyOf nell:relatedto .

nell:inverseoflanguegeschoolincity rdfs:comment "Describes the language schools for specific languages in a city"^^xsd:string ;
    rdfs:domain nell:city ;
    rdfs:range nell:language ;
    rdfs:subPropertyOf nell:relatedto .

nell:inverseofmagazineisleadbyceo rdfs:comment "Identifies the CEO of a Magazine"^^xsd:string ;
    rdfs:domain nell:ceo ;
    rdfs:range nell:magazine ;
    rdfs:subPropertyOf nell:relatedto .

nell:inverseofmalemovedtostateorprovince rdfs:comment "Describes the male people that moved to live in a state or province"^^xsd:string ;
    rdfs:domain nell:stateorprovince ;
    rdfs:range nell:male ;
    rdfs:subPropertyOf nell:inverseofpersonmovedtostateorprovince .

nell:inverseofmammaleatsinsect rdfs:comment "Describes the insects that mammals eats"^^xsd:string ;
    rdfs:domain nell:insect ;
    rdfs:range nell:mammal ;
    rdfs:subPropertyOf nell:inverseofanimalfeedoninsect .

nell:inverseofmammalinducesemotion rdfs:comment "The emotion that human beings generally have by looking at a mammal"^^xsd:string ;
    rdfs:domain nell:emotion ;
    rdfs:range nell:mammal ;
    rdfs:subPropertyOf nell:relatedto .

nell:inverseofmammalsuchasmammal rdfs:comment "Describes the specific actors types that are generalizations of actors"^^xsd:string ;
    rdfs:domain nell:mammal ;
    rdfs:range nell:mammal ;
    rdfs:subPropertyOf nell:specializationof .

nell:inverseofmeatcomesfromanimal rdfs:comment "Describes the animals and their meat cuts"^^xsd:string ;
    rdfs:domain nell:animal ;
    rdfs:range nell:meat ;
    rdfs:subPropertyOf nell:relatedto .

nell:inverseofmountainatgeopoliticallocation rdfs:comment "geopoliticallocation and mountain are related"^^xsd:string ;
    rdfs:domain nell:geopoliticallocation ;
    rdfs:range nell:mountain ;
    rdfs:subPropertyOf nell:atlocation .

nell:inverseofmoviessuchasmovies rdfs:comment "Describes the movies types that are generalizations of specific movies"^^xsd:string ;
    rdfs:domain nell:movie ;
    rdfs:range nell:movie ;
    rdfs:subPropertyOf nell:specializationof .

nell:inverseofmusicalartisthadapetanimal rdfs:comment "Describes the pet animals that musical artists have or had"^^xsd:string ;
    rdfs:domain nell:animal ;
    rdfs:range nell:musicartist ;
    rdfs:subPropertyOf nell:relatedto .

nell:inverseofmusicfestivalssuchasmusicfestivals rdfs:comment "Describes the musicfestivals types that are generalizations of specific musicfestivals"^^xsd:string ;
    rdfs:domain nell:musicfestival ;
    rdfs:range nell:musicfestival ;
    rdfs:subPropertyOf nell:specializationof .

nell:inverseofmusicgenressuchasmusicgenres rdfs:comment "Describes the musicgenre types that are generalizations of specific musicgenres"^^xsd:string ;
    rdfs:domain nell:musicgenre ;
    rdfs:range nell:musicgenre ;
    rdfs:subPropertyOf nell:specializationof .

nell:inverseofmusicsongisatrackofmusicalbum rdfs:comment "Identifies a music song which is a track of a music album"^^xsd:string ;
    rdfs:domain nell:musicalbum ;
    rdfs:range nell:musicsong ;
    rdfs:subPropertyOf nell:relatedto .

nell:inverseofnewpaperhaswebsite rdfs:comment "Present the oficial website of a newspaper"^^xsd:string ;
    rdfs:domain nell:website ;
    rdfs:range nell:newspaper ;
    rdfs:subPropertyOf nell:officialwebsiteoforganization .

nell:inverseofpersongraduatedfromuniversity rdfs:comment "Describes the people graduated from a university"^^xsd:string ;
    rdfs:domain nell:university ;
    rdfs:range nell:person ;
    rdfs:subPropertyOf nell:schoolgraduatedperson .

nell:inverseofplantgrowinginplant rdfs:comment "Describes the plants that grow on other plants"^^xsd:string ;
    rdfs:domain nell:plant ;
    rdfs:range nell:plant ;
    rdfs:subPropertyOf nell:relatedto .

nell:inverseofplantincludeplant rdfs:comment "Describes the subcategories of a plant"^^xsd:string ;
    rdfs:domain nell:plant ;
    rdfs:range nell:plant ;
    rdfs:subPropertyOf nell:specializationof .

nell:inverseofplantrepresentemotion rdfs:comment "Describes the emotions represented by a plant"^^xsd:string ;
    rdfs:domain nell:emotion ;
    rdfs:range nell:plant ;
    rdfs:subPropertyOf nell:relatedto .

nell:inverseofpoliticianuswenttoschool rdfs:comment "Describes the school where a US politician studied"^^xsd:string ;
    rdfs:domain nell:school ;
    rdfs:range nell:politicianus ;
    rdfs:subPropertyOf nell:relatedto .

nell:inverseofprofessionactsatthesameareaofpoliticissue rdfs:comment "Describes professions that work at the area of a political issue"^^xsd:string ;
    rdfs:domain nell:profession ;
    rdfs:range nell:politicsissue ;
    rdfs:subPropertyOf nell:relatedto .

nell:inverseofprofessionssuchasprofessions rdfs:comment "Describes the professions types that are generalizations of specific professions"^^xsd:string ;
    rdfs:domain nell:profession ;
    rdfs:range nell:profession ;
    rdfs:subPropertyOf nell:specializationof .

nell:inverseofreligionssuchasreligions rdfs:comment "Describes the religions types that are generalizations of specific religions"^^xsd:string ;
    rdfs:domain nell:religion ;
    rdfs:range nell:religion ;
    rdfs:subPropertyOf nell:specializationof .

nell:inverseofriveremptiesintoriver rdfs:comment "Describes the tributaries of a river"^^xsd:string ;
    rdfs:domain nell:river ;
    rdfs:range nell:river ;
    rdfs:subPropertyOf nell:locatedat .

nell:inverseofsoftwareprogrammedinprogramminglanguage rdfs:comment "Relates a software to its programming language"^^xsd:string ;
    rdfs:domain nell:programminglanguage ;
    rdfs:range nell:software ;
    rdfs:subPropertyOf nell:relatedto .

nell:inverseofsportfansincountry rdfs:comment "Describes the sports that have fans living in a country"^^xsd:string ;
    rdfs:domain nell:country ;
    rdfs:range nell:sport ;
    rdfs:subPropertyOf nell:relatedto .

nell:inverseofsportschoolincountry rdfs:comment "Describes the sports practiced in a country"^^xsd:string ;
    rdfs:domain nell:country ;
    rdfs:range nell:sport ;
    rdfs:subPropertyOf nell:relatedto .

nell:inverseofstadiumoreventvenuedisclosescompany rdfs:comment "Describes a stadium or event venue that discloses a company"^^xsd:string ;
    rdfs:domain nell:company ;
    rdfs:range nell:stadiumoreventvenue ;
    rdfs:subPropertyOf nell:relatedto .

nell:inverseofstateorprovinceattainstrainstation rdfs:comment "Describes the trainstantions location (state or province)"^^xsd:string ;
    rdfs:domain nell:trainstation ;
    rdfs:range nell:stateorprovince ;
    rdfs:subPropertyOf nell:relatedto .

nell:inverseoftelevisionshowssuchastelevisionshows rdfs:comment "Describes the televisionshows types that are generalizations of specific televisionshows"^^xsd:string ;
    rdfs:domain nell:televisionshow ;
    rdfs:range nell:televisionshow ;
    rdfs:subPropertyOf nell:specializationof .

nell:inverseoftoolssuchastools rdfs:comment "Describes the tools types that are generalizations of specific tools"^^xsd:string ;
    rdfs:domain nell:tool ;
    rdfs:range nell:tool ;
    rdfs:subPropertyOf nell:specializationof .

nell:inverseoftouristattraction a owl:AsymmetricProperty,
        owl:IrreflexiveProperty ;
    rdfs:comment "Describes the specific tourist attraction types that are generalizations of tourist attractions"^^xsd:string ;
    rdfs:domain nell:attraction ;
    rdfs:range nell:attraction ;
    rdfs:subPropertyOf nell:specializationof .

nell:inverseofuniversityledmusicfestival rdfs:comment "identifies the university that led a Musical Festival"^^xsd:string ;
    rdfs:domain nell:musicfestival ;
    rdfs:range nell:university ;
    rdfs:subPropertyOf nell:eventhasparticipantagent .

nell:inverseofvegetablecanbeservedwithgrain rdfs:comment "Describes the vegetables that are usually served with a grain"^^xsd:string ;
    rdfs:domain nell:grain ;
    rdfs:range nell:vegetable ;
    rdfs:subPropertyOf nell:itemusedwithitem .

nell:inverseofvegetableisproducedatcountry rdfs:comment "Describes the countries that are big produces of vegetables"^^xsd:string ;
    rdfs:domain nell:country ;
    rdfs:range nell:vegetable ;
    rdfs:subPropertyOf nell:locationofitemexistence .

nell:inverseofvegetableproductioninstateorprovince rdfs:comment "Describes the vegetables produced in a state or province"^^xsd:string ;
    rdfs:domain nell:stateorprovince ;
    rdfs:range nell:vegetable ;
    rdfs:subPropertyOf nell:locationofitemexistence .

nell:inverseofvideogamessuchasvideogames rdfs:comment "Describes the videogame types that are generalizations of specific videogames"^^xsd:string ;
    rdfs:domain nell:videogame ;
    rdfs:range nell:videogame ;
    rdfs:subPropertyOf nell:specializationof .

nell:inverseofweaponmadeincountry rdfs:comment "Describes the weapons produced by a country"^^xsd:string ;
    rdfs:domain nell:country ;
    rdfs:range nell:weapon ;
    rdfs:subPropertyOf nell:locationofitemexistence .

nell:inverseofweaponssuchasweapons rdfs:comment "Describes the weapons types that are generalizations of specific weapons"^^xsd:string ;
    rdfs:domain nell:weapon ;
    rdfs:range nell:weapon ;
    rdfs:subPropertyOf nell:specializationof .

nell:inverseofwineryatfarm rdfs:comment "farm and winery are related"^^xsd:string ;
    rdfs:domain nell:farm ;
    rdfs:range nell:winery ;
    rdfs:subPropertyOf nell:relatedto .

nell:inverseofwriterwasbornincity rdfs:comment "Describes the city where a write was born in"^^xsd:string ;
    rdfs:domain nell:city ;
    rdfs:range nell:person ;
    rdfs:subPropertyOf nell:cityofpersonbirth .

nell:inversoofairportsuchasairport rdfs:comment "Describes the airport types that are generalizations of specific aiports"^^xsd:string ;
    rdfs:domain nell:airport ;
    rdfs:range nell:airport ;
    rdfs:subPropertyOf nell:specializationof .

nell:invertebratefeedonfood rdfs:comment "Describes the foods that are eaten by an invertebrate"^^xsd:string ;
    rdfs:domain nell:invertebrate ;
    rdfs:range nell:food ;
    rdfs:subPropertyOf nell:animaleatfood .

nell:invertebratehascolor rdfs:comment "Describes the color of invertebrates"^^xsd:string ;
    rdfs:domain nell:invertebrate ;
    rdfs:range nell:color ;
    rdfs:subPropertyOf nell:relatedto .

nell:invertebrateturnintoinsect rdfs:comment "Describes the metamorphosis of some invertebrates into another insects"^^xsd:string ;
    rdfs:domain nell:invertebrate ;
    rdfs:range nell:insect ;
    rdfs:subPropertyOf nell:relatedto .

nell:islandhasskiarea rdfs:comment "Describes island that have ski a area"^^xsd:string ;
    rdfs:domain nell:island ;
    rdfs:range nell:skiarea ;
    rdfs:subPropertyOf nell:relatedto .

nell:ismultipleof rdfs:comment "Specifies the way in which a grouping of individual somethings can be referred to including but not limited to relating the plural form to the singular."^^xsd:string ;
    rdfs:domain nell:everypromotedthing ;
    rdfs:range nell:everypromotedthing ;
    rdfs:subPropertyOf nell:mutualproxyfor .

nell:isoneoccurrenceof rdfs:comment "Specifies the way in which a grouping of individual somethings can be referred to including but not limited to relating the plural form to the singular."^^xsd:string ;
    rdfs:domain nell:everypromotedthing ;
    rdfs:range nell:everypromotedthing ;
    rdfs:subPropertyOf nell:mutualproxyfor .

nell:isshorterthan rdfs:comment "Indicates that arg1 has a greater height than arg2"^^xsd:string ;
    rdfs:domain nell:everypromotedthing ;
    rdfs:range nell:everypromotedthing ;
    rdfs:subPropertyOf nell:relatedto .

nell:issueofpoliticsbill rdfs:comment "Issues that a legislative billl is concerned with."^^xsd:string ;
    rdfs:domain nell:politicsissue ;
    rdfs:range nell:politicsbill ;
    rdfs:subPropertyOf nell:relatedto .

nell:issueofpoliticsgroup rdfs:comment "Issues that a political group has concern about"^^xsd:string ;
    rdfs:domain nell:politicsissue ;
    rdfs:range nell:politicsgroup ;
    rdfs:subPropertyOf nell:relatedto .

nell:istallerthan rdfs:comment "Indicates that arg1 has a greater height than arg2"^^xsd:string ;
    rdfs:domain nell:everypromotedthing ;
    rdfs:range nell:everypromotedthing ;
    rdfs:subPropertyOf nell:relatedto .

nell:itemexistsatdate rdfs:comment "a item exists in a determined time (or date)"^^xsd:string ;
    rdfs:domain nell:item ;
    rdfs:range nell:date ;
    rdfs:subPropertyOf nell:atdate .

nell:iteminvolvedinevent rdfs:comment "Umbrella relation for identifying items in events."^^xsd:string ;
    rdfs:domain nell:item ;
    rdfs:range nell:event ;
    rdfs:subPropertyOf nell:subpartof .

nell:itemusedatlocation rdfs:comment "an item used in a specific place"^^xsd:string ;
    rdfs:domain nell:item ;
    rdfs:range nell:location ;
    rdfs:subPropertyOf nell:atlocation .

nell:jobpositioncanbethesameaspoliticaloffice rdfs:comment "Describes two instances that are the same thing in these two different categories"^^xsd:string ;
    rdfs:domain nell:jobposition ;
    rdfs:range nell:politicaloffice ;
    rdfs:subPropertyOf nell:canbethesameas .

nell:jobpositionheldbyperson rdfs:comment "This relation holds when the person has held the position at some point in some organization."^^xsd:string ;
    rdfs:domain nell:jobposition ;
    rdfs:range nell:person ;
    rdfs:subPropertyOf nell:relatedto .

nell:jobpositionusesacademicfield rdfs:comment "Academic fields useful for job positions"^^xsd:string ;
    rdfs:domain nell:jobposition ;
    rdfs:range nell:academicfield ;
    rdfs:subPropertyOf nell:relatedto .

nell:journalistwritesforpublication rdfs:comment "specifies that a particular journalist writes for a particular publication"^^xsd:string ;
    rdfs:domain nell:journalist ;
    rdfs:range nell:publication ;
    rdfs:subPropertyOf nell:worksfor .

nell:judge rdfs:comment "a judge in a court of law"^^xsd:string ;
    rdfs:subClassOf nell:person .

nell:kitchenitem rdfs:comment "Any item that might be found in a commercial or residential kitchen that is used for cullinary purposes or in pursuit of the same (e.g. a cupboard)."^^xsd:string ;
    rdfs:subClassOf nell:householditem .

nell:lakeinstate rdfs:comment "The state/province a river is in."^^xsd:string ;
    rdfs:domain nell:lake ;
    rdfs:range nell:stateorprovince ;
    rdfs:subPropertyOf nell:locationlocatedwithinlocation .

nell:languageofcity rdfs:comment "Typical language spoken in a city (official or otherwise)"^^xsd:string ;
    rdfs:domain nell:language ;
    rdfs:range nell:city ;
    rdfs:subPropertyOf nell:relatedto .

nell:languageofcountry rdfs:comment "Typical language spoken in a country (official or otherwise)"^^xsd:string ;
    rdfs:domain nell:language ;
    rdfs:range nell:country ;
    rdfs:subPropertyOf nell:relatedto .

nell:languageofsportsgame rdfs:comment "Describes the origin language of the sports name"^^xsd:string ;
    rdfs:domain nell:language ;
    rdfs:range nell:sport ;
    rdfs:subPropertyOf nell:relatedto .

nell:languageofuniversity rdfs:comment "Language spoken at a college/university."^^xsd:string ;
    rdfs:domain nell:language ;
    rdfs:range nell:university ;
    rdfs:subPropertyOf nell:relatedto .

nell:languageschoolincity rdfs:comment "Describes the language schools for specific languages in a city"^^xsd:string ;
    rdfs:domain nell:language ;
    rdfs:range nell:city ;
    rdfs:subPropertyOf nell:relatedto .

nell:languagespokenatisland rdfs:comment "Describes languages spoken at islands"^^xsd:string ;
    rdfs:domain nell:language ;
    rdfs:range nell:island ;
    rdfs:subPropertyOf nell:relatedto .

nell:latitudelongitude rdfs:comment "the latitude and longitude of this location or the latitude and longitude typically associated with this thing"^^xsd:string ;
    rdfs:domain nell:everypromotedthing ;
    rdfs:range nell:llcoordinate ;
    rdfs:subPropertyOf nell:relatedto .

nell:latitudelongitudeof rdfs:comment "the latitude and longitude of this location or the latitude and longitude typically associated with this thing"^^xsd:string ;
    rdfs:domain nell:llcoordinate ;
    rdfs:range nell:everypromotedthing ;
    rdfs:subPropertyOf nell:relatedto .

nell:launchingproductcompany rdfs:domain nell:productlaunchevent ;
    rdfs:range nell:company ;
    rdfs:subPropertyOf nell:relatedto .

nell:launchingproducttype rdfs:domain nell:productlaunchevent ;
    rdfs:range nell:product ;
    rdfs:subPropertyOf nell:relatedto .

nell:leaguecoaches rdfs:comment "specifies that a particular coach coaches a team that plays in a particular league"^^xsd:string ;
    rdfs:domain nell:sportsleague ;
    rdfs:range nell:coach ;
    rdfs:subPropertyOf nell:organizationhasperson .

nell:leagueteams rdf:first <http://www.semanticweb.org/ontologies/NELL#_:y33> ;
    rdfs:comment "The league that a team plays in."^^xsd:string ;
    rdfs:domain nell:sportsleague ;
    rdfs:range nell:sportsteam ;
    rdfs:subPropertyOf nell:superpartoforganization .

nell:legume rdfs:comment "plant in the family Fabaceae (or Leguminosae) or a fruit of these specific plants. A legume fruit is a simple dry fruit that develops from a simple carpel and usually dehisces (opens along a seam) on two sides."^^xsd:string ;
    rdfs:subClassOf nell:fruit .

nell:locationexistsatdate rdfs:comment "Most general location-to-date relation. Note that locations are not eternal."^^xsd:string ;
    rdfs:domain nell:location ;
    rdfs:range nell:date ;
    rdfs:subPropertyOf nell:atdate .

nell:locationinzipcode rdfs:comment "Describes one or more locations to which a zipcode may correspond."^^xsd:string ;
    rdfs:domain nell:location ;
    rdfs:range nell:zipcode ;
    rdfs:subPropertyOf nell:locatedat .

nell:locationofbombing rdfs:domain nell:location ;
    rdfs:range nell:bombingevent ;
    rdfs:subPropertyOf nell:relatedto .

nell:locationofearthquake rdfs:domain nell:location ;
    rdfs:range nell:earthquakeevent ;
    rdfs:subPropertyOf nell:relatedto .

nell:locationofitemuse rdfs:comment "an item used in a specific place"^^xsd:string ;
    rdfs:domain nell:location ;
    rdfs:range nell:item ;
    rdfs:subPropertyOf nell:locatedat .

nell:locationofprotest rdfs:domain nell:location ;
    rdfs:range nell:protestevent ;
    rdfs:subPropertyOf nell:relatedto .

nell:locationofroadaccident rdfs:domain nell:location ;
    rdfs:range nell:roadaccidentevent ;
    rdfs:subPropertyOf nell:relatedto .

nell:locationrepresentedbypolitician rdfs:comment "Describes the city state country or other location represented by a politician"^^xsd:string ;
    rdfs:domain nell:location ;
    rdfs:range nell:politician ;
    rdfs:subPropertyOf nell:locationrelatedtoagent .

nell:loseringame rdfs:comment "Specifies that a particular team that played in a particular sportsGame was the loser thereof."^^xsd:string ;
    rdfs:domain nell:sportsteam ;
    rdfs:range nell:sportsgame ;
    rdfs:subPropertyOf nell:teamingame .

nell:losingscoreofsportsgame rdfs:comment "Specifies the score with which the loosing team in a particular sportsGame lost."^^xsd:string ;
    rdfs:domain nell:nonneginteger ;
    rdfs:range nell:sportsgame ;
    rdfs:subPropertyOf nell:relatedto .

nell:lymphnode rdfs:comment "a lymph node in the body"^^xsd:string ;
    rdfs:subClassOf nell:bodypart .

nell:lyrics rdfs:comment "Refernce to the lyrics of a song as distinct from a reference to the song itself"^^xsd:string ;
    rdfs:subClassOf nell:creativework .

nell:magazinecontainspublication rdfs:comment "Magazine in which a publication was published in"^^xsd:string ;
    rdfs:domain nell:magazine ;
    rdfs:range nell:publication ;
    rdfs:subPropertyOf nell:superpartof .

nell:magazineisleadbyceo rdfs:comment "Identifies the CEO of a Magazine"^^xsd:string ;
    rdfs:domain nell:magazine ;
    rdfs:range nell:ceo ;
    rdfs:subPropertyOf nell:relatedto .

nell:magnitudeofearthquaque rdfs:domain nell:everypromotedthing ;
    rdfs:range nell:earthquakeevent ;
    rdfs:subPropertyOf nell:relatedto .

nell:malecanbethesameascomedian rdfs:comment "Describes two instances that are the same thing in these two different categories"^^xsd:string ;
    rdfs:domain nell:male ;
    rdfs:range nell:comedian ;
    rdfs:subPropertyOf nell:canbethesameas .

nell:malemovedtostateorprovince rdfs:comment "Describes the male people that moved to live in a state or province"^^xsd:string ;
    rdfs:domain nell:male ;
    rdfs:range nell:stateorprovince ;
    rdfs:subPropertyOf nell:personmovedtostateorprovince .

nell:mammalcanbeirritatedbyarthropod rdfs:comment "Arthropode that usually irritates mammal"^^xsd:string ;
    rdfs:domain nell:mammal ;
    rdfs:range nell:arthropod ;
    rdfs:subPropertyOf nell:relatedto .

nell:mammaleatsinsect rdfs:comment "Describes the insects that mammals eats"^^xsd:string ;
    rdfs:domain nell:mammal ;
    rdfs:range nell:insect ;
    rdfs:subPropertyOf nell:animalthatfeedoninsect .

nell:mammalinducesemotion rdfs:comment "The emotion that human beings generally have by looking at a mammal"^^xsd:string ;
    rdfs:domain nell:mammal ;
    rdfs:range nell:emotion ;
    rdfs:subPropertyOf nell:relatedto .

nell:mammalsuchasmammal rdfs:comment "Describes the specific actors types that are generalizations of actors"^^xsd:string ;
    rdfs:domain nell:mammal ;
    rdfs:range nell:mammal ;
    rdfs:subPropertyOf nell:generalizationof .

nell:marriedinyear rdfs:comment "This relation holds when a person married some other person in the specified year."^^xsd:string ;
    rdfs:domain nell:person ;
    rdfs:range nell:year ;
    rdfs:subPropertyOf nell:atdate .

nell:meatcomesfromanimal rdfs:comment "Describes the animals and their meat cuts"^^xsd:string ;
    rdfs:domain nell:meat ;
    rdfs:range nell:animal ;
    rdfs:subPropertyOf nell:relatedto .

nell:mediatype rdfs:comment "the means of communication as radio and television newspapers and magazines that reach or influence people widely "^^xsd:string ;
    rdfs:subClassOf nell:item .

nell:medicalprocedure rdfs:comment "The medical treatment type is used for any medical intervention designed to treat and cure human diseases and medical conditions. This type includes both curative and palliative treatments"^^xsd:string ;
    rdfs:subClassOf nell:abstractthing .

nell:meetingeventtitleatdate rdfs:comment "When a particular meeting will take place"^^xsd:string ;
    rdfs:domain nell:meetingeventtitle ;
    rdfs:range nell:dateliteral ;
    rdfs:subPropertyOf nell:eventdate .

nell:meetingeventtitlehasmeetingeventtype rdfs:comment "What series of meetings a particular meeting belongs to or what kind of a meeting it is"^^xsd:string ;
    rdfs:domain nell:meetingeventtitle ;
    rdfs:range nell:meetingeventtype ;
    rdfs:subPropertyOf nell:relatedto .

nell:meetingeventtitlehasspeakingperson rdfs:comment "Who will be speaking at a particular meeting"^^xsd:string ;
    rdfs:domain nell:meetingeventtitle ;
    rdfs:range nell:person ;
    rdfs:subPropertyOf nell:eventhasparticipantagent .

nell:meetingeventtitleinbuilding rdfs:comment "In which building a particular meeting will take place"^^xsd:string ;
    rdfs:domain nell:meetingeventtitle ;
    rdfs:range nell:building ;
    rdfs:subPropertyOf nell:eventatlocation .

nell:meetingeventtitleinofficebuildingroom rdfs:comment "In which room a particular meeting will take place"^^xsd:string ;
    rdfs:domain nell:meetingeventtitle ;
    rdfs:range nell:officebuildingroom ;
    rdfs:subPropertyOf nell:eventatlocation .

nell:meetingeventtypeincludesmeetingeventtitle rdfs:comment "What series of meetings a particular meeting belongs to or what kind of a meeting it is"^^xsd:string ;
    rdfs:domain nell:meetingeventtype ;
    rdfs:range nell:meetingeventtitle ;
    rdfs:subPropertyOf nell:relatedto .

nell:militaryconflict rdfs:comment "A military conflict is any event that involves armed forces acting in hostility. This includes wars battles and guerilla actions."^^xsd:string ;
    rdfs:subClassOf nell:militaryeventtype .

nell:mlalgorithm rdfs:comment "Any algorithm or class of algorithms that is used at any stage of machine learning."^^xsd:string ;
    rdfs:subClassOf nell:abstractthing .

nell:mlareaexpert rdfs:comment "specifies that a particular ML author is an expert in a particular ML area"^^xsd:string ;
    rdfs:domain nell:mlarea ;
    rdfs:range nell:mlauthor ;
    rdfs:subPropertyOf nell:relatedto .

nell:mlauthorexpertin rdfs:comment "specifies that a particular ML author is an expert in a particular ML area"^^xsd:string ;
    rdfs:domain nell:mlauthor ;
    rdfs:range nell:mlarea ;
    rdfs:subPropertyOf nell:relatedto .

nell:mlauthorofsoftware rdfs:comment "Specifies ML software that is written by a particular ML author"^^xsd:string ;
    rdfs:domain nell:mlauthor ;
    rdfs:range nell:mlsoftware ;
    rdfs:subPropertyOf nell:agentcreated,
        nell:agentinvolvedwithitem .

nell:mlconference rdfs:comment "A conference in the area of machine learning"^^xsd:string ;
    rdfs:subClassOf nell:conference .

nell:mldataset rdfs:comment "A dataset used in machine learning"^^xsd:string ;
    rdfs:subClassOf nell:abstractthing .

nell:mlmetric rdfs:comment "A metric used to evaluate machine learning methods"^^xsd:string ;
    rdfs:subClassOf nell:abstractthing .

nell:mlsoftwareauthor rdfs:comment "Specifies ML software that is written by a particular ML author"^^xsd:string ;
    rdfs:domain nell:mlsoftware ;
    rdfs:range nell:mlauthor ;
    rdfs:subPropertyOf nell:createdbyagent,
        nell:iteminvolvedwithagent .

nell:model rdfs:comment "a person who is paid to be a fashion model"^^xsd:string ;
    rdfs:subClassOf nell:person .

nell:monarch rdfs:comment "A monarch is a person who heads a monarchy such as a king or queen"^^xsd:string ;
    rdfs:subClassOf nell:person .

nell:month rdfs:comment "Twelve months of the year."^^xsd:string ;
    rdfs:subClassOf nell:date .

nell:monument rdfs:comment "An architectural structure (usually public) which is erected to commemorate a person place event or group."^^xsd:string ;
    rdfs:subClassOf nell:attraction,
        nell:building .

nell:mountainatgeopoliticallocation rdfs:comment "geopoliticallocation and mountain are related"^^xsd:string ;
    rdfs:domain nell:mountain ;
    rdfs:range nell:geopoliticallocation ;
    rdfs:subPropertyOf nell:locatedat .

nell:mountaininstate rdfs:comment "State/province a mountain is located in."^^xsd:string ;
    rdfs:domain nell:mountain ;
    rdfs:range nell:stateorprovince ;
    rdfs:subPropertyOf nell:locationlocatedwithinlocation .

nell:mountainrange rdfs:comment "A mountain range is a group of mountains bordered by lowlands or separated from other mountain ranges by passes or rivers."^^xsd:string ;
    rdfs:subClassOf nell:location .

nell:moviedirectedbydirector rdfs:comment "to direct a monvie"^^xsd:string ;
    rdfs:domain nell:movie ;
    rdfs:range nell:director ;
    rdfs:subPropertyOf nell:creativeworkcontributedtobyagent .

nell:moviessuchasmovies rdfs:comment "Describes the movies types that are generalizations of specific movies"^^xsd:string ;
    rdfs:domain nell:movie ;
    rdfs:range nell:movie ;
    rdfs:subPropertyOf nell:generalizationof .

nell:moviestaractor rdfs:comment "to perform as an actor (in movie) "^^xsd:string ;
    rdfs:domain nell:movie ;
    rdfs:range nell:actor ;
    rdfs:subPropertyOf nell:creativeworkcontributedtobyagent .

nell:moviethatgeneratestelevisionshow rdfs:comment "Movie that a television show was based in"^^xsd:string ;
    rdfs:domain nell:movie ;
    rdfs:range nell:televisionshow ;
    rdfs:subPropertyOf nell:relatedto .

nell:musclelocatedinbodypart rdfs:comment "Describes the muscles in body parts"^^xsd:string ;
    rdfs:domain nell:muscle ;
    rdfs:range nell:bodypart ;
    rdfs:subPropertyOf nell:subpartof .

nell:museumincity rdfs:comment "The city that a museum is located in"^^xsd:string ;
    rdfs:domain nell:museum ;
    rdfs:range nell:city ;
    rdfs:subPropertyOf nell:attractionofcity,
        nell:buildinglocatedincity .

nell:musicalartisthadapetanimal rdfs:comment "Describes the pet animals that musical artists have or had"^^xsd:string ;
    rdfs:domain nell:musicartist ;
    rdfs:range nell:animal ;
    rdfs:subPropertyOf nell:relatedto .

nell:musicartistgenre rdfs:comment "Specifies that a musicArtist performs in a particular genre"^^xsd:string ;
    rdfs:domain nell:musicartist ;
    rdfs:range nell:musicgenre ;
    rdfs:subPropertyOf nell:relatedto .

nell:musicartistmusician rdfs:comment "Specifies that a particular musician has performed as particular musicArtist"^^xsd:string ;
    rdfs:domain nell:musicartist ;
    rdfs:range nell:musician ;
    rdfs:subPropertyOf nell:organizationhasperson .

nell:musicfestivalssuchasmusicfestivals rdfs:comment "Describes the musicfestivals types that are generalizations of specific musicfestivals"^^xsd:string ;
    rdfs:domain nell:musicfestival ;
    rdfs:range nell:musicfestival ;
    rdfs:subPropertyOf nell:generalizationof .

nell:musicgenreartist rdfs:comment "Specifies that a musicArtist performs in a particular genre"^^xsd:string ;
    rdfs:domain nell:musicgenre ;
    rdfs:range nell:musicartist ;
    rdfs:subPropertyOf nell:relatedto .

nell:musicgenressuchasmusicgenres a owl:AsymmetricProperty,
        owl:IrreflexiveProperty ;
    rdfs:comment "Describes the musicgenre types that are generalizations of specific musicgenres"^^xsd:string ;
    rdfs:domain nell:musicgenre ;
    rdfs:range nell:musicgenre ;
    rdfs:subPropertyOf nell:generalizationof .

nell:musicianinmusicartist rdfs:comment "Specifies that a particular musician has performed as particular musicArtist"^^xsd:string ;
    rdfs:domain nell:musician ;
    rdfs:range nell:musicartist ;
    rdfs:subPropertyOf nell:personbelongstoorganization .

nell:musicianplaysinstrument rdfs:comment "Specifies that a musical instrument is played by a paritcular musician"^^xsd:string ;
    rdfs:domain nell:musician ;
    rdfs:range nell:musicinstrument ;
    rdfs:subPropertyOf nell:agentinvolvedwithitem .

nell:musicsongisatrackofmusicalbum rdfs:comment "Identifies a music song which is a track of a music album"^^xsd:string ;
    rdfs:domain nell:musicsong ;
    rdfs:range nell:musicalbum ;
    rdfs:subPropertyOf nell:relatedto .

nell:nerve rdfs:comment "a single nerve cell or bundle of nerve cells"^^xsd:string ;
    rdfs:subClassOf nell:bodypart .

nell:newpaperhaswebsite rdfs:comment "Present the oficial website of a newspaper"^^xsd:string ;
    rdfs:domain nell:newspaper ;
    rdfs:range nell:website ;
    rdfs:subPropertyOf nell:organizationhasofficialwebsite .

nell:newspaperincity rdfs:comment "Specifies the city in which a particular newspaper is headquartered"^^xsd:string ;
    rdfs:domain nell:newspaper ;
    rdfs:range nell:city ;
    rdfs:subPropertyOf nell:agentactsinlocation .

nell:nondiseasecondition rdfs:comment "Those physiologicalConditions that normal and expected parts of life (such as pregnancy or teething) that are not diseases but which do affect the normal functioning of the body."^^xsd:string ;
    rdfs:subClassOf nell:physiologicalcondition .

nell:nonprofitorganization rdfs:comment "A non-profit organization is a legally-constituted organization that does not make a profit from its operations."^^xsd:string ;
    rdfs:subClassOf nell:organization .

nell:numberofarrestedinbombing rdfs:domain nell:nonneginteger ;
    rdfs:range nell:bombingevent ;
    rdfs:subPropertyOf nell:relatedto .

nell:numberofcasualtiesinearthquake rdfs:domain nell:nonneginteger ;
    rdfs:range nell:earthquakeevent ;
    rdfs:subPropertyOf nell:relatedto .

nell:numberofcasualtiesinroadaccident rdfs:domain nell:nonneginteger ;
    rdfs:range nell:roadaccidentevent ;
    rdfs:subPropertyOf nell:relatedto .

nell:numberofinjuredinbombing rdfs:domain nell:nonneginteger ;
    rdfs:range nell:bombingevent ;
    rdfs:subPropertyOf nell:relatedto .

nell:numberofinjuredinearthquake rdfs:domain nell:nonneginteger ;
    rdfs:range nell:earthquakeevent ;
    rdfs:subPropertyOf nell:relatedto .

nell:numberofinjuredinprotest rdfs:domain nell:nonneginteger ;
    rdfs:range nell:protestevent ;
    rdfs:subPropertyOf nell:relatedto .

nell:numberofinjuredinroadaccident rdfs:domain nell:nonneginteger ;
    rdfs:range nell:roadaccidentevent ;
    rdfs:subPropertyOf nell:relatedto .

nell:numberofkilledinbombing rdfs:domain nell:nonneginteger ;
    rdfs:range nell:bombingevent ;
    rdfs:subPropertyOf nell:relatedto .

nell:nut rdfs:comment "hard-shelled fruit of some plants having an indehiscent seed."^^xsd:string ;
    rdfs:subClassOf nell:fruit .

nell:objectcontainsobject rdfs:comment "meronym"^^xsd:string ;
    rdfs:domain nell:visualizableobject ;
    rdfs:range nell:visualizableobject ;
    rdfs:subPropertyOf nell:relatedto .

nell:objectfoundinscene rdfs:comment "Object found in scene (NEIL)"^^xsd:string ;
    rdfs:domain nell:visualizableobject ;
    rdfs:range nell:visualizablescene ;
    rdfs:subPropertyOf nell:relatedto .

nell:objectlookslikeobject a owl:IrreflexiveProperty,
        owl:SymmetricProperty ;
    rdfs:comment "Object looks like (NEIL)"^^xsd:string ;
    rdfs:domain nell:visualizablething ;
    rdfs:range nell:visualizablething ;
    rdfs:subPropertyOf nell:relatedto .

nell:objectpartofobject rdfs:comment "meronym"^^xsd:string ;
    rdfs:domain nell:visualizableobject ;
    rdfs:range nell:visualizableobject ;
    rdfs:subPropertyOf nell:relatedto .

nell:officebuildingroomhostsmeetingeventtitle rdfs:comment "In which room a particular meeting will take place"^^xsd:string ;
    rdfs:domain nell:officebuildingroom ;
    rdfs:range nell:meetingeventtitle ;
    rdfs:subPropertyOf nell:locationofevent .

nell:officebuildingroominbuilding rdfs:comment "Which office-style building a particular room is found in"^^xsd:string ;
    rdfs:domain nell:officebuildingroom ;
    rdfs:range nell:building ;
    rdfs:subPropertyOf nell:locationlocatedwithinlocation .

nell:officeheldbypoliticianus rdfs:comment "U.S. Politician who holds an office"^^xsd:string ;
    rdfs:domain nell:politicaloffice ;
    rdfs:range nell:politicianus ;
    rdfs:subPropertyOf nell:officeheldbypolitician .

nell:officeitem rdfs:comment "Items usually found in an office that are used for clerical or intellectual work."^^xsd:string ;
    rdfs:subClassOf nell:item .

nell:oilgasfield rdfs:comment "An field from which oil or natural gas are extracted."^^xsd:string ;
    rdfs:subClassOf nell:geolocatablething,
        nell:visualizablescene .

nell:olympics rdfs:comment "are a major international event featuring summer and winter sports in which thousands of athletes participate in a variety of competitions. The Games are currently held every two years with Summer and Winter Olympic Games alternating although they occur every four years within their respective seasonal games."^^xsd:string ;
    rdfs:subClassOf nell:sportsevent .

nell:organizationacronymhasname rdfs:comment "this short name or acronym refers to this organization"^^xsd:string ;
    rdfs:domain nell:organization ;
    rdfs:range nell:organization ;
    rdfs:subPropertyOf nell:organizationalsoknownas .

nell:organizationcreatedatdate rdfs:comment "The date on which a given organization was founded"^^xsd:string ;
    rdfs:domain nell:organization ;
    rdfs:range nell:date ;
    rdfs:subPropertyOf nell:atdate .

nell:organizationcreatedbyperson rdfs:comment "The person organization or geopoiltical entity that founded the given organization"^^xsd:string ;
    rdfs:domain nell:organization ;
    rdfs:range nell:person ;
    rdfs:subPropertyOf nell:createdbyagent .

nell:organizationdissolvedatdate rdfs:comment "The date on which a given organization was dissolved"^^xsd:string ;
    rdfs:domain nell:organization ;
    rdfs:range nell:date ;
    rdfs:subPropertyOf nell:atdate .

nell:organizationhasbuilding rdfs:comment "Which organization a building belongs to"^^xsd:string ;
    rdfs:domain nell:organization ;
    rdfs:range nell:building ;
    rdfs:subPropertyOf nell:organizationactsinlocation .

nell:organizationheadquarteredincountry rdfs:comment "The country where a given organization is headquartered"^^xsd:string ;
    rdfs:domain nell:organization ;
    rdfs:range nell:country ;
    rdfs:subPropertyOf nell:organizationactsinlocation .

nell:organizationheadquarteredinstateorprovince rdfs:comment "The state or province where a given organization is headquartered"^^xsd:string ;
    rdfs:domain nell:organization ;
    rdfs:range nell:stateorprovince ;
    rdfs:subPropertyOf nell:organizationactsinlocation .

nell:organizationhiredperson rdfs:comment "This relation connects an organization to individuals that it hired. It does include people hired as contractors not just people hired as employees. It does not include elected officials. It does not include organizations that may be hired for some particular purpose. Typically hiring someone does involve paying them though that is seldom stated explicitly when the relation is mentioned. A hiring event (the actual initiation of the employment) must be mentioned for this relation to apply; if the text just says that Mary Smith works for IBM that is not enough to assert a hired relation."^^xsd:string ;
    rdfs:domain nell:organization ;
    rdfs:range nell:person ;
    rdfs:subPropertyOf nell:worker .

nell:organizationnamehasacronym a owl:AsymmetricProperty,
        owl:IrreflexiveProperty ;
    rdfs:comment "this short name or acronym refers to this organization"^^xsd:string ;
    rdfs:domain nell:organization ;
    rdfs:range nell:organization ;
    rdfs:subPropertyOf nell:organizationalsoknownas .

nell:organizationterminatedperson rdfs:comment "This relation holds when the organization has teminated the employment relationship. This includes firings RIFs resignations and retirements. Normal ending of a contract does not constitute terminatedEmployment. A termination event (the endinf of the employment) must be mentioned for this relation to apply; if the text just says that Mary Smith used to work for IBM that is not enough to assert a terminatedEmployment relation."^^xsd:string ;
    rdfs:domain nell:organization ;
    rdfs:range nell:person ;
    rdfs:subPropertyOf nell:worker .

nell:ownedbyagent rdfs:comment "an agent owns any object animal product company etc."^^xsd:string ;
    rdfs:domain nell:everypromotedthing ;
    rdfs:range nell:humanagent ;
    rdfs:subPropertyOf nell:relatedto .

nell:parkincity rdfs:comment "The city a park is located in."^^xsd:string ;
    rdfs:domain nell:park ;
    rdfs:range nell:city ;
    rdfs:subPropertyOf nell:attractionofcity .

nell:parlourgame rdfs:comment "Parlour games drawing room games car games and similar passtimes that are not card games dice games board games etc."^^xsd:string ;
    rdfs:subClassOf nell:traditionalgame .

nell:perceptionaction rdfs:comment "An event that involves someone perceiving something"^^xsd:string ;
    rdfs:subClassOf nell:abstractthing .

nell:perceptionevent rdfs:comment "Something that can be perceived by someone."^^xsd:string ;
    rdfs:subClassOf nell:abstractthing .

nell:personafricacanbethesameaswriter rdfs:comment "Describes writers that are the same instances as personafrica"^^xsd:string ;
    rdfs:domain nell:personafrica ;
    rdfs:range nell:writer ;
    rdfs:subPropertyOf nell:canbethesameas .

nell:personalcareitem rdfs:comment "Items used by people to care for their bodies or to maintain a certain appearance. Could also be called toiletries."^^xsd:string ;
    rdfs:subClassOf nell:product,
        nell:visualizableobject .

nell:personantarctica rdfs:comment "Placeholder in case we change the definition of personByLocation categories such that there would be anyone to put here (there are no countries in Antarctica of which to be a citizen)."^^xsd:string ;
    rdfs:subClassOf nell:personbylocation .

nell:personasia rdfs:comment "citizens of countries in Asia"^^xsd:string ;
    rdfs:subClassOf nell:personbylocation .

nell:personaustralia rdfs:comment "citizens of Australia"^^xsd:string ;
    rdfs:subClassOf nell:personbylocation .

nell:personbirthdate rdfs:comment "the date on which this person was born"^^xsd:string ;
    rdfs:domain nell:person ;
    rdfs:range nell:dateliteral ;
    rdfs:subPropertyOf nell:atdate .

nell:personbornincountry rdfs:comment "the country that a person was born in"^^xsd:string ;
    rdfs:domain nell:person ;
    rdfs:range nell:country ;
    rdfs:subPropertyOf nell:personborninlocation .

nell:personborninstateorprovince rdfs:comment "the state or province that a person was born in"^^xsd:string ;
    rdfs:domain nell:person ;
    rdfs:range nell:stateorprovince ;
    rdfs:subPropertyOf nell:personborninlocation .

nell:personcanada rdfs:comment "citizens of Canada"^^xsd:string ;
    rdfs:subClassOf nell:personnorthamerica .

nell:personchargedwithcrime rdfs:comment "Charges or crimes (alleged or convicted) of the given person"^^xsd:string ;
    rdfs:domain nell:person ;
    rdfs:range nell:crimeorcharge ;
    rdfs:subPropertyOf nell:agentparticipatedinevent .

nell:persondeathdate rdfs:comment "the date on which this person died"^^xsd:string ;
    rdfs:domain nell:person ;
    rdfs:range nell:dateliteral ;
    rdfs:subPropertyOf nell:atdate .

nell:persondiedatage rdfs:comment "the age at which this person died"^^xsd:string ;
    rdfs:domain nell:person ;
    rdfs:range nell:nonneginteger ;
    rdfs:subPropertyOf nell:relatedto .

nell:persondiedincity rdfs:comment "the city that a person died in"^^xsd:string ;
    rdfs:domain nell:person ;
    rdfs:range nell:city ;
    rdfs:subPropertyOf nell:persondiedinlocation .

nell:persondiedincountry a owl:FunctionalProperty ;
    rdfs:comment "the country that a person died in"^^xsd:string ;
    rdfs:domain nell:person ;
    rdfs:range nell:country ;
    rdfs:subPropertyOf nell:persondiedinlocation .

nell:persondiedinstateorprovince rdfs:comment "the state or province that a person died in"^^xsd:string ;
    rdfs:domain nell:person ;
    rdfs:range nell:stateorprovince ;
    rdfs:subPropertyOf nell:persondiedinlocation .

nell:personeurope rdfs:comment "citizens of countries in Europe"^^xsd:string ;
    rdfs:subClassOf nell:personbylocation .

nell:persongraduatedfromuniversity rdfs:comment "Describes the people graduated from a university"^^xsd:string ;
    rdfs:domain nell:person ;
    rdfs:range nell:university ;
    rdfs:subPropertyOf nell:persongraduatedschool .

nell:personhasage rdfs:comment "the age of this person"^^xsd:string ;
    rdfs:domain nell:person ;
    rdfs:range nell:nonneginteger ;
    rdfs:subPropertyOf nell:relatedto .

nell:personhasbiologicalfather rdfs:comment "is biological father of a person"^^xsd:string ;
    rdfs:domain nell:person ;
    rdfs:range nell:male ;
    rdfs:subPropertyOf nell:createdbyagent,
        nell:personhasfather .

nell:personhasbiologicalmother rdfs:comment "is biological mother of a person"^^xsd:string ;
    rdfs:domain nell:person ;
    rdfs:range nell:female ;
    rdfs:subPropertyOf nell:createdbyagent,
        nell:personhasmother .

nell:personhascitizenship rdfs:comment "the citizenship of a person"^^xsd:string ;
    rdfs:domain nell:person ;
    rdfs:range nell:country ;
    rdfs:subPropertyOf nell:agentrelatedtolocation .

nell:personhasethnicity rdfs:comment "The ethnicity of a person"^^xsd:string ;
    rdfs:domain nell:person ;
    rdfs:range nell:ethnicgroup ;
    rdfs:subPropertyOf nell:relatedto .

nell:personhasjobposition rdfs:comment "This relation holds when the person has held the position at some point in some organization."^^xsd:string ;
    rdfs:domain nell:person ;
    rdfs:range nell:jobposition ;
    rdfs:subPropertyOf nell:relatedto .

nell:personhasreligion rdfs:comment "The religion to which a person has belonged."^^xsd:string ;
    rdfs:domain nell:person ;
    rdfs:range nell:religion ;
    rdfs:subPropertyOf nell:relatedto .

nell:personhasresidenceincity rdfs:comment "the city that a person has residence in"^^xsd:string ;
    rdfs:domain nell:person ;
    rdfs:range nell:city ;
    rdfs:subPropertyOf nell:personhasresidenceinlocation .

nell:personhasresidenceincountry rdfs:comment "the country that a person has residence in"^^xsd:string ;
    rdfs:domain nell:person ;
    rdfs:range nell:country ;
    rdfs:subPropertyOf nell:personhasresidenceinlocation .

nell:personhasresidenceingeopoliticallocation rdfs:comment "the geopolitical location that person has residence in"^^xsd:string ;
    rdfs:domain nell:person ;
    rdfs:range nell:geopoliticallocation ;
    rdfs:subPropertyOf nell:personhasresidenceinlocation .

nell:personhasresidenceinstateorprovince rdfs:comment "the state or province that a person has residence in"^^xsd:string ;
    rdfs:domain nell:person ;
    rdfs:range nell:stateorprovince ;
    rdfs:subPropertyOf nell:personhasresidenceinlocation .

nell:personhiredbyorganization rdfs:comment "This relation connects an organization to individuals that it hired. It does include people hired as contractors not just people hired as employees. It does not include elected officials. It does not include organizations that may be hired for some particular purpose. Typically hiring someone does involve paying them though that is seldom stated explicitly when the relation is mentioned. A hiring event (the actual initiation of the employment) must be mentioned for this relation to apply; if the text just says that Mary Smith works for IBM that is not enough to assert a hired relation."^^xsd:string ;
    rdfs:domain nell:person ;
    rdfs:range nell:organization ;
    rdfs:subPropertyOf nell:worksfor .

nell:personinacademicfield rdfs:comment "People trained or active in a given academic field"^^xsd:string ;
    rdfs:domain nell:person ;
    rdfs:range nell:academicfield ;
    rdfs:subPropertyOf nell:relatedto .

nell:personineconomicsector rdfs:comment "People who work in a given economic sector"^^xsd:string ;
    rdfs:domain nell:person ;
    rdfs:range nell:economicsector ;
    rdfs:subPropertyOf nell:relatedto .

nell:personleadscity rdfs:comment "specifies that a particular person is the leader (e.g. Mayor) of a particular city"^^xsd:string ;
    rdfs:domain nell:politician ;
    rdfs:range nell:city ;
    rdfs:subPropertyOf nell:personleadsgeopoliticalorganization .

nell:personleadscountry rdfs:comment "specifies that a particular person is the leader of a particular country"^^xsd:string ;
    rdfs:domain nell:politician ;
    rdfs:range nell:country ;
    rdfs:subPropertyOf nell:agentcontrols,
        nell:agentrelatedtolocation,
        nell:proxyfor .

nell:personmexico rdfs:comment "citizens of Mexico"^^xsd:string ;
    rdfs:subClassOf nell:personnorthamerica .

nell:personsouthamerica rdfs:comment "citizens of countries in South America"^^xsd:string ;
    rdfs:subClassOf nell:personbylocation .

nell:personspeakingatmeetingeventtitle rdfs:comment "Who will be speaking at a particular meeting"^^xsd:string ;
    rdfs:domain nell:person ;
    rdfs:range nell:meetingeventtitle ;
    rdfs:subPropertyOf nell:agentparticipatedinevent .

nell:personterminatedbyorganization rdfs:comment "This relation holds when the organization has teminated the employment relationship. This includes firings RIFs resignations and retirements. Normal ending of a contract does not constitute terminatedEmployment. A termination event (the endinf of the employment) must be mentioned for this relation to apply; if the text just says that Mary Smith used to work for IBM that is not enough to assert a terminatedEmployment relation."^^xsd:string ;
    rdfs:domain nell:person ;
    rdfs:range nell:organization ;
    rdfs:subPropertyOf nell:worksfor .

nell:personwrittenaboutinpublication rdfs:comment "Specifies that a particular person has been written about in a particular publication"^^xsd:string ;
    rdfs:domain nell:person ;
    rdfs:range nell:publication ;
    rdfs:subPropertyOf nell:relatedto .

nell:petroleumrefiningcompany rdfs:comment "a company in the petroleum sector"^^xsd:string ;
    rdfs:subClassOf nell:company .

nell:physicalaction rdfs:comment "An event that involves someone doing something with their physical body."^^xsd:string ;
    rdfs:subClassOf nell:abstractthing .

nell:physicalcharacteristic rdfs:comment "Features of a substance that are primarily sensory (physical) and generally measurable (businessdictionary.com)"^^xsd:string ;
    rdfs:subClassOf nell:abstractthing .

nell:physicsterm rdfs:comment "Any word with a specific meaning in the physics domain"^^xsd:string ;
    rdfs:subClassOf nell:abstractthing .

nell:physiologicalconditionpossiblytreatedbydrug rdfs:comment "relates a substance to a condition that it might treat. This relation includes conditions that the substance has been designed or approved to treat as well as conditions for which it is being investigated as a possible treatment.  Common folk remedies would also be eligible for this relation.  For example it would be reasonable to say that \"chicken noodle soup\" is a possible treatment for \"colds\"."^^xsd:string ;
    rdfs:domain nell:physiologicalcondition ;
    rdfs:range nell:drug ;
    rdfs:subPropertyOf nell:relatedto .

nell:physiologicalconditionstudedbyperson rdfs:comment "This predicate holds between a HumanAgent and a condition and means that the HumanAgent performs research related to condition."^^xsd:string ;
    rdfs:domain nell:physiologicalcondition ;
    rdfs:range nell:person ;
    rdfs:subPropertyOf nell:relatedto .

nell:placeofworshippracticesreligion rdfs:comment "The religion practied in a place of worship."^^xsd:string ;
    rdfs:domain nell:placeofworship ;
    rdfs:range nell:religion ;
    rdfs:subPropertyOf nell:locatedat .

nell:planet rdfs:comment "is a celestial body orbiting a star or stellar remnant that is massive enough to be rounded by its own gravity is not massive enough to cause thermonuclear fusion and has cleared its neighbouring region of planetesimals"^^xsd:string ;
    rdfs:subClassOf nell:location .

nell:plantgrowinginplant rdfs:comment "Describes the plants that grow on other plants"^^xsd:string ;
    rdfs:domain nell:plant ;
    rdfs:range nell:plant ;
    rdfs:subPropertyOf nell:relatedto .

nell:plantincludeplant a owl:AsymmetricProperty,
        owl:IrreflexiveProperty ;
    rdfs:comment "Describes the subcategories of a plant"^^xsd:string ;
    rdfs:domain nell:plant ;
    rdfs:range nell:plant ;
    rdfs:subPropertyOf nell:generalizationof .

nell:plantrepresentemotion rdfs:comment "Describes the emotions represented by a plant"^^xsd:string ;
    rdfs:domain nell:plant ;
    rdfs:range nell:emotion ;
    rdfs:subPropertyOf nell:relatedto .

nell:poem rdfs:comment "This type is for all kinds of poems from epics to doggerel."^^xsd:string ;
    rdfs:subClassOf nell:creativework .

nell:politicalgroupofpoliticianus rdfs:comment "U.S. Politician who is member of a political group"^^xsd:string ;
    rdfs:domain nell:politicsgroup ;
    rdfs:range nell:politicianus ;
    rdfs:subPropertyOf nell:politicalgroupofpolitician .

nell:politicalofficecanbethesameasjobposition rdfs:comment "Describes two instances that are the same thing in these two different categories"^^xsd:string ;
    rdfs:domain nell:politicaloffice ;
    rdfs:range nell:jobposition ;
    rdfs:subPropertyOf nell:canbethesameas .

nell:politicalparty rdfs:comment "organized political group that primarily aims for the attainment of political power and public office for its designated members."^^xsd:string ;
    rdfs:subClassOf nell:nongovorganization .

nell:politicianrepresentslocation rdfs:comment "Describes the city state country or other location represented by a politician"^^xsd:string ;
    rdfs:domain nell:politician ;
    rdfs:range nell:location ;
    rdfs:subPropertyOf nell:agentrelatedtolocation .

nell:politicianusendorsedbypoliticianus rdfs:comment "U.S. Politician that endorses another U.S. politician"^^xsd:string ;
    rdfs:domain nell:politicianus ;
    rdfs:range nell:politicianus ;
    rdfs:subPropertyOf nell:politicianendorsedbypolitician .

nell:politicianusendorsespoliticianus a owl:IrreflexiveProperty ;
    rdfs:comment "U.S. Politician that endorses another U.S. politician"^^xsd:string ;
    rdfs:domain nell:politicianus ;
    rdfs:range nell:politicianus ;
    rdfs:subPropertyOf nell:politicianendorsespolitician .

nell:politicianusholdsoffice rdfs:comment "U.S. Politician who holds an office"^^xsd:string ;
    rdfs:domain nell:politicianus ;
    rdfs:range nell:politicaloffice ;
    rdfs:subPropertyOf nell:politicianholdsoffice .

nell:politicianusmemberofpoliticalgroup rdfs:comment "U.S. Politician who is member of a political group"^^xsd:string ;
    rdfs:domain nell:politicianus ;
    rdfs:range nell:politicsgroup ;
    rdfs:subPropertyOf nell:politicianmemberofpoliticsgroup .

nell:politicianussponsoredpoliticsbill rdfs:comment "U.S. Politician sponsoring a particular legislative bill"^^xsd:string ;
    rdfs:domain nell:politicianus ;
    rdfs:range nell:politicsbill ;
    rdfs:subPropertyOf nell:politiciansponsoredpoliticsbill .

nell:politicianuswenttoschool rdfs:comment "Describes the school where a US politician studied"^^xsd:string ;
    rdfs:domain nell:politicianus ;
    rdfs:range nell:school ;
    rdfs:subPropertyOf nell:relatedto .

nell:politicsbillconcernsissue rdfs:comment "Issues that a legislative billl is concerned with."^^xsd:string ;
    rdfs:domain nell:politicsbill ;
    rdfs:range nell:politicsissue ;
    rdfs:subPropertyOf nell:relatedto .

nell:politicsbillsponsoredbypoliticianus rdfs:comment "U.S. Politician sponsoring a particular legislative bill"^^xsd:string ;
    rdfs:domain nell:politicsbill ;
    rdfs:range nell:politicianus ;
    rdfs:subPropertyOf nell:politicsbillsponsoredbypolitician .

nell:politicsblog rdfs:comment "A blog substantially and charactarizably but not exclusively devoted to politics or political issues.  A general current-events blog such as might be equated with a general newspaper should not be classified as a politicsBlog although an identifyable subsection or the blog of a particular staff member could be."^^xsd:string ;
    rdfs:subClassOf nell:blog .

nell:politicsgroupconcernsissue rdfs:comment "Issues that a political group has concern about"^^xsd:string ;
    rdfs:domain nell:politicsgroup ;
    rdfs:range nell:politicsissue ;
    rdfs:subPropertyOf nell:relatedto .

nell:port rdfs:comment "a location on a coast or shore containing one or more harbors where ships can dock and transfer people or cargo to or from land. Port locations are selected to optimize access to land and navigable water for commercial demand and for shelter from wind and waves. Ports with deeper water are rarer but can handle larger more economical ships. Since ports throughout history handled every kind of traffic support and storage facilities vary widely may extend for miles and dominate the local economy. Some ports have an important perhaps exclusively military role."^^xsd:string ;
    rdfs:subClassOf nell:attraction .

nell:predecessorofproductlaunch rdfs:domain nell:product ;
    rdfs:range nell:productlaunchevent ;
    rdfs:subPropertyOf nell:relatedto .

nell:priceofproductlaunch rdfs:domain nell:nonneginteger ;
    rdfs:range nell:productlaunchevent ;
    rdfs:subPropertyOf nell:relatedto .

nell:prodctlaunchingproductcompetitor rdfs:domain nell:productlaunchevent ;
    rdfs:range nell:product ;
    rdfs:subPropertyOf nell:relatedto .

nell:prodctlaunchingproductprice rdfs:domain nell:productlaunchevent ;
    rdfs:range nell:nonneginteger ;
    rdfs:subPropertyOf nell:relatedto .

nell:producesproducttype rdfs:comment "Specifies that a particular compnay produces a particular type of product"^^xsd:string ;
    rdfs:domain nell:company ;
    rdfs:range nell:item ;
    rdfs:subPropertyOf nell:agentcreated,
        nell:agentinvolvedwithitem .

nell:productbeinglauched rdfs:domain nell:productlaunchevent ;
    rdfs:range nell:product ;
    rdfs:subPropertyOf nell:relatedto .

nell:productinstanceof rdfs:comment "Specifies that a particular product is a particular kind of thing"^^xsd:string ;
    rdfs:domain nell:product ;
    rdfs:range nell:item ;
    rdfs:subPropertyOf nell:specializationof .

nell:productinstances rdfs:comment "Specifies that a particular product is a particular kind of thing"^^xsd:string ;
    rdfs:domain nell:item ;
    rdfs:range nell:product ;
    rdfs:subPropertyOf nell:generalizationof .

nell:productlauchcompetingcompany rdfs:domain nell:productlaunchevent ;
    rdfs:range nell:company ;
    rdfs:subPropertyOf nell:relatedto .

nell:productlauchpredecessor rdfs:domain nell:productlaunchevent ;
    rdfs:range nell:product ;
    rdfs:subPropertyOf nell:relatedto .

nell:productlauchvenue rdfs:domain nell:productlaunchevent ;
    rdfs:range nell:location ;
    rdfs:subPropertyOf nell:relatedto .

nell:productofproductlaunch rdfs:domain nell:product ;
    rdfs:range nell:productlaunchevent ;
    rdfs:subPropertyOf nell:relatedto .

nell:productproducedincountry rdfs:comment "Describes the products produced by a country"^^xsd:string ;
    rdfs:domain nell:product ;
    rdfs:range nell:country ;
    rdfs:subPropertyOf nell:itemexistsatlocation .

nell:producttypeofproductlaunch rdfs:domain nell:product ;
    rdfs:range nell:productlaunchevent ;
    rdfs:subPropertyOf nell:relatedto .

nell:professionactsatthesameareaofpoliticissue rdfs:comment "Describes professions that work at the area of a political issue"^^xsd:string ;
    rdfs:domain nell:politicsissue ;
    rdfs:range nell:profession ;
    rdfs:subPropertyOf nell:relatedto .

nell:professionalorganization rdfs:comment "A professional organization is an organization of people who work in a particular field."^^xsd:string ;
    rdfs:subClassOf nell:organization .

nell:professionistypeofprofession rdfs:comment "Type-specific generalization of professions."^^xsd:string ;
    rdfs:domain nell:profession ;
    rdfs:range nell:profession ;
    rdfs:subPropertyOf nell:specializationof .

nell:professionssuchasprofessions rdfs:comment "Describes the professions types that are generalizations of specific professions"^^xsd:string ;
    rdfs:domain nell:profession ;
    rdfs:range nell:profession ;
    rdfs:subPropertyOf nell:generalizationof .

nell:professiontypehasprofession a owl:AsymmetricProperty,
        owl:IrreflexiveProperty ;
    rdfs:comment "Type-specific generalization of professions."^^xsd:string ;
    rdfs:domain nell:profession ;
    rdfs:range nell:profession ;
    rdfs:subPropertyOf nell:generalizationof .

nell:professionusestool rdfs:comment "those who practice this profession use this tool"^^xsd:string ;
    rdfs:domain nell:profession ;
    rdfs:range nell:tool ;
    rdfs:subPropertyOf nell:relatedto .

nell:professor rdfs:comment "A faculty member at a university or college"^^xsd:string ;
    rdfs:subClassOf nell:person .

nell:protestcomentedby rdfs:domain nell:protestevent ;
    rdfs:range nell:person ;
    rdfs:subPropertyOf nell:relatedto .

nell:protestdamaged rdfs:domain nell:protestevent ;
    rdfs:range nell:geolocatablething ;
    rdfs:subPropertyOf nell:relatedto .

nell:protesteventtime rdfs:domain nell:protestevent ;
    rdfs:range nell:time ;
    rdfs:subPropertyOf nell:relatedto .

nell:protesthadactor rdfs:domain nell:protestevent ;
    rdfs:range nell:person ;
    rdfs:subPropertyOf nell:relatedto .

nell:protesthadvictim rdfs:domain nell:protestevent ;
    rdfs:range nell:person ;
    rdfs:subPropertyOf nell:relatedto .

nell:protesthadweapon rdfs:domain nell:protestevent ;
    rdfs:range nell:weapon ;
    rdfs:subPropertyOf nell:relatedto .

nell:protestinjured rdfs:domain nell:protestevent ;
    rdfs:range nell:person ;
    rdfs:subPropertyOf nell:relatedto .

nell:protestinjurednumber rdfs:domain nell:protestevent ;
    rdfs:range nell:nonneginteger ;
    rdfs:subPropertyOf nell:relatedto .

nell:protestocurredin rdfs:domain nell:protestevent ;
    rdfs:range nell:location ;
    rdfs:subPropertyOf nell:relatedto .

nell:publicationjournalist rdfs:comment "specifies that a particular journalist writes for a particular publication"^^xsd:string ;
    rdfs:domain nell:publication ;
    rdfs:range nell:journalist ;
    rdfs:subPropertyOf nell:worker .

nell:publicationpublishedinmagazine rdfs:comment "Magazine in which a publication was published in"^^xsd:string ;
    rdfs:domain nell:publication ;
    rdfs:range nell:magazine ;
    rdfs:subPropertyOf nell:subpartof .

nell:publicationwritesabout rdfs:comment "Specifies that a particular person has been written about in a particular publication"^^xsd:string ;
    rdfs:domain nell:publication ;
    rdfs:range nell:person ;
    rdfs:subPropertyOf nell:relatedto .

nell:race rdfs:comment "A sport race is a competition of speed against an objective criterion usually a clock or to a specific point. The competitors in a race try to complete a given task in the shortest amount of time. Typically this involves traversing some distance but it can be any other task involving speed to reach a specific goal."^^xsd:string ;
    rdfs:subClassOf nell:sportsevent .

nell:radiostationincity rdfs:comment "Specifies that a particular radio station is headquarted in a particular city"^^xsd:string ;
    rdfs:domain nell:radiostation ;
    rdfs:range nell:city ;
    rdfs:subPropertyOf nell:hasofficeincity .

nell:reasonofcollision rdfs:domain nell:everypromotedthing ;
    rdfs:range nell:roadaccidentevent ;
    rdfs:subPropertyOf nell:relatedto .

nell:recipe rdfs:comment "A recipe is a method of preparing a dish. Dishes may have multiple recipes. For instance there may be many different recipes for chocolate chip cookies."^^xsd:string ;
    rdfs:subClassOf nell:abstractthing .

nell:recordlabel rdfs:comment "A record label is a company that releases music albums."^^xsd:string ;
    rdfs:subClassOf nell:mediacompany .

nell:refineryproduct rdfs:comment "a product derived from a petroleum refinery"^^xsd:string ;
    rdfs:subClassOf nell:item .

nell:releasedateexpectedfordrug rdfs:comment "This predicate represents the relationship between a pharmaceutical substance and the date when it is expected to be approved for legal marketing. For our purposes the date will typically correspond to a date for FDA approval but the relationship itself is not restricted to approval for sale in the United States."^^xsd:string ;
    rdfs:domain nell:date ;
    rdfs:range nell:drug ;
    rdfs:subPropertyOf nell:dateof .

nell:religionofperson rdfs:comment "The religion to which a person has belonged."^^xsd:string ;
    rdfs:domain nell:religion ;
    rdfs:range nell:person ;
    rdfs:subPropertyOf nell:relatedto .

nell:religionssuchasreligions rdfs:comment "Describes the religions types that are generalizations of specific religions"^^xsd:string ;
    rdfs:domain nell:religion ;
    rdfs:range nell:religion ;
    rdfs:subPropertyOf nell:generalizationof .

nell:religionusesplaceofworship rdfs:comment "The religion practied in a place of worship."^^xsd:string ;
    rdfs:domain nell:religion ;
    rdfs:range nell:placeofworship ;
    rdfs:subPropertyOf nell:atlocation .

nell:reptile rdfs:comment "Reptiles are animals in the (Linnaean) class Reptilia. They are characterized by breathing air laying tough-shelled amniotic eggs and having skin covered in scales and/or scutes."^^xsd:string ;
    rdfs:subClassOf nell:vertebrate .

nell:researchproject rdfs:comment "A specific research effort or a research center"^^xsd:string ;
    rdfs:subClassOf nell:abstractthing .

nell:restaurantincity rdfs:comment "The city a restaurant is located in."^^xsd:string ;
    rdfs:domain nell:restaurant ;
    rdfs:range nell:city ;
    rdfs:subPropertyOf nell:buildinglocatedincity .

nell:restaurantlocatedinskyscraper rdfs:comment "Describes restaurants located in skyscrapers"^^xsd:string ;
    rdfs:domain nell:restaurant ;
    rdfs:range nell:skyscraper ;
    rdfs:subPropertyOf nell:locationlocatedwithinlocation .

nell:retailstore rdfs:comment "Brick & mortar retail stores and franchises. Retail means selling goods not services (e.g. prepared food)"^^xsd:string ;
    rdfs:subClassOf nell:building .

nell:riveremptiesintoriver a owl:AsymmetricProperty,
        owl:IrreflexiveProperty ;
    rdfs:comment "Describes the tributaries of a river"^^xsd:string ;
    rdfs:domain nell:river ;
    rdfs:range nell:river ;
    rdfs:subPropertyOf nell:atlocation .

nell:riverflowsthroughcity rdfs:comment "Rivers that flow or through or immediately adjacent to the city."^^xsd:string ;
    rdfs:domain nell:river ;
    rdfs:range nell:city ;
    rdfs:subPropertyOf nell:locatedat .

nell:roadaccidentcasualtiesnumber rdfs:domain nell:roadaccidentevent ;
    rdfs:range nell:nonneginteger ;
    rdfs:subPropertyOf nell:relatedto .

nell:roadaccidentcomentedby rdfs:domain nell:roadaccidentevent ;
    rdfs:range nell:person ;
    rdfs:subPropertyOf nell:relatedto .

nell:roadaccidenteventtime rdfs:domain nell:roadaccidentevent ;
    rdfs:range nell:time ;
    rdfs:subPropertyOf nell:relatedto .

nell:roadaccidenthadguilty rdfs:domain nell:roadaccidentevent ;
    rdfs:range nell:person ;
    rdfs:subPropertyOf nell:relatedto .

nell:roadaccidenthadreason rdfs:domain nell:roadaccidentevent ;
    rdfs:range nell:everypromotedthing ;
    rdfs:subPropertyOf nell:relatedto .

nell:roadaccidenthadvictim rdfs:domain nell:roadaccidentevent ;
    rdfs:range nell:person ;
    rdfs:subPropertyOf nell:relatedto .

nell:roadaccidentinjured rdfs:domain nell:roadaccidentevent ;
    rdfs:range nell:person ;
    rdfs:subPropertyOf nell:relatedto .

nell:roadaccidentinjurednumber rdfs:domain nell:roadaccidentevent ;
    rdfs:range nell:nonneginteger ;
    rdfs:subPropertyOf nell:relatedto .

nell:roadaccidentocurredin rdfs:domain nell:roadaccidentevent ;
    rdfs:range nell:location ;
    rdfs:subPropertyOf nell:relatedto .

nell:roomcancontainfurniture rdfs:comment "Relates furniture to rooms in which it is often found"^^xsd:string ;
    rdfs:domain nell:room ;
    rdfs:range nell:furniture ;
    rdfs:subPropertyOf nell:roomcancontainitem .

nell:scenecontainsobject rdfs:comment "Object found in scene (NEIL)"^^xsd:string ;
    rdfs:domain nell:visualizablescene ;
    rdfs:range nell:visualizableobject ;
    rdfs:subPropertyOf nell:relatedto .

nell:scientistcanbethesameaswriter rdfs:comment "Describes two instances that are the same thing in these two different categories"^^xsd:string ;
    rdfs:domain nell:scientist ;
    rdfs:range nell:writer ;
    rdfs:subPropertyOf nell:canbethesameas .

nell:scoreofsportsgame rdfs:comment "the score of this game"^^xsd:string ;
    rdfs:domain nell:gamescore ;
    rdfs:range nell:sportsgame ;
    rdfs:subPropertyOf nell:relatedto .

nell:securityinbombing rdfs:domain nell:agent ;
    rdfs:range nell:bombingevent ;
    rdfs:subPropertyOf nell:relatedto .

nell:shapeofobject rdfs:comment "Object has shape (NEIL)"^^xsd:string ;
    rdfs:domain nell:geometricshape ;
    rdfs:range nell:visualizablething ;
    rdfs:subPropertyOf nell:relatedto .

nell:shoppingmallincity rdfs:comment "The city a shopping mall is located in."^^xsd:string ;
    rdfs:domain nell:shoppingmall ;
    rdfs:range nell:city ;
    rdfs:subPropertyOf nell:buildinglocatedincity .

nell:sideeffectcausedbydrug rdfs:comment "This predicate indicates that the use of a drug has a physiologicalCondition as a side-effect. Uses of this predicate may include both very common side-effects and rare but reported side-effects."^^xsd:string ;
    rdfs:domain nell:physiologicalcondition ;
    rdfs:range nell:drug ;
    rdfs:subPropertyOf nell:relatedto .

nell:sisterof rdfs:comment "person has a sister"^^xsd:string ;
    rdfs:domain nell:female ;
    rdfs:range nell:person ;
    rdfs:subPropertyOf nell:hassibling .

nell:skyscrapercontainsrestaurant rdfs:comment "Describes restaurants located in skyscrapers"^^xsd:string ;
    rdfs:domain nell:skyscraper ;
    rdfs:range nell:restaurant ;
    rdfs:subPropertyOf nell:locationcontainslocation .

nell:sociopolitical rdfs:comment "Any socio-political word (?!)"^^xsd:string ;
    rdfs:subClassOf nell:abstractthing .

nell:softwareisprogrammedinprogramminglanguage rdfs:comment "Relates a software to its programming language"^^xsd:string ;
    rdfs:domain nell:software ;
    rdfs:range nell:programminglanguage ;
    rdfs:subPropertyOf nell:relatedto .

nell:sourceofearthquake rdfs:domain nell:everypromotedthing ;
    rdfs:range nell:earthquakeevent ;
    rdfs:subPropertyOf nell:relatedto .

nell:sportfansincountry rdfs:comment "Describes the sports that have fans living in a country"^^xsd:string ;
    rdfs:domain nell:sport ;
    rdfs:range nell:country ;
    rdfs:subPropertyOf nell:relatedto .

nell:sporthassportsteamposition rdf:first <http://www.semanticweb.org/ontologies/NELL#_:y17> ;
    rdfs:comment "The relation between a sport and team positions filled by athletes"^^xsd:string ;
    rdfs:domain nell:sport ;
    rdfs:range nell:sportsteamposition ;
    rdfs:subPropertyOf nell:relatedto .

nell:sportnamehasoriginlanguage rdfs:comment "Describes the origin language of the sports name"^^xsd:string ;
    rdfs:domain nell:sport ;
    rdfs:range nell:language ;
    rdfs:subPropertyOf nell:relatedto .

nell:sportschoolincountry rdfs:comment "Describes the sports practiced in a country"^^xsd:string ;
    rdfs:domain nell:sport ;
    rdfs:range nell:country ;
    rdfs:subPropertyOf nell:relatedto .

nell:sportsgameawayteam rdfs:comment "Specifies that a particular team is the away team in a particular sportsGame."^^xsd:string ;
    rdfs:domain nell:sportsgame ;
    rdfs:range nell:sportsteam ;
    rdfs:subPropertyOf nell:sportsgameteam .

nell:sportsgamedate rdfs:comment "the date on which this game occurred"^^xsd:string ;
    rdfs:domain nell:sportsgame ;
    rdfs:range nell:dateliteral ;
    rdfs:subPropertyOf nell:eventdate .

nell:sportsgamehometeam rdfs:comment "Specifies that a particular team is the home team in a particular sportsGame"^^xsd:string ;
    rdfs:domain nell:sportsgame ;
    rdfs:range nell:sportsteam ;
    rdfs:subPropertyOf nell:sportsgameteam .

nell:sportsgameloser rdfs:comment "Specifies that a particular team that played in a particular sportsGame was the loser thereof."^^xsd:string ;
    rdfs:domain nell:sportsgame ;
    rdfs:range nell:sportsteam ;
    rdfs:subPropertyOf nell:sportsgameteam .

nell:sportsgameloserscore rdfs:comment "Specifies the score with which the loosing team in a particular sportsGame lost."^^xsd:string ;
    rdfs:domain nell:sportsgame ;
    rdfs:range nell:nonneginteger ;
    rdfs:subPropertyOf nell:relatedto .

nell:sportsgamescore rdfs:comment "the score of this game"^^xsd:string ;
    rdfs:domain nell:sportsgame ;
    rdfs:range nell:gamescore ;
    rdfs:subPropertyOf nell:relatedto .

nell:sportsgamesport a owl:FunctionalProperty ;
    rdfs:comment "Specifies the sport that was played in a particular sportsGame."^^xsd:string ;
    rdfs:domain nell:sportsgame ;
    rdfs:range nell:sport ;
    rdfs:subPropertyOf nell:relatedto .

nell:sportsgamewinner rdfs:comment "Specifies that a particular team that played in a particular sportsGame was the winner thereof."^^xsd:string ;
    rdfs:domain nell:sportsgame ;
    rdfs:range nell:sportsteam ;
    rdfs:subPropertyOf nell:sportsgameteam .

nell:sportsgamewinnerscore rdfs:comment "Specifies the score with which the winning team in a particular sportsGame lost."^^xsd:string ;
    rdfs:domain nell:sportsgame ;
    rdfs:range nell:nonneginteger ;
    rdfs:subPropertyOf nell:relatedto .

nell:sportsportsgameexample rdfs:comment "Specifies the sport that was played in a particular sportsGame."^^xsd:string ;
    rdfs:domain nell:sport ;
    rdfs:range nell:sportsgame ;
    rdfs:subPropertyOf nell:relatedto .

nell:sportsteampositionathlete rdf:first <http://www.semanticweb.org/ontologies/NELL#_:y18> ;
    rdfs:comment "The team position played by an athlete."^^xsd:string ;
    rdfs:domain nell:sportsteamposition ;
    rdfs:range nell:athlete ;
    rdfs:subPropertyOf nell:relatedto .

nell:sportsteampositionforsport rdfs:comment "The relation between a sport and team positions filled by athletes"^^xsd:string ;
    rdfs:domain nell:sportsteamposition ;
    rdfs:range nell:sport ;
    rdfs:subPropertyOf nell:relatedto .

nell:sportsteampositionreceivedathlete rdfs:domain nell:sportsteamposition ;
    rdfs:range nell:athlete ;
    rdfs:subPropertyOf nell:relatedto .

nell:sportteam rdfs:comment "The sport that a team plays."^^xsd:string ;
    rdfs:domain nell:sport ;
    rdfs:range nell:sportsteam ;
    rdfs:subPropertyOf nell:relatedto .

nell:sportusesequipment rdfs:comment "Specifies equipment that is used by a particular sport."^^xsd:string ;
    rdfs:domain nell:sport ;
    rdfs:range nell:sportsequipment ;
    rdfs:subPropertyOf nell:relatedto .

nell:stadiumalsoknownas rdfs:comment "this is another name for this stadium or event venue"^^xsd:string ;
    rdfs:domain nell:stadiumoreventvenue ;
    rdfs:range nell:stadiumoreventvenue ;
    rdfs:subPropertyOf nell:synonymfor .

nell:stadiumhometeam rdfs:comment "The stadium or other sporting venue which a team designates as its \"home.\" Typically a large percentage of the team's games occur in this location."^^xsd:string ;
    rdfs:domain nell:stadiumoreventvenue ;
    rdfs:range nell:sportsteam ;
    rdfs:subPropertyOf nell:locationactedinbyorganization .

nell:stadiumhometoathlete rdfs:comment "a sports arena usually oval or horseshoe-shaped with tiers of seats for spectators (which is home for an athlete) "^^xsd:string ;
    rdfs:domain nell:stadiumoreventvenue ;
    rdfs:range nell:athlete ;
    rdfs:subPropertyOf nell:locationactedinbyagent .

nell:stadiumhometoleague rdfs:comment "specifies that a particular league uses a particular venue for its games"^^xsd:string ;
    rdfs:domain nell:stadiumoreventvenue ;
    rdfs:range nell:sportsleague ;
    rdfs:subPropertyOf nell:locationactedinbyorganization .

nell:stadiumhometosport rdfs:comment "Specifies that a particular sport is played in a particular venue"^^xsd:string ;
    rdfs:domain nell:stadiumoreventvenue ;
    rdfs:range nell:sport ;
    rdfs:subPropertyOf nell:relatedto .

nell:stadiumlocatedincity rdfs:comment "The city where a stadium is located"^^xsd:string ;
    rdfs:domain nell:stadiumoreventvenue ;
    rdfs:range nell:city ;
    rdfs:subPropertyOf nell:attractionofcity,
        nell:buildinglocatedincity,
        nell:proxyof .

nell:stadiumoreventvenuedisclosescompany rdfs:comment "Describes a stadium or event venue that discloses a company"^^xsd:string ;
    rdfs:domain nell:stadiumoreventvenue ;
    rdfs:range nell:company ;
    rdfs:subPropertyOf nell:relatedto .

nell:statecontainsfarm rdfs:comment "The state/province a farm is located in"^^xsd:string ;
    rdfs:domain nell:stateorprovince ;
    rdfs:range nell:farm ;
    rdfs:subPropertyOf nell:locationcontainslocation .

nell:statehascapital a owl:FunctionalProperty ;
    rdf:first <http://www.semanticweb.org/ontologies/NELL#_:y16>,
        <http://www.semanticweb.org/ontologies/NELL#_:y26>,
        <http://www.semanticweb.org/ontologies/NELL#_:y37> ;
    rdfs:comment "The capital city of a state where the main governing apparatus is located."^^xsd:string ;
    rdfs:domain nell:stateorprovince ;
    rdfs:range nell:city ;
    rdfs:subPropertyOf nell:proxyof,
        nell:statecontainscity .

nell:statehaslake rdfs:comment "The state/province a river is in."^^xsd:string ;
    rdfs:domain nell:stateorprovince ;
    rdfs:range nell:lake ;
    rdfs:subPropertyOf nell:locationcontainslocation .

nell:statehasmountain rdfs:comment "State/province a mountain is located in."^^xsd:string ;
    rdfs:domain nell:stateorprovince ;
    rdfs:range nell:mountain ;
    rdfs:subPropertyOf nell:locationcontainslocation .

nell:statelocatedincountry rdfs:comment "The country which the state or province is a part of."^^xsd:string ;
    rdfs:domain nell:stateorprovince ;
    rdfs:range nell:country ;
    rdfs:subPropertyOf nell:statelocatedingeopoliticallocation .

nell:stateorprovinceattainstrainstation rdfs:comment "Describes the trainstantions location (state or province)"^^xsd:string ;
    rdfs:domain nell:stateorprovince ;
    rdfs:range nell:trainstation ;
    rdfs:subPropertyOf nell:relatedto .

nell:stateorprovinceisborderedbystateorprovince a owl:IrreflexiveProperty,
        owl:SymmetricProperty ;
    rdfs:comment "Describes the states that borders a state"^^xsd:string ;
    rdfs:domain nell:stateorprovince ;
    rdfs:range nell:stateorprovince ;
    rdfs:subPropertyOf nell:relatedto .

nell:stateorprovinceofpersonbirth rdfs:comment "the state or province that a person was born in"^^xsd:string ;
    rdfs:domain nell:stateorprovince ;
    rdfs:range nell:person ;
    rdfs:subPropertyOf nell:locationofpersonbirth .

nell:stateorprovinceofpersondeath rdfs:comment "the state or province that a person died in"^^xsd:string ;
    rdfs:domain nell:stateorprovince ;
    rdfs:range nell:person ;
    rdfs:subPropertyOf nell:locationofpersondeath .

nell:stateorprovinceresidenceofperson rdfs:comment "the state or province that a person has residence in"^^xsd:string ;
    rdfs:domain nell:stateorprovince ;
    rdfs:range nell:person ;
    rdfs:subPropertyOf nell:locationresidenceofperson .

nell:streetincity rdfs:comment "this street is at least partly inside this city"^^xsd:string ;
    rdfs:domain nell:street ;
    rdfs:range nell:city ;
    rdfs:subPropertyOf nell:locationlocatedwithinlocation .

nell:subfieldofacademicfield rdfs:comment "Subfields within a given academic field"^^xsd:string ;
    rdfs:domain nell:academicfield ;
    rdfs:range nell:academicfield ;
    rdfs:subPropertyOf nell:subjectconcernedbyacademicfield,
        nell:subpartof .

nell:tableitem rdfs:comment "Any item that is commonly found on a table."^^xsd:string ;
    rdfs:subClassOf nell:householditem .

nell:targetinbombing rdfs:domain nell:everypromotedthing ;
    rdfs:range nell:bombingevent ;
    rdfs:subPropertyOf nell:relatedto .

nell:teamalsoknownas a owl:IrreflexiveProperty,
        owl:SymmetricProperty ;
    rdfs:comment "this is another name for this team"^^xsd:string ;
    rdfs:domain nell:sportsteam ;
    rdfs:range nell:sportsteam ;
    rdfs:subPropertyOf nell:organizationalsoknownas .

nell:teamcoach rdfs:comment "specifies that a particular coach coaches a particular team"^^xsd:string ;
    rdfs:domain nell:sportsteam ;
    rdfs:range nell:coach ;
    rdfs:subPropertyOf nell:worker .

nell:teammate a owl:IrreflexiveProperty,
        owl:SymmetricProperty ;
    rdfs:comment "Two athletes are teammates if they play on the same team."^^xsd:string ;
    rdfs:domain nell:athlete ;
    rdfs:range nell:athlete ;
    rdfs:subPropertyOf nell:agentcollaborateswithagent .

nell:teamplaysagainstteam a owl:IrreflexiveProperty,
        owl:SymmetricProperty ;
    rdfs:comment "Teams that play against each other competitively"^^xsd:string ;
    rdfs:domain nell:sportsteam ;
    rdfs:range nell:sportsteam ;
    rdfs:subPropertyOf nell:agentcompeteswithagent .

nell:teamplaysincity rdfs:comment "The home city of a sports team typically a location where the team frequently competes."^^xsd:string ;
    rdfs:domain nell:sportsteam ;
    rdfs:range nell:city ;
    rdfs:subPropertyOf nell:organizationactsinlocation,
        nell:proxyof .

nell:teamplaysinleague rdfs:comment "The league that a team plays in."^^xsd:string ;
    rdfs:domain nell:sportsteam ;
    rdfs:range nell:sportsleague ;
    rdfs:subPropertyOf nell:subpartoforganization .

nell:teamplayssport rdfs:comment "The sport that a team plays."^^xsd:string ;
    rdfs:domain nell:sportsteam ;
    rdfs:range nell:sport ;
    rdfs:subPropertyOf nell:relatedto .

nell:televisioncompanyaffiliate a owl:InverseFunctionalProperty ;
    rdfs:comment "The network that a TV station gets its programming from"^^xsd:string ;
    rdfs:domain nell:televisionnetwork ;
    rdfs:range nell:televisionstation ;
    rdfs:subPropertyOf nell:superpartoforganization .

nell:televisionshowisbasedonmovie rdfs:comment "Movie that a television show was based in"^^xsd:string ;
    rdfs:domain nell:televisionshow ;
    rdfs:range nell:movie ;
    rdfs:subPropertyOf nell:relatedto .

nell:televisionshowssuchastelevisionshows rdfs:comment "Describes the televisionshows types that are generalizations of specific televisionshows"^^xsd:string ;
    rdfs:domain nell:televisionshow ;
    rdfs:range nell:televisionshow ;
    rdfs:subPropertyOf nell:generalizationof .

nell:televisionstationaffiliatedwith rdfs:comment "The network that a TV station gets its programming from"^^xsd:string ;
    rdfs:domain nell:televisionstation ;
    rdfs:range nell:televisionnetwork ;
    rdfs:subPropertyOf nell:subpartoforganization .

nell:televisionstationincity rdfs:comment "The city where a TV station is located or broadcasts to."^^xsd:string ;
    rdfs:domain nell:televisionstation ;
    rdfs:range nell:city ;
    rdfs:subPropertyOf nell:hasofficeincity .

nell:terroristorganization rdfs:comment "an organization that is involved in terrorist activities."^^xsd:string ;
    rdfs:subClassOf nell:organization .

nell:thinghascolor rdfs:comment "Object has color (NEIL)"^^xsd:string ;
    rdfs:domain nell:visualizablething ;
    rdfs:range nell:color ;
    rdfs:subPropertyOf nell:relatedto .

nell:thinghasshape rdfs:comment "Object has shape (NEIL)"^^xsd:string ;
    rdfs:domain nell:visualizablething ;
    rdfs:range nell:geometricshape ;
    rdfs:subPropertyOf nell:relatedto .

nell:timeofbombing rdfs:domain nell:time ;
    rdfs:range nell:bombingevent ;
    rdfs:subPropertyOf nell:relatedto .

nell:timeofearthquake rdfs:domain nell:time ;
    rdfs:range nell:earthquakeevent ;
    rdfs:subPropertyOf nell:relatedto .

nell:timeofprotest rdfs:domain nell:time ;
    rdfs:range nell:protestevent ;
    rdfs:subPropertyOf nell:relatedto .

nell:timeofroadaccident rdfs:domain nell:time ;
    rdfs:range nell:roadaccidentevent ;
    rdfs:subPropertyOf nell:relatedto .

nell:toolssuchastools rdfs:comment "Describes the tools types that are generalizations of specific tools"^^xsd:string ;
    rdfs:domain nell:tool ;
    rdfs:range nell:tool ;
    rdfs:subPropertyOf nell:generalizationof .

nell:toolusedbyprofession rdfs:comment "those who practice this profession use this tool"^^xsd:string ;
    rdfs:domain nell:tool ;
    rdfs:range nell:profession ;
    rdfs:subPropertyOf nell:relatedto .

nell:touristattractionsuchastouristattraction rdfs:comment "Describes the specific tourist attraction types that are generalizations of tourist attractions"^^xsd:string ;
    rdfs:domain nell:attraction ;
    rdfs:range nell:attraction ;
    rdfs:subPropertyOf nell:generalizationof .

nell:tradeunion rdfs:comment "A trade union (aka labor union) is an organization which represents workers in a certain industry or profession."^^xsd:string ;
    rdfs:subClassOf nell:organization .

nell:trail rdfs:comment "Trails for hiking walking biking or even driving.  Routes with street addresses cannot be trails."^^xsd:string ;
    rdfs:subClassOf nell:location .

nell:trainstationincity rdfs:comment "The city a train station is in."^^xsd:string ;
    rdfs:domain nell:trainstation ;
    rdfs:range nell:city ;
    rdfs:subPropertyOf nell:locationlocatedwithinlocation .

nell:transportationincity a owl:FunctionalProperty ;
    rdfs:comment "City of a transportation system."^^xsd:string ;
    rdfs:domain nell:transportation ;
    rdfs:range nell:city ;
    rdfs:subPropertyOf nell:attractionofcity .

nell:trophywonbycoaches rdfs:comment "specifies that a particular coach coaches a team that won a particular award or trophy"^^xsd:string ;
    rdfs:domain nell:awardtrophytournament ;
    rdfs:range nell:coach ;
    rdfs:subPropertyOf nell:relatedto .

nell:trophywonbyteam rdfs:comment "Trophies that a team has won"^^xsd:string ;
    rdfs:domain nell:awardtrophytournament ;
    rdfs:range nell:sportsteam ;
    rdfs:subPropertyOf nell:relatedto .

nell:typeproducedby rdfs:comment "Specifies that a particular compnay produces a particular type of product"^^xsd:string ;
    rdfs:domain nell:item ;
    rdfs:range nell:company ;
    rdfs:subPropertyOf nell:createdbyagent,
        nell:iteminvolvedwithagent .

nell:universityhasacademicprogram rdfs:comment "this academic program is offered by this university"^^xsd:string ;
    rdfs:domain nell:university ;
    rdfs:range nell:academicfield ;
    rdfs:subPropertyOf nell:relatedto .

nell:universityincity rdfs:comment "The city a university is located in."^^xsd:string ;
    rdfs:domain nell:university ;
    rdfs:range nell:city ;
    rdfs:subPropertyOf nell:organizationactsinlocation .

nell:universityledmusicfestival rdfs:comment "identifies the university that led a Musical Festival"^^xsd:string ;
    rdfs:domain nell:university ;
    rdfs:range nell:musicfestival ;
    rdfs:subPropertyOf nell:agentparticipatedinevent .

nell:universityoperatesinlanguage rdfs:comment "Language spoken at a college/university."^^xsd:string ;
    rdfs:domain nell:university ;
    rdfs:range nell:language ;
    rdfs:subPropertyOf nell:relatedto .

nell:vegetablecanbeservedwithgrain rdfs:comment "Describes the vegetables that are usually served with a grain"^^xsd:string ;
    rdfs:domain nell:vegetable ;
    rdfs:range nell:grain ;
    rdfs:subPropertyOf nell:itemusedwithitem .

nell:vegetablecanbethesameasagriculturalproduct rdfs:comment "Describes two instances that are the same thing in these two different categories"^^xsd:string ;
    rdfs:domain nell:vegetable ;
    rdfs:range nell:agriculturalproduct ;
    rdfs:subPropertyOf nell:canbethesameas .

nell:vegetableisproducedatcountry rdfs:comment "Describes the countries that are big produces of vegetables"^^xsd:string ;
    rdfs:domain nell:vegetable ;
    rdfs:range nell:country ;
    rdfs:subPropertyOf nell:itemexistsatlocation .

nell:vegetableproductioninstateorprovince rdfs:comment "Describes the vegetables produced in a state or province"^^xsd:string ;
    rdfs:domain nell:vegetable ;
    rdfs:range nell:stateorprovince ;
    rdfs:subPropertyOf nell:itemexistsatlocation .

nell:vehicleistypeofvehicle rdfs:comment "Type-specific generalization of vehicles."^^xsd:string ;
    rdfs:domain nell:vehicle ;
    rdfs:range nell:vehicle ;
    rdfs:subPropertyOf nell:specializationof .

nell:vehicletypehasvehicle rdfs:comment "Type-specific generalization of vehicles."^^xsd:string ;
    rdfs:domain nell:vehicle ;
    rdfs:range nell:vehicle ;
    rdfs:subPropertyOf nell:generalizationof .

nell:vein rdfs:comment "A vein is a blood vessel that carries blood toward the heart."^^xsd:string ;
    rdfs:subClassOf nell:bodypart .

nell:venueofproductlaunch rdfs:domain nell:location ;
    rdfs:range nell:productlaunchevent ;
    rdfs:subPropertyOf nell:relatedto .

nell:victiminbombing rdfs:domain nell:person ;
    rdfs:range nell:bombingevent ;
    rdfs:subPropertyOf nell:relatedto .

nell:victiminearthquake rdfs:domain nell:victim ;
    rdfs:range nell:earthquakeevent ;
    rdfs:subPropertyOf nell:relatedto .

nell:victiminprotest rdfs:domain nell:person ;
    rdfs:range nell:protestevent ;
    rdfs:subPropertyOf nell:relatedto .

nell:victiminroadaccident rdfs:domain nell:person ;
    rdfs:range nell:roadaccidentevent ;
    rdfs:subPropertyOf nell:relatedto .

nell:videogamessuchasvideogames rdfs:comment "Describes the videogame types that are generalizations of specific videogames"^^xsd:string ;
    rdfs:domain nell:videogame ;
    rdfs:range nell:videogame ;
    rdfs:subPropertyOf nell:generalizationof .

nell:virus rdfs:comment "A small infectious agent that replicates only inside the living cells of other organisms"^^xsd:string ;
    rdfs:subClassOf nell:species .

nell:visualappearanceof rdfs:comment "The NEIL-learned visual appearance of something"^^xsd:string ;
    rdfs:domain nell:url ;
    rdfs:range nell:visualizablething ;
    rdfs:subPropertyOf nell:locatedat .

nell:visualartformartist rdfs:comment "The type of visual art that a visualArtist produces. Also known as an artist's medium."^^xsd:string ;
    rdfs:domain nell:visualartform ;
    rdfs:range nell:visualartist ;
    rdfs:subPropertyOf nell:relatedto .

nell:visualartistartform rdfs:comment "The type of visual art that a visualArtist produces. Also known as an artist's medium."^^xsd:string ;
    rdfs:domain nell:visualartist ;
    rdfs:range nell:visualartform ;
    rdfs:subPropertyOf nell:relatedto .

nell:visualartistartmovement rdfs:comment "The art movements or styles that a visualArtist is associated with."^^xsd:string ;
    rdfs:domain nell:visualartist ;
    rdfs:range nell:visualartmovement ;
    rdfs:subPropertyOf nell:relatedto .

nell:visualartmovementartist rdfs:comment "The art movements or styles that a visualArtist is associated with."^^xsd:string ;
    rdfs:domain nell:visualartmovement ;
    rdfs:range nell:visualartist ;
    rdfs:subPropertyOf nell:relatedto .

nell:wallitem rdfs:comment "Any item that is commonly found on a wall"^^xsd:string ;
    rdfs:subClassOf nell:householditem .

nell:wascollidedin rdfs:domain nell:everypromotedthing ;
    rdfs:range nell:roadaccidentevent ;
    rdfs:subPropertyOf nell:relatedto .

nell:weaponmadeincountry rdfs:comment "Describes the weapons produced by a country"^^xsd:string ;
    rdfs:domain nell:weapon ;
    rdfs:range nell:country ;
    rdfs:subPropertyOf nell:itemexistsatlocation .

nell:weaponssuchasweapons a owl:AsymmetricProperty,
        owl:IrreflexiveProperty ;
    rdfs:comment "Describes the weapons types that are generalizations of specific weapons"^^xsd:string ;
    rdfs:domain nell:weapon ;
    rdfs:range nell:weapon ;
    rdfs:subPropertyOf nell:generalizationof .

nell:weaponusedinprotest rdfs:domain nell:weapon ;
    rdfs:range nell:protestevent ;
    rdfs:subPropertyOf nell:relatedto .

nell:weatherphenomenon rdfs:comment "Anything that happens naturally in the atmosphere"^^xsd:string ;
    rdfs:subClassOf nell:event .

nell:wifeof rdfs:comment "person has a wife"^^xsd:string ;
    rdfs:domain nell:female ;
    rdfs:range nell:person ;
    rdfs:subPropertyOf nell:hasspouse .

nell:wikipediaurlof rdfs:comment "The Wikipedia page for a given category instance"^^xsd:string ;
    rdfs:domain nell:url ;
    rdfs:range nell:everypromotedthing ;
    rdfs:subPropertyOf nell:locatedat .

nell:wineproducedbywinery rdfs:comment "Describes the wines sold by a winery"^^xsd:string ;
    rdfs:domain nell:wine ;
    rdfs:range nell:winery ;
    rdfs:subPropertyOf nell:iteminvolvedwithagent .

nell:wineryatfarm rdfs:comment "farm and winery are related"^^xsd:string ;
    rdfs:domain nell:winery ;
    rdfs:range nell:farm ;
    rdfs:subPropertyOf nell:relatedto .

nell:wineryproduceswine rdfs:comment "Describes the wines sold by a winery"^^xsd:string ;
    rdfs:domain nell:winery ;
    rdfs:range nell:wine ;
    rdfs:subPropertyOf nell:agentinvolvedwithitem .

nell:winneringame rdfs:comment "Specifies that a particular team that played in a particular sportsGame was the winner thereof."^^xsd:string ;
    rdfs:domain nell:sportsteam ;
    rdfs:range nell:sportsgame ;
    rdfs:subPropertyOf nell:teamingame .

nell:winningscoreofsportsgame rdfs:comment "Specifies the score with which the winning team in a particular sportsGame lost."^^xsd:string ;
    rdfs:domain nell:nonneginteger ;
    rdfs:range nell:sportsgame ;
    rdfs:subPropertyOf nell:relatedto .

nell:writecanbethesameasscientist rdfs:comment "Describes two instances that are the same thing in these two different categories"^^xsd:string ;
    rdfs:domain nell:writer ;
    rdfs:range nell:scientist ;
    rdfs:subPropertyOf nell:canbethesameas .

nell:writercanbethesameaspersonafrica rdfs:comment "Describes writers that are the same instances as personafrica"^^xsd:string ;
    rdfs:domain nell:writer ;
    rdfs:range nell:personafrica ;
    rdfs:subPropertyOf nell:canbethesameas .

nell:writerwasbornincity rdfs:comment "Describes the city where a write was born in"^^xsd:string ;
    rdfs:domain nell:person ;
    rdfs:range nell:city ;
    rdfs:subPropertyOf nell:personbornincity .

nell:writerwrotebook rdfs:comment "author of a book"^^xsd:string ;
    rdfs:domain nell:writer ;
    rdfs:range nell:book ;
    rdfs:subPropertyOf nell:agentcontributedtocreativework .

nell:yearofmarriage rdfs:comment "This relation holds when a person married some other person in the specified year."^^xsd:string ;
    rdfs:domain nell:year ;
    rdfs:range nell:person ;
    rdfs:subPropertyOf nell:dateof .

nell:zipcodeinlocation rdfs:comment "Describes one or more locations to which a zipcode may correspond."^^xsd:string ;
    rdfs:domain nell:zipcode ;
    rdfs:range nell:location ;
    rdfs:subPropertyOf nell:atlocation .

nell:zooincity rdfs:comment "The city a zoo is located in"^^xsd:string ;
    rdfs:domain nell:zoo ;
    rdfs:range nell:city ;
    rdfs:subPropertyOf nell:attractionofcity .

() rdf:rest <http://www.semanticweb.org/ontologies/NELL#_:y10>,
        <http://www.semanticweb.org/ontologies/NELL#_:y12>,
        <http://www.semanticweb.org/ontologies/NELL#_:y14>,
        <http://www.semanticweb.org/ontologies/NELL#_:y16>,
        <http://www.semanticweb.org/ontologies/NELL#_:y18>,
        <http://www.semanticweb.org/ontologies/NELL#_:y2>,
        <http://www.semanticweb.org/ontologies/NELL#_:y20>,
        <http://www.semanticweb.org/ontologies/NELL#_:y22>,
        <http://www.semanticweb.org/ontologies/NELL#_:y24>,
        <http://www.semanticweb.org/ontologies/NELL#_:y26>,
        <http://www.semanticweb.org/ontologies/NELL#_:y28>,
        <http://www.semanticweb.org/ontologies/NELL#_:y30>,
        <http://www.semanticweb.org/ontologies/NELL#_:y32>,
        <http://www.semanticweb.org/ontologies/NELL#_:y34>,
        <http://www.semanticweb.org/ontologies/NELL#_:y36>,
        <http://www.semanticweb.org/ontologies/NELL#_:y38>,
        <http://www.semanticweb.org/ontologies/NELL#_:y4>,
        <http://www.semanticweb.org/ontologies/NELL#_:y40>,
        <http://www.semanticweb.org/ontologies/NELL#_:y6>,
        <http://www.semanticweb.org/ontologies/NELL#_:y8> .

nell:academicfieldconcernssubject rdfs:comment "Subjects of study within a given academic field"^^xsd:string ;
    rdfs:domain nell:academicfield ;
    rdfs:range nell:everypromotedthing ;
    rdfs:subPropertyOf nell:relatedto .

nell:acquired a owl:AsymmetricProperty,
        owl:IrreflexiveProperty ;
    rdfs:comment "to come into possession or ownership of; get as one's own "^^xsd:string ;
    rdfs:domain nell:company ;
    rdfs:range nell:company ;
    rdfs:subPropertyOf nell:superpartoforganization .

nell:acquiredby rdfs:comment "to come into possession or ownership of; get as one's own "^^xsd:string ;
    rdfs:domain nell:company ;
    rdfs:range nell:company ;
    rdfs:subPropertyOf nell:subpartoforganization .

nell:agenthaswebsite rdfs:comment "The organization that operates a website"^^xsd:string ;
    rdfs:domain nell:agent ;
    rdfs:range nell:website ;
    rdfs:subPropertyOf nell:agentrelatedtolocation .

nell:agentleadsorganization rdfs:comment "General relation as with certain political positions we have an agent that controls the thing that he works for"^^xsd:string ;
    rdfs:domain nell:humanagent ;
    rdfs:range nell:organization ;
    rdfs:subPropertyOf nell:agentcontrols,
        nell:agentrepresentsorganization .

nell:agentrepresentsorganization rdfs:comment "Specialization of proxyFor for agent-to-organization relations. populate=false only because presumed to be uninteresting"^^xsd:string ;
    rdfs:domain nell:humanagent ;
    rdfs:range nell:organization ;
    rdfs:subPropertyOf nell:agentbelongstoorganization,
        nell:proxyfor .

nell:animalthatfeedoninsect rdfs:comment "Describes the animals that feed on Insects"^^xsd:string ;
    rdfs:domain nell:animal ;
    rdfs:range nell:insect ;
    rdfs:subPropertyOf nell:animalpreyson .

nell:athleteinjuredhisbodypart rdfs:comment "Describes the athletes that had injured any body part"^^xsd:string ;
    rdfs:domain nell:athlete ;
    rdfs:range nell:bodypart ;
    rdfs:subPropertyOf nell:relatedto .

nell:athleteplaysforteam rdfs:comment "to join together in a team "^^xsd:string ;
    rdfs:domain nell:athlete ;
    rdfs:range nell:sportsteam ;
    rdfs:subPropertyOf nell:personbelongstoorganization .

nell:citylocatedincountry rdfs:comment "specifies that a particular city is located in a particular country"^^xsd:string ;
    rdfs:domain nell:city ;
    rdfs:range nell:country ;
    rdfs:subPropertyOf nell:citylocatedingeopoliticallocation .

nell:citylocatedinstate rdfs:comment "specifies that a particular city is located in a particular state or province"^^xsd:string ;
    rdfs:domain nell:city ;
    rdfs:range nell:stateorprovince ;
    rdfs:subPropertyOf nell:citylocatedingeopoliticallocation .

nell:cityoforganizationheadquarters a owl:InverseFunctionalProperty ;
    rdf:first <http://www.semanticweb.org/ontologies/NELL#_:y2>,
        <http://www.semanticweb.org/ontologies/NELL#_:y36>,
        <http://www.semanticweb.org/ontologies/NELL#_:y38>,
        <http://www.semanticweb.org/ontologies/NELL#_:y4> ;
    rdfs:comment "The city where a given organization is headquartered"^^xsd:string ;
    rdfs:domain nell:city ;
    rdfs:range nell:organization ;
    rdfs:subPropertyOf nell:locationactedinbyorganization .

nell:cityofpersonbirth rdfs:comment "the city that a person was born in"^^xsd:string ;
    rdfs:domain nell:city ;
    rdfs:range nell:person ;
    rdfs:subPropertyOf nell:locationofpersonbirth .

nell:consumerelectronicitem rdfs:comment "An item intended for ordinary people that runs on electricity excluding appliances. This category includes accessories for consumer electronic items such as video games and DVDs."^^xsd:string ;
    rdfs:subClassOf nell:item .

nell:countrystates a owl:InverseFunctionalProperty ;
    rdf:first <http://www.semanticweb.org/ontologies/NELL#_:y12>,
        <http://www.semanticweb.org/ontologies/NELL#_:y13>,
        <http://www.semanticweb.org/ontologies/NELL#_:y25> ;
    rdfs:comment "The country which the state or province is a part of."^^xsd:string ;
    rdfs:domain nell:country ;
    rdfs:range nell:stateorprovince ;
    rdfs:subPropertyOf nell:geopoliticallocationcontainsstate .

nell:fatherofperson rdfs:comment "father of a person"^^xsd:string ;
    rdfs:domain nell:male ;
    rdfs:range nell:person ;
    rdfs:subPropertyOf nell:parentofperson .

nell:geopoliticallocationresidenceofpersion rdfs:comment "the geopolitical location that person has residence in"^^xsd:string ;
    rdfs:domain nell:geopoliticallocation ;
    rdfs:range nell:person ;
    rdfs:subPropertyOf nell:locationresidenceofperson .

nell:geopoliticalorganizationleadbyperson rdfs:comment "specifies that a particular person plays a leading role in a particular geopolitical organization (which includes the governments of countries)"^^xsd:string ;
    rdfs:domain nell:geopoliticalorganization ;
    rdfs:range nell:person ;
    rdfs:subPropertyOf nell:organizationleadbyperson .

nell:inverseofanimalfeedoninsect rdfs:comment "Describes the animals that feed on Insects"^^xsd:string ;
    rdfs:domain nell:insect ;
    rdfs:range nell:animal ;
    rdfs:subPropertyOf nell:animalpredators .

nell:inverseofathleteinjuredhisbodypart rdfs:comment "Describes the athletes that had injured any body part"^^xsd:string ;
    rdfs:domain nell:bodypart ;
    rdfs:range nell:athlete ;
    rdfs:subPropertyOf nell:relatedto .

nell:inverseofpersonmovedtostateorprovince rdfs:comment "Describes the people that moved to live in a state or province"^^xsd:string ;
    rdfs:domain nell:stateorprovince ;
    rdfs:range nell:person ;
    rdfs:subPropertyOf nell:locationresidenceofperson .

nell:itemfoundinroom rdfs:comment "Relates items to rooms in which they are often found"^^xsd:string ;
    rdfs:domain nell:item ;
    rdfs:range nell:room ;
    rdfs:subPropertyOf nell:itemexistsatlocation .

nell:leagueplayers rdf:first <http://www.semanticweb.org/ontologies/NELL#_:y27> ;
    rdfs:comment "a group of athletic teams organized to promote mutual interests and to compete chiefly among themselves "^^xsd:string ;
    rdfs:domain nell:sportsleague ;
    rdfs:range nell:athlete ;
    rdfs:subPropertyOf nell:organizationhasperson .

nell:leaguestadiums rdfs:comment "specifies that a particular league uses a particular venue for its games"^^xsd:string ;
    rdfs:domain nell:sportsleague ;
    rdfs:range nell:stadiumoreventvenue ;
    rdfs:subPropertyOf nell:organizationactsinlocation .

nell:militaryeventtype rdfs:comment "A military event type is simply a sub-type (or sub-category) of the category military event."^^xsd:string ;
    rdfs:subClassOf nell:event .

nell:motherofperson rdfs:comment "mother of a person"^^xsd:string ;
    rdfs:domain nell:female ;
    rdfs:range nell:person ;
    rdfs:subPropertyOf nell:parentofperson .

nell:nongovorganization rdfs:comment "Politically-active or governmentally-active organizations that are not part of the government including but not limited to some NGOs"^^xsd:string ;
    rdfs:subClassOf nell:politicsgroup .

nell:officeheldbypolitician rdfs:comment "Specifies that a particular politician holds a particular office"^^xsd:string ;
    rdfs:domain nell:politicaloffice ;
    rdfs:range nell:politician ;
    rdfs:subPropertyOf nell:relatedto .

nell:officialwebsiteoforganization rdfs:comment "An official top-level URL for an organization's website"^^xsd:string ;
    rdfs:domain nell:website ;
    rdfs:range nell:organization ;
    rdfs:subPropertyOf nell:websiteoperatedbyagent .

nell:organizationhasofficialwebsite rdfs:comment "An official top-level URL for an organization's website"^^xsd:string ;
    rdfs:domain nell:organization ;
    rdfs:range nell:website ;
    rdfs:subPropertyOf nell:agenthaswebsite .

nell:organizationhastopmember rdfs:comment "Identifies people in high-level leading positions at organizations.  Applicable positions have authority over the entire organization (e.g. presidents VPs directors and C-level executives) not merely over departments or subsidiaries."^^xsd:string ;
    rdfs:domain nell:company ;
    rdfs:range nell:person ;
    rdfs:subPropertyOf nell:organizationleadbyperson,
        nell:worker .

nell:organizationheadquarteredincity rdfs:comment "The city where a given organization is headquartered"^^xsd:string ;
    rdfs:domain nell:organization ;
    rdfs:range nell:city ;
    rdfs:subPropertyOf nell:organizationactsinlocation .

nell:organizationleadbyagent rdfs:comment "General relation as with certain political positions we have an agent that controls the thing that he works for"^^xsd:string ;
    rdfs:domain nell:organization ;
    rdfs:range nell:humanagent ;
    rdfs:subPropertyOf nell:controlledbyagent,
        nell:organizationrepresentedbyagent .

nell:organizationrepresentedbyagent rdfs:comment "Specialization of proxyFor for agent-to-organization relations. populate=false only because presumed to be uninteresting"^^xsd:string ;
    rdfs:domain nell:organization ;
    rdfs:range nell:humanagent ;
    rdfs:subPropertyOf nell:organizationhasagent,
        nell:proxyof .

nell:personattendsschool rdfs:comment "person has attended a school"^^xsd:string ;
    rdfs:domain nell:person ;
    rdfs:range nell:school ;
    rdfs:subPropertyOf nell:personbelongstoorganization .

nell:personbornincity rdfs:comment "the city that a person was born in"^^xsd:string ;
    rdfs:domain nell:person ;
    rdfs:range nell:city ;
    rdfs:subPropertyOf nell:personborninlocation .

nell:persongraduatedschool rdfs:comment "This holds when the person has graduated from the educational institution at some time. This includes high schools say as well as universities. A division of an institution (\"Yale Business School\") will be scored as the same answer as the institution as a whole (\"Yale\")."^^xsd:string ;
    rdfs:domain nell:person ;
    rdfs:range nell:school ;
    rdfs:subPropertyOf nell:personattendsschool .

nell:personhasfather rdfs:comment "father of a person"^^xsd:string ;
    rdfs:domain nell:person ;
    rdfs:range nell:male ;
    rdfs:subPropertyOf nell:personhasparent .

nell:personhasmother rdfs:comment "mother of a person"^^xsd:string ;
    rdfs:domain nell:person ;
    rdfs:range nell:female ;
    rdfs:subPropertyOf nell:personhasparent .

nell:personleadsgeopoliticalorganization rdfs:comment "specifies that a particular person plays a leading role in a particular geopolitical organization (which includes the governments of countries)"^^xsd:string ;
    rdfs:domain nell:person ;
    rdfs:range nell:geopoliticalorganization ;
    rdfs:subPropertyOf nell:personleadsorganization .

nell:personmovedtostateorprovince rdf:first <http://www.semanticweb.org/ontologies/NELL#_:y22> ;
    rdfs:comment "Describes the people that moved to live in a state or province"^^xsd:string ;
    rdfs:domain nell:person ;
    rdfs:range nell:stateorprovince ;
    rdfs:subPropertyOf nell:personhasresidenceinlocation .

nell:personus rdfs:comment "citizens of the U.S.A."^^xsd:string ;
    rdfs:subClassOf nell:personnorthamerica .

nell:players rdf:first <http://www.semanticweb.org/ontologies/NELL#_:y31> ;
    rdfs:comment "to engage in (a game pastime etc.) "^^xsd:string ;
    rdfs:domain nell:sport ;
    rdfs:range nell:athlete ;
    rdfs:subPropertyOf nell:relatedto .

nell:politicalgroupofpolitician rdfs:comment "Specifies that a particular politician belongs to a particular"^^xsd:string ;
    rdfs:domain nell:politicsgroup ;
    rdfs:range nell:politician ;
    rdfs:subPropertyOf nell:organizationhasperson .

nell:politicianendorsedbypolitician rdfs:comment "Politician that endorses another politician"^^xsd:string ;
    rdfs:domain nell:politician ;
    rdfs:range nell:politician ;
    rdfs:subPropertyOf nell:agentcollaborateswithagent .

nell:politicianendorsespolitician rdfs:comment "Politician that endorses another politician"^^xsd:string ;
    rdfs:domain nell:politician ;
    rdfs:range nell:politician ;
    rdfs:subPropertyOf nell:agentcollaborateswithagent .

nell:politicianholdsoffice rdfs:comment "Specifies that a particular politician holds a particular office"^^xsd:string ;
    rdfs:domain nell:politician ;
    rdfs:range nell:politicaloffice ;
    rdfs:subPropertyOf nell:relatedto .

nell:politicianmemberofpoliticsgroup rdfs:comment "Specifies that a particular politician belongs to a particular"^^xsd:string ;
    rdfs:domain nell:politician ;
    rdfs:range nell:politicsgroup ;
    rdfs:subPropertyOf nell:personbelongstoorganization .

nell:politiciansponsoredpoliticsbill rdfs:comment "Politician(s) sponsoring a particular legislative bill"^^xsd:string ;
    rdfs:domain nell:politician ;
    rdfs:range nell:politicsbill ;
    rdfs:subPropertyOf nell:relatedto .

nell:politicsbillsponsoredbypolitician rdfs:comment "Politician(s) sponsoring a particular legislative bill"^^xsd:string ;
    rdfs:domain nell:politicsbill ;
    rdfs:range nell:politician ;
    rdfs:subPropertyOf nell:relatedto .

nell:producedby rdfs:comment "Specifies that a particular compnay produces a particular product"^^xsd:string ;
    rdfs:domain nell:product ;
    rdfs:range nell:company ;
    rdfs:subPropertyOf nell:createdbyagent,
        nell:iteminvolvedwithagent .

nell:producesproduct rdfs:comment "Specifies that a particular compnay produces a particular product"^^xsd:string ;
    rdfs:domain nell:company ;
    rdfs:range nell:product ;
    rdfs:subPropertyOf nell:agentcreated,
        nell:agentinvolvedwithitem .

nell:roomcancontainitem rdfs:comment "Relates items to rooms in which they are often found"^^xsd:string ;
    rdfs:domain nell:room ;
    rdfs:range nell:item ;
    rdfs:subPropertyOf nell:locationofitemexistence .

nell:schoolattendedbyperson rdfs:comment "person has attended a school"^^xsd:string ;
    rdfs:domain nell:school ;
    rdfs:range nell:person ;
    rdfs:subPropertyOf nell:organizationhasperson .

nell:schoolgraduatedperson rdfs:comment "This holds when the person has graduated from the educational institution at some time. This includes high schools say as well as universities. A division of an institution (\"Yale Business School\") will be scored as the same answer as the institution as a whole (\"Yale\")."^^xsd:string ;
    rdfs:domain nell:school ;
    rdfs:range nell:person ;
    rdfs:subPropertyOf nell:schoolattendedbyperson .

nell:sportusesstadium rdfs:comment "Specifies that a particular sport is played in a particular venue"^^xsd:string ;
    rdfs:domain nell:sport ;
    rdfs:range nell:stadiumoreventvenue ;
    rdfs:subPropertyOf nell:relatedto .

nell:statecontainscity a owl:InverseFunctionalProperty ;
    rdf:first <http://www.semanticweb.org/ontologies/NELL#_:y10>,
        <http://www.semanticweb.org/ontologies/NELL#_:y14>,
        <http://www.semanticweb.org/ontologies/NELL#_:y3> ;
    rdfs:comment "specifies that a particular city is located in a particular state or province"^^xsd:string ;
    rdfs:domain nell:stateorprovince ;
    rdfs:range nell:city ;
    rdfs:subPropertyOf nell:geopoliticallocationcontainscity .

nell:statelocatedingeopoliticallocation rdfs:comment "specifies that a particular state or province is located in a particular geopolitical location"^^xsd:string ;
    rdfs:domain nell:stateorprovince ;
    rdfs:range nell:geopoliticallocation ;
    rdfs:subPropertyOf nell:locationlocatedwithinlocation .

nell:subjectconcernedbyacademicfield rdfs:comment "Subjects of study within a given academic field"^^xsd:string ;
    rdfs:domain nell:everypromotedthing ;
    rdfs:range nell:academicfield ;
    rdfs:subPropertyOf nell:relatedto .

nell:teamhomestadium rdfs:comment "The stadium or other sporting venue which a team designates as its \"home.\" Typically a large percentage of the team's games occur in this location."^^xsd:string ;
    rdfs:domain nell:sportsteam ;
    rdfs:range nell:stadiumoreventvenue ;
    rdfs:subPropertyOf nell:organizationactsinlocation .

nell:teammember rdf:first <http://www.semanticweb.org/ontologies/NELL#_:y19>,
        <http://www.semanticweb.org/ontologies/NELL#_:y34>,
        <http://www.semanticweb.org/ontologies/NELL#_:y5> ;
    rdfs:comment "to join together in a team "^^xsd:string ;
    rdfs:domain nell:sportsteam ;
    rdfs:range nell:athlete ;
    rdfs:subPropertyOf nell:organizationhasperson .

nell:teamwontrophy rdfs:comment "Trophies that a team has won"^^xsd:string ;
    rdfs:domain nell:sportsteam ;
    rdfs:range nell:awardtrophytournament ;
    rdfs:subPropertyOf nell:relatedto .

nell:topmemberoforganization rdfs:comment "Identifies people in high-level leading positions at organizations.  Applicable positions have authority over the entire organization (e.g. presidents VPs directors and C-level executives) not merely over departments or subsidiaries."^^xsd:string ;
    rdfs:domain nell:person ;
    rdfs:range nell:company ;
    rdfs:subPropertyOf nell:personleadsorganization,
        nell:worksfor .

nell:websiteoperatedbyagent rdfs:comment "The organization that operates a website"^^xsd:string ;
    rdfs:domain nell:website ;
    rdfs:range nell:agent ;
    rdfs:subPropertyOf nell:locationrelatedtoagent .

<http://www.semanticweb.org/ontologies/NELL#_:y1> owl:propertyChainAxiom nell:countryoforganizationheadquarters .

<http://www.semanticweb.org/ontologies/NELL#_:y10> rdf:rest <http://www.semanticweb.org/ontologies/NELL#_:y9> .

<http://www.semanticweb.org/ontologies/NELL#_:y11> owl:propertyChainAxiom nell:geopoliticallocationcontainsstate .

<http://www.semanticweb.org/ontologies/NELL#_:y12> rdf:rest <http://www.semanticweb.org/ontologies/NELL#_:y11> .

<http://www.semanticweb.org/ontologies/NELL#_:y13> owl:propertyChainAxiom nell:countrycities .

<http://www.semanticweb.org/ontologies/NELL#_:y14> rdf:rest <http://www.semanticweb.org/ontologies/NELL#_:y13> .

<http://www.semanticweb.org/ontologies/NELL#_:y15> owl:propertyChainAxiom nell:geopoliticallocationcontainscity .

<http://www.semanticweb.org/ontologies/NELL#_:y16> rdf:rest <http://www.semanticweb.org/ontologies/NELL#_:y15> .

<http://www.semanticweb.org/ontologies/NELL#_:y17> owl:propertyChainAxiom nell:players .

<http://www.semanticweb.org/ontologies/NELL#_:y18> rdf:rest <http://www.semanticweb.org/ontologies/NELL#_:y17> .

<http://www.semanticweb.org/ontologies/NELL#_:y19> owl:propertyChainAxiom nell:teamwontrophy .

<http://www.semanticweb.org/ontologies/NELL#_:y2> rdf:rest <http://www.semanticweb.org/ontologies/NELL#_:y1> .

<http://www.semanticweb.org/ontologies/NELL#_:y20> rdf:rest <http://www.semanticweb.org/ontologies/NELL#_:y19> .

<http://www.semanticweb.org/ontologies/NELL#_:y21> owl:propertyChainAxiom nell:countrystates .

<http://www.semanticweb.org/ontologies/NELL#_:y22> rdf:rest <http://www.semanticweb.org/ontologies/NELL#_:y21> .

<http://www.semanticweb.org/ontologies/NELL#_:y23> owl:propertyChainAxiom nell:countryoforganizationheadquarters .

<http://www.semanticweb.org/ontologies/NELL#_:y24> rdf:rest <http://www.semanticweb.org/ontologies/NELL#_:y23> .

<http://www.semanticweb.org/ontologies/NELL#_:y25> owl:propertyChainAxiom nell:countrycities .

<http://www.semanticweb.org/ontologies/NELL#_:y26> rdf:rest <http://www.semanticweb.org/ontologies/NELL#_:y25> .

<http://www.semanticweb.org/ontologies/NELL#_:y27> owl:propertyChainAxiom nell:leaguestadiums .

<http://www.semanticweb.org/ontologies/NELL#_:y28> rdf:rest <http://www.semanticweb.org/ontologies/NELL#_:y27> .

<http://www.semanticweb.org/ontologies/NELL#_:y29> owl:propertyChainAxiom nell:geopoliticallocationresidenceofpersion .

<http://www.semanticweb.org/ontologies/NELL#_:y3> owl:propertyChainAxiom nell:stateorprovinceoforganizationheadquarters .

<http://www.semanticweb.org/ontologies/NELL#_:y30> rdf:rest <http://www.semanticweb.org/ontologies/NELL#_:y29> .

<http://www.semanticweb.org/ontologies/NELL#_:y31> owl:propertyChainAxiom nell:sportusesstadium .

<http://www.semanticweb.org/ontologies/NELL#_:y32> rdf:rest <http://www.semanticweb.org/ontologies/NELL#_:y31> .

<http://www.semanticweb.org/ontologies/NELL#_:y33> owl:propertyChainAxiom nell:leagueplayers .

<http://www.semanticweb.org/ontologies/NELL#_:y34> rdf:rest <http://www.semanticweb.org/ontologies/NELL#_:y33> .

<http://www.semanticweb.org/ontologies/NELL#_:y35> owl:propertyChainAxiom nell:countryoforganizationheadquarters .

<http://www.semanticweb.org/ontologies/NELL#_:y36> rdf:rest <http://www.semanticweb.org/ontologies/NELL#_:y35> .

<http://www.semanticweb.org/ontologies/NELL#_:y37> owl:propertyChainAxiom nell:stateorprovinceoforganizationheadquarters .

<http://www.semanticweb.org/ontologies/NELL#_:y38> rdf:rest <http://www.semanticweb.org/ontologies/NELL#_:y37> .

<http://www.semanticweb.org/ontologies/NELL#_:y39> owl:propertyChainAxiom nell:geopoliticallocationcontainscity .

<http://www.semanticweb.org/ontologies/NELL#_:y4> rdf:rest <http://www.semanticweb.org/ontologies/NELL#_:y3> .

<http://www.semanticweb.org/ontologies/NELL#_:y40> rdf:rest <http://www.semanticweb.org/ontologies/NELL#_:y39> .

<http://www.semanticweb.org/ontologies/NELL#_:y5> owl:propertyChainAxiom nell:teamhomestadium .

<http://www.semanticweb.org/ontologies/NELL#_:y6> rdf:rest <http://www.semanticweb.org/ontologies/NELL#_:y5> .

<http://www.semanticweb.org/ontologies/NELL#_:y7> owl:propertyChainAxiom nell:geopoliticallocationcontainscity .

<http://www.semanticweb.org/ontologies/NELL#_:y8> rdf:rest <http://www.semanticweb.org/ontologies/NELL#_:y7> .

<http://www.semanticweb.org/ontologies/NELL#_:y9> owl:propertyChainAxiom nell:geopoliticallocationcontainscity .

nell:agenthierarchicallyaboveagent rdfs:domain nell:agent ;
    rdfs:range nell:agent ;
    rdfs:subPropertyOf nell:agentcollaborateswithagent,
        nell:agentcontrols .

nell:agenthierarchicallybelowagent rdfs:domain nell:agent ;
    rdfs:range nell:agent ;
    rdfs:subPropertyOf nell:agentcollaborateswithagent,
        nell:controlledbyagent .

nell:animalpredators rdfs:comment "Animals that are hunted and eaten by this animal."^^xsd:string ;
    rdfs:domain nell:animal ;
    rdfs:range nell:animal ;
    rdfs:subPropertyOf nell:agentcompeteswithagent .

nell:animalpreyson a owl:ReflexiveProperty ;
    rdfs:comment "Animals that are hunted and eaten by this animal."^^xsd:string ;
    rdfs:domain nell:animal ;
    rdfs:range nell:animal ;
    rdfs:subPropertyOf nell:agentcompeteswithagent .

nell:animalsuchasinvertebrate rdfs:comment "Describes the invertebrate that are from a specific type of animals"^^xsd:string ;
    rdfs:domain nell:animal ;
    rdfs:range nell:invertebrate ;
    rdfs:subPropertyOf nell:animaltypehasanimal .

nell:automobilemodel rdfs:comment "A model is a specific car carried under a make."^^xsd:string ;
    rdfs:subClassOf nell:vehicle .

nell:bone rdfs:comment "a bone or bone structure in a vertebrate"^^xsd:string ;
    rdfs:subClassOf nell:bodypart .

nell:caf_ rdfs:subClassOf nell:company,
        nell:location .

nell:candy rdfs:comment "A food which is made primarily of sugar and generally sold for wide distribution. This would include many dessert items like pie and cake that might not be strictly \"candy\" per se."^^xsd:string ;
    rdfs:subClassOf nell:food .

nell:ceoof rdfs:comment "specifies that a particular CEO is the CEO of a particular company"^^xsd:string ;
    rdfs:domain nell:ceo ;
    rdfs:range nell:company ;
    rdfs:subPropertyOf nell:topmemberoforganization .

nell:citylocatedingeopoliticallocation rdfs:comment "specifies that a particular city is located in a particular geopolitical location"^^xsd:string ;
    rdfs:domain nell:city ;
    rdfs:range nell:geopoliticallocation ;
    rdfs:subPropertyOf nell:locationlocatedwithinlocation .

nell:coffeedrink rdfs:subClassOf nell:beverage .

nell:companyceo rdfs:comment "specifies that a particular CEO is the CEO of a particular company"^^xsd:string ;
    rdfs:domain nell:company ;
    rdfs:range nell:ceo ;
    rdfs:subPropertyOf nell:organizationhastopmember .

nell:countryhascompanyoffice rdfs:comment "specifies that a particular company has offices in a particular country"^^xsd:string ;
    rdfs:domain nell:country ;
    rdfs:range nell:company ;
    rdfs:subPropertyOf nell:locationactedinbyorganization .

nell:crimeorcharge rdfs:comment "A crime or other kind of offence or violation with which a person can be charged"^^xsd:string ;
    rdfs:subClassOf nell:event .

nell:crustacean rdfs:comment "form a very large group of arthropods usually treated as a subphylum which includes such familiar animals as crabs lobsters crayfish shrimp krill and barnacles. Like other arthropods crustaceans have an exoskeleton which they moult to grow. They are distinguished from other groups of arthropods such as insects myriapods and chelicerates by the possession of biramous (two-parted) limbs and by the nauplius form of the larvae."^^xsd:string ;
    rdfs:subClassOf nell:arthropod .

nell:currency rdfs:comment "A currency is money that is used (or has been used) as a medium of exchange"^^xsd:string ;
    rdfs:subClassOf nell:abstractthing .

nell:dateevent rdfs:comment "specifies that the duration of a particular event overlapped with a particular date."^^xsd:string ;
    rdfs:domain nell:dateliteral ;
    rdfs:range nell:event ;
    rdfs:subPropertyOf nell:dateof .

nell:ethnicgroup rdfs:comment "A group of individuals that share common characteristics such as ancestry country of origin language religion culture and physical appearance."^^xsd:string ;
    rdfs:subClassOf nell:abstractthing .

nell:eventatlocation rdfs:comment "the location that an event is happened at"^^xsd:string ;
    rdfs:domain nell:event ;
    rdfs:range nell:location ;
    rdfs:subPropertyOf nell:atlocation .

nell:eventdate rdfs:comment "specifies that the duration of a particular event overlapped with a particular date."^^xsd:string ;
    rdfs:domain nell:event ;
    rdfs:range nell:dateliteral ;
    rdfs:subPropertyOf nell:atdate .

nell:furniture rdfs:comment "Any functional or decorative mobile object with which a dwelling might be said to be \"furnished\" or any immobile variant of the same (such as an oven built into a wall)."^^xsd:string ;
    rdfs:subClassOf nell:householditem .

nell:gamescore rdfs:subClassOf nell:abstractthing .

nell:geopoliticalentity rdfs:comment "That which would an object of geopolitical analysis including but not limited to countries administrative or de facto subdivisions thereof supernational groupings and organizations geographical regions and cultural groups."^^xsd:string ;
    rdfs:subClassOf nell:abstractthing .

nell:geopoliticallocationcontainsstate rdf:first <http://www.semanticweb.org/ontologies/NELL#_:y15>,
        <http://www.semanticweb.org/ontologies/NELL#_:y9> ;
    rdfs:comment "specifies that a particular state or province is located in a particular geopolitical location"^^xsd:string ;
    rdfs:domain nell:geopoliticallocation ;
    rdfs:range nell:stateorprovince ;
    rdfs:subPropertyOf nell:locationcontainslocation .

nell:hasofficeincountry rdfs:comment "specifies that a particular company has offices in a particular country"^^xsd:string ;
    rdfs:domain nell:company ;
    rdfs:range nell:country ;
    rdfs:subPropertyOf nell:organizationactsinlocation .

nell:hospital rdfs:comment "A hospital is an institution for health care often but not always providing for longer-term patient stays.  All varieties of hospitals -- private public military etc. -- are included."^^xsd:string ;
    rdfs:subClassOf nell:building .

nell:inverseofanimalsuchasinvertebrate rdfs:comment "Describes the invertebrate that are from a specific type of animals"^^xsd:string ;
    rdfs:domain nell:invertebrate ;
    rdfs:range nell:animal ;
    rdfs:subPropertyOf nell:animalistypeofanimal .

nell:journalist rdfs:comment "Journalists are professionals who work in journalism. They collect and report news."^^xsd:string ;
    rdfs:subClassOf nell:person .

nell:landscapefeatures rdfs:comment "This type captures geographical features of the Earth including landforms bodies of water underwater landforms caves and similar locations."^^xsd:string ;
    rdfs:subClassOf nell:location,
        nell:visualizablescene .

nell:llcoordinate rdfs:comment "Longitude is the angular distance of a point's meridian from the Prime (Greenwich) Meridian"^^xsd:string ;
    rdfs:subClassOf nell:abstractthing .

nell:locationofevent rdfs:comment "the location that an event is happened at"^^xsd:string ;
    rdfs:domain nell:location ;
    rdfs:range nell:event ;
    rdfs:subPropertyOf nell:locatedat .

nell:meat rdfs:comment "A type of animal flesh that is used as food. (Wikipedia)"^^xsd:string ;
    rdfs:subClassOf nell:food .

nell:meetingeventtype rdfs:comment "A kind of meeting the name of a series of meetings or some other way to refer to a category of meeting"^^xsd:string ;
    rdfs:subClassOf nell:event .

nell:mlarea rdfs:comment "A specific area of investigation within the sub-field of machine learning."^^xsd:string ;
    rdfs:subClassOf nell:abstractthing .

nell:mlsoftware rdfs:comment "A software package that offers machine learning functionality"^^xsd:string ;
    rdfs:subClassOf nell:software .

nell:mollusk rdfs:comment "invertebrate having a soft unsegmented body usually enclosed in a shell"^^xsd:string ;
    rdfs:subClassOf nell:invertebrate .

nell:muscle rdfs:comment "A muscle is a contractile form of tissue which animals use to effect movement."^^xsd:string ;
    rdfs:subClassOf nell:bodypart .

nell:museum rdfs:comment "A museum is a \"permanent institution in the service of society and of its development open to the public which acquires conserves researches communicates and exhibits the tangible and intangible heritage of humanity and its environment for the purposes of education study and enjoyment\" as defined by the International Council of Museums."^^xsd:string ;
    rdfs:subClassOf nell:attraction,
        nell:building .

nell:musicalbum rdfs:comment "A collection of Musical Tracks (recordings of Songs) released in a common format such as Compact Disc or LP. An album is typically associated with a single Musical Artist unless it is a compilation which is a collection of tracks by various artists.  (FreeBase)"^^xsd:string ;
    rdfs:subClassOf nell:creativework .

nell:musicinstrument rdfs:comment "A Musical instrument is a device constructed or modified with the purpose of making music. In principle anything that produces sound and can somehow be controlled by a musician can serve as a musical instrument. (See e.g. the hardart.)"^^xsd:string ;
    rdfs:subClassOf nell:item,
        nell:visualizableobject .

nell:musicsong rdfs:comment "A song is any musical work including instrumentals as well as songs with lyrics."^^xsd:string ;
    rdfs:subClassOf nell:creativework .

nell:organizationleadbyperson rdfs:comment "person leading an organization/company"^^xsd:string ;
    rdfs:domain nell:organization ;
    rdfs:range nell:person ;
    rdfs:subPropertyOf nell:organizationleadbyagent .

nell:parentofperson a owl:AsymmetricProperty,
        owl:IrreflexiveProperty ;
    rdfs:comment "parent of a person"^^xsd:string ;
    rdfs:domain nell:person ;
    rdfs:range nell:person ;
    rdfs:subPropertyOf nell:hasfamilymember .

nell:personafrica rdfs:comment "citizens of countries in Africa"^^xsd:string ;
    rdfs:subClassOf nell:personbylocation .

nell:personalsoknownas a owl:IrreflexiveProperty,
        owl:SymmetricProperty ;
    rdfs:comment "this is another name for this person"^^xsd:string ;
    rdfs:domain nell:person ;
    rdfs:range nell:person ;
    rdfs:subPropertyOf nell:synonymfor .

nell:personhasparent rdfs:comment "parent of a person"^^xsd:string ;
    rdfs:domain nell:person ;
    rdfs:range nell:person ;
    rdfs:subPropertyOf nell:hasfamilymember .

nell:personleadsorganization rdf:first <http://www.semanticweb.org/ontologies/NELL#_:y24> ;
    rdfs:comment "person leading an organization/company"^^xsd:string ;
    rdfs:domain nell:person ;
    rdfs:range nell:organization ;
    rdfs:subPropertyOf nell:agentleadsorganization .

nell:placeofworship rdfs:comment "A place of worship is a building which is used by members of a religion for worship."^^xsd:string ;
    rdfs:subClassOf nell:building .

nell:programminglanguage rdfs:comment "A language used to give instructions to a computer"^^xsd:string ;
    rdfs:subClassOf nell:abstractthing .

nell:radiostation rdfs:comment "A radio station is a broadcaster which transmits audio. This category includes broadcast radio satellite radio and internet radio stations."^^xsd:string ;
    rdfs:subClassOf nell:geolocatablething,
        nell:mediacompany .

nell:scientist rdfs:comment "A scientist is a professional who performs research to discover the rules which govern the natural world. This category includes mathematicians even though math isn't really a science."^^xsd:string ;
    rdfs:subClassOf nell:person .

nell:shoppingmall rdfs:comment "A shopping mall is a building or group of buildings containing many stores restaurants and businesses."^^xsd:string ;
    rdfs:subClassOf nell:building .

nell:skiarea rdfs:comment "A place to ski"^^xsd:string ;
    rdfs:subClassOf nell:attraction .

nell:skyscraper rdfs:comment "A very tall building"^^xsd:string ;
    rdfs:subClassOf nell:building .

nell:sportsequipment rdfs:comment "Anything which is used to play a sport"^^xsd:string ;
    rdfs:subClassOf nell:item,
        nell:visualizableobject .

nell:stateorprovinceoforganizationheadquarters a owl:InverseFunctionalProperty ;
    rdfs:comment "The state or province where a given organization is headquartered"^^xsd:string ;
    rdfs:domain nell:stateorprovince ;
    rdfs:range nell:organization ;
    rdfs:subPropertyOf nell:locationactedinbyorganization .

nell:street rdfs:comment "A route of travel that has a single name indicating its entirety and that could have a street address (as distinct from trail which may not feature addresses)"^^xsd:string ;
    rdfs:subClassOf nell:geolocatablething,
        nell:location .

nell:televisionnetwork rdfs:comment "Category for different types of TV networks (currently closed-world limited to major American networks)"^^xsd:string ;
    rdfs:subClassOf nell:mediacompany .

nell:transportation rdfs:comment "a mode of travel such as rail transport or automobile. It is a category defining a means of moving from one location to another."^^xsd:string ;
    rdfs:subClassOf nell:attraction .

nell:videogamesystem rdfs:comment "includes any form of electronic game device from handheld units as small as a phone to large powerful computer systems and even arcade coin-operated systems."^^xsd:string ;
    rdfs:subClassOf nell:consumerelectronicitem .

nell:visualartform rdfs:comment "A categorization of the visual arts. An art form is a specific form for artistic expression to take.An art form more or less corresponds to the tools or materials used to create an art work (FreeBase)"^^xsd:string ;
    rdfs:subClassOf nell:creativework .

nell:visualartmovement rdfs:comment "A tendency or style in art with a specific common philosophy or goal followed by a group of artists during a restricted period of time or at least with the heyday of the movement more or less strictly so restricted (usually a few months years or decades) (FreeBase).  This does not include things that are merly genres such as \"fantasy art\" or \"oceanic art\"."^^xsd:string ;
    rdfs:subClassOf nell:abstractthing .

nell:wine rdfs:comment "Types of wines or specific vintanges of particular wineries"^^xsd:string ;
    rdfs:subClassOf nell:beverage .

nell:year rdfs:comment "Four-digit years"^^xsd:string ;
    rdfs:subClassOf nell:date .

nell:zipcode rdfs:comment "US ZIP codes. Other postal codes are not allowed"^^xsd:string ;
    rdfs:subClassOf nell:location .

nell:zoo rdfs:comment "facility in which animals are confined within enclosures displayed to the public and in which they may also be bred."^^xsd:string ;
    rdfs:subClassOf nell:attraction .

nell:agentbelongstoorganization rdfs:comment "to be in the relation of a member adherent inhabitant etc "^^xsd:string ;
    rdfs:domain nell:humanagent ;
    rdfs:range nell:organization ;
    rdfs:subPropertyOf nell:agenthierarchicallybelowagent,
        nell:subpartof .

nell:agentcontributedtocreativework rdfs:comment "Specifies that a particular agent contributed to the production or creation of a particular creativeWork. An actor in a movie contributes to that movie but agentCreated would probably be to strong an assertion for that."^^xsd:string ;
    rdfs:domain nell:agent ;
    rdfs:range nell:creativework ;
    rdfs:subPropertyOf nell:relatedto .

nell:agentcontrols rdfs:comment "to exercise restraint or direction over; dominate; command "^^xsd:string ;
    rdfs:domain nell:agent ;
    rdfs:range nell:everypromotedthing ;
    rdfs:subPropertyOf nell:relatedto .

nell:agentinteractswithagent rdfs:comment "to act one upon another "^^xsd:string ;
    rdfs:domain nell:agent ;
    rdfs:range nell:agent ;
    rdfs:subPropertyOf nell:relatedto .

nell:animaleatfood rdfs:comment "Describes the foods that are eaten by an animal"^^xsd:string ;
    rdfs:domain nell:animal ;
    rdfs:range nell:food ;
    rdfs:subPropertyOf nell:relatedto .

nell:animalistypeofanimal rdfs:comment "Type-specific generalization of animals."^^xsd:string ;
    rdfs:domain nell:animal ;
    rdfs:range nell:animal ;
    rdfs:subPropertyOf nell:specializationof .

nell:animaltypehasanimal a owl:AsymmetricProperty,
        owl:IrreflexiveProperty ;
    rdfs:comment "Type-specific generalization of animals."^^xsd:string ;
    rdfs:domain nell:animal ;
    rdfs:range nell:animal ;
    rdfs:subPropertyOf nell:generalizationof .

nell:blog rdfs:comment "A blog (or weblog) is a user-generated website where entries are made in journal style and displayed in a reverse chronological order. Blogs often provide commentary or news on a particular subject such as food politics or local news; some function as more personal online diaries."^^xsd:string ;
    rdfs:subClassOf nell:publication,
        nell:website .

nell:controlledbyagent rdfs:comment "to exercise restraint or direction over; dominate; command "^^xsd:string ;
    rdfs:domain nell:everypromotedthing ;
    rdfs:range nell:agent ;
    rdfs:subPropertyOf nell:relatedto .

nell:countrycities a owl:InverseFunctionalProperty ;
    rdf:first <http://www.semanticweb.org/ontologies/NELL#_:y1>,
        <http://www.semanticweb.org/ontologies/NELL#_:y8> ;
    rdfs:comment "specifies that a particular city is located in a particular country"^^xsd:string ;
    rdfs:domain nell:country ;
    rdfs:range nell:city ;
    rdfs:subPropertyOf nell:geopoliticallocationcontainscity .

nell:countryoforganizationheadquarters a owl:InverseFunctionalProperty ;
    rdfs:comment "The country where a given organization is headquartered"^^xsd:string ;
    rdfs:domain nell:country ;
    rdfs:range nell:organization ;
    rdfs:subPropertyOf nell:locationactedinbyorganization .

nell:creativeworkcontributedtobyagent rdfs:comment "Specifies that a particular agent contributed to the production or creation of a particular creativeWork. An actor in a movie contributes to that movie but agentCreated would probably be to strong an assertion for that."^^xsd:string ;
    rdfs:domain nell:creativework ;
    rdfs:range nell:agent ;
    rdfs:subPropertyOf nell:relatedto .

nell:fruit rdfs:comment "A structure of a plant that contains its seeds. This is closer to the botanical definition than the cullinary / colloquial definition but is technically niether."^^xsd:string ;
    rdfs:subClassOf nell:food .

nell:game rdfs:comment "General parent category for more specific kinds of games"^^xsd:string ;
    rdfs:subClassOf nell:abstractthing .

nell:inverseofanimaleatfood rdfs:comment "Describes the foods that are eaten by an animal"^^xsd:string ;
    rdfs:domain nell:food ;
    rdfs:range nell:animal ;
    rdfs:subPropertyOf nell:relatedto .

nell:locationofpersonbirth rdfs:comment "the location that a person is born in"^^xsd:string ;
    rdfs:domain nell:location ;
    rdfs:range nell:person ;
    rdfs:subPropertyOf nell:locationactedinbyagent .

nell:locationofpersondeath rdfs:comment "the location that a person died in"^^xsd:string ;
    rdfs:domain nell:location ;
    rdfs:range nell:person ;
    rdfs:subPropertyOf nell:locationactedinbyagent .

nell:organizationhasagent rdfs:comment "to be in the relation of a member adherent inhabitant etc "^^xsd:string ;
    rdfs:domain nell:organization ;
    rdfs:range nell:humanagent ;
    rdfs:subPropertyOf nell:agenthierarchicallyaboveagent,
        nell:superpartof .

nell:personborninlocation a owl:FunctionalProperty ;
    rdfs:comment "the location that a person is born in"^^xsd:string ;
    rdfs:domain nell:person ;
    rdfs:range nell:location ;
    rdfs:subPropertyOf nell:agentactsinlocation .

nell:persondiedinlocation rdfs:comment "the location that a person died in"^^xsd:string ;
    rdfs:domain nell:person ;
    rdfs:range nell:location ;
    rdfs:subPropertyOf nell:agentactsinlocation .

nell:personnorthamerica rdfs:comment "citizens of countries in North America"^^xsd:string ;
    rdfs:subClassOf nell:personbylocation .

nell:subpartoforganization a owl:AsymmetricProperty,
        owl:IrreflexiveProperty ;
    rdfs:comment "one organization is a subpart of a larger controlling organization"^^xsd:string ;
    rdfs:domain nell:organization ;
    rdfs:range nell:organization ;
    rdfs:subPropertyOf nell:agentbelongstoorganization .

nell:superpartoforganization rdfs:comment "one organization is a subpart of a larger controlling organization"^^xsd:string ;
    rdfs:domain nell:organization ;
    rdfs:range nell:organization ;
    rdfs:subPropertyOf nell:organizationhasagent .

nell:traditionalgame rdfs:comment "Includes all non-sports non-electronic games including board games parlor games and card games."^^xsd:string ;
    rdfs:subClassOf nell:game .

nell:agentcompeteswithagent a owl:ReflexiveProperty,
        owl:SymmetricProperty ;
    rdfs:comment "Non-cooperative interaction. Primary alternative to agentCollaboratesWithAgent."^^xsd:string ;
    rdfs:domain nell:agent ;
    rdfs:range nell:agent ;
    rdfs:subPropertyOf nell:agentinteractswithagent .

nell:agentparticipatedinevent rdfs:comment "identifies participants in events"^^xsd:string ;
    rdfs:domain nell:agent ;
    rdfs:range nell:event ;
    rdfs:subPropertyOf nell:subpartof .

nell:amphibian rdfs:comment "Amphibians (class Amphibia from Amphi- meaning \"on both sides\" and -bios meaning \"life\") such as frogs salamanders and caecilians are ectothermic (or cold-blooded) animals that metamorphose from a juvenile water-breathing form either to an adult air-breathing form or to a paedomorph that retains some juvenile characteristics."^^xsd:string ;
    rdfs:subClassOf nell:vertebrate .

nell:archaea rdfs:comment "single-celled organisms lacking nuclei formerly called archaebacteria but now known to differ fundamentally from bacteria"^^xsd:string ;
    rdfs:subClassOf nell:species .

nell:architect rdfs:comment "a person who designs buildings or other structures"^^xsd:string ;
    rdfs:subClassOf nell:person .

nell:automobileengine rdfs:comment "The engine type is to be used to classify specific powerplants used in an automobile. These may be year-specific but more frequently they often span multiple years models makes and generations."^^xsd:string ;
    rdfs:subClassOf nell:product .

nell:bacteria rdfs:comment "single-celled or noncellular spherical or spiral or rod-shaped organisms lacking chlorophyll that reproduce by fission;"^^xsd:string ;
    rdfs:subClassOf nell:species .

nell:bakedgood rdfs:comment "A food which is made through baking in an oven"^^xsd:string ;
    rdfs:subClassOf nell:food .

nell:bird rdfs:comment "Birds (class Aves) are winged bipedal endothermic (warm-blooded) egg-laying vertebrate animals."^^xsd:string ;
    rdfs:subClassOf nell:vertebrate .

nell:buildingfeature rdfs:comment "Any physical property or physical attribute that a building might have."^^xsd:string ;
    rdfs:subClassOf nell:item .

nell:buildingmaterial rdfs:comment "The construction material used for building"^^xsd:string ;
    rdfs:subClassOf nell:abstractthing .

nell:cityhascompanyoffice rdfs:comment "specifies that a particular company has offices in a particular city"^^xsd:string ;
    rdfs:domain nell:city ;
    rdfs:range nell:company ;
    rdfs:subPropertyOf nell:locationactedinbyorganization .

nell:comedian rdfs:comment "a person who makes a living by making you laugh"^^xsd:string ;
    rdfs:subClassOf nell:person .

nell:director rdfs:comment "Movie directors."^^xsd:string ;
    rdfs:subClassOf nell:person .

nell:eventhasparticipantagent rdfs:comment "identifies participants in events"^^xsd:string ;
    rdfs:domain nell:event ;
    rdfs:range nell:agent ;
    rdfs:subPropertyOf nell:superpartof .

nell:fish rdfs:comment "A fish is any aquatic vertebrate animal that is covered with scales and equipped with two sets of paired fins and several unpaired fins. Most fish are \"cold-blooded\" or ectothermic allowing their body temperatures to vary as ambient temperatures change."^^xsd:string ;
    rdfs:subClassOf nell:vertebrate .

nell:geometricshape rdfs:comment "geometrical information that remains when location scale and rotational effects are filtered out from an object "^^xsd:string ;
    rdfs:subClassOf nell:abstractthing,
        nell:visualizableattribute .

nell:hasfamilymember a owl:IrreflexiveProperty,
        owl:SymmetricProperty ;
    rdfs:comment "two persons are family members"^^xsd:string ;
    rdfs:domain nell:person ;
    rdfs:range nell:person ;
    rdfs:subPropertyOf nell:agentinteractswithagent .

nell:hasofficeincity rdfs:comment "specifies that a particular company has offices in a particular city"^^xsd:string ;
    rdfs:domain nell:company ;
    rdfs:range nell:city ;
    rdfs:subPropertyOf nell:organizationactsinlocation .

nell:hassibling a owl:IrreflexiveProperty,
        owl:SymmetricProperty ;
    rdfs:comment "two persons are siblings"^^xsd:string ;
    rdfs:domain nell:person ;
    rdfs:range nell:person ;
    rdfs:subPropertyOf nell:hasfamilymember .

nell:hasspouse a owl:IrreflexiveProperty,
        owl:SymmetricProperty ;
    rdfs:comment "person has a spouse"^^xsd:string ;
    rdfs:domain nell:person ;
    rdfs:range nell:person ;
    rdfs:subPropertyOf nell:hasfamilymember .

nell:hobby rdfs:comment "A hobby is an activity undertaken for pleasure in one's spare time. Some hobbies exist primarily as hobbies while others might be practiced professionally by some people but as hobbies by others.  This can include sport activities."^^xsd:string ;
    rdfs:subClassOf nell:abstractthing .

nell:island rdfs:comment "any piece of land surrounded entirely by water"^^xsd:string ;
    rdfs:subClassOf nell:geopoliticallocation .

nell:lake rdfs:comment "A lake is a body of water surrounded entirely by land. For the purposes of this schema any such body regardless of size should be considered a lake. This includes ponds but excludes such bodies as marshes bogs fens etc."^^xsd:string ;
    rdfs:subClassOf nell:geolocatablething,
        nell:location .

nell:magazine rdfs:comment "A magazine is a periodical bound typically published less frequently than daily. This includes electronic magazines. For lack of a better definitional boundary this therefore includes any periodical that is not instead a newspaper."^^xsd:string ;
    rdfs:subClassOf nell:publication .

nell:mlauthor rdfs:comment "A machine learning author is a person who has published research in the field of machine learning."^^xsd:string ;
    rdfs:subClassOf nell:person .

nell:mountain rdfs:comment "A mountain is a landform that extends above the surrounding terrain in a limited area. A mountain is generally steeper than a hill but there is considerable overlap and usage often depends on local custom."^^xsd:string ;
    rdfs:subClassOf nell:geolocatablething,
        nell:location .

nell:musician rdfs:comment "A musician is a person who sings or plays a musical instrument as part of a musical act."^^xsd:string ;
    rdfs:subClassOf nell:person .

nell:newspaper rdfs:comment "A newspaper is a periodical which is printed in a specific format (i.e. on newsprint) describes recent events and is typically published daily."^^xsd:string ;
    rdfs:subClassOf nell:publication .

nell:officebuildingroom rdfs:comment "A room designation such as would be used for rooms in an office building"^^xsd:string ;
    rdfs:subClassOf nell:room .

nell:organizationalsoknownas a owl:IrreflexiveProperty,
        owl:SymmetricProperty ;
    rdfs:comment "this is another name for this organization"^^xsd:string ;
    rdfs:domain nell:organization ;
    rdfs:range nell:organization ;
    rdfs:subPropertyOf nell:synonymfor .

nell:park rdfs:comment "Public local/state/national parks as well as amusement parks and other privately-run attractions."^^xsd:string ;
    rdfs:subClassOf nell:attraction,
        nell:geolocatablething .

nell:protein rdfs:comment "Proteins are any complex organic compounds that consist of one or more chains of amino acids. Proteins are typically essential components of any living cell and indispensable to the proper functioning of all organisms."^^xsd:string ;
    rdfs:subClassOf nell:abstractthing .

nell:restaurant rdfs:comment "The restaurant type represents single restaurants as well as restaurant chains."^^xsd:string ;
    rdfs:subClassOf nell:building .

nell:scientificterm rdfs:comment "a scientific term for prerequisite detection (currently ML and AI focused)"^^xsd:string ;
    rdfs:subClassOf nell:abstractthing .

nell:software rdfs:comment "software that runs on a computer."^^xsd:string ;
    rdfs:subClassOf nell:product .

nell:sportsevent rdfs:comment "is when a sport is played or otherwise engaged in including but not limited to what would be termed a \"sports game\".  See child categories for examples."^^xsd:string ;
    rdfs:subClassOf nell:event .

nell:sportsgameteam rdfs:comment "Specifies the teams that played in a particular sports game"^^xsd:string ;
    rdfs:domain nell:sportsgame ;
    rdfs:range nell:sportsteam ;
    rdfs:subPropertyOf nell:eventhasparticipantagent .

nell:teamingame rdfs:comment "Specifies the teams that played in a particular sports game"^^xsd:string ;
    rdfs:domain nell:sportsteam ;
    rdfs:range nell:sportsgame ;
    rdfs:subPropertyOf nell:agentparticipatedinevent .

nell:televisionstation rdfs:comment "A television station is a broadcaster which transmits television (audio & video)."^^xsd:string ;
    rdfs:subClassOf nell:geolocatablething,
        nell:mediacompany .

nell:trainstation rdfs:comment "railway station (mainly British Commonwealth) or railroad station (mainly US)) is a railway facility where trains regularly stop to load or unload passengers or freight (goods). It generally consists of a platform next to the tracks and a building (depot) providing related services such as ticket sales and waiting rooms."^^xsd:string ;
    rdfs:subClassOf nell:building .

nell:url rdfs:comment "A URL"^^xsd:string ;
    rdfs:subClassOf nell:website .

nell:victim rdfs:comment "a victim of an event could be a person or a group of person like childrens students soldiers drivers etc"^^xsd:string ;
    rdfs:subClassOf nell:abstractthing .

nell:videogame rdfs:comment "A video game is a piece of interactive software used primarily for entertainment including computer games console games arcade games and hand-held games. However this category excludes video game consoles."^^xsd:string ;
    rdfs:subClassOf nell:game,
        nell:software .

nell:visualartist rdfs:comment "A visual artist creates artistic works which are mainly experienced by sight. This category includes painters sculptors and architects but excludes authors."^^xsd:string ;
    rdfs:subClassOf nell:person .

nell:visualizableattribute rdfs:comment "a visual attribute (for NEIL)"^^xsd:string ;
    rdfs:subClassOf nell:visualizablething .

nell:winery rdfs:comment "Companies that produce and sell wines"^^xsd:string ;
    rdfs:subClassOf nell:company .

nell:conference rdfs:comment "A conference is a regular or recurring meeting of people to \"confer\" about a topic. It may take many forms."^^xsd:string ;
    rdfs:subClassOf nell:event .

nell:itemusedwithitem rdfs:comment "Most general item-to-item relation."^^xsd:string ;
    rdfs:domain nell:item ;
    rdfs:range nell:item ;
    rdfs:subPropertyOf nell:relatedto .

nell:locationresidenceofperson rdfs:comment "the location that person has residence in"^^xsd:string ;
    rdfs:domain nell:location ;
    rdfs:range nell:person ;
    rdfs:subPropertyOf nell:locationactedinbyagent .

nell:mediacompany rdfs:comment "Any company that deals in the production or marketing of media goods (film audio literature journalistic etc.)"^^xsd:string ;
    rdfs:subClassOf nell:company .

nell:mutualproxyfor a owl:IrreflexiveProperty,
        owl:SymmetricProperty ;
    rdfs:comment "two things can be taken to refer to each other equally"^^xsd:string ;
    rdfs:domain nell:everypromotedthing ;
    rdfs:range nell:everypromotedthing ;
    rdfs:subPropertyOf nell:relatedto .

nell:personhasresidenceinlocation rdfs:comment "the location that person has residence in"^^xsd:string ;
    rdfs:domain nell:person ;
    rdfs:range nell:location ;
    rdfs:subPropertyOf nell:agentactsinlocation .

nell:room rdfs:comment "A conceptually-distinct subspace within a building. The entire space within a building could be considered to be a room in the case of say a one-room schoolhouse."^^xsd:string ;
    rdfs:subClassOf nell:location .

nell:vehicle rdfs:comment "Any vessel or other conveyance machine used for purposes of travel. Apparel and other personal affects e.g. shoes or walking sticks do not count."^^xsd:string ;
    rdfs:subClassOf nell:product,
        nell:visualizableobject .

nell:visualizablescene rdfs:comment "a visual scene (for NEIL's scene classifiers)"^^xsd:string ;
    rdfs:subClassOf nell:visualizablething .

nell:worker rdfs:comment "to be employed esp. as a means of earning one's livelihood "^^xsd:string ;
    rdfs:domain nell:organization ;
    rdfs:range nell:person ;
    rdfs:subPropertyOf nell:organizationhasperson .

nell:worksfor rdfs:comment "to be employed esp. as a means of earning one's livelihood "^^xsd:string ;
    rdfs:domain nell:person ;
    rdfs:range nell:organization ;
    rdfs:subPropertyOf nell:personbelongstoorganization .

nell:airport rdfs:comment "A place where airplanes helicopters or other flying vehicles land and take off"^^xsd:string ;
    rdfs:subClassOf nell:building .

nell:aquarium rdfs:comment "the aquatic counterpart of a zoo housing living aquatic species for viewing"^^xsd:string ;
    rdfs:subClassOf nell:attraction .

nell:arachnid rdfs:comment "air-breathing arthropods characterized by simple eyes and four pairs of legs"^^xsd:string ;
    rdfs:subClassOf nell:arthropod .

nell:book rdfs:comment "A book is a written work or a collection of written works in book form. \"Book\" represents the abstract notion of a particular book rather than a particular edition."^^xsd:string ;
    rdfs:subClassOf nell:creativework .

nell:celebrity rdfs:comment "A celebrity is a person who is frequently featured in the media and is recognizable by the general public."^^xsd:string ;
    rdfs:subClassOf nell:person .

nell:clothing rdfs:comment "This type is for kinds of garments or clothing. For lack of a meaningful way to constrain this category through definition or existent sibling categories particularly when it comes to adorning the body for purposes of fashion (e.g. jewlery colored contact lenses costumery) or of utility (e.g. armor kneepads or other sports equipment corrective lenses) this will include anything wearable."^^xsd:string ;
    rdfs:subClassOf nell:item .

nell:color rdfs:comment "Color (or colour) is the visual perceptual property corresponding in humans to the categories called red yellow white etc."^^xsd:string ;
    rdfs:subClassOf nell:abstractthing,
        nell:visualizableattribute .

nell:criminal rdfs:comment "a person who commits a crime"^^xsd:string ;
    rdfs:subClassOf nell:person .

nell:economicsector rdfs:comment "An economy may include several sectors (also called industries) "^^xsd:string ;
    rdfs:subClassOf nell:abstractthing .

nell:emotion rdfs:comment "Emotion is the complex psychophysiological experience of an individual's state of mind as interacting with biochemical (internal) and environmental (external) influences "^^xsd:string ;
    rdfs:subClassOf nell:abstractthing .

nell:geopoliticallocationcontainscity rdfs:comment "specifies that a particular city is located in a particular geopolitical location"^^xsd:string ;
    rdfs:domain nell:geopoliticallocation ;
    rdfs:range nell:city ;
    rdfs:subPropertyOf nell:locationcontainslocation .

nell:grain rdfs:comment "dry seed-like fruit produced by the cereal grasses: e.g. wheat barley Indian corn"^^xsd:string ;
    rdfs:subClassOf nell:fruit .

nell:hotel rdfs:comment "This type is intended to be used for hotels bed and breakfasts backpacker hostels or any other such place you might stay while travelling"^^xsd:string ;
    rdfs:subClassOf nell:building .

nell:jobposition rdfs:comment "Positions are job titles or named roles within an organization. Examples include \"CEO\" \"President\" \"mayor\" \"vice president for research\" \"sergeant\" etc. They do not include generic activities or career terms like \"pianist\" \"researcher\" \"scientist\" etc."^^xsd:string ;
    rdfs:subClassOf nell:profession .

nell:musicartist rdfs:comment "An individual or a group that performs or makes music. Musical artists should typically have performed in front of an audience on a regular basis or have recorded musical tracks or musical albums. (FreeBase)"^^xsd:string ;
    rdfs:subClassOf nell:organization .

nell:musicfestival rdfs:comment "A Music Festival is a musical event where live music is played typically by multiple musical artists. A festival may be a singular event or a recurring one."^^xsd:string ;
    rdfs:subClassOf nell:event .

nell:musicgenre rdfs:comment "A style or classification of music (FreeBase)"^^xsd:string ;
    rdfs:subClassOf nell:abstractthing .

nell:politicaloffice rdfs:comment "This type is for the office title or position within a government.  It includes both single-person offices (prime minister emperor mayor) titles of members of a governing body (representative sentator MP) and titles of additional positions within a governing body (leader of the opposition speaker of the house)."^^xsd:string ;
    rdfs:subClassOf nell:abstractthing .

nell:politicsbill rdfs:comment "A legislative bill passed enacted or otherwise."^^xsd:string ;
    rdfs:subClassOf nell:abstractthing .

nell:politicsissue rdfs:comment "An issue of political concern"^^xsd:string ;
    rdfs:subClassOf nell:abstractthing .

nell:proxyfor rdfs:comment "one thing can be taken to refer to another but the reverse is not necessarily or equally so"^^xsd:string ;
    rdfs:domain nell:everypromotedthing ;
    rdfs:range nell:everypromotedthing ;
    rdfs:subPropertyOf nell:mutualproxyfor .

nell:proxyof a owl:IrreflexiveProperty ;
    rdfs:comment "one thing can be taken to refer to another but the reverse is not necessarily or equally so"^^xsd:string ;
    rdfs:domain nell:everypromotedthing ;
    rdfs:range nell:everypromotedthing ;
    rdfs:subPropertyOf nell:mutualproxyfor .

nell:river rdfs:comment "A river is a natural waterway usually formed by water derived from either precipitation or glacial meltwater and flows from higher ground to lower ground. Most commonly rivers flow on the surface but there are many examples of underground rivers. In some areas of highly variable rainfall some rivers carry water only occasionally and may be dry for several years at a time. Such waterways of all sizes including streams and creeks can be listed under this type."^^xsd:string ;
    rdfs:subClassOf nell:geolocatablething,
        nell:location .

nell:species rdfs:comment "is one of the basic units of biological classification and a taxonomic rank. A species is often defined as a group of organisms capable of interbreeding and producing fertile offspring."^^xsd:string ;
    rdfs:subClassOf nell:abstractthing .

nell:sportsteamposition rdfs:comment "The name of a position on a sports team (e.g. quarterback)"^^xsd:string ;
    rdfs:subClassOf nell:abstractthing .

nell:televisionshow rdfs:comment "Television shows or a television series that includes multiple episodes"^^xsd:string ;
    rdfs:subClassOf nell:creativework .

nell:tool rdfs:comment "none"^^xsd:string ;
    rdfs:subClassOf nell:item .

nell:writer rdfs:comment "A writer is a person who produces written work. This category includes book authors poets and playwrights."^^xsd:string ;
    rdfs:subClassOf nell:person .

nell:agentactsinlocation rdfs:comment "As with agentInteractsWithAgent we take existing at a location to be an action at that location."^^xsd:string ;
    rdfs:domain nell:agent ;
    rdfs:range nell:location ;
    rdfs:subPropertyOf nell:agentrelatedtolocation .

nell:agentcreated rdfs:comment "general relation to identify creation and authorships"^^xsd:string ;
    rdfs:domain nell:agent ;
    rdfs:range nell:everypromotedthing ;
    rdfs:subPropertyOf nell:relatedto .

nell:agentinvolvedwithitem rdfs:comment "Most general agent-to-item relation. As with agentInteractsWithAgent we'll use this for states of being as well as actions at least for now."^^xsd:string ;
    rdfs:domain nell:agent ;
    rdfs:range nell:item ;
    rdfs:subPropertyOf nell:relatedto .

nell:agentrelatedtolocation rdfs:comment "Most general agent-to-location relation"^^xsd:string ;
    rdfs:domain nell:agent ;
    rdfs:range nell:location ;
    rdfs:subPropertyOf nell:atlocation .

nell:attractionofcity rdfs:comment "The city that an attraction is located in"^^xsd:string ;
    rdfs:domain nell:attraction ;
    rdfs:range nell:city ;
    rdfs:subPropertyOf nell:locationlocatedwithinlocation .

nell:buildinglocatedincity rdfs:comment "specifies that a particular building is located in a particular city"^^xsd:string ;
    rdfs:domain nell:building ;
    rdfs:range nell:city ;
    rdfs:subPropertyOf nell:locationlocatedwithinlocation .

nell:cityattractions a owl:InverseFunctionalProperty ;
    rdfs:comment "The city that an attraction is located in"^^xsd:string ;
    rdfs:domain nell:city ;
    rdfs:range nell:attraction ;
    rdfs:subPropertyOf nell:locationcontainslocation .

nell:citycontainsbuilding a owl:InverseFunctionalProperty ;
    rdfs:comment "specifies that a particular building is located in a particular city"^^xsd:string ;
    rdfs:domain nell:city ;
    rdfs:range nell:building ;
    rdfs:subPropertyOf nell:locationcontainslocation .

nell:createdbyagent rdfs:comment "general relation to identify creation and authorships"^^xsd:string ;
    rdfs:domain nell:everypromotedthing ;
    rdfs:range nell:agent ;
    rdfs:subPropertyOf nell:relatedto .

nell:geopoliticalorganization rdfs:comment "Those geopolitical entities that are organizations"^^xsd:string ;
    rdfs:subClassOf nell:geopoliticalentity,
        nell:organization .

nell:iteminvolvedwithagent rdfs:comment "Most general agent-to-item relation. As with agentInteractsWithAgent we'll use this for states of being as well as actions at least for now."^^xsd:string ;
    rdfs:domain nell:item ;
    rdfs:range nell:agent ;
    rdfs:subPropertyOf nell:relatedto .

nell:locationactedinbyagent rdfs:comment "As with agentInteractsWithAgent we take existing at a location to be an action at that location."^^xsd:string ;
    rdfs:domain nell:location ;
    rdfs:range nell:agent ;
    rdfs:subPropertyOf nell:locationrelatedtoagent .

nell:locationrelatedtoagent rdfs:comment "Most general agent-to-location relation"^^xsd:string ;
    rdfs:domain nell:location ;
    rdfs:range nell:agent ;
    rdfs:subPropertyOf nell:locatedat .

nell:personbylocation rdfs:comment "Parent category to break up people by regional/national location which exists as a way to constrain some of the political predicates to the U.S.  For simplicity of decision-making we use \"citizenship\" as the rule for belongingness in these categories; this is probably \"good enough\" for what we want to do with the political predicates."^^xsd:string ;
    rdfs:subClassOf nell:person .

nell:synonymfor a owl:IrreflexiveProperty,
        owl:SymmetricProperty ;
    rdfs:comment "Two strings are synonyms if both of them frequently refer to the same real-world concept in text."^^xsd:string ;
    rdfs:domain nell:everypromotedthing ;
    rdfs:range nell:everypromotedthing ;
    rdfs:subPropertyOf nell:mutualproxyfor .

nell:vertebrate rdfs:comment "An animal which has a back bone"^^xsd:string ;
    rdfs:subClassOf nell:animal .

nell:astronaut rdfs:comment "An astronaut is a person that has flown in outer space. Not used for animals sent to space experimentally."^^xsd:string ;
    rdfs:subClassOf nell:person .

nell:bank rdfs:comment "Umbrella category for all kinds of banks"^^xsd:string ;
    rdfs:subClassOf nell:company .

nell:chemical rdfs:comment "A chemical compound is a molecular substance consisting of multiple atoms which are bonded together by a chemical reaction. This type can be used for compounds made of the same element (e.g. allotropes) or multiple different elements. Compounds are different from chemical mixtures because mixtures can be mixed and separated physically without a reaction; The elements of the periodic table"^^xsd:string ;
    rdfs:subClassOf nell:abstractthing .

nell:householditem rdfs:comment "Any item that could reasonably be found in or about a residence."^^xsd:string ;
    rdfs:subClassOf nell:item .

nell:itemexistsatlocation rdfs:comment "An item that is typically found in a particular place. While most any item could concievably exist at most any place the intent for this relation and its children is to capture \"common knowledge\" about what would be expected to be found where."^^xsd:string ;
    rdfs:domain nell:item ;
    rdfs:range nell:location ;
    rdfs:subPropertyOf nell:atlocation .

nell:locationofitemexistence rdfs:comment "An item that is typically found in a particular place. While most any item could concievably exist at most any place the intent for this relation and its children is to capture \"common knowledge\" about what would be expected to be found where."^^xsd:string ;
    rdfs:domain nell:location ;
    rdfs:range nell:item ;
    rdfs:subPropertyOf nell:locatedat .

nell:organizationhasperson rdfs:comment "organization or company that person is belonged to"^^xsd:string ;
    rdfs:domain nell:organization ;
    rdfs:range nell:person ;
    rdfs:subPropertyOf nell:organizationhasagent .

nell:personbelongstoorganization rdfs:comment "organization or company that person is belonged to"^^xsd:string ;
    rdfs:domain nell:person ;
    rdfs:range nell:organization ;
    rdfs:subPropertyOf nell:agentbelongstoorganization .

nell:politicsgroup rdfs:comment "Organizations which may or may not be part of the government that act in the arenas of politics or government."^^xsd:string ;
    rdfs:subClassOf nell:geopoliticalorganization .

nell:religion rdfs:comment "Religious sects denominations and (meta-)organizations. NOT church buildings or individual chapters/institutions."^^xsd:string ;
    rdfs:subClassOf nell:abstractthing .

nell:sportsleague rdfs:comment "A sports league is an association of teams that compete with each other in a sport. Sports leagues include conferences and divisions of other sports leagues."^^xsd:string ;
    rdfs:subClassOf nell:organization .

nell:time rdfs:comment "a specific time"^^xsd:string ;
    rdfs:subClassOf nell:abstractthing .

nell:weapon rdfs:comment "A weapon is any tool used for fighting"^^xsd:string ;
    rdfs:subClassOf nell:item,
        nell:visualizableobject .

nell:website rdfs:comment "A Website or (Web site) is a collection of web pages typically common to a particular domain name or subdomain on the World Wide Web on the Internet. A web page is a document typically written in HTML that is almost always accessible via HTTP a protocol that transfers information from the website's server to display in the user's Web browser."^^xsd:string ;
    rdfs:subClassOf nell:location .

nell:agentcollaborateswithagent a owl:IrreflexiveProperty,
        owl:SymmetricProperty ;
    rdfs:comment "to work one with another; cooperate as on a literary work "^^xsd:string ;
    rdfs:domain nell:agent ;
    rdfs:range nell:agent ;
    rdfs:subPropertyOf nell:agentinteractswithagent .

nell:atdate rdfs:comment "assigns dates to things."^^xsd:string ;
    rdfs:domain nell:everypromotedthing ;
    rdfs:range nell:date ;
    rdfs:subPropertyOf nell:relatedto .

nell:dateof rdfs:comment "assigns dates to things."^^xsd:string ;
    rdfs:domain nell:date ;
    rdfs:range nell:everypromotedthing ;
    rdfs:subPropertyOf nell:relatedto .

nell:publication rdfs:subClassOf nell:mediacompany .

nell:subpartof a owl:AsymmetricProperty,
        owl:IrreflexiveProperty ;
    rdfs:comment "a portion or division of a whole that is separate or distinct; piece fragment fraction or section; constituent "^^xsd:string ;
    rdfs:domain nell:everypromotedthing ;
    rdfs:range nell:everypromotedthing ;
    rdfs:subPropertyOf nell:relatedto .

nell:superpartof rdfs:comment "a portion or division of a whole that is separate or distinct; piece fragment fraction or section; constituent "^^xsd:string ;
    rdfs:domain nell:everypromotedthing ;
    rdfs:range nell:everypromotedthing ;
    rdfs:subPropertyOf nell:relatedto .

nell:actor rdfs:comment "An actor is a person who performs in movies television plays or other forms of entertainment."^^xsd:string ;
    rdfs:subClassOf nell:person .

nell:automobilemaker rdfs:comment "A company that manufactures motor-powered vehicles (eg. cars motorcycles buses trucks and motorized bikes)"^^xsd:string ;
    rdfs:subClassOf nell:company .

nell:awardtrophytournament rdfs:comment "Sports award is a CVT which connects together the winner of a sports award the award they won the season for which they won the award and the team they represented (if applicable)."^^xsd:string ;
    rdfs:subClassOf nell:abstractthing .

nell:ceo rdfs:comment "A CEO is the chief executive officer of a company."^^xsd:string ;
    rdfs:subClassOf nell:person .

nell:creativework rdfs:comment "the product of any creative effort including movies paintings musical songs etc."^^xsd:string ;
    rdfs:subClassOf nell:abstractthing .

nell:dateliteral rdfs:comment "represents a date."^^xsd:string ;
    rdfs:subClassOf nell:date .

nell:drug rdfs:comment "A drug is a chemical substance that has or is reputed to have a phyisological effect on an organism. Medicinal herbal and illegal drugs can be included in this type."^^xsd:string ;
    rdfs:subClassOf nell:product .

nell:farm rdfs:comment "an area of land including various structures devoted primarily to the practice of producing and managing food (produce grains or livestock) fibres and increasingly fuel."^^xsd:string ;
    rdfs:subClassOf nell:location .

nell:female rdfs:comment "This category includes all female human beings."^^xsd:string ;
    rdfs:subClassOf nell:person .

nell:invertebrate rdfs:comment "An animal which does not have a back bone"^^xsd:string ;
    rdfs:subClassOf nell:animal .

nell:locationactedinbyorganization rdfs:comment "location of an organization or company"^^xsd:string ;
    rdfs:domain nell:location ;
    rdfs:range nell:organization ;
    rdfs:subPropertyOf nell:locationactedinbyagent .

nell:meetingeventtitle rdfs:comment "The title of a meeting (such as a presentation)"^^xsd:string ;
    rdfs:subClassOf nell:event .

nell:movie rdfs:comment "A release of a visual narrative composed of a series of moving images that is considered a complete presentation and is intended to be classified as a film. A film can be of any length of running time and presented in a theatrical television internet-streaming and direct-to-home-video presentation. (FreeBase)"^^xsd:string ;
    rdfs:subClassOf nell:creativework .

nell:organizationactsinlocation rdfs:comment "location of an organization or company"^^xsd:string ;
    rdfs:domain nell:organization ;
    rdfs:range nell:location ;
    rdfs:subPropertyOf nell:agentactsinlocation .

nell:school rdfs:comment "A school is an organization whose primary function is education. This category includes universities K-12 schools and trade schools."^^xsd:string ;
    rdfs:subClassOf nell:organization .

nell:vegetable rdfs:comment "An edible plant or part of a plant other than a sweet fruit or seed. This usually means the leaf stem or root of a plant.  This is meant to dovetail with the more botanical definition we have of fruit and to not allow cullinary / colloquial vegetables that qualify for membership in our fruit category.  Mushrooms are not vegetables."^^xsd:string ;
    rdfs:subClassOf nell:food .

nell:visualizablething rdfs:comment "something which can be recognized visually"^^xsd:string ;
    rdfs:subClassOf nell:everypromotedthing .

nell:artery rdfs:comment "Arteries are muscular blood vessels that carry blood away from the heart."^^xsd:string ;
    rdfs:subClassOf nell:bodypart .

nell:beverage rdfs:comment "A liquid meant for human consumption"^^xsd:string ;
    rdfs:subClassOf nell:food .

nell:humanagent rdfs:comment "Those things to which we can ascribe agency that are composed of one or more humans"^^xsd:string ;
    rdfs:subClassOf nell:agent .

nell:male rdfs:comment "This category includes all male human beings."^^xsd:string ;
    rdfs:subClassOf nell:person .

nell:mammal rdfs:comment "Mammals (formally Mammalia) are a class of vertebrate air-breathing animals whose females are characterized by the possession of mammary glands while both males and females are characterized by hair and/or fur three middle ear bones used in hearing and a neocortex region in the brain."^^xsd:string ;
    rdfs:subClassOf nell:vertebrate .

nell:physiologicalcondition rdfs:comment "Most instances will be diseases or other abnormalities. However this category also includes conditions such as pregnancy or teething that are entirely normal and expected but which are nevertheless exception and can require extra care."^^xsd:string ;
    rdfs:subClassOf nell:abstractthing .

nell:politicianus rdfs:comment "Politicians of the U.S.A"^^xsd:string ;
    rdfs:subClassOf nell:personus,
        nell:politician .

nell:visualizableobject rdfs:comment "a visual object (for NEIL)"^^xsd:string ;
    rdfs:subClassOf nell:visualizablething .

nell:atlocation rdfs:comment "assigns locations to things."^^xsd:string ;
    rdfs:domain nell:everypromotedthing ;
    rdfs:range nell:location ;
    rdfs:subPropertyOf nell:relatedto .

nell:locatedat rdfs:comment "assigns locations to things."^^xsd:string ;
    rdfs:domain nell:location ;
    rdfs:range nell:everypromotedthing ;
    rdfs:subPropertyOf nell:relatedto .

nell:profession rdfs:comment "The career or job which a person performs for most of their working life or for which they are best known (FreeBase)"^^xsd:string ;
    rdfs:subClassOf nell:abstractthing .

nell:disease rdfs:comment "A disease is an abnormal condition of the human body that causes discomfort or impairs bodily functions. This type also includes medical conditions such as injuries disabilities disorders syndromes etc. that affect the normal functioning of a person whether physically or mentally."^^xsd:string ;
    rdfs:subClassOf nell:physiologicalcondition .

nell:language rdfs:comment "Spoken human languages (and dialects)."^^xsd:string ;
    rdfs:subClassOf nell:abstractthing .

nell:locationcontainslocation a owl:AsymmetricProperty,
        owl:IrreflexiveProperty ;
    rdfs:comment "a location that is a subpart of another location"^^xsd:string ;
    rdfs:domain nell:location ;
    rdfs:range nell:location ;
    rdfs:subPropertyOf nell:locatedat,
        nell:superpartof .

nell:locationlocatedwithinlocation rdfs:comment "a location that is a subpart of another location"^^xsd:string ;
    rdfs:domain nell:location ;
    rdfs:range nell:location ;
    rdfs:subPropertyOf nell:atlocation,
        nell:subpartof .

nell:plant rdfs:comment "Member of kingdom plantae. A seed is considered to be a plant because it has been fertilized although the larger structure of a fruit which merely contains a seed is not itself a plant.  A picked flower such as a product sold as such is not a plant because it is something that has a new name as a result of a mortal action on a plant."^^xsd:string ;
    rdfs:subClassOf nell:item,
        nell:species .

nell:university rdfs:comment "A university is a post-high school educational institution. This category includes colleges and technical schools."^^xsd:string ;
    rdfs:subClassOf nell:geolocatablething,
        nell:school .

nell:bodypart rdfs:comment "Refers to any part of the human body. It can be either visible to the naked eye (gross anatomical structure) or microscopic."^^xsd:string ;
    rdfs:subClassOf nell:item .

nell:canbethesameas rdfs:comment "Describes two instances that are the same thing in different categories"^^xsd:string ;
    rdfs:domain nell:everypromotedthing ;
    rdfs:range nell:everypromotedthing ;
    rdfs:subPropertyOf nell:relatedto .

nell:coach rdfs:comment "A coach is a trainer for a sports team. He leads the team in exercises and manages the team during gameplay. This category includes assistant coaches and other trainers."^^xsd:string ;
    rdfs:subClassOf nell:person .

nell:geopoliticallocation rdfs:comment "Those geopolitical entities that are location"^^xsd:string ;
    rdfs:subClassOf nell:geopoliticalentity,
        nell:location .

nell:productlaunchevent rdfs:subClassOf nell:event .

nell:stadiumoreventvenue rdfs:comment "A building where large spectator events (usually sporting events) take place."^^xsd:string ;
    rdfs:subClassOf nell:attraction,
        nell:building .

nell:politician rdfs:comment "Any person who has held or sought a position in a government. The term \"politician\" may not be strictly accurate for some positions such as kings but we have to call it something!"^^xsd:string ;
    rdfs:subClassOf nell:person .

nell:academicfield rdfs:comment "A field of study is the field area or discipline which is the focus of study of a student or academic or which is taught in a school."^^xsd:string ;
    rdfs:subClassOf nell:abstractthing .

nell:date rdfs:comment "a particular month day and year at which some event happened or will happen; the time or period to which any event or thing belongs; period in general "^^xsd:string ;
    rdfs:subClassOf nell:abstractthing .

nell:insect rdfs:comment "class within the arthropods that have a chitinous exoskeleton a three-part body (head thorax and abdomen) three pairs of jointed legs compound eyes and two antennae"^^xsd:string ;
    rdfs:subClassOf nell:arthropod .

nell:protestevent rdfs:subClassOf nell:event .

nell:attraction rdfs:comment "sight or feature that you might visit as a tourist. Examples include monuments parks museums and the like. This type includes Location which means it is usually used for things which are themselves locations (like those described above"^^xsd:string ;
    rdfs:subClassOf nell:location .

nell:product rdfs:comment "none"^^xsd:string ;
    rdfs:subClassOf nell:item .

nell:food rdfs:comment "A food is any edible substance with nutritional value whether it's a basic foodstuff like rice or apples or a commercial product like Poptarts or I Can't Believe It's Not Butter.  \"Nutritional value\" encompasses anything useful for growth or life such as water so long as the organism gets it through ingestion."^^xsd:string ;
    rdfs:subClassOf nell:item,
        nell:visualizableobject .

nell:roadaccidentevent rdfs:subClassOf nell:event .

nell:sport rdfs:comment "A game which involves some form of physical prowess (i.e. athleticism as opposed to the physical prowess needed for a parlour game like Pin the Tail on the Donkey).  Note that this does not include non-game sports; those may be hobbies instead."^^xsd:string ;
    rdfs:subClassOf nell:abstractthing .

nell:sportsgame rdfs:comment "A sports game is a particular instance of a sporting event where teams or athletes compete. This could be a series of matches if the competitors remain the same but this does not extend to something like a tournament or season where the series of matches draws on different combinations from a set of teams."^^xsd:string ;
    rdfs:subClassOf nell:game,
        nell:sportsevent .

nell:arthropod rdfs:comment "Arthropods are members of the phylum Arthropoda."^^xsd:string ;
    rdfs:subClassOf nell:invertebrate .

nell:earthquakeevent rdfs:subClassOf nell:event .

nell:geolocatablething rdfs:subClassOf nell:everypromotedthing .

nell:building rdfs:comment "A building is a man-made structure designed for shelter or for continuous or periodic occupancy. All buildings are structures and therefore typed \"Structure\" which imparts other basic properties (see /architecture/structure). If something is not a structure it can't be typed as a building.  This category does not include complexes of individual buildings."^^xsd:string ;
    rdfs:subClassOf nell:geolocatablething,
        nell:location .

nell:agriculturalproduct rdfs:comment "a living thing (or something derived therefrom) which is specifically cultivated and produced to sustain or enrich life"^^xsd:string ;
    rdfs:subClassOf nell:item .

nell:nonneginteger rdfs:subClassOf nell:abstractthing .

nell:bombingevent rdfs:subClassOf nell:event .

nell:animal rdfs:comment "A collection of common-sense animals more understandable to children than biologists.  It's OK to include both general kinds of animals such as bird but also common varieties of birds such as finch and robin. (FreeBase)  As with plant any mortal action upon an animal or action on a dead animal that results in something with a new name (e.g. milking shearing slaughtering or cooking it) results in something that is no longer an animal."^^xsd:string ;
    rdfs:subClassOf nell:agent,
        nell:species .

nell:sportsteam rdfs:comment "A sports team is a group of athletes who play a sport together competitively"^^xsd:string ;
    rdfs:subClassOf nell:geolocatablething,
        nell:organization .

nell:item rdfs:comment "Any tangible thing that does not have the power to act (agency)"^^xsd:string ;
    rdfs:subClassOf nell:everypromotedthing .

nell:agent rdfs:comment "a person or business authorized to act on another's behalf; a person or thing that acts or has the power to act; a natural force or object producing or used for obtaining specific results "^^xsd:string ;
    rdfs:subClassOf nell:everypromotedthing .

nell:stateorprovince rdfs:comment "In general the top-level administrative or political subdivision within a country."^^xsd:string ;
    rdfs:subClassOf nell:geolocatablething,
        nell:geopoliticallocation,
        nell:geopoliticalorganization .

nell:event rdfs:comment "An event is a topic that can be described by the time or date at which it happened. Long-lasting events may be described as occurring between two dates. It is sometimes appropriate to create abstract events as collections of other events"^^xsd:string ;
    rdfs:subClassOf nell:abstractthing .

nell:generalizationof a owl:AsymmetricProperty,
        owl:IrreflexiveProperty ;
    rdfs:comment "one thing is a more specific kind of another thing"^^xsd:string ;
    rdfs:domain nell:everypromotedthing ;
    rdfs:range nell:everypromotedthing ;
    rdfs:subPropertyOf nell:relatedto .

nell:specializationof rdfs:comment "one thing is a more specific kind of another thing"^^xsd:string ;
    rdfs:domain nell:everypromotedthing ;
    rdfs:range nell:everypromotedthing ;
    rdfs:subPropertyOf nell:relatedto .

nell:athlete rdfs:comment "An athlete is a person who plays a sport competitively."^^xsd:string ;
    rdfs:subClassOf nell:person .

nell:company rdfs:comment "A company is an organization whose goal is to make money"^^xsd:string ;
    rdfs:subClassOf nell:organization .

nell:abstractthing rdfs:comment "thought quality characteristic apart from concrete realities specific objects or actual instances; theoretical not applied or practical "^^xsd:string ;
    rdfs:subClassOf nell:everypromotedthing .

nell:organization rdfs:comment "An organization is an organized body of members or people with a particular purpose; in the Freebase context a organization doesn't have a business association like a company.  Companies have their own type in the business domain located here.  In addition many types of organizations have their own more specialized co-types that give them additional properties."^^xsd:string ;
    rdfs:subClassOf nell:humanagent .

nell:country rdfs:comment "The type \"country\" in Freebase can and should be used with a variety of topics. The most common will be probably be current and former independent nations potentially including composite entities such as empires. It can also be used for autonomous entities within such a composite such as the four current constituent countries (England Northern Ireland Scotland and Wales) of the United Kingdom.  Anything having an ISO country code qualifies as a country including contested countries like Taiwan and including territories of minor or no population."^^xsd:string ;
    rdfs:subClassOf nell:geolocatablething,
        nell:geopoliticallocation,
        nell:geopoliticalorganization .

nell:location rdfs:comment "The Location type is used for any topic with a fixed location on the planet Earth. It includes geographic features such as oceans and mountains political entities like cities and man-made objects like buildings"^^xsd:string ;
    rdfs:subClassOf nell:everypromotedthing .

nell:everypromotedthing rdfs:comment "every promoted category instance in KB"^^xsd:string .

nell:city rdfs:comment "City/town/village refers to all named inhabited places at the most locally recognized level but above the level of neighborhood. It is the most local region where there is a form of government or self-organization.   Cities/towns/villages are larger than neighborhoods and are typically contained within a larger administrative division such as a county department province etc. It should be noted however that large or significant cities may themselves also function as higher-level administrative divisions.   For more information please see the Freebase wiki page on City/Town/Village."^^xsd:string ;
    rdfs:subClassOf nell:geolocatablething,
        nell:geopoliticallocation,
        nell:geopoliticalorganization,
        nell:visualizablescene .

nell:person rdfs:comment "A person is a human being (man woman or child) known to have actually existed. Living persons celebrities and politicians are persons as are deceased persons."^^xsd:string ;
    rdfs:subClassOf nell:humanagent .

nell:relatedto rdfs:comment "associated; connected "^^xsd:string ;
    rdfs:domain nell:everypromotedthing ;
    rdfs:range nell:everypromotedthing .

